@prefix schema: <http://schema.org/> .
@prefix prod:  <https://w3id.org/product#> .
@prefix owl:   <http://www.w3.org/2002/07/owl#> .
@prefix bot:   <https://w3id.org/bot#> .
@prefix xsd:   <http://www.w3.org/2001/XMLSchema#> .
@prefix sgfn:  <http://w3id.org/sparql-generate/fn/> .
@prefix voaf:  <http://purl.org/vocommons/voaf#> .
@prefix rdfs:  <http://www.w3.org/2000/01/rdf-schema#> .
@prefix props: <https://w3id.org/product/props/> .
@prefix ex:    <http://example.org/> .
@prefix rdf:   <http://www.w3.org/1999/02/22-rdf-syntax-ns#> .
@prefix sgiter: <http://w3id.org/sparql-generate/iter/> .
@prefix dcterms: <http://purl.org/dc/terms/> .
@prefix vann:  <http://purl.org/vocab/vann/> .
@prefix vs:    <http://www.w3.org/2003/06/sw-vocab-status/ns#> .
@prefix foaf:  <http://xmlns.com/foaf/0.1/> .

props:bladeAction  rdfs:comment  "Blade action."@en ;
        rdfs:label             "bladeAction"@en ;
        schema:domainIncludes  <https://w3id.org/product/Damper> .

props:coreSetHorizontal
        a                      owl:DatatypeProperty ;
        rdfs:comment           "Degree of horizontal (in the X-axis of the LocalPlacement) blade set from the centerline."@en , "水平翼の中心線からの水平（ローカル座標のＸ軸）面の羽根角度"@ja-JP , "Degré d'inclinaison horizontale (selon l'axe X par rapport au positionnement local) de la lame mesuré depuis la ligne médiane."@fr-FR ;
        rdfs:label             "coreSetHorizontal"@en , "水平羽根角度"@ja-JP , "PositionHorizontaleCentre"@fr-FR ;
        rdfs:range             <https://w3id.org/measurement/planeAngle> ;
        schema:domainIncludes  <https://w3id.org/product/AirTerminal> .

props:speakerDriverSize
        rdfs:comment           "Indicates the number of drivers and their sizes."@en , "ドライバユニットと数を示す。"@ja-JP , "드라이버 유닛과 수를 나타낸다"@ko-KR ;
        rdfs:label             "speakerDriverSize"@en , "スピーカードライバサイズ"@ja-JP , "스피커 드라이버"@ko-KR ;
        schema:domainIncludes  <https://w3id.org/product/AudioVisualAppliance#SPEAKER> .

props:halogenProof  a          owl:DatatypeProperty ;
        rdfs:comment           "煙や刺激臭のあるガスの発生が少ないケーブル。"@ja-JP , "Produces small amount of smoke and irritating Deaerator/Gas."@en , "연기와 자극적인 냄새가있는 가스의 발생이 적은 케이블"@ko-KR , "Produces small amount of smoke and irritating deaerator/gas."@en , "少量の煙および刺激する脱気/ガスを生成。"@ja-JP , "소량의 연기와 자극 탈기 / 가스를 생성합니다."@ko-KR ;
        rdfs:label             "에코 케이블"@ko-KR , "ハロゲン証明"@ja-JP , "할로겐 증명"@ko-KR , "エコケーブル"@ja-JP , "halogenProof"@en ;
        rdfs:range             xsd:boolean ;
        schema:domainIncludes  <https://w3id.org/product/CableSegment#CORESEGMENT> , <https://w3id.org/product/CableSegment#CABLESEGMENT> .

props:energyLoss  a            owl:DatatypeProperty ;
        rdfs:comment           "The sum of energy losses for the spaces served by the system during the peak heating conditions."@en , "ピーク時空調システム最大暖房負荷を提供する際の熱ロス。"@ja-JP , "최대 공조 시스템 최대 난방 부하를 제공할 수있는 열 손실"@ko-KR ;
        rdfs:label             "energyLoss"@en , "熱（エネルギー）ロス"@ja-JP , "열(에너지)로스"@ko-KR ;
        rdfs:range             <https://w3id.org/measurement/power> ;
        schema:domainIncludes  bot:Zone .

props:totalCoolingCapacity
        a                      owl:DatatypeProperty ;
        rdfs:comment           "Total cooling capacity. This includes cooling capacity of beam and cooling capacity of supply air."@en ;
        rdfs:label             "totalCoolingCapacity"@en ;
        rdfs:range             <https://w3id.org/product/TimeSeries> ;
        rdfs:range             [ owl:allValuesFrom  <https://w3id.org/measurement/power> ;
                                 owl:onProperty     <https://w3id.org/measurement/seriesOf>
                               ] ;
        schema:domainIncludes  <https://w3id.org/product/CooledBeam> .

props:videoScaleMode  rdfs:comment  "비디오 크기 조정모드를 나타낸다."@ko-KR , "Indicates video scaling modes."@en , "ビデオスケーリングモードを示す。"@ja-JP , "비디오 크기 조정 모드를 나타낸다."@ko-KR ;
        rdfs:label             "비디오 스케일 모드"@ko-KR , "videoScaleMode"@en , "비디오 스케일"@ko-KR , "ビデオスケールモード"@ja-JP ;
        schema:domainIncludes  <https://w3id.org/product/AudioVisualAppliance#PROJECTOR> , <https://w3id.org/product/AudioVisualAppliance#DISPLAY> .

props:flammabilityRating
        a                      owl:DatatypeProperty ;
        rdfs:comment           "Classement de l'inflammabilité de l'élément selon la classification nationale de sécurité incendie."@fr-FR , "Angabe zur Entflammbarkeit des Materials gemäß der nationalen oder regionalen Normen."@de-DE , "Flammability Rating for this object.\nIt is given according to the national building code that governs the rating of flammability for materials."@en , "可燃性等級。当該国の建築法規による。"@ja-JP ;
        rdfs:label             "Inflammabilité"@fr-FR , "Entflammbarkeitsklasse"@de-DE , "flammabilityRating"@en , "可燃性等級"@ja-JP ;
        rdfs:range             xsd:string ;
        schema:domainIncludes  <https://w3id.org/product/Covering> .

props:minimumPartLoadRatio
        a                      owl:DatatypeProperty ;
        rdfs:comment           "Minimum part load ratio as a fraction of nominal capacity."@en , "Coefficient minimum de charge partielle en tant que fraction de la puissance nominale."@fr-FR ;
        rdfs:label             "minimumPartLoadRatio"@en , "CoefficientMinimalChargePartielle"@fr-FR ;
        rdfs:range             <https://w3id.org/measurement/positiveRatio> ;
        schema:domainIncludes  <https://w3id.org/product/Compressor> .

props:operatingMode  rdfs:comment  "Identifies the operating mode of the boiler."@en , "ボイラの動作モードのID　（固定、２段階、比例．．．）"@ja-JP , "Identifie le mode de fonctionnement de la chaudière."@fr-FR ;
        rdfs:label             "operatingMode"@en , "動作モード"@ja-JP , "ModeFonctionnement"@fr-FR ;
        schema:domainIncludes  <https://w3id.org/product/Boiler> .

props:partLoadRatio  a         owl:DatatypeProperty ;
        rdfs:comment           "Ratio of the real to the nominal capacity."@en , "Ratio entre capacité effective et capacité nominale"@fr-FR , "設計容量との比"@ja-JP ;
        rdfs:label             "partLoadRatio"@en , "部分負荷比"@ja-JP , "Taux de charge"@fr-FR ;
        rdfs:range             <https://w3id.org/product/TimeSeries> ;
        rdfs:range             [ owl:allValuesFrom  <https://w3id.org/measurement/normalisedRatio> ;
                                 owl:onProperty     <https://w3id.org/measurement/seriesOf>
                               ] ;
        schema:domainIncludes  <https://w3id.org/product/Boiler> .

props:numberOfCores  a         owl:DatatypeProperty ;
        rdfs:comment           "The number of cores in Cable/Bus."@en , "ケーブルや母線の芯数を示す。"@ja-JP , "케이블과 모선의 심수 보여준다."@ko-KR ;
        rdfs:label             "numberOfCores"@en , "芯数"@ja-JP , "심수"@ko-KR ;
        rdfs:range             xsd:int ;
        schema:domainIncludes  <https://w3id.org/product/CableSegment#CABLESEGMENT> .

props:operationalEfficiency
        a                      owl:DatatypeProperty ;
        rdfs:comment           "運転効率：\n全入力エネルギ（電力または燃料）でボイラ出力を割る"@ja-JP , "Operational efficiency: boiler output divided by total energy input (electrical and fuel)."@en , "Efficacité opérationnelle: production de la chaudière divisée par l'apport total d'énergie (électrique et combustible)."@fr-FR ;
        rdfs:label             "operationalEfficiency"@en , "EfficacitéOpérationnelle"@fr-FR , "運転効率"@ja-JP ;
        rdfs:range             <https://w3id.org/product/TimeSeries> ;
        rdfs:range             [ owl:allValuesFrom  <https://w3id.org/measurement/normalisedRatio> ;
                                 owl:onProperty     <https://w3id.org/measurement/seriesOf>
                               ] ;
        schema:domainIncludes  <https://w3id.org/product/Boiler> .

props:acquisitionMethod
        rdfs:comment           "The means by which survey data was acquired."@en , "La méthode utilisée pour effectuer le relevé."@fr-FR ;
        rdfs:label             "acquisitionMethod"@en , "MethodeAcquisition"@fr-FR ;
        schema:domainIncludes  <https://w3id.org/product/Annotation#SurveyArea> .

props:supplyAirTemperatureCooling
        a                      owl:DatatypeProperty ;
        rdfs:comment           "冷房時の給気温度"@ja-JP , "Supply air temperature in cooling mode."@en , "Température de l'air soufflé en mode refroidissement"@fr-FR ;
        rdfs:label             "Température de l'air soufflé en refroidissement"@fr-FR , "supplyAirTemperatureCooling"@en , "冷房給気温度"@ja-JP ;
        rdfs:range             <https://w3id.org/product/TimeSeries> ;
        rdfs:range             [ owl:allValuesFrom  <https://w3id.org/measurement/thermodynamicTemperature> ;
                                 owl:onProperty     <https://w3id.org/measurement/seriesOf>
                               ] ;
        schema:domainIncludes  <https://w3id.org/product/AirTerminal> .

props:setbackDistance
        a                      owl:DatatypeProperty ;
        rdfs:comment           "Setback distance from the point of connection on the major element along the axis of the minor element (e.g. distance from a public road at which the line of sigfht is measured."@en , "Distance de recul le long de l'axe de l'élément secondaire depuis le point de jonction sur l'élément principal (par exemple, distance depuis la route principale à partir de laquelle la visibilité est appréciée)."@fr-FR , "副要素の軸に沿った主要素の接続点からの後退距離（例えば、可視線が測定される公道からの距離）。"@ja-JP ;
        rdfs:label             "setbackDistance"@en , "DistanceRecul"@fr-FR , "後退距離"@ja-JP ;
        rdfs:range             <https://w3id.org/measurement/positiveLength> ;
        schema:domainIncludes  <https://w3id.org/product/Annotation#LineOfSight> .

props:sealMaterial  a          owl:ObjectProperty ;
        rdfs:comment           "The material from which the damper seals are constructed."@en ;
        rdfs:label             "sealMaterial"@en ;
        rdfs:range             <https://w3id.org/product/MaterialDefinition> ;
        schema:domainIncludes  <https://w3id.org/product/Damper> .

props:connectionSize  a        owl:DatatypeProperty ;
        rdfs:comment           "Duct connection diameter."@en ;
        rdfs:label             "connectionSize"@en ;
        rdfs:range             <https://w3id.org/measurement/length> ;
        schema:domainIncludes  <https://w3id.org/product/CooledBeam#ACTIVE> .

props:compressorTotalHeatGain
        a                      owl:DatatypeProperty ;
        rdfs:comment           "Compressor total heat gain."@en , "Gain thermique total au niveau du compresseur."@fr-FR ;
        rdfs:label             "compressorTotalHeatGain"@en , "GainThermiqueTotalCompresseur"@fr-FR ;
        rdfs:range             <https://w3id.org/product/TimeSeries> ;
        rdfs:range             [ owl:allValuesFrom  <https://w3id.org/measurement/power> ;
                                 owl:onProperty     <https://w3id.org/measurement/seriesOf>
                               ] ;
        schema:domainIncludes  <https://w3id.org/product/Compressor> .

props:ratedTemperature
        rdfs:comment           "使用できることが許可されている許容温度。"@ja-JP , "장치를 사용할 보장된 온도 상한은 최대."@ko-KR , "사용할 수있는 권한이있는 허용 온도"@ko-KR , "The range of allowed temerature that a device is certified to handle. The upper bound of this value is the maximum."@en , "機器を使用できる保障された温度。上限値は最大値。"@ja-JP ;
        rdfs:label             "定格温度"@ja-JP , "정격 온도"@ko-KR , "ratedTemperature"@en ;
        schema:domainIncludes  <https://w3id.org/product/CableSegment#CABLESEGMENT> , <https://w3id.org/product/CableSegment#CORESEGMENT> .

props:nominalUA  a             owl:DatatypeProperty ;
        rdfs:comment           "Nominal UA value."@en , "Valeur nominale du coefficient de transmission thermique totale."@fr-FR ;
        rdfs:label             "nominalUA"@en , "UANominale"@fr-FR ;
        rdfs:range             xsd:decimal ;
        schema:domainIncludes  <https://w3id.org/product/Coil> .

props:finishType  rdfs:comment  "The type of finish for the air terminal."@en , "ターミナルの仕上げの形式（ANNODIZED,塗装他）"@ja-JP , "Le type de finition du terminal de ventilation."@fr-FR ;
        rdfs:label             "finishType"@en , "仕上げ形式"@ja-JP , "TypeFinition"@fr-FR ;
        schema:domainIncludes  <https://w3id.org/product/AirTerminal> .

props:assetInsuranceType
        rdfs:comment           "Identifies the predefined types of insurance rating from which the type required may be set."@en , "保険の定義済み種別。"@ja-JP ;
        rdfs:label             "assetInsuranceType"@en , "資産保険種別"@ja-JP ;
        schema:domainIncludes  <https://w3id.org/product/Asset> .

props:assessmentDate  a        owl:DatatypeProperty ;
        rdfs:comment           "Date on which the overall condition is assessed"@en , "全体状況を評価した日。"@ja-JP ;
        rdfs:label             "assessmentDate"@en , "評価日"@ja-JP ;
        rdfs:range             xsd:date ;
        schema:domainIncludes  <https://w3id.org/product/Element> .

props:internalSurfaceArea
        a                      owl:DatatypeProperty ;
        rdfs:comment           "Internal surface area."@en ;
        rdfs:label             "internalSurfaceArea"@en ;
        rdfs:range             <https://w3id.org/measurement/area> ;
        schema:domainIncludes  <https://w3id.org/product/Condenser> .

props:currentCarryingCapasity
        a                      owl:DatatypeProperty ;
        rdfs:comment           "Maximum value of electric current which can be carried continuously by a conductor, a device or an apparatus, under specified conditions without its steady-state temperature exceeding a  specified value. Based on IEC60826-11-13. NOTE: The temperature specified value is maximum Design Ambient Temperature."@en ;
        rdfs:label             "currentCarryingCapasity"@en ;
        rdfs:range             <https://w3id.org/measurement/electricCurrent> ;
        schema:domainIncludes  <https://w3id.org/product/CableSegment> .

props:designAmbientTemperature
        rdfs:comment           "The highest and lowest local ambient temperature likely to be encountered."@en ;
        rdfs:label             "designAmbientTemperature"@en ;
        schema:domainIncludes  <https://w3id.org/product/CableSegment> .

props:basinReserveVolume
        a                      owl:DatatypeProperty ;
        rdfs:comment           "Volume between operating and overflow levels in cooling tower basin."@en ;
        rdfs:label             "basinReserveVolume"@en ;
        rdfs:range             <https://w3id.org/measurement/volume> ;
        schema:domainIncludes  <https://w3id.org/product/CoolingTower> .

props:totalUACurves  rdfs:comment  "Total UA curves, UA - air and water velocities, UA = [(C1 * AirFlowRate^0.8)^-1 + (C2 * WaterFlowRate^0.8)^-1]^-1.  Note: as two variables are used, DefiningValues and DefinedValues are null, and values are stored in IfcTable in the following order: AirFlowRate,WaterFlowRate,UA.  The IfcTable is related to IfcPropertyTableValue using IfcMetric and IfcPropertyConstraintRelationship."@en , "Courbes de coefficient de transmission thermique total - vitesses de l'eau et de l'air, U.S = [(C1*DébitAéraulique^0,8)^-1 + (C2*DébitHydraulique^0,8)^-1]^-1.\nRemarque: comme deux variables sont utilisées, ValeursDefinir et ValeursDéfinies sont nulles, et les valeurs sont enregistrées dans IfcTable dans l'ordre suivant:\nDébitAéraulique, DebitHydraulique, U.S.\nLe IfcTable est lié à IfcPropertyTableValue en utilisant IfcMetric et IfcPropertyConstraintRelationship."@fr-FR ;
        rdfs:label             "totalUACurves"@en , "CourbesCoefficientTransmissionThermiqueTotal"@fr-FR ;
        schema:domainIncludes  <https://w3id.org/product/Coil> .

props:mountingType  rdfs:comment  "The way the air terminal is mounted to the ceiling, wall, etc.\n\nSurface: mounted to the surface of something (e.g., wall, duct, etc.).\nFlat flush: mounted flat and flush with a surface.\nLay-in: mounted in a lay-in type ceiling (e.g., a dropped ceiling grid)."@en , "ターミナルが天井や壁などに取り付けられる方法。\n表面、水平、LAYIN他\n表面：何か（壁・ダクト等）の表面に取り付け\nFLATFLUSH：表面に水平・Flushni取り付け\nLAYIN：天井にlay-in形式での取り付け（下がり天井格子など）"@ja-JP , "La façon d'être fixé pour le terminal de ventilation au plafond, mur, etc.\n\nSurface: Fixé sur la surface de quelque chose (Ex: mur, conduit, etc.)\nAlignement plat: Fixé plat et dans l'alignement d'une surface.\nInsertion: Fixé dans un type de plafond avec capacité d'insertion (Ex: faux-plafondsuspendu)"@fr-FR ;
        rdfs:label             "mountingType"@en , "取り付け形式"@ja-JP , "ModeFixation"@fr-FR ;
        schema:domainIncludes  <https://w3id.org/product/AirTerminal> .

props:supplyAirConnectionType
        rdfs:comment           "The manner in which the pipe connection is made to the cooled beam."@en ;
        rdfs:label             "supplyAirConnectionType"@en ;
        schema:domainIncludes  <https://w3id.org/product/CooledBeam#ACTIVE> .

props:depth  a                 owl:DatatypeProperty ;
        rdfs:comment           "La profondeur requise ou épaisseur de la réservation."@fr-FR , "空間の厚さに対しての深さが提示されます。"@ja-JP , "空构件的深度或厚度。"@zh-CN , "Geforderte Tiefe des Durchbruchs für eine Nische oder Aussparung. Wenn nicht angegeben, dann ist der geforderte Durchbruch eine Durchbruchsöffnung."@de-DE , "The requested depth or thickness of the provision for void."@en ;
        rdfs:label             "深度"@zh-CN , "Profondeur"@fr-FR , "深さ"@ja-JP , "Tiefe"@de-DE , "depth"@en ;
        rdfs:range             <https://w3id.org/measurement/positiveLength> ;
        schema:domainIncludes  <https://w3id.org/product/BuildingElementProxy#PROVISIONFORVOID> .

props:atmosphericPressure
        a                      owl:DatatypeProperty ;
        rdfs:comment           "周囲大気圧"@ja-JP , "Pression atmosphérique ambiante."@fr-FR , "Ambient atmospheric pressure."@en , "Pression atmosphérique ambiante"@fr-FR ;
        rdfs:label             "大気圧"@ja-JP , "atmosphericPressure"@en , "Pression atmosphérique"@fr-FR ;
        rdfs:range             <https://w3id.org/product/TimeSeries> ;
        rdfs:range             [ owl:allValuesFrom  <https://w3id.org/measurement/pressure> ;
                                 owl:onProperty     <https://w3id.org/measurement/seriesOf>
                               ] ;
        rdfs:range             [ owl:allValuesFrom  <https://w3id.org/measurement/pressure> ;
                                 owl:onProperty     <https://w3id.org/measurement/seriesOf>
                               ] ;
        schema:domainIncludes  <https://w3id.org/product/AirTerminalBox> , <https://w3id.org/product/Coil> .

props:supplyWaterTemperatureHeating
        a                      owl:DatatypeProperty ;
        rdfs:comment           "Supply water temperature in heating mode."@en ;
        rdfs:label             "supplyWaterTemperatureHeating"@en ;
        rdfs:range             <https://w3id.org/product/TimeSeries> ;
        rdfs:range             [ owl:allValuesFrom  <https://w3id.org/measurement/thermodynamicTemperature> ;
                                 owl:onProperty     <https://w3id.org/measurement/seriesOf>
                               ] ;
        schema:domainIncludes  <https://w3id.org/product/CooledBeam> .

props:integratedLightingType
        rdfs:comment           "Integrated lighting in cooled beam."@en ;
        rdfs:label             "integratedLightingType"@en ;
        schema:domainIncludes  <https://w3id.org/product/CooledBeam> .

props:conduitShapeType
        rdfs:comment           "The shape of the conduit segment."@en , "電線管の形状タイプ。\n（円筒形,卵形,その他,不明,なし）"@ja-JP , "전선관의 형상 타입. (원통형, 계란 모양, 기타 알 수 없음) \""@ko-KR ;
        rdfs:label             "conduitShapeType"@en , "電線管のタイプ"@ja-JP , "전선관의 유형"@ko-KR ;
        schema:domainIncludes  <https://w3id.org/product/CableCarrierSegment#CONDUITSEGMENT> .

props:remainingWork  a         owl:DatatypeProperty ;
        rdfs:comment           "The remaining work on behalf of the resource allocation."@en , "資源配分のための残存している作業。"@ja-JP ;
        rdfs:label             "remainingWork"@en , "残存作業時間"@ja-JP ;
        rdfs:range             <https://w3id.org/product/TimeSeries> ;
        rdfs:range             [ owl:allValuesFrom  xsd:duration ;
                                 owl:onProperty     <https://w3id.org/measurement/seriesOf>
                               ] ;
        schema:domainIncludes  <https://w3id.org/product/ConstructionResource> .

props:hasCover  a              owl:DatatypeProperty ;
        rdfs:comment           "Indication of whether the cable tray has a cover (=TRUE) or not (= FALSE). By default, this value should be set to FALSE.."@en , "カバー付かどうか。"@ja-JP , "커버 유무"@ko-KR ;
        rdfs:label             "hasCover"@en , "カバー"@ja-JP , "커버"@ko-KR ;
        rdfs:range             xsd:boolean ;
        schema:domainIncludes  <https://w3id.org/product/CableCarrierSegment#CABLETRAYSEGMENT> .

props:compressorCondenserHeatGain
        a                      owl:DatatypeProperty ;
        rdfs:comment           "Heat gain between condenser inlet to compressor outlet."@en ;
        rdfs:label             "compressorCondenserHeatGain"@en ;
        rdfs:range             <https://w3id.org/product/TimeSeries> ;
        rdfs:range             [ owl:allValuesFrom  <https://w3id.org/measurement/thermodynamicTemperature> ;
                                 owl:onProperty     <https://w3id.org/measurement/seriesOf>
                               ] ;
        schema:domainIncludes  <https://w3id.org/product/Condenser> .

props:name  a                  owl:DatatypeProperty ;
        rdfs:comment           "The name of the air side system."@en , "空調方式の名称。"@ja-JP , "공조 방식의 명칭"@ko-KR ;
        rdfs:label             "name"@en , "名前"@ja-JP , "이름"@ko-KR ;
        rdfs:range             xsd:string ;
        schema:domainIncludes  bot:Zone .

props:nominalPowerConsumption
        a                      owl:DatatypeProperty ;
        rdfs:comment           "Nominal total power consumption."@en , "Puissance de consommation totale nominale."@fr-FR ;
        rdfs:label             "nominalPowerConsumption"@en , "ConsommationPuissanceNominale"@fr-FR ;
        rdfs:range             <https://w3id.org/measurement/power> ;
        schema:domainIncludes  <https://w3id.org/product/Chiller> .

props:displayWidth  a          owl:DatatypeProperty ;
        rdfs:comment           "Indicates the physical width of the screen (only the display surface)."@en , "画面の幅を示す。"@ja-JP , "화면 너비를 보여준다"@ko-KR ;
        rdfs:label             "displayWidth"@en , "画面幅"@ja-JP , "화면 폭"@ko-KR ;
        rdfs:range             <https://w3id.org/measurement/positiveLength> ;
        schema:domainIncludes  <https://w3id.org/product/AudioVisualAppliance#DISPLAY> .

props:airDiffusionPerformanceIndex
        a                      owl:DatatypeProperty ;
        rdfs:comment           "The Air Diffusion Performance Index (ADPI) is used for cooling mode conditions. If several measurements of air velocity and air temperature are made throughout the occupied zone of a space, the ADPI is the percentage of locations where measurements were taken that meet the specifications for effective draft temperature and air velocity."@en , "空気拡散性能指標（ADPI)は冷房時に使用される。\n空気速度および気温のいくつかの測定が空間の居住域の隅々でなされる場合、ADPIは有効な草案の温度および空気速度のための仕様に遭遇する測定が得られた位置の割合である。"@ja-JP , "L'Indice de Performance de Diffusion d'Air (ADPI) est utilisé pour des conditions en mode rafraîchissement. Si plusieurs mesures de vitesses et températures de l'air sont réalisées à travers toute une zone occupée d'un espace,  l'ADPI est le pourcentage des emplacements où les mesures ont été réalisées et qui vérifient les caractéristiques pour une température de courant d'air et de vitesse d'air effectives."@fr-FR ;
        rdfs:label             "airDiffusionPerformanceIndex"@en , "空気拡散性能指標"@ja-JP , "Indice de performance de diffusion de l'air"@fr-FR ;
        rdfs:range             xsd:decimal ;
        schema:domainIncludes  <https://w3id.org/product/AirTerminal> .

props:impedence  a             owl:DatatypeProperty ;
        rdfs:comment           "Indicates the speaker impedence."@en , "インピーダンス値を示す。"@ja-JP , "임피던스 값을 나타낸다."@ko-KR ;
        rdfs:label             "impedence"@en , "インピーダンス値"@ja-JP , "임피던스"@ko-KR ;
        rdfs:range             <https://w3id.org/measurement/frequency> ;
        schema:domainIncludes  <https://w3id.org/product/AudioVisualAppliance#SPEAKER> .

props:isRigid  a               owl:DatatypeProperty ;
        rdfs:comment           "Indication of whether the conduit is rigid (= TRUE) or flexible (= FALSE)."@en , "鋼管か否か。"@ja-JP ;
        rdfs:label             "isRigid"@en , "鋼管"@ja-JP , "강관"@ko-KR ;
        rdfs:range             xsd:boolean ;
        schema:domainIncludes  <https://w3id.org/product/CableCarrierSegment#CONDUITSEGMENT> .

props:capacityControl
        rdfs:comment           "FanCycling: Fan is cycled on and off to control duty.\nTwoSpeedFan: Fan is switched between low and high speed to control duty.\nVariableSpeedFan: Fan speed is varied to control duty.\nDampersControl: Dampers modulate the air flow to control duty.\nBypassValveControl: Bypass valve modulates the water flow to control duty.\nMultipleSeriesPumps: Turn on/off multiple series pump to control duty.\nTwoSpeedPump: Switch between high/low pump speed to control duty.\nVariableSpeedPump: vary pump speed to control duty."@en ;
        rdfs:label             "capacityControl"@en ;
        schema:domainIncludes  <https://w3id.org/product/CoolingTower> .

props:fluid  a                 owl:ObjectProperty ;
        rdfs:comment           "The properties of the hydronic fluid used for heat transfer within the coil tubes."@en , "Les propriétés du fluide utilisé pour l'échange thermique à l'intérieur des tubes de la batterie."@fr-FR ;
        rdfs:label             "fluid"@en , "Fluide"@fr-FR ;
        rdfs:range             <https://w3id.org/product/MaterialDefinition> ;
        schema:domainIncludes  <https://w3id.org/product/Coil> .

props:maximumCableLength
        a                      owl:DatatypeProperty ;
        rdfs:comment           "Maximum cable length based on voltagedrop. NOTE: This value may also be specified as a constraint within an IFC model if required but is included within the property set at this stage pending implementation of the required capabilities within software applications."@en ;
        rdfs:label             "maximumCableLength"@en ;
        rdfs:range             <https://w3id.org/measurement/length> ;
        schema:domainIncludes  <https://w3id.org/product/CableSegment> .

props:actualWork  a            owl:DatatypeProperty ;
        rdfs:comment           "The actual work on behalf of the resource allocation."@en , "資源配分のための実績の作業。"@ja-JP ;
        rdfs:label             "actualWork"@en , "実績作業時間"@ja-JP ;
        rdfs:range             <https://w3id.org/product/TimeSeries> ;
        rdfs:range             [ owl:allValuesFrom  xsd:duration ;
                                 owl:onProperty     <https://w3id.org/measurement/seriesOf>
                               ] ;
        schema:domainIncludes  <https://w3id.org/product/ConstructionResource> .

props:concreteCoverAtLinks
        a                      owl:DatatypeProperty ;
        rdfs:comment           "国の建築基準に従い、補強筋をコンクリートの被りで保護する。"@ja-JP , "The protective concrete cover at the reinforcement links according to local building regulations."@en , "국가의 건축 기준에 따라 보강근 콘크리트의 입고로 보호"@ko-KR , "Abstand zwischen der Betonoberfläche und der Außenkante der vom Beton umhüllten Bewehrungsverbindungsstäben."@de-DE ;
        rdfs:label             "Betonüberdeckung Verbindungsstäbe"@de-DE , "보강근 콘크리트 입고"@ko-KR , "補強筋のコンクリート被り"@ja-JP , "concreteCoverAtLinks"@en ;
        rdfs:range             <https://w3id.org/measurement/positiveLength> ;
        schema:domainIncludes  <https://w3id.org/product/BuildingElement> .

props:playerMediaEject
        a                      owl:DatatypeProperty ;
        rdfs:comment           "Indicates whether the media can be ejected from the player (if physical media)."@en , "メディアを取り出すことができるかどうかを示す。"@ja-JP , "미디어를 꺼낼 수 있는지 여부를 나타낸다."@ko-KR ;
        rdfs:label             "playerMediaEject"@en , "メディア取り出し可否"@ja-JP , "미디어 꺼내기 여부"@ko-KR ;
        rdfs:range             xsd:boolean ;
        schema:domainIncludes  <https://w3id.org/product/AudioVisualAppliance#PLAYER> .

props:coefficientOfPerformance
        a                      owl:DatatypeProperty ;
        rdfs:comment           "Coefficient of performance (COP)."@en , "Coefficient de performance (COP)."@fr-FR , "The Coefficient of performance (COP) is the ratio of heat removed to energy input. \nThe energy input may be obtained by multiplying \nPset_DistributionPortPHistoryGas.FlowRate on the 'Fuel' port of the IfcChiller by Pset_MaterialFuel.LowerHeatingValue.  \nThe IfcDistributionPort for fuel has an associated IfcMaterial with fuel properties and is assigned to an IfcPerformanceHistory object nested within this IfcPerformanceHistory object."@en , "Le coefficient de performance (COP) est le rapport entre l'énergie calorifique fournie sur l'énergie abosrbée.\nL'énergie fournie peut être obtenue en multipliant Pset_DistributionPortHistoryGas.flowRate depuis le port du IfcChiller par Pset_MaterialFuel.LowerHeatingValue.\nLe IfcDistributionPort pour combustible est associé à IfcMaterial pour les propriétés du combustible et est atrribué à l'objet IfcPerformanceHistory situé à l'intérieur même de cet objet IfcPerformanceHistory."@fr-FR ;
        rdfs:label             "coefficientOfPerformance"@en , "CoefficientDePerformance"@fr-FR , "CoefficientPerformance"@fr-FR ;
        rdfs:range             <https://w3id.org/product/TimeSeries> ;
        rdfs:range             [ owl:allValuesFrom  <https://w3id.org/measurement/positiveRatio> ;
                                 owl:onProperty     <https://w3id.org/measurement/seriesOf>
                               ] ;
        rdfs:range             [ owl:allValuesFrom  <https://w3id.org/measurement/positiveRatio> ;
                                 owl:onProperty     <https://w3id.org/measurement/seriesOf>
                               ] ;
        schema:domainIncludes  <https://w3id.org/product/Compressor> , <https://w3id.org/product/Chiller> .

props:frequencyResponse
        rdfs:comment           "Indicates the output over a specified range of frequencies."@en , "周波数範囲での出力を示す。"@ja-JP , "주파수 범위에서 출력을 보여준다."@ko-KR ;
        rdfs:label             "frequencyResponse"@en , "周波数応答"@ja-JP , "주파수 응답"@ko-KR ;
        schema:domainIncludes  <https://w3id.org/product/AudioVisualAppliance#SPEAKER> .

props:nominalCoolingCapacity
        a                      owl:DatatypeProperty ;
        rdfs:comment           "Nominal cooling capacity."@en ;
        rdfs:label             "nominalCoolingCapacity"@en ;
        rdfs:range             <https://w3id.org/measurement/power> ;
        schema:domainIncludes  <https://w3id.org/product/CooledBeam> .

props:refrigerantType
        a                      owl:ObjectProperty ;
        rdfs:comment           "Refrigerant material."@en , "Type de réfrigérant"@fr-FR ;
        rdfs:label             "refrigerantType"@en , "TypeRéfrigérant"@fr-FR ;
        rdfs:range             <https://w3id.org/product/MaterialDefinition> ;
        schema:domainIncludes  <https://w3id.org/product/Compressor> .

props:temperatureRange
        rdfs:comment           "Temperature range."@en , "Temperature range within which the air terminal is designed to operate."@en , "操作されるターミナルの温度範囲"@ja-JP , "Plage de température dans laquelle le terminal de ventilation est prévu de fonctionner."@fr-FR ;
        rdfs:label             "temperatureRange"@en , "温度範囲"@ja-JP , "PlageTemperature"@fr-FR ;
        schema:domainIncludes  <https://w3id.org/product/Damper> , <https://w3id.org/product/AirTerminal> .

props:hasDefrost  a            owl:DatatypeProperty ;
        rdfs:comment           "has the heat exchanger has defrost function or not."@en , "熱交換器のデフロスト機能有無"@ja-JP , "Possède ou non une fonction dégel sur l'échangeur de chaleur"@fr-FR ;
        rdfs:label             "hasDefrost"@en , "デフロスト有無"@ja-JP , "PossèdeDégel"@fr-FR ;
        rdfs:range             xsd:boolean ;
        schema:domainIncludes  <https://w3id.org/product/AirToAirHeatRecovery> .

props:nominalEnergyConsumption
        a                      owl:DatatypeProperty ;
        rdfs:comment           "Nominal fuel consumption rate required to produce the total boiler heat output."@en , "ボイラ最大能力時の設計燃料消費量"@ja-JP , "Consommation nominale de combustible correspondant à la production nominale totale de la chaudière."@fr-FR ;
        rdfs:label             "nominalEnergyConsumption"@en , "設計エネルギー消費量"@ja-JP , "Consommation nominale d'energie"@fr-FR ;
        rdfs:range             <https://w3id.org/measurement/power> ;
        schema:domainIncludes  <https://w3id.org/product/Boiler> .

props:nominalSurroundingHumidityCooling
        a                      owl:DatatypeProperty ;
        rdfs:comment           "Nominal surrounding humidity (refers to nominal cooling capacity)."@en ;
        rdfs:label             "nominalSurroundingHumidityCooling"@en ;
        rdfs:range             <https://w3id.org/measurement/normalisedRatio> ;
        schema:domainIncludes  <https://w3id.org/product/CooledBeam> .

props:controlDamperOperation
        rdfs:comment           "The inherent characteristic of the control damper operation."@en ;
        rdfs:label             "controlDamperOperation"@en ;
        schema:domainIncludes  <https://w3id.org/product/Damper#CONTROLDAMPER> .

props:reinforcementStrengthClass
        a                      owl:DatatypeProperty ;
        rdfs:comment           "Classification of the reinforcement strength in accordance with the concrete design code which is applied in the project. The reinforcing strength class often combines strength and ductility."@en ;
        rdfs:label             "reinforcementStrengthClass"@en ;
        rdfs:range             xsd:string ;
        schema:domainIncludes  <https://w3id.org/product/BuildingElement> .

props:grossPlannedArea
        a                      owl:DatatypeProperty ;
        rdfs:comment           "계획된 그로스 면적. 건물 계획시 사용됩니다."@ko-KR , "計画された建物階のグロス面積。建物計画に際に使用。"@ja-JP , "Surface programmée brute totale de l'étage. Telle que définie lors de la programmation."@fr-FR , "Surface programmée brute totale du bâtiment. Telle que définie lors de la programmation."@fr-FR , "Geforderte Bruttofläche des Geschosses laut Raumprogramm."@de-DE , "計画されたグロス面積。建物計画に際に使用。"@ja-JP , "계획된 건물 층 그로스 면적. 건물 계획시 사용됩니다."@ko-KR , "Total planned area for the building storey. Used for programming the building storey."@en , "Total planned gross area for the building  Used for programming the building."@en , "Geforderte Bruttofläche des Gebäudes laut Raumprogramm."@de-DE ;
        rdfs:label             "계획 그로스 면적"@ko-KR , "計画グロス面積"@ja-JP , "Bruttofläche nach Raumprogramm"@de-DE , "grossPlannedArea"@en , "Surface programmée brute"@fr-FR ;
        rdfs:range             <https://w3id.org/measurement/area> ;
        schema:domainIncludes  <https://w3id.org/product/Building> , <https://w3id.org/product/BuildingStorey> .

props:coolingWaterFlowRate
        a                      owl:DatatypeProperty ;
        rdfs:comment           "Water flow rate for cooling."@en ;
        rdfs:label             "coolingWaterFlowRate"@en ;
        rdfs:range             <https://w3id.org/product/TimeSeries> ;
        rdfs:range             [ owl:allValuesFrom  <https://w3id.org/measurement/volumetricFlowRate> ;
                                 owl:onProperty     <https://w3id.org/measurement/seriesOf>
                               ] ;
        schema:domainIncludes  <https://w3id.org/product/CooledBeam> .

props:liftElevationDifference
        a                      owl:DatatypeProperty ;
        rdfs:comment           "Elevation difference between cooling tower sump and the top of the tower."@en ;
        rdfs:label             "liftElevationDifference"@en ;
        rdfs:range             <https://w3id.org/measurement/positiveLength> ;
        schema:domainIncludes  <https://w3id.org/product/CoolingTower> .

props:assessmentCondition
        a                      owl:DatatypeProperty ;
        rdfs:comment           "The overall condition of a product based on an assessment of the contributions to the overall condition made by the various criteria considered. The meanings given to the values of assessed condition should be agreed and documented by local agreements. For instance, is overall condition measured on a scale of 1 - 10 or by assigning names such as Good, OK, Poor."@en , "様々な基準を用いた評価による製品に関する全体的な状態。評価された状態値の意味は、ローカル協定によって同意され、文書化されなければならない。例えば、状態を1から10の値で計測したり、Good, Ok, Poor等で表す。"@ja-JP ;
        rdfs:label             "assessmentCondition"@en , "評価状態"@ja-JP ;
        rdfs:range             xsd:string ;
        schema:domainIncludes  <https://w3id.org/product/Element> .

props:leakageFullyClosed
        a                      owl:DatatypeProperty ;
        rdfs:comment           "Leakage when fully closed."@en ;
        rdfs:label             "leakageFullyClosed"@en ;
        rdfs:range             <https://w3id.org/measurement/volumetricFlowRate> ;
        schema:domainIncludes  <https://w3id.org/product/Damper> .

props:coreSetVertical
        a                      owl:DatatypeProperty ;
        rdfs:comment           "Degree of vertical (in the Y-axis of the LocalPlacement) blade set from the centerline."@en , "垂直翼の中心線からの垂直（ローカル座標のＹ軸）方向の羽根角度"@ja-JP , "Degré d'inclinaison verticale (selon l'axe Y par rapport au positionnement local) de la lame mesuré depuis la ligne médiane."@fr-FR ;
        rdfs:label             "coreSetVertical"@en , "垂直羽根角度"@ja-JP , "PositionVerticalCentre"@fr-FR ;
        rdfs:range             <https://w3id.org/measurement/planeAngle> ;
        schema:domainIncludes  <https://w3id.org/product/AirTerminal> .

props:nominalReturnWaterTemperatureCooling
        a                      owl:DatatypeProperty ;
        rdfs:comment           "Nominal return water temperature (refers to nominal cooling capacity)."@en ;
        rdfs:label             "nominalReturnWaterTemperatureCooling"@en ;
        rdfs:range             <https://w3id.org/measurement/thermodynamicTemperature> ;
        schema:domainIncludes  <https://w3id.org/product/CooledBeam> .

props:projectorType  rdfs:comment  "Indicates the type of projector."@en , "プロジェクタの形式を示す。"@ja-JP , "프로젝터의 형식을 보여준다."@ko-KR ;
        rdfs:label             "projectorType"@en , "プロジェクター形式"@ja-JP , "프로젝터 형식"@ko-KR ;
        schema:domainIncludes  <https://w3id.org/product/AudioVisualAppliance#PROJECTOR> .

props:pressureLossCoefficient
        a                      owl:DatatypeProperty ;
        rdfs:comment           "Pressure loss coefficient."@en ;
        rdfs:label             "pressureLossCoefficient"@en ;
        rdfs:range             <https://w3id.org/product/TimeSeries> ;
        rdfs:range             [ owl:allValuesFrom  <https://w3id.org/measurement/ratio> ;
                                 owl:onProperty     <https://w3id.org/measurement/seriesOf>
                               ] ;
        schema:domainIncludes  <https://w3id.org/product/Damper> .

props:numberOfStoreys
        a                      owl:DatatypeProperty ;
        rdfs:comment           "The number of storeys within a building.\nCaptured for those cases where the IfcBuildingStorey entity is not used. Note that if IfcBuilingStorey is asserted and the number of storeys in a building can be determined from it, then this approach should be used in preference to setting a property for the number of storeys."@en , "Le nombre de niveaux dans un bâtiment, à indiquer lorsque la classe IfcBuildingStorey n'est pas  utilisée. Il est préférable de créer des instances d'IfcBuildingStorey et d'en déduire le nombre de niveaux plutôt que de saisir cette propriété."@fr-FR , "Anzahl der Vollgeschosse des Gebäudes. \n\nDieses Attribute soll nur dann eingefügt werden, wenn keine Geschosse als Objekte, IfcBuildingStorey, beinhaltet sind. Bei Unstimmigkeiten hat die Anzahl der IfcBuildingStorey Objekte Priorität."@de-DE , "건물 층 수. IfcBuildingStorey 수와 관계없이 취급한다."@ko-KR , "建物階の数。IfcBuildingStoreyの数とは関係なく扱う。"@ja-JP ;
        rdfs:label             "Geschossanzahl"@de-DE , "階数"@ja-JP , "NombreNiveaux"@fr-FR , "층 수"@ko-KR , "numberOfStoreys"@en ;
        rdfs:range             xsd:int ;
        schema:domainIncludes  <https://w3id.org/product/Building> .

props:interiorHeatTransferCoefficient
        a                      owl:DatatypeProperty ;
        rdfs:comment           "Interior heat transfer coefficient associated with interior surface area."@en ;
        rdfs:label             "interiorHeatTransferCoefficient"@en ;
        rdfs:range             <https://w3id.org/product/TimeSeries> ;
        rdfs:range             [ owl:allValuesFrom  <https://w3id.org/measurement/thermalTransmittance> ;
                                 owl:onProperty     <https://w3id.org/measurement/seriesOf>
                               ] ;
        schema:domainIncludes  <https://w3id.org/product/Condenser> .

props:partialLoadEfficiencyCurves
        rdfs:comment           "Boiler efficiency as a function of the partial load factor; E = f (partialLaodfactor)."@en , "部分負荷係数の関数としてのボイラ効率　　E=f(部分負荷率）"@ja-JP , "Rendement de la chaudière en fonction de la facteur de charge partielle; E= f(FacteurChargePartielle)."@fr-FR ;
        rdfs:label             "partialLoadEfficiencyCurves"@en , "部分負荷効率曲線"@ja-JP , "CourbesEfficacitéChargePartielle"@fr-FR ;
        schema:domainIncludes  <https://w3id.org/product/Boiler> .

props:nominalInletAirPressure
        a                      owl:DatatypeProperty ;
        rdfs:comment           "Nominal airflow inlet static pressure."@en , "入口静圧の設計値"@ja-JP , "Pression statique en débit d'air nominal à l'entrée"@fr-FR ;
        rdfs:label             "nominalInletAirPressure"@en , "設計入口空気圧"@ja-JP , "Pression nominale à l'entrée d'air"@fr-FR ;
        rdfs:range             <https://w3id.org/measurement/pressure> ;
        schema:domainIncludes  <https://w3id.org/product/AirTerminalBox> .

props:panTiltZoomPreset
        rdfs:comment           "Indicates pan/tilt/zoom position presets."@en , "パン・チルト・ズーム機能の初期設定。"@ja-JP ;
        rdfs:label             "panTiltZoomPreset"@en , "パン・チルト・ズーム初期設定"@ja-JP ;
        schema:domainIncludes  <https://w3id.org/product/AudioVisualAppliance#CAMERA> .

props:fullLoadRatioCurve
        rdfs:comment           "Ratio of actual power to full load power as a quadratic function of part load, at certain condensing and evaporating temperature, FracFullLoadPower = f ( PartLoadRatio)."@en , "Rapport entre la puissance instantanée et la puissance à pleine charge comme fonction quadratique de charge partielle, pour une certaine température de condensation et une température d'évaporation, FracFullLoadPower= f (CoefficientChargePartielle)"@fr-FR ;
        rdfs:label             "fullLoadRatioCurve"@en , "CourbeFonctionnementPleineCharge"@fr-FR ;
        schema:domainIncludes  <https://w3id.org/product/Chiller> .

props:coefficientOfPerformanceCurve
        rdfs:comment           "Chiller coefficient of performance (COP) is function of condensing temperature and evaporating temperature, data is in table form, COP= f (TempCon, TempEvp), COP = a2+b2*Tei+c2*Tei^2+d2*Tci+e2*Tci^2+f2*Tei*Tci. \nThis table uses multiple input variables; to represent, both DefiningValues and DefinedValues lists are null and IfcTable is attached using IfcPropertyConstraintRelationship and IfcMetric.  Columns are specified in the following order: \n1.IfcPositiveRatioMeasure:CoefficientOfPerformance\n2.IfcThermodynamicTemperatureMeasure:CondensingTemperature\n3.IfcThermodynamicTemperatureMeasure:EvaporatingTemperature"@en , "Coefficient de Performance (COP) du groupe froid qui est une fonction de la température de condensation et de la température d'évaporation, les informations sont sous la forme d'un tableau, COP = f(TempCon,TempEvp), COP = a2+b1*Tei+c2*Tei^2+d2*Tci+e2*Tci^2+f2*Tei*Tci.\nCe tableau utilises plusieurs entrées variables; pour la  représenter, DefiningValues et DefinedValues sont pour les deux nulles et IfcTable est attachée en utilisant IfcPropertyConstraintRelationship et IfcMetric. Les colonnes sont indiquées dans l'ordre suivant:\n1. IfcPowerMeasureCapacity\n2. IfcThermodynamicTemperatureMeasure: CondensingTemperature\n3. IfcThermodynamicTemperatureMeasure: EvaporatingTemperature"@fr-FR ;
        rdfs:label             "coefficientOfPerformanceCurve"@en , "CourbeCOP"@fr-FR ;
        schema:domainIncludes  <https://w3id.org/product/Chiller> .

props:enabled  a               owl:DatatypeProperty ;
        rdfs:comment           "Indicates whether alarm is enabled or disabled over time."@en ;
        rdfs:label             "enabled"@en ;
        rdfs:range             <https://w3id.org/product/TimeSeries> ;
        rdfs:range             [ owl:allValuesFrom  xsd:boolean ;
                                 owl:onProperty     <https://w3id.org/measurement/seriesOf>
                               ] ;
        schema:domainIncludes  <https://w3id.org/product/Alarm> .

props:performance  a           owl:ObjectProperty ;
        rdfs:comment           "Water temperature change as a function of wet-bulb temperature, water entering temperature, water flow rate, air flow rate, Tdiff = f ( Twet-bulb, Twater,in, mwater, mair)."@en ;
        rdfs:label             "performance"@en ;
        rdfs:range             <https://w3id.org/measurement/TimeSeries> ;
        schema:domainIncludes  <https://w3id.org/product/CoolingTower> .

props:signalTimeDecrease
        a                      owl:DatatypeProperty ;
        rdfs:comment           "Time factor used for exponential decrease."@en , "미분 시간 (Td)"@ko-KR ;
        rdfs:label             "signalTimeDecrease"@en , "미분 시간 (Td)"@ko-KR ;
        rdfs:range             <https://w3id.org/measurement/time> ;
        schema:domainIncludes  <https://w3id.org/product/Controller#PROPORTIONAL> .

props:airFlowrateRange
        rdfs:comment           "Air flowrate range within which the air terminal is designed to operate."@en , "操作されるターミナル内の空気流の範囲"@ja-JP , "Plage de débit de ventilation dans laquelle le terminal de ventilation est prévu de fonctionner."@fr-FR ;
        rdfs:label             "airFlowrateRange"@en , "流量範囲"@ja-JP , "PlageDébitVentilation"@fr-FR ;
        schema:domainIncludes  <https://w3id.org/product/AirTerminal> .

props:heatExchangeSurfaceArea
        a                      owl:DatatypeProperty ;
        rdfs:comment           "Heat exchange surface area associated with U-value."@en , "Surface d'échange thermique associé à la valeur U."@fr-FR ;
        rdfs:label             "heatExchangeSurfaceArea"@en , "SurfaceEchangeThermique"@fr-FR ;
        rdfs:range             <https://w3id.org/measurement/area> ;
        schema:domainIncludes  <https://w3id.org/product/Coil> .

props:nominalCondensingTemperature
        a                      owl:DatatypeProperty ;
        rdfs:comment           "Chiller condensing temperature."@en , "Température de condensation du groupe froid."@fr-FR ;
        rdfs:label             "nominalCondensingTemperature"@en , "TemperatureCondensationNominale"@fr-FR ;
        rdfs:range             <https://w3id.org/measurement/thermodynamicTemperature> ;
        schema:domainIncludes  <https://w3id.org/product/Chiller> .

props:secondarySurfaceArea
        a                      owl:DatatypeProperty ;
        rdfs:comment           "Secondary heat transfer surface area created by fins."@en , "Surface d'échange thermique au secondaire crée par les ailettes."@fr-FR ;
        rdfs:label             "secondarySurfaceArea"@en , "SurfaceEchangeSecondaire"@fr-FR ;
        rdfs:range             <https://w3id.org/measurement/area> ;
        schema:domainIncludes  <https://w3id.org/product/Coil> .

props:coilFaceArea  a          owl:DatatypeProperty ;
        rdfs:comment           "Coil face area in the direction against air the flow."@en , "Surface d'échange de la batterie dans la direction contraire du jet."@fr-FR ;
        rdfs:label             "coilFaceArea"@en , "SurfaceEchangeBatterie"@fr-FR ;
        rdfs:range             <https://w3id.org/measurement/area> ;
        schema:domainIncludes  <https://w3id.org/product/Coil> .

props:sensibleHeatRatio
        a                      owl:DatatypeProperty ;
        rdfs:comment           "Air-side sensible heat ratio, or fraction of sensible heat transfer to the total heat transfer."@en , "Ratio de chaleur sensible, ou fraction d'échange thermique sensible sur la chaleur thermique totale échangée."@fr-FR ;
        rdfs:label             "sensibleHeatRatio"@en , "RatioChaleurSensible"@fr-FR ;
        rdfs:range             <https://w3id.org/measurement/normalisedRatio> ;
        schema:domainIncludes  <https://w3id.org/product/Coil> .

props:ventilation  a           owl:DatatypeProperty ;
        rdfs:comment           "Required outside air ventilation."@en , "要求された外気量。"@ja-JP , "요청한 외기 량"@ko-KR ;
        rdfs:label             "ventilation"@en , "外気量"@ja-JP , "외기량"@ko-KR ;
        rdfs:range             <https://w3id.org/measurement/volumetricFlowRate> ;
        schema:domainIncludes  bot:Zone .

props:functionReliable
        a                      owl:DatatypeProperty ;
        rdfs:comment           "コアの維持は特定（テスト）の時間と条件でプロパティ/関数を指定する。標準会議（IEC）規格に準拠。"@ja-JP , "핵심 정비는 특정 (테스트) 시간과 조건의 속성 / 함수를 지정한다. 표준 회의 (IEC) 규격을 준수합니다."@ko-KR , "ケーブルや母線が与えられた時間と条件の中で規定される機能、性質を維持すること。これはIEC基準による。"@ja-JP , "케이블 및 모선 주어진 시간과 조건에서 규정하는 기능, 성질을 유지한다. 이것은 IEC 기준에 의한다."@ko-KR , "Cable/bus maintain given properties/functions over a given (tested) time and conditions. According to IEC standard."@en , "Core maintain given properties/functions over a given (tested) time and conditions. According to (IEC) standard."@en ;
        rdfs:label             "機能信頼性"@ja-JP , "functionReliable"@en , "기능 신뢰성"@ko-KR , "신뢰할 수있는 기능"@ko-KR , "信頼性のある機能"@ja-JP ;
        rdfs:range             xsd:boolean ;
        schema:domainIncludes  <https://w3id.org/product/CableSegment#CABLESEGMENT> , <https://w3id.org/product/CableSegment#CORESEGMENT> .

props:nominalHeatRejectionRate
        a                      owl:DatatypeProperty ;
        rdfs:comment           "Sum of the refrigeration effect and the heat equivalent of the power input to the compressor."@en , "Somme de l'effet de réfrigération et de la chaleur équivalente à la puisssance absorbée par le compresseur."@fr-FR ;
        rdfs:label             "nominalHeatRejectionRate"@en , "CoefficientEvacuationNominaleChaleur"@fr-FR ;
        rdfs:range             <https://w3id.org/measurement/power> ;
        schema:domainIncludes  <https://w3id.org/product/Chiller> .

props:hasSoundAttenuation
        a                      owl:DatatypeProperty ;
        rdfs:comment           "TRUE if the coil has sound attenuation, FALSE if it does not."@en , "VRAI si la batterie possède une correction acoustique, FAUX si ce n'est pas le cas."@fr-FR ;
        rdfs:label             "hasSoundAttenuation"@en , "PossedeCorrectionAcoustique"@fr-FR ;
        rdfs:range             xsd:boolean ;
        schema:domainIncludes  <https://w3id.org/product/Coil> .

props:airflowType  rdfs:comment  "Enumeration defining the functional type of air flow through the terminal."@en , "ターミナルを通過する気流の機能タイプ（給気、還気、排気他）"@ja-JP , "Enumération définissant le type fonctionnel de débit à travers le terminal"@fr-FR ;
        rdfs:label             "airflowType"@en , "エアフロータイプ"@ja-JP , "Type de débit d'air"@fr-FR ;
        schema:domainIncludes  <https://w3id.org/product/AirTerminal> .

props:secondaryAirflowRateRange
        rdfs:comment           "possible range of secondary airflow that can be delivered."@en , "二次側の送風可能範囲"@ja-JP , "Plage possible de débit d'air au secondaire qui peut être fourni."@fr-FR ;
        rdfs:label             "secondaryAirflowRateRange"@en , "二次側風量範囲"@ja-JP , "PlageDébitAirSecondaire"@fr-FR ;
        schema:domainIncludes  <https://w3id.org/product/AirToAirHeatRecovery> .

props:ladderConfiguration
        a                      owl:DatatypeProperty ;
        rdfs:comment           "Description of the configuration of the ladder structure used."@en , "使用されるはしご構造の概要説明。"@ja-JP , "사용되는 사다리 구조의 개요 설명."@ko-KR ;
        rdfs:label             "ladderConfiguration"@en , "梯子設定"@ja-JP , "사다리 설정"@ko-KR ;
        rdfs:range             xsd:string ;
        schema:domainIncludes  <https://w3id.org/product/CableCarrierSegment#CABLELADDERSEGMENT> .

props:marketSubCategoriesAvailableFuture
        rdfs:comment           "A list of the sub categories of property that are expected to be available in the future expressed in terms of IfcLabel."@en , "Liste de sous catégories disponibles dans le futur."@fr-FR ;
        rdfs:label             "marketSubCategoriesAvailableFuture"@en , "DisponibilitesFuturesParSousCategories"@fr-FR ;
        schema:domainIncludes  <https://w3id.org/product/Building> .

props:planningControlStatus
        a                      owl:DatatypeProperty ;
        rdfs:comment           "Label of zoning category or class, or planning control category for the site or facility."@en , "Catégorie de zone ou classe, ou catégorie relativement à un planning de contrôle pour le site ou l'ensemble immobilier."@fr-FR ;
        rdfs:label             "planningControlStatus"@en , "EtatPlanningControle"@fr-FR ;
        rdfs:range             xsd:string ;
        schema:domainIncludes  <https://w3id.org/product/Building> .

props:sheathColors  rdfs:comment  "Colour of the core (derived from IEC 60757). Note that the combined color 'GreenAndYellow' shall be used only as Protective Earth (PE) conductors according to the requirements of IEC 60446."@en , "コア色（IEC60757による）。緑と黄色の混合色の保護接地（PE）の導体は、IEC60446の要件に応じて注意して使用。"@ja-JP , "녹색과 노란색 혼합 색상의 보호 접지 (PE) 도체는 IEC60446의 요구에 따라주의하여 사용."@ko-KR ;
        rdfs:label             "sheathColors"@en , "シース色"@ja-JP , "코어 색"@ko-KR ;
        schema:domainIncludes  <https://w3id.org/product/CableSegment#CORESEGMENT> .

props:signalOffset  a          owl:DatatypeProperty ;
        rdfs:comment           "Offset constant added to modfied signal."@en , "오프셋 상수 변경 신호에 추가됨"@ko-KR ;
        rdfs:label             "signalOffset"@en , "옵셋"@ko-KR ;
        rdfs:range             xsd:decimal ;
        schema:domainIncludes  <https://w3id.org/product/Controller#FLOATING> .

props:fullLoadRatio  a         owl:DatatypeProperty ;
        rdfs:comment           "Ratio of actual power to full load power as a quadratic function of part load, at certain condensing and evaporating temperature, FracFullLoadPower = f ( PartLoadRatio)."@en , "Rapport entre puissance actuelle sur la puissance à pleine charge, comme fonction quadratique de la charge partielle, à une température de condensation et une température d'évaporation donnée, FracFullLoadPower = f (RapportChargePartielle)."@fr-FR ;
        rdfs:label             "fullLoadRatio"@en , "CoefficientChargeTotale"@fr-FR ;
        rdfs:range             <https://w3id.org/product/TimeSeries> ;
        rdfs:range             [ owl:allValuesFrom  <https://w3id.org/measurement/normalisedRatio> ;
                                 owl:onProperty     <https://w3id.org/measurement/seriesOf>
                               ] ;
        schema:domainIncludes  <https://w3id.org/product/Compressor> .

props:thermalTransmittance
        a                      owl:DatatypeProperty ;
        rdfs:comment           "Thermal transmittance coefficient (U-Value) of the element. Here the total thermal transmittance coefficient through the beam within the direction of the thermal flow (including all materials).\n\nNote: new property in IFC4"@en , "材料の熱貫流率（U値）。ここでは、煙突全体の熱の流れる方向の熱貫流率（全ての材料を含む）。"@ja-JP , "材料的导热系数（U值）。\n表示该烟囱在传热方向上的整体导热系数（包括所有材料）。\n注：IFC2x4新添属性"@zh-CN , "Thermal transmittance coefficient (U-Value) of the element. It is the total thermal transmittance coefficient through the building element proxy within the direction of the thermal flow (including all materials).\n\nNote: new property in IFC4"@en , "Thermal transmittance coefficient (U-Value) of the element. Here the total thermal transmittance coefficient through the column within the direction of the thermal flow (including all materials).\n\nNore: new property in IFC4"@en , "Coefficient de transmission thermique surfacique (U). C'est le coefficient global de transmission thermique à travers le mur dans la direction du flux thermique (tous matériaux inclus). Nouvelle propriété de la version 2x4."@fr-FR , "Wärmedurchgangskoeffizient (U-Wert) der Materialschichten.\nHier der Gesamtwärmedurchgangskoeffizient des Balkens (in Richtung des Wärmeflusses), angegeben ohne den inneren und äußeren Wärmeübergangswiderstand."@de-DE , "材料的导热系数（U值）。\n\n表示该梁在传热方向上的整体导热系数（包括所有材料）。\n\n注：IFC2x4新添属性"@zh-CN , "Wärmedurchgangskoeffizient (U-Wert) der Materialschichten.\nHier der Gesamtwärmedurchgangskoeffizient des Schornsteins (in Richtung des Wärmeflusses), angegeben ohne den inneren und äußeren Wärmeübergangswiderstand."@de-DE , "Coefficient de transmission thermique surfacique (U). C'est le coefficient global de transmission thermique à travers la poutre dans la direction du flux thermique (tous matériaux inclus). Nouvelle propriété de la version 2x4."@fr-FR , "Coefficient de transmission thermique surfacique (U). C'est le coefficient global de transmission thermique à travers le revêtement dans la direction du flux thermique (tous matériaux inclus). Nouvelle propriété de la version 2x4."@fr-FR , "Thermal transmittance coefficient (U-Value) of a material.\nHere the total thermal transmittance coefficient through the wall (including all materials)."@en , "Coefficient de transmission thermique surfacique (U). C'est le coefficient global de transmission thermique à travers le poteau dans la direction du flux thermique (tous matériaux inclus). Nouvelle propriété de la version 2x4."@fr-FR , "材料的导热系数（U值）。\n\n表示该柱在传热方向上的整体导热系数（包括所有材料）。\n\n注：IFC2x4新添属性"@zh-CN , "熱貫流率U値。ここでは柱を通した熱移動の方向における全体の熱還流率を示す。"@ja-JP , "Coefficient de transmission thermique surfacique (U). C'est le coefficient global de transmission thermique à travers la cheminée dans la direction du flux thermique (tous matériaux inclus). Nouvelle propriété de la version 2x4."@fr-FR , "熱貫流率U値。ここではオブジェクトを通した熱移動の方向における全体の熱還流率を示す。"@ja-JP , "Coefficient de transmission thermique surfacique (U). C'est le coefficient global de transmission thermique à travers l'élément dans la direction du flux thermique (tous matériaux inclus). Nouvelle propriété de la version 2x4."@fr-FR , "熱貫流率U値。ここではカーテンウォールを通した熱移動の方向における全体の熱還流率を示す。"@ja-JP , "熱貫流率U値。ここではカバリングを通した熱移動の方向における全体の熱還流率を示す。"@ja-JP , "熱貫流率U値。\nここでは（すべての材料を含む）梁を通した熱移動の方向における全体の熱還流率を示す。\n注：IFC2x4の新しいプロパティ"@ja-JP , "Thermal transmittance coefficient (U-Value) of an element. \nHere the total thermal transmittance coefficient through the covering (including all materials)."@en , "Wärmedurchgangskoeffizient (U-Wert) der Materialschichten. Angegeben wird der  Gesamtwärmedurchgangskoeffizient des Proxy-Elements (in Richtung des Wärmeflusses), ohne den inneren und äußeren Wärmeübergangswiderstand."@de-DE , "Thermal transmittance coefficient (U-Value) of an element. Here the total thermal transmittance coefficient through the chimney within the direction of the thermal flow (including all materials)."@en , "Wärmedurchgangskoeffizient (U-Wert) der Materialschichten.\nHier der Gesamtwärmedurchgangskoeffizient der Bekleidung (für alle Schichten)."@de-DE , "材料的导热系数（U值）。\n表示穿过该墙的整体导热系数（包括所有材料）。"@zh-CN , "材料的导热系数（U值）。\n表示该烟囱在传热方向上的整体导热系数（包括所有材料）。"@zh-CN , "材料的导热系数（U值）。\n表示穿过该覆盖层的整体导热系数（包括所有材料）。"@zh-CN ;
        rdfs:label             "Transmission thermique surfacique"@fr-FR , "TransmissionThermique"@fr-FR , "导热系数"@zh-CN , "thermalTransmittance"@en , "U-Wert"@de-DE , "熱貫流率"@ja-JP ;
        rdfs:range             <https://w3id.org/measurement/thermalTransmittance> ;
        schema:domainIncludes  <https://w3id.org/product/Beam> , <https://w3id.org/product/CurtainWall> , <https://w3id.org/product/Column> , <https://w3id.org/product/Covering> , <https://w3id.org/product/BuildingElementProxy> , <https://w3id.org/product/Chimney> .

props:sensibleHeatTransferRate
        a                      owl:DatatypeProperty ;
        rdfs:comment           "Puissance thermique sensible"@fr-FR , "顕熱交換量"@ja-JP , "Sensible heat transfer rate."@en ;
        rdfs:label             "sensibleHeatTransferRate"@en , "顕熱交換量"@ja-JP , "PuissanceThermiqueSensible"@fr-FR ;
        rdfs:range             <https://w3id.org/product/TimeSeries> ;
        rdfs:range             [ owl:allValuesFrom  <https://w3id.org/measurement/power> ;
                                 owl:onProperty     <https://w3id.org/measurement/seriesOf>
                               ] ;
        schema:domainIncludes  <https://w3id.org/product/AirToAirHeatRecovery> .

props:airPressureRange
        rdfs:comment           "Allowable air static pressure range at the entrance of the air terminal box."@en , "ターミナル入り口での許容静圧範囲"@ja-JP , "Plage admise de la pression statique de l'air à l'entrée du registre terminal de ventilation"@fr-FR ;
        rdfs:label             "airPressureRange"@en , "空気圧範囲"@ja-JP , "Plage de pression d'air"@fr-FR ;
        schema:domainIncludes  <https://w3id.org/product/AirTerminalBox> .

props:diameter  a              owl:DatatypeProperty ;
        rdfs:comment           "空构件的直径（在立面图中），仅当“形状”属性为“圆形”时适用。"@zh-CN , "Geforderte Durchmesser des Durchbruchs, wird nur dann angegeben, wenn der Wert des Attributes \"Form\" gleich \"Rund\" ist."@de-DE , "The requested diameter (in elevation) of the provision for void, only provided if the Shape property is set to \"round\"."@en , "空間における直径（高さにおける）を求める定義です。「円」形状プロパティのみに提示されます。"@ja-JP , "Le diamètre requis de la réservation (en élévation). Fournie seulement si la propriété Forme a pour valeur \"Round\"."@fr-FR ;
        rdfs:label             "直径"@ja-JP , "直径"@zh-CN , "Diamètre"@fr-FR , "diameter"@en , "Durchmesser"@de-DE ;
        rdfs:range             <https://w3id.org/measurement/positiveLength> ;
        schema:domainIncludes  <https://w3id.org/product/BuildingElementProxy#PROVISIONFORVOID> .

props:leakageCurve  rdfs:comment  "Leakage versus pressure drop; Leakage = f (pressure)."@en ;
        rdfs:label             "leakageCurve"@en ;
        schema:domainIncludes  <https://w3id.org/product/Damper> .

props:fireProtectionClass
        a                      owl:DatatypeProperty ;
        rdfs:comment           "Zugewiesene Gebäudeklasse nach der nationalen Brandschutzverordnung."@de-DE , "主要な防火等級。関連する建築基準法、消防法などの国家基準を参照。"@ja-JP , "Classe principale de protection contre le risque incendie, selon la réglementation nationale."@fr-FR , "주요 방화 등급. 관련 건축 기준법, 소방법 등의 국가 표준을 참조하십시오."@ko-KR , "Main fire protection class for the building which is assigned from the fire protection classification table as given by the relevant national building code."@en ;
        rdfs:label             "耐火等級"@ja-JP , "fireProtectionClass"@en , "방화 등급"@ko-KR , "Gebäudeklasse Brandschutz"@de-DE , "RisqueIncendieUsageSecondaire"@fr-FR ;
        rdfs:range             xsd:string ;
        schema:domainIncludes  <https://w3id.org/product/Building> .

props:range  rdfs:comment      "The physical range of values."@en , "The physical range of values supported by the device."@en ;
        rdfs:label             "range"@en ;
        schema:domainIncludes  <https://w3id.org/product/Controller#PROPORTIONAL> , <https://w3id.org/product/Controller#MULTIPOSITION> , <https://w3id.org/product/Controller#FLOATING> .

props:heatRejectionRate
        a                      owl:DatatypeProperty ;
        rdfs:comment           "Sum of the refrigeration effect and the heat equivalent of the power input to the compressor."@en ;
        rdfs:label             "heatRejectionRate"@en ;
        rdfs:range             <https://w3id.org/product/TimeSeries> ;
        rdfs:range             [ owl:allValuesFrom  <https://w3id.org/measurement/power> ;
                                 owl:onProperty     <https://w3id.org/measurement/seriesOf>
                               ] ;
        schema:domainIncludes  <https://w3id.org/product/Condenser> .

props:capacityCurve  rdfs:comment  "Chiller cooling capacity is a function of condensing temperature and evaporating temperature, data is in table form, Capacity = f (TempCon, TempEvp), capacity = a1+b1*Tei+c1*Tei^2+d1*Tci+e1*Tci^2+f1*Tei*Tci. \nThis table uses multiple input variables; to represent, both DefiningValues and DefinedValues lists are null and IfcTable is attached using IfcPropertyConstraintRelationship and IfcMetric.  Columns are specified in the following order: \n1.IfcPowerMeasure:Capacity\n2.IfcThermodynamicTemperatureMeasure:CondensingTemperature\n3.IfcThermodynamicTemperatureMeasure:EvaporatingTemperature"@en , "Puissance frigoifique du groupe froid qui est une fonction de la température de condensation et de la température d'évaporation, les informations sont sous la forme d'un tableau, Puissance = f(TempCon,TempEvp), puissance = a1+b1*Tei+c1*Tei^2+d1*Tci+e1*Tci^2+f1*Tei*Tci.\nCe tableau utilises plusieurs entrées variables; pour la  représenter, DefiningValues et DefinedValues sont pour les deux nulles et IfcTable est attachée en utilisant IfcPropertyConstraintRelationship et IfcMetric. Les colonnes sont indiquées dans l'ordre suivant:\n1. IfcPowerMeasure: Capacity\n2. IfcThermodynamicTemperatureMeasure: CondensingTemperature\n3. IfcThermodynamicTemperatureMeasure: EvaporatingTemperature"@fr-FR ;
        rdfs:label             "capacityCurve"@en , "CourbePuissance"@fr-FR ;
        schema:domainIncludes  <https://w3id.org/product/Chiller> .

props:videoCaptureInterval
        rdfs:comment           "Indicates video frame capture time intervals."@en , "撮影間隔を示す。"@ja-JP ;
        rdfs:label             "videoCaptureInterval"@en , "撮影間隔"@ja-JP ;
        schema:domainIncludes  <https://w3id.org/product/AudioVisualAppliance#CAMERA> .

props:width  a                 owl:DatatypeProperty ;
        rdfs:comment           "La largeur requise de la réservation (extension horizontale en élévation). Fournie seulement si la propriété Forme a pour valeur \"Rectangle\"."@fr-FR , "Geforderte Breite des Durchbruchs, wird nur dann angegeben, wenn der Wert des Attributes \"Form\" gleich \"Rechteck\" ist."@de-DE , "空間の幅（高さにおける水平方向の拡張）を求める定義です。「四角形」の形状プロパティのみ提示されます。"@ja-JP , "The requested width (horizontal extension in elevation) of the provision for void, only provided if the Shape property is set to \"rectangle\"."@en , "空构件的宽度（在立面图中水平方向的长度），仅当“形状”属性为“矩形”时适用。"@zh-CN ;
        rdfs:label             "宽度"@zh-CN , "Largeur"@fr-FR , "Breite"@de-DE , "width"@en , "幅"@ja-JP ;
        rdfs:range             <https://w3id.org/measurement/positiveLength> ;
        schema:domainIncludes  <https://w3id.org/product/BuildingElementProxy#PROVISIONFORVOID> .

props:netPlannedArea  a        owl:DatatypeProperty ;
        rdfs:comment           "계획된 건물 층 인터넷 공간이 있습니다. 건물 계획시 사용됩니다."@ko-KR , "Geforderte Nettofläche des Geschosses laut Raumprogramm."@de-DE , "計画されたネット面積。建物計画に際に使用。（通常は、柱型等を抜いた面積となる）"@ja-JP , "Surface programmée nette totale de l'étage. Telle que définie lors de la programmation."@fr-FR , "Surface programmée nette totale du bâtiment. Telle que définie lors de la programmation."@fr-FR , "Total planned net area for the building storey. Used for programming the building storey."@en , "計画された建物階のネット面積。建物計画の際に使用。"@ja-JP , "Geforderte Nettofläche des Gebäudes laut Raumprogramm."@de-DE , "Total planned net area for the building  Used for programming the building."@en ;
        rdfs:label             "Surface programmée nette"@fr-FR , "Nettofläche nach Raumprogramm"@de-DE , "계획 인터넷 면적"@ko-KR , "netPlannedArea"@en , "計画ネット面積"@ja-JP ;
        rdfs:range             <https://w3id.org/measurement/area> ;
        schema:domainIncludes  <https://w3id.org/product/Building> , <https://w3id.org/product/BuildingStorey> .

props:nominalSurroundingTemperatureHeating
        a                      owl:DatatypeProperty ;
        rdfs:comment           "Nominal surrounding temperature (refers to nominal heating capacity)."@en ;
        rdfs:label             "nominalSurroundingTemperatureHeating"@en ;
        rdfs:range             <https://w3id.org/measurement/thermodynamicTemperature> ;
        schema:domainIncludes  <https://w3id.org/product/CooledBeam> .

props:actuationType  rdfs:comment  "Enumeration that identifies the different types of dampers."@en ;
        rdfs:label             "actuationType"@en ;
        schema:domainIncludes  <https://w3id.org/product/Damper#FIRESMOKEDAMPER> , <https://w3id.org/product/Damper#FIREDAMPER> .

props:flowArrangement
        rdfs:comment           "CounterFlow: Air and water flow enter in different directions.\nCrossFlow: Air and water flow are perpendicular.\nParallelFlow: air and water flow enter in same directions."@en ;
        rdfs:label             "flowArrangement"@en ;
        schema:domainIncludes  <https://w3id.org/product/CoolingTower> .

props:userCorrectionFactor
        a                      owl:DatatypeProperty ;
        rdfs:comment           "An arbitrary correction factor that may be applied by the user."@en ;
        rdfs:label             "userCorrectionFactor"@en ;
        rdfs:range             xsd:decimal ;
        schema:domainIncludes  <https://w3id.org/product/CableSegment> .

props:crossSectionalArea
        a                      owl:DatatypeProperty ;
        rdfs:comment           "Cross section area of the phase(s) lead(s)."@en , "位相、リードの断面積。"@ja-JP , "리드 단면적."@ko-KR ;
        rdfs:label             "crossSectionalArea"@en , "断面積"@ja-JP , "단면적 영역"@ko-KR ;
        rdfs:range             <https://w3id.org/measurement/area> ;
        schema:domainIncludes  <https://w3id.org/product/CableSegment#CONDUCTORSEGMENT> .

props:tileWidth  a             owl:DatatypeProperty ;
        rdfs:comment           "Breite der Unterdeckenplatten, oder -panele, die zur Verkleidung verwendet werden."@de-DE , "Largeur des carreaux de plafond. Cette propriété est donnée en complément de la représentation de la forme et des paramètres géométriques qui la déterminent. En cas d'incohérence entre ces paramètres géométriques et cette propriété, ce sont les paramètres géométriques qui priment."@fr-FR , "天花板面砖的宽度。\n该属性所提供的尺寸信息是对内部形状描述和几何参数的补充。如果几何参数与该属性所提供的尺寸属性不符，应以几何参数为准。"@zh-CN , "Width of ceiling tiles. The size information is provided in addition to the shape representation and the geometric parameters used within. In cases of inconsistency between the geometric parameters and the size properties, provided in the attached property set, the geometric parameters take precedence."@en ;
        rdfs:label             "Deckenplattenbreite"@de-DE , "Largeur des carreaux"@fr-FR , "tileWidth"@en , "面砖宽度"@zh-CN ;
        rdfs:range             <https://w3id.org/measurement/positiveLength> ;
        schema:domainIncludes  <https://w3id.org/product/Covering#CEILING> .

props:refrigerantClass
        rdfs:comment           "Refrigerant class used by the condenser.\n\nCFC: Chlorofluorocarbons.\nHCFC: Hydrochlorofluorocarbons.\nHFC: Hydrofluorocarbons."@en , "Refrigerant class used by the compressor.\n\nCFC: Chlorofluorocarbons.\nHCFC: Hydrochlorofluorocarbons.\nHFC: Hydrofluorocarbons."@en , "Classe de réfrigérant utilisé par le compresseur.\n\nCFC\nHCFC\nHFC"@fr-FR ;
        rdfs:label             "refrigerantClass"@en , "ClasseRéfrigérant"@fr-FR ;
        schema:domainIncludes  <https://w3id.org/product/Condenser> , <https://w3id.org/product/Compressor> .

props:displayType  rdfs:comment  "Indicates the type of display."@en , "画面の種類を示す。"@ja-JP , "화면 종류를 나타낸다"@ko-KR ;
        rdfs:label             "displayType"@en , "画面種類"@ja-JP , "화면 유형"@ko-KR ;
        schema:domainIncludes  <https://w3id.org/product/AudioVisualAppliance#DISPLAY> .

props:signalTime  a            owl:DatatypeProperty ;
        rdfs:comment           "Time factor used for integral and running average controllers."@en , "시간 요소는 INTEGRAL (적분)과 AVERAGE ((이동) 평균) 컨트롤러에 사용됨"@ko-KR ;
        rdfs:label             "signalTime"@en , "시간 요소"@ko-KR ;
        rdfs:range             <https://w3id.org/measurement/time> ;
        schema:domainIncludes  <https://w3id.org/product/Controller#FLOATING> .

props:waterRequirement
        a                      owl:DatatypeProperty ;
        rdfs:comment           "Make-up water requirements."@en ;
        rdfs:label             "waterRequirement"@en ;
        rdfs:range             <https://w3id.org/measurement/volumetricFlowRate> ;
        schema:domainIncludes  <https://w3id.org/product/CoolingTower> .

props:nominalEfficiency
        a                      owl:DatatypeProperty ;
        rdfs:comment           "Efficactié nominale du groupe froid sous les conditions nominales."@fr-FR , "Efficacité nominale de la chaudière tel que définie par le constructeur.\nPour les chaudières à eau chaude, une fonction de la température en entrée par rapport à la température de sortie.\nRemarque: Comme deux variables sont utilisées ValeurDefinir et ValeursDefinies sont nulles, et les valeurs sont enregistrées dans IfcTable dans l'ordre suivant:\n- TempératureEntrée (IfcThermodynamicTemperatureMeasure) et TempératureSortie (IfcThermodynamicTemperatureMeasure) dans ValeursDefinir , et EfficacitéNominale (IfcNormalisedRatioMeasure) dansValeursDefinies.\nIfcTable est lié à IfcPropertyTableValue qui utilise IfcMetric et IfcPropertyConstraintRelationship."@fr-FR , "Nominal chiller efficiency under nominal conditions."@en , "Efficacité nominale de la chaudière tel que définie par le constructeur.\nPour les chaudières à vapeur, une fonction de la température en entrée par rapport à la pression de vapeur.\nRemarque: Comme deux variables sont utilisées ValeurDefinir et ValeursDefinies sont nulles, et les valeurs sont enregistrées dans IfcTable dans l'ordre suivant:\n- TempératureEntrée (IfcThermodynamicTemperatureMeasure) et TempératureSortie (IfcThermodynamicTemperatureMeasure) dans ValeursDefinir , et EfficacitéNominale (IfcNormalisedRatioMeasure) dansValeursDefinies.\nPar exemple, ValeursDefinir (TempératureEntrée, TempératureSortie), ValeursDefinies (nul, RendementNominal).\nIfcTable est lié à IfcPropertyTableValue qui utilise IfcMetric et IfcPropertyConstraintRelationship."@fr-FR , "The nominal efficiency of the boiler as defined by the manufacturer. For steam boilers, a function of inlet temperature versus steam pressure.  Note: as two variables are used, DefiningValues and DefinedValues are null, and values are stored in IfcTable in the following order: InletTemperature(IfcThermodynamicTemperatureMeasure) and OutletTemperature(IfcThermodynamicTemperatureMeasure) in DefiningValues, and NominalEfficiency(IfcNormalisedRatioMeasure) in DefinedValues. For example, DefininfValues(InletTemp, OutletTemp), DefinedValues(null, NominalEfficiency).  The IfcTable is related to IfcPropertyTableValue using IfcMetric and IfcPropertyConstraintRelationship."@en , "The nominal efficiency of the boiler as defined by the manufacturer. For water boilers, a function of inlet versus outlet temperature. Note: as two variables are used, DefiningValues and DefinedValues are null, and values are stored in IfcTable in the following order: InletTemperature(IfcThermodynamicTemperatureMeasure), OutletTemperature(IfcThermodynamicTemperatureMeasure), NominalEfficiency(IfcNormalizedRatioMeasure).  The IfcTable is related to IfcPropertyTableValue using IfcMetric and IfcPropertyConstraintRelationship."@en ;
        rdfs:label             "EfficacitéNominale"@fr-FR , "nominalEfficiency"@en ;
        rdfs:range             <https://w3id.org/measurement/positiveRatio> ;
        schema:domainIncludes  <https://w3id.org/product/Boiler#STEAM> , <https://w3id.org/product/Chiller> , <https://w3id.org/product/Boiler#WATER> .

props:isHorizontalBusbar
        a                      owl:DatatypeProperty ;
        rdfs:comment           "Indication of whether the busbar occurrences are routed horizontally (= TRUE) or vertically (= FALSE)."@en , "母線は、水平方向にルーティングされるかどうかを示す（= TRUE）または垂直方向に（= FALSE）を返します。"@ja-JP , "모선은 가로로 라우팅되는지 여부를 나타내는 (= TRUE) 또는 수직 (= FALSE)를 반환합니다."@ko-KR ;
        rdfs:label             "isHorizontalBusbar"@en , "水平母線"@ja-JP , "수평 모선"@ko-KR ;
        rdfs:range             xsd:boolean ;
        schema:domainIncludes  <https://w3id.org/product/CableSegment#BUSBARSEGMENT> .

props:waterStorageCapacity
        a                      owl:DatatypeProperty ;
        rdfs:comment           "Water storage capacity."@en , "缶内水量"@ja-JP , "Capacité de réserve en eau"@fr-FR ;
        rdfs:label             "waterStorageCapacity"@en , "缶内水量"@ja-JP , "CapacitéRéservoirEau"@fr-FR ;
        rdfs:range             <https://w3id.org/measurement/volume> ;
        schema:domainIncludes  <https://w3id.org/product/Boiler> .

props:totalEffectivenessTable
        a                      owl:ObjectProperty ;
        rdfs:comment           "Total heat transfer effectiveness curve as a function of the primary and secondary air flow rate."@en , "一次と二次空気量の関数としての全熱交換効率曲線"@ja-JP , "Courbe d'efficacité d'échange thermique total en tant que fonction du débit d'air au primaire et débit d'air au secondaire"@fr-FR ;
        rdfs:label             "totalEffectivenessTable"@en , "全熱効率テーブル"@ja-JP , "DiagrammeEfficacitéTotale"@fr-FR ;
        rdfs:range             <https://w3id.org/measurement/TimeSeries> ;
        schema:domainIncludes  <https://w3id.org/product/AirToAirHeatRecovery> .

props:isPermanentID  a         owl:DatatypeProperty ;
        rdfs:comment           "Indicates whether the identity assigned to a building is permanent (= TRUE) or temporary (=FALSE)."@en , "建物IDが恒久的なIDかどうかのブーリアン値。"@ja-JP , "Indique si l'identifiant attribuée au bâtiment est permanent (=VRAI) ou temporaire (=FAUX)."@fr-FR , "Angabe, on das angegebene Gebäudekennzeichen permanent ist (TRUE), oder eine temporäre Antragsnummer (FALSE)."@de-DE , "건물 ID가 영구적인 ID 여부값"@ko-KR ;
        rdfs:label             "IdPermanent"@fr-FR , "Gebäudekennzeichen permanent"@de-DE , "영구 ID 구분"@ko-KR , "永久ID区分"@ja-JP , "isPermanentID"@en ;
        rdfs:range             xsd:boolean ;
        schema:domainIncludes  <https://w3id.org/product/Building> .

props:tenureModesAvailableNow
        rdfs:comment           "A list of the tenure modes that are currently available expressed in terms of IfcLabel."@en , "Liste des possibilités d'occupation actuelles."@fr-FR ;
        rdfs:label             "tenureModesAvailableNow"@en , "PossibilitesOccupationActuelles"@fr-FR ;
        schema:domainIncludes  <https://w3id.org/product/Building> .

props:operation  rdfs:comment  "The operational mechanism for the damper operation."@en ;
        rdfs:label             "operation"@en ;
        schema:domainIncludes  <https://w3id.org/product/Damper> .

props:sound  a                 owl:DatatypeProperty ;
        rdfs:comment           "騒音性能"@ja-JP , "Performance acoustique"@fr-FR , "Sound performance."@en ;
        rdfs:label             "sound"@en , "Acoustique"@fr-FR , "騒音"@ja-JP ;
        rdfs:range             <https://w3id.org/product/TimeSeries> ;
        rdfs:range             [ owl:allValuesFrom  <https://w3id.org/measurement/soundPressure> ;
                                 owl:onProperty     <https://w3id.org/measurement/seriesOf>
                               ] ;
        schema:domainIncludes  <https://w3id.org/product/AirTerminalBox> .

props:soilConductivity
        a                      owl:DatatypeProperty ;
        rdfs:comment           "Thermal conductivity of soil. Generally, within standards such as IEC 60364-5-52, table 52A-16, the resistivity of soil is required (measured in [SI] units of degK.m /W). This is the reciprocal of the conductivity value and needs to be calculated accordingly."@en ;
        rdfs:label             "soilConductivity"@en ;
        rdfs:range             <https://w3id.org/measurement/thermalConductivity> ;
        schema:domainIncludes  <https://w3id.org/product/CableSegment> .

props:tunerMode  rdfs:comment  "Indicates the tuner modes (or bands).  For example, 'AnalogCable', 'DigitalAir', 'AM', 'FM'."@en , "受信可能な放送モードを示す。"@ja-JP , "수신 가능한 방송 모드를 나타낸다."@ko-KR ;
        rdfs:label             "tunerMode"@en , "チューナーモード"@ja-JP , "튜너 모드"@ko-KR ;
        schema:domainIncludes  <https://w3id.org/product/AudioVisualAppliance#TUNER> .

props:roll  a                  owl:DatatypeProperty ;
        rdfs:comment           "柱の長軸に対する回転。"@ja-JP , "Drehwinkel der Stütze relative zur globalen X Ausrichtung (O Grad). Bei nicht-vertikalen Stützen wird die Verdrehung analog zu den Balken (Verkippung gegen die Vertikale) angegeben.\n\nDieser Parameter wird zusätzlich zur geometrischen Repräsentation bereitgestellt. Im Fall der Inkonsistenz zwischen dem Parameter und der Geometrie hat die geometrische Repräsention Priorität. Dieser Parameter ist für CAD Software write-only."@de-DE , "Kippwinkel des Balkens relative zur Vertikalen (O Grad).\n\nDieser Parameter wird zusätzlich zur geometrischen Repräsentation bereitgestellt. Im Fall der Inkonsistenz zwischen dem Parameter und der Geometrie hat die geometrische Repräsention Priorität. Dieser Parameter ist für CAD Software write-only."@de-DE , "相对于纵轴的旋转角。对全局坐标系中的垂直柱，该属性为相对于X轴的角度。（若轮廓方向在X轴上，则转角为0。）对全局坐标系中的非垂直柱，该属性为相对于Z轴的角度。（若轮廓方向在Z轴上，则转角为0。）\n该属性所提供的形状信息是对内部形状描述和几何参数的补充。如果几何参数与该属性所提供的形状属性不符，应以几何参数为准。对CAD等几何编辑程序，该属性应为只写类型。\n注：IFC2x4新添属性"@zh-CN , "Rotation autour de l'axe longitudinal - relativement à l'axe Z pour toutes les poutres qui ne sont pas verticales relativement au repère absolu (la direction du profil est celle de l'axe Z si la valeur de la propriété est 0). Cette propriété est donnée en complément de la représentation de la forme de l'élément et des paramètres géométriques qui la déterminent. En cas d'incohérence entre ces paramètres géométriques et cette propriété, ce sont les paramètres géométriques qui priment. Les applications qui déterminent la géométrie comme les logiciels de CAO ne doivent pas autoriser la modification de cette propriété. Note : nouvelle propriété de la version IFC2x4."@fr-FR , "Rotation against the longitudinal axis - relative to the global Z direction for all beams that are non-vertical in regard to the global coordinate system (Profile direction equals global Z is Roll = 0.)\n\nThe shape information is provided in addition to the shape representation and the geometric parameters used within. In cases of inconsistency between the geometric parameters and the shape properties, provided in the attached property, the geometric parameters take precedence.  For geometry editing applications, like CAD: this value should be write-only.\n\nNote: new property in IFC4"@en , "梁の材軸に対する回転。\n-この材軸はグローバル座標系で非垂直な全ての梁に対してグローバルZ方向へ相対する。（表示方向は、グローバルZの回転方向を0とする。）\n\nその形状（梁の回転）情報は、表示のための形状に内部で使用される幾何学的パラメータを加えて提供される。形状情報と内部の幾何学的パラメータに矛盾が生じた場合は、幾何学的パラメータが優先される。幾何学的パラメ－タ編集アプリケーションでは、CADと同様に、この値は書き込み専用とする。\n\n注：IFC2x4の新しいプロパティ"@ja-JP , "Rotation against the longitudinal axis - relative to the global  X direction for all columns that are vertical in regard to the global coordinate system (Profile direction equals global X is Roll = 0.). For all non-vertical columns the following applies:  Roll is relative to the global Z direction f(Profile direction of non-vertical columns that equals global Z is Roll = 0.)\n\nThe shape information is provided in addition to the shape representation and the geometric parameters used within. In cases of inconsistency between the geometric parameters and the shape properties, provided in the attached property, the geometric parameters take precedence.  For geometry editing applications, like CAD: this value should be write-only.\n\nNote: new property in IFC4"@en , "Rotation autour de l'axe longitudinal - relativement à l'axe X pour tous les poteaux qui sont verticaux relativement au repère absolu (la direction du profil est celle de l'axe X si la valeur est 0). Pour tous les poteaux non verticaux, la valeur de la propriété est relative à l'axe Z (la direction du profil des poteaux non verticaux est celle de l'axe Z si la valeur est 0). \nCette propriété est donnée en complément de la représentation de la forme de l'élément et des paramètres géométriques qui la déterminent. En cas d'incohérence entre ces paramètres géométriques et cette propriété, ce sont les paramètres géométriques qui priment. Les applications qui déterminent la géométrie comme les logiciels de CAO ne doivent pas autoriser la modification de cette propriété. Note : nouvelle propriété de la version IFC2x4."@fr-FR , "相对于纵轴的旋转角。对全局坐标系中的非垂直梁，该属性为相对于Z轴的角度。（若轮廓方向在Z轴上，则转角为0。）\n该属性所提供的形状信息是对内部形状描述和几何参数的补充。如果几何参数与该属性所提供的形状属性不符，应以几何参数为准。对CAD等几何编辑程序，该属性应为只写类型。\n注：IFC2x4新添属性"@zh-CN ;
        rdfs:label             "Kippwinkel"@de-DE , "回転"@ja-JP , "Drehwinkel"@de-DE , "转角"@zh-CN , "RotationAutourAxeLongitudinal"@fr-FR , "roll"@en ;
        rdfs:range             <https://w3id.org/measurement/planeAngle> ;
        schema:domainIncludes  <https://w3id.org/product/Column> , <https://w3id.org/product/Beam> .

props:overallDiameter
        a                      owl:DatatypeProperty ;
        rdfs:comment           "The overall diameter of a Cable/Bus."@en , "케이블과 모선의 외형 치수 (직경)를 나타낸다."@ko-KR , "전체 직경 (최대 공간)."@ko-KR , "全体の直径（最大スペース）。"@ja-JP , "The overall diameter of a core (maximun space used)."@en , "ケーブルや母線の外形寸法（直径）を示す。"@ja-JP ;
        rdfs:label             "overallDiameter"@en , "全径"@ja-JP , "直径"@ja-JP , "전체 직경"@ko-KR , "직경"@ko-KR ;
        rdfs:range             <https://w3id.org/measurement/positiveLength> ;
        schema:domainIncludes  <https://w3id.org/product/CableSegment#CORESEGMENT> , <https://w3id.org/product/CableSegment#CABLESEGMENT> .

props:weight  a                owl:DatatypeProperty ;
        rdfs:comment           "케이블의 무게"@ko-KR , "ケーブルの重量。"@ja-JP , "코어 kg / km의 무게."@ko-KR , "Weight of core kg/km."@en , "コアkg/kmの重量。"@ja-JP , "Weight of cable kg/km."@en ;
        rdfs:label             "weight"@en , "무게"@ko-KR , "重量"@ja-JP ;
        rdfs:range             <https://w3id.org/measurement/mass> ;
        schema:domainIncludes  <https://w3id.org/product/CableSegment#CABLESEGMENT> , <https://w3id.org/product/CableSegment#CORESEGMENT> .

props:airSideSystemType
        rdfs:comment           "This enumeration specifies the basic types of possible air side systems (e.g., Constant Volume, Variable Volume, etc.)."@en ;
        rdfs:label             "airSideSystemType"@en ;
        schema:domainIncludes  bot:Zone .

props:flowPattern  rdfs:comment  "Flow pattern."@en , "流れ種類（単一直線、腹式直線、４方向、放射状、SWIRL、DISPLACEMENT、COMPACT他）"@ja-JP , "Forme du flux"@fr-FR ;
        rdfs:label             "flowPattern"@en , "流れ種類"@ja-JP , "FormeFlux"@fr-FR ;
        schema:domainIncludes  <https://w3id.org/product/AirTerminal> .

props:numberOfSlots  a         owl:DatatypeProperty ;
        rdfs:comment           "Number of slots."@en , "スロット数"@ja-JP , "Nombre de fentes"@fr-FR ;
        rdfs:label             "numberOfSlots"@en , "スロット数"@ja-JP , "NombreDeFentes"@fr-FR ;
        rdfs:range             xsd:int ;
        schema:domainIncludes  <https://w3id.org/product/AirTerminal> .

props:refreshRate  a           owl:DatatypeProperty ;
        rdfs:comment           "Indicates the display refresh frequency."@en , "リフレッシュレート周波数範囲を示す。"@ja-JP , "빈도 재생 빈도 주파수 범위를 나타낸다."@ko-KR ;
        rdfs:label             "refreshRate"@en , "リフレッシュレート"@ja-JP , "재생"@ko-KR ;
        rdfs:range             <https://w3id.org/measurement/frequency> ;
        schema:domainIncludes  <https://w3id.org/product/AudioVisualAppliance#DISPLAY> .

props:tiltHorizontal  rdfs:comment  "Indicates horizontal range for pivoting, where positive values indicate the camera rotating clockwise,"@en , "チルト水平の可動角度を示す。"@ja-JP ;
        rdfs:label             "tiltHorizontal"@en , "チルト水平方向可動角度"@ja-JP ;
        schema:domainIncludes  <https://w3id.org/product/AudioVisualAppliance#CAMERA> .

props:force  a                 owl:DatatypeProperty ;
        rdfs:comment           "Indicates the maximum close-off force for the actuator."@en , "アクチュエータの最大締め切り力を示す。"@ja-JP , "액츄에이터의 최대 마감 힘을 보여준다."@ko-KR ;
        rdfs:label             "force"@en , "最大推力"@ja-JP , "최대추력"@ko-KR ;
        rdfs:range             <https://w3id.org/measurement/force> ;
        schema:domainIncludes  <https://w3id.org/product/Actuator> .

props:maximumAirFlowRate
        a                      owl:DatatypeProperty ;
        rdfs:comment           "Maximum allowable air flow rate."@en ;
        rdfs:label             "maximumAirFlowRate"@en ;
        rdfs:range             <https://w3id.org/measurement/volumetricFlowRate> ;
        schema:domainIncludes  <https://w3id.org/product/Damper> .

props:sprinklerProtection
        a                      owl:DatatypeProperty ;
        rdfs:comment           "Indication selon laquelle ce bâtimentbénéficie d'une protection par sprinkler (VRAI) ou non (FAUX)"@fr-FR , "Indication whether this object is sprinkler protected (TRUE) or not (FALSE)."@en , "スプリンクラー設備の有無を示すブーリアン値。"@ja-JP , "스프링 클러 설비의 유무를 나타내는 값"@ko-KR , "Indication selon laquelle ce bâtiment bénéficie d'une protection par sprinkler (VRAI) ou non (FAUX)."@fr-FR , "Angabe, ob das Gebäude durch eine Sprinkleranlage geschützt wird (WAHR) oder nicht (FALSCH)."@de-DE , "Angabe, ob des Geschoss durch eine Sprinkleranlage geschützt wird (WAHR) oder nicht (FALSCH)."@de-DE ;
        rdfs:label             "Sprinklerschutz"@de-DE , "sprinklerProtection"@en , "スプリンクラー防御"@ja-JP , "스프링 클러 방어"@ko-KR , "ProtectionParSprinkler"@fr-FR ;
        rdfs:range             xsd:boolean ;
        schema:domainIncludes  <https://w3id.org/product/Building> , <https://w3id.org/product/BuildingStorey> .

props:ambientDesignDryBulbTemperature
        a                      owl:DatatypeProperty ;
        rdfs:comment           "Ambient design dry bulb temperature used for selecting the cooling tower."@en ;
        rdfs:label             "ambientDesignDryBulbTemperature"@en ;
        rdfs:range             <https://w3id.org/measurement/thermodynamicTemperature> ;
        schema:domainIncludes  <https://w3id.org/product/CoolingTower> .

props:rangeAngle  a            owl:DatatypeProperty ;
        rdfs:comment           "Indicates the maximum rotation the actuator must traverse."@en , "アクチュエータが動く最大回転角を示す。"@ja-JP , "액츄에이터가 움직이는 최대 회전각을 나타낸다."@ko-KR ;
        rdfs:label             "rangeAngle"@en , "最大回転角"@ja-JP , "최대 회전각"@ko-KR ;
        rdfs:range             <https://w3id.org/measurement/planeAngle> ;
        schema:domainIncludes  <https://w3id.org/product/Actuator> .

props:idealShaftPower
        a                      owl:DatatypeProperty ;
        rdfs:comment           "Compressor shaft power under ideal conditions."@en , "Puissance au niveau de l'arbre du compresseur sous conditions idéales."@fr-FR ;
        rdfs:label             "idealShaftPower"@en , "PuissanceArbreMaximale"@fr-FR ;
        rdfs:range             <https://w3id.org/measurement/power> ;
        schema:domainIncludes  <https://w3id.org/product/Compressor> .

props:powerState  a            owl:DatatypeProperty ;
        rdfs:comment           "Indicates the power state of the device where True is on and False is off."@en , "機器の電源オンオフの時間ごとの状態を示す。"@ja-JP ;
        rdfs:label             "powerState"@en , "電源状態"@ja-JP ;
        rdfs:range             <https://w3id.org/product/TimeSeries> ;
        rdfs:range             [ owl:allValuesFrom  xsd:boolean ;
                                 owl:onProperty     <https://w3id.org/measurement/seriesOf>
                               ] ;
        rdfs:range             [ owl:allValuesFrom  xsd:boolean ;
                                 owl:onProperty     <https://w3id.org/measurement/seriesOf>
                               ] ;
        schema:domainIncludes  <https://w3id.org/product/CommunicationsAppliance> , <https://w3id.org/product/AudioVisualAppliance> .

props:surfaceSpreadOfFlame
        a                      owl:DatatypeProperty ;
        rdfs:comment           "Indique comment les flammes se propagent sur une surface. Indication donnée selon le Code National du Bâtiment régissant le comportement au feu des matériaux."@fr-FR , "火炎表面伝播性。当該国の建築法規による。"@ja-JP , "炎がどのように材料の表面を広がるかという指標。材料の炎に対する振る舞いについての国家建築規則に従って提供される。"@ja-JP , "Indication on how the flames spread around the surface,\nIt is given according to the national building code that governs the fire behaviour for materials."@en , "German-description-5"@de-DE , "Beschreibung des Brandverhaltens des Bauteils gemäß der nationalen oder regionalen  Brandschutzverordnung."@de-DE ;
        rdfs:label             "surfaceSpreadOfFlame"@en , "Brandverhalten"@de-DE , "Propagation des flammes en surface"@fr-FR , "火炎表面伝播性"@ja-JP , "火炎伝播性"@ja-JP , "SurfacePropagationFlamme"@fr-FR ;
        rdfs:range             xsd:string ;
        schema:domainIncludes  <https://w3id.org/product/Covering> , <https://w3id.org/product/CurtainWall> .

props:buildingID  a            owl:DatatypeProperty ;
        rdfs:comment           "Gebäudekennzeichen dieses Gebäudes. Während der Baueingabe ist es das temporäre Kennzeichnen des Bauantrags."@de-DE , "건물에 부여되는 고유 식별자이다. 계획 요청시 사용되는 초기 임시 식별자이다. 이 임시 식별자는 건물이 정식으로 등록된 경우에 영구적인 식별자로 변경된다."@ko-KR , "Un identifiant unique attribué au bâtiment. Un identifiant temporaire est attribué au moment de la programmation. Il est ensuite remplacé par un identifiant permanent lorsque le bâtiment est enregistré dans une base de données de nature règlementaire."@fr-FR , "建物に付与されるユニークな識別子。計画要請の際に使用される初期の一時的な識別子。この一時的な識別子は、建物が正式に登録された際に恒久的な識別子へと変更される。"@ja-JP , "A unique identifier assigned to a building. A temporary identifier is initially assigned at the time of making a planning application. This temporary identifier is changed to a permanent identifier when the building is registered into a statutory buildings and properties database."@en ;
        rdfs:label             "buildingID"@en , "IdBatiment"@fr-FR , "建物記号"@ja-JP , "Gebäudekennzeichen"@de-DE , "건물 ID"@ko-KR ;
        rdfs:range             xsd:string ;
        schema:domainIncludes  <https://w3id.org/product/Building> .

props:distanceBetweenParallelCircuits
        a                      owl:DatatypeProperty ;
        rdfs:comment           "Distance measured between parallel circuits."@en ;
        rdfs:label             "distanceBetweenParallelCircuits"@en ;
        rdfs:range             <https://w3id.org/measurement/length> ;
        schema:domainIncludes  <https://w3id.org/product/CableSegment> .

props:panHorizontal  rdfs:comment  "Indicates horizontal range for panning."@en , "水平方向の可動範囲を示す。"@ja-JP ;
        rdfs:label             "panHorizontal"@en , "パン水平方向可動範囲"@ja-JP ;
        schema:domainIncludes  <https://w3id.org/product/AudioVisualAppliance#CAMERA> .

props:capacity  a              owl:DatatypeProperty ;
        rdfs:comment           "The product of the  ideal capacity and the overall volumetric efficiency of the compressor."@en , "Le produit de la puissance optimale par le rendement global du compresseur."@fr-FR , "Cooling tower capacity in terms of heat transfer rate of the cooling tower between air stream and water stream."@en ;
        rdfs:label             "Puissance"@fr-FR , "capacity"@en ;
        rdfs:range             <https://w3id.org/product/TimeSeries> ;
        rdfs:range             [ owl:allValuesFrom  <https://w3id.org/measurement/power> ;
                                 owl:onProperty     <https://w3id.org/measurement/seriesOf>
                               ] ;
        rdfs:range             [ owl:allValuesFrom  <https://w3id.org/measurement/power> ;
                                 owl:onProperty     <https://w3id.org/measurement/seriesOf>
                               ] ;
        schema:domainIncludes  <https://w3id.org/product/CoolingTower> , <https://w3id.org/product/Chiller> .

props:nominalHeatTransferCoefficient
        a                      owl:DatatypeProperty ;
        rdfs:comment           "Nominal overall heat transfer coefficient associated with nominal heat transfer area."@en ;
        rdfs:label             "nominalHeatTransferCoefficient"@en ;
        rdfs:range             <https://w3id.org/measurement/thermalTransmittance> ;
        schema:domainIncludes  <https://w3id.org/product/Condenser> .

props:neckAirVelocity
        a                      owl:DatatypeProperty ;
        rdfs:comment           "Vitesse de l'air au point le plus étroit"@fr-FR , "ネックの風速"@ja-JP , "Air velocity at the neck."@en ;
        rdfs:label             "ネック風速"@ja-JP , "Vitesse de l'air au point le plus étroit"@fr-FR , "neckAirVelocity"@en ;
        rdfs:range             <https://w3id.org/product/TimeSeries> ;
        rdfs:range             [ owl:allValuesFrom  <https://w3id.org/measurement/linearVelocity> ;
                                 owl:onProperty     <https://w3id.org/measurement/seriesOf>
                               ] ;
        schema:domainIncludes  <https://w3id.org/product/AirTerminal> .

props:energyGainTotal
        a                      owl:DatatypeProperty ;
        rdfs:comment           "The total amount of energy gains for the spaces served by the system during the peak cooling conditions, plus any system-level total energy gains."@en , "居室の最大冷房負荷と空調システム（機器等）の再熱負荷による最大熱負荷。"@ja-JP , "거실 최대 냉방 부하 및 공조 시스템 (장비 등) 재열 부하에 의한 최대 열부하."@ko-KR ;
        rdfs:label             "energyGainTotal"@en , "総熱取得"@ja-JP , "총 열 검색"@ko-KR ;
        rdfs:range             <https://w3id.org/measurement/power> ;
        schema:domainIncludes  bot:Zone .

props:closeOffRating  a        owl:DatatypeProperty ;
        rdfs:comment           "Close off rating."@en ;
        rdfs:label             "closeOffRating"@en ;
        rdfs:range             <https://w3id.org/measurement/pressure> ;
        schema:domainIncludes  <https://w3id.org/product/Damper> .

props:sumpHeaterPower
        a                      owl:DatatypeProperty ;
        rdfs:comment           "Electrical heat power of sump heater."@en ;
        rdfs:label             "sumpHeaterPower"@en ;
        rdfs:range             <https://w3id.org/product/TimeSeries> ;
        rdfs:range             [ owl:allValuesFrom  <https://w3id.org/measurement/power> ;
                                 owl:onProperty     <https://w3id.org/measurement/seriesOf>
                               ] ;
        schema:domainIncludes  <https://w3id.org/product/CoolingTower> .

props:refrigerantMaterial
        a                      owl:ObjectProperty ;
        rdfs:comment           "The refrigerant material used for heat transfer purposes."@en ;
        rdfs:label             "refrigerantMaterial"@en ;
        rdfs:range             <https://w3id.org/product/MaterialDefinition> ;
        schema:domainIncludes  <https://w3id.org/product/Condenser> .

props:waterPressureDropCurves
        a                      owl:DatatypeProperty ;
        rdfs:comment           "Water pressure drop as function of water flow rate."@en ;
        rdfs:label             "waterPressureDropCurves"@en ;
        rdfs:range             <https://w3id.org/product/TimeSeries> ;
        rdfs:range             [ owl:allValuesFrom  <https://w3id.org/measurement/pressure> ;
                                 owl:onProperty     <https://w3id.org/measurement/seriesOf>
                               ] ;
        schema:domainIncludes  <https://w3id.org/product/CooledBeam> .

props:shape  a                 owl:DatatypeProperty ;
        rdfs:comment           "Forme du terminal de ventilation. La fente est généralement un long et étroit appareil d'apport avec un rapport de forme généralement supérieur à 10 pour 1."@fr-FR , "空間の形状を定義します。少なくとも「四角形」、「円」、「未定義」の値を含みます。"@ja-JP , "Anforderung an die Form des Durchbruchs, vordefinierte Werte sind \"Rechteck\", \"Rund\", und \"Nicht definiert\"."@de-DE , "도체의 형상을 표시합니다."@ko-KR , "The shape form of the provision for void, the minimum set of agreed values includes 'Rectangle', 'Round', and 'Undefined'."@en , "空构件的形状，当前得到认可的值至少包括“矩形”、“圆形”及“未定义”。"@zh-CN , "La forme de la réservation. L'ensemble des valeurs autorisées contient au moins \"Rectangle\", \"Round\" et \"Undefined\"."@fr-FR , "Indication of the shape of the conductor."@en , "ターミナルの形状（円状、四角形、正方形、スロット他）。　スロット（溝状）は一般的にアスペクト比１０以上が典型的である。"@ja-JP , "導体の形状を表示。"@ja-JP , "Shape of the air terminal. Slot is typically a long narrow supply device with an aspect ratio generally greater than 10 to 1."@en ;
        rdfs:label             "Form"@de-DE , "형상"@ko-KR , "Forme"@fr-FR , "shape"@en , "形状"@zh-CN , "形状"@ja-JP ;
        rdfs:range             xsd:string ;
        schema:domainIncludes  <https://w3id.org/product/BuildingElementProxy#PROVISIONFORVOID> , <https://w3id.org/product/AirTerminal> , <https://w3id.org/product/CableSegment#CONDUCTORSEGMENT> .

props:airPressureDropCurves
        a                      owl:DatatypeProperty , owl:ObjectProperty ;
        rdfs:comment           "Air pressure drop as function of air flow rate."@en , "風量の関数としての空気圧力降下"@ja-JP , "Perte de charge aéraulique fonction du débit d'air"@fr-FR ;
        rdfs:label             "CourbesPerteChargeAir"@fr-FR , "空気圧力降下曲線"@ja-JP , "airPressureDropCurves"@en ;
        rdfs:range             <https://w3id.org/measurement/TimeSeries> , <https://w3id.org/product/TimeSeries> ;
        rdfs:range             [ owl:allValuesFrom  <https://w3id.org/measurement/pressure> ;
                                 owl:onProperty     <https://w3id.org/measurement/seriesOf>
                               ] ;
        schema:domainIncludes  <https://w3id.org/product/AirToAirHeatRecovery> , <https://w3id.org/product/CooledBeam#ACTIVE> .

props:returnWaterTemperatureHeating
        a                      owl:DatatypeProperty ;
        rdfs:comment           "Return water temperature in heating mode."@en ;
        rdfs:label             "returnWaterTemperatureHeating"@en ;
        rdfs:range             <https://w3id.org/product/TimeSeries> ;
        rdfs:range             [ owl:allValuesFrom  <https://w3id.org/measurement/thermodynamicTemperature> ;
                                 owl:onProperty     <https://w3id.org/measurement/seriesOf>
                               ] ;
        schema:domainIncludes  <https://w3id.org/product/CooledBeam> .

props:nominalAirFlowRate
        a                      owl:DatatypeProperty ;
        rdfs:comment           "Nominal airflow rate."@en , "Débit d'air nominal"@fr-FR , "設計風量範囲"@ja-JP , "Nominal air flow rate."@en ;
        rdfs:label             "nominalAirFlowRate"@en , "設計風量範囲"@ja-JP , "Débit d'air nominal"@fr-FR ;
        rdfs:range             <https://w3id.org/measurement/volumetricFlowRate> ;
        schema:domainIncludes  <https://w3id.org/product/AirTerminalBox> , <https://w3id.org/product/Damper> .

props:strengthClass  a         owl:DatatypeProperty ;
        rdfs:comment           "Classification of the concrete strength in accordance with the concrete design code which is applied in the project."@en , "Klassifikation der Betonfestigkeit gemäß der aktuellen, im Projekt angewandten, Norm."@de-DE ;
        rdfs:label             "strengthClass"@en , "Betonfestigkeitsklasse"@de-DE ;
        rdfs:range             xsd:string ;
        schema:domainIncludes  <https://w3id.org/product/BuildingElement> .

props:correctionFactorForHeating
        a                      owl:DatatypeProperty ;
        rdfs:comment           "Correction factor k as a function of water flow rate (used to calculate heating capacity)."@en ;
        rdfs:label             "correctionFactorForHeating"@en ;
        rdfs:range             <https://w3id.org/product/TimeSeries> ;
        rdfs:range             [ owl:allValuesFrom  xsd:decimal ;
                                 owl:onProperty     <https://w3id.org/measurement/seriesOf>
                               ] ;
        schema:domainIncludes  <https://w3id.org/product/CooledBeam> .

props:loadSafetyFactor
        a                      owl:DatatypeProperty ;
        rdfs:comment           "Load safety factor."@en , "空調負荷計算用の安全率（割増係数）。"@ja-JP , "공조 부하 계산을위한 안전율 (할증 계수)"@ko-KR ;
        rdfs:label             "loadSafetyFactor"@en , "負荷の安全率"@ja-JP , "부하의 안전율"@ko-KR ;
        rdfs:range             <https://w3id.org/measurement/positiveRatio> ;
        schema:domainIncludes  bot:Zone .

props:frameMaterial  a         owl:ObjectProperty ;
        rdfs:comment           "The material from which the damper frame is constructed."@en ;
        rdfs:label             "frameMaterial"@en ;
        rdfs:range             <https://w3id.org/product/MaterialDefinition> ;
        schema:domainIncludes  <https://w3id.org/product/Damper> .

props:signalTimeIncrease
        a                      owl:DatatypeProperty ;
        rdfs:comment           "Time factor used for exponential increase."@en , "적분 시간 (Ti)"@ko-KR ;
        rdfs:label             "signalTimeIncrease"@en , "적분 시간 (Ti)"@ko-KR ;
        rdfs:range             <https://w3id.org/measurement/time> ;
        schema:domainIncludes  <https://w3id.org/product/Controller#PROPORTIONAL> .

props:controlType  a           owl:DatatypeProperty ;
        rdfs:comment           "The type of signal modification.\nPROPORTIONAL: Output is proportional to the control error. The gain of a proportional control (Kp) will have the effect of reducing the rise time and reducing , but never eliminating, the steady-state error of the variable controlled. \nPROPORTIONALINTEGRAL: Part of the output is proportional to the control error and part is proportional to the time integral of the control error. Adding the gain of an integral control (Ki) will have the effect of eliminating the steady-state error of the variable controlled, but it may make the transient response worse. \nPROPORTIONALINTEGRALDERIVATIVE: Part of the output is proportional to the control error, part is proportional to the time integral of the control error and part is proportional to the time derivative of the control error. Adding the gain of a derivative control (Kd) will have the effect of increasing the stability of the system, reducing the overshoot, and improving the transient response of the variable controlled."@en , "신호 변경 유형   P (비례), I (적분), D (미분)의 조합 PROPORTIONAL :   P (비례) 제어 PROPORTIONALINTEGRAL :   PI (비례 적분) 제어 PROPORTIONALINTEGRALDERIVATIVE :   PID (비례 적분 미분) 제어"@ko-KR , "The type of signal modification effected and applicable ports:\n\nINPUT: Controller element is a dedicated input.\nOUTPUT: Controller element is a dedicated output.\nVARIABLE: Controller element is an in-memory variable."@en , "The type of discrete digital controller: \n\nPRIMARY: Controller has built-in communication interface for PC connection, may manage secondary controllers.\nSECONDARY: Controller communicates with primary controller and its own managed devices."@en , "컨트롤러는 항상 하나의 출력 포트와 가변 입력 포트 유형에 따라있는 한결 : output = SignalOffset 수정자 : output = input * SignalFactor + SignalOffset 절대치 : output = | input | 역수 : output = 1.0 / input 지연 : output = 지연 (input, SignalTime 후) 이동 평균 : output = 평균 (inputN, SignalTime 사이) 미분 : output = 미분 (inputN, SignalTime 사이) 적분 : output = 적분 (inputN, SignalTime 사이) 바이너리 : output = SignalOffset ※ input = TRUE의 경우 누적 : output = accumulator       ※ accumulator = 펄스 카운트 * SignalOffset       ※ if (accumulator> SignalFactor) accumulator - = SignalFactor       ??? 펄스 카운터 : output = input * SignalMultiplier       ※ input 펄스 카운트, SignalMultiplier은 원인 불명       ??? 총 : output = input1 + input2 뺄셈 : output = input1 - input2 적립 : output = input1 * input2 나누기 : output = input1 / input2 평균 : output = (input1 + input2) / 2 최대 : output = input1 or input2 ※보다 큰 최소 : output = input1 or input2 ※보다 작은"@ko-KR , "The type of signal modification effected and applicable ports:\n\nLOWERLIMITSWITCH: Single analog input is read and if less than Value.LowerBound then True is written to the output value.\nUPPERLIMITSWITCH: Single analog input is read and if more than Value.UpperBound then True is written to the output value.\nLOWERBANDSWITCH: Single analog input is read and if less than Value.LowerBound+BandWidth then True is written to the output value.\nUPPERBANDSWITCH: Single analog input is read and if more than Value.UpperBound-BandWidth then True is written to the output value.\nNOT: Single binary input is read and the opposite value is written to the output value.\nAND: Two binary inputs are read and if both are True then True is written to the output value.\nOR: Two binary inputs are read and if either is True then True is written to the output value.\nXOR: Two binary inputs are read and if one is true then True is written to the output value.\nCALENDAR: No inputs; the current time is compared with an IfcWorkCalendar to which the IfcController is assigned and True is written if active.\nINPUT: Controller element is a dedicated input.\nOUTPUT: Controller element is a dedicated output.\nVARIABLE: Controller element is an in-memory variable."@en , "The type of control used to operate the damper (e.g., Open/Closed Indicator, Resetable Temperature Sensor, Temperature Override, etc.) ."@en , "신호 변경 유형 리미트 스위치가 범위를 Pset_ControllerTypeValue 값을 묶여 속성에 의해 결정 하한 : if (Value.LowerBound> Input) output = TRUE 상한 : if (Value.UpperBound <Input) output = TRUE 하한 + 불감대 : if (Value.LowerBound + BandWidth> Input) output = TRUE 최대 - 불감대 : if (Value.UpperBound - BandWidth <Input) output = TRUE 논리 부정 : output = NOT (input) 논리적 : output = AND (input1, input2) 논리합 : output = OR (input, input2) 배타적 논리합 : output = XOR (input, input2) 달력 : output = TRUE ※ 컨트롤러에 입력없이하고 IfcWorkCalendar 컨트롤러가 할당되어 현재 시간인 경우"@ko-KR , "The type of control used to operate the damper (e.g., Open/Closed Indicator, Resetable Temperature Sensor, Temperature Override, etc.)."@en , "The type of signal modification effected and applicable ports: \n\nCONSTANT: No inputs; SignalOffset is written to the output value.\nMODIFIER: Single analog input is read, added to SignalOffset, multiplied by SignalFactor, and written to the output value.\nABSOLUTE: Single analog input is read and absolute value is written to the output value.\nINVERSE: Single analog input is read, 1.0 is divided by the input value and written to the output value.\nHYSTERISIS: Single analog input is read, delayed according to SignalTime, and written to the output value.\nRUNNINGAVERAGE: Single analog input is read, averaged over SignalTime, and written to the output value.\nDERIVATIVE: Single analog input is read and the rate of change during the SignalTime is written to the output value.\nINTEGRAL: Single analog input is read and the average value during the SignalTime is written to the output value.\nBINARY: Single binary input is read and SignalOffset is written to the output value if True.\nACCUMULATOR: Single binary input is read, and for each pulse the SignalOffset is added to the accumulator, and while the accumulator is greater than the SignalFactor, the accumulator is decremented by SignalFactor and the integer result is incremented by one.\nPULSECONVERTER: Single integer input is read, and for each increment the SignalMultiplier is added and written to the output value.\nSUM: Two analog inputs are read, added, and written to the output value.\nSUBTRACT: Two analog inputs are read, subtracted, and written to the output value.\nPRODUCT: Two analog inputs are read, multiplied, and written to the output value.\nDIVIDE: Two analog inputs are read, divided, and written to the output value.\nAVERAGE: Two analog inputs are read and the average is written to the output value.\nMAXIMUM: Two analog inputs are read and the maximum is written to the output value.\nMINIMUM: Two analog inputs are read and the minimum is written to the output value..\nINPUT: Controller element is a dedicated input.\nOUTPUT: Controller element is a dedicated output.\nVARIABLE: Controller element is an in-memory variable."@en ;
        rdfs:label             "controlType"@en , "PROPORTIONAL 유형"@ko-KR , "FLOATING 유형"@ko-KR , "TWOPOSITION 유형"@ko-KR ;
        rdfs:range             xsd:string ;
        schema:domainIncludes  <https://w3id.org/product/Controller#TWOPOSITION> , <https://w3id.org/product/Damper#FIRESMOKEDAMPER> , <https://w3id.org/product/Controller#MULTIPOSITION> , <https://w3id.org/product/Damper#SMOKEDAMPER> , <https://w3id.org/product/Controller#PROGRAMMABLE> , <https://w3id.org/product/Controller#FLOATING> , <https://w3id.org/product/Controller#PROPORTIONAL> .

props:fluidPressureRange
        rdfs:comment           "Allowable water working pressure range inside the tube."@en , "Plage de pression hydraulique fonctionnelle admissible dans le tube."@fr-FR ;
        rdfs:label             "fluidPressureRange"@en , "PlagePressionFluide"@fr-FR ;
        schema:domainIncludes  <https://w3id.org/product/Coil> .

props:heatOutput  rdfs:comment  "Total nominal heat output as listed by the Boiler manufacturer. For water boilers, it is a function of inlet versus outlet temperature. For steam boilers, it is a function of inlet temperature versus steam pressure.  Note: as two variables are used, DefiningValues and DefinedValues are null, and values are stored in IfcTable in the following order: InletTemperature(IfcThermodynamicTemperatureMeasure), OutletTemperature(IfcThermodynamicTemperatureMeasure), HeatOutput(IfcEnergyMeasure).  The IfcTable is related to IfcPropertyTableValue using IfcMetric and IfcPropertyConstraintRelationship."@en , "Rendement total nominal tel que défini par le constructeur de chaudière.\nPour les chaudières à eau chaude, une fonction de la température en entrée par rapport à la température de sortie.\nRemarque: Comme deux variables sont utilisées ValeurDefinir et ValeursDefinies sont nulles, et les valeurs sont enregistrées dans IfcTable dans l'ordre suivant:\n- TempératureEntrée (IfcThermodynamicTemperatureMeasure) et TempératureSortie (IfcThermodynamicTemperatureMeasure) dans ValeursDefinir , et Rendement de chaleur (IfcEnergyMeasure) dansValeursDefinies.\nIfcPropertyTable est lié à IfcMetric qui utilise IfcMetric et IfcPropertyConstraintRelationship."@fr-FR , "Total nominal heat output as listed by the Boiler manufacturer. For steam boilers, it is a function of inlet temperature versus steam pressure.  Note: as two variables are used, DefiningValues and DefinedValues are null, and values are stored in IfcTable in the following order: InletTemperature(IfcThermodynamicTemperatureMeasure) and OutletTemperature(IfcThermodynamicTemperatureMeasure) in DefiningValues, and HeatOutput(IfcEnergyMeasure) in DefinedValues. For example, DefiningValues(InletTemp, OutletTemp), DefinedValues(null, HeatOutput). The IfcTable is related to IfcPropertyTableValue using IfcMetric and IfcPropertyConstraintRelationship."@en , "Rendement total nominal tel que défini par le constructeur de chaudière.\nPour les chaudières à vapeur, une fonction de la température en entrée par rapport à la pression de vapeur.\nRemarque: Comme deux variables sont utilisées ValeurDefinir et ValeursDefinies sont nulles, et les valeurs sont enregistrées dans IfcTable dans l'ordre suivant:\n- TempératureEntrée (IfcThermodynamicTemperatureMeasure) et TempératureSortie (IfcThermodynamicTemperatureMeasure) dans ValeursDefinir , et Rendement de chaleur (IfcEnergyMeasure) dansValeursDefinies.\nPar exemple, ValeursDefinir (TempératureEntrée, TempératureSortie), ValeursDefinies (nul, RendementChaleur).\nIfcPropertyTable est lié à IfcMetric qui utilise IfcMetric et IfcPropertyConstraintRelationship."@fr-FR ;
        rdfs:label             "heatOutput"@en , "RendementChaleur"@fr-FR ;
        schema:domainIncludes  <https://w3id.org/product/Boiler#WATER> , <https://w3id.org/product/Boiler#STEAM> .

props:nominalDamperDiameter
        a                      owl:DatatypeProperty ;
        rdfs:comment           "Nominal damper diameter."@en , "ダンパ直径の設計値"@ja-JP , "Diamètre nominal clapet"@fr-FR ;
        rdfs:label             "nominalDamperDiameter"@en , "設計ダンパ直径"@ja-JP , "Diamètre nominal clapet"@fr-FR ;
        rdfs:range             <https://w3id.org/measurement/positiveLength> ;
        schema:domainIncludes  <https://w3id.org/product/AirTerminalBox> .

props:speakerType  rdfs:comment  "Indicates the type of speaker."@en , "スピーカーのタイプを示す。"@ja-JP , "스피커의 타입을 나타낸다."@ko-KR ;
        rdfs:label             "speakerType"@en , "スピーカータイプ"@ja-JP , "스피커 타입"@ko-KR ;
        schema:domainIncludes  <https://w3id.org/product/AudioVisualAppliance#SPEAKER> .

props:structuralClass
        a                      owl:DatatypeProperty ;
        rdfs:comment           "The structural class defined for the concrete structure (e.g. '1')."@en , "構造クラスはコンクリート構造を定義した。（例えば「１」）"@ja-JP , "구조 클래스는 콘크리트 구조를 정의했다 (예를 들어 \"1\")"@ko-KR ;
        rdfs:label             "structuralClass"@en , "構造クラス"@ja-JP , "구조 클래스"@ko-KR ;
        rdfs:range             xsd:string ;
        schema:domainIncludes  <https://w3id.org/product/BuildingElement> .

props:temperatureEffectiveness
        a                      owl:DatatypeProperty ;
        rdfs:comment           "Efficacité thermique sensible: rapport entre la différence de températures pour le flux primaire sur la différence maximale d'échange possible."@fr-FR , "温度熱交換効率：\n最大可能温度変化に対する一次側温度変化の比"@ja-JP , "Temperature heat transfer effectiveness: The ratio of primary airflow temperature changes to maximum possible temperature changes."@en ;
        rdfs:label             "温度効率"@ja-JP , "EfficacitéTempérature"@fr-FR , "temperatureEffectiveness"@en ;
        rdfs:range             <https://w3id.org/product/TimeSeries> ;
        rdfs:range             [ owl:allValuesFrom  <https://w3id.org/measurement/normalisedRatio> ;
                                 owl:onProperty     <https://w3id.org/measurement/seriesOf>
                               ] ;
        schema:domainIncludes  <https://w3id.org/product/AirToAirHeatRecovery> .

props:exposureClass  a         owl:DatatypeProperty ;
        rdfs:comment           "Classification of exposure to environmental conditions, usually specified in accordance with the concrete design code which is applied in the project."@en , "Klassifikation der Widerstandsfähigkeit gegenüber chemischen und physikalischen Einwirkungen gemäß der aktuellen, im Projekt angewandten, Norm."@de-DE ;
        rdfs:label             "exposureClass"@en , "Expositionsklasse"@de-DE ;
        rdfs:range             xsd:string ;
        schema:domainIncludes  <https://w3id.org/product/BuildingElement> .

props:primaryEnergyConsumption
        a                      owl:DatatypeProperty ;
        rdfs:comment           "Boiler primary energy source consumption (i.e., the fuel consumed for changing the thermodynamic state of the fluid)."@en , "Consommation d'énergie primaire de la chaudière(c'est-à-dire le combustible consommé pour le changement d'état thermodynamique du fluide)."@fr-FR , "ボイラ一次エネルギ消費量（つまり流体の熱力学状態変更のために消費された燃料）"@ja-JP ;
        rdfs:label             "一次エネルギ消費量"@ja-JP , "primaryEnergyConsumption"@en , "ConsommationEnergiePrimaire"@fr-FR ;
        rdfs:range             <https://w3id.org/product/TimeSeries> ;
        rdfs:range             [ owl:allValuesFrom  <https://w3id.org/measurement/power> ;
                                 owl:onProperty     <https://w3id.org/measurement/seriesOf>
                               ] ;
        schema:domainIncludes  <https://w3id.org/product/Boiler> .

props:operationalTemperatureRange
        rdfs:comment           "Allowable operation ambient air temperature range."@en , "Opération admise sur la plage de température de l'air ambiant"@fr-FR , "動作を許容する周囲温度の範囲"@ja-JP , "Allowable operational air temperature range."@en , "Plage de température fonctionnelle admissible."@fr-FR ;
        rdfs:label             "動作温度範囲"@ja-JP , "operationalTemperatureRange"@en , "PlageTemperatureFonctionnelle"@fr-FR , "PlageTempératureOpérationelle"@fr-FR ;
        schema:domainIncludes  <https://w3id.org/product/AirToAirHeatRecovery> , <https://w3id.org/product/Coil> .

props:airflowSensible
        a                      owl:DatatypeProperty ;
        rdfs:comment           "The air flowrate required to satisfy the sensible peak loads."@en , "最大潜熱負荷に対応する給気量。"@ja-JP , "최대 잠열 부하에 대한 급기 량"@ko-KR ;
        rdfs:label             "airflowSensible"@en , "顕熱空調給気量"@ja-JP , "현열 공조 급기 량"@ko-KR ;
        rdfs:range             <https://w3id.org/measurement/volumetricFlowRate> ;
        schema:domainIncludes  bot:Zone .

props:load  a                  owl:DatatypeProperty ;
        rdfs:comment           "Charge effective de la chaudière."@fr-FR , "ボイラ実負荷"@ja-JP , "Boiler real load."@en ;
        rdfs:label             "Charge"@fr-FR , "負荷"@ja-JP , "load"@en ;
        rdfs:range             <https://w3id.org/product/TimeSeries> ;
        rdfs:range             [ owl:allValuesFrom  <https://w3id.org/measurement/power> ;
                                 owl:onProperty     <https://w3id.org/measurement/seriesOf>
                               ] ;
        schema:domainIncludes  <https://w3id.org/product/Boiler> .

props:torqueRange  rdfs:comment  "Torque range: minimum operational torque to maximum allowable torque."@en ;
        rdfs:label             "torqueRange"@en ;
        schema:domainIncludes  <https://w3id.org/product/Damper#CONTROLDAMPER> .

props:slotLength  a            owl:DatatypeProperty ;
        rdfs:comment           "Slot length."@en , "スロット長"@ja-JP , "Longueur de la fente"@fr-FR ;
        rdfs:label             "slotLength"@en , "スロット長"@ja-JP , "ElongueurFente"@fr-FR ;
        rdfs:range             <https://w3id.org/measurement/positiveLength> ;
        schema:domainIncludes  <https://w3id.org/product/AirTerminal> .

props:rentalRatesInCategoryNow
        rdfs:comment           "Range of the cost rates for property currently available in the required category."@en , "Prix actuel des loyers pour la catégorie considérée."@fr-FR ;
        rdfs:label             "rentalRatesInCategoryNow"@en , "PrixActuelLoyerParCategorie"@fr-FR ;
        schema:domainIncludes  <https://w3id.org/product/Building> .

props:hasSoundAttenuator
        a                      owl:DatatypeProperty ;
        rdfs:comment           "Terminal box has a sound attenuator."@en , "ターミナルに消音があるか否か　（あればTRUE)"@ja-JP , "If TRUE, the air terminal has sound attenuation."@en , "Si VRAI, le terminal de ventilation possède une correction acoustique."@fr-FR , "Le registre terminal possède une correction acoustique"@fr-FR , "ターミナルに消音が付いている場合に真"@ja-JP ;
        rdfs:label             "hasSoundAttenuator"@en , "消音有無"@ja-JP , "Possède correction acoustique"@fr-FR , "PossèdeCorrectionAcoustique"@fr-FR ;
        rdfs:range             xsd:boolean ;
        schema:domainIncludes  <https://w3id.org/product/AirTerminalBox> , <https://w3id.org/product/AirTerminal> .

props:inputFlowrate  a         owl:DatatypeProperty ;
        rdfs:comment           "Maximum hydraulic flowrate requirement."@en , "최대 제어 공기 유량"@ko-KR , "最大流量。"@ja-JP , "最大制御空気流量。"@ja-JP , "Maximum input control air flowrate requirement."@en , "최대 유량"@ko-KR ;
        rdfs:label             "入力流量"@ja-JP , "입력 유량"@ko-KR , "inputFlowrate"@en ;
        rdfs:range             <https://w3id.org/measurement/volumetricFlowRate> ;
        schema:domainIncludes  <https://w3id.org/product/Actuator#PNEUMATICACTUATOR> , <https://w3id.org/product/Actuator#HYDRAULICACTUATOR> .

props:actuatorInputPower
        a                      owl:DatatypeProperty ;
        rdfs:comment           "Maximum input power requirement."@en , "最大入力電力。"@ja-JP , "최대 입력 전력"@ko-KR ;
        rdfs:label             "actuatorInputPower"@en , "入力電力"@ja-JP , "입력 전력"@ko-KR ;
        rdfs:range             <https://w3id.org/measurement/power> ;
        schema:domainIncludes  <https://w3id.org/product/Actuator#ELECTRICACTUATOR> .

props:uACurve  a               owl:ObjectProperty ;
        rdfs:comment           "UA value as a  function of fan speed at certain water flow rate, UA = f ( fan speed)."@en ;
        rdfs:label             "uACurve"@en ;
        rdfs:range             <https://w3id.org/measurement/TimeSeries> ;
        schema:domainIncludes  <https://w3id.org/product/CoolingTower> .

props:yearOfConstruction
        a                      owl:DatatypeProperty ;
        rdfs:comment           "Year of construction of this building, including expected year of completion."@en , "Année de construction de ce bâtiment, incluant l'année de parfait achèvement."@fr-FR , "시공 년. 준공 예정 년 포함한다."@ko-KR , "Jahr der Errichtung des Gebäudes, einschließliich des Jahres der geplanten Fertigstellung."@de-DE , "施工の年。竣工の予想年も含む。"@ja-JP ;
        rdfs:label             "시공 년"@ko-KR , "施工年"@ja-JP , "AnneeConstruction"@fr-FR , "yearOfConstruction"@en , "Baujahr"@de-DE ;
        rdfs:range             xsd:string ;
        schema:domainIncludes  <https://w3id.org/product/Building> .

props:coreIdentifier  a        owl:DatatypeProperty ;
        rdfs:comment           "The core identification used  Identifiers may be used such as by color (Black, Brown, Grey) or by number (1, 2, 3) or by IEC phase reference (L1, L2, L3) etc."@en , "コアの識別は、色（ブラック、ブラウン、グレー）又は番号（1、2、3）又はIECの位相基準（L1、L2、L3）などを使用。"@ja-JP , "코어 식별 색 (블랙, 브라운, 그레이) 또는 번호 (1,2,3) 또는 IEC의 위상 기준 (L1, L2, L3)를 사용."@ko-KR ;
        rdfs:label             "coreIdentifier"@en , "コア識別子"@ja-JP , "코어 식별자"@ko-KR ;
        rdfs:range             xsd:string ;
        schema:domainIncludes  <https://w3id.org/product/CableSegment#CORESEGMENT> .

props:tunerChannel  rdfs:comment  "Indicates the tuner channels, if applicable."@en , "設定可能なチャンネルを示す。"@ja-JP , "가능한 채널을 보여준다."@ko-KR ;
        rdfs:label             "tunerChannel"@en , "チューナーチャンネル"@ja-JP , "튜너 채널 선택"@ko-KR ;
        schema:domainIncludes  <https://w3id.org/product/AudioVisualAppliance#TUNER> .

props:roadVisibleDistanceRight
        a                      owl:DatatypeProperty ;
        rdfs:comment           "Distance visible to the right of the access."@en , "Distance de visibilité à la droite de l'accès."@fr-FR , "右側の経路に可視出来る距離。"@ja-JP ;
        rdfs:label             "roadVisibleDistanceRight"@en , "DistanceVisibiliteCoteDroit"@fr-FR , "右側道路可視距離"@ja-JP ;
        rdfs:range             <https://w3id.org/measurement/positiveLength> ;
        schema:domainIncludes  <https://w3id.org/product/Annotation#LineOfSight> .

props:hasAntiStaticSurface
        a                      owl:DatatypeProperty ;
        rdfs:comment           "Indique si la finition est conçue pour être anti statique (VRAI) ou non (FAUX)."@fr-FR , "Indication whether the surface finish is designed to prevent electrostatic charge (TRUE) or not (FALSE)."@en , "表示表面处理是否设计为防静电的。"@zh-CN , "Angabe, ob der Bodenbelag eine antistatische Oberfläche hat (JA), oder nicht (NEIN)."@de-DE ;
        rdfs:label             "表面是否防静电"@zh-CN , "Antistatische Oberfläche"@de-DE , "Anti statique"@fr-FR , "hasAntiStaticSurface"@en ;
        rdfs:range             xsd:boolean ;
        schema:domainIncludes  <https://w3id.org/product/Covering#FLOORING> .

props:numberOfCompartments
        a                      owl:DatatypeProperty ;
        rdfs:comment           "The number of separate internal compartments within the trunking."@en , "管の区別される内部区画の個数。"@ja-JP , "관 구분되는 내부 파티션 개수"@ko-KR ;
        rdfs:label             "numberOfCompartments"@en , "区画数"@ja-JP , "구획 수"@ko-KR ;
        rdfs:range             xsd:int ;
        schema:domainIncludes  <https://w3id.org/product/CableCarrierSegment#CABLETRUNKINGSEGMENT> .

props:scheduleCost  a          owl:DatatypeProperty ;
        rdfs:comment           "The budgeted cost on behalf of the resource allocation."@en , "資源配分のための予定されているコスト。"@ja-JP ;
        rdfs:label             "scheduleCost"@en , "予定コスト"@ja-JP ;
        rdfs:range             <https://w3id.org/product/TimeSeries> ;
        rdfs:range             [ owl:allValuesFrom  <https://w3id.org/measurement/monetary> ;
                                 owl:onProperty     <https://w3id.org/measurement/seriesOf>
                               ] ;
        schema:domainIncludes  <https://w3id.org/product/ConstructionResource> .

props:waterFoulingResistance
        a                      owl:DatatypeProperty ;
        rdfs:comment           "Fouling resistance on water/air side."@en ;
        rdfs:label             "waterFoulingResistance"@en ;
        rdfs:range             <https://w3id.org/product/TimeSeries> ;
        rdfs:range             [ owl:allValuesFrom  <https://w3id.org/measurement/thermalResistance> ;
                                 owl:onProperty     <https://w3id.org/measurement/seriesOf>
                               ] ;
        schema:domainIncludes  <https://w3id.org/product/Condenser> .

props:dimensionalAccuracyClass
        a                      owl:DatatypeProperty ;
        rdfs:comment           "Classification designation of the dimensional accuracy requirement according to local standards."@en , "国の基準が求める寸法精度の分類指定。"@ja-JP , "국가 표준이 요구하는 치수 정밀도의 분류 지정"@ko-KR ;
        rdfs:label             "dimensionalAccuracyClass"@en , "寸法精度クラス"@ja-JP , "치수 정밀도 클래스"@ko-KR ;
        rdfs:range             xsd:string ;
        schema:domainIncludes  <https://w3id.org/product/BuildingElement> .

props:sensibleEffectiveness
        a                      owl:DatatypeProperty ;
        rdfs:comment           "顕熱効率\n効率は、最大可能熱交換に対する熱交換の比率で定義される"@ja-JP , "Sensible heat transfer effectiveness, where effectiveness is defined as the ratio of heat transfer to maximum possible heat transfer."@en , "Efficacité d'échange de chaleur sensible, où l'efficacité est définie par le rapport entre l'échange de chaleur effectif et l'échange maximum possible."@fr-FR ;
        rdfs:label             "EfficacitéSensible"@fr-FR , "顕熱効率"@ja-JP , "sensibleEffectiveness"@en ;
        rdfs:range             <https://w3id.org/product/TimeSeries> ;
        rdfs:range             [ owl:allValuesFrom  <https://w3id.org/measurement/normalisedRatio> ;
                                 owl:onProperty     <https://w3id.org/measurement/seriesOf>
                               ] ;
        schema:domainIncludes  <https://w3id.org/product/AirToAirHeatRecovery> .

props:waterPressureDropCurve
        rdfs:comment           "Water pressure drop curve, pressure drop – flow rate curve, WaterPressureDrop = f(WaterflowRate)."@en , "Courbe de perte de charge hydraulique, courbe perte de charge - débit, perte de charge = f(DébitHydraulique)."@fr-FR ;
        rdfs:label             "waterPressureDropCurve"@en , "CourbePerteChargeHydraulique"@fr-FR ;
        schema:domainIncludes  <https://w3id.org/product/Coil> .

props:isHorizontalCable
        a                      owl:DatatypeProperty ;
        rdfs:comment           "Indication of whether the cable occurrences are mounted horizontally (= TRUE) or vertically (= FALSE)."@en ;
        rdfs:label             "isHorizontalCable"@en ;
        rdfs:range             xsd:boolean ;
        schema:domainIncludes  <https://w3id.org/product/CableSegment> .

props:pressureDrop  a          owl:DatatypeProperty ;
        rdfs:comment           "Pressure drop."@en , "Drop in total pressure between inlet and outlet at nominal air-flow rate."@en , "設定風量での入口/出口間の全圧降下"@ja-JP , "Chute de pression totale entre l'entrée et la sortie en débit d'air nominal"@fr-FR ;
        rdfs:label             "圧力降下"@ja-JP , "Chute de pression"@fr-FR , "pressureDrop"@en ;
        rdfs:range             <https://w3id.org/product/TimeSeries> ;
        rdfs:range             [ owl:allValuesFrom  <https://w3id.org/measurement/pressure> ;
                                 owl:onProperty     <https://w3id.org/measurement/seriesOf>
                               ] ;
        rdfs:range             [ owl:allValuesFrom  <https://w3id.org/measurement/pressure> ;
                                 owl:onProperty     <https://w3id.org/measurement/seriesOf>
                               ] ;
        schema:domainIncludes  <https://w3id.org/product/AirTerminal> , <https://w3id.org/product/Damper> .

props:energyGainSensible
        a                      owl:DatatypeProperty ;
        rdfs:comment           "The sum of total energy gains for the spaces served by the system during the peak cooling conditions, plus any system-level sensible energy gains."@en , "ピーク時各居室の最大冷房負荷と空調システムの顕熱負荷による最大顕熱負荷。"@ja-JP , "최대 각 거실 최대 냉방 부하 및 공조 시스템의 현열 부하에 의한 최대 현열 부하"@ko-KR ;
        rdfs:label             "energyGainSensible"@en , "顕熱空調負荷"@ja-JP , "현열 공조 부하"@ko-KR ;
        rdfs:range             <https://w3id.org/measurement/power> ;
        schema:domainIncludes  bot:Zone .

props:hasThermalInsulation
        a                      owl:DatatypeProperty ;
        rdfs:comment           "If TRUE, the air terminal has thermal insulation."@en , "ターミナルに断熱がある場合に真"@ja-JP , "Si VRAI, le terminal de ventilation possède une isolation thermique."@fr-FR ;
        rdfs:label             "hasThermalInsulation"@en , "断熱有無"@ja-JP , "PossèdeIsolationThermique"@fr-FR ;
        rdfs:range             xsd:boolean ;
        schema:domainIncludes  <https://w3id.org/product/AirTerminal> .

props:accuracyQualityExpected
        a                      owl:DatatypeProperty ;
        rdfs:comment           "A measure of the accuracy quality of survey points as expected expressed in percentage terms."@en , "Mesure de la précision attendue des points de relevé, exprimée en pourcentage."@fr-FR ;
        rdfs:label             "accuracyQualityExpected"@en , "PrecisionAttendue"@fr-FR ;
        rdfs:range             <https://w3id.org/measurement/ratio> ;
        schema:domainIncludes  <https://w3id.org/product/Annotation#SurveyArea> .

props:controlStrategy
        rdfs:comment           "FixedExitingWaterTemp: The capacity is controlled to maintain a fixed exiting water temperature.\nWetBulbTempReset: The set-point is reset based on the wet-bulb temperature."@en ;
        rdfs:label             "controlStrategy"@en ;
        schema:domainIncludes  <https://w3id.org/product/CoolingTower> .

props:firmwareVersion
        a                      owl:DatatypeProperty ;
        rdfs:comment           "Indicates version of device firmware according to device manufacturer."@en , "컨트롤러 펌웨어 버전"@ko-KR ;
        rdfs:label             "firmwareVersion"@en , "펌웨어 버전"@ko-KR ;
        rdfs:range             xsd:string ;
        schema:domainIncludes  <https://w3id.org/product/Controller#PROGRAMMABLE> .

props:idealCapacity  a         owl:DatatypeProperty ;
        rdfs:comment           "Compressor capacity under ideal conditions."@en , "Puissance maximale sous des conditions idéales"@fr-FR ;
        rdfs:label             "idealCapacity"@en , "PuissanceMaximale"@fr-FR ;
        rdfs:range             <https://w3id.org/measurement/power> ;
        schema:domainIncludes  <https://w3id.org/product/Compressor> .

props:heatTransferTypeEnum
        rdfs:comment           "Type of heat transfer between the two air streams."@en , "空気間の熱交換の種類（顕熱、潜熱…）"@ja-JP , "Type de transfert de chaleur entre deux flux d'air."@fr-FR ;
        rdfs:label             "heatTransferTypeEnum"@en , "熱交換種類"@ja-JP , "TypeEchangeChaleurEnum"@fr-FR ;
        schema:domainIncludes  <https://w3id.org/product/AirToAirHeatRecovery> .

props:sizingMethod  rdfs:comment  "Identifies whether the damper is sized nominally or with exact measurements:\n\nNOMINAL: Nominal sizing method. \nEXACT: Exact sizing method."@en ;
        rdfs:label             "sizingMethod"@en ;
        schema:domainIncludes  <https://w3id.org/product/Damper> .

props:waterFlowControlSystemType
        rdfs:comment           "Factory fitted waterflow control system."@en ;
        rdfs:label             "waterFlowControlSystemType"@en ;
        schema:domainIncludes  <https://w3id.org/product/CooledBeam> .

props:actualCompletion
        a                      owl:DatatypeProperty ;
        rdfs:comment           "The actual completion percentage of the allocation."@en , "実績の完了率。"@ja-JP ;
        rdfs:label             "actualCompletion"@en , "実績完了率"@ja-JP ;
        rdfs:range             <https://w3id.org/product/TimeSeries> ;
        rdfs:range             [ owl:allValuesFrom  <https://w3id.org/measurement/normalisedRatio> ;
                                 owl:onProperty     <https://w3id.org/measurement/seriesOf>
                               ] ;
        schema:domainIncludes  <https://w3id.org/product/ConstructionResource> .

props:isentropicEfficiency
        a                      owl:DatatypeProperty ;
        rdfs:comment           "Ratio of the work required for isentropic compression of the gas to work input to the compressor shaft."@en , "Rapport entre le travail requis pour une compression isentropique du gaz et le travail fourni à l'arbre du compresseur."@fr-FR ;
        rdfs:label             "isentropicEfficiency"@en , "RendementIsentropique"@fr-FR ;
        rdfs:range             <https://w3id.org/product/TimeSeries> ;
        rdfs:range             [ owl:allValuesFrom  <https://w3id.org/measurement/normalisedRatio> ;
                                 owl:onProperty     <https://w3id.org/measurement/seriesOf>
                               ] ;
        schema:domainIncludes  <https://w3id.org/product/Compressor> .

props:location  rdfs:comment   "Location  (a single type of diffuser can be used for multiple locations); high means close to ceiling."@en , "制気口の取り付け位置（壁面高所・低部、天井ぺり、天井中央、床、床下他）"@ja-JP , "Emplacement (un seul type de diffuseur peut être utilisé pour des emplaments multiples); Haut signifie proche du plafond."@fr-FR ;
        rdfs:label             "location"@en , "位置"@ja-JP , "Emplacement"@fr-FR ;
        schema:domainIncludes  <https://w3id.org/product/AirTerminal> .

props:sprayType  rdfs:comment  "SprayFilled: Water is sprayed into airflow.\nSplashTypeFill: water cascades over successive rows of splash bars.\nFilmTypeFill: water flows in a thin layer over closely spaced sheets."@en ;
        rdfs:label             "sprayType"@en ;
        schema:domainIncludes  <https://w3id.org/product/CoolingTower> .

props:auxiliaryEnergyConsumption
        a                      owl:DatatypeProperty ;
        rdfs:comment           "Boiler secondary energy source consumption (i.e., the electricity consumed by electrical devices such as fans and pumps)."@en , "ボイラ補助エネルギ消費量（つまりファンおよびポンプのような電気装置によって消費される電気）"@ja-JP , "Consommation d'énergie secondaire de la chaudière(c'est-à-dire l'électricité consommée pour les équipements électriques tels que ventilateurs et circulateurs)."@fr-FR ;
        rdfs:label             "auxiliaryEnergyConsumption"@en , "補助エネルギ消費量"@ja-JP , "ConsommationEnergieAuxiliaire"@fr-FR ;
        rdfs:range             <https://w3id.org/product/TimeSeries> ;
        rdfs:range             [ owl:allValuesFrom  <https://w3id.org/measurement/power> ;
                                 owl:onProperty     <https://w3id.org/measurement/seriesOf>
                               ] ;
        schema:domainIncludes  <https://w3id.org/product/Boiler> .

props:correctionFactorForCooling
        a                      owl:DatatypeProperty ;
        rdfs:comment           "Correction factor k as a function of water flow rate (used to calculate cooling capacity)."@en ;
        rdfs:label             "correctionFactorForCooling"@en ;
        rdfs:range             <https://w3id.org/product/TimeSeries> ;
        rdfs:range             [ owl:allValuesFrom  xsd:decimal ;
                                 owl:onProperty     <https://w3id.org/measurement/seriesOf>
                               ] ;
        schema:domainIncludes  <https://w3id.org/product/CooledBeam> .

props:hasProtectiveEarth
        a                      owl:DatatypeProperty ;
        rdfs:comment           "One core has protective earth marked insulation, Yellow/Green."@en , "各ケーブルは黄色や緑で塗色された絶縁体をもっている。"@ja-JP , "각 케이블은 노란색 또는 녹색으로 도색되었다 절연체를 가지고있다."@ko-KR ;
        rdfs:label             "hasProtectiveEarth"@en , "保護用接地の有無"@ja-JP , "보호 접지의 유무"@ko-KR ;
        rdfs:range             xsd:boolean ;
        schema:domainIncludes  <https://w3id.org/product/CableSegment#CABLESEGMENT> .

props:neckArea  a              owl:DatatypeProperty ;
        rdfs:comment           "Neck area of the air terminal."@en , "ターミナルのネック面積"@ja-JP , "Partie la plus étroite du terminal de ventilation."@fr-FR ;
        rdfs:label             "neckArea"@en , "ネック面積"@ja-JP , "ZoneReduction"@fr-FR ;
        rdfs:range             <https://w3id.org/measurement/area> ;
        schema:domainIncludes  <https://w3id.org/product/AirTerminal> .

props:faceVelocity  a          owl:DatatypeProperty ;
        rdfs:comment           "Air velocity through the coil."@en , "Vitesse de l'air à travers la batterie."@fr-FR ;
        rdfs:label             "faceVelocity"@en , "VitesseFace"@fr-FR ;
        rdfs:range             <https://w3id.org/product/TimeSeries> ;
        rdfs:range             [ owl:allValuesFrom  <https://w3id.org/measurement/linearVelocity> ;
                                 owl:onProperty     <https://w3id.org/measurement/seriesOf>
                               ] ;
        schema:domainIncludes  <https://w3id.org/product/Coil> .

props:supplyWaterTemperatureCooling
        a                      owl:DatatypeProperty ;
        rdfs:comment           "Supply water temperature in cooling mode."@en ;
        rdfs:label             "supplyWaterTemperatureCooling"@en ;
        rdfs:range             <https://w3id.org/product/TimeSeries> ;
        rdfs:range             [ owl:allValuesFrom  <https://w3id.org/measurement/thermodynamicTemperature> ;
                                 owl:onProperty     <https://w3id.org/measurement/seriesOf>
                               ] ;
        schema:domainIncludes  <https://w3id.org/product/CooledBeam> .

props:entranceLevel  a         owl:DatatypeProperty ;
        rdfs:comment           "Angabe, ob der Gebäudeeingang sich in diesem Geschoss befinded (WAHR), oder nicht (FALSCH)."@de-DE , "Indication si l'étage est au niveau d'une entrée (VRAI) ou non (FAUX)"@fr-FR , "Indication whether this building storey is an entrance level to the building (TRUE), or (FALSE) if otherwise."@en , "エントランスレベルかどうかを示すブーリアン値。"@ja-JP , "입구 레벨 여부를 나타내는 값"@ko-KR ;
        rdfs:label             "입구 레벨"@ko-KR , "Eingangsebene"@de-DE , "entranceLevel"@en , "エントランスレベル"@ja-JP , "NiveauEntrée"@fr-FR ;
        rdfs:range             xsd:boolean ;
        schema:domainIncludes  <https://w3id.org/product/BuildingStorey> .

props:scheduleCompletion
        a                      owl:DatatypeProperty ;
        rdfs:comment           "The scheduled completion percentage of the allocation."@en , "予定された完了率。"@ja-JP ;
        rdfs:label             "scheduleCompletion"@en , "予定完了率"@ja-JP ;
        rdfs:range             <https://w3id.org/product/TimeSeries> ;
        rdfs:range             [ owl:allValuesFrom  <https://w3id.org/measurement/normalisedRatio> ;
                                 owl:onProperty     <https://w3id.org/measurement/seriesOf>
                               ] ;
        schema:domainIncludes  <https://w3id.org/product/ConstructionResource> .

props:user  a                  owl:DatatypeProperty ;
        rdfs:comment           "Indicates acknowledging user over time by identification corresponding to IfcPerson.Identification on an IfcActor."@en ;
        rdfs:label             "user"@en ;
        rdfs:range             <https://w3id.org/product/TimeSeries> ;
        rdfs:range             [ owl:allValuesFrom  xsd:string ;
                                 owl:onProperty     <https://w3id.org/measurement/seriesOf>
                               ] ;
        schema:domainIncludes  <https://w3id.org/product/Alarm> .

props:frameThickness  a        owl:DatatypeProperty ;
        rdfs:comment           "The thickness of the damper frame material."@en ;
        rdfs:label             "frameThickness"@en ;
        rdfs:range             <https://w3id.org/measurement/positiveLength> ;
        schema:domainIncludes  <https://w3id.org/product/Damper> .

props:requestComments
        a                      owl:DatatypeProperty ;
        rdfs:comment           "Comments that may be made on the request."@en , "要請を作成する人物の名称。"@ja-JP ;
        rdfs:label             "requestComments"@en , "要請ソース名"@ja-JP ;
        rdfs:range             xsd:string ;
        schema:domainIncludes  <https://w3id.org/product/ActionRequest> .

props:integralConstant
        a                      owl:DatatypeProperty ;
        rdfs:comment           "The integral gain factor of the controller (usually referred to as Ki).  Asserted where ControlType is PROPORTIONALINTEGRAL or PROPORTIONALINTEGRALDERIVATIVE."@en , "적분 게인 (Ki)"@ko-KR ;
        rdfs:label             "integralConstant"@en , "적분 게인 (Ki)"@ko-KR ;
        rdfs:range             xsd:decimal ;
        schema:domainIncludes  <https://w3id.org/product/Controller#PROPORTIONAL> .

props:pipeConnectionEnum
        rdfs:comment           "The manner in which the pipe connection is made to the cooled beam."@en ;
        rdfs:label             "pipeConnectionEnum"@en ;
        schema:domainIncludes  <https://w3id.org/product/CooledBeam> .

props:internalWaterVolume
        a                      owl:DatatypeProperty ;
        rdfs:comment           "Internal volume of condenser (water side)."@en ;
        rdfs:label             "internalWaterVolume"@en ;
        rdfs:range             <https://w3id.org/measurement/volume> ;
        schema:domainIncludes  <https://w3id.org/product/Condenser> .

props:application  rdfs:comment  "Indicates application of controller."@en , "Indicates application of actuator."@en ;
        rdfs:label             "application"@en ;
        schema:domainIncludes  <https://w3id.org/product/Controller#PROGRAMMABLE> , <https://w3id.org/product/Actuator> .

props:videoCaptionMode
        rdfs:comment           "クローズドキャプションモードを示す。(字幕機能）"@ja-JP , "자막 모드를 나타낸다.(자막 기능)"@ko-KR , "Indicates closed captioning modes."@en , "자막 모드를 나타낸다. (자막 기능)"@ko-KR , "Indicates video closed captioning modes."@en ;
        rdfs:label             "비디오 캡쳐모드"@ko-KR , "ビデオキャプションモード"@ja-JP , "videoCaptionMode"@en , "비디오 캡션 모드"@ko-KR ;
        schema:domainIncludes  <https://w3id.org/product/AudioVisualAppliance#PROJECTOR> , <https://w3id.org/product/AudioVisualAppliance#DISPLAY> .

props:constructionMethod
        a                      owl:DatatypeProperty ;
        rdfs:comment           "The type of construction action to the building, the project deals with, e.g. new construction, renovation, refurbishment, etc."@en , "Designator for whether the concrete element is constructed on site or prefabricated. Allowed values are: 'In-Situ' vs 'Precast'."@en , "Angabe, ob dieses Betonbauteil als Ortbeton (\"In-Situ\") oder als Fertigteil (\"Precast\") ausgeführt werden soll."@de-DE , "Le type d'intervention sur le bâtiment : construction neuve, rénovation, réhabilitation, etc."@fr-FR , "공사의 유형. 예 : 신축 리노베이션 · 개장 등."@ko-KR , "工事におけるタイプ。例：新築・リノベーション・改装等。"@ja-JP , "Wesentliche Konstruktionsart des Gebäudes (Stahlbeton, Stahlbau, Holzfachwerk, etc.)"@de-DE ;
        rdfs:label             "constructionMethod"@en , "工事種別"@ja-JP , "Ausführung"@de-DE , "RisqueIncendieUsagePrincipal"@fr-FR , "공사 종류"@ko-KR , "Konstruktionsart"@de-DE ;
        rdfs:range             xsd:string ;
        schema:domainIncludes  <https://w3id.org/product/BuildingElement> , <https://w3id.org/product/Building> .

props:contrastRatio  a         owl:DatatypeProperty ;
        rdfs:comment           "Indicates the display contrast ratio."@en , "コントラスト比を示す。"@ja-JP , "명암비를 보여준다"@ko-KR ;
        rdfs:label             "contrastRatio"@en , "コントラスト比"@ja-JP , "명암비"@ko-KR ;
        rdfs:range             <https://w3id.org/measurement/positiveRatio> ;
        schema:domainIncludes  <https://w3id.org/product/AudioVisualAppliance#DISPLAY> .

props:touchScreen  rdfs:comment  "Indicates touchscreen support."@en , "タッチスクリーンのサポートを示す。"@ja-JP , "터치 스크린 지원을 보여준다"@ko-KR ;
        rdfs:label             "touchScreen"@en , "タッチスクリーン"@ja-JP , "터치 스크린"@ko-KR ;
        schema:domainIncludes  <https://w3id.org/product/AudioVisualAppliance#DISPLAY> .

props:externalSurfaceArea
        a                      owl:DatatypeProperty ;
        rdfs:comment           "External surface area (both primary and secondary area)."@en ;
        rdfs:label             "externalSurfaceArea"@en ;
        rdfs:range             <https://w3id.org/measurement/area> ;
        schema:domainIncludes  <https://w3id.org/product/Condenser> .

props:status  a                owl:DatatypeProperty ;
        rdfs:comment           "エラーコードまたはIDを示す。例：'ConfigurationError', 'NotConnected', 'DeviceFailure', 'SensorFailure', 'LastKnown, 'CommunicationsFailure', 'OutOfService'."@ja-JP , "Indicates an error code or identifier, whose meaning is specific to the particular automation system.  Example values include: 'ConfigurationError', 'NotConnected', 'DeviceFailure', 'SensorFailure', 'LastKnown, 'CommunicationsFailure', 'OutOfService'."@en , "대체 기능으로 수동 조작이 제공되는지 (= TRUE) 여부 (= FALSE)를 확인한다. 수동으로 조작하는 액츄에이터의 경우는이 값을 기본값으로 FALSE로 설정해야하므로주의한다."@ko-KR , "Etat de l'élément, utilisé avant tout pour les projets de rénovation et réaménagement. L'état assigné peut être \"Nouveau\" - l'élément prévu pour du neuf, \"Existant\" - l'élément existait et est maintenu, \"Démoli\" - l'élément existait mais doit être démoli/supprimé, \"Provisoire\" - l'élément existera à titre provisoire seulement (comme un support structurel par exemple)."@fr-FR , "Status of the element, predominately used in renovation or retrofitting projects. The status can be assigned to as \"New\" - element designed as new addition, \"Existing\" - element exists and remains, \"Demolish\" - element existed but is to be demolished,  \"Temporary\" - element will exists only temporary (like a temporary support structure)."@en , "Statut de l'élément, principalement utilisé dans les projets de rénovation et de réhabilitation. Le statut a pour valeur NOUVEAU pour un nouvel élément, EXISTANT pour un élément existant qui est conservé, DEMOLI pour un élément existant à démolir et TEMPORAIRE pour un élément temporaire (comme une structure support provisoire)."@fr-FR , "Status bzw. Phase des Bauteils insbesondere beim Bauen im Bestand. \"Neu\" (new) neues Bauteil als Ergänzung, \"Bestand\" (existing) bestehendes Bauteil, dass erhalten bleibt, \"Abbruch\" (demolish) Bauteil, das abgebrochen wird, \"Temporär\" (temporary) Bauteil und andere Bauelemente, die vorübergehend eingebaut werden (wie Abstützungen, etc.)"@de-DE , "要素（主にリノベーションまたは改修プロジェクトにおいて）の状態。 状態は、「新規(New)」－新しく追加される要素。「既存」－要素は存在し、かつ残りもの。「破壊」－要素は存在したが、廃棄されるもの。「一時的」－一時的に存在する要素（一時的にサポートしている構造のようなもの）。"@ja-JP , "요청한 액츄에이터의 안전 장치 유형을 표시"@ko-KR , "현재 전원 상태를 나타냄"@ko-KR ;
        rdfs:label             "状態"@ja-JP , "재정 기능의 유무"@ko-KR , "Etat"@fr-FR , "Status"@de-DE , "전원 상태"@ko-KR , "status"@en , "Statut"@fr-FR , "페일 세이프 유형"@ko-KR ;
        rdfs:range             <https://w3id.org/product/TimeSeries> ;
        rdfs:range             [ owl:allValuesFrom  xsd:string ;
                                 owl:onProperty     <https://w3id.org/measurement/seriesOf>
                               ] ;
        rdfs:range             [ owl:allValuesFrom  xsd:string ;
                                 owl:onProperty     <https://w3id.org/measurement/seriesOf>
                               ] ;
        schema:domainIncludes  <https://w3id.org/product/Beam> , <https://w3id.org/product/CableFitting> , <https://w3id.org/product/Chiller> , <https://w3id.org/product/CurtainWall> , <https://w3id.org/product/BuildingElementProxy> , <https://w3id.org/product/AudioVisualAppliance> , <https://w3id.org/product/CableSegment> , <https://w3id.org/product/Coil> , <https://w3id.org/product/Compressor> , <https://w3id.org/product/Alarm> , <https://w3id.org/product/Actuator> , <https://w3id.org/product/Burner> , <https://w3id.org/product/AirTerminalBox> , <https://w3id.org/product/CoolingTower> , <https://w3id.org/product/AirToAirHeatRecovery> , <https://w3id.org/product/Covering> , <https://w3id.org/product/Damper> , <https://w3id.org/product/Column> , <https://w3id.org/product/CommunicationsAppliance> , <https://w3id.org/product/Controller> , <https://w3id.org/product/CableCarrierFitting> , <https://w3id.org/product/Chimney> , <https://w3id.org/product/CableCarrierSegment> , <https://w3id.org/product/Boiler> , <https://w3id.org/product/CooledBeam> , <https://w3id.org/product/AirTerminal> .

props:volumetricEfficiency
        a                      owl:DatatypeProperty ;
        rdfs:comment           "Ratio of the actual volume of gas entering the compressor to the theoretical displacement of the compressor."@en , "Rapport entre le volume effectif de gaz rentrant dans le compresseur et le volume déplacé théorique du compresseur."@fr-FR ;
        rdfs:label             "volumetricEfficiency"@en , "RendementVolumétrique"@fr-FR ;
        rdfs:range             <https://w3id.org/product/TimeSeries> ;
        rdfs:range             [ owl:allValuesFrom  <https://w3id.org/measurement/normalisedRatio> ;
                                 owl:onProperty     <https://w3id.org/measurement/seriesOf>
                               ] ;
        schema:domainIncludes  <https://w3id.org/product/Compressor> .

props:playerMediaFormat
        rdfs:comment           "Indicates supported media formats."@en , "サポートされているメディアのフォーマットを示す。"@ja-JP , "지원되는 미디어 형식을 보여준다."@ko-KR ;
        rdfs:label             "playerMediaFormat"@en , "メディアフォーマット"@ja-JP , "미디어 포맷"@ko-KR ;
        schema:domainIncludes  <https://w3id.org/product/AudioVisualAppliance#PLAYER> .

props:arrangementType
        rdfs:comment           "Terminal box arrangement.\nSingleDuct: Terminal box receives warm or cold air from a single air supply duct.\nDualDuct: Terminal box receives warm and cold air from separate air supply ducts."@en , "ターミナルボックスの形式。\n単一ダクト：単一のダクトから、温風または冷風を受け取る\nデュアルダクト：温風、冷風を分離されたダクトから受け取る"@ja-JP , "Configuration du registre terminal.\nConduit unique: le registre terminal reçoit de l'air chaud ou froid depuis un conduit unique d'amenée d'air"@fr-FR ;
        rdfs:label             "arrangementType"@en , "ターミナル形式"@ja-JP , "Type de configuration"@fr-FR ;
        schema:domainIncludes  <https://w3id.org/product/AirTerminalBox> .

props:proportionalConstant
        a                      owl:DatatypeProperty ;
        rdfs:comment           "The proportional gain factor of the controller (usually referred to as Kp)."@en , "비례 게인 (Kp)"@ko-KR ;
        rdfs:label             "proportionalConstant"@en , "비례 게인 (Kp)"@ko-KR ;
        rdfs:range             xsd:decimal ;
        schema:domainIncludes  <https://w3id.org/product/Controller#PROPORTIONAL> .

props:material  rdfs:comment   "Type of material from which the conductor is constructed."@en , "導体を構成する材料のタイプ。"@ja-JP , "도체를 구성하는 재료의 종류."@ko-KR ;
        rdfs:label             "material"@en , "材料"@ja-JP , "도체의 기능 유형."@ko-KR ;
        schema:domainIncludes  <https://w3id.org/product/CableSegment#CONDUCTORSEGMENT> .

props:nominalSupplyWaterTemperatureHeating
        a                      owl:DatatypeProperty ;
        rdfs:comment           "Nominal supply water temperature (refers to nominal heating capacity)."@en ;
        rdfs:label             "nominalSupplyWaterTemperatureHeating"@en ;
        rdfs:range             <https://w3id.org/measurement/thermodynamicTemperature> ;
        schema:domainIncludes  <https://w3id.org/product/CooledBeam> .

props:occupancyType  a         owl:DatatypeProperty ;
        rdfs:comment           "Type d'occupation. Est défini selon le Code National en vigueur."@fr-FR , "점령 자의 유형. 건축 기준법을 준수합니다."@ko-KR , "Hauptnutzungsart des Gebäudes (Schulbau. Kaufhaus, etc.). Wird verwendet, wenn keine allgemein anerkanntes Klassifizierungssystem angewandt wird."@de-DE , "Occupancy type for this object.\nIt is defined according to the presiding national building code."@en , "占有者のタイプ。建築基準法に準拠。"@ja-JP ;
        rdfs:label             "점유자 유형"@ko-KR , "占有者タイプ"@ja-JP , "TypeOccupation"@fr-FR , "Nutzungsart"@de-DE , "occupancyType"@en ;
        rdfs:range             xsd:string ;
        schema:domainIncludes  <https://w3id.org/product/Building> .

props:coilWidth  a             owl:DatatypeProperty ;
        rdfs:comment           "Width of coil."@en ;
        rdfs:label             "coilWidth"@en ;
        rdfs:range             <https://w3id.org/measurement/positiveLength> ;
        schema:domainIncludes  <https://w3id.org/product/CooledBeam> .

props:concreteCoverAtMainBars
        a                      owl:DatatypeProperty ;
        rdfs:comment           "Abstand zwischen der Betonoberfläche und der Außenkante den vom Beton umhüllten Bewehrungshauptstäben."@de-DE , "국가의 건축 기준에 따라 주로 철근을 콘크리트 입고로 보호"@ko-KR , "国の建築基準に従い、主鉄筋をコンクリートの被りで保護する。"@ja-JP , "The protective concrete cover at the main reinforcing bars according to local building regulations."@en ;
        rdfs:label             "Betonüberdeckung Hauptstäbe"@de-DE , "主筋のコンクリート被り"@ja-JP , "concreteCoverAtMainBars"@en , "주근 콘크리트 입고"@ko-KR ;
        rdfs:range             <https://w3id.org/measurement/positiveLength> ;
        schema:domainIncludes  <https://w3id.org/product/BuildingElement> .

props:heatTransferSurfaceArea
        a                      owl:DatatypeProperty ;
        rdfs:comment           "Total heat transfer area of the vessel."@en , "容器の伝熱部面積の合計"@ja-JP , "Surface totale d'échange de chaleur du foyer"@fr-FR ;
        rdfs:label             "heatTransferSurfaceArea"@en , "伝熱面積"@ja-JP , "SurfaceEchangeChaleur"@fr-FR ;
        rdfs:range             <https://w3id.org/measurement/area> ;
        schema:domainIncludes  <https://w3id.org/product/Boiler> .

props:condensingTemperature
        a                      owl:DatatypeProperty ;
        rdfs:comment           "Refrigerant condensing temperature."@en ;
        rdfs:label             "condensingTemperature"@en ;
        rdfs:range             <https://w3id.org/product/TimeSeries> ;
        rdfs:range             [ owl:allValuesFrom  <https://w3id.org/measurement/thermodynamicTemperature> ;
                                 owl:onProperty     <https://w3id.org/measurement/seriesOf>
                               ] ;
        schema:domainIncludes  <https://w3id.org/product/Condenser> .

props:remainingCost  a         owl:DatatypeProperty ;
        rdfs:comment           "The remaining cost on behalf of the resource allocation."@en , "資源配分のための残存しているコスト。"@ja-JP ;
        rdfs:label             "remainingCost"@en , "残存コスト"@ja-JP ;
        rdfs:range             <https://w3id.org/product/TimeSeries> ;
        rdfs:range             [ owl:allValuesFrom  <https://w3id.org/measurement/monetary> ;
                                 owl:onProperty     <https://w3id.org/measurement/seriesOf>
                               ] ;
        schema:domainIncludes  <https://w3id.org/product/ConstructionResource> .

props:nominalPartLoadRatio
        rdfs:comment           "Allowable part load ratio range."@en , "許容部分負荷比範囲"@ja-JP , "Plage de charge partielle admissible"@fr-FR ;
        rdfs:label             "nominalPartLoadRatio"@en , "設計部分負荷比率"@ja-JP , "PlageNominaleChargePartielle"@fr-FR ;
        schema:domainIncludes  <https://w3id.org/product/Boiler> .

props:value  a                 owl:DatatypeProperty ;
        rdfs:comment           "The expected range and default value.  While the property data type is IfcReal (to support all cases including when the units are unknown), a unit may optionally be provided to indicate the measure and unit.  The LowerLimitValue and UpperLimitValue must fall within the physical Range and may be used to determine extents when charting Pset_ControllerPHistory.Value."@en , "The default value such as normally-closed or normally-open."@en , "The expected range and default value.  While the property data type is IfcReal (to support all cases including when the units are unknown), a unit may optionally be provided to indicate the measure and unit."@en , "시간이 지남에 오류 상태를 나타내는 Pset_ControllerTypeValue.Fault에 대응 ※ 설정 가능한 정보는 IfcTimeSeries 속성 참조"@ko-KR , "Indicates values over time which may be recorded continuously or only when changed beyond a particular deadband.  The range of possible values is defined by the Value property on the corresponding occurrence property set (Pset_ControllerTypeFloating, Pset_ControllerTypeProportional, Pset_ControllerTypeMultiPosition, or Pset_ControllerTypeTwoPosition)."@en , "時間とともに値を示す。\nPset_ControllerTypeValue.Valueに対応\n※ 設定可能情報は IfcTimeSeriesプロパティ参照"@ja-JP , "The expected range and default value.  The LowerLimitValue and UpperLimitValue must fall within the physical Range."@en ;
        rdfs:label             "value"@en , "이상 출력 시계열 상수"@ko-KR , "デフォルト出力時系列定数"@ja-JP ;
        rdfs:range             <https://w3id.org/product/TimeSeries> , xsd:boolean ;
        rdfs:range             [ owl:allValuesFrom  xsd:decimal ;
                                 owl:onProperty     <https://w3id.org/measurement/seriesOf>
                               ] ;
        schema:domainIncludes  <https://w3id.org/product/Controller#TWOPOSITION> , <https://w3id.org/product/Controller> , <https://w3id.org/product/Controller#FLOATING> , <https://w3id.org/product/Controller#MULTIPOSITION> , <https://w3id.org/product/Controller#PROPORTIONAL> .

props:carrierStackNumber
        a                      owl:DatatypeProperty ;
        rdfs:comment           "Number of carrier segments (tray, ladder etc.) that are vertically stacked (vertical is measured as the z-axis of the local coordinate system of the carrier segment)."@en ;
        rdfs:label             "carrierStackNumber"@en ;
        rdfs:range             xsd:int ;
        schema:domainIncludes  <https://w3id.org/product/CableSegment> .

props:severity  a              owl:DatatypeProperty ;
        rdfs:comment           "Indicates alarm severity over time, where the scale of values is determined by the control system configuration.  A zero value indicates no present alarm."@en ;
        rdfs:label             "severity"@en ;
        rdfs:range             <https://w3id.org/product/TimeSeries> ;
        rdfs:range             [ owl:allValuesFrom  xsd:int ;
                                 owl:onProperty     <https://w3id.org/measurement/seriesOf>
                               ] ;
        schema:domainIncludes  <https://w3id.org/product/Alarm> .

props:bladePositionAngle
        a                      owl:DatatypeProperty ;
        rdfs:comment           "Blade position angle; angle between the blade and flow direction ( 0 - 90)."@en ;
        rdfs:label             "bladePositionAngle"@en ;
        rdfs:range             <https://w3id.org/product/TimeSeries> ;
        rdfs:range             [ owl:allValuesFrom  <https://w3id.org/measurement/positivePlaneAngle> ;
                                 owl:onProperty     <https://w3id.org/measurement/seriesOf>
                               ] ;
        schema:domainIncludes  <https://w3id.org/product/Damper> .

props:reinforcementAreaRatio
        a                      owl:DatatypeProperty ;
        rdfs:comment           "The required ratio of the effective area of the reinforcement to the effective area of the concrete At any section of a reinforced concrete structural element."@en , "Das geforderte Verhältnis der effektiven flächenbezogenen Masse der Bewehrung im Verhältnis zur effektiven Fläche des Betons für dieses Element."@de-DE ;
        rdfs:label             "reinforcementAreaRatio"@en , "Bewehrungsgrad Fläche"@de-DE ;
        rdfs:range             <https://w3id.org/measurement/areaDensity> ;
        schema:domainIncludes  <https://w3id.org/product/BuildingElement> .

props:defrostTemperatureEffectiveness
        a                      owl:DatatypeProperty ;
        rdfs:comment           "Temperature heat transfer effectiveness when defrosting is active."@en , "デフロスト作動時の温度熱交換効率"@ja-JP , "Efficacité thermique sensible lorsque le mode dégel est actif"@fr-FR ;
        rdfs:label             "デフロスト温度効率"@ja-JP , "defrostTemperatureEffectiveness"@en , "EfficacitéTemperatureDégel"@fr-FR ;
        rdfs:range             <https://w3id.org/product/TimeSeries> ;
        rdfs:range             [ owl:allValuesFrom  <https://w3id.org/measurement/normalisedRatio> ;
                                 owl:onProperty     <https://w3id.org/measurement/seriesOf>
                               ] ;
        schema:domainIncludes  <https://w3id.org/product/AirToAirHeatRecovery> .

props:maximumWorkingPressure
        a                      owl:DatatypeProperty ;
        rdfs:comment           "Maximum working pressure."@en ;
        rdfs:label             "maximumWorkingPressure"@en ;
        rdfs:range             <https://w3id.org/measurement/pressure> ;
        schema:domainIncludes  <https://w3id.org/product/Damper> .

props:throw  a                 owl:DatatypeProperty ;
        rdfs:comment           "Distance cooled beam throws the air."@en ;
        rdfs:label             "throw"@en ;
        rdfs:range             <https://w3id.org/product/TimeSeries> ;
        rdfs:range             [ owl:allValuesFrom  <https://w3id.org/measurement/positiveLength> ;
                                 owl:onProperty     <https://w3id.org/measurement/seriesOf>
                               ] ;
        schema:domainIncludes  <https://w3id.org/product/CooledBeam#ACTIVE> .

props:height  a                owl:DatatypeProperty ;
        rdfs:comment           "空間の高さ（高さにおける垂直方向の拡張）を求める定義です。「四角形」の形状プロパティのみ提示されます。"@ja-JP , "The requested height (vertical extension in elevation) of the provision for void\", only provided if the Shape property is set to \"rectangle\"."@en , "Geforderte Höhe des Durchbruchs, wird nur dann angegeben, wenn der Wert des Attributes \"Form\" gleich \"Rechteck\" ist."@de-DE , "La hauteur requise de la réservation (extension verticale en élévation). Fournie seulement si la propriété Forme a pour valeur \"Rectangle\"."@fr-FR , "空构件的高度（在立面图中竖直方向的长度），仅当“形状”属性为“矩形”时适用。"@zh-CN ;
        rdfs:label             "Hauteur"@fr-FR , "Höhe"@de-DE , "高さ"@ja-JP , "高度"@zh-CN , "height"@en ;
        rdfs:range             <https://w3id.org/measurement/positiveLength> ;
        schema:domainIncludes  <https://w3id.org/product/BuildingElementProxy#PROVISIONFORVOID> .

props:compressorCondenserPressureDrop
        a                      owl:DatatypeProperty ;
        rdfs:comment           "Pressure drop between condenser inlet and compressor outlet."@en ;
        rdfs:label             "compressorCondenserPressureDrop"@en ;
        rdfs:range             <https://w3id.org/product/TimeSeries> ;
        rdfs:range             [ owl:allValuesFrom  <https://w3id.org/measurement/pressure> ;
                                 owl:onProperty     <https://w3id.org/measurement/seriesOf>
                               ] ;
        schema:domainIncludes  <https://w3id.org/product/Condenser> .

props:marketSubCategoriesAvailableNow
        rdfs:comment           "A list of the sub categories of property that are currently available expressed in terms of IfcLabel."@en , "Liste de sous catégories actuellement disponibles"@fr-FR ;
        rdfs:label             "marketSubCategoriesAvailableNow"@en , "DisponibilitesActuellesParSousCategories"@fr-FR ;
        schema:domainIncludes  <https://w3id.org/product/Building> .

props:leakage  a               owl:DatatypeProperty ;
        rdfs:comment           "Air leakage rate."@en ;
        rdfs:label             "leakage"@en ;
        rdfs:range             <https://w3id.org/product/TimeSeries> ;
        rdfs:range             [ owl:allValuesFrom  <https://w3id.org/measurement/volumetricFlowRate> ;
                                 owl:onProperty     <https://w3id.org/measurement/seriesOf>
                               ] ;
        schema:domainIncludes  <https://w3id.org/product/Damper> .

props:marketSubCategory
        a                      owl:DatatypeProperty ;
        rdfs:comment           "Sous catégorie d'usage."@fr-FR , "Subset of category of use e.g. multi-family, 2 bedroom, low rise."@en , "Sous catégorie d'usage (exemple : collectif, deux pièces,…)"@fr-FR ;
        rdfs:label             "SousCategorieUsage"@fr-FR , "marketSubCategory"@en , "SousCategorieMarche"@fr-FR ;
        rdfs:range             xsd:string ;
        schema:domainIncludes  <https://w3id.org/product/Building> .

props:visibleAngleLeft
        a                      owl:DatatypeProperty ;
        rdfs:comment           "Angle of visibility to the left of the access."@en , "Angle de visibilité à la gauche de l'accès."@fr-FR , "左側の経路に可視出来る角度。"@ja-JP ;
        rdfs:label             "visibleAngleLeft"@en , "VisibiliteAngleGauche"@fr-FR , "左側可視角度"@ja-JP ;
        rdfs:range             <https://w3id.org/measurement/positivePlaneAngle> ;
        schema:domainIncludes  <https://w3id.org/product/Annotation#LineOfSight> .

props:bladeThickness  a        owl:DatatypeProperty ;
        rdfs:comment           "The thickness of the damper blade."@en ;
        rdfs:label             "bladeThickness"@en ;
        rdfs:range             <https://w3id.org/measurement/positiveLength> ;
        schema:domainIncludes  <https://w3id.org/product/Damper> .

props:softwareVersion
        a                      owl:DatatypeProperty ;
        rdfs:comment           "Indicates version of application software according to systems integrator."@en , "컨트롤러 소프트웨어 버전"@ko-KR ;
        rdfs:label             "softwareVersion"@en , "소프트웨어 버전"@ko-KR ;
        rdfs:range             xsd:string ;
        schema:domainIncludes  <https://w3id.org/product/Controller#PROGRAMMABLE> .

props:energyEfficiencyRatio
        a                      owl:DatatypeProperty ;
        rdfs:comment           "L'EER ou Energy Efficiency Ratio est le coefficient d'efficacité frigorifique, rapport entre entre l'énergie utile frigorifique divisée parénergie absorbée au compresseur.\nPar définition, l'unité est le BTU/hour par Watt.\nLa puissance électrique fournie peut être obtenue depuis Pset_DistributionPortHistoryElectrical.RealPower sur le port \"Power\"  du IfcChiller."@fr-FR , "EER, coefficient d'efficacité Thermique"@fr-FR , "The Energy efficiency ratio (EER) is the ratio of net cooling capacity to the total input rate of electric power applied.  By definition, the units are BTU/hour per Watt.\nThe input electric power may be obtained from Pset_DistributionPortPHistoryElectrical.RealPower on the 'Power' port of the IfcChiller."@en , "Energy efficiency ratio (EER)."@en ;
        rdfs:label             "CoefficientEfficacitéThermique"@fr-FR , "energyEfficiencyRatio"@en , "CoefficientEfficacitéEnergétique"@fr-FR ;
        rdfs:range             <https://w3id.org/product/TimeSeries> ;
        rdfs:range             [ owl:allValuesFrom  xsd:decimal ;
                                 owl:onProperty     <https://w3id.org/measurement/seriesOf>
                               ] ;
        rdfs:range             [ owl:allValuesFrom  xsd:decimal ;
                                 owl:onProperty     <https://w3id.org/measurement/seriesOf>
                               ] ;
        schema:domainIncludes  <https://w3id.org/product/Chiller> , <https://w3id.org/product/Compressor> .

props:nominalWaterFlowHeating
        a                      owl:DatatypeProperty ;
        rdfs:comment           "Nominal water flow (refers to nominal heating capacity)."@en ;
        rdfs:label             "nominalWaterFlowHeating"@en ;
        rdfs:range             <https://w3id.org/measurement/volumetricFlowRate> ;
        schema:domainIncludes  <https://w3id.org/product/CooledBeam> .

props:nominalEvaporatingTemperature
        a                      owl:DatatypeProperty ;
        rdfs:comment           "Chiller evaporating temperature."@en , "Température d'évaporation du groupe froid."@fr-FR ;
        rdfs:label             "nominalEvaporatingTemperature"@en , "TempératureEvaporationNominale"@fr-FR ;
        rdfs:range             <https://w3id.org/measurement/thermodynamicTemperature> ;
        schema:domainIncludes  <https://w3id.org/product/Chiller> .

props:stroke  a                owl:DatatypeProperty ;
        rdfs:comment           "Indicates the maximum distance the actuator must traverse."@en , "アクチュエータが動く最大距離を示す。"@ja-JP , "액츄에이터가 움직이는 최대 거리를 보여준다."@ko-KR ;
        rdfs:label             "stroke"@en , "ストローク"@ja-JP , "입력"@ko-KR ;
        rdfs:range             <https://w3id.org/measurement/length> ;
        schema:domainIncludes  <https://w3id.org/product/Actuator> .

props:isExternal  a            owl:DatatypeProperty ;
        rdfs:comment           "表示该构件是否设计为外部构件。若是，则该构件为外部构件，朝向建筑物的外侧。"@zh-CN , "Indication whether the element is designed for use in the exterior (TRUE) or not (FALSE). If (TRUE) it is an external element and faces the outside of the building."@en , "Angabe, ob dieses Bauteil ein Aussenbauteil ist (JA) oder ein Innenbauteil (NEIN). Als Aussenbauteil grenzt es an den Aussenraum (oder Erdreich, oder Wasser)."@de-DE , "表示该图元是否设计为外部构件。若是，则该图元为外部图元，朝向建筑物的外部。"@zh-CN , "この要素が外部に用いられるか（TRUE）、否か（FALSE）を示す。（TRUE)の場合、これは外部要素で、建物の外部に面している。"@ja-JP , "Indique si l'élément est conçu pour être utilisé à l'extérieur (VRAI) ou non (FAUX). Si VRAI, c'est un élément extérieur qui donne sur l'extérieur du bâtiment."@fr-FR , "外部の部材かどうかを示すブーリアン値。もしTRUEの場合、外部の部材で建物の外側に面している。"@ja-JP , "Angabe, ob dieser Bekleidung eine Außenbekleidung ist (JA) oder ein Innenbekleidung (NEIN)."@de-DE ;
        rdfs:label             "外部"@ja-JP , "是否外部构件"@zh-CN , "Est extérieur"@fr-FR , "isExternal"@en , "EstExterieur"@fr-FR , "外部区分"@ja-JP , "Außenbauteil"@de-DE ;
        rdfs:range             xsd:boolean ;
        schema:domainIncludes  <https://w3id.org/product/CurtainWall> , <https://w3id.org/product/Beam> , <https://w3id.org/product/Covering> , <https://w3id.org/product/Column> , <https://w3id.org/product/BuildingElementProxy> , <https://w3id.org/product/Chimney> .

props:videoResolutionMode
        rdfs:comment           "ビデオ解像度モードを示す。"@ja-JP , "解像度モードを示す。"@ja-JP , "비디오 해상도를 보여준다."@ko-KR , "Indicates video resolution modes."@en , "해상도를 보여준다"@ko-KR , "모드해상도를 보여준다"@ko-KR ;
        rdfs:label             "비디오 해상도 모드"@ko-KR , "videoResolutionMode"@en , "解像度モード"@ja-JP , "ビデオ解像度モード"@ja-JP , "디스플레이 모드"@ko-KR ;
        schema:domainIncludes  <https://w3id.org/product/AudioVisualAppliance#PROJECTOR> , <https://w3id.org/product/AudioVisualAppliance#CAMERA> , <https://w3id.org/product/AudioVisualAppliance#DISPLAY> .

props:reheatType  rdfs:comment  "Terminal box reheat type."@en , "ターミナルの再熱方式\n（電気、水コイル、蒸気コイル、ガス加熱．．．）"@ja-JP , "Type de réchauffage d'un registre terminal de ventilation"@fr-FR ;
        rdfs:label             "reheatType"@en , "再熱形式"@ja-JP , "Type de réchauffage"@fr-FR ;
        schema:domainIncludes  <https://w3id.org/product/AirTerminalBox> .

props:refrigerantFoulingResistance
        a                      owl:DatatypeProperty ;
        rdfs:comment           "Fouling resistance on the refrigerant side."@en ;
        rdfs:label             "refrigerantFoulingResistance"@en ;
        rdfs:range             <https://w3id.org/product/TimeSeries> ;
        rdfs:range             [ owl:allValuesFrom  <https://w3id.org/measurement/thermalResistance> ;
                                 owl:onProperty     <https://w3id.org/measurement/seriesOf>
                               ] ;
        schema:domainIncludes  <https://w3id.org/product/Condenser> .

props:numberOfDrafts  a        owl:DatatypeProperty ;
        rdfs:comment           "单根烟囱内的烟道数目，烟道即烟囱内供空气流通的连续孔道。"@zh-CN , "Nombre de conduits, percements continus par lesquels passe l'air à l'intérieur d'une cheminée simple."@fr-FR , "Number of the chimney drafts, continuous holes in the chimney through which the air passes, within the single chimney."@en , "一つの煙突で、煙突の筒（chimney draft）、空気が流れる連続した穴の数。"@ja-JP , "Anzahl der Schornsteinzüge innerhalb eines Schornsteins. Gewöhnlich ein-, zwei, drei oder vierzügig."@de-DE ;
        rdfs:label             "烟道数"@zh-CN , "Nombre de conduits"@fr-FR , "穴の数"@ja-JP , "Zügigkeit"@de-DE , "numberOfDrafts"@en ;
        rdfs:range             <https://w3id.org/measurement/count> ;
        schema:domainIncludes  <https://w3id.org/product/Chimney> .

props:displayHeight  a         owl:DatatypeProperty ;
        rdfs:comment           "Indicates the physical height of the screen (only the display surface)."@en , "画面の高さを示す。"@ja-JP , "화면의 높이를 나타낸다"@ko-KR ;
        rdfs:label             "displayHeight"@en , "画面高さ"@ja-JP , "화면 높이"@ko-KR ;
        rdfs:range             <https://w3id.org/measurement/positiveLength> ;
        schema:domainIncludes  <https://w3id.org/product/AudioVisualAppliance#DISPLAY> .

props:damperPosition  a        owl:DatatypeProperty ;
        rdfs:comment           "Position de contrôle du registre, compris entre 0 et 1."@fr-FR , "制御ダンパの開度（０～１）"@ja-JP , "Damper position (0-1); damper position ( 0=closed=90deg position angle, 1=open=0deg position angle."@en , "Control damper position, ranging from 0 to 1."@en ;
        rdfs:label             "Position du registre"@fr-FR , "damperPosition"@en , "ダンパ開度"@ja-JP ;
        rdfs:range             <https://w3id.org/product/TimeSeries> ;
        rdfs:range             [ owl:allValuesFrom  <https://w3id.org/measurement/normalisedRatio> ;
                                 owl:onProperty     <https://w3id.org/measurement/seriesOf>
                               ] ;
        rdfs:range             [ owl:allValuesFrom  <https://w3id.org/measurement/normalisedRatio> ;
                                 owl:onProperty     <https://w3id.org/measurement/seriesOf>
                               ] ;
        schema:domainIncludes  <https://w3id.org/product/AirTerminalBox> , <https://w3id.org/product/Damper> .

props:construction  rdfs:comment  "Purpose of informing on how the vonductor is constucted (interwined or solid). I.e. Solid (IEV 461-01-06), stranded (IEV 461-01-07), solid-/finestranded(IEV 461-01-11) (not flexible/flexible)."@en , "導体の構成（より線か単線）の定義。すなわち単線（IEV 461-01-06）、より線（IEV 461-01-07）、フレキシブル導体（IEV 461-01-11）（フレキシブルか否か）で定義。"@ja-JP , "도체 구성 (연선 또는 단선)의 정의 즉 단선 (IEV 461-01-06), 트위스트 (IEV 461-01-07), 플렉서블 도체 (IEV 461-01-11) (유연한 아닌지 가) 정의"@ko-KR ;
        rdfs:label             "construction"@en , "構造"@ja-JP , "구조"@ko-KR ;
        schema:domainIncludes  <https://w3id.org/product/CableSegment#CONDUCTORSEGMENT> .

props:yearOfLastRefurbishment
        a                      owl:DatatypeProperty ;
        rdfs:comment           "Year of last major refurbishment, or reconstruction, of the building (applies to reconstruction works)."@en , "Jahr der letzten Renovierung des Gebäudes."@de-DE , "Année de la dernière rénovation majeure ou de la reconstruction du bâtiment."@fr-FR ;
        rdfs:label             "yearOfLastRefurbishment"@en , "letztes Renovierungsjahr"@de-DE , "Année de la dernière rénovation"@fr-FR ;
        rdfs:range             xsd:string ;
        schema:domainIncludes  <https://w3id.org/product/Building> .

props:lossCoefficentCurve
        rdfs:comment           "Loss coefficient – blade position angle curve; ratio of pressure drop to velocity pressure versus blade angle; C = f (blade angle position)."@en ;
        rdfs:label             "lossCoefficentCurve"@en ;
        schema:domainIncludes  <https://w3id.org/product/Damper> .

props:temperatureRating
        a                      owl:DatatypeProperty ;
        rdfs:comment           "Temperature rating."@en ;
        rdfs:label             "temperatureRating"@en ;
        rdfs:range             <https://w3id.org/measurement/thermodynamicTemperature> ;
        schema:domainIncludes  <https://w3id.org/product/Damper> .

props:fragilityRating
        a                      owl:DatatypeProperty ;
        rdfs:comment           "脆弱性等級。当該国の建築法規による。"@ja-JP , "Indication de la fragilité du revêtement selon une classification nationale."@fr-FR , "Angabe zur Zerbrechlichkeit des Materials (zum Beispiel unter Brandlast oder Erschütterung) gemäß der nationalen oder regionalen Normen."@de-DE , "Indication on the fragility of the covering (e.g., under fire conditions).  It is given according to the national building code that might provide a classification for fragility."@en ;
        rdfs:label             "脆弱性等級"@ja-JP , "Fragilitätsklasse"@de-DE , "Fragilité"@fr-FR , "fragilityRating"@en ;
        rdfs:range             xsd:string ;
        schema:domainIncludes  <https://w3id.org/product/Covering> .

props:numberofBlades  a        owl:DatatypeProperty ;
        rdfs:comment           "Number of blades."@en ;
        rdfs:label             "numberofBlades"@en ;
        rdfs:range             xsd:int ;
        schema:domainIncludes  <https://w3id.org/product/Damper> .

props:concreteCover  a         owl:DatatypeProperty ;
        rdfs:comment           "The protective concrete cover at the reinforcing bars according to local building regulations."@en , "Abstand zwischen der Betonoberfläche und der Außenkante einer vom Beton umhüllten Bewehrung."@de-DE ;
        rdfs:label             "concreteCover"@en , "Betonüberdeckung"@de-DE ;
        rdfs:range             <https://w3id.org/measurement/positiveLength> ;
        schema:domainIncludes  <https://w3id.org/product/BuildingElement> .

props:selfExtinguishing60332_1
        a                      owl:DatatypeProperty ;
        rdfs:comment           "IEC 60332.1.に規定されている自己消火ケーブル。"@ja-JP , "自動消火ケーブル/コアはIEC 60332.1に準じる。"@ja-JP , "Self Extinguishing cable/core according to IEC 60332.1."@en , "IEC 60332.1.에 규정되어있는 자기 소화 케이블"@ko-KR , "자동 소화 케이블 / 코어는 IEC 60332.1에 준한다"@ko-KR ;
        rdfs:label             "자동 소화 60332_1"@ko-KR , "自己消火ケーブル"@ja-JP , "selfExtinguishing60332_1"@en , "自動消火60332_1"@ja-JP , "자기 소화 케이블"@ko-KR ;
        rdfs:range             xsd:boolean ;
        schema:domainIncludes  <https://w3id.org/product/CableSegment#CABLESEGMENT> , <https://w3id.org/product/CableSegment#CORESEGMENT> .

props:airflowRateRange
        rdfs:comment           "Range of airflow that can be delivered."@en , "Possible range of airflow that can be delivered."@en , "Plage possible de débit aéraulique pouvant être délivré. Pour les cas où il n'y a pas de débit à travers la batterie (par ex. batterie électrique en plancher), alors la valeur est zéro."@fr-FR , "送風できる風量の範囲"@ja-JP , "Plage de débit d'air pouvant être fourni."@fr-FR , "Possible range of airflow that can be delivered.  For cases where there is no airflow across the coil (e.g. electric coil in a floor slab), then the value is zero."@en ;
        rdfs:label             "PlageDébitAéraulique"@fr-FR , "風量範囲"@ja-JP , "Domaine de débit d'air"@fr-FR , "airflowRateRange"@en ;
        schema:domainIncludes  <https://w3id.org/product/CooledBeam#ACTIVE> , <https://w3id.org/product/AirTerminalBox> , <https://w3id.org/product/Coil> .

props:primarySurfaceArea
        a                      owl:DatatypeProperty ;
        rdfs:comment           "Primary heat transfer surface area of the tubes and headers."@en , "Surface d'échange thermique au primaire des tubes et aux collecteurs."@fr-FR ;
        rdfs:label             "primarySurfaceArea"@en , "SurfaceEchangePrimaire"@fr-FR ;
        rdfs:range             <https://w3id.org/measurement/area> ;
        schema:domainIncludes  <https://w3id.org/product/Coil> .

props:nominalSurroundingTemperatureCooling
        a                      owl:DatatypeProperty ;
        rdfs:comment           "Nominal surrounding temperature (refers to nominal cooling capacity)."@en ;
        rdfs:label             "nominalSurroundingTemperatureCooling"@en ;
        rdfs:range             <https://w3id.org/measurement/thermodynamicTemperature> ;
        schema:domainIncludes  <https://w3id.org/product/CooledBeam> .

props:nominalHeatTransferArea
        a                      owl:DatatypeProperty ;
        rdfs:comment           "Nominal heat transfer surface area associated with nominal overall heat transfer coefficient."@en ;
        rdfs:label             "nominalHeatTransferArea"@en ;
        rdfs:range             <https://w3id.org/measurement/area> ;
        schema:domainIncludes  <https://w3id.org/product/Condenser> .

props:numberOfParallelCircuits
        a                      owl:DatatypeProperty ;
        rdfs:comment           "Number of parallel circuits."@en ;
        rdfs:label             "numberOfParallelCircuits"@en ;
        rdfs:range             xsd:int ;
        schema:domainIncludes  <https://w3id.org/product/CableSegment> .

props:category  a              owl:DatatypeProperty ;
        rdfs:comment           "Designation of the category into which the actors in the population belong."@en , "母集団の中の関与者のカテゴリー（部門・分野）の指定。"@ja-JP , "该组参与者所属的类别。"@zh-CN ;
        rdfs:label             "category"@en , "部門"@ja-JP , "类别"@zh-CN ;
        rdfs:range             xsd:string ;
        schema:domainIncludes  <https://w3id.org/product/Actor> .

props:waterPressureRange
        rdfs:comment           "Allowable water circuit working pressure range."@en ;
        rdfs:label             "waterPressureRange"@en ;
        schema:domainIncludes  <https://w3id.org/product/CooledBeam> .

props:slope  a                 owl:DatatypeProperty ;
        rdfs:comment           "傾斜角度。水平を0度とする。"@ja-JP , "傾斜角度。水平を0度とする。\n\nその形状（傾斜梁）情報は、表示のための形状に内部で使用される幾何学的パラメータを加えて提供される。形状情報と内部の幾何学的パラメータに矛盾が生じた場合は、幾何学的パラメータが優先される。幾何学的パラメ－タ編集アプリケーションでは、CADと同様に、この値は書き込み専用とする。"@ja-JP , "Slope angle - relative to horizontal (0.0 degrees).\n\nThe shape information is provided in addition to the shape representation and the geometric parameters used within. In cases of inconsistency between the geometric parameters and the shape properties, provided in the attached property, the geometric parameters take precedence.   For geometry editing applications, like CAD: this value should be write-only."@en , "Angle d'inclinaison avec l'horizontale (0 degrés). Cette propriété  est donnée en complément de la représentation de la forme et des paramètres géométriques qui la déterminent. En cas d'incohérence entre ces paramètres géométriques et cette propriété, ce sont les paramètres géométriques qui priment. Les applications qui déterminent la géométrie comme les logiciels de CAO ne doivent pas autoriser la modification de cette propriété"@fr-FR , "Angle d'inclinaison avec l'horizontale (0 degrés). Cette propriété est donnée en complément de la représentation de la forme et des paramètres géométriques qui la déterminent. En cas d'incohérence entre ces paramètres géométriques et cette propriété, ce sont les paramètres géométriques qui priment."@fr-FR , "相对于水平（0.0度）方向的坡度角。\n该属性所提供的形状信息是对内部形状描述和几何参数的补充。如果几何参数与该属性所提供的形状属性不符，应以几何参数为准。对CAD等几何编辑程序，该属性应为只写类型。"@zh-CN , "Slope angle - relative to horizontal (0.0 degrees).\n\nThe shape information is provided in addition to the shape representation and the geometric parameters used within. In cases of inconsistency between the geometric parameters and the shape properties, provided in the attached property, the geometric parameters take precedence.  For geometry editing applications, like CAD: this value should be write-only."@en , "Neigungswinkel des Balkens relative zur Horizontalen (0 Grad).\n\nDieser Parameter wird zusätzlich zur geometrischen Repräsentation bereitgestellt. Im Fall der Inkonsistenz zwischen dem Parameter und der Geometrie hat die geometrische Repräsention Priorität. Dieser Parameter ist für CAD Software write-only."@de-DE , "Neigungswinkel der Stütze relative zur Horizontalen (0 Grad).\n\nDieser Parameter wird zusätzlich zur geometrischen Repräsentation bereitgestellt. Im Fall der Inkonsistenz zwischen dem Parameter und der Geometrie hat die geometrische Repräsention Priorität. Dieser Parameter ist für CAD Software write-only."@de-DE ;
        rdfs:label             "Neigungswinkel"@de-DE , "slope"@en , "Inclinaison"@fr-FR , "傾斜"@ja-JP , "坡度"@zh-CN ;
        rdfs:range             <https://w3id.org/measurement/planeAngle> ;
        schema:domainIncludes  <https://w3id.org/product/Beam> , <https://w3id.org/product/Column> .

props:openPressureDrop
        a                      owl:DatatypeProperty ;
        rdfs:comment           "Total pressure drop across damper."@en ;
        rdfs:label             "openPressureDrop"@en ;
        rdfs:range             <https://w3id.org/measurement/pressure> ;
        schema:domainIncludes  <https://w3id.org/product/Damper> .

props:receiverType  rdfs:comment  "Indicates the type of receiver."@en , "受信機の形式を示す。"@ja-JP , "수신기의 형식을 보여준다."@ko-KR ;
        rdfs:label             "receiverType"@en , "受信機形式"@ja-JP , "수신기 형식"@ko-KR ;
        schema:domainIncludes  <https://w3id.org/product/AudioVisualAppliance#RECEIVER> .

props:position  a              owl:DatatypeProperty ;
        rdfs:comment           "해당 프로젝트에서 사용이 유형에 대한 참조 ID (예 : 'A-1') ※ 기본이있는 경우 그 기호를 사용"@ko-KR , "アクチュエータの時間ごとの位置を示す値。0.0が完全に閉じられた状態で、1.0が完全に開いた状態。"@ja-JP , "Indicates position of the actuator over time where 0.0 is fully closed and 1.0 is fully open."@en ;
        rdfs:label             "참조 ID"@ko-KR , "position"@en , "位置"@ja-JP ;
        rdfs:range             <https://w3id.org/product/TimeSeries> ;
        rdfs:range             [ owl:allValuesFrom  <https://w3id.org/measurement/normalisedRatio> ;
                                 owl:onProperty     <https://w3id.org/measurement/seriesOf>
                               ] ;
        schema:domainIncludes  <https://w3id.org/product/Actuator> .

props:manualOverride  a        owl:DatatypeProperty ;
        rdfs:comment           "Identifies whether hand-operated operation is provided as an override (= TRUE) or not (= FALSE). Note that this value should be set to FALSE by default in the case of a Hand Operated Actuator."@en , "オーバーライド機能として手動操作が提供されるか (= TRUE) 、否か （= FALSE)を識別する。手動で操作するアクチュエータの場合は、この値をデフォルトとしてFALSEに設定する必要があるので注意すること。"@ja-JP ;
        rdfs:label             "manualOverride"@en , "オーバーライド機能の有無"@ja-JP ;
        rdfs:range             xsd:boolean ;
        schema:domainIncludes  <https://w3id.org/product/Actuator> .

props:cameraType  rdfs:comment  "Indicates the type of camera."@en , "カメラの形式を示す。"@ja-JP , "카메라의 형식을 보여준다."@ko-KR ;
        rdfs:label             "cameraType"@en , "カメラ形式"@ja-JP , "카메라 형식"@ko-KR ;
        schema:domainIncludes  <https://w3id.org/product/AudioVisualAppliance#CAMERA> .

props:torque  a                owl:DatatypeProperty ;
        rdfs:comment           "Indicates the maximum close-off torque for the actuator."@en , "アクチュエータの最大締め切りトルクを示す。"@ja-JP , "액츄에이터의 최대 마감 토크를 나타낸다."@ko-KR ;
        rdfs:label             "torque"@en , "最大トルク"@ja-JP , "최대 토크"@ko-KR ;
        rdfs:range             <https://w3id.org/measurement/torque> ;
        schema:domainIncludes  <https://w3id.org/product/Actuator> .

props:speakerMounting
        rdfs:comment           "Indicates how the speaker is designed to be mounted."@en , "取付可能な方法を示す。"@ja-JP , "붙일 수있는 방법을 보여준다."@ko-KR ;
        rdfs:label             "speakerMounting"@en , "取付可能方法"@ja-JP , "설치 가능 방법"@ko-KR ;
        schema:domainIncludes  <https://w3id.org/product/AudioVisualAppliance#SPEAKER> .

props:frameDepth  a            owl:DatatypeProperty ;
        rdfs:comment           "The length (or depth) of the damper frame."@en ;
        rdfs:label             "frameDepth"@en ;
        rdfs:range             <https://w3id.org/measurement/positiveLength> ;
        schema:domainIncludes  <https://w3id.org/product/Damper> .

props:isFreeHanging  a         owl:DatatypeProperty ;
        rdfs:comment           "Is it free hanging type (not mounted in a false ceiling)?"@en ;
        rdfs:label             "isFreeHanging"@en ;
        rdfs:range             xsd:boolean ;
        schema:domainIncludes  <https://w3id.org/product/CooledBeam> .

props:logarithmicMeanTemperatureDifference
        a                      owl:DatatypeProperty ;
        rdfs:comment           "Logarithmic mean temperature difference between refrigerant and water or air."@en ;
        rdfs:label             "logarithmicMeanTemperatureDifference"@en ;
        rdfs:range             <https://w3id.org/product/TimeSeries> ;
        rdfs:range             [ owl:allValuesFrom  <https://w3id.org/measurement/thermodynamicTemperature> ;
                                 owl:onProperty     <https://w3id.org/measurement/seriesOf>
                               ] ;
        schema:domainIncludes  <https://w3id.org/product/Condenser> .

props:condenserMeanVoidFraction
        a                      owl:DatatypeProperty ;
        rdfs:comment           "Mean void fraction in condenser."@en ;
        rdfs:label             "condenserMeanVoidFraction"@en ;
        rdfs:range             <https://w3id.org/product/TimeSeries> ;
        rdfs:range             [ owl:allValuesFrom  <https://w3id.org/measurement/normalisedRatio> ;
                                 owl:onProperty     <https://w3id.org/measurement/seriesOf>
                               ] ;
        schema:domainIncludes  <https://w3id.org/product/Condenser> .

props:humidityEffectiveness
        a                      owl:DatatypeProperty ;
        rdfs:comment           "湿度熱交換効率：\n最大可能絶対湿度変化に対する一次側絶対湿度変化の比"@ja-JP , "Efficacité sur transfert de chaleur latente: rapport entre difference de températures"@fr-FR , "Humidity heat transfer effectiveness: The ratio of primary airflow absolute humidity changes to maximum possible absolute humidity changes."@en ;
        rdfs:label             "湿度効率"@ja-JP , "humidityEffectiveness"@en , "EfficacitéLatente"@fr-FR ;
        rdfs:range             <https://w3id.org/product/TimeSeries> ;
        rdfs:range             [ owl:allValuesFrom  <https://w3id.org/measurement/normalisedRatio> ;
                                 owl:onProperty     <https://w3id.org/measurement/seriesOf>
                               ] ;
        schema:domainIncludes  <https://w3id.org/product/AirToAirHeatRecovery> .

props:airflowCurve  a          owl:DatatypeProperty ;
        rdfs:comment           "Air flowrate versus damper position relationship;airflow = f ( valve position)."@en , "ダンパ開度と風量の関係　　風量＝f(開度)"@ja-JP , "Relation entre débit d'air par rapport à la position du registre; Débit d'air = f (position du clapet)"@fr-FR ;
        rdfs:label             "airflowCurve"@en , "流量曲線"@ja-JP , "Courbe de débit d'air"@fr-FR ;
        rdfs:range             <https://w3id.org/product/TimeSeries> ;
        rdfs:range             [ owl:allValuesFrom  <https://w3id.org/measurement/volumetricFlowRate> ;
                                 owl:onProperty     <https://w3id.org/measurement/seriesOf>
                               ] ;
        schema:domainIncludes  <https://w3id.org/product/AirTerminalBox> .

props:bladeEdge  rdfs:comment  "Blade edge."@en ;
        rdfs:label             "bladeEdge"@en ;
        schema:domainIncludes  <https://w3id.org/product/Damper> .

props:accuracyQualityObtained
        a                      owl:DatatypeProperty ;
        rdfs:comment           "A measure of the accuracy quality of survey points as obtained expressed in percentage terms."@en , "Mesure de la précision obtenue des points de relevé, exprimée en pourcentage."@fr-FR ;
        rdfs:label             "accuracyQualityObtained"@en , "PrecisionObtenue"@fr-FR ;
        rdfs:range             <https://w3id.org/measurement/ratio> ;
        schema:domainIncludes  <https://w3id.org/product/Annotation#SurveyArea> .

props:nominalWidth  a          owl:DatatypeProperty ;
        rdfs:comment           "The nominal width of the segment."@en , "폭 치수"@ko-KR , "呼び幅寸法。"@ja-JP , "폭 치수."@ko-KR ;
        rdfs:label             "공칭 폭"@ko-KR , "公称幅"@ja-JP , "nominalWidth"@en ;
        rdfs:range             <https://w3id.org/measurement/positiveLength> ;
        schema:domainIncludes  <https://w3id.org/product/CableCarrierSegment#CABLETRAYSEGMENT> , <https://w3id.org/product/CableCarrierSegment#CABLELADDERSEGMENT> , <https://w3id.org/product/CableCarrierSegment#CABLETRUNKINGSEGMENT> , <https://w3id.org/product/CableCarrierSegment#CONDUITSEGMENT> .

props:infiltrationDiversitySummer
        a                      owl:DatatypeProperty ;
        rdfs:comment           "Diversity factor for Summer infiltration."@en , "夏期すき間換気率。"@ja-JP , "여름 틈새 환기 비율"@ko-KR ;
        rdfs:label             "infiltrationDiversitySummer"@en , "夏期すき間換気率"@ja-JP , "여름틈새 환기 비율"@ko-KR ;
        rdfs:range             <https://w3id.org/measurement/positiveRatio> ;
        schema:domainIncludes  bot:Zone .

props:dischargeDirection
        rdfs:comment           "Discharge direction of the air terminal.\n\nParallel: discharges parallel to mounting surface designed so that flow attaches to the surface.\nPerpendicular:  discharges away from mounting surface.\nAdjustable: both parallel and perpendicular discharge."@en , "ターミナルの吐き出し方向\n水平：取り付け面と水平に吐き出し\n垂直：取り付け面から離れた方向に吐き出し\n調節可能：水平・垂直方向両方に調整"@ja-JP , "Direction d'émission du terminal de ventilation.\n\nParallèle: émission parallèle à la surface de fixation conçu de façon à ce que le flux se colle à la surface.\nPerpendiculaire: émission s'éloignant de la surface de fixation.\nRéglable: émission parallèle et aussi s'éloignant de la surface de fixation."@fr-FR ;
        rdfs:label             "dischargeDirection"@en , "吐き出し方向"@ja-JP , "DirectionEmission"@fr-FR ;
        schema:domainIncludes  <https://w3id.org/product/AirTerminal> .

props:rentalRatesInCategoryFuture
        rdfs:comment           "Range of the cost rates for property expected to be available in the future in the required category."@en , "Prix futur des loyers pour la catégorie considérée."@fr-FR ;
        rdfs:label             "rentalRatesInCategoryFuture"@en , "PrixFuturLoyerParCategorie"@fr-FR ;
        schema:domainIncludes  <https://w3id.org/product/Building> .

props:assessmentDescription
        a                      owl:DatatypeProperty ;
        rdfs:comment           "Qualitative description of the condition."@en , "状態に関する定性的な記述。"@ja-JP ;
        rdfs:label             "assessmentDescription"@en , "評価記述"@ja-JP ;
        rdfs:range             xsd:string ;
        schema:domainIncludes  <https://w3id.org/product/Element> .

props:coilLength  a            owl:DatatypeProperty ;
        rdfs:comment           "Length of coil."@en ;
        rdfs:label             "coilLength"@en ;
        rdfs:range             <https://w3id.org/measurement/positiveLength> ;
        schema:domainIncludes  <https://w3id.org/product/CooledBeam> .

props:derivativeConstant
        a                      owl:DatatypeProperty ;
        rdfs:comment           "The derivative gain factor of the controller (usually referred to as Kd).  Asserted where ControlType is PROPORTIONALINTEGRALDERIVATIVE."@en , "미분 게인 (Kd)"@ko-KR ;
        rdfs:label             "derivativeConstant"@en , "미분 게인 (Kd)"@ko-KR ;
        rdfs:range             xsd:decimal ;
        schema:domainIncludes  <https://w3id.org/product/Controller#PROPORTIONAL> .

props:lubricantPumpHeatGain
        a                      owl:DatatypeProperty ;
        rdfs:comment           "Lubricant pump heat gain."@en , "Gain thermique par lubrification de la pompe à chaleur."@fr-FR ;
        rdfs:label             "lubricantPumpHeatGain"@en , "GainThermiqueLubrifiantPompe"@fr-FR ;
        rdfs:range             <https://w3id.org/product/TimeSeries> ;
        rdfs:range             [ owl:allValuesFrom  <https://w3id.org/measurement/power> ;
                                 owl:onProperty     <https://w3id.org/measurement/seriesOf>
                               ] ;
        schema:domainIncludes  <https://w3id.org/product/Compressor> .

props:narrativeText  a         owl:DatatypeProperty ;
        rdfs:comment           "Information sur l'usage des bâtiments voisins"@fr-FR , "Added information relating to the adjacent building use that is not appropriate to the general descriptive text associated with an entity through the inherited IfcRoot.Description."@en , "Information relative aux bâtiments voisins qui n'est pas appropriée au texte d'ordre général que l'on peut saisir dans l'attribut hérité IfcRoot.Description."@fr-FR ;
        rdfs:label             "CommentaireUsage"@fr-FR , "narrativeText"@en , "TexteLibre"@fr-FR ;
        rdfs:range             xsd:string ;
        schema:domainIncludes  <https://w3id.org/product/Building> .

props:coolingTemperatureDelta
        a                      owl:DatatypeProperty ;
        rdfs:comment           "Cooling temperature difference for calculating space air flow rates."@en , "空調送風量計算用の冷房給気温度差。"@ja-JP , "에어컨 송풍 량 계산을위한 냉방 급기 온도차"@ko-KR ;
        rdfs:label             "coolingTemperatureDelta"@en , "冷房時送風温度差"@ja-JP , "냉방시 돌풍 온도차"@ko-KR ;
        rdfs:range             <https://w3id.org/measurement/thermodynamicTemperature> ;
        schema:domainIncludes  bot:Zone .

props:scheduleWork  a          owl:DatatypeProperty ;
        rdfs:comment           "The scheduled work on behalf of the resource allocation."@en , "資源配分のための予定された作業。"@ja-JP ;
        rdfs:label             "scheduleWork"@en , "予定作業時間"@ja-JP ;
        rdfs:range             <https://w3id.org/product/TimeSeries> ;
        rdfs:range             [ owl:allValuesFrom  xsd:duration ;
                                 owl:onProperty     <https://w3id.org/measurement/seriesOf>
                               ] ;
        schema:domainIncludes  <https://w3id.org/product/ConstructionResource> .

props:screenDiameter  a        owl:DatatypeProperty ;
        rdfs:comment           "遮へい層の径、厚さ。"@ja-JP , "The diameter of the screen around a cable or bus segment (if present)."@en , "코어 부분 (있는 경우)의 측면에 지름."@ko-KR , "The diameter of the screen around a core segment (if present)."@en , "차폐 층의 직경, 두께."@ko-KR , "コア部分（存在する場合）の面の直径。"@ja-JP ;
        rdfs:label             "스크린 지름"@ko-KR , "screenDiameter"@en , "スクリーン径"@ja-JP , "실드 직경"@ko-KR , "シールド径"@ja-JP ;
        rdfs:range             <https://w3id.org/measurement/positiveLength> ;
        schema:domainIncludes  <https://w3id.org/product/CableSegment#CABLESEGMENT> , <https://w3id.org/product/CableSegment#CORESEGMENT> .

props:uAcurves  a              owl:ObjectProperty ;
        rdfs:comment           "UV = f (VExterior, VInterior), UV as a function of interior and exterior fluid flow velocity at the entrance."@en ;
        rdfs:label             "uAcurves"@en ;
        rdfs:range             <https://w3id.org/measurement/TimeSeries> ;
        schema:domainIncludes  <https://w3id.org/product/Condenser> .

props:flowControlType
        rdfs:comment           "Type of flow control element that may be included as a part of the construction of the air terminal."@en , "ターミナルの構成の一部として含まれる流量制御の形式\n（ダンパー、ベローズ、無し…）"@ja-JP , "Nature de la commande de flux d'un élément qui pourrait être inclus en tant que tel dans le terminal de ventilation."@fr-FR ;
        rdfs:label             "flowControlType"@en , "流量制御形式"@ja-JP , "NatureCommandeFlux"@fr-FR ;
        schema:domainIncludes  <https://w3id.org/product/AirTerminal> .

props:returnWaterTemperatureCooling
        a                      owl:DatatypeProperty ;
        rdfs:comment           "Return water temperature in cooling mode."@en ;
        rdfs:label             "returnWaterTemperatureCooling"@en ;
        rdfs:range             <https://w3id.org/product/TimeSeries> ;
        rdfs:range             [ owl:allValuesFrom  <https://w3id.org/measurement/thermodynamicTemperature> ;
                                 owl:onProperty     <https://w3id.org/measurement/seriesOf>
                               ] ;
        schema:domainIncludes  <https://w3id.org/product/CooledBeam> .

props:totalHeatTransferRate
        a                      owl:DatatypeProperty ;
        rdfs:comment           "Puissance thermique totale"@fr-FR , "Total heat transfer rate."@en , "全熱交換量"@ja-JP ;
        rdfs:label             "totalHeatTransferRate"@en , "PuissanceThermiqueTotale"@fr-FR , "全熱交換量"@ja-JP ;
        rdfs:range             <https://w3id.org/product/TimeSeries> ;
        rdfs:range             [ owl:allValuesFrom  <https://w3id.org/measurement/power> ;
                                 owl:onProperty     <https://w3id.org/measurement/seriesOf>
                               ] ;
        schema:domainIncludes  <https://w3id.org/product/AirToAirHeatRecovery> .

props:finish  a                owl:DatatypeProperty ;
        rdfs:comment           "该构件的表面处理方式。仅供参考。"@zh-CN , "Finish selection for this object.\nHere specification of the surface finish for informational purposes."@en , "仕上げ選択に関する情報。表面仕上げに関する仕様。"@ja-JP , "Oberflächenbehandlung oder Oberflächengüte, wie \"poliert\", \"schalungsrau\", imprägniert."@de-DE , "Finition de cet objet. Spécification de la finition donnée à titre informatif."@fr-FR ;
        rdfs:label             "Finition"@fr-FR , "表面处理"@zh-CN , "仕上げ"@ja-JP , "Oberflächengüte"@de-DE , "finish"@en ;
        rdfs:range             xsd:string ;
        schema:domainIncludes  <https://w3id.org/product/Covering> .

props:mediaContent  a          owl:DatatypeProperty ;
        rdfs:comment           "Indicates the media content storage location, such as URLs to camera footage within particular time periods."@en ;
        rdfs:label             "mediaContent"@en ;
        rdfs:range             <https://w3id.org/product/TimeSeries> ;
        rdfs:range             [ owl:allValuesFrom  xsd:string ;
                                 owl:onProperty     <https://w3id.org/measurement/seriesOf>
                               ] ;
        schema:domainIncludes  <https://w3id.org/product/AudioVisualAppliance> .

props:beamHeatingCapacity
        a                      owl:DatatypeProperty ;
        rdfs:comment           "Heating capacity of beam. This excludes heating capacity of supply air."@en ;
        rdfs:label             "beamHeatingCapacity"@en ;
        rdfs:range             <https://w3id.org/product/TimeSeries> ;
        rdfs:range             [ owl:allValuesFrom  <https://w3id.org/measurement/power> ;
                                 owl:onProperty     <https://w3id.org/measurement/seriesOf>
                               ] ;
        schema:domainIncludes  <https://w3id.org/product/CooledBeam> .

props:totalEffectiveness
        a                      owl:DatatypeProperty ;
        rdfs:comment           "Rendement thermique: rapport entre la chaleur effective échangée et l'échange maximum possible."@fr-FR , "Total heat transfer effectiveness: The ratio of heat transfer to the maximum possible heat transfer."@en , "全熱効率\n最大可能熱交換に対する熱交換の比率"@ja-JP ;
        rdfs:label             "全熱効率"@ja-JP , "totalEffectiveness"@en , "Rendement thermique"@fr-FR ;
        rdfs:range             <https://w3id.org/product/TimeSeries> ;
        rdfs:range             [ owl:allValuesFrom  <https://w3id.org/measurement/normalisedRatio> ;
                                 owl:onProperty     <https://w3id.org/measurement/seriesOf>
                               ] ;
        schema:domainIncludes  <https://w3id.org/product/AirToAirHeatRecovery> .

props:inputPressure  a         owl:DatatypeProperty ;
        rdfs:comment           "アクチュエータへの最大設計圧力。"@ja-JP , "Maximum input control air pressure requirement."@en , "Maximum design pressure for the actuator."@en , "최대 제어 공압"@ko-KR , "最大制御空気圧。"@ja-JP , "액츄에이터의 최대 설계 압력"@ko-KR ;
        rdfs:label             "inputPressure"@en , "入力圧力"@ja-JP , "입력 압력"@ko-KR ;
        rdfs:range             <https://w3id.org/measurement/pressure> ;
        schema:domainIncludes  <https://w3id.org/product/Actuator#HYDRAULICACTUATOR> , <https://w3id.org/product/Actuator#PNEUMATICACTUATOR> .

props:effectiveArea  a         owl:DatatypeProperty ;
        rdfs:comment           "Effective discharge area of the air terminal."@en , "ターミナルの有効吹き出し範囲"@ja-JP , "Zone d'émission efficace du terminal de ventilation."@fr-FR ;
        rdfs:label             "effectiveArea"@en , "有効面積"@ja-JP , "ZoneEfficace"@fr-FR ;
        rdfs:range             <https://w3id.org/measurement/area> ;
        schema:domainIncludes  <https://w3id.org/product/AirTerminal> .

props:span  a                  owl:DatatypeProperty ;
        rdfs:comment           "Portée libre de la poutre. Cette propriété  est donnée en complément de la représentation de la forme et des paramètres géométriques qui la déterminent. En cas d'incohérence entre ces paramètres géométriques et cette propriété, ce sont les paramètres géométriques qui priment. Les applications qui déterminent la géométrie comme les logiciels de CAO ne doivent pas autoriser la modification de cette propriété."@fr-FR , "Clear span for this object.\n\nThe shape information is provided in addition to the shape representation and the geometric parameters used within. In cases of inconsistency between the geometric parameters and the shape properties, provided in the attached property, the geometric parameters take precedence. For geometry editing applications, like CAD: this value should be write-only."@en , "该对象的净跨度。\n该属性所提供的形状信息是对内部形状描述和几何参数的补充。如果几何参数与该属性所提供的形状属性不符，应以几何参数为准。对CAD等几何编辑程序，该属性应为只写类型。"@zh-CN , "Lichte Spannweite des Balkens für die statische Anforderung,\n\nDieser Parameter wird zusätzlich zur geometrischen Repräsentation bereitgestellt. Im Fall der Inkonsistenz zwischen dem Parameter und der Geometrie hat die geometrische Repräsention Priorität. Dieser Parameter ist für CAD Software write-only."@de-DE , "このオブジェクトの全長。\n\nその形状（オブジェクトの全長）情報は、表示のための形状に内部で使用される幾何学的パラメータを加えて提供される。形状情報と内部の幾何学的パラメータに矛盾が生じた場合は、幾何学的パラメータが優先される。幾何学的パラメ－タ編集アプリケーションでは、CADと同様に、この値は書き込み専用とする。"@ja-JP ;
        rdfs:label             "全長"@ja-JP , "跨度"@zh-CN , "span"@en , "Spannweite"@de-DE , "PorteeLibre"@fr-FR ;
        rdfs:range             <https://w3id.org/measurement/positiveLength> ;
        schema:domainIncludes  <https://w3id.org/product/Beam> .

props:heatTransferCoefficient
        a                      owl:ObjectProperty ;
        rdfs:comment           "Heat transfer coefficient-area product."@en ;
        rdfs:label             "heatTransferCoefficient"@en ;
        rdfs:range             <https://w3id.org/measurement/TimeSeries> ;
        schema:domainIncludes  <https://w3id.org/product/CoolingTower> .

props:energySource  rdfs:comment  "Enumeration defining the energy source or fuel cumbusted to generate heat."@en , "加熱に使用する燃料のエネルギ種類　（石炭、石炭粉末、電気、ガス、油、プロパン、木材、木材チップ、木材ペレット、木粉、他）"@ja-JP , "Liste définissant les sources d'énergie ou combustibles pour générer la chaleur."@fr-FR ;
        rdfs:label             "エネルギ源"@ja-JP , "energySource"@en , "エネルギ種別"@ja-JP , "SourceEnergie"@fr-FR ;
        schema:domainIncludes  <https://w3id.org/product/Burner> , <https://w3id.org/product/Boiler> .

props:labels  rdfs:comment     "Table mapping values to labels, where such labels indicate the meanings of True and False, such as 'Open' and 'Closed'"@en , "Table mapping values to labels, where each entry corresponds to an integer within the ValueRange."@en , "Table mapping values to labels, where such labels indicate transition points such as 'Hi', 'Lo', 'HiHi', or 'LoLo'."@en ;
        rdfs:label             "labels"@en ;
        schema:domainIncludes  <https://w3id.org/product/Controller#TWOPOSITION> , <https://w3id.org/product/Controller#PROPORTIONAL> , <https://w3id.org/product/Controller#MULTIPOSITION> , <https://w3id.org/product/Controller#FLOATING> .

props:energySourceConsumption
        a                      owl:DatatypeProperty ;
        rdfs:comment           "Consommation d'énergie."@fr-FR , "Energy consumption."@en , "エネルギ消費量"@ja-JP ;
        rdfs:label             "エネルギ消費量"@ja-JP , "ConsommationSourceEnergie."@fr-FR , "energySourceConsumption"@en ;
        rdfs:range             <https://w3id.org/product/TimeSeries> ;
        rdfs:range             [ owl:allValuesFrom  <https://w3id.org/measurement/energy> ;
                                 owl:onProperty     <https://w3id.org/measurement/seriesOf>
                               ] ;
        schema:domainIncludes  <https://w3id.org/product/Boiler> .

props:brightness  a            owl:DatatypeProperty ;
        rdfs:comment           "Indicates the display brightness."@en , "明るさ示す。"@ja-JP , "밝기 보여준다"@ko-KR ;
        rdfs:label             "brightness"@en , "明るさ"@ja-JP , "밝기"@ko-KR ;
        rdfs:range             <https://w3id.org/measurement/illuminance> ;
        schema:domainIncludes  <https://w3id.org/product/AudioVisualAppliance#DISPLAY> .

props:bladeShape  rdfs:comment  "Blade shape. Flat means triple V-groove."@en ;
        rdfs:label             "bladeShape"@en ;
        schema:domainIncludes  <https://w3id.org/product/Damper> .

props:infiltrationDiversityWinter
        a                      owl:DatatypeProperty ;
        rdfs:comment           "Diversity factor for Winter infiltration."@en , "冬期すき間換気率。"@ja-JP , "겨울철 틈새 환기 비율"@ko-KR ;
        rdfs:label             "infiltrationDiversityWinter"@en , "冬期すき間換気率"@ja-JP , "겨울철 틈새 환기 비율"@ko-KR ;
        rdfs:range             <https://w3id.org/measurement/positiveRatio> ;
        schema:domainIncludes  bot:Zone .

props:latentHeatTransferRate
        a                      owl:DatatypeProperty ;
        rdfs:comment           "潜熱交換量"@ja-JP , "Puissance thermique latente"@fr-FR , "Latent heat transfer rate."@en ;
        rdfs:label             "latentHeatTransferRate"@en , "潜熱交換量"@ja-JP , "PuissanceThermiqueLatente"@fr-FR ;
        rdfs:range             <https://w3id.org/product/TimeSeries> ;
        rdfs:range             [ owl:allValuesFrom  <https://w3id.org/measurement/power> ;
                                 owl:onProperty     <https://w3id.org/measurement/seriesOf>
                               ] ;
        schema:domainIncludes  <https://w3id.org/product/AirToAirHeatRecovery> .

props:nominalHeight  a         owl:DatatypeProperty ;
        rdfs:comment           "The nominal height of the segment."@en , "呼び高寸法。"@ja-JP , "고 치수"@ko-KR , "고치수"@ko-KR ;
        rdfs:label             "공칭높이"@ko-KR , "공칭 높이"@ko-KR , "公称高"@ja-JP , "nominalHeight"@en ;
        rdfs:range             <https://w3id.org/measurement/positiveLength> ;
        schema:domainIncludes  <https://w3id.org/product/CableCarrierSegment#CABLELADDERSEGMENT> , <https://w3id.org/product/CableCarrierSegment#CONDUITSEGMENT> , <https://w3id.org/product/CableCarrierSegment#CABLETRAYSEGMENT> , <https://w3id.org/product/CableCarrierSegment#CABLETRUNKINGSEGMENT> .

props:nominalLatentCapacity
        a                      owl:DatatypeProperty ;
        rdfs:comment           "Nominal latent capacity."@en , "Puissance latente nominale."@fr-FR ;
        rdfs:label             "nominalLatentCapacity"@en , "PuissanceLatenteNominale"@fr-FR ;
        rdfs:range             <https://w3id.org/measurement/power> ;
        schema:domainIncludes  <https://w3id.org/product/Coil> .

props:requestSourceLabel
        a                      owl:DatatypeProperty ;
        rdfs:comment           "A specific name or label that further qualifies the identity of a request source. In the event of an email, this may be the email address."@en , "要請がなされる源のあらかじめ定義されたタイプの識別子。"@ja-JP ;
        rdfs:label             "requestSourceLabel"@en , "要請ソースタイプ"@ja-JP ;
        rdfs:range             xsd:string ;
        schema:domainIncludes  <https://w3id.org/product/ActionRequest> .

props:tileLength  a            owl:DatatypeProperty ;
        rdfs:comment           "天花板面砖的长度。\n该属性所提供的尺寸信息是对内部形状描述和几何参数的补充。如果几何参数与该属性所提供的尺寸属性不符，应以几何参数为准。"@zh-CN , "Length of ceiling tiles. The size information is provided in addition to the shape representation and the geometric parameters used within. In cases of inconsistency between the geometric parameters and the size properties, provided in the attached property set, the geometric parameters take precedence."@en , "Longueur des carreaux de plafond. Cette propriété est donnée en complément de la représentation de la forme et des paramètres géométriques qui la déterminent. En cas d'incohérence entre ces paramètres géométriques et cette propriété, ce sont les paramètres géométriques qui priment."@fr-FR , "Länge der Unterdeckenplatten, oder -panele, die zur Verkleidung verwendet werden."@de-DE ;
        rdfs:label             "Deckenplattenlänge"@de-DE , "面砖长度"@zh-CN , "Longueur des carreaux"@fr-FR , "tileLength"@en ;
        rdfs:range             <https://w3id.org/measurement/positiveLength> ;
        schema:domainIncludes  <https://w3id.org/product/Covering#CEILING> .

props:nominalReturnWaterTemperatureHeating
        a                      owl:DatatypeProperty ;
        rdfs:comment           "Nominal return water temperature (refers to nominal heating capacity)."@en ;
        rdfs:label             "nominalReturnWaterTemperatureHeating"@en ;
        rdfs:range             <https://w3id.org/measurement/thermodynamicTemperature> ;
        schema:domainIncludes  <https://w3id.org/product/CooledBeam> .

props:visibleAngleRight
        a                      owl:DatatypeProperty ;
        rdfs:comment           "Angle of visibility to the right of the access."@en , "Angle de visibilité à la droite de l'accès."@fr-FR , "右側の経路に可視出来る角度。"@ja-JP ;
        rdfs:label             "visibleAngleRight"@en , "VisibiliteAngleDroit"@fr-FR , "右側可視角度"@ja-JP ;
        rdfs:range             <https://w3id.org/measurement/positivePlaneAngle> ;
        schema:domainIncludes  <https://w3id.org/product/Annotation#LineOfSight> .

props:sprinklerProtectionAutomatic
        a                      owl:DatatypeProperty ;
        rdfs:comment           "Indication whether this object has an automatic sprinkler protection (TRUE) or not (FALSE)."@en , "스프링 클러 설비가 자동 여부를 나타내는 값"@ko-KR , "Indication whether this object has an automatic sprinkler protection (TRUE) or not (FALSE).\nIt should only be given, if the property \"SprinklerProtection\" is set to TRUE."@en , "Indication selon laquelle ce bâtiment bénéficie d'une protection automatique par sprinkler (VRAI) ou non (FAUX)."@fr-FR , "Indication selon laquelle ce bâtiment bénéficie d'une protection automatique par sprinkler (VRAI) ou non (FAUX). Indication à ne fournir que si la propriété \"SprinklerProtection\" est cochée \"VRAI\"."@fr-FR , "Angabe, ob das Geschoss durch eine automatische Sprinkleranlage geschützt wird (WAHR) oder nicht (FALSCH)."@de-DE , "Angabe, ob das Gebäude durch eine automatische Sprinkleranlage geschützt wird (WAHR) oder nicht (FALSCH)."@de-DE , "スプリンクラー設備が自動かどうか示すブーリアン値。"@ja-JP ;
        rdfs:label             "스프링 클러 방어 자동 구분"@ko-KR , "sprinklerProtectionAutomatic"@en , "Sprinklerschutz automatisch"@de-DE , "スプリンクラー防御自動区分"@ja-JP , "ProtectionAutomatiqueParSprinkler"@fr-FR ;
        rdfs:range             xsd:boolean ;
        schema:domainIncludes  <https://w3id.org/product/Building> , <https://w3id.org/product/BuildingStorey> .

props:videoResolutionWidth
        a                      owl:DatatypeProperty ;
        rdfs:comment           "水平方向のピクセル数。"@ja-JP , "水平方向のピクセル数を示す。"@ja-JP , "가로 픽셀 수입니다."@ko-KR , "가로 픽셀 수를 나타낸다."@ko-KR , "Indicates the number of horizontal pixels, e.g. 1920."@en , "Indicates the number of horizontal pixels (the largest native video resolution width)."@en ;
        rdfs:label             "videoResolutionWidth"@en , "水平解像度"@ja-JP , "수평 해상도"@ko-KR ;
        rdfs:range             xsd:int ;
        schema:domainIncludes  <https://w3id.org/product/AudioVisualAppliance#PROJECTOR> , <https://w3id.org/product/AudioVisualAppliance#DISPLAY> , <https://w3id.org/product/AudioVisualAppliance#CAMERA> .

props:ambientDesignWetBulbTemperature
        a                      owl:DatatypeProperty ;
        rdfs:comment           "Ambient design wet bulb temperature used for selecting the cooling tower."@en ;
        rdfs:label             "ambientDesignWetBulbTemperature"@en ;
        rdfs:range             <https://w3id.org/measurement/thermodynamicTemperature> ;
        schema:domainIncludes  <https://w3id.org/product/CoolingTower> .

props:totalHeatingCapacity
        a                      owl:DatatypeProperty ;
        rdfs:comment           "Total heating capacity. This includes heating capacity of beam and heating capacity of supply air."@en ;
        rdfs:label             "totalHeatingCapacity"@en ;
        rdfs:range             <https://w3id.org/product/TimeSeries> ;
        rdfs:range             [ owl:allValuesFrom  <https://w3id.org/measurement/power> ;
                                 owl:onProperty     <https://w3id.org/measurement/seriesOf>
                               ] ;
        schema:domainIncludes  <https://w3id.org/product/CooledBeam> .

props:airFlowrateVersusFlowControlElement
        rdfs:comment           "Air flowrate versus flow control element position at nominal pressure drop."@en , "標準の圧力低下における流量制御装置の位置に対する流量"@ja-JP , "Débit d'air par rapport à la position de l'élément de contrôle du flux en perte de charge nominale"@fr-FR ;
        rdfs:label             "airFlowrateVersusFlowControlElement"@en , "流量制御特性"@ja-JP , "DébitAirContreElementControleFlux"@fr-FR ;
        schema:domainIncludes  <https://w3id.org/product/AirTerminal> .

props:bypassFactor  a          owl:DatatypeProperty ;
        rdfs:comment           "Fraction of air that is bypassed by the coil (0-1)."@en , "Fraction de l'air qui est bypassé par la batterie (0 à 1)."@fr-FR ;
        rdfs:label             "bypassFactor"@en , "FacteurBypass"@fr-FR ;
        rdfs:range             <https://w3id.org/measurement/normalisedRatio> ;
        schema:domainIncludes  <https://w3id.org/product/Coil> .

props:coilCoolant  rdfs:comment  "The fluid used for heating or cooling used by the hydronic coil."@en , "Le fluide utilisé pour chauffer ou refroidir dans la batterie deux tubes."@fr-FR ;
        rdfs:label             "coilCoolant"@en , "RefrigerantBatterie"@fr-FR ;
        schema:domainIncludes  <https://w3id.org/product/Coil> .

props:outletTemperatureRange
        rdfs:comment           "Allowable outlet temperature of either the water or the steam."@en , "水または蒸気のどちらかの許容出口温度"@ja-JP , "Température admissible de sortie de l'eau ou de la vapeur"@fr-FR ;
        rdfs:label             "outletTemperatureRange"@en , "出口温度範囲"@ja-JP , "PlageTempératureSortie"@fr-FR ;
        schema:domainIncludes  <https://w3id.org/product/Boiler> .

props:nominalCapacity
        a                      owl:DatatypeProperty ;
        rdfs:comment           "Compressor nameplate capacity."@en , "Nominal cooling tower capacity in terms of heat transfer rate of the cooling tower between air stream and water stream at nominal conditions."@en , "Puissance froid nominale du groupe froid aux conditions standardisées telles que définies par l'organisation faisant autorité."@fr-FR , "Nominal cooling capacity of chiller at standardized conditions as defined by the agency having jurisdiction."@en , "Puissance du compresseur au niveau de sa plaque."@fr-FR ;
        rdfs:label             "PuissanceCompresseur"@fr-FR , "nominalCapacity"@en , "PuissanceNominale"@fr-FR ;
        rdfs:range             <https://w3id.org/measurement/power> ;
        schema:domainIncludes  <https://w3id.org/product/Chiller> , <https://w3id.org/product/CoolingTower> , <https://w3id.org/product/Compressor> .

props:throwLength  a           owl:DatatypeProperty ;
        rdfs:comment           "The horizontal or vertical axial distance an airstream travels after leaving an AirTerminal before the maximum stream velocity is reduced to a specified terminal velocity under isothermal conditions at the upper value of the AirFlowrateRange."@en , "ターミナルからの水平または垂直の到達距離\n流量範囲の最大値での吐き出し速度が設定された流速に減速するまでの上限値"@ja-JP , "La distance axiale horizontale ou verticale un jet d'air parcourt après avoir quitté un terminal de ventilation avant que la vittesse d'éjection maximale est réduite à une vitessedu terminal spécifique dans des conditions isothermes pour la valeur la plus élevée de la plage de débit d'air."@fr-FR ;
        rdfs:label             "throwLength"@en , "到達距離"@ja-JP , "Longueur de jet"@fr-FR ;
        rdfs:range             <https://w3id.org/measurement/length> ;
        schema:domainIncludes  <https://w3id.org/product/AirTerminal> .

props:combustionEfficiency
        a                      owl:DatatypeProperty ;
        rdfs:comment           "Efficacité de la combustion sous conditions nominales."@fr-FR , "設計条件での燃焼効率"@ja-JP , "Combustion efficiency under nominal condition."@en ;
        rdfs:label             "combustionEfficiency"@en , "燃焼効率"@ja-JP , "EfficacitéCombustion"@fr-FR ;
        rdfs:range             <https://w3id.org/product/TimeSeries> ;
        rdfs:range             [ owl:allValuesFrom  <https://w3id.org/measurement/normalisedRatio> ;
                                 owl:onProperty     <https://w3id.org/measurement/seriesOf>
                               ] ;
        schema:domainIncludes  <https://w3id.org/product/Boiler> .

props:polarity  a              owl:DatatypeProperty ;
        rdfs:comment           "True indicates normal polarity; False indicates reverse polarity."@en ;
        rdfs:label             "polarity"@en ;
        rdfs:range             xsd:boolean ;
        schema:domainIncludes  <https://w3id.org/product/Controller#TWOPOSITION> .

props:hasHotGasBypass
        a                      owl:DatatypeProperty ;
        rdfs:comment           "Whether or not hot gas bypass is provided for the compressor. TRUE = Yes, FALSE = No."@en , "Qu'il y ait ou non un bypass du gaz chaud fourni au niveau du compresseur, VRAI= oui, FAUX= Non."@fr-FR ;
        rdfs:label             "hasHotGasBypass"@en , "PossedeBypassGazChaud"@fr-FR ;
        rdfs:range             xsd:boolean ;
        schema:domainIncludes  <https://w3id.org/product/Compressor> .

props:permeability  a          owl:DatatypeProperty ;
        rdfs:comment           "Ratio of the permeability of the ceiling.\nThe ration can be used to indicate an open ceiling (that enables identification of whether ceiling construction should be considered as impeding distribution of sprinkler water, light etc. from installations within the ceiling area)."@en , "Durchlässigkeit der Unterdecke als Faktor zwischen 0 Undurchlässig und 1 völlig durchlässig. Der Faktor kann zur Abschätzung genutzt werden, ob die Unterdecke zur Decke hin offen und durchlässig (für Licht, Wasser und Sicht) ist."@de-DE , "天花板的渗透比率。\n该比率可用以表示开敞式天花板（表示天花板能否阻隔其内侧的喷淋水、光线等的）。"@zh-CN , "Ratio de perméabilité du plafond. Ce ratio peut être utilisé pour désigner un plafond ouvert (cela permet de savoir si la pose du plafond empêche la distribution de fluides à partir d'installations situées dans le faux plafond)."@fr-FR ;
        rdfs:label             "Durchlässigkeit"@de-DE , "渗透率"@zh-CN , "permeability"@en , "Perméabilité"@fr-FR ;
        rdfs:range             <https://w3id.org/measurement/normalisedRatio> ;
        schema:domainIncludes  <https://w3id.org/product/Covering#CEILING> .

props:vacancyRateInCategoryNow
        a                      owl:DatatypeProperty ;
        rdfs:comment           "Percentage of vacancy found in the particular category currently."@en , "Taux actuel de vacance pour la catégorie."@fr-FR ;
        rdfs:label             "vacancyRateInCategoryNow"@en , "TauxVacanceActuelParCategorie"@fr-FR ;
        rdfs:range             <https://w3id.org/measurement/positiveRatio> ;
        schema:domainIncludes  <https://w3id.org/product/Building> .

props:powerSource  rdfs:comment  "Type of power driving the compressor."@en , "Type de puissance fournie au compresseur"@fr-FR ;
        rdfs:label             "powerSource"@en , "SourcePuissance"@fr-FR ;
        schema:domainIncludes  <https://w3id.org/product/Compressor> .

props:system  a                owl:DatatypeProperty ;
        rdfs:comment           "Angabe zu welcher Anlage (oder Anlagen) der Durchbruch benötigt wird."@de-DE , "需要空构件的建筑服务系统，例如，“空调”、“给排水”、“电气”等。"@zh-CN , "Le système qui requiert la réservation (exemples : \"Conditionnement d'air\", \"Plomberie\", \"Electricité\")"@fr-FR , "he building service system that requires the provision for voids, e.g. 'Air Conditioning', 'Plumbing', 'Electro', etc."@en , "空間に提示される建物サービスシステムです。例えば「空調」「配管」「電気」です。"@ja-JP ;
        rdfs:label             "Système"@fr-FR , "Anlage"@de-DE , "系统"@zh-CN , "システム"@ja-JP , "system"@en ;
        rdfs:range             xsd:string ;
        schema:domainIncludes  <https://w3id.org/product/BuildingElementProxy#PROVISIONFORVOID> .

props:centerlineAirVelocity
        rdfs:comment           "Centerline air velocity versus distance from the diffuser and temperature differential; a function of distance from diffuser and temperature difference between supply air and room air."@en , "吹出口かからの距離と温度差に対する中心速度、\n給気と室内空気の間の吹出口かからの距離と温度差の関数"@ja-JP , "Vitesse de l'air en axe central de jet par rapport à la distance entre le diffuseur et la température différentielle; une fonction de la distance entre le diffuseur et la différence de température entre celui de l'air fourni et celui de l'air de la pièce."@fr-FR ;
        rdfs:label             "centerlineAirVelocity"@en , "中心空気速度"@ja-JP , "Vitesse de l'air en axe central de jet"@fr-FR ;
        schema:domainIncludes  <https://w3id.org/product/AirTerminal> .

props:heatingTemperatureDelta
        a                      owl:DatatypeProperty ;
        rdfs:comment           "Heating temperature difference for calculating space air flow rates."@en , "空調送風量計算用の暖房給気温度差。"@ja-JP , "에어컨 송풍 량 계산을위한 난방 급기 온도차"@ko-KR ;
        rdfs:label             "heatingTemperatureDelta"@en , "暖房時送風温度差"@ja-JP , "난방시 돌풍 온도차"@ko-KR ;
        rdfs:range             <https://w3id.org/measurement/thermodynamicTemperature> ;
        schema:domainIncludes  bot:Zone .

props:installationMethodFlagEnum
        rdfs:comment           "Special installation conditions relating to particular types of installation based on IEC60364-5-52:2001 reference installation methods C and D."@en ;
        rdfs:label             "installationMethodFlagEnum"@en ;
        schema:domainIncludes  <https://w3id.org/product/CableSegment> .

props:nominalSize  a           owl:DatatypeProperty ;
        rdfs:comment           "Indicates the diagonal screen size."@en , "画面の対角線サイズを示す。"@ja-JP , "화면의 대각선 크기를 나타낸다."@ko-KR ;
        rdfs:label             "nominalSize"@en , "画面公称サイズ"@ja-JP , "화면 공칭 크기"@ko-KR ;
        rdfs:range             <https://w3id.org/measurement/positiveLength> ;
        schema:domainIncludes  <https://w3id.org/product/AudioVisualAppliance#DISPLAY> .

props:condition  a             owl:DatatypeProperty ;
        rdfs:comment           "Table mapping alarm condition identifiers to descriptive labels, which may be used for interpreting Pset_AlarmPHistory.Condition."@en , "Pset_AlarmPHistory.Conditionで使用される、警報条件の識別子とラベル情報のマッピングを行う。"@ja-JP , "Indicates alarm condition over time.  The range of possible values and their meanings is defined by Pset_AlarmTypeCommon.Condition.  An empty value indicates no present alarm condition."@en ;
        rdfs:label             "条件"@ja-JP , "condition"@en ;
        rdfs:range             <https://w3id.org/product/TimeSeries> ;
        rdfs:range             [ owl:allValuesFrom  xsd:string ;
                                 owl:onProperty     <https://w3id.org/measurement/seriesOf>
                               ] ;
        schema:domainIncludes  <https://w3id.org/product/Alarm> .

props:closureRatingEnum
        rdfs:comment           "Enumeration that identifies the closure rating for the damper."@en ;
        rdfs:label             "closureRatingEnum"@en ;
        schema:domainIncludes  <https://w3id.org/product/Damper#FIRESMOKEDAMPER> , <https://w3id.org/product/Damper#FIREDAMPER> .

props:playerType  rdfs:comment  "Indicates the type of player."@en , "再生可能な形式を示す。"@ja-JP , "재생 가능한 형식을 보여준다."@ko-KR ;
        rdfs:label             "playerType"@en , "プレイヤー形式"@ja-JP , "플레이어 형식"@ko-KR ;
        schema:domainIncludes  <https://w3id.org/product/AudioVisualAppliance#PLAYER> .

props:housingThickness
        a                      owl:DatatypeProperty ;
        rdfs:comment           "Air terminal box housing material thickness."@en , "ターミナルのハウジング材の板厚"@ja-JP , "Epaisseur du matériau réalisant l'enveloppe du registre terminal de ventilation"@fr-FR ;
        rdfs:label             "housingThickness"@en , "ハウジング板厚"@ja-JP , "Epaisseur de l'enveloppe"@fr-FR ;
        rdfs:range             <https://w3id.org/measurement/length> ;
        schema:domainIncludes  <https://w3id.org/product/AirTerminalBox> .

props:tunerFrequency  rdfs:comment  "Indicates the tuner frequencies, if applicable."@en , "対応周波数帯を示す。"@ja-JP , "주파수 대역을 나타낸다."@ko-KR ;
        rdfs:label             "tunerFrequency"@en , "周波数"@ja-JP , "주파수 대응"@ko-KR ;
        schema:domainIncludes  <https://w3id.org/product/AudioVisualAppliance#TUNER> .

props:standard  a              owl:DatatypeProperty ;
        rdfs:comment           "使用されるケーブル、busbarの定義のために使用される標準仕様。"@ja-JP , "使用するコアの定義に適用される基準の指定。"@ja-JP , "The designation of the standard applicable for the definition of the core used."@en , "사용되는 케이블, busbar의 정의를 위해 사용되는 표준."@ko-KR , "The designation of the standard applicable for the definition of the Cable/Bus used."@en , "사용하는 코어의 정의에 적용되는 기준 지정"@ko-KR ;
        rdfs:label             "基準"@ja-JP , "標準"@ja-JP , "기준"@ko-KR , "standard"@en , "표준"@ko-KR ;
        rdfs:range             xsd:string ;
        schema:domainIncludes  <https://w3id.org/product/CableSegment#CABLESEGMENT> , <https://w3id.org/product/CableSegment#CORESEGMENT> .

props:fireRating  a            owl:DatatypeProperty ;
        rdfs:comment           "Fire rating for the element.\nIt is given according to the national fire safety classification."@en , "主要な耐火等級。関連する建築基準法、消防法などの国家基準を参照。"@ja-JP , "Classement au feu de l'élément donné selon la classification nationale de sécurité incendie."@fr-FR , "Feuerwiderstandsklasse gemäß der nationalen oder regionalen Brandschutzverordnung."@de-DE , "当該オブジェクトの耐火等級。国で定めた耐火安全等級分類による。"@ja-JP , "耐火等級。当該国の建築法規による。"@ja-JP , "Fire rating for the element. It is given according to the national fire safety classification."@en , "Feuerwiderstandasklasse gemäß der nationalen oder regionalen Brandschutzverordnung."@de-DE , "Fire rating for this object.\nIt is given according to the national fire safety classification."@en , "Fire rating given according to the national fire safety classification."@en , "该构件的防火等级。\n该属性的依据为国家防火安全分级。"@zh-CN ;
        rdfs:label             "ResistanceAuFeu"@fr-FR , "Résistance au feu"@fr-FR , "防火等级"@zh-CN , "fireRating"@en , "Feuerwiderstandsklasse"@de-DE , "耐火等級"@ja-JP ;
        rdfs:range             xsd:string ;
        schema:domainIncludes  <https://w3id.org/product/BuildingElementProxy> , <https://w3id.org/product/Beam> , <https://w3id.org/product/Column> , <https://w3id.org/product/Covering> , <https://w3id.org/product/Chimney> , <https://w3id.org/product/CurtainWall> .

props:returnAirFractionRange
        rdfs:comment           "Allowable return air fraction range as a fraction of discharge airflow."@en , "送風量の一部としての許容還気風量"@ja-JP , "Plage possiblede la fraction d'air repris en tant que fraction de l'air rejeté"@fr-FR ;
        rdfs:label             "returnAirFractionRange"@en , "還気風量比"@ja-JP , "Plage pour la fraction d'air repris"@fr-FR ;
        schema:domainIncludes  <https://w3id.org/product/AirTerminalBox> .

props:ratedVoltage  rdfs:comment  "사용할 수있는 권한이있는 허용 전압."@ko-KR , "使用できることが許可されている許容電圧。"@ja-JP , "장치를 사용할 보장된 전압. 상한은 최대."@ko-KR , "機器を使用できる保障された電圧。上限値は最大値。"@ja-JP , "The range of allowed voltage that a device is certified to handle. The upper bound of this value is the maximum."@en ;
        rdfs:label             "정격 전압"@ko-KR , "ratedVoltage"@en , "定格電圧"@ja-JP ;
        schema:domainIncludes  <https://w3id.org/product/CableSegment#CABLESEGMENT> , <https://w3id.org/product/CableSegment#CORESEGMENT> .

props:audioAmplification
        rdfs:comment           "Indicates audio amplification frequency ranges."@en , "再生周波数帯域を示す。"@ja-JP , "재생 주파수 대역을 나타낸다."@ko-KR ;
        rdfs:label             "audioAmplification"@en , "オーディオアンプ"@ja-JP , "오디오 앰프"@ko-KR ;
        schema:domainIncludes  <https://w3id.org/product/AudioVisualAppliance#RECEIVER> , <https://w3id.org/product/AudioVisualAppliance#AMPLIFIER> .

props:frameType  a             owl:DatatypeProperty ;
        rdfs:comment           "The type of frame used by the damper (e.g., Standard, Single Flange, Single Reversed Flange, Double Flange, etc.)."@en ;
        rdfs:label             "frameType"@en ;
        rdfs:range             xsd:string ;
        schema:domainIncludes  <https://w3id.org/product/Damper> .

props:actualCost  a            owl:DatatypeProperty ;
        rdfs:comment           "The actual cost on behalf of the resource allocation."@en , "資源配分のための実績のコスト。"@ja-JP ;
        rdfs:label             "actualCost"@en , "実績コスト"@ja-JP ;
        rdfs:range             <https://w3id.org/product/TimeSeries> ;
        rdfs:range             [ owl:allValuesFrom  <https://w3id.org/measurement/monetary> ;
                                 owl:onProperty     <https://w3id.org/measurement/seriesOf>
                               ] ;
        schema:domainIncludes  <https://w3id.org/product/ConstructionResource> .

props:numberOfCells  a         owl:DatatypeProperty ;
        rdfs:comment           "Number of cells in one cooling tower unit."@en ;
        rdfs:label             "numberOfCells"@en ;
        rdfs:range             xsd:int ;
        schema:domainIncludes  <https://w3id.org/product/CoolingTower> .

props:mechanicalEfficiency
        a                      owl:DatatypeProperty ;
        rdfs:comment           "Ratio of the work (as measured) delivered to the gas to the work input to the compressor shaft."@en , "Rapport entre le travail fourni (tel que mesuré) au gaz et le travail fourni à l'arbre du compresseur."@fr-FR ;
        rdfs:label             "mechanicalEfficiency"@en , "RendementMécanique"@fr-FR ;
        rdfs:range             <https://w3id.org/product/TimeSeries> ;
        rdfs:range             [ owl:allValuesFrom  <https://w3id.org/measurement/normalisedRatio> ;
                                 owl:onProperty     <https://w3id.org/measurement/seriesOf>
                               ] ;
        schema:domainIncludes  <https://w3id.org/product/Compressor> .

props:assetTaxType  rdfs:comment  "Identifies the predefined types of taxation group from which the type required may be set."@en , "税の定義済み種別。"@ja-JP ;
        rdfs:label             "assetTaxType"@en , "資産税種別"@ja-JP ;
        schema:domainIncludes  <https://w3id.org/product/Asset> .

props:description  a           owl:DatatypeProperty ;
        rdfs:comment           "The description of the air side system."@en , "空調方式の説明。"@ja-JP , "공조 방식 설명"@ko-KR ;
        rdfs:label             "description"@en , "説明"@ja-JP , "설명"@ko-KR ;
        rdfs:range             xsd:string ;
        schema:domainIncludes  bot:Zone .

props:compressionEfficiency
        a                      owl:DatatypeProperty ;
        rdfs:comment           "Ratio of the work required for isentropic compression of the gas to the work delivered to the gas within the compression volume (as obtained by measurement)."@en , "Rapport entre le travail requis pour une compression isentropique du gaz et le travail fourni au gaz dans le volume comprimé (telq qu'obtenu par mesure)."@fr-FR ;
        rdfs:label             "compressionEfficiency"@en , "RendementCompression"@fr-FR ;
        rdfs:range             <https://w3id.org/product/TimeSeries> ;
        rdfs:range             [ owl:allValuesFrom  <https://w3id.org/measurement/normalisedRatio> ;
                                 owl:onProperty     <https://w3id.org/measurement/seriesOf>
                               ] ;
        schema:domainIncludes  <https://w3id.org/product/Compressor> .

props:totalAirflow  a          owl:DatatypeProperty ;
        rdfs:comment           "The total design supply air flowrate required for the system for either heating or cooling conditions, whichever is greater."@en , "暖房、冷房の条件の、いずれか大きい条件で要求される設計給気量。"@ja-JP , "난방, 냉방 조건 중 하나 큰 조건에서 요구되는 설계 급기 량"@ko-KR ;
        rdfs:label             "totalAirflow"@en , "給気量"@ja-JP , "급기량"@ko-KR ;
        rdfs:range             <https://w3id.org/measurement/volumetricFlowRate> ;
        schema:domainIncludes  bot:Zone .

props:combustionTemperature
        a                      owl:DatatypeProperty ;
        rdfs:comment           "燃焼室平均温度"@ja-JP , "Average combustion chamber temperature."@en , "Température de combustion moyenne au foyer."@fr-FR ;
        rdfs:label             "TempératureCombustion"@fr-FR , "燃焼温度"@ja-JP , "combustionTemperature"@en ;
        rdfs:range             <https://w3id.org/product/TimeSeries> ;
        rdfs:range             [ owl:allValuesFrom  <https://w3id.org/measurement/thermodynamicTemperature> ;
                                 owl:onProperty     <https://w3id.org/measurement/seriesOf>
                               ] ;
        schema:domainIncludes  <https://w3id.org/product/Boiler> .

props:pressureRating  a        owl:DatatypeProperty ;
        rdfs:comment           "Nominal pressure rating of the boiler as rated by the agency having jurisdiction."@en , "管轄組織により設定されたボイラの常用圧力"@ja-JP , "Pression nominale admissible de la chaudière comme classée par l'organisme qui fait autorité."@fr-FR ;
        rdfs:label             "pressureRating"@en , "常用圧力"@ja-JP , "PressionAdmissibleNominale"@fr-FR ;
        rdfs:range             <https://w3id.org/measurement/pressure> ;
        schema:domainIncludes  <https://w3id.org/product/Boiler> .

props:airFlowConfiguration
        rdfs:comment           "Air flow configuration type of cooled beam."@en ;
        rdfs:label             "airFlowConfiguration"@en ;
        schema:domainIncludes  <https://w3id.org/product/CooledBeam#ACTIVE> .

props:tenureModesAvailableFuture
        rdfs:comment           "A list of the tenure modes that are expected to be available in the future expressed in terms of IfcLabel."@en , "Liste des possibilités d'occupation futures."@fr-FR ;
        rdfs:label             "tenureModesAvailableFuture"@en , "PossibilitesOccupationFutures"@fr-FR ;
        schema:domainIncludes  <https://w3id.org/product/Building> .

props:wetCoilFraction
        a                      owl:DatatypeProperty ;
        rdfs:comment           "Fraction of coil surface area that is wet (0-1)."@en , "Fraction de la surface de la batterie qui est humide (0 à 1)."@fr-FR ;
        rdfs:label             "wetCoilFraction"@en , "FractionBatterieHumide"@fr-FR ;
        rdfs:range             <https://w3id.org/measurement/normalisedRatio> ;
        schema:domainIncludes  <https://w3id.org/product/Coil> .

props:fanPower  a              owl:DatatypeProperty ;
        rdfs:comment           "Fan motor loads contributing to the cooling load."@en , "送風機モーターからの熱取得。"@ja-JP , "송풍기 모터의 열 취득"@ko-KR ;
        rdfs:label             "fanPower"@en , "送風機電力消費量"@ja-JP , "송풍기 소비 전력"@ko-KR ;
        rdfs:range             <https://w3id.org/measurement/power> ;
        schema:domainIncludes  bot:Zone .

props:slotWidth  a             owl:DatatypeProperty ;
        rdfs:comment           "Slot width."@en , "スロット巾"@ja-JP , "Epaisseur de la fente"@fr-FR ;
        rdfs:label             "slotWidth"@en , "スロット巾"@ja-JP , "EpaisseurFente"@fr-FR ;
        rdfs:range             <https://w3id.org/measurement/positiveLength> ;
        schema:domainIncludes  <https://w3id.org/product/AirTerminal> .

props:coreType  rdfs:comment   "Identifies the way the core of the AirTerminal is constructed."@en , "取り付けられたターミナルのコアの定義方法（SHUTTERBLADE, CURVEDBLADE, REMOVABLE, REVERSIBLEなど）"@ja-JP , "Caractérise comment la partie centrale du terminal de ventilation est fabriquée."@fr-FR ;
        rdfs:label             "coreType"@en , "コア形式"@ja-JP , "TypePartieCentrale"@fr-FR ;
        schema:domainIncludes  <https://w3id.org/product/AirTerminal> .

props:videoResolutionHeight
        a                      owl:DatatypeProperty ;
        rdfs:comment           "垂直方向のピクセル数を示す。"@ja-JP , "수직 픽셀 수를 나타낸다."@ko-KR , "세로 픽셀 수를 나타낸다."@ko-KR , "Indicates the number of vertical pixels, e.g. 1080."@en , "세로 픽셀 수."@ko-KR , "Indicates the number of vertical pixels (the largest native video resolution height)."@en , "垂直方向のピクセル数。"@ja-JP ;
        rdfs:label             "videoResolutionHeight"@en , "수직 해상도"@ko-KR , "垂直解像度"@ja-JP ;
        rdfs:range             xsd:int ;
        schema:domainIncludes  <https://w3id.org/product/AudioVisualAppliance#CAMERA> , <https://w3id.org/product/AudioVisualAppliance#DISPLAY> , <https://w3id.org/product/AudioVisualAppliance#PROJECTOR> .

props:bladeMaterial  a         owl:ObjectProperty ;
        rdfs:comment           "The material from which the damper blades are constructed."@en ;
        rdfs:label             "bladeMaterial"@en ;
        rdfs:range             <https://w3id.org/product/MaterialDefinition> ;
        schema:domainIncludes  <https://w3id.org/product/Damper> .

props:nominalHeatingCapacity
        a                      owl:DatatypeProperty ;
        rdfs:comment           "Nominal heating capacity."@en ;
        rdfs:label             "nominalHeatingCapacity"@en ;
        rdfs:range             <https://w3id.org/measurement/power> ;
        schema:domainIncludes  <https://w3id.org/product/CooledBeam> .

props:primaryAirflowRateRange
        rdfs:comment           "possible range of primary airflow that can be delivered.."@en , "一次側の送風可能範囲"@ja-JP , "Plage possible de débit d'air au primaire qui peut être fourni."@fr-FR ;
        rdfs:label             "primaryAirflowRateRange"@en , "一次側風量範囲"@ja-JP , "PlageDébitAirPrimaire"@fr-FR ;
        schema:domainIncludes  <https://w3id.org/product/AirToAirHeatRecovery> .

props:hasNonSkidSurface
        a                      owl:DatatypeProperty ;
        rdfs:comment           "表示表面处理是否设计为防滑的。"@zh-CN , "Angabe, ob der Bodenbelag eine nichtrutschende Oberfläche hat (JA), oder nicht (NEIN)."@de-DE , "Indication whether the surface finish is designed to prevent slippery (TRUE) or not (FALSE)."@en , "Indique si la finition est conçue pour être anti dérapante (VRAI) ou non (FAUX)."@fr-FR ;
        rdfs:label             "Anti dérapant"@fr-FR , "hasNonSkidSurface"@en , "表面是否防滑"@zh-CN , "Nichtrutschende Oberfläche"@de-DE ;
        rdfs:range             xsd:boolean ;
        schema:domainIncludes  <https://w3id.org/product/Covering#FLOORING> .

props:electricActuatorType
        rdfs:comment           "Enumeration that identifies electric actuator as defined by its operational principle."@en , "作動原理によって定義された電気式アクチュエータを識別する一覧。"@ja-JP , "작동 원리에 의해 정의된 전기식 액츄에이터를 식별하는 목록"@ko-KR ;
        rdfs:label             "electricActuatorType"@en , "電気式アクチュエータタイプ"@ja-JP , "전기식 액추에이터 유형"@ko-KR ;
        schema:domainIncludes  <https://w3id.org/product/Actuator#ELECTRICACTUATOR> .

props:maximumPartLoadRatio
        a                      owl:DatatypeProperty ;
        rdfs:comment           "Maximum part load ratio as a fraction of nominal capacity."@en , "Coefficient maximal de charge partielle en tant que fraction de la puissance nominale."@fr-FR ;
        rdfs:label             "maximumPartLoadRatio"@en , "CoefficientMaximalChargePartielle"@fr-FR ;
        rdfs:range             <https://w3id.org/measurement/positiveRatio> ;
        schema:domainIncludes  <https://w3id.org/product/Compressor> .

props:shaftPower  a            owl:DatatypeProperty ;
        rdfs:comment           "The actual shaft power input to the compressor."@en , "La puissance mécanique appliquée au niveau de l'arbre du compresseur."@fr-FR ;
        rdfs:label             "shaftPower"@en , "PuissanceArbre"@fr-FR ;
        rdfs:range             <https://w3id.org/product/TimeSeries> ;
        rdfs:range             [ owl:allValuesFrom  <https://w3id.org/measurement/power> ;
                                 owl:onProperty     <https://w3id.org/measurement/seriesOf>
                               ] ;
        schema:domainIncludes  <https://w3id.org/product/Compressor> .

props:hasFan  a                owl:DatatypeProperty ;
        rdfs:comment           "Terminal box has a fan inside (fan powered box)."@en , "内部に送風機を持つ時にTRUE"@ja-JP , "Le registre terminal possède dans son  intérieur un ventilateur (registre motorisé)"@fr-FR ;
        rdfs:label             "hasFan"@en , "送風機有無"@ja-JP , "Possède ventilateur"@fr-FR ;
        rdfs:range             xsd:boolean ;
        schema:domainIncludes  <https://w3id.org/product/AirTerminalBox> .

props:marketCategory  a        owl:DatatypeProperty ;
        rdfs:comment           "Category of use e.g. residential, commercial, recreation etc."@en , "Catégorie d'usage (résidentiel, commercial, loisir,…)"@fr-FR ;
        rdfs:label             "CategorieUsage"@fr-FR , "marketCategory"@en , "CategorieMarche"@fr-FR ;
        rdfs:range             xsd:string ;
        schema:domainIncludes  <https://w3id.org/product/Building> .

props:faceType  rdfs:comment   "Identifies how the terminal face of an AirTerminal is constructed."@en , "ターミナル表面の形式定義"@ja-JP , "Caractérise comment le côté du terminal d'un terminal de ventilation est fabriqué."@fr-FR ;
        rdfs:label             "faceType"@en , "表面タイプ"@ja-JP , "TypeCôté"@fr-FR ;
        schema:domainIncludes  <https://w3id.org/product/AirTerminal> .

props:impellerDiameter
        a                      owl:DatatypeProperty ;
        rdfs:comment           "Diameter of compressor impeller - used to scale performance of geometrically similar compressors."@en , "Diamètre du rotor du compresseur - utilisé pour dimensionner les performances des compresseurs géométriquement similaires."@fr-FR ;
        rdfs:label             "impellerDiameter"@en , "DiametreRotor"@fr-FR ;
        rdfs:range             <https://w3id.org/measurement/positiveLength> ;
        schema:domainIncludes  <https://w3id.org/product/Compressor> .

props:inductionRatio  rdfs:comment  "Induction ratio versus distance from the diffuser and its discharge direction; induction ratio (or entrainment ratio) is the ratio of the volumetric flow rate in the jet to the volumetric flow rate at the air terminal."@en , "制気口からの距離とその排出方向に対する誘引比、\n誘導比（または同調比）は、エアターミナルでの体積流量に対する噴流の体積流量の比である。"@ja-JP , "Taux d'induction par rapport à la distance entre le diffuseur et sa direction de rejet;\nLe taux d'induction est le rapport entre  le débit volumique d'air dans le jet sur  le débit volumique d'air au niveau du terminal."@fr-FR ;
        rdfs:label             "inductionRatio"@en , "誘引率"@ja-JP , "Taux d'induction"@fr-FR ;
        schema:domainIncludes  <https://w3id.org/product/AirTerminal> .

props:specialConstruction
        a                      owl:DatatypeProperty ;
        rdfs:comment           "Special construction capabilities like self-supporting, flat devidable cable or bus flat non devidable cable or bus supporting elements inside (steal, textile, concentric conductor). Note that materials used should be agreed between exchange participants before use."@en , "特殊な構造を備えた性能－たとえば、平型フレキシブルケーブルあるいは硬い平型母線ケーブル、あるいは母線で内部に鉄製、繊維、同心導体で構成されているサポートを持っている。\n注記）使用する材料は、使用前に交流参加者間で合意すること。"@ja-JP , "특수한 구조를 갖춘 성능 - 예를 들어, 평형 플렉시블 케이블 또는 딱딱한 평형 모선 케이블 또는 모선 내부에 철제, 섬유, 동심 도체로 구성되어있는 지원이있다. 주) 사용하는 재료는 사용 전에 교류 참가자 사이에 동의한다."@ko-KR ;
        rdfs:label             "specialConstruction"@en , "特別な施工方法"@ja-JP , "특별한 시공 방법"@ko-KR ;
        rdfs:range             xsd:string ;
        schema:domainIncludes  <https://w3id.org/product/CableSegment#CABLESEGMENT> .

props:installationMethod
        a                      owl:DatatypeProperty ;
        rdfs:comment           "Method of installation of cable/conductor. Installation methods are typically defined by reference in standards such as IEC 60364-5-52, table 52A-1 or BS7871 Appendix 4 Table 4A1 etc. Selection of the value to be used should be determined from such a standard according to local usage."@en ;
        rdfs:label             "installationMethod"@en ;
        rdfs:range             xsd:string ;
        schema:domainIncludes  <https://w3id.org/product/CableSegment> .

props:mountingMethod  rdfs:comment  "The method of mounting cable segment occurrences on a cable carrier occurrence from which the method required can be selected. This is for the purpose of carrying out 'worst case' cable sizing calculations and may be a conceptual requirement rather than a statement of the physical occurrences of cable and carrier segments."@en ;
        rdfs:label             "mountingMethod"@en ;
        schema:domainIncludes  <https://w3id.org/product/CableSegment> .

props:function  rdfs:comment   "Type of function for which the conductor is intended."@en , "導体の機能のタイプ。"@ja-JP , "도체의 기능 유형."@ko-KR ;
        rdfs:label             "function"@en , "機能"@ja-JP , "기능"@ko-KR ;
        schema:domainIncludes  <https://w3id.org/product/CableSegment#CONDUCTORSEGMENT> .

props:constructionToleranceClass
        a                      owl:DatatypeProperty ;
        rdfs:comment           "Classification designation of the on-site construction tolerances according to local standards."@en , "国の基準が求める現場での製造許容の分類指定。"@ja-JP , "국가 표준이 요구하는 현장에서 제조 허용 범주 지정"@ko-KR ;
        rdfs:label             "constructionToleranceClass"@en , "製造許容クラス"@ja-JP , "제조 허용 클래스"@ko-KR ;
        rdfs:range             xsd:string ;
        schema:domainIncludes  <https://w3id.org/product/BuildingElement> .

props:operationTemperatureRange
        a                      owl:DatatypeProperty ;
        rdfs:comment           "許容周囲温度範囲"@ja-JP , "Allowable operational range of the ambient air temperature."@en , "Allowable operation ambient air temperature range."@en , "Plage opérationnelle possible de la température de l'air ambiant"@fr-FR ;
        rdfs:label             "動作温度範囲"@ja-JP , "Plage de température d'exploitation"@fr-FR , "operationTemperatureRange"@en ;
        rdfs:range             <https://w3id.org/measurement/thermodynamicTemperature> ;
        schema:domainIncludes  <https://w3id.org/product/AirTerminalBox> , <https://w3id.org/product/CoolingTower> .

props:powerLoss  a             owl:DatatypeProperty ;
        rdfs:comment           "Total loss of power across this cable."@en ;
        rdfs:label             "powerLoss"@en ;
        rdfs:range             <https://w3id.org/measurement/electricCurrent> ;
        schema:domainIncludes  <https://w3id.org/product/CableSegment> .

props:nominalSensibleCapacity
        a                      owl:DatatypeProperty ;
        rdfs:comment           "Nominal sensible capacity."@en , "Puissance sensible nominale."@fr-FR ;
        rdfs:label             "nominalSensibleCapacity"@en , "PuissanceSensibleNominale"@fr-FR ;
        rdfs:range             <https://w3id.org/measurement/power> ;
        schema:domainIncludes  <https://w3id.org/product/Coil> .

props:acknowledge  a           owl:DatatypeProperty ;
        rdfs:comment           "Indicates acknowledgement status where False indicates acknowlegement is required and outstanding, True indicates condition has been acknowedged, and Unknown indicates no acknowledgement is required.  Upon resetting the condition, then acknowledgement reverts to Unknown."@en ;
        rdfs:label             "acknowledge"@en ;
        rdfs:range             <https://w3id.org/product/TimeSeries> ;
        rdfs:range             [ owl:allValuesFrom  xsd:boolean ;
                                 owl:onProperty     <https://w3id.org/measurement/seriesOf>
                               ] ;
        schema:domainIncludes  <https://w3id.org/product/Alarm> .

props:failPosition  rdfs:comment  "Specifies the required fail-safe position of the actuator."@en , "要求されたアクチュエータのフェールセーフタイプを示す。"@ja-JP , "대체 기능으로 수동 조작이 제공되는지 (= TRUE) 여부 (= FALSE)를 확인한다. 수동으로 조작하는 액츄에이터의 경우는이 값을 기본값으로 FALSE로 설정해야하므로주의한다."@ko-KR ;
        rdfs:label             "failPosition"@en , "フェールセーフタイプ"@ja-JP , "재정 기능의 유무"@ko-KR ;
        schema:domainIncludes  <https://w3id.org/product/Actuator> .

props:reference  a             owl:DatatypeProperty ;
        rdfs:comment           "Kennzeichen für diese bauliche System in dem Projekt (z.B. 'TRA/EL1'). Die Kennzeichensystematik hängt von den jeweiligen nationalen/regionalen Regelungen ab."@de-DE , "このプロジェクトにおける参照記号(例：A-1)"@ja-JP , "해당 프로젝트에 정의된 형식의 참조 ID (예 : A-1) 승인된 분류에 존재하지 않을 때 사용된다. 참조"@ko-KR , "認識された分類体系で参照する分類がない場合にこのプロジェクト固有の参照記号（例：タイプ'A-1'）が与えられる。"@ja-JP , "Identifikator der projektinternen Referenz für dieses Gebäude, z.B. nach der Gebäudelassifizierung des Bauherrn. Wird verwendet, wenn keine allgemein anerkanntes Klassifizierungssystem angewandt wird."@de-DE , "해당 프로젝트에서 사용이 유형에 대한 참조 ID (예 : 'A-1') ※ 기본이있는 경우 그 기호를 사용"@ko-KR , "Référence à l'identifiant d'un type spécifié dans le contexte de ce projet (exemple : \"type A1\"). A fournir s'il n'y a pas de référence à une classification en usage."@fr-FR , "当該プロジェクトで定義する形式の参照ID（例：A-1)、承認された分類に存在しないときに使用される。"@ja-JP , "Référence à l'identifiant d'un type spécifié dans le contexte du projet (exemple : \"type A1\") pour désigner un \"type de construction\". Une alternative au nom d'un objet type lorsque les objets types ne sont pas gérés par le logiciel."@fr-FR , "Reference ID for this specified type in this project (e.g. type 'A-1'). Used to store the non-classification driven internal project type."@en , "Bezeichnung zur Zusammenfassung gleichartiger Bauteile zu einem Bauteiltyp (auch Konstruktionstyp genannt). Alternativ zum Namen des \"Typobjekts\", insbesondere wenn die Software keine Typen unterstützt."@de-DE , "해당프로젝트에 정의도니 형식의 참조ID (예 : A-1) 승인된 분류에 존재하지 않을 때 사용된다."@ko-KR , "若未采用已知的分类系统，则该属性为该项目中该类型构件的参考编号（例如，类型A-1）。"@zh-CN , "Identifikator der projektinternen Referenz für dieses Geschoss, z.B. nach der Geschossklassifizierung des Bauherrn. Wird verwendet, wenn keine allgemein anerkanntes Klassifizierungssystem angewandt wird."@de-DE , "このプロジェクトにおける参照記号(例：A-1)。分類コードではなく内部で使用されるプロジェクトタイプとして使用されるもの。"@ja-JP , "이 프로젝트의 참조 ID (예 : A-1). 분류 코드가 아닌 내부에서 사용되는 프로젝트 형식으로 사용됩니다."@ko-KR , "Référence à l'identifiant d'un type spécifié dans le contexte du projet (exemple : \"type A1\"). Utilisé pour enregistrer un type sans recourir à une classification."@fr-FR , "该项目中该类型构件的参考编号（例如，类型A-1）。"@zh-CN , "Identification de référence pour ce type spécifique à ce projet, c'est-à-dire type'A-1', fourni à partir du moment où, s'il n'y a pas de référence de classification par rapport à un système de classification reconnu et en usage."@fr-FR , "このプロジェクトにおける建物システムの指定されたインスタンスの参照記号"@ja-JP , "该项目中该特定建筑系统实例的参考编号（例如，“TRA/EL1”）。该属性值由当地编码规范决定。"@zh-CN , "Reference ID for this specified type in this project (e.g. type 'A-1'), provided, if there is no classification reference to a recognized classification system used."@en , "Reference ID for this specified type in this project (e.g. type 'A-1'), Also referred to as \"construction type\". It should be provided as an alternative to the name of the \"object type\", if the software does not support object types."@en , "해당 프로젝트에 정의된 형식의 참조 ID (예 : A-1) 승인된 분류에 존재하지 않을 때 사용된다."@ko-KR , "Reference ID for this specified instance of building system in this project (e.g. 'TRA/EL1'), The reference values depend on the local code of practice."@en ;
        rdfs:label             "Bauteiltyp"@de-DE , "参照記号"@ja-JP , "Référence"@fr-FR , "참조 ID"@ko-KR , "参照"@ja-JP , "참조"@ko-KR , "参考号"@zh-CN , "Kennzeichen"@de-DE , "Referenz ID"@de-DE , "Reference"@fr-FR , "reference"@en , "참조ID"@ko-KR ;
        rdfs:range             xsd:string ;
        schema:domainIncludes  <https://w3id.org/product/CableCarrierFitting> , <https://w3id.org/product/Damper> , <https://w3id.org/product/CooledBeam> , <https://w3id.org/product/Coil> , <https://w3id.org/product/Beam> , <https://w3id.org/product/CommunicationsAppliance> , <https://w3id.org/product/CableCarrierSegment> , <https://w3id.org/product/CurtainWall> , <https://w3id.org/product/BuildingSystem> , <https://w3id.org/product/Chiller> , <https://w3id.org/product/Boiler> , <https://w3id.org/product/CableSegment> , <https://w3id.org/product/AudioVisualAppliance> , <https://w3id.org/product/AirTerminal> , <https://w3id.org/product/Burner> , <https://w3id.org/product/Alarm> , <https://w3id.org/product/Column> , <https://w3id.org/product/Building> , <https://w3id.org/product/Actuator> , <https://w3id.org/product/BuildingElementProxy> , <https://w3id.org/product/CableFitting> , <https://w3id.org/product/BuildingStorey> , <https://w3id.org/product/AirTerminalBox> , <https://w3id.org/product/CoolingTower> , <https://w3id.org/product/Chimney> , <https://w3id.org/product/Controller> , <https://w3id.org/product/Covering> , <https://w3id.org/product/AirToAirHeatRecovery> , <https://w3id.org/product/Compressor> , <https://w3id.org/product/Condenser> .

props:acousticRating  a        owl:DatatypeProperty ;
        rdfs:comment           "Schallschutzklasse gemäß der nationalen oder regionalen Schallschutzverordnung."@de-DE , "遮音等級情報。関連する建築基準法を参照。"@ja-JP , "Acoustic rating for this object.\nIt is provided according to the national building code. It indicates the sound transmission resistance of this object by an index ratio (instead of providing full sound absorbtion values)."@en , "Acoustic rating for this object.\nIt is giving according to the national building code. It indicates the sound transmission resistance of this object by an index ration (instead of providing full sound absorbtion values)."@en , "遮音等級。当該国の建築法規による。\nこのオブジェクトの音の透過損失を等級値で示す。"@ja-JP , "该构件的隔音等级。\n该属性的依据为国家建筑规范。为表示该构件隔音效果的比率（而不是完全吸收声音的值）。"@zh-CN , "Classement acoustique de cet objet. Donné selon le Code National du Bâtiment. Il indique la résistance à la transmission du son de cet objet par une valeur de référence (au lieu de fournir les valeurs totales d'absorption du son)."@fr-FR ;
        rdfs:label             "Isolation acoustique"@fr-FR , "IsolationAcoustique"@fr-FR , "隔音等级"@zh-CN , "遮音等級"@ja-JP , "acousticRating"@en , "Schallschutzklasse"@de-DE ;
        rdfs:range             xsd:string ;
        schema:domainIncludes  <https://w3id.org/product/Covering> , <https://w3id.org/product/CurtainWall> .

props:compressorTotalEfficiency
        a                      owl:DatatypeProperty ;
        rdfs:comment           "Ratio of the thermal cooling capacity to electrical input."@en , "Rapport entre la puissance frigorifique et l'énergie électrique absorbée."@fr-FR ;
        rdfs:label             "compressorTotalEfficiency"@en , "RendementGlobalIsentropique"@fr-FR ;
        rdfs:range             <https://w3id.org/product/TimeSeries> ;
        rdfs:range             [ owl:allValuesFrom  <https://w3id.org/measurement/normalisedRatio> ;
                                 owl:onProperty     <https://w3id.org/measurement/seriesOf>
                               ] ;
        schema:domainIncludes  <https://w3id.org/product/Compressor> .

props:coilConnectionDirection
        rdfs:comment           "Coil connection direction (facing into the air stream)."@en , "Direction de la connexion à la batterie (en face du jet d'air)"@fr-FR ;
        rdfs:label             "coilConnectionDirection"@en , "DirectionConnexionBatterie"@fr-FR ;
        schema:domainIncludes  <https://w3id.org/product/Coil> .

props:hasReturnAir  a          owl:DatatypeProperty ;
        rdfs:comment           "Terminal box has return air mixed with supply air from duct work."@en , "ターミナルで還気を混合しているか否か（していればTRUE)"@ja-JP , "Le registre terminal a son air de reprise mélangé avec une amenée d'air issu du réseau de ventilation"@fr-FR ;
        rdfs:label             "hasReturnAir"@en , "還気有無"@ja-JP , "Possède air  repris"@fr-FR ;
        rdfs:range             xsd:boolean ;
        schema:domainIncludes  <https://w3id.org/product/AirTerminalBox> .

props:panVertical  rdfs:comment  "Indicates vertical range for panning."@en , "垂直方向の可動範囲を示す。"@ja-JP ;
        rdfs:label             "panVertical"@en , "パン垂直方向可動範囲"@ja-JP ;
        schema:domainIncludes  <https://w3id.org/product/AudioVisualAppliance#CAMERA> .

props:maximumOutletPressure
        a                      owl:DatatypeProperty ;
        rdfs:comment           "Maximum steam outlet pressure."@en , "最大出口蒸気圧力"@ja-JP , "Pression vapeur en sortie maximale"@fr-FR ;
        rdfs:label             "maximumOutletPressure"@en , "最大出口圧力"@ja-JP , "PressionSortieAdmissible"@fr-FR ;
        rdfs:range             xsd:string ;
        schema:domainIncludes  <https://w3id.org/product/Boiler#STEAM> .

props:exteriorHeatTransferCoefficient
        a                      owl:DatatypeProperty ;
        rdfs:comment           "Exterior heat transfer coefficient associated with exterior surface area."@en ;
        rdfs:label             "exteriorHeatTransferCoefficient"@en ;
        rdfs:range             <https://w3id.org/product/TimeSeries> ;
        rdfs:range             [ owl:allValuesFrom  <https://w3id.org/measurement/thermalTransmittance> ;
                                 owl:onProperty     <https://w3id.org/measurement/seriesOf>
                               ] ;
        schema:domainIncludes  <https://w3id.org/product/Condenser> .

props:amplifierType  rdfs:comment  "Indicates the type of amplifier."@en , "アンプの形式を示す。"@ja-JP , "앰프의 형식을 보여준다."@ko-KR ;
        rdfs:label             "amplifierType"@en , "アンプ形式"@ja-JP , "앰프 형식"@ko-KR ;
        schema:domainIncludes  <https://w3id.org/product/AudioVisualAppliance#AMPLIFIER> .

props:aboveGround  a           owl:DatatypeProperty ;
        rdfs:comment           "Angabe, ob dieses Geschoss vollständig überhalb oberirdisch ist (WAHR), vollständig unterirdisch (FALSCH), oder teilweise unter- und überirdisch (UNKNOWN)."@de-DE , "이 건물 층이 지상 (TRUE), 지하 (FALSE), 일부 지하 부분 (UNKOWN) 여부를 나타내는 논리 값."@ko-KR , "この建物階が地上(TRUE)、地下(FALSE)、一部が地下部分(UNKOWN)かどうかを示すロジカル値。"@ja-JP , "Indication whether this building storey is fully above ground (TRUE), or below ground (FALSE), or partially above and below ground (UNKNOWN) - as in sloped terrain."@en , "Indication si l'étage est complètement au dessus du niveau du sol (VRAI), au dessous du niveau du sol (FAUX) ou partiellement enterré (INCONNU) comme dans le cas d'un terrain en pente."@fr-FR ;
        rdfs:label             "地上判別"@ja-JP , "AuDessusSol"@fr-FR , "Oberirdisches Geschoss"@de-DE , "aboveGround"@en , "지상 여부"@ko-KR ;
        rdfs:range             xsd:boolean ;
        schema:domainIncludes  <https://w3id.org/product/BuildingStorey> .

props:fireResistanceRating
        a                      owl:DatatypeProperty ;
        rdfs:comment           "Measure of the fire resistance rating in hours (e.g., 1.5 hours, 2 hours, etc.)."@en ;
        rdfs:label             "fireResistanceRating"@en ;
        rdfs:range             xsd:string ;
        schema:domainIncludes  <https://w3id.org/product/Damper#FIRESMOKEDAMPER> , <https://w3id.org/product/Damper#FIREDAMPER> .

props:isLandmarked  a          owl:DatatypeProperty ;
        rdfs:comment           "Indique si le bâtiment est classé aux monuments historiques (VRAI) ou non (FAUX), ou si l'information n'est pas connue."@fr-FR , "이 건물은 역사적인 건물 있는지 여부를 나타내는 값"@ko-KR , "この建物は歴史的な建物かどうかを示すブーリアン値。"@ja-JP , "Angabe, ob das Gebäude dem Denkmalschutz unterliegt (WAHR) oder nicht (FALSCH)."@de-DE , "This builing is listed as a historic building (TRUE), or not (FALSE), or unknown."@en ;
        rdfs:label             "ランドマーク区分"@ja-JP , "ClasseMonumentHistorique"@fr-FR , "Denkmalschutz"@de-DE , "isLandmarked"@en , "랜드마크 구분"@ko-KR ;
        rdfs:range             xsd:boolean ;
        schema:domainIncludes  <https://w3id.org/product/Building> .

props:supplyAirTemperatureHeating
        a                      owl:DatatypeProperty ;
        rdfs:comment           "暖房時の給気温度"@ja-JP , "Température de l'air soufflé en mode chauffage"@fr-FR , "Supply air temperature in heating mode."@en ;
        rdfs:label             "暖房給気温度"@ja-JP , "supplyAirTemperatureHeating"@en , "Température de l'air soufflé en chauffage"@fr-FR ;
        rdfs:range             <https://w3id.org/product/TimeSeries> ;
        rdfs:range             [ owl:allValuesFrom  <https://w3id.org/measurement/thermodynamicTemperature> ;
                                 owl:onProperty     <https://w3id.org/measurement/seriesOf>
                               ] ;
        schema:domainIncludes  <https://w3id.org/product/AirTerminal> .

props:nominalSupplyWaterTemperatureCooling
        a                      owl:DatatypeProperty ;
        rdfs:comment           "Nominal supply water temperature (refers to nominal cooling capacity)."@en ;
        rdfs:label             "nominalSupplyWaterTemperatureCooling"@en ;
        rdfs:range             <https://w3id.org/measurement/thermodynamicTemperature> ;
        schema:domainIncludes  <https://w3id.org/product/CooledBeam> .

props:reinforcementVolumeRatio
        a                      owl:DatatypeProperty ;
        rdfs:comment           "The required ratio of the effective mass of the reinforcement to the effective volume of the concrete of a reinforced concrete structural element."@en , "Das geforderte Verhältnis der effektiven Masse der Bewehrung im Verhältnis zur effektiven Masse des Betons für dieses Element."@de-DE ;
        rdfs:label             "reinforcementVolumeRatio"@en , "Bewehrungsgrad Volumen"@de-DE ;
        rdfs:range             <https://w3id.org/measurement/massDensity> ;
        schema:domainIncludes  <https://w3id.org/product/BuildingElement> .

props:compressorCapacity
        a                      owl:DatatypeProperty ;
        rdfs:comment           "The product of the  ideal capacity and the overall volumetric efficiency of the compressor."@en , "Le produit de la puissance optimale par le rendement global du compresseur."@fr-FR ;
        rdfs:label             "compressorCapacity"@en , "PuissanceCompresseur"@fr-FR ;
        rdfs:range             <https://w3id.org/product/TimeSeries> ;
        rdfs:range             [ owl:allValuesFrom  <https://w3id.org/measurement/power> ;
                                 owl:onProperty     <https://w3id.org/measurement/seriesOf>
                               ] ;
        schema:domainIncludes  <https://w3id.org/product/Compressor> .

props:airSideSystemDistributionType
        rdfs:comment           "This enumeration defines the basic types of air side systems (e.g., SingleDuct, DualDuct, Multizone, etc.)."@en , "基本的な空調方式（単一ダクト、二重ダクト、マルチゾーン等）。"@ja-JP , "기본적인 공조 방식 (단일 덕트, 이중 덕트, 멀티존 등)"@ko-KR ;
        rdfs:label             "airSideSystemDistributionType"@en , "搬送方式"@ja-JP , "반송방식"@ko-KR ;
        schema:domainIncludes  bot:Zone .

props:combustible  a           owl:DatatypeProperty ;
        rdfs:comment           "German-description-4"@de-DE , "Indique si l'objet est réalisé à partir de matériau combustible (VRAI) ou non (FAUX)."@fr-FR , "Angabe ob das Bauteil brennbares Material enthält (WAHR) oder nicht (FALSCH)."@de-DE , "この部材が可燃性物質で作られているかどうかを示すブーリアン値。"@ja-JP , "Indication whether the object is made from combustible material (TRUE) or not (FALSE)."@en , "表示该构件是否由可燃材料制成。"@zh-CN ;
        rdfs:label             "combustible"@en , "可燃性区分"@ja-JP , "是否可燃"@zh-CN , "Combustible"@fr-FR , "Brennbares Material"@de-DE ;
        rdfs:range             xsd:boolean ;
        schema:domainIncludes  <https://w3id.org/product/CurtainWall> , <https://w3id.org/product/Covering> .

props:loadBearingCapacity
        a                      owl:DatatypeProperty ;
        rdfs:comment           "Maximum load bearing capacity of the floor structure throughtout the storey as designed."@en , "Maximale Deckentragfähigkeit in diesem Geschoss."@de-DE , "Capacité porteuse maximale de la structure du plancher tel que conçu pour cet étage."@fr-FR ;
        rdfs:label             "loadBearingCapacity"@en , "Deckentragfähigkeit"@de-DE , "Capacité porteuse"@fr-FR ;
        rdfs:range             <https://w3id.org/measurement/planarForce> ;
        schema:domainIncludes  <https://w3id.org/product/BuildingStorey> .

props:airPressureDropCurve
        a                      owl:ObjectProperty ;
        rdfs:comment           "Air pressure drop curve, pressure drop – flow rate curve, AirPressureDrop = f (AirflowRate)."@en , "Courbe de perte de charge aéraulique, courbe perte de charge/débit."@fr-FR ;
        rdfs:label             "airPressureDropCurve"@en , "CourbePerteDeChargeAir"@fr-FR ;
        rdfs:range             <https://w3id.org/measurement/TimeSeries> ;
        schema:domainIncludes  <https://w3id.org/product/Coil> .

props:numberOfActors  a        owl:DatatypeProperty ;
        rdfs:comment           "The number of actors that are to be dealt with together in the population."@en , "母集団において取り扱われる関与者の数。"@ja-JP , "该组参与者的总数。"@zh-CN ;
        rdfs:label             "numberOfActors"@en , "関与者数"@ja-JP , "参与者数"@zh-CN ;
        rdfs:range             <https://w3id.org/measurement/count> ;
        schema:domainIncludes  <https://w3id.org/product/Actor> .

props:hasIntegralControl
        a                      owl:DatatypeProperty ;
        rdfs:comment           "If TRUE, a self powered temperature control is included in the AirTerminal."@en , "もし真なら、ターミナルに自身による温度制御が含まれる"@ja-JP , "Si VRAI, une commande interne de la température est incluse dans le terminal de ventilation."@fr-FR ;
        rdfs:label             "hasIntegralControl"@en , "自己制御有無"@ja-JP , "PossèdeContrôleTotal"@fr-FR ;
        rdfs:range             xsd:boolean ;
        schema:domainIncludes  <https://w3id.org/product/AirTerminal> .

props:isMountedFlatCable
        a                      owl:DatatypeProperty ;
        rdfs:comment           "Indication of whether the cable occurrences are mounted flat (= TRUE) or in a trefoil pattern (= FALSE)."@en ;
        rdfs:label             "isMountedFlatCable"@en ;
        rdfs:range             xsd:boolean ;
        schema:domainIncludes  <https://w3id.org/product/CableSegment> .

props:inputPower  a            owl:DatatypeProperty ;
        rdfs:comment           "Input power to the compressor motor."@en , "Puissance fournie au moteur du compresseur."@fr-FR ;
        rdfs:label             "inputPower"@en , "PuissanceEntréeMoteur"@fr-FR ;
        rdfs:range             <https://w3id.org/product/TimeSeries> ;
        rdfs:range             [ owl:allValuesFrom  <https://w3id.org/measurement/power> ;
                                 owl:onProperty     <https://w3id.org/measurement/seriesOf>
                               ] ;
        schema:domainIncludes  <https://w3id.org/product/Compressor> .

props:mediaSource  a           owl:DatatypeProperty ;
        rdfs:comment           "미디어 소스 정의된 유형 (IfcDistributionPort with FlowDirection = SINK and PredefinedType = AUDIOVISUAL) 및 audio / video 구성 집합에 해당하는 이름."@ko-KR , "メディアソースと定義済みタイプ(IfcDistributionPort with FlowDirection=SINK and PredefinedType=AUDIOVISUAL)及びaudio/videoを構成する集合に対応する名前。"@ja-JP , "Indicates the media source where the identifier corresponds to an entry within the table of available media sources on Pset_AudioVisualApplianceTypeCommon.MediaSource."@en , "Indicates media sources and corresponding names of ports (IfcDistributionPort with FlowDirection=SINK and PredefinedType=AUDIOVISUAL) or aggregated audio/video components (IfcAudioVisualAppliance)."@en ;
        rdfs:label             "미디어 소스"@ko-KR , "メディアソース"@ja-JP , "mediaSource"@en ;
        rdfs:range             <https://w3id.org/product/TimeSeries> ;
        rdfs:range             [ owl:allValuesFrom  xsd:string ;
                                 owl:onProperty     <https://w3id.org/measurement/seriesOf>
                               ] ;
        schema:domainIncludes  <https://w3id.org/product/AudioVisualAppliance> .

props:isOutdoors  a            owl:DatatypeProperty ;
        rdfs:comment           "Indicates if camera is designed to be used outdoors."@en , "屋外利用が可能かどうかを示す。"@ja-JP , "옥외 이용이 가능한지 여부를 나타냅니다."@ko-KR ;
        rdfs:label             "isOutdoors"@en , "屋外対応の可否"@ja-JP , "실외 여부"@ko-KR ;
        rdfs:range             xsd:boolean ;
        schema:domainIncludes  <https://w3id.org/product/AudioVisualAppliance#CAMERA> .

props:maximumOperatingTemperature
        a                      owl:DatatypeProperty ;
        rdfs:comment           "The maximum temperature at which a cable or bus is certified to operate."@en , "ケーブルや母線の最大動作温度を示す。"@ja-JP , "케이블과 모선의 최대 작동 온도를 나타낸다."@ko-KR ;
        rdfs:label             "maximumOperatingTemperature"@en , "許容最高温度"@ja-JP , "허용 최고 온도"@ko-KR ;
        rdfs:range             <https://w3id.org/measurement/thermodynamicTemperature> ;
        schema:domainIncludes  <https://w3id.org/product/CableSegment#CABLESEGMENT> .

props:requestSourceName
        a                      owl:ObjectProperty ;
        rdfs:comment           "The person making the request, where known."@en , "要請源の識別を確認するための特定の名称またはラベル。電子メールの場合、電子メールアドレスに相当する。"@ja-JP ;
        rdfs:label             "requestSourceName"@en , "要請ソースラベル"@ja-JP ;
        rdfs:range             foaf:Person ;
        schema:domainIncludes  <https://w3id.org/product/ActionRequest> .

props:heatingWaterFlowRate
        a                      owl:DatatypeProperty ;
        rdfs:comment           "Water flow rate for heating."@en ;
        rdfs:label             "heatingWaterFlowRate"@en ;
        rdfs:range             <https://w3id.org/product/TimeSeries> ;
        rdfs:range             [ owl:allValuesFrom  <https://w3id.org/measurement/volumetricFlowRate> ;
                                 owl:onProperty     <https://w3id.org/measurement/seriesOf>
                               ] ;
        schema:domainIncludes  <https://w3id.org/product/CooledBeam> .

props:soundCurve  a            owl:ObjectProperty ;
        rdfs:comment           "Regenerated sound versus air-flow rate."@en , "Son généré par rapport au débit aéraulique."@fr-FR ;
        rdfs:label             "soundCurve"@en , "CourbeSon"@fr-FR ;
        rdfs:range             <https://w3id.org/measurement/TimeSeries> ;
        schema:domainIncludes  <https://w3id.org/product/Coil> .

props:contourValue  a          owl:DatatypeProperty ;
        rdfs:comment           "Valeur de l'élévation du contour au dessus ou au dessous d'un plan de référence."@fr-FR , "Value of the elevation of the contour above or below a reference plane."@en , "参照平面に対する等高線の高さ値。"@ja-JP , "참조 평면에 대한 등고선의 높이 값."@ko-KR ;
        rdfs:label             "contourValue"@en , "ValeurContour"@fr-FR , "등고선 값"@ko-KR , "等高線値"@ja-JP ;
        rdfs:range             <https://w3id.org/measurement/length> ;
        schema:domainIncludes  <https://w3id.org/product/Annotation#ContourLine> .

props:roadVisibleDistanceLeft
        a                      owl:DatatypeProperty ;
        rdfs:comment           "Distance visible to the left of the access."@en , "Distance de visibilité à la gauche de l'accès."@fr-FR , "左側の経路に可視出来る距離。"@ja-JP ;
        rdfs:label             "roadVisibleDistanceLeft"@en , "DistanceVisibiliteCoteGauche"@fr-FR , "左側道路可視距離"@ja-JP ;
        rdfs:range             <https://w3id.org/measurement/positiveLength> ;
        schema:domainIncludes  <https://w3id.org/product/Annotation#LineOfSight> .

props:lightingDiversity
        a                      owl:DatatypeProperty ;
        rdfs:comment           "Lighting diversity."@en , "照明負荷係数。"@ja-JP , "조명 부하 계수"@ko-KR ;
        rdfs:label             "lightingDiversity"@en , "照明負荷係数"@ja-JP , "조명부하계수"@ko-KR ;
        rdfs:range             <https://w3id.org/measurement/positiveRatio> ;
        schema:domainIncludes  bot:Zone .

props:internalRefrigerantVolume
        a                      owl:DatatypeProperty ;
        rdfs:comment           "Internal volume of condenser (refrigerant side)."@en ;
        rdfs:label             "internalRefrigerantVolume"@en ;
        rdfs:range             <https://w3id.org/measurement/volume> ;
        schema:domainIncludes  <https://w3id.org/product/Condenser> .

props:audioVolume  a           owl:DatatypeProperty ;
        rdfs:comment           "Indicates discrete audio volume levels and corresponding sound power offsets, if applicable.  Missing values may be interpolated."@en , "Indicates the audio volume level where the integer level corresponds to an entry or interpolation within Pset_AudioVisualApplianceTypeCommon.AudioVolume."@en ;
        rdfs:label             "audioVolume"@en ;
        rdfs:range             <https://w3id.org/product/TimeSeries> ;
        rdfs:range             [ owl:allValuesFrom  xsd:int ;
                                 owl:onProperty     <https://w3id.org/measurement/seriesOf>
                               ] ;
        schema:domainIncludes  <https://w3id.org/product/AudioVisualAppliance> .

props:skillLevel  a            owl:DatatypeProperty ;
        rdfs:comment           "Skill level exhibited by the actor and which indicates an extent of their capability to perform actions on the artefacts upon which they can act."@en , "関与者が示すスキルレベル（技能・技量段階）、および実行されるアクションへの能力を示すもの。"@ja-JP , "参与者具备的技能的等级，即他们在专业领域内所能展示的能力。"@zh-CN ;
        rdfs:label             "skillLevel"@en , "技能段階"@ja-JP , "技能等级"@zh-CN ;
        rdfs:range             xsd:string ;
        schema:domainIncludes  <https://w3id.org/product/Actor> .

props:loadBearing  a           owl:DatatypeProperty ;
        rdfs:comment           "荷重に関係している部材かどうかを示すブーリアン値。"@ja-JP , "オブジェクトが荷重を保持するか（TRUE）、保持しないか（FALSE）を示す。"@ja-JP , "Indicates whether the object is intended to carry loads (TRUE) or not (FALSE)."@en , "Angabe, ob dieses Bauteil tragend ist (JA) oder nichttragend (NEIN)"@de-DE , "Indique si l'objet est censé porter des charges (VRAI) ou non (FAUX)."@fr-FR , "表示该对象是否需要承重。"@zh-CN ;
        rdfs:label             "耐力部材"@ja-JP , "loadBearing"@en , "Tragendes Bauteil"@de-DE , "Porteur"@fr-FR , "是否承重"@zh-CN ;
        rdfs:range             xsd:boolean ;
        schema:domainIncludes  <https://w3id.org/product/Chimney> , <https://w3id.org/product/BuildingElementProxy> , <https://w3id.org/product/Beam> , <https://w3id.org/product/Column> .

props:tunerType  rdfs:comment  "Indicates the tuner type."@en , "チューナータイプを示す。"@ja-JP , "튜너 타입을 나타낸다"@ko-KR ;
        rdfs:label             "tunerType"@en , "チューナータイプ"@ja-JP , "튜너 타입"@ko-KR ;
        schema:domainIncludes  <https://w3id.org/product/AudioVisualAppliance#TUNER> .

props:isWaterStorageHeater
        a                      owl:DatatypeProperty ;
        rdfs:comment           "This is used to identify if the boiler has storage capacity (TRUE). If FALSE, then there is no storage capacity built into the boiler, such as an instantaneous hot water heater."@en , "給湯用の缶体があればTRUE、（瞬間湯沸かし器のように）ボイラにタンクがなければFALSE"@ja-JP , "Utilisé pour identifier si la chaudière une capacité de réserve en eau (VRAI). Si FAUX, alors il n'y a pas de capacité de réserve intégrée dans la chaudière, tel qu'un chauffe-eau instantané."@fr-FR ;
        rdfs:label             "isWaterStorageHeater"@en , "給湯タンク有無"@ja-JP , "AvoirChauffeEau"@fr-FR ;
        rdfs:range             xsd:boolean ;
        schema:domainIncludes  <https://w3id.org/product/Boiler> .

props:maximumShortCircuitTemperature
        a                      owl:DatatypeProperty ;
        rdfs:comment           "The maximum short circuit temperature at which a cable or bus is certified to operate."@en , "ケーブルや母線の最大短絡温度を示す。"@ja-JP , "케이블과 모선의 최대 단락 온도를 나타낸다."@ko-KR ;
        rdfs:label             "maximumShortCircuitTemperature"@en , "短絡許容最高温度"@ja-JP , "단락 허용 최고 온도"@ko-KR ;
        rdfs:range             <https://w3id.org/measurement/thermodynamicTemperature> ;
        schema:domainIncludes  <https://w3id.org/product/CableSegment#CABLESEGMENT> .

props:assetAccountingType
        rdfs:comment           "Identifies the predefined types of risk from which the type required may be set."@en , "会計の定義済み種別。"@ja-JP ;
        rdfs:label             "assetAccountingType"@en , "資産会計種別"@ja-JP ;
        schema:domainIncludes  <https://w3id.org/product/Asset> .

props:sensibleEffectivenessTable
        a                      owl:ObjectProperty ;
        rdfs:comment           "Sensible heat transfer effectiveness curve as a function of the primary and secondary air flow rate."@en , "一次と二次空気量の関数としての顕熱交換効率曲線"@ja-JP , "Courbe d'efficacité d'échange thermique sensible, en tant que fonction du débit d'air au primaire et débit d'air au secondaire"@fr-FR ;
        rdfs:label             "sensibleEffectivenessTable"@en , "顕熱効率テーブル"@ja-JP , "DiagrammeEfficacitéSensible"@fr-FR ;
        rdfs:range             <https://w3id.org/measurement/TimeSeries> ;
        schema:domainIncludes  <https://w3id.org/product/AirToAirHeatRecovery> .

props:tiltVertical  rdfs:comment  "Indicates vertical range for pivoting, where 0.0 is level, +90 degrees is looking up, -90 degrees is looking down."@en , "チルト垂直の可動角度を示す。"@ja-JP ;
        rdfs:label             "tiltVertical"@en , "チルト垂直方向可動角度"@ja-JP ;
        schema:domainIncludes  <https://w3id.org/product/AudioVisualAppliance#CAMERA> .

props:fusibleLinkTemperature
        a                      owl:DatatypeProperty ;
        rdfs:comment           "The temperature that the fusible link melts."@en ;
        rdfs:label             "fusibleLinkTemperature"@en ;
        rdfs:range             <https://w3id.org/measurement/thermodynamicTemperature> ;
        schema:domainIncludes  <https://w3id.org/product/Damper#FIRESMOKEDAMPER> , <https://w3id.org/product/Damper#FIREDAMPER> .

props:regeneratedSoundCurve
        rdfs:comment           "Regenerated sound versus air flow rate."@en ;
        rdfs:label             "regeneratedSoundCurve"@en ;
        schema:domainIncludes  <https://w3id.org/product/Damper> .

props:nominalWaterFlowCooling
        a                      owl:DatatypeProperty ;
        rdfs:comment           "Nominal water flow (refers to nominal cooling capacity)."@en ;
        rdfs:label             "nominalWaterFlowCooling"@en ;
        rdfs:range             <https://w3id.org/measurement/volumetricFlowRate> ;
        schema:domainIncludes  <https://w3id.org/product/CooledBeam> .

props:frictionHeatGain
        a                      owl:DatatypeProperty ;
        rdfs:comment           "Friction heat gain."@en , "Gain thermique par friction."@fr-FR ;
        rdfs:label             "frictionHeatGain"@en , "GainThermiqueFriction"@fr-FR ;
        rdfs:range             <https://w3id.org/product/TimeSeries> ;
        rdfs:range             [ owl:allValuesFrom  <https://w3id.org/measurement/power> ;
                                 owl:onProperty     <https://w3id.org/measurement/seriesOf>
                               ] ;
        schema:domainIncludes  <https://w3id.org/product/Compressor> .

props:applianceDiversity
        a                      owl:DatatypeProperty ;
        rdfs:comment           "Diversity of appliance load."@en , "機器の負荷率。"@ja-JP , "기기의 부하율"@ko-KR ;
        rdfs:label             "applianceDiversity"@en , "機器の負荷率"@ja-JP , "기기의 부하율"@ko-KR ;
        rdfs:range             <https://w3id.org/measurement/positiveRatio> ;
        schema:domainIncludes  bot:Zone .

props:placementType  rdfs:comment  "Indicates the placement of the coil.  \nFLOOR indicates an under floor heater (if coil type is WATERHEATINGCOIL or ELECTRICHEATINGCOIL); \nCEILING indicates a cooling ceiling (if coil type is WATERCOOLINGCOIL);\nUNIT indicates that the coil is part of a cooling or heating unit, like cooled beam, etc."@en , "Précise l'implantation de la batterie.\nPLANCHER indique que c'est un plancher chauffant (si le type de batterie is BATTERIEEAUCHAUDE ou CABLECHAUFFANTLECTRIQUE);\nPLAFOND indique un plafond rafraïchissant (si le type de la batterie est BATTERIEEAUFROIDE); UNITE indique que la batterie fait partie d'une unité de chauffage ou de refroidissement, tel que poutre froide, etc."@fr-FR ;
        rdfs:label             "placementType"@en , "TypeImplantation"@fr-FR ;
        schema:domainIncludes  <https://w3id.org/product/Coil> .

props:selfExtinguishing60332_3
        a                      owl:DatatypeProperty ;
        rdfs:comment           "自己消化ケーブル/コアはIEC 60332.3.に準じる。"@ja-JP , "Self Extinguishing cable/core according to IEC 60332.3."@en , "IEC 60332.3.에 규정되어있는 자기 소화 케이블"@ko-KR , "자기 소화 케이블 / 코어는 IEC 60332.3.에 준한다."@ko-KR , "IEC 60332.3.に規定されている自己消火ケーブル。"@ja-JP ;
        rdfs:label             "자기 소화 케이블"@ko-KR , "자동 소화 60332_3"@ko-KR , "自動消火60332_3"@ja-JP , "selfExtinguishing60332_3"@en , "自己消火ケーブル"@ja-JP ;
        rdfs:range             xsd:boolean ;
        schema:domainIncludes  <https://w3id.org/product/CableSegment#CORESEGMENT> , <https://w3id.org/product/CableSegment#CABLESEGMENT> .

props:vacancyRateInCategoryFuture
        a                      owl:DatatypeProperty ;
        rdfs:comment           "Percentage of vacancy found in the particular category expected in the future."@en , "Taux de vacance attendu dans le futur pour la catégorie."@fr-FR ;
        rdfs:label             "vacancyRateInCategoryFuture"@en , "TauxVacanceFuturParCategorie"@fr-FR ;
        rdfs:range             <https://w3id.org/measurement/positiveRatio> ;
        schema:domainIncludes  <https://w3id.org/product/Building> .

props:coilFluidArrangement
        rdfs:comment           "Fluid flow arrangement of the coil.\n\nCrossCounterFlow: Air and water flow enter in different directions.\nCrossFlow: Air and water flow are perpendicular.\nCrossParallelFlow: Air and water flow enter in same directions."@en , "Disposition du flux du fluide dans la batterie."@fr-FR ;
        rdfs:label             "coilFluidArrangement"@en , "DispositionFluideBatterie"@fr-FR ;
        schema:domainIncludes  <https://w3id.org/product/Coil> .

props:finishColor  a           owl:DatatypeProperty ;
        rdfs:comment           "La couleur de finition du terminal de ventilation."@fr-FR , "ターミナルの仕上げ色"@ja-JP , "The finish color for the air terminal."@en , "Finish color for cooled beam."@en ;
        rdfs:label             "finishColor"@en , "仕上げ色"@ja-JP , "CouleurFinition"@fr-FR ;
        rdfs:range             xsd:string ;
        schema:domainIncludes  <https://w3id.org/product/AirTerminal> , <https://w3id.org/product/CooledBeam> .

props:zoom  rdfs:comment       "Indicates the zoom range."@en , "ズーム可能範囲（倍率）を示す。"@ja-JP ;
        rdfs:label             "zoom"@en , "ズーム"@ja-JP ;
        schema:domainIncludes  <https://w3id.org/product/AudioVisualAppliance#CAMERA> .

props:signalFactor  a          owl:DatatypeProperty ;
        rdfs:comment           "Factor multiplied onto offset signal."@en , "인자는 오프셋 신호 곱셈"@ko-KR ;
        rdfs:label             "signalFactor"@en , "요소"@ko-KR ;
        rdfs:range             xsd:decimal ;
        schema:domainIncludes  <https://w3id.org/product/Controller#FLOATING> .

props:beamCoolingCapacity
        a                      owl:DatatypeProperty ;
        rdfs:comment           "Cooling capacity of beam. This excludes cooling capacity of supply air."@en ;
        rdfs:label             "beamCoolingCapacity"@en ;
        rdfs:range             <https://w3id.org/product/TimeSeries> ;
        rdfs:range             [ owl:allValuesFrom  <https://w3id.org/measurement/power> ;
                                 owl:onProperty     <https://w3id.org/measurement/seriesOf>
                               ] ;
        schema:domainIncludes  <https://w3id.org/product/CooledBeam> .

props:quality  a               owl:DatatypeProperty ;
        rdfs:comment           "計測の品質を示す値。"@ja-JP , "요청한 액츄에이터의 안전 장치 유형을 표시"@ko-KR , "시간이 지남에 값을 나타내는 Pset_ControllerTypeValue.Value에 대응 ※ 설정 가능한 정보는 IfcTimeSeries 속성 참조"@ko-KR , "Indicates the quality of measurement or failure condition, which may be further qualified by the Status.  True: measured values are considered reliable; False: measured values are considered not reliable (i.e. a fault has been detected); Unknown: reliability of values is uncertain."@en ;
        rdfs:label             "페일 세이프 유형"@ko-KR , "기본 출력 시계열 상수"@ko-KR , "quality"@en , "品質"@ja-JP ;
        rdfs:range             <https://w3id.org/product/TimeSeries> ;
        rdfs:range             [ owl:allValuesFrom  xsd:boolean ;
                                 owl:onProperty     <https://w3id.org/measurement/seriesOf>
                               ] ;
        rdfs:range             [ owl:allValuesFrom  xsd:boolean ;
                                 owl:onProperty     <https://w3id.org/measurement/seriesOf>
                               ] ;
        schema:domainIncludes  <https://w3id.org/product/Controller> , <https://w3id.org/product/Actuator> .

props:circuitType  rdfs:comment  "OpenCircuit: Exposes water directly to the cooling atmosphere.\nCloseCircuit: The fluid is separated from the atmosphere by a heat exchanger.\nWet: The air stream or the heat exchange surface is evaporatively cooled.\nDry: No evaporation into the air stream.\nDryWet: A combination of a dry tower and a wet tower."@en ;
        rdfs:label             "circuitType"@en ;
        schema:domainIncludes  <https://w3id.org/product/CoolingTower> .

props:workingPressure
        a                      owl:DatatypeProperty ;
        rdfs:comment           "Pression de fonctionnement de la chaudière."@fr-FR , "ボイラ運転圧力"@ja-JP , "Boiler working pressure."@en ;
        rdfs:label             "workingPressure"@en , "作動圧力"@ja-JP , "PressionFonctionnement"@fr-FR ;
        rdfs:range             <https://w3id.org/product/TimeSeries> ;
        rdfs:range             [ owl:allValuesFrom  <https://w3id.org/measurement/pressure> ;
                                 owl:onProperty     <https://w3id.org/measurement/seriesOf>
                               ] ;
        schema:domainIncludes  <https://w3id.org/product/Boiler> .

props:waterInletTemperatureRange
        rdfs:comment           "Allowable water inlet temperature range."@en , "入口水温範囲"@ja-JP , "Plage de température de l'alimentation en eau admissible"@fr-FR ;
        rdfs:label             "waterInletTemperatureRange"@en , "入口水温範囲"@ja-JP , "PlageTempératureAlimentationEau"@fr-FR ;
        schema:domainIncludes  <https://w3id.org/product/Boiler> .

props:audioMode  rdfs:comment  "Indicates audio sound modes and corresponding labels, if applicable."@en , "オーディオサウンドモードの設定。"@ja-JP , "오디오 사운드 모드 설정."@ko-KR ;
        rdfs:label             "audioMode"@en , "オーディオモード"@ja-JP , "오디오 모드"@ko-KR ;
        schema:domainIncludes  <https://w3id.org/product/AudioVisualAppliance#RECEIVER> , <https://w3id.org/product/AudioVisualAppliance#DISPLAY> , <https://w3id.org/product/AudioVisualAppliance#AMPLIFIER> .

props:compressorSpeed
        a                      owl:DatatypeProperty ;
        rdfs:comment           "Compressor speed."@en , "Vitesse du compresseur"@fr-FR ;
        rdfs:label             "compressorSpeed"@en , "VitesseCompresseur"@fr-FR ;
        rdfs:range             <https://w3id.org/measurement/rotationalFrequency> ;
        schema:domainIncludes  <https://w3id.org/product/Compressor> .

props:orientation  rdfs:comment  "The intended orientation for the damper as specified by the manufacturer."@en ;
        rdfs:label             "orientation"@en ;
        schema:domainIncludes  <https://w3id.org/product/Damper> .

props:faceArea  a              owl:DatatypeProperty ;
        rdfs:comment           "Face area open to the airstream."@en ;
        rdfs:label             "faceArea"@en ;
        rdfs:range             <https://w3id.org/measurement/area> ;
        schema:domainIncludes  <https://w3id.org/product/Damper> .

props:airFlowRate  a           owl:DatatypeProperty ;
        rdfs:comment           "The actual airflow rate as designed."@en , "Air flow rate."@en , "Volumetric flow rate."@en , "Débit d'air volumique"@fr-FR , "送風量"@ja-JP ;
        rdfs:label             "airFlowRate"@en , "風量"@ja-JP , "Débit d'air"@fr-FR ;
        rdfs:range             <https://w3id.org/product/TimeSeries> , <https://w3id.org/measurement/volumetricFlowRate> ;
        rdfs:range             [ owl:allValuesFrom  <https://w3id.org/measurement/volumetricFlowRate> ;
                                 owl:onProperty     <https://w3id.org/measurement/seriesOf>
                               ] ;
        rdfs:range             [ owl:allValuesFrom  <https://w3id.org/measurement/volumetricFlowRate> ;
                                 owl:onProperty     <https://w3id.org/measurement/seriesOf>
                               ] ;
        rdfs:range             [ owl:allValuesFrom  <https://w3id.org/measurement/volumetricFlowRate> ;
                                 owl:onProperty     <https://w3id.org/measurement/seriesOf>
                               ] ;
        schema:domainIncludes  <https://w3id.org/product/AirTerminal> , <https://w3id.org/product/Damper> , <https://w3id.org/product/CooledBeam#ACTIVE> .
