@prefix schema: <http://schema.org/> .
@prefix prod:  <https://w3id.org/product#> .
@prefix owl:   <http://www.w3.org/2002/07/owl#> .
@prefix xsd:   <http://www.w3.org/2001/XMLSchema#> .
@prefix sgfn:  <http://w3id.org/sparql-generate/fn/> .
@prefix voaf:  <http://purl.org/vocommons/voaf#> .
@prefix rdfs:  <http://www.w3.org/2000/01/rdf-schema#> .
@prefix props: <https://w3id.org/product/props/> .
@prefix ex:    <http://example.org/> .
@prefix rdf:   <http://www.w3.org/1999/02/22-rdf-syntax-ns#> .
@prefix sgiter: <http://w3id.org/sparql-generate/iter/> .
@prefix dcterms: <http://purl.org/dc/terms/> .
@prefix vann:  <http://purl.org/vocab/vann/> .
@prefix vs:    <http://www.w3.org/2003/06/sw-vocab-status/ns#> .
@prefix foaf:  <http://xmlns.com/foaf/0.1/> .

props:columnShoeCasingHeight
        a                      owl:DatatypeProperty ;
        rdfs:comment           "The height of the column shoe casing."@en , "柱脚ケーシングの板厚。"@ja-JP , "기둥 다리 케이스의 두께"@ko-KR ;
        rdfs:label             "columnShoeCasingHeight"@en , "ケーシング厚"@ja-JP , "케이스 두께"@ko-KR ;
        rdfs:range             <https://w3id.org/product/PositiveLengthMeasure> ;
        schema:domainIncludes  <https://w3id.org/product/DiscreteAccessory%2FSHOE> .

props:bulbLiquidColor
        a                      owl:DatatypeProperty ;
        rdfs:comment           "The color of the liquid in the bulb for a bulb activated sprinkler. Note that the liquid color varies according to the activation temperature requirement of the sprinkler head. Note also that this property does not need to be asserted for quick response activated sprinklers."@en , "バルブ作動スプリンクラーのバルブ液体色の設定。液体色は、スプリンクラーヘッドの作動温度に応じて変化する。また、この属性は、高速応答スプリンクラーは設定する必要はない。"@ja-JP ;
        rdfs:label             "bulbLiquidColor"@en , "バルブ液体色"@ja-JP ;
        schema:domainIncludes  <https://w3id.org/product/FireSuppressionTerminal%2FSPRINKLER> .

props:columnShoeBasePlateWidth
        a                      owl:DatatypeProperty ;
        rdfs:comment           "The width of the column shoe base plate."@en , "柱脚ベースプレートの幅。"@ja-JP , "기둥 다리 받침판 폭"@ko-KR ;
        rdfs:label             "columnShoeBasePlateWidth"@en , "ベースプレート幅"@ja-JP , "베이스 플레이트 폭"@ko-KR ;
        rdfs:range             <https://w3id.org/product/PositiveLengthMeasure> ;
        schema:domainIncludes  <https://w3id.org/product/DiscreteAccessory%2FSHOE> .

props:reasonForChange
        a                      owl:DatatypeProperty ;
        rdfs:comment           "A description of the problem for why a change is needed."@en , "変更が必要となる問題の記述。"@ja-JP ;
        rdfs:label             "reasonForChange"@en , "変更理由"@ja-JP ;
        rdfs:range             xsd:string ;
        schema:domainIncludes  <https://w3id.org/product/ProjectOrder%2FCHANGEORDER> .

props:surface2  a              owl:DatatypeProperty ;
        rdfs:comment           "See Surface1."@en ;
        rdfs:label             "surface2"@en ;
        rdfs:range             xsd:string ;
        schema:domainIncludes  <https://w3id.org/product/Fastener%2FWELD> .

props:heatTransferMedium
        a                      owl:DatatypeProperty ;
        rdfs:comment           "Enumeration defining the heat transfer medium if applicable."@en , "列挙体は熱媒体を必要に応じて定義します。"@ja-JP ;
        rdfs:label             "heatTransferMedium"@en , "熱媒体"@ja-JP ;
        schema:domainIncludes  <https://w3id.org/product/SpaceHeater> .

props:nutShape  a              owl:DatatypeProperty ;
        rdfs:comment           "Shape of the nut, e.g. 'Hexagon', 'Cap', 'Castle', 'Wing'"@en ;
        rdfs:label             "nutShape"@en ;
        rdfs:range             xsd:string ;
        schema:domainIncludes  <https://w3id.org/product/MechanicalFastener%2FBOLT> .

props:dryBulbTemperature
        a                      owl:DatatypeProperty ;
        rdfs:comment           "Dry bulb temperature of the air."@en , "乾球温度による熱負荷。"@ja-JP , "건구온도에의한 열부하"@ko-KR , "Loads from the dry bulb temperature."@en ;
        rdfs:label             "乾球温度"@ja-JP , "dryBulbTemperature"@en , "건구온도"@ko-KR ;
        schema:domainIncludes  <https://w3id.org/product/DistributionPort%2FAIRCONDITIONING> , <https://w3id.org/product/Space> .

props:formStrippingStrength
        a                      owl:DatatypeProperty ;
        rdfs:comment           "The minimum required compressive strength of the concrete at form stripping time."@en , "脱型時におけるコンクリートの最小必要圧縮強度。"@ja-JP ;
        rdfs:label             "formStrippingStrength"@en , "脱型強度"@ja-JP ;
        rdfs:range             <https://w3id.org/product/PressureMeasure> ;
        schema:domainIncludes  <https://w3id.org/product/BuildingElement> .

props:volumetricFlowRate
        a                      owl:DatatypeProperty ;
        rdfs:comment           "流体の体積流量。"@ja-JP , "The volumetric flow rate of the fluid."@en ;
        rdfs:label             "体積流量"@ja-JP , "volumetricFlowRate"@en ;
        schema:domainIncludes  <https://w3id.org/product/DistributionPort%2FCHEMICAL> , <https://w3id.org/product/DistributionPort%2FAIRCONDITIONING> .

props:current  a               owl:DatatypeProperty ;
        rdfs:comment           "The actual current and operable range."@en , "実電流と動作可能範囲。"@ja-JP , "Log of electrical current."@en , "電流のログ。"@ja-JP ;
        rdfs:label             "current"@en , "電流"@ja-JP ;
        schema:domainIncludes  <https://w3id.org/product/DistributionPort%2FELECTRICAL> .

props:housingThickness
        a                      owl:DatatypeProperty ;
        rdfs:comment           "Air terminal box housing material thickness."@en , "ターミナルのハウジング材の板厚"@ja-JP , "Epaisseur du matériau réalisant l'enveloppe du registre terminal de ventilation"@fr-FR ;
        rdfs:label             "housingThickness"@en , "ハウジング板厚"@ja-JP , "Epaisseur de l'enveloppe"@fr-FR ;
        rdfs:range             <https://w3id.org/product/LengthMeasure> ;
        schema:domainIncludes  <https://w3id.org/product/AirTerminalBox> .

props:airDiffusionPerformanceIndex
        a                      owl:DatatypeProperty ;
        rdfs:comment           "The Air Diffusion Performance Index (ADPI) is used for cooling mode conditions. If several measurements of air velocity and air temperature are made throughout the occupied zone of a space, the ADPI is the percentage of locations where measurements were taken that meet the specifications for effective draft temperature and air velocity."@en , "空気拡散性能指標（ADPI)は冷房時に使用される。\n空気速度および気温のいくつかの測定が空間の居住域の隅々でなされる場合、ADPIは有効な草案の温度および空気速度のための仕様に遭遇する測定が得られた位置の割合である。"@ja-JP , "L'Indice de Performance de Diffusion d'Air (ADPI) est utilisé pour des conditions en mode rafraîchissement. Si plusieurs mesures de vitesses et températures de l'air sont réalisées à travers toute une zone occupée d'un espace,  l'ADPI est le pourcentage des emplacements où les mesures ont été réalisées et qui vérifient les caractéristiques pour une température de courant d'air et de vitesse d'air effectives."@fr-FR ;
        rdfs:label             "airDiffusionPerformanceIndex"@en , "空気拡散性能指標"@ja-JP , "Indice de performance de diffusion de l'air"@fr-FR ;
        rdfs:range             xsd:decimal ;
        schema:domainIncludes  <https://w3id.org/product/AirTerminal> .

props:spaceTemperatureSummerMax
        a                      owl:DatatypeProperty ;
        rdfs:comment           "공간이나 영역 혹서 계절 (여름)의 최고 온도 이용자 / 설계자의 관점에서 요구된다."@ko-KR , "Maximal geforderte Raumtemperatur aus dem Raumprogramm für die Auslegung der Raumkühlung."@de-DE , "Maximal temperature of the space or zone for the hot (summer) period, that is required from user/designer view point and provided as requirement for cooling."@en , "空間またはゾーンの暑熱季(夏季)の最高温度。利用者/設計者の視点から要求される。"@ja-JP , "Température maximale de l'espace ou de la zone  en été. Spécifiée par l'usager ou le concepteur et utilisée comme consigne pour le refroidissement."@fr-FR ;
        rdfs:label             "spaceTemperatureSummerMax"@en , "Température maximale en été"@fr-FR , "여름최고온도"@ko-KR , "Raumtemperatur Kühlung Maximal"@de-DE , "夏季最高室内温度"@ja-JP ;
        rdfs:range             <https://w3id.org/product/ThermodynamicTemperatureMeasure> ;
        schema:domainIncludes  <https://w3id.org/product/Space> , <https://w3id.org/product/cSpatialZone> , <https://w3id.org/product/cZone> .

props:exteriorHeatTransferCoefficient
        a                      owl:DatatypeProperty ;
        rdfs:comment           "外表面に関連づけられた外表面熱交換係数"@ja-JP , "Exterior heat transfer coefficient associated with exterior surface area."@en ;
        rdfs:label             "外表面熱交換係数"@ja-JP , "exteriorHeatTransferCoefficient"@en ;
        schema:domainIncludes  <https://w3id.org/product/Evaporator> , <https://w3id.org/product/Condenser> .

props:contourValue  a          owl:DatatypeProperty ;
        rdfs:comment           "Valeur de l'élévation du contour au dessus ou au dessous d'un plan de référence."@fr-FR , "Value of the elevation of the contour above or below a reference plane."@en , "参照平面に対する等高線の高さ値。"@ja-JP , "참조 평면에 대한 등고선의 높이 값."@ko-KR ;
        rdfs:label             "contourValue"@en , "ValeurContour"@fr-FR , "등고선 값"@ko-KR , "等高線値"@ja-JP ;
        rdfs:range             <https://w3id.org/product/LengthMeasure> ;
        schema:domainIncludes  <https://w3id.org/product/Annotation%2FContourLine> .

props:volume  a                owl:DatatypeProperty ;
        rdfs:comment           "Total volume of fluid in the tubes and their headers."@en , "チューブとヘッダー内の総流量"@ja-JP ;
        rdfs:label             "volume"@en , "流量"@ja-JP ;
        rdfs:range             <https://w3id.org/product/VolumeMeasure> ;
        schema:domainIncludes  <https://w3id.org/product/TubeBundle> .

props:toggleSwitchType
        a                      owl:DatatypeProperty ;
        rdfs:comment           "A list of the available types of toggle switch from which that required may be selected."@en , "選択が必要となる、トグルスイッチの一覧リスト。"@ja-JP , "선택이 필요한 토글 스위치 목록"@ko-KR ;
        rdfs:label             "toggleSwitchType"@en , "レバースイッチタイプ"@ja-JP , "레버스위치 유형"@ko-KR ;
        schema:domainIncludes  <https://w3id.org/product/SwitchingDevice%2FTOGGLESWITCH> .

props:primaryAirflowRateRange
        a                      owl:DatatypeProperty ;
        rdfs:comment           "possible range of primary airflow that can be delivered.."@en , "一次側の送風可能範囲"@ja-JP , "Plage possible de débit d'air au primaire qui peut être fourni."@fr-FR ;
        rdfs:label             "primaryAirflowRateRange"@en , "一次側風量範囲"@ja-JP , "PlageDébitAirPrimaire"@fr-FR ;
        schema:domainIncludes  <https://w3id.org/product/AirToAirHeatRecovery> .

props:aspectRatio  a           owl:DatatypeProperty ;
        rdfs:comment           "The default aspect ratio."@en , "デフォルトアスペクト比。"@ja-JP , "기본 화면 비율."@ko-KR ;
        rdfs:label             "aspectRatio"@en , "アスペクト比"@ja-JP , "화면 비율"@ko-KR ;
        rdfs:range             xsd:decimal ;
        schema:domainIncludes  <https://w3id.org/product/DistributionSystem%2FVENTILATION> .

props:nominalSensibleCapacity
        a                      owl:DatatypeProperty ;
        rdfs:comment           "Nominal sensible capacity."@en , "Puissance sensible nominale."@fr-FR ;
        rdfs:label             "nominalSensibleCapacity"@en , "PuissanceSensibleNominale"@fr-FR ;
        rdfs:range             <https://w3id.org/product/PowerMeasure> ;
        schema:domainIncludes  <https://w3id.org/product/Coil> .

props:urinalType  a            owl:DatatypeProperty ;
        rdfs:comment           "Selection of the type of urinal from the enumerated list of types where:-\n\nBowl: Individual wall mounted urinal.\nSlab: Urinal that consists of a slab or sheet fixed to a wall and down which urinal flows into a floor channel.\nStall: Floor mounted urinal that consists of an elliptically shaped sanitary stall fixed to a wall and down which urine flows into a floor channel.\nTrough: Wall mounted urinal of elongated rectangular shape on plan, that can be used by more than one person at a time."@en , "下記のリストより小便器タイプを選択\n\n便器：壁に設置された独立した小便器\n床：壁や床の溝へ流れるように固定されている\n個室：衛生個室の床や壁に楕円形に設置されたフロア\n溝：一人以上の人数が同時に使用できるよう、壁に直角に長く引き伸ばした形"@ja-JP ;
        rdfs:label             "urinalType"@en , "小便器タイプ"@ja-JP ;
        schema:domainIncludes  <https://w3id.org/product/SanitaryTerminal%2FURINAL> .

props:edgeFixingPlateFlangeWidthInPlaneZ
        a                      owl:DatatypeProperty ;
        rdfs:comment           "The flange width of the L-shaped edge plate in plane Z."@en , "L型端部プレートのZ面フランジ幅。"@ja-JP , "L 형 단부 플레이트 Z면 플랜지 폭"@ko-KR ;
        rdfs:label             "edgeFixingPlateFlangeWidthInPlaneZ"@en , "フランジ幅Z"@ja-JP , "플랜지 폭 Z"@ko-KR ;
        rdfs:range             <https://w3id.org/product/PositiveLengthMeasure> ;
        schema:domainIncludes  <https://w3id.org/product/DiscreteAccessory%2FEdge%20fixing%20plate> .

props:flangeTable  a           owl:DatatypeProperty ;
        rdfs:comment           "Designation of the standard table to which the flange conforms."@en , "フランジ形状の名称基準"@ja-JP ;
        rdfs:label             "flangeTable"@en , "フランジ基準"@ja-JP ;
        rdfs:range             xsd:string ;
        schema:domainIncludes  <https://w3id.org/product/PipeSegment> .

props:acquisitionMethod
        a                      owl:DatatypeProperty ;
        rdfs:comment           "The means by which survey data was acquired."@en , "La méthode utilisée pour effectuer le relevé."@fr-FR ;
        rdfs:label             "acquisitionMethod"@en , "MethodeAcquisition"@fr-FR ;
        schema:domainIncludes  <https://w3id.org/product/Annotation%2FSurveyArea> .

props:flammabilityRating
        a                      owl:DatatypeProperty ;
        rdfs:comment           "Classement de l'inflammabilité de l'élément selon la classification nationale de sécurité incendie."@fr-FR , "Angabe zur Entflammbarkeit des Materials gemäß der nationalen oder regionalen Normen."@de-DE , "Flammability Rating for this object.\nIt is given according to the national building code that governs the rating of flammability for materials."@en , "可燃性等級。当該国の建築法規による。"@ja-JP ;
        rdfs:label             "Inflammabilité"@fr-FR , "Entflammbarkeitsklasse"@de-DE , "flammabilityRating"@en , "可燃性等級"@ja-JP ;
        rdfs:range             xsd:string ;
        schema:domainIncludes  <https://w3id.org/product/Covering> .

props:supplyAirTemperatureCooling
        a                      owl:DatatypeProperty ;
        rdfs:comment           "Supply air temperature in cooling mode."@en , "冷房時の給気温度"@ja-JP , "Température de l'air soufflé en mode refroidissement"@fr-FR ;
        rdfs:label             "supplyAirTemperatureCooling"@en , "冷房給気温度"@ja-JP , "Température de l'air soufflé en refroidissement"@fr-FR ;
        schema:domainIncludes  <https://w3id.org/product/AirTerminal> .

props:iCS60898  a              owl:DatatypeProperty ;
        rdfs:comment           "The service breaking capacity in [A] for an MCB tested in accordance with the IEC 60898 series."@en , "IECの60898シリーズに基づいてテストされたMCBの遮断使用容量を[A]で設定。"@ja-JP , "IEC의 60898 시리즈를 기반으로 시험한 MCB 차단 사용 용량 [A]로 설정."@ko-KR ;
        rdfs:label             "iCS60898"@en , "ICS60898"@ja-JP , "ICS60898"@ko-KR ;
        rdfs:range             <https://w3id.org/product/ElectricCurrentMeasure> ;
        schema:domainIncludes  <https://w3id.org/product/ProtectiveDevice%2FCIRCUITBREAKER> .

props:numberOfGangs  a         owl:DatatypeProperty ;
        rdfs:comment           "스위치 버튼 수"@ko-KR , "Number of gangs/buttons on this switch."@en , "슬롯 스위치 / 콘센트 (가장 일반적으로 1,2,3 또는 4)에서 사용할 수있는 수."@ko-KR , "スロットスイッチ/コンセント（最も一般的に1、2、3、または4）で使用可能な数。"@ja-JP , "スイッチのボタン数"@ja-JP , "Number of slots available for switches/outlets (most commonly 1, 2, 3, or 4)."@en ;
        rdfs:label             "버튼 수"@ko-KR , "numberOfGangs"@en , "분기의 수"@ko-KR , "ボタン数"@ja-JP , "分岐の数"@ja-JP ;
        rdfs:range             xsd:int ;
        schema:domainIncludes  <https://w3id.org/product/JunctionBox> , <https://w3id.org/product/SwitchingDevice> .

props:longOutsideLowerBarPitch
        a                      owl:DatatypeProperty ;
        rdfs:comment           "The pitch length of the long outside lower bar."@en , "長辺方向・柱列帯・下端の鉄筋間隔。"@ja-JP ;
        rdfs:label             "longOutsideLowerBarPitch"@en , "長辺・柱列帯・下端ピッチ"@ja-JP ;
        rdfs:range             <https://w3id.org/product/PositiveLengthMeasure> ;
        schema:domainIncludes  <https://w3id.org/product/Slab> .

props:reinforcement  a         owl:DatatypeProperty ;
        rdfs:comment           "The type of reinforcement, if any, used for the duct segment."@en , "ダクト直管に何か使用されている場合の補強種類"@ja-JP ;
        rdfs:label             "reinforcement"@en , "補強"@ja-JP ;
        rdfs:range             xsd:string ;
        schema:domainIncludes  <https://w3id.org/product/DuctSegment> .

props:processName  a           owl:DatatypeProperty ;
        rdfs:comment           "Name of the welding process.  Alternative to the numeric Process property."@en ;
        rdfs:label             "processName"@en ;
        rdfs:range             xsd:string ;
        schema:domainIncludes  <https://w3id.org/product/Fastener%2FWELD> .

props:layup  a                 owl:DatatypeProperty ;
        rdfs:comment           "Configuration of the lamination."@en ;
        rdfs:label             "layup"@en ;
        rdfs:range             xsd:string ;
        schema:domainIncludes  <https://w3id.org/product/Material%2FWood> .

props:dischargeVelocity
        a                      owl:DatatypeProperty ;
        rdfs:comment           "The speed at which air discharges from the fan through the fan housing discharge opening."@en , "ファン吐出口からの吐出風速"@ja-JP ;
        rdfs:label             "dischargeVelocity"@en , "吐出速度"@ja-JP ;
        schema:domainIncludes  <https://w3id.org/product/Fan> .

props:n20Content  a            owl:DatatypeProperty ;
        rdfs:comment           "Nitrous oxide (N2O) content of the products of combustion. This is measured in weight of N2O per unit weight and is therefore unitless."@en ;
        rdfs:label             "n20Content"@en ;
        rdfs:range             <https://w3id.org/product/PositiveRatioMeasure> ;
        schema:domainIncludes  <https://w3id.org/product/Material> .

props:draftSideOffset
        a                      owl:DatatypeProperty ;
        rdfs:comment           "Draft side offset of the profile."@en ;
        rdfs:label             "draftSideOffset"@en ;
        rdfs:range             <https://w3id.org/product/NonNegativeLengthMeasure> ;
        schema:domainIncludes  <https://w3id.org/product/ArbitraryProfileDefWithVoids> .

props:outputCapacityCurve
        a                      owl:DatatypeProperty ;
        rdfs:comment           "Partial output capacity curve (as a function of water temperature); Q = f (Twater)."@en , "部分的アウトプット能力曲線（水温の関数として）"@ja-JP ;
        rdfs:label             "outputCapacityCurve"@en , "部分的アウトプット能力曲線"@ja-JP ;
        schema:domainIncludes  <https://w3id.org/product/SpaceHeater> .

props:substanceDetected
        a                      owl:DatatypeProperty ;
        rdfs:comment           "Identification of the substance that is being detected according to chemical formula.  For example, calcium carbonate is 'CaCO3'"@en , "検出されている物質の識別。"@ja-JP , "검출되는 물질의 식별."@ko-KR ;
        rdfs:label             "substanceDetected"@en , "対象物質"@ja-JP , "대상 물질"@ko-KR ;
        rdfs:range             xsd:string ;
        schema:domainIncludes  <https://w3id.org/product/Sensor%2FIONCONCENTRATIONSENSOR> .

props:displayHeight  a         owl:DatatypeProperty ;
        rdfs:comment           "Indicates the physical height of the screen (only the display surface)."@en , "画面の高さを示す。"@ja-JP , "화면의 높이를 나타낸다"@ko-KR ;
        rdfs:label             "displayHeight"@en , "画面高さ"@ja-JP , "화면 높이"@ko-KR ;
        rdfs:range             <https://w3id.org/product/PositiveLengthMeasure> ;
        schema:domainIncludes  <https://w3id.org/product/AudioVisualAppliance%2FDISPLAY> .

props:warrantyPeriod  a        owl:DatatypeProperty ;
        rdfs:comment           "The time duration during which a manufacturer or supplier guarantees or warrants the performance of an artefact."@en ;
        rdfs:label             "warrantyPeriod"@en ;
        rdfs:range             <https://w3id.org/product/TimeMeasure> ;
        schema:domainIncludes  <https://w3id.org/product/Element> .

props:xDirectionTieHoopBarPitch
        a                      owl:DatatypeProperty ;
        rdfs:comment           "The X direction pitch length of the tie hoop."@en , "Ｘ方向巾止筋の間隔。"@ja-JP ;
        rdfs:label             "xDirectionTieHoopBarPitch"@en , "Ｘ方向巾止め筋間隔"@ja-JP ;
        rdfs:range             <https://w3id.org/product/PositiveLengthMeasure> ;
        schema:domainIncludes  <https://w3id.org/product/Column> .

props:naturalVentilation
        a                      owl:DatatypeProperty ;
        rdfs:comment           "Anforderung, ob der Raum eine natürliche Lüftung haben soll (WAHR), oder eine künstliche Lüftung (Falsch)."@de-DE , "공간이 자연 환기가 있는지 환기있는 여부를 나타내는 값"@ko-KR , "Indique si la ventilation de l'espace doit être naturelle (VRAI) ou mécanique (FAUX)."@fr-FR , "Indication whether the space is required to have natural ventilation (TRUE) or mechanical ventilation (FALSE)."@en , "空間が自然換気を持つか機械換気を持つかを示すブーリアン値。(TRUE)有、(FALSE)なし。"@ja-JP ;
        rdfs:label             "Ventilation naturelle"@fr-FR , "自然換気"@ja-JP , "Natürliche Lüftung"@de-DE , "자연환기"@ko-KR , "naturalVentilation"@en ;
        rdfs:range             xsd:boolean ;
        schema:domainIncludes  <https://w3id.org/product/Space> , <https://w3id.org/product/cZone> , <https://w3id.org/product/cSpatialZone> .

props:mountingOffset  a        owl:DatatypeProperty ;
        rdfs:comment           "カウンター用途として、カウンターとシンクの間に垂直洗浄に据付される廃水機器。"@ja-JP , "調理台に設置されたシンクに、上端と調理台間で垂直に補正されること。"@ja-JP , "For cunter top maounted sinks, the vertical offset between the top of the sink and the counter top."@en , "For cunter top maounted basins the vertical offset between the top of the sink and the counter top."@en ;
        rdfs:label             "mountingOffset"@en , "据付補正"@ja-JP ;
        rdfs:range             <https://w3id.org/product/LengthMeasure> ;
        schema:domainIncludes  <https://w3id.org/product/SanitaryTerminal%2FWASHHANDBASIN> , <https://w3id.org/product/SanitaryTerminal%2FSINK> .

props:momentOfInertiaY
        a                      owl:DatatypeProperty ;
        rdfs:comment           "Moment of inertia about ys (second moment of area, about ys). For example measured in mm4."@en ;
        rdfs:label             "momentOfInertiaY"@en ;
        rdfs:range             <https://w3id.org/product/MomentOfInertiaMeasure> ;
        schema:domainIncludes  <https://w3id.org/product/ProfileDef> .

props:weatherDataDate
        a                      owl:DatatypeProperty ;
        rdfs:comment           "The date for which the weather data was gathered."@en , "気象台所在地の気象データ。"@ja-JP , "기상대 지역의 기상 데이터입니다."@ko-KR ;
        rdfs:label             "weatherDataDate"@en , "気象データ"@ja-JP , "기상데이터"@ko-KR ;
        rdfs:range             xsd:dateTime ;
        schema:domainIncludes  <https://w3id.org/product/Building> .

props:selfClosing  a           owl:DatatypeProperty ;
        rdfs:comment           "Indique si cet objet est conçu pour une fermeture automatique après usage (VRAI) ou non (FAUX)"@fr-FR , "このドアが自動的に閉まる機能を有するかどうかのブーリアン値。"@ja-JP , "表示该构件是否设计为自动关闭。"@zh-CN , "Indication whether this object is designed to close automatically after use (TRUE) or not (FALSE)."@en , "Angabe, ob die Tür sicher und selbständig nach der Benutzung durch einen Türschließer schließt (Ja) oder nicht (NEIN)."@de-DE ;
        rdfs:label             "selfClosing"@en , "是否自动关闭"@zh-CN , "Selbstschliessend"@de-DE , "自動ドア閉機能区分"@ja-JP , "FermetureAutomatique"@fr-FR ;
        rdfs:range             xsd:boolean ;
        schema:domainIncludes  <https://w3id.org/product/Door> .

props:combustible  a           owl:DatatypeProperty ;
        rdfs:comment           "German-description-4"@de-DE , "Indique si l'objet est réalisé à partir de matériau combustible (VRAI) ou non (FAUX)."@fr-FR , "Angabe ob das Bauteil brennbares Material enthält (WAHR) oder nicht (FALSCH)."@de-DE , "この部材が可燃性物質で作られているかどうかを示すブーリアン値。"@ja-JP , "Indication whether the object is made from combustible material (TRUE) or not (FALSE)."@en , "表示该构件是否由可燃材料制成。"@zh-CN , "Indique si l'objet est fait de matière combustible (VRAI) ou non (FAUX)."@fr-FR ;
        rdfs:label             "combustible"@en , "可燃性区分"@ja-JP , "是否可燃"@zh-CN , "Combustible"@fr-FR , "Brennbares Material"@de-DE ;
        rdfs:range             xsd:boolean ;
        schema:domainIncludes  <https://w3id.org/product/Slab> , <https://w3id.org/product/CurtainWall> , <https://w3id.org/product/Covering> , <https://w3id.org/product/Wall> .

props:bladeAction  a           owl:DatatypeProperty ;
        rdfs:comment           "Blade action."@en ;
        rdfs:label             "bladeAction"@en ;
        schema:domainIncludes  <https://w3id.org/product/Damper> .

props:nominalDepth  a          owl:DatatypeProperty ;
        rdfs:comment           "要素の深さ。"@ja-JP , "タンクの公称深さ　　注：水平円筒形タンクに対しては必須ではない"@ja-JP , "装置の基礎に配管吸入口から測定した深さ。"@ja-JP , "The nominal depth of the tank.\n\nNote: Not required for a horizontal cylindrical tank."@en , "Nominal or quoted depth of the object measured from the inlet drain connection to the base of the unit."@en , "公称または引用深さ。"@ja-JP , "The nominal depth of the furniture of this type. The size information is provided in addition to the shape representation and the geometric parameters used within. In cases of inconsistency between the geometric parameters and the size properties, provided in the attached property set, the geometric parameters take precedence."@en , "Nominal or quoted depth of the object."@en ;
        rdfs:label             "公称深さ"@ja-JP , "深さ"@ja-JP , "nominalDepth"@en ;
        rdfs:range             <https://w3id.org/product/PositiveLengthMeasure> ;
        schema:domainIncludes  <https://w3id.org/product/WasteTerminal%2FWASTEDISPOSALUNIT> , <https://w3id.org/product/SanitaryTerminal%2FWASHHANDBASIN> , <https://w3id.org/product/SanitaryTerminal%2FBATH> , <https://w3id.org/product/SanitaryTerminal%2FSINK> , <https://w3id.org/product/SanitaryTerminal%2FSHOWER> , <https://w3id.org/product/Tank> , <https://w3id.org/product/Furniture> , <https://w3id.org/product/SanitaryTerminal%2FURINAL> , <https://w3id.org/product/SanitaryTerminal%2FSANITARYFOUNTAIN> , <https://w3id.org/product/SanitaryTerminal%2FBIDET> , <https://w3id.org/product/SanitaryTerminal%2FTOILETPAN> .

props:scheduledFrequency
        a                      owl:DatatypeProperty ;
        rdfs:comment           "The period of time between expected instantiations of a work order that may have been predefined."@en ;
        rdfs:label             "scheduledFrequency"@en ;
        rdfs:range             <https://w3id.org/product/TimeMeasure> ;
        schema:domainIncludes  <https://w3id.org/product/ProjectOrder%2FMAINTENANCEWORKORDER> .

props:requiredSlope  a         owl:DatatypeProperty ;
        rdfs:comment           "Inclinaison de la rampe par rapport à l'horizontal (0 degrés). Valeur maximale de l'inclinaison du passage selon le code applicable ou pour respecter des contraintes additionnelles."@fr-FR , "German-description-3"@de-DE , "要求される傾斜角度。水平を０度とする。"@ja-JP , "构件所需的相对于水平（0.0度）方向的坡度角。\n建筑规范或其他规定要求的通道的最大坡度。"@zh-CN , "Required sloping angle of the object  - relative to horizontal (0.0 degrees).\nRequired maximum slope for the passageway according to the applicable building code or additional requirements."@en ;
        rdfs:label             "InclinaisonRequise"@fr-FR , "要求傾斜"@ja-JP , "erforderliche Neigung"@de-DE , "requiredSlope"@en , "所需坡度"@zh-CN ;
        rdfs:range             <https://w3id.org/product/PlaneAngleMeasure> ;
        schema:domainIncludes  <https://w3id.org/product/Ramp> .

props:eutrophication  a        owl:DatatypeProperty ;
        rdfs:comment           "Quantity of eutrophicating compounds calculated in equivalent PO4."@en , "算出されたPO4と等しい富栄養化を混合する量。"@ja-JP , "PO4 (인산)에 상응하는 환산되는 부영 양화 성분 물량"@ko-KR , "Quantité de composés responsables de l'eutrophisation exprimée en équivalent P04 [NDT : selon la norme PrEN15804:2008]"@fr-FR ;
        rdfs:label             "부영 양화"@ko-KR , "Eutrophisation"@fr-FR , "富栄養化"@ja-JP , "eutrophication"@en ;
        rdfs:range             <https://w3id.org/product/MassMeasure> ;
        schema:domainIncludes  <https://w3id.org/product/Element> .

props:junctionLeftAngle
        a                      owl:DatatypeProperty ;
        rdfs:comment           "The change of direction of flow for the left junction."@en , "左継ぎ手の流れの方向の変化"@ja-JP ;
        rdfs:label             "junctionLeftAngle"@en , "左継ぎ手角度"@ja-JP ;
        rdfs:range             <https://w3id.org/product/PositivePlaneAngleMeasure> ;
        schema:domainIncludes  <https://w3id.org/product/PipeFitting%2FJUNCTION> .

props:audioMode  a             owl:DatatypeProperty ;
        rdfs:comment           "오디오 사운드 모드 설정."@ko-KR , "Indicates audio sound modes and corresponding labels, if applicable."@en , "オーディオサウンドモードの設定。"@ja-JP ;
        rdfs:label             "오디오 모드"@ko-KR , "オーディオモード"@ja-JP , "audioMode"@en ;
        schema:domainIncludes  <https://w3id.org/product/AudioVisualAppliance%2FAMPLIFIER> , <https://w3id.org/product/AudioVisualAppliance%2FDISPLAY> , <https://w3id.org/product/AudioVisualAppliance%2FRECEIVER> .

props:diagonalTrussBaseBarDiameter
        a                      owl:DatatypeProperty ;
        rdfs:comment           "The nominal diameter of the base bar."@en , "ベースバーの公称直径。"@ja-JP , "기반 막대의 공칭 지름"@ko-KR ;
        rdfs:label             "diagonalTrussBaseBarDiameter"@en , "ベースバー径"@ja-JP , "기반 막대 지름"@ko-KR ;
        rdfs:range             <https://w3id.org/product/PositiveLengthMeasure> ;
        schema:domainIncludes  <https://w3id.org/product/DiscreteAccessory%2FDiagonal%20truss%20connector> .

props:thermalTransmittanceSummer
        a                      owl:DatatypeProperty ;
        rdfs:comment           "素材の熱透過係数（U値）。夏期のガラスの熱透過係数だけ、U値として参照される"@ja-JP , "Thermal transmittance coefficient (U-Value) of a material.\nSummer thermal transmittance coefficient of the glazing only, often referred to as (U-value)."@en , "材料的导热系数（U值）。\n仅玻璃的夏季导热系数，常以U值表示。"@zh-CN , "German-description-17"@de-DE , "Coefficient de transmission thermique (U) d'un matériau. Coefficient de transmission thermique en été du vitrage seul, souvent désigné comme étant Uw."@fr-FR ;
        rdfs:label             "German-name-15"@de-DE , "TransmittanceThermiqueEte"@fr-FR , "thermalTransmittanceSummer"@en , "夏季导热系数"@zh-CN , "夏期の熱透過係数"@ja-JP ;
        rdfs:range             <https://w3id.org/product/ThermalTransmittanceMeasure> ;
        schema:domainIncludes  <https://w3id.org/product/cWindow> , <https://w3id.org/product/Door> .

props:tubingLength  a          owl:DatatypeProperty ;
        rdfs:comment           "Water tube length inside the component."@en , "構成要素における水管の長さ"@ja-JP ;
        rdfs:label             "tubingLength"@en , "チューブの長さ"@ja-JP ;
        rdfs:range             <https://w3id.org/product/PositiveLengthMeasure> ;
        schema:domainIncludes  <https://w3id.org/product/SpaceHeater%2FRADIATOR> .

props:spaceTemperatureSummerMin
        a                      owl:DatatypeProperty ;
        rdfs:comment           "Minimal geforderte Raumtemperatur aus dem Raumprogramm für die Auslegung der Raumkühlung."@de-DE , "空間またはゾーンの暑熱季(夏季)の最低温度。利用者/設計者の視点から要求される。"@ja-JP , "Température minimale de l'espace ou de la zone  en été. Spécifiée par l'usager ou le concepteur et utilisée comme consigne pour le refroidissement."@fr-FR , "Minimal temperature of the space or zone for the hot (summer) period, that is required from user/designer view point and provided as requirement for cooling."@en , "공간이나 영역 혹서 계절 (여름)의 최저 온도. 이용자 / 설계자의 관점에서 요구된다."@ko-KR ;
        rdfs:label             "Température minimale en été"@fr-FR , "Raumtemperatur Kühlung Minimal"@de-DE , "여름최저온도"@ko-KR , "夏季最低室内温度"@ja-JP , "spaceTemperatureSummerMin"@en ;
        rdfs:range             <https://w3id.org/product/ThermodynamicTemperatureMeasure> ;
        schema:domainIncludes  <https://w3id.org/product/cSpatialZone> , <https://w3id.org/product/Space> , <https://w3id.org/product/cZone> .

props:returnWaterTemperatureHeating
        a                      owl:DatatypeProperty ;
        rdfs:comment           "Return water temperature in heating mode."@en ;
        rdfs:label             "returnWaterTemperatureHeating"@en ;
        schema:domainIncludes  <https://w3id.org/product/CooledBeam> .

props:washerShape  a           owl:DatatypeProperty ;
        rdfs:comment           "Shape of the washers, e.g. 'Standard', 'Square'"@en ;
        rdfs:label             "washerShape"@en ;
        rdfs:range             xsd:string ;
        schema:domainIncludes  <https://w3id.org/product/MechanicalFastener%2FBOLT> .

props:initialTension  a        owl:DatatypeProperty ;
        rdfs:comment           "The initial stress of the tendon. This property applies to prestressed concrete elements only."@en , "緊張材の初期応力。この属性はプレストレストコンクリート要素のみに適用される。"@ja-JP ;
        rdfs:label             "initialTension"@en , "初引張力"@ja-JP ;
        rdfs:range             <https://w3id.org/product/PressureMeasure> ;
        schema:domainIncludes  <https://w3id.org/product/BuildingElement> .

props:functionReliable
        a                      owl:DatatypeProperty ;
        rdfs:comment           "コアの維持は特定（テスト）の時間と条件でプロパティ/関数を指定する。標準会議（IEC）規格に準拠。"@ja-JP , "핵심 정비는 특정 (테스트) 시간과 조건의 속성 / 함수를 지정한다. 표준 회의 (IEC) 규격을 준수합니다."@ko-KR , "ケーブルや母線が与えられた時間と条件の中で規定される機能、性質を維持すること。これはIEC基準による。"@ja-JP , "케이블 및 모선 주어진 시간과 조건에서 규정하는 기능, 성질을 유지한다. 이것은 IEC 기준에 의한다."@ko-KR , "Cable/bus maintain given properties/functions over a given (tested) time and conditions. According to IEC standard."@en , "Core maintain given properties/functions over a given (tested) time and conditions. According to (IEC) standard."@en ;
        rdfs:label             "機能信頼性"@ja-JP , "functionReliable"@en , "기능 신뢰성"@ko-KR , "신뢰할 수있는 기능"@ko-KR , "信頼性のある機能"@ja-JP ;
        rdfs:range             xsd:boolean ;
        schema:domainIncludes  <https://w3id.org/product/CableSegment%2FCABLESEGMENT> , <https://w3id.org/product/CableSegment%2FCORESEGMENT> .

props:nominalCurrent  a        owl:DatatypeProperty ;
        rdfs:comment           "定格電流[A]を少なくても1つ値をセットしなければならない。\n セット内の任意の値の値を超えてはならない。\n 定格電流は、同じブレーカ部に関連付けられている。"@ja-JP , "The nominal current that is designed to be measured."@en , "A set of nominal currents in [A] for which the data of this instance is valid. At least one value shall be provided. Any value in the set shall not exceed the value of the \nUltimateRatedCurrent associated with the same breaker unit."@en , "정격 전류 [A]를 적어도 1 개의 값을 설정해야한다.   동일한 차단기부와 연결된 정격전류는세트 내의 임의의 값은 초과할 수 없다."@ko-KR ;
        rdfs:label             "定格電流"@ja-JP , "정격전류"@ko-KR , "nominalCurrent"@en ;
        rdfs:range             <https://w3id.org/product/ElectricCurrentMeasure> ;
        schema:domainIncludes  <https://w3id.org/product/FlowMeter%2FENERGYMETER> , <https://w3id.org/product/ProtectiveDevice> .

props:spilloverLevel  a        owl:DatatypeProperty ;
        rdfs:comment           "The level at which water spills out of the object."@en , "The level at which water spills out of the terminal."@en , "水がこぼれるレベル。"@ja-JP , "継手からの水位。"@ja-JP ;
        rdfs:label             "spilloverLevel"@en , "流出レベル"@ja-JP , "水位"@ja-JP ;
        rdfs:range             <https://w3id.org/product/PositiveLengthMeasure> ;
        schema:domainIncludes  <https://w3id.org/product/SanitaryTerminal%2FTOILETPAN> , <https://w3id.org/product/SanitaryTerminal%2FURINAL> , <https://w3id.org/product/WasteTerminal%2FFLOORTRAP> , <https://w3id.org/product/SanitaryTerminal%2FBIDET> .

props:displaySize  a           owl:DatatypeProperty ;
        rdfs:comment           "表示のサイズ。 棒温度計の場合では、軸の長さになる。 ダイヤル温度計に関しては、ダイヤルの直径になる。"@ja-JP , "The physical size of the display. In the case of a stem thermometer, this will be the length of the stem. For a dial thermometer, it will be the diameter of the dial."@en , "表示のサイズ。 ダイヤル圧力計に関しては、ダイヤルの直径になる。"@ja-JP , "The physical size of the display. For a dial pressure gauge it will be the diameter of the dial."@en , "표시의 크기입니다. 막대 온도계의 경우, 축의 길이가된다. 다이얼 온도계에 대해서는 다이얼 직경된다."@ko-KR , "표시의 크기입니다. 다이얼 게이지에 관해서는 전화 직경된다."@ko-KR ;
        rdfs:label             "表示サイズ"@ja-JP , "디스플레이 크기"@ko-KR , "displaySize"@en ;
        rdfs:range             <https://w3id.org/product/PositiveLengthMeasure> ;
        schema:domainIncludes  <https://w3id.org/product/FlowInstrument%2FTHERMOMETER> , <https://w3id.org/product/FlowInstrument%2FPRESSUREGAUGE> .

props:evaporatingTemperature
        a                      owl:DatatypeProperty ;
        rdfs:comment           "Refrigerant evaporating temperature."@en , "蒸発温度"@ja-JP ;
        rdfs:label             "evaporatingTemperature"@en , "蒸発温度"@ja-JP ;
        schema:domainIncludes  <https://w3id.org/product/Evaporator> .

props:mainColor  a             owl:DatatypeProperty ;
        rdfs:comment           "The main color of the furniture of this type."@en ;
        rdfs:label             "mainColor"@en ;
        rdfs:range             xsd:string ;
        schema:domainIncludes  <https://w3id.org/product/Furniture> .

props:versionDate  a           owl:DatatypeProperty ;
        rdfs:comment           "The date on which the version of the agreement became applicable."@en ;
        rdfs:label             "versionDate"@en ;
        rdfs:range             xsd:date ;
        schema:domainIncludes  <https://w3id.org/product/SpatialStructureElement> .

props:thickness  a             owl:DatatypeProperty ;
        rdfs:comment           "Thickness of the fin."@en , "フィンの厚さ"@ja-JP ;
        rdfs:label             "thickness"@en , "厚さ"@ja-JP ;
        rdfs:range             <https://w3id.org/product/PositiveLengthMeasure> ;
        schema:domainIncludes  <https://w3id.org/product/TubeBundle%2FFINNED> .

props:isPotable  a             owl:DatatypeProperty ;
        rdfs:comment           "If TRUE, then the water is considered potable."@en ;
        rdfs:label             "isPotable"@en ;
        rdfs:range             xsd:boolean ;
        schema:domainIncludes  <https://w3id.org/product/Material> .

props:scheduleWork  a          owl:DatatypeProperty ;
        rdfs:comment           "The scheduled work on behalf of the resource allocation."@en , "資源配分のための予定された作業。"@ja-JP ;
        rdfs:label             "scheduleWork"@en , "予定作業時間"@ja-JP ;
        schema:domainIncludes  <https://w3id.org/product/ConstructionResource> .

props:saturationEfficiency
        a                      owl:DatatypeProperty ;
        rdfs:comment           "Saturation efficiency: Ratio of leaving air absolute humidity to the maximum absolute humidity."@en , "飽和比率：最大絶対湿度に対する現在の絶対湿度の割合"@ja-JP ;
        rdfs:label             "saturationEfficiency"@en , "飽和比率"@ja-JP ;
        schema:domainIncludes  <https://w3id.org/product/Humidifier> .

props:massFlowRate  a          owl:DatatypeProperty ;
        rdfs:comment           "流体の質量流量。"@ja-JP , "The mass flow rate of the fluid."@en ;
        rdfs:label             "質量流量"@ja-JP , "massFlowRate"@en ;
        schema:domainIncludes  <https://w3id.org/product/DistributionPort%2FCHEMICAL> , <https://w3id.org/product/DistributionPort%2FAIRCONDITIONING> .

props:invertElevation
        a                      owl:DatatypeProperty ;
        rdfs:comment           "The invert elevation relative to the datum established for the project."@en ;
        rdfs:label             "invertElevation"@en ;
        rdfs:range             <https://w3id.org/product/LengthMeasure> ;
        schema:domainIncludes  <https://w3id.org/product/PipeSegment> .

props:maximumPartLoadRatio
        a                      owl:DatatypeProperty ;
        rdfs:comment           "Maximum part load ratio as a fraction of nominal capacity."@en , "Coefficient maximal de charge partielle en tant que fraction de la puissance nominale."@fr-FR ;
        rdfs:label             "maximumPartLoadRatio"@en , "CoefficientMaximalChargePartielle"@fr-FR ;
        rdfs:range             <https://w3id.org/product/PositiveRatioMeasure> ;
        schema:domainIncludes  <https://w3id.org/product/Compressor> .

props:concreteCover  a         owl:DatatypeProperty ;
        rdfs:comment           "The protective concrete cover at the reinforcing bars according to local building regulations."@en , "Abstand zwischen der Betonoberfläche und der Außenkante einer vom Beton umhüllten Bewehrung."@de-DE ;
        rdfs:label             "concreteCover"@en , "Betonüberdeckung"@de-DE ;
        rdfs:range             <https://w3id.org/product/PositiveLengthMeasure> ;
        schema:domainIncludes  <https://w3id.org/product/BuildingElement> .

props:coreSpacing  a           owl:DatatypeProperty ;
        rdfs:comment           "Core spacing of the profile."@en ;
        rdfs:label             "coreSpacing"@en ;
        rdfs:range             <https://w3id.org/product/PositiveLengthMeasure> ;
        schema:domainIncludes  <https://w3id.org/product/ArbitraryProfileDefWithVoids> .

props:diagonalTrussHeight
        a                      owl:DatatypeProperty ;
        rdfs:comment           "The overall height of the truss connector."@en , "トラス接続部材の全体の高さ。"@ja-JP , "트러스 연결 부재의 전체 높이"@ko-KR ;
        rdfs:label             "diagonalTrussHeight"@en , "全体高さ"@ja-JP , "전체 높이"@ko-KR ;
        rdfs:range             <https://w3id.org/product/PositiveLengthMeasure> ;
        schema:domainIncludes  <https://w3id.org/product/DiscreteAccessory%2FDiagonal%20truss%20connector> .

props:areaPerOccupant
        a                      owl:DatatypeProperty ;
        rdfs:comment           "Taux de remplissage de l'espace pour l'usage type"@fr-FR , "Design occupancy loading for this type of usage assigned to this space."@en , "Anteil der Raumfläche pro Benutzer für Nutzung des Raums."@de-DE , "この空間に割り当てられた用途に対する想定利用負荷。"@ja-JP ;
        rdfs:label             "Fläche pro Nutzer"@de-DE , "利用者毎面積"@ja-JP , "areaPerOccupant"@en , "SurfaceParOccupant"@fr-FR ;
        rdfs:range             <https://w3id.org/product/AreaMeasure> ;
        schema:domainIncludes  <https://w3id.org/product/Space> , <https://w3id.org/product/cZone> , <https://w3id.org/product/cSpatialZone> .

props:fireResistanceRating
        a                      owl:DatatypeProperty ;
        rdfs:comment           "Measure of the fire resistance rating in hours (e.g., 1.5 hours, 2 hours, etc.)."@en ;
        rdfs:label             "fireResistanceRating"@en ;
        rdfs:range             xsd:string ;
        schema:domainIncludes  <https://w3id.org/product/Damper%2FFIRESMOKEDAMPER> , <https://w3id.org/product/Damper%2FFIREDAMPER> .

props:nominalSize  a           owl:DatatypeProperty ;
        rdfs:comment           "Indicates the diagonal screen size."@en , "画面の対角線サイズを示す。"@ja-JP , "화면의 대각선 크기를 나타낸다."@ko-KR ;
        rdfs:label             "nominalSize"@en , "画面公称サイズ"@ja-JP , "화면 공칭 크기"@ko-KR ;
        rdfs:range             <https://w3id.org/product/PositiveLengthMeasure> ;
        schema:domainIncludes  <https://w3id.org/product/AudioVisualAppliance%2FDISPLAY> .

props:classificationAuthority
        a                      owl:DatatypeProperty ;
        rdfs:comment           "The name of the authority that applies the classification of service to the hose reel (e.g. NFPA/FEMA)."@en , "ホースリールの分類認証機関の名称。（例　NFPA/ FEMA）"@ja-JP ;
        rdfs:label             "classificationAuthority"@en , "分類認証機関"@ja-JP ;
        rdfs:range             xsd:string ;
        schema:domainIncludes  <https://w3id.org/product/FireSuppressionTerminal%2FHOSEREEL> .

props:function  a              owl:DatatypeProperty ;
        rdfs:comment           "Type of function for which the conductor is intended."@en , "導体の機能のタイプ。"@ja-JP , "도체의 기능 유형."@ko-KR ;
        rdfs:label             "function"@en , "機能"@ja-JP , "기능"@ko-KR ;
        schema:domainIncludes  <https://w3id.org/product/CableSegment%2FCONDUCTORSEGMENT> .

props:hasHotGasBypass
        a                      owl:DatatypeProperty ;
        rdfs:comment           "Whether or not hot gas bypass is provided for the compressor. TRUE = Yes, FALSE = No."@en , "Qu'il y ait ou non un bypass du gaz chaud fourni au niveau du compresseur, VRAI= oui, FAUX= Non."@fr-FR ;
        rdfs:label             "hasHotGasBypass"@en , "PossedeBypassGazChaud"@fr-FR ;
        rdfs:range             xsd:boolean ;
        schema:domainIncludes  <https://w3id.org/product/Compressor> .

props:headShape  a             owl:DatatypeProperty ;
        rdfs:comment           "Shape of the bolt's head, e.g. 'Hexagon', 'Countersunk', 'Cheese'"@en ;
        rdfs:label             "headShape"@en ;
        rdfs:range             xsd:string ;
        schema:domainIncludes  <https://w3id.org/product/MechanicalFastener%2FBOLT> .

props:nominalCapacity
        a                      owl:DatatypeProperty ;
        rdfs:comment           "The total nominal or design volumetric capacity of the tank."@en , "Compressor nameplate capacity."@en , "タンクの総公称又は設計容量"@ja-JP , "Nominal cooling tower capacity in terms of heat transfer rate of the cooling tower between air stream and water stream at nominal conditions."@en , "Puissance froid nominale du groupe froid aux conditions standardisées telles que définies par l'organisation faisant autorité."@fr-FR , "Nominal cooling capacity of chiller at standardized conditions as defined by the agency having jurisdiction."@en , "Puissance du compresseur au niveau de sa plaque."@fr-FR ;
        rdfs:label             "PuissanceCompresseur"@fr-FR , "公称容量"@ja-JP , "nominalCapacity"@en , "PuissanceNominale"@fr-FR ;
        rdfs:range             <https://w3id.org/product/PowerMeasure> , <https://w3id.org/product/VolumeMeasure> ;
        schema:domainIncludes  <https://w3id.org/product/Tank> , <https://w3id.org/product/Chiller> , <https://w3id.org/product/CoolingTower> , <https://w3id.org/product/Compressor> .

props:freezingPoint  a         owl:DatatypeProperty ;
        rdfs:comment           "The freezing point of the material (fluid)."@en ;
        rdfs:label             "freezingPoint"@en ;
        rdfs:range             <https://w3id.org/product/ThermodynamicTemperatureMeasure> ;
        schema:domainIncludes  <https://w3id.org/product/Material> .

props:limitingTerminalSize
        a                      owl:DatatypeProperty ;
        rdfs:comment           "The maximum terminal size capacity of the device."@en , "装置に接続される最大サイズ。"@ja-JP , "장치에 연결되는 최대 크기입니다."@ko-KR ;
        rdfs:label             "limitingTerminalSize"@en , "接続限界値"@ja-JP , "연결 한계"@ko-KR ;
        rdfs:range             <https://w3id.org/product/AreaMeasure> ;
        schema:domainIncludes  <https://w3id.org/product/ProtectiveDeviceTrippingUnit> .

props:nominalSurroundingTemperatureHeating
        a                      owl:DatatypeProperty ;
        rdfs:comment           "Nominal surrounding temperature (refers to nominal heating capacity)."@en ;
        rdfs:label             "nominalSurroundingTemperatureHeating"@en ;
        rdfs:range             <https://w3id.org/product/ThermodynamicTemperatureMeasure> ;
        schema:domainIncludes  <https://w3id.org/product/CooledBeam> .

props:grossPlannedArea
        a                      owl:DatatypeProperty ;
        rdfs:comment           "객실의 총 계획 면적 글로스. 공간 계획시 사용된다."@ko-KR , "계획된 그로스 면적. 건물 계획시 사용됩니다."@ko-KR , "計画された建物階のグロス面積。建物計画に際に使用。"@ja-JP , "Total planned gross area for the zone. Used for programming the zone."@en , "Surface programmée brute totale de la pièce. Telle que définie lors de la programmation."@fr-FR , "Surface programmée brute totale de l'étage. Telle que définie lors de la programmation."@fr-FR , "Surface programmée brute totale du bâtiment. Telle que définie lors de la programmation."@fr-FR , "Geforderte Bruttofläche des Geschosses laut Raumprogramm."@de-DE , "Total planned gross area for the space. Used for programming the space."@en , "計画されたグロス面積。建物計画に際に使用。"@ja-JP , "계획된 건물 층 그로스 면적. 건물 계획시 사용됩니다."@ko-KR , "Total planned area for the building storey. Used for programming the building storey."@en , "Total planned gross area for the building  Used for programming the building."@en , "Geforderte Bruttofläche des Gebäudes laut Raumprogramm."@de-DE ;
        rdfs:label             "계획 그로스 면적"@ko-KR , "計画グロス面積"@ja-JP , "Bruttofläche nach Raumprogramm"@de-DE , "grossPlannedArea"@en , "Surface programmée brute"@fr-FR ;
        rdfs:range             <https://w3id.org/product/AreaMeasure> ;
        schema:domainIncludes  <https://w3id.org/product/Building> , <https://w3id.org/product/Space> , <https://w3id.org/product/Zone> , <https://w3id.org/product/BuildingStorey> .

props:flowPattern  a           owl:DatatypeProperty ;
        rdfs:comment           "Flow pattern."@en , "流れ種類（単一直線、腹式直線、４方向、放射状、SWIRL、DISPLACEMENT、COMPACT他）"@ja-JP , "Forme du flux"@fr-FR ;
        rdfs:label             "flowPattern"@en , "流れ種類"@ja-JP , "FormeFlux"@fr-FR ;
        schema:domainIncludes  <https://w3id.org/product/AirTerminal> .

props:warrantyEndDate
        a                      owl:DatatypeProperty ;
        rdfs:comment           "The date on which the warranty expires."@en ;
        rdfs:label             "warrantyEndDate"@en ;
        rdfs:range             xsd:date ;
        schema:domainIncludes  <https://w3id.org/product/Element> .

props:numberOfRows  a          owl:DatatypeProperty ;
        rdfs:comment           "Number of tube rows in the tube bundle assembly."@en , "チューブの集合の組立におけるチューブ列数"@ja-JP ;
        rdfs:label             "numberOfRows"@en , "列数"@ja-JP ;
        rdfs:range             xsd:int ;
        schema:domainIncludes  <https://w3id.org/product/TubeBundle> .

props:shadingDeviceType
        a                      owl:DatatypeProperty ;
        rdfs:comment           "Specifies the type of shading device."@en , "日除け装置の種別を設定する。"@ja-JP , "Spécifies le type de protection solaire."@fr-FR ;
        rdfs:label             "shadingDeviceType"@en , "Sonnenschutztyp"@de-DE , "日除け装置種別"@ja-JP , "Type de protection solaire"@fr-FR ;
        schema:domainIncludes  <https://w3id.org/product/ShadingDevice> .

props:washHandBasinType
        a                      owl:DatatypeProperty ;
        rdfs:comment           "Defines the types of wash hand basin that may be specified where:\n\n\nDentalCuspidor: Waste water appliance that receives and flushes away mouth washings\n.\nHandRinse: Wall mounted wash hand basin that has an overall width of 500mm or less\n.\nHospital: Wash hand basin that has a smooth easy clean surface without tapholes or overflow slot for use where hygiene is of prime importance. \n\nTipup: Wash hand basin mounted on pivots so that it can be emptied by tilting.\n\nVanity: Wash hand basin for installation into a horizontal surface.\n\nWashfountain: Wash hand basin that is circular, semi-circular or polygonal on plan, at which more than one person can wash at the same time.\nWashingTrough: Wash hand basin of elongated rectangular shape in plan, at which more than one person can wash at the same time."@en , "手洗いの種類は設置される場所で定義されます。\n\n歯科用痰壷：口をゆすぐ際に受けて流す廃水機器\n手洗い：500ｍｍ以下の幅の壁掛け型手洗い\n病院用：サイフォンか氾濫防止弁が付いた衛生が最優先とされる場所で使用される手洗い洗面器\n上げ起こし型：角度調整によって空にできる軸上に設置された手洗い\n化粧台：地平面に設置された手洗い台\n洗浄噴水型：一人以上の人間が同時に使用できる円・半円・多角形の洗面台\n洗浄ボウル：一人以上の人間が同時に使用できる多角形の洗面台"@ja-JP ;
        rdfs:label             "washHandBasinType"@en , "手洗い種類"@ja-JP ;
        schema:domainIncludes  <https://w3id.org/product/SanitaryTerminal%2FWASHHANDBASIN> .

props:isCoated  a              owl:DatatypeProperty ;
        rdfs:comment           "Indique si le verre a subi un traitement de surface (VRAI) ou non (FAUX)."@fr-FR , "Indication whether the glass is coated with a material (TRUE) or not (FALSE)."@en , "表示玻璃是否具有某种材料的镀膜。"@zh-CN , "ガラスがコーティングされいるか（TRUE）否か（FALSE）示す。"@ja-JP , "German-description-9"@de-DE ;
        rdfs:label             "コーティング"@ja-JP , "是否镀膜"@zh-CN , "VitrageTraite"@fr-FR , "isCoated"@en , "German-name-9"@de-DE ;
        rdfs:range             xsd:boolean ;
        schema:domainIncludes  <https://w3id.org/product/cWindow> , <https://w3id.org/product/Door> .

props:span  a                  owl:DatatypeProperty ;
        rdfs:comment           "Portée libre de la poutre. Cette propriété  est donnée en complément de la représentation de la forme et des paramètres géométriques qui la déterminent. En cas d'incohérence entre ces paramètres géométriques et cette propriété, ce sont les paramètres géométriques qui priment. Les applications qui déterminent la géométrie comme les logiciels de CAO ne doivent pas autoriser la modification de cette propriété."@fr-FR , "Portée libre. Cette propriété est donnée en complément de la représentation de la forme de l'élément et des paramètres géométriques qui la déterminent. En cas d'incohérence entre ces paramètres géométriques et cette propriété, ce sont les paramètres géométriques qui priment."@fr-FR , "Clear span for this object.\n\nThe shape information is provided in addition to the shape representation and the geometric parameters used within. In cases of inconsistency between the geometric parameters and the shape properties, provided in the attached property, the geometric parameters take precedence. For geometry editing applications, like CAD: this value should be write-only."@en , "该对象的净跨度。\n该属性所提供的形状信息是对内部形状描述和几何参数的补充。如果几何参数与该属性所提供的形状属性不符，应以几何参数为准。对CAD等几何编辑程序，该属性应为只写类型。"@zh-CN , "Clear span for this object.\nThe shape information is provided in addition to the shape representation and the geometric parameters used within. In cases of inconsistency between the geometric parameters and the shape properties, provided in the attached property, the geometric parameters take precedence."@en , "Lichte Spannweite des Balkens für die statische Anforderung,\n\nDieser Parameter wird zusätzlich zur geometrischen Repräsentation bereitgestellt. Im Fall der Inkonsistenz zwischen dem Parameter und der Geometrie hat die geometrische Repräsention Priorität. Dieser Parameter ist für CAD Software write-only."@de-DE , "このオブジェクトの全長。\n\nその形状（オブジェクトの全長）情報は、表示のための形状に内部で使用される幾何学的パラメータを加えて提供される。形状情報と内部の幾何学的パラメータに矛盾が生じた場合は、幾何学的パラメータが優先される。幾何学的パラメ－タ編集アプリケーションでは、CADと同様に、この値は書き込み専用とする。"@ja-JP , "German-description-2"@de-DE , "このオブジェクトの全長。"@ja-JP ;
        rdfs:label             "全長"@ja-JP , "跨度"@zh-CN , "span"@en , "Spannweite"@de-DE , "PorteeLibre"@fr-FR ;
        rdfs:range             <https://w3id.org/product/PositiveLengthMeasure> ;
        schema:domainIncludes  <https://w3id.org/product/Beam> , <https://w3id.org/product/Member> .

props:temperatureEffectiveness
        a                      owl:DatatypeProperty ;
        rdfs:comment           "Temperature heat transfer effectiveness: The ratio of primary airflow temperature changes to maximum possible temperature changes."@en , "温度熱交換効率：\n最大可能温度変化に対する一次側温度変化の比"@ja-JP , "Efficacité thermique sensible: rapport entre la différence de températures pour le flux primaire sur la différence maximale d'échange possible."@fr-FR ;
        rdfs:label             "temperatureEffectiveness"@en , "温度効率"@ja-JP , "EfficacitéTempérature"@fr-FR ;
        schema:domainIncludes  <https://w3id.org/product/AirToAirHeatRecovery> .

props:capColor  a              owl:DatatypeProperty ;
        rdfs:comment           "Color of the caps of the hydrant.\n\nNote: Consult local fire regulations for statutory colors that may be required for hydrant caps in particular circumstances."@en , "消火栓キャップの色。\n\n注意：特定の状況で消火栓キャップに求められる地域消防規則法定色による。"@ja-JP ;
        rdfs:label             "capColor"@en , "キャップ色"@ja-JP ;
        rdfs:range             xsd:string ;
        schema:domainIncludes  <https://w3id.org/product/FireSuppressionTerminal%2FFIREHYDRANT> .

props:sensitivity  a           owl:DatatypeProperty ;
        rdfs:comment           "Current leakage to an unwanted leading path during normal operation (IEC 151-14-49)."@en , "通常操作における望ましくない引き込みパスとの電流鎖交 (IEC 151-14-49)。"@ja-JP , "装置のメイン回路を流れる瞬時電流の合計ベクトルの関連する rms 値、特定の条件になると機器が動作するようになる（IEC 61008-1)。"@ja-JP , "The rated rms value of the vector sum of the instantaneous currents flowing in the main circuits of the device which causes the device to operate under specified conditions. (IEC 61008-1)."@en , "정상 작동의 원치 않는 철회 경로와 전류 사슬 교환 (IEC 151-14-49)."@ko-KR , "장치의 기본 회로를 흐르는 순간 전류의 합계 벡터 관련 rms 값이 특정 조건이되면 장치가 작동하게된다 (IEC 61008-1)."@ko-KR ;
        rdfs:label             "감도"@ko-KR , "感度"@ja-JP , "sensitivity"@en ;
        rdfs:range             <https://w3id.org/product/ElectricCurrentMeasure> ;
        schema:domainIncludes  <https://w3id.org/product/ProtectiveDevice%2FRESIDUALCURRENTSWITCH> , <https://w3id.org/product/ProtectiveDevice%2FRESIDUALCURRENTCIRCUITBREAKER> , <https://w3id.org/product/ProtectiveDevice%2FEARTHLEAKAGECIRCUITBREAKER> .

props:typeDesignator  a        owl:DatatypeProperty ;
        rdfs:comment           "Type designator for the precast concrete slab, expressing mainly the component type. Possible values are “Hollow-core”, “Double-tee”, “Flat plank”, etc."@en , "プレキャストコンクリート要素の特定子（部位）を記述する。内容はローカルな（各国の）標準（規格）に依存する。例えばフィンランドでは、柱はP、梁はKのように通常、頭文字1文字で表す。"@ja-JP , "Type designator for the precast concrete element. The content depends on local standards. For instance in Finland it usually a one-letter acronym, e.g. P=Column, K=reinforced concrete beam,etc."@en ;
        rdfs:label             "特定子の記述"@ja-JP , "typeDesignator"@en ;
        rdfs:range             xsd:string ;
        schema:domainIncludes  <https://w3id.org/product/Slab> , <https://w3id.org/product/BuildingElement> .

props:sprinklerProtection
        a                      owl:DatatypeProperty ;
        rdfs:comment           "Angabe, ob der Raum durch eine Sprinkleranlage geschützt wird (WAHR) oder nicht (FALSCH)."@de-DE , "스프링 클러 설비의 유무를 나타내는 부울 값입니다. (TRUE) 유 (FALSE) 없음."@ko-KR , "Indication selon laquelle ce bâtimentbénéficie d'une protection par sprinkler (VRAI) ou non (FAUX)"@fr-FR , "Indication whether this object is sprinkler protected (TRUE) or not (FALSE)."@en , "スプリンクラー設備の有無を示すブーリアン値。(TRUE)有、(FALSE)なし。"@ja-JP , "スプリンクラー設備の有無を示すブーリアン値。"@ja-JP , "스프링 클러 설비의 유무를 나타내는 값"@ko-KR , "Indication selon laquelle ce bâtiment bénéficie d'une protection par sprinkler (VRAI) ou non (FAUX)."@fr-FR , "Indication whether the space is sprinkler protected (TRUE) or not (FALSE)."@en , "Angabe, ob das Gebäude durch eine Sprinkleranlage geschützt wird (WAHR) oder nicht (FALSCH)."@de-DE , "Angabe, ob des Geschoss durch eine Sprinkleranlage geschützt wird (WAHR) oder nicht (FALSCH)."@de-DE ;
        rdfs:label             "Sprinklerschutz"@de-DE , "sprinklerProtection"@en , "スプリンクラー防御"@ja-JP , "스프링 클러 방어"@ko-KR , "ProtectionParSprinkler"@fr-FR ;
        rdfs:range             xsd:boolean ;
        schema:domainIncludes  <https://w3id.org/product/Building> , <https://w3id.org/product/cSpatialZone> , <https://w3id.org/product/BuildingStorey> , <https://w3id.org/product/cZone> , <https://w3id.org/product/Space> .

props:protectedOpening
        a                      owl:DatatypeProperty ;
        rdfs:comment           "Indication whether the opening is considered to be protected under fire safety considerations. If (TRUE) it counts as a protected opening under the applicable building code, (FALSE) otherwise."@en , "開港が安全性を考慮した保護機能があるかどうかを示すブーリアン値。適用される建築基準などにより保護されている場合(TRUE)、そうではない場合(FALSE）となる。"@ja-JP , "Indique si l'ouverture fait l'objet d'une protection incendie. Si (VRAI) elle est considérée comme une ouverture avec protection conformément à la règlementation applicable, (FAUX) sinon."@fr-FR ;
        rdfs:label             "protectedOpening"@en , "保護"@ja-JP , "Ouverture avec protection incendie"@fr-FR ;
        rdfs:range             xsd:boolean ;
        schema:domainIncludes  <https://w3id.org/product/OpeningElement> .

props:connectionSubtype
        a                      owl:DatatypeProperty ;
        rdfs:comment           "The physical port connection subtype that further qualifies the ConnectionType.  The following values are recommended:\nACPLUG: A, B, C, D, E, F, EF, G, H, I, J, K, L, M; RADIO: IEEE802.11g, IEEE802.11n\n; RJ: 4P4C, 6P2C, 8P8C; DIN: Mini3P, Mini4P, Mini5P, Mini6P, Mini7P, Mini8P, Mini9P \nDSub: DA15, DB25, DC37, DD50, DE9, DE15 \nEIAJ: RC5720\nHDMI: A, B, C\nTRS: TS_Mini, TS_SubMini, TRS_Mini, TRS_SubMini"@en , "物理ポート接続のサブタイプ。接続タイプ以外の情報を設定する場合に使用。下記の値を設定：\n\n- ACプラグ: A, B, C, D, E, F, EF, G, H, I, J, K, L, M"@ja-JP ;
        rdfs:label             "connectionSubtype"@en , "接続サブタイプ"@ja-JP ;
        rdfs:range             xsd:string ;
        schema:domainIncludes  <https://w3id.org/product/DistributionPort%2FELECTRICAL> .

props:drainSize  a             owl:DatatypeProperty ;
        rdfs:comment           "要素への接続口径。"@ja-JP , "要素の排水口接続口サイズ。"@ja-JP , "The size of the drain outlet connection from the object."@en , "要素から排水溝への下水管サイズ。"@ja-JP , "排水口の接続のサイズ。"@ja-JP ;
        rdfs:label             "ドレインサイズ"@ja-JP , "管口径"@ja-JP , "管径"@ja-JP , "drainSize"@en , "下水管サイズ"@ja-JP ;
        rdfs:range             <https://w3id.org/product/PositiveLengthMeasure> ;
        schema:domainIncludes  <https://w3id.org/product/SanitaryTerminal%2FBIDET> , <https://w3id.org/product/SanitaryTerminal%2FSINK> , <https://w3id.org/product/SanitaryTerminal%2FSANITARYFOUNTAIN> , <https://w3id.org/product/SanitaryTerminal%2FBATH> , <https://w3id.org/product/SanitaryTerminal%2FSHOWER> , <https://w3id.org/product/SanitaryTerminal%2FWASHHANDBASIN> .

props:fireHydrantType
        a                      owl:DatatypeProperty ;
        rdfs:comment           "Defines the range of hydrant types from which the required type can be selected where.\n\nDryBarrel:\t A hydrant that has isolating valves fitted below ground and that may be used where the possibility of water freezing is a consideration.\nWetBarrel:\t A hydrant that has isolating valves fitted above ground and that may be used where there is no possibility of water freezing."@en , "消火栓の必要なタイプを定義する。\n\n乾式l：凍結の可能性のあるとき地中に開放弁セット。\n\n湿式：凍結の可能性のないとき地上に開放弁セット。"@ja-JP ;
        rdfs:label             "fireHydrantType"@en , "消火栓のタイプ"@ja-JP ;
        schema:domainIncludes  <https://w3id.org/product/FireSuppressionTerminal%2FFIREHYDRANT> .

props:nominalLatentCapacity
        a                      owl:DatatypeProperty ;
        rdfs:comment           "Nominal latent capacity."@en , "Puissance latente nominale."@fr-FR ;
        rdfs:label             "nominalLatentCapacity"@en , "PuissanceLatenteNominale"@fr-FR ;
        rdfs:range             <https://w3id.org/product/PowerMeasure> ;
        schema:domainIncludes  <https://w3id.org/product/Coil> .

props:heatingDryBulb  a        owl:DatatypeProperty ;
        rdfs:comment           "난방 설계 외기 건구 온도"@ko-KR , "난방 설계의 실내 디자인 건구 온도"@ko-KR , "Outside dry bulb temperature for heating design."@en , "暖房用設計用外気乾球温度。"@ja-JP , "暖房設計における室内設計乾球温度。"@ja-JP , "Inside dry bulb temperature for heating design."@en ;
        rdfs:label             "暖房用設計外気乾球温度"@ja-JP , "暖房設計温度"@ja-JP , "heatingDryBulb"@en , "난방 설계 외기 건구 온도"@ko-KR , "난방 설계온도"@ko-KR ;
        rdfs:range             <https://w3id.org/product/ThermodynamicTemperatureMeasure> ;
        schema:domainIncludes  <https://w3id.org/product/Building> , <https://w3id.org/product/Space> .

props:convectorType  a         owl:DatatypeProperty ;
        rdfs:comment           "Indicates the type of convector, whether forced air (mechanically driven) or natural (gravity)."@en , "強制空気(機械的に運転される)か自然な(重力)であることにかかわらず対流式暖房器のタイプを示します。"@ja-JP ;
        rdfs:label             "convectorType"@en , "対流タイプ"@ja-JP ;
        schema:domainIncludes  <https://w3id.org/product/SpaceHeater%2FCONVECTOR> .

props:lowerTime2  a            owl:DatatypeProperty ;
        rdfs:comment           "The time in [s], indicating the tripping times of the upper time/current curve at the LowerCurrent2."@en , "[s]の時間,下電流2より下部の特性曲線のトリップ時間を示す。"@ja-JP , "[s] 시간, 아래 전류 2보다 하부의 특성 곡선의 트립 시간을 보여준다."@ko-KR ;
        rdfs:label             "lowerTime2"@en , "下時間2"@ja-JP , "하 시간 2"@ko-KR ;
        rdfs:range             <https://w3id.org/product/TimeMeasure> ;
        schema:domainIncludes  <https://w3id.org/product/ProtectiveDeviceTrippingUnit> .

props:airFlowConfiguration
        a                      owl:DatatypeProperty ;
        rdfs:comment           "Air flow configuration type of cooled beam."@en ;
        rdfs:label             "airFlowConfiguration"@en ;
        schema:domainIncludes  <https://w3id.org/product/CooledBeam%2FACTIVE> .

props:shortTimeFunction
        a                      owl:DatatypeProperty ;
        rdfs:comment           "Applying short time function A flag indicating that the short time function of the device is used. The value should be set to FALSE for devices not having a short time function, or if the short time function is not selected to be used."@en ;
        rdfs:label             "shortTimeFunction"@en ;
        rdfs:range             xsd:boolean ;
        schema:domainIncludes  <https://w3id.org/product/ProtectiveDevice> .

props:higherHeatingValue
        a                      owl:DatatypeProperty ;
        rdfs:comment           "Higher Heating Value is defined as the amount of energy released (MJ/kg) when a fuel is burned completely, and H2O is in liquid form in the combustion products."@en ;
        rdfs:label             "higherHeatingValue"@en ;
        rdfs:range             <https://w3id.org/product/HeatingValueMeasure> ;
        schema:domainIncludes  <https://w3id.org/product/Material> .

props:signalTimeDecrease
        a                      owl:DatatypeProperty ;
        rdfs:comment           "Time factor used for exponential decrease."@en , "미분 시간 (Td)"@ko-KR ;
        rdfs:label             "signalTimeDecrease"@en , "미분 시간 (Td)"@ko-KR ;
        rdfs:range             <https://w3id.org/product/TimeMeasure> ;
        schema:domainIncludes  <https://w3id.org/product/Controller%2FPROPORTIONAL> .

props:currentCarryingCapasity
        a                      owl:DatatypeProperty ;
        rdfs:comment           "Maximum value of electric current which can be carried continuously by a conductor, a device or an apparatus, under specified conditions without its steady-state temperature exceeding a  specified value. Based on IEC60826-11-13. NOTE: The temperature specified value is maximum Design Ambient Temperature."@en ;
        rdfs:label             "currentCarryingCapasity"@en ;
        rdfs:range             <https://w3id.org/product/ElectricCurrentMeasure> ;
        schema:domainIncludes  <https://w3id.org/product/CableSegment> .

props:conditionCommencement
        a                      owl:DatatypeProperty ;
        rdfs:comment           "Condition of property provided on commencement of the agreement e.g. cold shell, warm lit shell, broom clean, turn-key."@en ;
        rdfs:label             "conditionCommencement"@en ;
        rdfs:range             xsd:string ;
        schema:domainIncludes  <https://w3id.org/product/SpatialStructureElement> .

props:playerMediaFormat
        a                      owl:DatatypeProperty ;
        rdfs:comment           "Indicates supported media formats."@en , "サポートされているメディアのフォーマットを示す。"@ja-JP , "지원되는 미디어 형식을 보여준다."@ko-KR ;
        rdfs:label             "playerMediaFormat"@en , "メディアフォーマット"@ja-JP , "미디어 포맷"@ko-KR ;
        schema:domainIncludes  <https://w3id.org/product/AudioVisualAppliance%2FPLAYER> .

props:glassLayers  a           owl:DatatypeProperty ;
        rdfs:comment           "Nombre de couches de verre dans le cadre. Exemple : 2 pour le double vitrage."@fr-FR , "ガラスの枚数。例：\"2\"はペアガラス。"@ja-JP , "框内玻璃的层数。例如：”2”表示双层玻璃。"@zh-CN , "Number of glass layers within the frame. E.g. \"2\" for double glazing."@en , "German-description-1"@de-DE ;
        rdfs:label             "ガラス枚数"@ja-JP , "NombreVitrages"@fr-FR , "German-name-1"@de-DE , "玻璃层数"@zh-CN , "glassLayers"@en ;
        rdfs:range             <https://w3id.org/product/CountMeasure> ;
        schema:domainIncludes  <https://w3id.org/product/cWindow> , <https://w3id.org/product/Door> .

props:heatOutput  a            owl:DatatypeProperty ;
        rdfs:comment           "Total nominal heat output as listed by the Boiler manufacturer. For water boilers, it is a function of inlet versus outlet temperature. For steam boilers, it is a function of inlet temperature versus steam pressure.  Note: as two variables are used, DefiningValues and DefinedValues are null, and values are stored in IfcTable in the following order: InletTemperature(IfcThermodynamicTemperatureMeasure), OutletTemperature(IfcThermodynamicTemperatureMeasure), HeatOutput(IfcEnergyMeasure).  The IfcTable is related to IfcPropertyTableValue using IfcMetric and IfcPropertyConstraintRelationship."@en , "Rendement total nominal tel que défini par le constructeur de chaudière.\nPour les chaudières à eau chaude, une fonction de la température en entrée par rapport à la température de sortie.\nRemarque: Comme deux variables sont utilisées ValeurDefinir et ValeursDefinies sont nulles, et les valeurs sont enregistrées dans IfcTable dans l'ordre suivant:\n- TempératureEntrée (IfcThermodynamicTemperatureMeasure) et TempératureSortie (IfcThermodynamicTemperatureMeasure) dans ValeursDefinir , et Rendement de chaleur (IfcEnergyMeasure) dansValeursDefinies.\nIfcPropertyTable est lié à IfcMetric qui utilise IfcMetric et IfcPropertyConstraintRelationship."@fr-FR , "Total nominal heat output as listed by the Boiler manufacturer. For steam boilers, it is a function of inlet temperature versus steam pressure.  Note: as two variables are used, DefiningValues and DefinedValues are null, and values are stored in IfcTable in the following order: InletTemperature(IfcThermodynamicTemperatureMeasure) and OutletTemperature(IfcThermodynamicTemperatureMeasure) in DefiningValues, and HeatOutput(IfcEnergyMeasure) in DefinedValues. For example, DefiningValues(InletTemp, OutletTemp), DefinedValues(null, HeatOutput). The IfcTable is related to IfcPropertyTableValue using IfcMetric and IfcPropertyConstraintRelationship."@en , "Rendement total nominal tel que défini par le constructeur de chaudière.\nPour les chaudières à vapeur, une fonction de la température en entrée par rapport à la pression de vapeur.\nRemarque: Comme deux variables sont utilisées ValeurDefinir et ValeursDefinies sont nulles, et les valeurs sont enregistrées dans IfcTable dans l'ordre suivant:\n- TempératureEntrée (IfcThermodynamicTemperatureMeasure) et TempératureSortie (IfcThermodynamicTemperatureMeasure) dans ValeursDefinir , et Rendement de chaleur (IfcEnergyMeasure) dansValeursDefinies.\nPar exemple, ValeursDefinir (TempératureEntrée, TempératureSortie), ValeursDefinies (nul, RendementChaleur).\nIfcPropertyTable est lié à IfcMetric qui utilise IfcMetric et IfcPropertyConstraintRelationship."@fr-FR ;
        rdfs:label             "heatOutput"@en , "RendementChaleur"@fr-FR ;
        schema:domainIncludes  <https://w3id.org/product/Boiler%2FWATER> , <https://w3id.org/product/Boiler%2FSTEAM> .

props:lightFixtureMountingType
        a                      owl:DatatypeProperty ;
        rdfs:comment           "A list of the available types of mounting for light fixtures from which that required may be selected."@en , "照明器具の取付方法をリストから選択。"@ja-JP , "조명기구의 설치 방법을 목록에서 선택합니다."@ko-KR ;
        rdfs:label             "lightFixtureMountingType"@en , "照明器具取付方法"@ja-JP , "조명기구 설치방법"@ko-KR ;
        schema:domainIncludes  <https://w3id.org/product/LightFixture> .

props:temperatureSensorType
        a                      owl:DatatypeProperty ;
        rdfs:comment           "Enumeration that Identifies the types of temperature sensor that can be specified."@en , "明示された温度センサーのタイプを識別する一覧。"@ja-JP , "명시된 온도 센서 유형을 식별하는 목록."@ko-KR ;
        rdfs:label             "temperatureSensorType"@en , "温度センサータイプ"@ja-JP , "온도 센서 타입"@ko-KR ;
        schema:domainIncludes  <https://w3id.org/product/Sensor%2FTEMPERATURESENSOR> .

props:totalHeatingLoad
        a                      owl:DatatypeProperty ;
        rdfs:comment           "The peak total heating load for the building, zone or space."@en , "建物、ゾーン、部屋のピーク時の暖房負荷。"@ja-JP , "건물 영역 방 최대 난방 부하."@ko-KR ;
        rdfs:label             "totalHeatingLoad"@en , "暖房負荷"@ja-JP , "난방 부하"@ko-KR ;
        rdfs:range             <https://w3id.org/product/PowerMeasure> ;
        schema:domainIncludes  <https://w3id.org/product/SpatialElement> .

props:faucetOperation
        a                      owl:DatatypeProperty ;
        rdfs:comment           "Defines the range of ways in which a faucet can be operated that may be specified where:\n\nCeramicDisc: Quick action faucet with a ceramic seal to open or close the orifice\n.\nLeverHandle: Quick action faucet that is operated by a lever handle\n.\nNonConcussiveSelfClosing:\t Self closing faucet that does not induce surge pressure\n.\nQuarterTurn: Quick action faucet that can be fully opened or shut by turning the operating mechanism through 90 degrees.\nQuickAction: Faucet that can be opened or closed fully with a single small movement of the operating mechanism\n.\nScrewDown: Faucet in which a plate or disc is moved, by the rotation of a screwed spindle, to close or open the orifice.\nSelfClosing: Faucet that is opened by pressure of the top of an operating spindle and is closed under the action of a spring or weight when the pressure is released.\nTimedSelfClosing: \tSelf closing faucet that discharges for a predetermined period of time\n."@en , "水栓の操作方法の範囲をここで明確に定義する：\nCeramicDisc = 口を開閉するセラミックシールを持った急操作水栓　LeverHandle = レバーハンドルで操作される急操作水栓　SelfClosing =サージ圧をもたらさない自閉水栓　QuarterTurn =90度、操作機構を回すことで全開又は全閉できる急操作水栓　QuickAction =操作機構の一つの小さな動きで全開又は全閉できる水栓　ScrewDown =口を開閉するためにねじの主軸を回して中の板又は円板を動かす水栓　SelfClosing = 操作主軸の頂部の圧力で開けられ、圧力が開放された時は、ばね又は錘の動作で閉められる水栓　TimedSelfClosing =前もって決められた時間、吐出する自閉水栓"@ja-JP ;
        rdfs:label             "faucetOperation"@en , "水栓操作"@ja-JP ;
        schema:domainIncludes  <https://w3id.org/product/Valve%2FFAUCET> .

props:fittingLossFactor
        a                      owl:DatatypeProperty ;
        rdfs:comment           "A factor that determines the pressure loss due to friction through the fitting."@en , "接合部を通過する際の摩擦による圧力損失を決める係数"@ja-JP ;
        rdfs:label             "fittingLossFactor"@en , "継ぎ手接合部損失係数"@ja-JP ;
        rdfs:range             xsd:decimal ;
        schema:domainIncludes  <https://w3id.org/product/PipeFitting> .

props:setbackDistance
        a                      owl:DatatypeProperty ;
        rdfs:comment           "Setback distance from the point of connection on the major element along the axis of the minor element (e.g. distance from a public road at which the line of sigfht is measured."@en , "Distance de recul le long de l'axe de l'élément secondaire depuis le point de jonction sur l'élément principal (par exemple, distance depuis la route principale à partir de laquelle la visibilité est appréciée)."@fr-FR , "副要素の軸に沿った主要素の接続点からの後退距離（例えば、可視線が測定される公道からの距離）。"@ja-JP ;
        rdfs:label             "setbackDistance"@en , "DistanceRecul"@fr-FR , "後退距離"@ja-JP ;
        rdfs:range             <https://w3id.org/product/PositiveLengthMeasure> ;
        schema:domainIncludes  <https://w3id.org/product/Annotation%2FLineOfSight> .

props:outsideDiameter
        a                      owl:DatatypeProperty ;
        rdfs:comment           "Actual outside diameter of the tube in the tube bundle."@en , "チューブ束内のチューブ実外径"@ja-JP ;
        rdfs:label             "outsideDiameter"@en , "外径"@ja-JP ;
        rdfs:range             <https://w3id.org/product/PositiveLengthMeasure> ;
        schema:domainIncludes  <https://w3id.org/product/TubeBundle> .

props:isOffWhenLfunctionOn
        a                      owl:DatatypeProperty ;
        rdfs:comment           "Indication whether the S-function is automatically switched off when the I-function is switched on."@en ;
        rdfs:label             "isOffWhenLfunctionOn"@en ;
        rdfs:range             xsd:boolean ;
        schema:domainIncludes  <https://w3id.org/product/ProtectiveDeviceTrippingUnit> .

props:flowControlType
        a                      owl:DatatypeProperty ;
        rdfs:comment           "Type of flow control element that may be included as a part of the construction of the air terminal."@en , "ターミナルの構成の一部として含まれる流量制御の形式\n（ダンパー、ベローズ、無し…）"@ja-JP , "Nature de la commande de flux d'un élément qui pourrait être inclus en tant que tel dans le terminal de ventilation."@fr-FR ;
        rdfs:label             "flowControlType"@en , "流量制御形式"@ja-JP , "NatureCommandeFlux"@fr-FR ;
        schema:domainIncludes  <https://w3id.org/product/AirTerminal> .

props:solarAbsorption
        a                      owl:DatatypeProperty ;
        rdfs:comment           "German-description-13"@de-DE , "(Asol). Ratio du rayonnement solaire incident qui est absorbé par le vitrage. Somme de l'absorption distribuée à l'extérieur (a) et à l'intérieur (qi). Noter l'équation suivante : Asol + Rsol + Tsol = 1."@fr-FR , "（Asol）被玻璃系统吸收的太阳入射辐射的比率，为传递到室外和室内的吸收的总量。注：以下等式成立Asol + Rsol + Tsol = 1"@zh-CN , "（Asol)ガラスで吸収される日射の比率。吸収の合計は外部（a）と、室内（qi）に分配される。以下の方程式に注意。Asol + Rsol + Tsol = 1"@ja-JP , "(Asol) The ratio of incident solar radiation that is absorbed by a glazing system. It is the sum of the absorption distributed to the exterior (a) and to the interior (qi). Note the following equation Asol + Rsol + Tsol = 1"@en ;
        rdfs:label             "solarAbsorption"@en , "日射吸収率"@ja-JP , "太阳能吸收率"@zh-CN , "Strahlungsabsorbtionsgrad"@de-DE , "AbsorptionRayonnementSolaire"@fr-FR ;
        rdfs:range             <https://w3id.org/product/NormalisedRatioMeasure> ;
        schema:domainIncludes  <https://w3id.org/product/cWindow> , <https://w3id.org/product/Door> .

props:countedEfficiency
        a                      owl:DatatypeProperty ;
        rdfs:comment           "Filter efficiency based the particle counts concentration before and after filter against particles with certain size distribution."@en ;
        rdfs:label             "countedEfficiency"@en ;
        schema:domainIncludes  <https://w3id.org/product/Filter> .

props:thermalIrTransmittance
        a                      owl:DatatypeProperty ;
        rdfs:comment           "Thermal IR transmittance at normal incidence. Defines the fraction of thermal energy that passes through per unit area, perpendicular to the surface."@en ;
        rdfs:label             "thermalIrTransmittance"@en ;
        rdfs:range             <https://w3id.org/product/PositiveRatioMeasure> ;
        schema:domainIncludes  <https://w3id.org/product/Material> .

props:rentalRatesInCategoryNow
        a                      owl:DatatypeProperty ;
        rdfs:comment           "Range of the cost rates for property currently available in the required category."@en , "Prix actuel des loyers pour la catégorie considérée."@fr-FR ;
        rdfs:label             "rentalRatesInCategoryNow"@en , "PrixActuelLoyerParCategorie"@fr-FR ;
        schema:domainIncludes  <https://w3id.org/product/Building> .

props:shortOutsideLowerBarPitch
        a                      owl:DatatypeProperty ;
        rdfs:comment           "The pitch length of the short outside lower bar."@en , "短辺方向・柱列帯・下端の鉄筋間隔。"@ja-JP ;
        rdfs:label             "shortOutsideLowerBarPitch"@en , "短辺・柱列帯・下端ピッチ"@ja-JP ;
        rdfs:range             <https://w3id.org/product/PositiveLengthMeasure> ;
        schema:domainIncludes  <https://w3id.org/product/Slab> .

props:compressionEfficiency
        a                      owl:DatatypeProperty ;
        rdfs:comment           "Ratio of the work required for isentropic compression of the gas to the work delivered to the gas within the compression volume (as obtained by measurement)."@en , "Rapport entre le travail requis pour une compression isentropique du gaz et le travail fourni au gaz dans le volume comprimé (telq qu'obtenu par mesure)."@fr-FR ;
        rdfs:label             "compressionEfficiency"@en , "RendementCompression"@fr-FR ;
        schema:domainIncludes  <https://w3id.org/product/Compressor> .

props:ceilingCovering
        a                      owl:DatatypeProperty ;
        rdfs:comment           "Label to indicate the material or finish of the space flooring. The label is used for room book information and often displayed in room stamp.\n\nThe material information is provided in absence of an IfcCovering (type=CEILING) object with own shape representation and material assignment. In case of inconsistency the material assigned to IfcCovering elements takes precedence."@en , "部屋の天井材質または仕上げに関するラベル（識別情報）。このラベル名は部屋リスト情報や部屋情報表示の際に利用される。"@ja-JP , "Indication sur la nature du revêtement de plafond […]. L'information sur le matériau est fournie en l'absence d'un objet de la classe IfcCovering (Type=CEILING) avec sa propre représentation de forme et une assignation à un matériau. En cas d'incohérence, c'est le matériau assigné à l'instance de IfcCovering qui prime."@fr-FR , "Angabe des Materials für die Deckenbekleidung oder den Deckenbelag (bzw. der Unterdecke). Diese Angabe wird im Raumbuch verwendet und oft im Raumstempel angezeigt.\n\nDie Materialangabe wird übernommen, wenn kein eigenes Bekleidungsobjekt (IfcCovering mit PredefinedType = CEILING) für die Deckenbekleidung dem Raum zugeordnet ist. Bei Inkonsistenzen (wenn beides gegeben ist), hat die Materialangabe des zugeordneten Bekleidungsobjekts Priorität."@de-DE ;
        rdfs:label             "ceilingCovering"@en , "天井仕上げ"@ja-JP , "RevetementPlafond"@fr-FR , "Deckenbekleidung"@de-DE ;
        rdfs:range             xsd:string ;
        schema:domainIncludes  <https://w3id.org/product/Space> .

props:isHighPressure  a        owl:DatatypeProperty ;
        rdfs:comment           "Indication of whether the flushing valve is suitable for use on a high pressure water main (set TRUE) or not (set FALSE)."@en , "フラッシュ弁の高圧給水主管への使用が適当かどうかの表示（適 TRUE）又は（不適 FALSE）"@ja-JP ;
        rdfs:label             "isHighPressure"@en , "高圧給水の有無"@ja-JP ;
        rdfs:range             xsd:boolean ;
        schema:domainIncludes  <https://w3id.org/product/Valve%2FFLUSHING> .

props:sinkType  a              owl:DatatypeProperty ;
        rdfs:comment           "Selection of the type of sink from the enumerated list of types where:-\n\nBelfast: \tDeep sink that has a plain edge and a weir overflow\n.\nBucket: \tSink at low level, with protected front edge, that facilitates filling and emptying buckets, usually with a hinged grid on which to stand them.\nCleaners:\t Sink, usually fixed at normal height (900mm), with protected front edge.\nCombination_Left:\t Sink with integral drainer on left hand side\n.\nCombination_Right: Sink with integral drainer on right hand side\n.\nCombination_Double: \tSink with integral drainer on both sides\n.\nDrip: Small sink that catches drips or flow from a faucet\n.\nLaboratory: Sink, of acid resisting material, with a top edge shaped to facilitate fixing to the underside of a desktop\n.\nLondon: Deep sink that has a plain edge and no overflow\n.\nPlaster: Sink with sediment receiver to prevent waste plaster passing into drains\n.\nPot: Large metal sink, with a standing waste, for washing cooking utensils\n.\nRinsing: Metal sink in which water can be heated and culinary utensils and tableware immersed at high temperature that destroys most harmful bacteria and allows subsequent self drying.\n.\nShelf: Ceramic sink with an integral back shelf through which water fittings are mounted\n.\nVegetablePreparation: \tLarge metal sink, with a standing waste, for washing and preparing vegetables\n."@en , "シンクタイプの選択\n\n・深流し：エッジが平らであふれにくい深いシンク\n• 下流し：先端が保護され、低水位用のシンク\n・掃除流し：先端が保護されたシンク（通常は900mm高さに調整されたもの）\n・左水切り：左側に水切りが付いているシンク\n・右水切り流し：右側に水切りが付いているシンク\n・両水切り流し：両側に水切りが付いているタイプ\n・点滴：蛇口からの流れや滴を捕まえる小さめのシンク\n・実験流し：デスク天板下が簡易的に固定された他耐酸性の材料を使ったシンク\n・ロンドン：オーバーフローなしのエッジが平らの深いシンク\n・石膏流し：廃石膏が排水管中に入ってしまうのをを防ぐため、沈殿物レシーバーが付いているシンク。\n・料理流し：ゴミの廃棄もできる調理用具を洗うためのシンク\n・すすぎ用の流し：高温滅菌ができる乾いた状態を保持できる鉄製のシンク\n・棚付き流し：金具の接続や設置ができる棚を後ろに持つセラミック製のシンク\n・野菜流し：ゴミの廃棄もできる、洗浄や調理の準備をする大きめの鉄製のシンク"@ja-JP ;
        rdfs:label             "sinkType"@en , "シンクの種類"@ja-JP ;
        schema:domainIncludes  <https://w3id.org/product/SanitaryTerminal%2FSINK> .

props:nominalPowerRate
        a                      owl:DatatypeProperty ;
        rdfs:comment           "Nominal fan power rate."@en , "設計動力"@ja-JP ;
        rdfs:label             "nominalPowerRate"@en , "設計動力"@ja-JP ;
        rdfs:range             <https://w3id.org/product/PowerMeasure> ;
        schema:domainIncludes  <https://w3id.org/product/Fan> .

props:setPointRadioactivity
        a                      owl:DatatypeProperty ;
        rdfs:comment           "The radioactivity value to be sensed. Use IfcPropertyBoundedValue.SetPointValue to set the set point value."@en , "感知される放射能。\nセットポイント値を置くために、IfcPropertyBoundedValue.SetPointValueを使用する。"@ja-JP , "감지되는 방사능. 세트 포인트 값을 넣으려면, IfcPropertyBoundedValue.SetPointValue를 사용하십시오."@ko-KR ;
        rdfs:label             "setPointRadioactivity"@en , "放射能設定値"@ja-JP , "방사능 설정"@ko-KR ;
        schema:domainIncludes  <https://w3id.org/product/Sensor%2FRADIOACTIVITYSENSOR> .

props:renewableEnergyConsumption
        a                      owl:DatatypeProperty ;
        rdfs:comment           "ISO21930 : 2007에 정의된 재생 가능 에너지 사용량"@ko-KR , "Quantity of renewable energy used as defined in ISO21930:2007"@en , "ISO21930:2007 で定義されている継続可能なエネルギー消費量。"@ja-JP , "Consommation d'énergie renouvelable telle que définie dans les normes ISO21930:2007 [NDT : ou NF P01-010]"@fr-FR ;
        rdfs:label             "継続可能なエネルギー消費量"@ja-JP , "재생 가능 에너지 소비"@ko-KR , "renewableEnergyConsumption"@en , "ConsommationEnergieRenouvelable"@fr-FR ;
        rdfs:range             <https://w3id.org/product/EnergyMeasure> ;
        schema:domainIncludes  <https://w3id.org/product/Element> .

props:shearDeformationAreaZ
        a                      owl:DatatypeProperty ;
        rdfs:comment           "Area of the profile for calculating the shear deformation due to a shear force parallel to zs. For example measured in mm². If given, the shear deformation area zs shall be non-negative."@en ;
        rdfs:label             "shearDeformationAreaZ"@en ;
        rdfs:range             <https://w3id.org/product/AreaMeasure> ;
        schema:domainIncludes  <https://w3id.org/product/ProfileDef> .

props:earthFault1PolePowerFactorMinimumState
        a                      owl:DatatypeProperty ;
        rdfs:comment           "Power factor of the minimum 1 pole earth fault current provided at the point of supply i.e. the fault between 1 phase and PE/PEN."@en , "電源供給時点の点1相とPE/PEN間の1極最小地絡電流力率。"@ja-JP , "전원 공급 시점 점 1 상 및 PE / PEN 사이의 1 극 최소 지락 전류 역률."@ko-KR ;
        rdfs:label             "earthFault1PolePowerFactorMinimumState"@en , "1極最小地絡電流力率"@ja-JP , "1극  최소 지락 전류 역률"@ko-KR ;
        rdfs:range             xsd:decimal ;
        schema:domainIncludes  <https://w3id.org/product/ElectricFlowStorageDevice> .

props:modelReference  a        owl:DatatypeProperty ;
        rdfs:comment           "The model number or designator of the product model (or product line) as assigned by the manufacturer of the manufactured item."@en ;
        rdfs:label             "modelReference"@en ;
        rdfs:range             xsd:string ;
        schema:domainIncludes  <https://w3id.org/product/Element> .

props:installationMethodFlagEnum
        a                      owl:DatatypeProperty ;
        rdfs:comment           "Special installation conditions relating to particular types of installation based on IEC60364-5-52:2001 reference installation methods C and D."@en ;
        rdfs:label             "installationMethodFlagEnum"@en ;
        schema:domainIncludes  <https://w3id.org/product/CableSegment> .

props:tankComposition
        a                      owl:DatatypeProperty ;
        rdfs:comment           "Defines the level of element composition where.\n\nCOMPLEX: A set of elementary units aggregated together to fulfill the overall  required purpose.\nELEMENT: A single elementary unit that may exist of itself or as an aggregation of partial units..\nPARTIAL: A partial elementary unit."@en , "定義　構成要素のレベル　　　　　　　　　　　　　　　　　　　　　　　複合：A　全般的に要求された目的を達成するために集められた基本ユニットのセット　　　　　　　　　　　　　　　　　　　　　　　　　　　　　　要素：A それ自身あるいは部分的ユニットの集まりとしてある単一基本ユニット　　　　　　　　　　　　　　　　　　　　　　　　　　　　　　　　部分的：A 部分的な基本単位"@ja-JP ;
        rdfs:label             "tankComposition"@en , "水槽構成"@ja-JP ;
        schema:domainIncludes  <https://w3id.org/product/Tank> .

props:bendRadius  a            owl:DatatypeProperty ;
        rdfs:comment           "The radius of bending if circular arc or zero if sharp bend."@en , "円弧の曲率半径？"@ja-JP ;
        rdfs:label             "bendRadius"@en , "曲率半径"@ja-JP ;
        rdfs:range             <https://w3id.org/product/PositiveLengthMeasure> ;
        schema:domainIncludes  <https://w3id.org/product/PipeFitting%2FBEND> .

props:parkingUse  a            owl:DatatypeProperty ;
        rdfs:comment           "Identifies the type of transporation for which the parking space is designed. Values are not predefined but might include car, compact car, motorcycle, bicycle, truck, bus etc."@en , "Identifie le type de véhicule pour lequel le parking a été conçu. Les valeurs possibles (voiture, bus, motos, vélos,…)  ne sont pas prédéfinies."@fr-FR , "どの車両種別の駐車場なのかを識別します。値はあらかじめ定められないが、自動車、小型車、オートバイ、自転車、トラック、バスなどを含んでいるかもしれません。"@ja-JP ;
        rdfs:label             "parkingUse"@en , "AccessibleHandicape"@fr-FR , "駐車場の用途"@ja-JP ;
        rdfs:range             xsd:string ;
        schema:domainIncludes  <https://w3id.org/product/Space%2FPARKING> .

props:floorAreaRatio  a        owl:DatatypeProperty ;
        rdfs:comment           "The ratio of all floor areas to the buildable area as the maximum floor area utilization of the site as a maximum value according to local building codes."@en , "Geschossflächenzahl als Verhältnis der gesamten Geschossfläche aller Vollgeschosse der baulichen Anlagen auf einem Baugrundstück zu der Fläche des Baugrundstücks."@de-DE , "Ratio de la surface totale de planchers à la surface constructible, indication de la valeur maximale de la surface de planchers selon la règlementation locale (coefficient d'occupation des sols, N.d.T.)"@fr-FR , "建築基準により最大となる床面積と敷地面積(IfcElementQuantities)の比率。"@ja-JP ;
        rdfs:label             "ratio de surface de planchers"@fr-FR , "容積率"@ja-JP , "floorAreaRatio"@en , "Geschossflächenzahl"@de-DE ;
        rdfs:range             <https://w3id.org/product/PositiveRatioMeasure> ;
        schema:domainIncludes  <https://w3id.org/product/Site> .

props:thicknessSwelling
        a                      owl:DatatypeProperty ;
        rdfs:comment           "Swelling ratio relative to board depth."@en ;
        rdfs:label             "thicknessSwelling"@en ;
        rdfs:range             <https://w3id.org/product/PositiveRatioMeasure> ;
        schema:domainIncludes  <https://w3id.org/product/Material%2FWood> .

props:totalHeatGain  a         owl:DatatypeProperty ;
        rdfs:comment           "The total amount of heat or energy gained by the space at the time of the space's peak cooling conditions."@en , "ピーク時の室内最大冷房負荷時に取得した顕熱或いはエネルギー。"@ja-JP , "최대의 실내 최대 냉방 부하 취득한 현열 또는 에너지."@ko-KR ;
        rdfs:label             "totalHeatGain"@en , "熱取得の合計"@ja-JP , "연 인수 금액"@ko-KR ;
        rdfs:range             <https://w3id.org/product/PowerMeasure> ;
        schema:domainIncludes  <https://w3id.org/product/Space> .

props:combustionEfficiency
        a                      owl:DatatypeProperty ;
        rdfs:comment           "Combustion efficiency under nominal condition."@en , "設計条件での燃焼効率"@ja-JP , "Efficacité de la combustion sous conditions nominales."@fr-FR ;
        rdfs:label             "combustionEfficiency"@en , "燃焼効率"@ja-JP , "EfficacitéCombustion"@fr-FR ;
        schema:domainIncludes  <https://w3id.org/product/Boiler> .

props:agreementType  a         owl:DatatypeProperty ;
        rdfs:comment           "Identifies the predefined types of property agreement from which the type required may be set."@en ;
        rdfs:label             "agreementType"@en ;
        schema:domainIncludes  <https://w3id.org/product/SpatialStructureElement> .

props:outOfPlaneNegative
        a                      owl:DatatypeProperty ;
        rdfs:comment           "Mechanical properties with respect to out-of-plane load i.e. for function as a plate; compression zone of unbalanced layups is stressed in tension."@en ;
        rdfs:label             "outOfPlaneNegative"@en ;
        schema:domainIncludes  <https://w3id.org/product/Material%2FWood> .

props:numberOfChairs  a        owl:DatatypeProperty ;
        rdfs:comment           "Maximum number of chairs that can fit with the table for normal use."@en ;
        rdfs:label             "numberOfChairs"@en ;
        rdfs:range             xsd:int ;
        schema:domainIncludes  <https://w3id.org/product/Furniture%2FTABLE> .

props:boreSize  a              owl:DatatypeProperty ;
        rdfs:comment           "The nominal bore of the pipe flange."@en , "フランジの呼び径"@ja-JP ;
        rdfs:label             "boreSize"@en , "フランジの内径のサイズ"@ja-JP ;
        rdfs:range             <https://w3id.org/product/PositiveLengthMeasure> ;
        schema:domainIncludes  <https://w3id.org/product/PipeSegment> .

props:longTimeDelay  a         owl:DatatypeProperty ;
        rdfs:comment           "Long time delay. The set value of the long time time-delay if adjustable."@en ;
        rdfs:label             "longTimeDelay"@en ;
        rdfs:range             <https://w3id.org/product/TimeMeasure> ;
        schema:domainIncludes  <https://w3id.org/product/ProtectiveDevice> .

props:lightingLoadIntensity
        a                      owl:DatatypeProperty ;
        rdfs:comment           "Average lighting load intensity in the space per unit area (PowerMeasure/IfcAreaMeasure)."@en , "単位面積あたり照明機器の平均電力消費量。\n（PowerMeasure/IfcAreaMeasure）"@ja-JP , "단위 면적 당 조명의 평균 전력 소비. (PowerMeasure / IfcAreaMeasure)"@ko-KR ;
        rdfs:label             "lightingLoadIntensity"@en , "照明負荷率"@ja-JP , "조명 부하율"@ko-KR ;
        rdfs:range             xsd:decimal ;
        schema:domainIncludes  <https://w3id.org/product/SpatialElement> .

props:shortTimeTrippingTime
        a                      owl:DatatypeProperty ;
        rdfs:comment           "Short time tripping time. The set value of the short time tripping time if adjustable."@en ;
        rdfs:label             "shortTimeTrippingTime"@en ;
        rdfs:range             <https://w3id.org/product/TimeMeasure> ;
        schema:domainIncludes  <https://w3id.org/product/ProtectiveDevice> .

props:isLandmarked  a          owl:DatatypeProperty ;
        rdfs:comment           "Indique si le bâtiment est classé aux monuments historiques (VRAI) ou non (FAUX), ou si l'information n'est pas connue."@fr-FR , "이 건물은 역사적인 건물 있는지 여부를 나타내는 값"@ko-KR , "この建物は歴史的な建物かどうかを示すブーリアン値。"@ja-JP , "Angabe, ob das Gebäude dem Denkmalschutz unterliegt (WAHR) oder nicht (FALSCH)."@de-DE , "This builing is listed as a historic building (TRUE), or not (FALSE), or unknown."@en ;
        rdfs:label             "ランドマーク区分"@ja-JP , "ClasseMonumentHistorique"@fr-FR , "Denkmalschutz"@de-DE , "isLandmarked"@en , "랜드마크 구분"@ko-KR ;
        rdfs:range             xsd:boolean ;
        schema:domainIncludes  <https://w3id.org/product/Building> .

props:totalCoolingLoad
        a                      owl:DatatypeProperty ;
        rdfs:comment           "The peak total cooling load for the building, zone or space."@en , "建物、ゾーン、部屋のピーク時の冷房負荷。"@ja-JP , "건물 영역 방 피크 냉방 부하."@ko-KR ;
        rdfs:label             "totalCoolingLoad"@en , "冷房負荷"@ja-JP , "냉방부하"@ko-KR ;
        rdfs:range             <https://w3id.org/product/PowerMeasure> ;
        schema:domainIncludes  <https://w3id.org/product/SpatialElement> .

props:centerCoreTopWidth
        a                      owl:DatatypeProperty ;
        rdfs:comment           "Center core top width of the profile."@en ;
        rdfs:label             "centerCoreTopWidth"@en ;
        rdfs:range             <https://w3id.org/product/PositiveLengthMeasure> ;
        schema:domainIncludes  <https://w3id.org/product/ArbitraryProfileDefWithVoids> .

props:corrosionTreatment
        a                      owl:DatatypeProperty ;
        rdfs:comment           "Determines corrosion treatment for metal components. This property is provided if the requirement needs to be expressed (a) independently of a material specification and (b) as a mere requirements statement rather than a workshop design/ processing feature."@en ;
        rdfs:label             "corrosionTreatment"@en ;
        schema:domainIncludes  <https://w3id.org/product/ElementComponent> .

props:seatingHeight  a         owl:DatatypeProperty ;
        rdfs:comment           "The value of seating height if the chair height is not adjustable."@en ;
        rdfs:label             "seatingHeight"@en ;
        rdfs:range             <https://w3id.org/product/PositiveLengthMeasure> ;
        schema:domainIncludes  <https://w3id.org/product/Furniture%2FCHAIR> .

props:nominalToppingThickness
        a                      owl:DatatypeProperty ;
        rdfs:comment           "The nominal thickness of the topping."@en ;
        rdfs:label             "nominalToppingThickness"@en ;
        rdfs:range             <https://w3id.org/product/PositiveLengthMeasure> ;
        schema:domainIncludes  <https://w3id.org/product/Slab> .

props:s  a                     owl:DatatypeProperty ;
        rdfs:comment           "Measure s according to ISO 2553"@en ;
        rdfs:label             "s"@en ;
        rdfs:range             <https://w3id.org/product/PositiveLengthMeasure> ;
        schema:domainIncludes  <https://w3id.org/product/Fastener%2FWELD> .

props:flangeChamfer  a         owl:DatatypeProperty ;
        rdfs:comment           "Flange chamfer of the profile."@en ;
        rdfs:label             "flangeChamfer"@en ;
        rdfs:range             <https://w3id.org/product/NonNegativeLengthMeasure> ;
        schema:domainIncludes  <https://w3id.org/product/ArbitraryClosedProfileDef> .

props:verticalBarPitch
        a                      owl:DatatypeProperty ;
        rdfs:comment           "The pitch length of the vertical bar."@en , "鉛直方向の補強筋の間隔。"@ja-JP ;
        rdfs:label             "verticalBarPitch"@en , "縦筋ピッチ"@ja-JP ;
        rdfs:range             <https://w3id.org/product/PositiveLengthMeasure> ;
        schema:domainIncludes  <https://w3id.org/product/Wall> .

props:nonRenewableEnergyConsumptionPerUnit
        a                      owl:DatatypeProperty ;
        rdfs:comment           "ISO21930:2007で定義される非再生エネルギーの使用量。"@ja-JP , "Consommation d'énergie non renouvelable telle que définie dans la norme ISO21930:2007 [NDT : et dans la norme NF P01-010]"@fr-FR , "ISO21930 : 2007에 정의된 재생 불가 에너지 사용량"@ko-KR , "Quantity of non-renewable energy used as defined in ISO21930:2007"@en ;
        rdfs:label             "nonRenewableEnergyConsumptionPerUnit"@en , "ConsommationEnergieNonRenouvelableParUnite"@fr-FR , "単位あたり再生不可エネルギ消費"@ja-JP , "단위당 재생 불가 에너지 소비"@ko-KR ;
        rdfs:range             <https://w3id.org/product/EnergyMeasure> ;
        schema:domainIncludes  <https://w3id.org/product/Element> .

props:handicapAccessible
        a                      owl:DatatypeProperty ;
        rdfs:comment           "Angabe, ob dieser Raum (wie z.B. eine Toilette) behindertengerecht zugänglich sein soll (JA) oder nicht (NEIN)."@de-DE , "Indication that this object is designed to be accessible by the handicapped. \nSet to (TRUE) if this stair is rated as handicap accessible  according the local building codes, otherwise (FALSE). Accessibility maybe provided by additional means."@en , "この空間がハンディキャップ者向けの空間かどうかを示す（TRUE）。例：公共トイレの場合。そうでなければ（FALSE）。この情報は、障害者向け利用の必要性や特別なデザインの必要性を示すために利用される。"@ja-JP , "Indique si l'élément est conçu pour être accessible aux handicapés (VRAI) ou non (FAUX). Cette information est souvent utilisée pour déclarer la nécessité d'un accès pour handicapés ou pour des contraintes spéciales de conception."@fr-FR , "이 방 (공간)이 핸디캡을위한 공간 여부를 나타내는 부울 값입니다. 예 : 공공 화장실의 경우 TRUE. 이 정보는 장애인을위한 이용의 필요성과 특별한 디자인의 필요성을 나타내기 위해 사용된다."@ko-KR , "Indication that this object is designed to be accessible by the handicapped. \nIt is giving according to the requirements of the national building code."@en , "Indication that this object is designed to be accessible by the handicapped. \nSet to (TRUE) if this ramp is rated as handicap accessible  according the local building codes, otherwise (FALSE)."@en , "この空間がハンディキャップ者向けの空間かどうかを示すブーリアン値。"@ja-JP , "Indique que cet objet est conçu pour être accessible aux handicapés. Indication donnée selon le Code National."@fr-FR , "この部屋（空間）がハンディキャップ者向けの空間かどうかを示すブーリアン値。例：公共トイレの場合TRUE。この情報は、障害者向け利用の必要性や特別なデザインの必要性を示すために利用される。"@ja-JP , "Indication whether this space (in case of e.g., a toilet) is designed to serve as an accessible space for handicapped people, e.g., for a public toilet (TRUE) or not (FALSE). This information is often used to declare the need for access for the disabled and for special design requirements of this space."@en , "German-description-7"@de-DE , "表示该构件是否设计为可供残疾人使用的无障碍设施。\n该属性的根据为国家建筑规范。"@zh-CN , "Angabe, ob die Tür behindertengerecht gemäß der nationalen oder regionalen Verordnung ist (JA), oder nicht (NEIN)."@de-DE , "공간이 핸디캡을위한 공간 여부를 나타내는 부울 값입니다. 예 : 공공 화장실의 경우 TRUE. 이 정보는 장애인을위한 이용의 필요성과 특별한 디자인의 필요성을 나타내기 위해 사용된다."@ko-KR ;
        rdfs:label             "ハンディキャップアクセス可能性"@ja-JP , "behindertengerecht zugänglich"@de-DE , "AccesHandicapes"@fr-FR , "AccessibleHandicapes"@fr-FR , "핸디캠 액세스 가능성"@ko-KR , "핸디캡 액세스 가능성"@ko-KR , "handicapAccessible"@en , "是否为无障碍设施"@zh-CN , "Behindertengerecht"@de-DE ;
        rdfs:range             xsd:boolean ;
        schema:domainIncludes  <https://w3id.org/product/Space> , <https://w3id.org/product/Zone> , <https://w3id.org/product/Ramp> , <https://w3id.org/product/Door> , <https://w3id.org/product/Stair> .

props:waterInletTemperatureRange
        a                      owl:DatatypeProperty ;
        rdfs:comment           "Allowable water inlet temperature range."@en , "入口水温範囲"@ja-JP , "Plage de température de l'alimentation en eau admissible"@fr-FR ;
        rdfs:label             "waterInletTemperatureRange"@en , "入口水温範囲"@ja-JP , "PlageTempératureAlimentationEau"@fr-FR ;
        schema:domainIncludes  <https://w3id.org/product/Boiler> .

props:columnShoeCasingWidth
        a                      owl:DatatypeProperty ;
        rdfs:comment           "The width of the column shoe casing."@en , "柱脚ケーシングの幅。"@ja-JP , "기둥 다리 케이스의 폭"@ko-KR ;
        rdfs:label             "columnShoeCasingWidth"@en , "ケーシング幅"@ja-JP , "케이스 폭"@ko-KR ;
        rdfs:range             <https://w3id.org/product/PositiveLengthMeasure> ;
        schema:domainIncludes  <https://w3id.org/product/DiscreteAccessory%2FSHOE> .

props:mixerControl  a          owl:DatatypeProperty ;
        rdfs:comment           "Defines the form of control of the mixing valve."@en , "混合弁の制御形式の定義"@ja-JP ;
        rdfs:label             "mixerControl"@en , "混合制御"@ja-JP ;
        schema:domainIncludes  <https://w3id.org/product/Valve%2FMIXING> .

props:maintenanceLevel
        a                      owl:DatatypeProperty ;
        rdfs:comment           "Adjustment of the service life resulting from the effect of the level or degree of maintenance applied to dcomponents."@en ;
        rdfs:label             "maintenanceLevel"@en ;
        schema:domainIncludes  <https://w3id.org/product/System> .

props:crossSectionArea
        a                      owl:DatatypeProperty ;
        rdfs:comment           "Area of the profile. For example measured in mm2. If given, the value of the cross section area shall be greater than zero."@en ;
        rdfs:label             "crossSectionArea"@en ;
        rdfs:range             <https://w3id.org/product/AreaMeasure> ;
        schema:domainIncludes  <https://w3id.org/product/ProfileDef> .

props:frameMaterial  a         owl:DatatypeProperty ;
        rdfs:comment           "Filter frame material."@en , "The material from which the damper frame is constructed."@en ;
        rdfs:label             "frameMaterial"@en ;
        schema:domainIncludes  <https://w3id.org/product/Filter%2FAIRPARTICLEFILTER> , <https://w3id.org/product/Damper> .

props:coreIdentifier  a        owl:DatatypeProperty ;
        rdfs:comment           "The core identification used  Identifiers may be used such as by color (Black, Brown, Grey) or by number (1, 2, 3) or by IEC phase reference (L1, L2, L3) etc."@en , "コアの識別は、色（ブラック、ブラウン、グレー）又は番号（1、2、3）又はIECの位相基準（L1、L2、L3）などを使用。"@ja-JP , "코어 식별 색 (블랙, 브라운, 그레이) 또는 번호 (1,2,3) 또는 IEC의 위상 기준 (L1, L2, L3)를 사용."@ko-KR ;
        rdfs:label             "coreIdentifier"@en , "コア識別子"@ja-JP , "코어 식별자"@ko-KR ;
        rdfs:range             xsd:string ;
        schema:domainIncludes  <https://w3id.org/product/CableSegment%2FCORESEGMENT> .

props:wireLoopBasePlateWidth
        a                      owl:DatatypeProperty ;
        rdfs:comment           "The width of the base plate."@en , "ベースプレートの幅。"@ja-JP , "베이스 플레이트 폭"@ko-KR ;
        rdfs:label             "wireLoopBasePlateWidth"@en , "ベースプレート幅"@ja-JP , "베이스 플레이트 폭"@ko-KR ;
        rdfs:range             <https://w3id.org/product/PositiveLengthMeasure> ;
        schema:domainIncludes  <https://w3id.org/product/DiscreteAccessory%2FWire%20loop> .

props:tunerChannel  a          owl:DatatypeProperty ;
        rdfs:comment           "Indicates the tuner channels, if applicable."@en , "設定可能なチャンネルを示す。"@ja-JP , "가능한 채널을 보여준다."@ko-KR ;
        rdfs:label             "tunerChannel"@en , "チューナーチャンネル"@ja-JP , "튜너 채널 선택"@ko-KR ;
        schema:domainIncludes  <https://w3id.org/product/AudioVisualAppliance%2FTUNER> .

props:isGuarded  a             owl:DatatypeProperty ;
        rdfs:comment           "Indication of whether the motor enclosure is guarded (= TRUE) or not (= FALSE)."@en , "モーターの筐体が守られているかどうかを示す。"@ja-JP , "모터의 케이스가 지켜지고 있는지 여부를 나타낸다."@ko-KR ;
        rdfs:label             "isGuarded"@en , "保護"@ja-JP , "보호"@ko-KR ;
        rdfs:range             xsd:boolean ;
        schema:domainIncludes  <https://w3id.org/product/ElectricMotor> .

props:concreteCoverAtMainBars
        a                      owl:DatatypeProperty ;
        rdfs:comment           "Abstand zwischen der Betonoberfläche und der Außenkante den vom Beton umhüllten Bewehrungshauptstäben."@de-DE , "국가의 건축 기준에 따라 주로 철근을 콘크리트 입고로 보호"@ko-KR , "国の建築基準に従い、主鉄筋をコンクリートの被りで保護する。"@ja-JP , "The protective concrete cover at the main reinforcing bars according to local building regulations."@en ;
        rdfs:label             "Betonüberdeckung Hauptstäbe"@de-DE , "主筋のコンクリート被り"@ja-JP , "concreteCoverAtMainBars"@en , "주근 콘크리트 입고"@ko-KR ;
        rdfs:range             <https://w3id.org/product/PositiveLengthMeasure> ;
        schema:domainIncludes  <https://w3id.org/product/BuildingElement> .

props:primaryFrequency
        a                      owl:DatatypeProperty ;
        rdfs:comment           "The frequency that is going to be transformed and that runs into the transformer on the primary side."@en , "変圧器の1次側に伝送される周波数。"@ja-JP , "변압기 1 차 측에 전송되는 주파수."@ko-KR ;
        rdfs:label             "primaryFrequency"@en , "第１周波数"@ja-JP , "제 1 주파수"@ko-KR ;
        rdfs:range             <https://w3id.org/product/FrequencyMeasure> ;
        schema:domainIncludes  <https://w3id.org/product/Transformer> .

props:plies  a                 owl:DatatypeProperty ;
        rdfs:comment           "Number of plies."@en ;
        rdfs:label             "plies"@en ;
        rdfs:range             xsd:int ;
        schema:domainIncludes  <https://w3id.org/product/Material%2FWood> .

props:unit  a                  owl:DatatypeProperty ;
        rdfs:comment           "Unité de la quantité prise en compte pour la détermination des impacts environnementaux."@fr-FR , "関連する環境指数値の数量単位。"@ja-JP , "환경 지표 값이 연결된 량의 단위"@ko-KR , "The unit of the quantity the environmental indicators values are related with."@en ;
        rdfs:label             "単位"@ja-JP , "unit"@en , "단위"@ko-KR , "Unite"@fr-FR ;
        rdfs:range             xsd:string ;
        schema:domainIncludes  <https://w3id.org/product/Element> .

props:hasHoseUnion  a          owl:DatatypeProperty ;
        rdfs:comment           "排水コックにホースユニオン継手が付いているかの表示．付き\n(= TRUE)無し (= FALSE)"@ja-JP , "Indicates whether the drawoff cock is fitted with a hose union connection (= TRUE) or not (= FALSE)."@en , "排水コックにホースユニオン継手が付いているかの表示．付き(= TRUE)無し (= FALSE)"@ja-JP , "Indicates whether the gas tap is fitted with a hose union connection (= TRUE) or not (= FALSE)."@en ;
        rdfs:label             "ホースユニオン付き"@ja-JP , "hasHoseUnion"@en ;
        rdfs:range             xsd:boolean ;
        schema:domainIncludes  <https://w3id.org/product/Valve%2FGASTAP> , <https://w3id.org/product/Valve%2FDRAWOFFCOCK> .

props:soilConductivity
        a                      owl:DatatypeProperty ;
        rdfs:comment           "Thermal conductivity of soil. Generally, within standards such as IEC 60364-5-52, table 52A-16, the resistivity of soil is required (measured in [SI] units of degK.m /W). This is the reciprocal of the conductivity value and needs to be calculated accordingly."@en ;
        rdfs:label             "soilConductivity"@en ;
        rdfs:range             <https://w3id.org/product/ThermalConductivityMeasure> ;
        schema:domainIncludes  <https://w3id.org/product/CableSegment> .

props:internalWidth  a         owl:DatatypeProperty ;
        rdfs:comment           "The internal width of the culvert."@en , "暗渠管の内幅"@ja-JP ;
        rdfs:label             "internalWidth"@en , "内幅"@ja-JP ;
        rdfs:range             <https://w3id.org/product/LengthMeasure> ;
        schema:domainIncludes  <https://w3id.org/product/PipeSegment%2FCULVERT> .

props:heatExchangeArea
        a                      owl:DatatypeProperty ;
        rdfs:comment           "Heat exchange area."@en , "熱交換面積"@ja-JP ;
        rdfs:label             "heatExchangeArea"@en , "熱交換面積"@ja-JP ;
        rdfs:range             <https://w3id.org/product/AreaMeasure> ;
        schema:domainIncludes  <https://w3id.org/product/EvaporativeCooler> .

props:frictionLoss  a          owl:DatatypeProperty ;
        rdfs:comment           "The pressure loss due to friction per unit length. (Data type = PressureMeasure/LengthMeasure)"@en , "単位長さあたりの圧力損失（計測した圧力損失/ダクト長さ）。"@ja-JP , "단위 길이 당 압력 손실 (측정 압력 손실 / 덕트 길이)."@ko-KR ;
        rdfs:label             "frictionLoss"@en , "摩擦損失"@ja-JP , "마찰 소실"@ko-KR ;
        rdfs:range             xsd:decimal ;
        schema:domainIncludes  <https://w3id.org/product/DistributionSystem%2FVENTILATION> .

props:setPointSound  a         owl:DatatypeProperty ;
        rdfs:comment           "The sound pressure value to be sensed. Use IfcPropertyBoundedValue.SetPointValue to set the set point value."@en , "感知される音圧。\nセットポイント値を置くために、IfcPropertyBoundedValue.SetPointValueを使用する。"@ja-JP , "감지되는 음압. 세트 포인트 값을 넣으려면, IfcPropertyBoundedValue.SetPointValue를 사용하십시오."@ko-KR ;
        rdfs:label             "setPointSound"@en , "音圧設定値"@ja-JP , "읍압 설정치"@ko-KR ;
        schema:domainIncludes  <https://w3id.org/product/Sensor%2FSOUNDSENSOR> .

props:resourceDepletionPerUnit
        a                      owl:DatatypeProperty ;
        rdfs:comment           "Quantity of resources used calculated in equivalent antimony"@en , "안티몬에 해당 환산된 사용 자원 량"@ko-KR , "アンチモンで計算される資源の使用量。"@ja-JP , "Quantité de ressources consommées exprimée en équivalent Antimoine telles que définies dans la norme  ISO21930:2007  [NDT : et dans la norme NF P01-010]"@fr-FR ;
        rdfs:label             "resourceDepletionPerUnit"@en , "단위당 자원소비"@ko-KR , "EpuisementRessourcesParUnite"@fr-FR , "単位あたり資源消費"@ja-JP ;
        rdfs:range             <https://w3id.org/product/MassMeasure> ;
        schema:domainIncludes  <https://w3id.org/product/Element> .

props:flushType  a             owl:DatatypeProperty ;
        rdfs:comment           "The property enumeration Pset_FlushTypeEnum defines the types of flushing mechanism that may be specified for cisterns and sanitary terminals where:-\n\nLever: \tFlushing is achieved by twisting a lever that causes a predetermined flow of water to be passed from a cistern to the sanitary terminal.\nPull: \tFlushing is achieved by pulling a handle or knob vertically upwards that causes a predetermined flow of water to be passed from a cistern to the sanitary terminal.\nPush: \tFlushing is achieved by pushing a button or plate that causes a predetermined flow of water to be passed from a cistern to the sanitary terminal.\nSensor: Flush is activated through an automatic sensing mechanism."@en , "列挙するプロパティはPset_FlushTypeEnumでは貯水槽や衛生配管の配置による、フラッシュメカニズムのタイプを定義する：\n\nレバー式：洗浄水は、レバーをねじることによって貯水タンクから衛生配管にの所定の流量を流す。\n\n引っ張り式：洗浄水は、ハンドルまたはノブを垂直方向に引くことによって貯水タンクから衛生配管にの所定の流量を流す。\n\n押しボタン式：洗浄水は、ボタンかプレートを押すことによって貯水タンクから衛生配管にの所定の流量を流す。\n\nセンサー式：洗浄水は、自動検出機構を介して作動する。"@ja-JP ;
        rdfs:label             "flushType"@en , "タイプフラッシュ"@ja-JP ;
        schema:domainIncludes  <https://w3id.org/product/SanitaryTerminal%2FCISTERN> .

props:pressureLossCoefficient
        a                      owl:DatatypeProperty ;
        rdfs:comment           "Pressure loss coefficient."@en ;
        rdfs:label             "pressureLossCoefficient"@en ;
        schema:domainIncludes  <https://w3id.org/product/Damper> .

props:color  a                 owl:DatatypeProperty ;
        rdfs:comment           "Color of the urinal."@en , "Color of the object."@en , "Color selection for this object."@en , "Principal color of the object."@en , "The color of the duct segment.\n\nNote: This is typically used for any duct segments with a painted surface which is not otherwise specified as a covering."@en , "配管部の内部粗度係数　記：この語はプラスチック配管にのみ使われる。しかしながら、保護のためではない塗装された表面を持つ配管にも使われる。"@ja-JP , "ダクト継手の色\nメモ：塗装されているときに使用される。他の場合は仕上げとして定義"@ja-JP , "主要な色。"@ja-JP , "要素の色。"@ja-JP , "The color of the pipe segment.\n\nNote: This is typically used only for plastic pipe segments. However, it may be used for any pipe segments with a painted surface which is not otherwise specified as a covering."@en , "Color selection for this object"@en , "配管部の内部粗度係数　記：プラスチック配管にのみ使われる。保護のためではない塗装された表面を持つ配管にも使われる。"@ja-JP ;
        rdfs:label             "color"@en , "色"@ja-JP ;
        rdfs:range             xsd:string ;
        schema:domainIncludes  <https://w3id.org/product/DuctSegment> , <https://w3id.org/product/DuctFitting> , <https://w3id.org/product/PipeSegment> , <https://w3id.org/product/SanitaryTerminal%2FSHOWER> , <https://w3id.org/product/PipeFitting> , <https://w3id.org/product/SanitaryTerminal%2FSINK> , <https://w3id.org/product/SanitaryTerminal%2FSANITARYFOUNTAIN> , <https://w3id.org/product/SanitaryTerminal%2FURINAL> , <https://w3id.org/product/SanitaryTerminal%2FWASHHANDBASIN> , <https://w3id.org/product/SanitaryTerminal%2FTOILETPAN> , <https://w3id.org/product/SanitaryTerminal%2FBATH> , <https://w3id.org/product/SanitaryTerminal%2FBIDET> .

props:flushingRate  a          owl:DatatypeProperty ;
        rdfs:comment           "The predetermined quantity of water to be flushed."@en , "予め決められた流される水量"@ja-JP ;
        rdfs:label             "flushingRate"@en , "フラッシュ率"@ja-JP ;
        rdfs:range             <https://w3id.org/product/VolumetricFlowRateMeasure> ;
        schema:domainIncludes  <https://w3id.org/product/Valve%2FFLUSHING> .

props:sensibleLoadToRadiant
        a                      owl:DatatypeProperty ;
        rdfs:comment           "Percent of sensible thermal load to radiant heat."@en ;
        rdfs:label             "sensibleLoadToRadiant"@en ;
        rdfs:range             <https://w3id.org/product/PositiveRatioMeasure> ;
        schema:domainIncludes  <https://w3id.org/product/LightFixture> .

props:tileLength  a            owl:DatatypeProperty ;
        rdfs:comment           "天花板面砖的长度。\n该属性所提供的尺寸信息是对内部形状描述和几何参数的补充。如果几何参数与该属性所提供的尺寸属性不符，应以几何参数为准。"@zh-CN , "Length of ceiling tiles. The size information is provided in addition to the shape representation and the geometric parameters used within. In cases of inconsistency between the geometric parameters and the size properties, provided in the attached property set, the geometric parameters take precedence."@en , "Longueur des carreaux de plafond. Cette propriété est donnée en complément de la représentation de la forme et des paramètres géométriques qui la déterminent. En cas d'incohérence entre ces paramètres géométriques et cette propriété, ce sont les paramètres géométriques qui priment."@fr-FR , "Länge der Unterdeckenplatten, oder -panele, die zur Verkleidung verwendet werden."@de-DE ;
        rdfs:label             "Deckenplattenlänge"@de-DE , "面砖长度"@zh-CN , "Longueur des carreaux"@fr-FR , "tileLength"@en ;
        rdfs:range             <https://w3id.org/product/PositiveLengthMeasure> ;
        schema:domainIncludes  <https://w3id.org/product/Covering%2FCEILING> .

props:nominalSumpLength
        a                      owl:DatatypeProperty ;
        rdfs:comment           "Nominal or quoted length measured along the x-axis in the local coordinate system or the radius (in the case of a circular shape in plan) of the sump."@en , "局所座標系のX軸に沿うか半径（円状の形の場合）で測定された、汚水槽の長さ。"@ja-JP ;
        rdfs:label             "nominalSumpLength"@en , "汚水槽長さ"@ja-JP ;
        rdfs:range             <https://w3id.org/product/PositiveLengthMeasure> ;
        schema:domainIncludes  <https://w3id.org/product/WasteTerminal%2FGULLYSUMP> .

props:roughness  a             owl:DatatypeProperty ;
        rdfs:comment           "Une mesure des déviations verticales de la surface."@fr-FR , "表面の垂直方向の偏差。"@ja-JP , "A measure of the vertical deviations of the surface."@en ;
        rdfs:label             "Rugosité"@fr-FR , "roughness"@en , "Rauheit der Oberfläche"@de-DE , "表面粗さ"@ja-JP ;
        rdfs:range             xsd:string ;
        schema:domainIncludes  <https://w3id.org/product/ShadingDevice> .

props:speakerDriverSize
        a                      owl:DatatypeProperty ;
        rdfs:comment           "Indicates the number of drivers and their sizes."@en , "ドライバユニットと数を示す。"@ja-JP , "드라이버 유닛과 수를 나타낸다"@ko-KR ;
        rdfs:label             "speakerDriverSize"@en , "スピーカードライバサイズ"@ja-JP , "스피커 드라이버"@ko-KR ;
        schema:domainIncludes  <https://w3id.org/product/AudioVisualAppliance%2FSPEAKER> .

props:airSideSystemType
        a                      owl:DatatypeProperty ;
        rdfs:comment           "This enumeration specifies the basic types of possible air side systems (e.g., Constant Volume, Variable Volume, etc.)."@en ;
        rdfs:label             "airSideSystemType"@en ;
        schema:domainIncludes  <https://w3id.org/product/Space> , <https://w3id.org/product/Zone> , <https://w3id.org/product/SpatialZone> .

props:workExecutionLevel
        a                      owl:DatatypeProperty ;
        rdfs:comment           "Adjustment of the service life resulting from the effect of the quality of work executed."@en ;
        rdfs:label             "workExecutionLevel"@en ;
        schema:domainIncludes  <https://w3id.org/product/System> .

props:actuatorInputPower
        a                      owl:DatatypeProperty ;
        rdfs:comment           "Maximum input power requirement."@en , "最大入力電力。"@ja-JP , "최대 입력 전력"@ko-KR ;
        rdfs:label             "actuatorInputPower"@en , "入力電力"@ja-JP , "입력 전력"@ko-KR ;
        rdfs:range             <https://w3id.org/product/PowerMeasure> ;
        schema:domainIncludes  <https://w3id.org/product/Actuator%2FELECTRICACTUATOR> .

props:saturationEfficiencyCurve
        a                      owl:DatatypeProperty ;
        rdfs:comment           "Saturation efficiency as a function of the air flow rate."@en ;
        rdfs:label             "saturationEfficiencyCurve"@en ;
        schema:domainIncludes  <https://w3id.org/product/Humidifier> .

props:zoom  a                  owl:DatatypeProperty ;
        rdfs:comment           "Indicates the zoom range."@en , "ズーム可能範囲（倍率）を示す。"@ja-JP ;
        rdfs:label             "zoom"@en , "ズーム"@ja-JP ;
        schema:domainIncludes  <https://w3id.org/product/AudioVisualAppliance%2FCAMERA> .

props:specialRequirements
        a                      owl:DatatypeProperty ;
        rdfs:comment           "Any additional special requirements that need to be included in the permit to work.\n\nNOTE - Additional permit requirements may be imposed according to the nature of the facility at which the work is carried out. For instance, in clean areas, special clothing may be required whilst in corrective institutions, it may be necessary to check in and check out tools that will be used for work as a safety precaution."@en ;
        rdfs:label             "specialRequirements"@en ;
        rdfs:range             xsd:string ;
        schema:domainIncludes  <https://w3id.org/product/Permit> .

props:pressureDropCurve
        a                      owl:DatatypeProperty ;
        rdfs:comment           "Under certain dust holding weight, DelPressure = f (fluidflowRate)"@en ;
        rdfs:label             "pressureDropCurve"@en ;
        schema:domainIncludes  <https://w3id.org/product/Filter%2FAIRPARTICLEFILTER> .

props:panMounting  a           owl:DatatypeProperty ;
        rdfs:comment           "The property enumeration Pset_SanitaryMountingEnum defines the forms of mounting or fixing of the sanitary terminal that may be specified within property sets used to define sanitary terminals (WC’s, basins, sinks, etc.) where:-\n\nBackToWall: \tA pedestal mounted sanitary terminal that fits flush to the wall at the rear to cover its service connections.\nPedestal: \tA floor mounted sanitary terminal that has an integral base.\nCounterTop: \tA sanitary terminal that is installed into a horizontal surface that is installed into a horizontal surface. Note: When applied to a wash hand basin, the term more normally used is ‘vanity’. See also Wash Hand Basin Type specification.\nWallHung: \tA sanitary terminal cantilevered clear of the floor."@en , "Pset_SanitaryMountingEnumは固定された衛生器具の接続点（トイレや洗面器、シンクなど）に取り付けられます。\n\n・床置き壁排出：背面の壁に接続口を合わせること。\n・台：床置きの衛生器具には基礎があること。\n・カウンター：衛生器具の表層が水平に設置されていること。※手洗い台として設置された場合「化粧台」として扱うこと。また、洗面台種類の規格表を参照のこと。\n・壁掛け型：衛生器具は片側固定がされ床から離れていること。"@ja-JP ;
        rdfs:label             "panMounting"@en , "取付方法"@ja-JP ;
        schema:domainIncludes  <https://w3id.org/product/SanitaryTerminal%2FTOILETPAN> .

props:shortCircuit1PolePowerFactorMinimumState
        a                      owl:DatatypeProperty ;
        rdfs:comment           "Power factor of the minimum 1 pole short circuit current provided at the point of supply i.e. the fault between 1 phase and N."@en , "電源供給時点の点1相とN間の1極最小短絡電流力率。"@ja-JP , "전원 공급 시점 점 1 단계와 N 사이의 1 극 최소 단락 전류 역률."@ko-KR ;
        rdfs:label             "shortCircuit1PolePowerFactorMinimumState"@en , "1極最小短絡電流力率"@ja-JP , "1 극 최소 단락 전류 역률"@ko-KR ;
        rdfs:range             xsd:decimal ;
        schema:domainIncludes  <https://w3id.org/product/ElectricFlowStorageDevice> .

props:wallThickness  a         owl:DatatypeProperty ;
        rdfs:comment           "ダクトスペース壁の厚さ。\n注：ダクトスペースの壁は単層と仮定する"@ja-JP , "The thickness of the chamber wall construction\nNOTE: It is assumed that chamber walls will be constructed at a single thickness."@en , "The thickness of the chamber wall construction\n.\nNOTE: It is assumed that chamber walls will be constructed at a single thickness."@en , "The thickness of the chamber wall construction.\nNOTE: It is assumed that chamber walls will be constructed at a single thickness."@en , "The thickness of the duct wall construction\nNOTE: It is assumed that chamber walls will be constructed at a single thickness."@en , "덕트 공간 벽 두께 참고 : 덕트 공간의 벽은 단층 가정"@ko-KR ;
        rdfs:label             "wallThickness"@en , "벽 두께"@ko-KR , "壁厚さ"@ja-JP , "壁の厚さ"@ja-JP ;
        rdfs:range             <https://w3id.org/product/PositiveLengthMeasure> ;
        schema:domainIncludes  <https://w3id.org/product/DistributionChamberElement%2FMANHOLE> , <https://w3id.org/product/DistributionChamberElement%2FINSPECTIONCHAMBER> , <https://w3id.org/product/DistributionChamberElement%2FMETERCHAMBER> , <https://w3id.org/product/DistributionChamberElement%2FFORMEDDUCT> , <https://w3id.org/product/DistributionChamberElement%2FVALVECHAMBER> .

props:roll  a                  owl:DatatypeProperty ;
        rdfs:comment           "柱の長軸に対する回転。"@ja-JP , "Drehwinkel der Stütze relative zur globalen X Ausrichtung (O Grad). Bei nicht-vertikalen Stützen wird die Verdrehung analog zu den Balken (Verkippung gegen die Vertikale) angegeben.\n\nDieser Parameter wird zusätzlich zur geometrischen Repräsentation bereitgestellt. Im Fall der Inkonsistenz zwischen dem Parameter und der Geometrie hat die geometrische Repräsention Priorität. Dieser Parameter ist für CAD Software write-only."@de-DE , "Kippwinkel des Balkens relative zur Vertikalen (O Grad).\n\nDieser Parameter wird zusätzlich zur geometrischen Repräsentation bereitgestellt. Im Fall der Inkonsistenz zwischen dem Parameter und der Geometrie hat die geometrische Repräsention Priorität. Dieser Parameter ist für CAD Software write-only."@de-DE , "相对于纵轴的旋转角。对全局坐标系中的非垂直构件，该属性为相对于Z轴的角度。（若轮廓方向在Z轴上，则转角为0。）\n该属性所提供的形状信息是对内部形状描述和几何参数的补充。如果几何参数与该属性所提供的形状属性不符，应以几何参数为准。对CAD等几何编辑程序，该属性应为只写类型。\n注：IFC2x4新添属性"@zh-CN , "相对于纵轴的旋转角。对全局坐标系中的垂直柱，该属性为相对于X轴的角度。（若轮廓方向在X轴上，则转角为0。）对全局坐标系中的非垂直柱，该属性为相对于Z轴的角度。（若轮廓方向在Z轴上，则转角为0。）\n该属性所提供的形状信息是对内部形状描述和几何参数的补充。如果几何参数与该属性所提供的形状属性不符，应以几何参数为准。对CAD等几何编辑程序，该属性应为只写类型。\n注：IFC2x4新添属性"@zh-CN , "Rotation autour de l'axe longitudinal - relativement à l'axe Z pour toutes les poutres qui ne sont pas verticales relativement au repère absolu (la direction du profil est celle de l'axe Z si la valeur de la propriété est 0). Cette propriété est donnée en complément de la représentation de la forme de l'élément et des paramètres géométriques qui la déterminent. En cas d'incohérence entre ces paramètres géométriques et cette propriété, ce sont les paramètres géométriques qui priment. Les applications qui déterminent la géométrie comme les logiciels de CAO ne doivent pas autoriser la modification de cette propriété. Note : nouvelle propriété de la version IFC2x4."@fr-FR , "Rotation against the longitudinal axis - relative to the global Z direction for all members that are non-vertical in regard to the global coordinate system (Profile direction equals global Z is Roll = 0.)\nThe shape information is provided in addition to the shape representation and the geometric parameters used within. In cases of inconsistency between the geometric parameters and the shape properties, provided in the attached property, the geometric parameters take precedence.\nNote: new property in IFC4."@en , "Rotation against the longitudinal axis - relative to the global Z direction for all beams that are non-vertical in regard to the global coordinate system (Profile direction equals global Z is Roll = 0.)\n\nThe shape information is provided in addition to the shape representation and the geometric parameters used within. In cases of inconsistency between the geometric parameters and the shape properties, provided in the attached property, the geometric parameters take precedence.  For geometry editing applications, like CAD: this value should be write-only.\n\nNote: new property in IFC4"@en , "梁の材軸に対する回転。\n-この材軸はグローバル座標系で非垂直な全ての梁に対してグローバルZ方向へ相対する。（表示方向は、グローバルZの回転方向を0とする。）\n\nその形状（梁の回転）情報は、表示のための形状に内部で使用される幾何学的パラメータを加えて提供される。形状情報と内部の幾何学的パラメータに矛盾が生じた場合は、幾何学的パラメータが優先される。幾何学的パラメ－タ編集アプリケーションでは、CADと同様に、この値は書き込み専用とする。\n\n注：IFC2x4の新しいプロパティ"@ja-JP , "Rotation against the longitudinal axis - relative to the global  X direction for all columns that are vertical in regard to the global coordinate system (Profile direction equals global X is Roll = 0.). For all non-vertical columns the following applies:  Roll is relative to the global Z direction f(Profile direction of non-vertical columns that equals global Z is Roll = 0.)\n\nThe shape information is provided in addition to the shape representation and the geometric parameters used within. In cases of inconsistency between the geometric parameters and the shape properties, provided in the attached property, the geometric parameters take precedence.  For geometry editing applications, like CAD: this value should be write-only.\n\nNote: new property in IFC4"@en , "オブジェクトの長軸に対する回転。"@ja-JP , "Rotation autour de l'axe longitudinal - relativement à l'axe X pour tous les poteaux qui sont verticaux relativement au repère absolu (la direction du profil est celle de l'axe X si la valeur est 0). Pour tous les poteaux non verticaux, la valeur de la propriété est relative à l'axe Z (la direction du profil des poteaux non verticaux est celle de l'axe Z si la valeur est 0). \nCette propriété est donnée en complément de la représentation de la forme de l'élément et des paramètres géométriques qui la déterminent. En cas d'incohérence entre ces paramètres géométriques et cette propriété, ce sont les paramètres géométriques qui priment. Les applications qui déterminent la géométrie comme les logiciels de CAO ne doivent pas autoriser la modification de cette propriété. Note : nouvelle propriété de la version IFC2x4."@fr-FR , "German-description-4"@de-DE , "相对于纵轴的旋转角。对全局坐标系中的非垂直梁，该属性为相对于Z轴的角度。（若轮廓方向在Z轴上，则转角为0。）\n该属性所提供的形状信息是对内部形状描述和几何参数的补充。如果几何参数与该属性所提供的形状属性不符，应以几何参数为准。对CAD等几何编辑程序，该属性应为只写类型。\n注：IFC2x4新添属性"@zh-CN , "Rotation autour de l'axe longitudinal - relativement à l'axe Z pour toutes les membrures qui ne sont pas verticales relativement au repère absolu (la direction du profil est celle de l'axe Z si la valeur de la propriété est 0). Cette propriété est donnée en complément de la représentation de la forme de l'élément et des paramètres géométriques qui la déterminent. En cas d'incohérence entre ces paramètres géométriques et cette propriété, ce sont les paramètres géométriques qui priment. Note : nouvelle propriété de la version IFC2x4."@fr-FR ;
        rdfs:label             "Kippwinkel"@de-DE , "回転"@ja-JP , "Drehwinkel"@de-DE , "转角"@zh-CN , "RotationAutourAxeLongitudinal"@fr-FR , "roll"@en ;
        rdfs:range             <https://w3id.org/product/PlaneAngleMeasure> ;
        schema:domainIncludes  <https://w3id.org/product/Column> , <https://w3id.org/product/Member> , <https://w3id.org/product/Beam> .

props:maximumSpaceSensibleLoad
        a                      owl:DatatypeProperty ;
        rdfs:comment           "Maximum or Peak sensible thermal load contributed to return air plenum by the light fixture."@en ;
        rdfs:label             "maximumSpaceSensibleLoad"@en ;
        rdfs:range             <https://w3id.org/product/PowerMeasure> ;
        schema:domainIncludes  <https://w3id.org/product/LightFixture> .

props:shortInsideCenterLowerBarPitch
        a                      owl:DatatypeProperty ;
        rdfs:comment           "The pitch length of the short inside center lower bar."@en , "短辺方向・柱間帯・下端中央の鉄筋間隔。"@ja-JP ;
        rdfs:label             "shortInsideCenterLowerBarPitch"@en , "短辺・柱列帯・下端中央ピッチ"@ja-JP ;
        rdfs:range             <https://w3id.org/product/PositiveLengthMeasure> ;
        schema:domainIncludes  <https://w3id.org/product/Slab> .

props:stemBaseFillet  a        owl:DatatypeProperty ;
        rdfs:comment           "Stem base fillet of the profile."@en ;
        rdfs:label             "stemBaseFillet"@en ;
        rdfs:range             <https://w3id.org/product/NonNegativeLengthMeasure> ;
        schema:domainIncludes  <https://w3id.org/product/ArbitraryClosedProfileDef> .

props:i4  a                    owl:DatatypeProperty ;
        rdfs:comment           "The lower electromagnetic testing current limit in [x In], indicating that for currents lower than I4, the tripping time shall be longer than the associated tripping time, T5, i.e. the device shall not trip instantaneous."@en , "電磁の低試験電流限界値を [x In], 電流は I4 よりも低い値を示す。トリップ時間は関連する T5 と瞬時に遮断する定格使用電流の時間よりも長い。"@ja-JP , "전자 낮은 시험 전류 한계를 [x In] 전류는 I4보다 낮은 값을 나타낸다. 트립 시간은 관련 T5 즉석에서 차단하는 정격 사용 전류의 시간보다 길다."@ko-KR ;
        rdfs:label             "i4"@en , "I4"@ja-JP , "I4"@ko-KR ;
        rdfs:range             xsd:decimal ;
        schema:domainIncludes  <https://w3id.org/product/ProtectiveDeviceTrippingUnit%2FELECTROMAGNETIC> .

props:condensingTemperature
        a                      owl:DatatypeProperty ;
        rdfs:comment           "Refrigerant condensing temperature."@en ;
        rdfs:label             "condensingTemperature"@en ;
        schema:domainIncludes  <https://w3id.org/product/Condenser> .

props:occupancyNumberPeak
        a                      owl:DatatypeProperty ;
        rdfs:comment           "この空間に割り当てられた活動を遂行するために必要な最大人数。"@ja-JP , "Nombre maximum d'occupants simultanés concernés par l'activité dans cet espace à l'heure de pointe."@fr-FR , "Maximal number of people required for the activity assigned to this space in peak time."@en , "Maximale Anzahl der Personen für deren  Aktivitäten der Raum vorgesehen ist."@de-DE ;
        rdfs:label             "利用人数ピーク"@ja-JP , "Maximale Belegung"@de-DE , "NombreOccupantsMax"@fr-FR , "occupancyNumberPeak"@en ;
        rdfs:range             <https://w3id.org/product/CountMeasure> ;
        schema:domainIncludes  <https://w3id.org/product/cZone> , <https://w3id.org/product/Space> , <https://w3id.org/product/cSpatialZone> .

props:n  a                     owl:DatatypeProperty ;
        rdfs:comment           "Count n according to ISO 2553"@en ;
        rdfs:label             "n"@en ;
        rdfs:range             <https://w3id.org/product/CountMeasure> ;
        schema:domainIncludes  <https://w3id.org/product/Fastener%2FWELD> .

props:accuracyQualityExpected
        a                      owl:DatatypeProperty ;
        rdfs:comment           "A measure of the accuracy quality of survey points as expected expressed in percentage terms."@en , "Mesure de la précision attendue des points de relevé, exprimée en pourcentage."@fr-FR ;
        rdfs:label             "accuracyQualityExpected"@en , "PrecisionAttendue"@fr-FR ;
        rdfs:range             <https://w3id.org/product/RatioMeasure> ;
        schema:domainIncludes  <https://w3id.org/product/Annotation%2FSurveyArea> .

props:relaxations  a           owl:DatatypeProperty ;
        rdfs:comment           "Measures of decrease in stress over long time intervals resulting from plastic flow. Different relaxation values for different initial stress levels for a material may be given. It describes the time dependent relative relaxation value for a given initial stress level at constant strain.\nRelating values are the \"RelaxationValue\". Related values are the \"InitialStress\""@en ;
        rdfs:label             "relaxations"@en ;
        schema:domainIncludes  <https://w3id.org/product/Material%2FSteel> .

props:capacityCurve  a         owl:DatatypeProperty ;
        rdfs:comment           "Chiller cooling capacity is a function of condensing temperature and evaporating temperature, data is in table form, Capacity = f (TempCon, TempEvp), capacity = a1+b1*Tei+c1*Tei^2+d1*Tci+e1*Tci^2+f1*Tei*Tci. \nThis table uses multiple input variables; to represent, both DefiningValues and DefinedValues lists are null and IfcTable is attached using IfcPropertyConstraintRelationship and IfcMetric.  Columns are specified in the following order: \n1.IfcPowerMeasure:Capacity\n2.IfcThermodynamicTemperatureMeasure:CondensingTemperature\n3.IfcThermodynamicTemperatureMeasure:EvaporatingTemperature"@en , "Puissance frigoifique du groupe froid qui est une fonction de la température de condensation et de la température d'évaporation, les informations sont sous la forme d'un tableau, Puissance = f(TempCon,TempEvp), puissance = a1+b1*Tei+c1*Tei^2+d1*Tci+e1*Tci^2+f1*Tei*Tci.\nCe tableau utilises plusieurs entrées variables; pour la  représenter, DefiningValues et DefinedValues sont pour les deux nulles et IfcTable est attachée en utilisant IfcPropertyConstraintRelationship et IfcMetric. Les colonnes sont indiquées dans l'ordre suivant:\n1. IfcPowerMeasure: Capacity\n2. IfcThermodynamicTemperatureMeasure: CondensingTemperature\n3. IfcThermodynamicTemperatureMeasure: EvaporatingTemperature"@fr-FR ;
        rdfs:label             "capacityCurve"@en , "CourbePuissance"@fr-FR ;
        schema:domainIncludes  <https://w3id.org/product/Chiller> .

props:location  a              owl:DatatypeProperty ;
        rdfs:comment           "Location  (a single type of diffuser can be used for multiple locations); high means close to ceiling."@en , "制気口の取り付け位置（壁面高所・低部、天井ぺり、天井中央、床、床下他）"@ja-JP , "Emplacement (un seul type de diffuseur peut être utilisé pour des emplaments multiples); Haut signifie proche du plafond."@fr-FR ;
        rdfs:label             "location"@en , "位置"@ja-JP , "Emplacement"@fr-FR ;
        schema:domainIncludes  <https://w3id.org/product/AirTerminal> .

props:cornerFixingPlateLength
        a                      owl:DatatypeProperty ;
        rdfs:comment           "The length of the L-shaped corner plate."@en , "L型コーナープレートの長さ。"@ja-JP , "L 형 코너 플레이트의 길이"@ko-KR ;
        rdfs:label             "cornerFixingPlateLength"@en , "長さ"@ja-JP , "길이"@ko-KR ;
        rdfs:range             <https://w3id.org/product/PositiveLengthMeasure> ;
        schema:domainIncludes  <https://w3id.org/product/DiscreteAccessory%2FCorner%20fixing%20plate> .

props:isOutdoors  a            owl:DatatypeProperty ;
        rdfs:comment           "Indicates if camera is designed to be used outdoors."@en , "屋外利用が可能かどうかを示す。"@ja-JP , "옥외 이용이 가능한지 여부를 나타냅니다."@ko-KR ;
        rdfs:label             "isOutdoors"@en , "屋外対応の可否"@ja-JP , "실외 여부"@ko-KR ;
        rdfs:range             xsd:boolean ;
        schema:domainIncludes  <https://w3id.org/product/AudioVisualAppliance%2FCAMERA> .

props:displayWidth  a          owl:DatatypeProperty ;
        rdfs:comment           "Indicates the physical width of the screen (only the display surface)."@en , "画面の幅を示す。"@ja-JP , "화면 너비를 보여준다"@ko-KR ;
        rdfs:label             "displayWidth"@en , "画面幅"@ja-JP , "화면 폭"@ko-KR ;
        rdfs:range             <https://w3id.org/product/PositiveLengthMeasure> ;
        schema:domainIncludes  <https://w3id.org/product/AudioVisualAppliance%2FDISPLAY> .

props:curveDesignation
        a                      owl:DatatypeProperty ;
        rdfs:comment           "제조 업체가 제공하는 지정된 토릿삔구 곡선. MCB 위해, 지정은 IEC 60898을 준수해야한다."@ko-KR , "The designation of the trippingcurve given by the manufacturer. For a MCB the designation should be in accordance with the designations given in IEC 60898."@en , "メーカーが提供する指定のトリッピングカーブ。MCBのために、指定はIEC 60898に準拠しなければならない。"@ja-JP ;
        rdfs:label             "곡성 지정"@ko-KR , "curveDesignation"@en , "곡선 지정"@ko-KR , "曲線指定"@ja-JP ;
        rdfs:range             xsd:string ;
        schema:domainIncludes  <https://w3id.org/product/ProtectiveDeviceTrippingUnit%2FELECTROMAGNETIC> , <https://w3id.org/product/ProtectiveDeviceTrippingUnit%2FTHERMAL> .

props:stemTopFillet  a         owl:DatatypeProperty ;
        rdfs:comment           "Stem top fillet of the profile."@en ;
        rdfs:label             "stemTopFillet"@en ;
        rdfs:range             <https://w3id.org/product/NonNegativeLengthMeasure> ;
        schema:domainIncludes  <https://w3id.org/product/ArbitraryClosedProfileDef> .

props:mountingType  a          owl:DatatypeProperty ;
        rdfs:comment           "La façon d'être fixé pour le terminal de ventilation au plafond, mur, etc.\n\nSurface: Fixé sur la surface de quelque chose (Ex: mur, conduit, etc.)\nAlignement plat: Fixé plat et dans l'alignement d'une surface.\nInsertion: Fixé dans un type de plafond avec capacité d'insertion (Ex: faux-plafondsuspendu)"@fr-FR , "The way the air terminal is mounted to the ceiling, wall, etc.\n\nSurface: mounted to the surface of something (e.g., wall, duct, etc.).\nFlat flush: mounted flat and flush with a surface.\nLay-in: mounted in a lay-in type ceiling (e.g., a dropped ceiling grid)."@en , "지얀 섹션 보트 상자 설치 방법."@ko-KR , "Method of mounting to be adopted for the type of junction box."@en , "ターミナルが天井や壁などに取り付けられる方法。\n表面、水平、LAYIN他\n表面：何か（壁・ダクト等）の表面に取り付け\nFLATFLUSH：表面に水平・Flushni取り付け\nLAYIN：天井にlay-in形式での取り付け（下がり天井格子など）"@ja-JP , "ジヤンクションボツクスの取り付け方法。"@ja-JP ;
        rdfs:label             "mountingType"@en , "설치"@ko-KR , "取り付け"@ja-JP , "取り付け形式"@ja-JP , "ModeFixation"@fr-FR ;
        schema:domainIncludes  <https://w3id.org/product/JunctionBox> , <https://w3id.org/product/AirTerminal> .

props:fractionRadiantHeatTransfer
        a                      owl:DatatypeProperty ;
        rdfs:comment           "Fraction of the total heat transfer rate as the radiant heat transfer."@en , "総合熱移動の内放射熱移動とみなされる部分"@ja-JP ;
        rdfs:label             "fractionRadiantHeatTransfer"@en , "放射熱移動フラクション"@ja-JP ;
        schema:domainIncludes  <https://w3id.org/product/SpaceHeater> .

props:humidityEffectiveness
        a                      owl:DatatypeProperty ;
        rdfs:comment           "Humidity heat transfer effectiveness: The ratio of primary airflow absolute humidity changes to maximum possible absolute humidity changes."@en , "湿度熱交換効率：\n最大可能絶対湿度変化に対する一次側絶対湿度変化の比"@ja-JP , "Efficacité sur transfert de chaleur latente: rapport entre difference de températures"@fr-FR ;
        rdfs:label             "humidityEffectiveness"@en , "湿度効率"@ja-JP , "EfficacitéLatente"@fr-FR ;
        schema:domainIncludes  <https://w3id.org/product/AirToAirHeatRecovery> .

props:nominalWeightedEfficiency
        a                      owl:DatatypeProperty ;
        rdfs:comment           "Nominal filter efficiency based the particle weight concentration before and after the filter against particles with a certain size distribution."@en ;
        rdfs:label             "nominalWeightedEfficiency"@en ;
        rdfs:range             xsd:decimal ;
        schema:domainIncludes  <https://w3id.org/product/Filter%2FAIRPARTICLEFILTER> .

props:sectionLength  a         owl:DatatypeProperty ;
        rdfs:comment           "The length of a section used in the construction of the tank."@en , "タンクの製作に使用されているセクションの長さ"@ja-JP ;
        rdfs:label             "sectionLength"@en , "セクションの長さ"@ja-JP ;
        rdfs:range             <https://w3id.org/product/PositiveLengthMeasure> ;
        schema:domainIncludes  <https://w3id.org/product/Tank%2FSECTIONAL> .

props:recirculatedAir
        a                      owl:DatatypeProperty ;
        rdfs:comment           "Loads from recirculated air."@en , "循環空気による熱負荷。"@ja-JP , "순환공기에 의한 열부하"@ko-KR ;
        rdfs:label             "recirculatedAir"@en , "循環空気"@ja-JP , "순환공기"@ko-KR ;
        schema:domainIncludes  <https://w3id.org/product/Space> .

props:furniturePanelType
        a                      owl:DatatypeProperty ;
        rdfs:comment           "Available panel types from which that required may be selected."@en ;
        rdfs:label             "furniturePanelType"@en ;
        schema:domainIncludes  <https://w3id.org/product/SystemFurnitureElement%2FPANEL> .

props:fireRating  a            owl:DatatypeProperty ;
        rdfs:comment           "Fire rating for the element.\nIt is given according to the national fire safety classification."@en , "主要な耐火等級。関連する建築基準法、消防法などの国家基準を参照。"@ja-JP , "Classement au feu de l'élément donné selon la classification nationale de sécurité incendie."@fr-FR , "Feuerwiderstandsklasse für den Brandschutz gemäß der nationalen oder regionalen Richtlinie die für den Brandschutz der Brandschutztür gewährleistet werden muss."@de-DE , "Feuerwiderstandsklasse gemäß der nationalen oder regionalen Brandschutzverordnung."@de-DE , "Fire rating for this object. It is given according to the national fire safety code or regulation."@en , "当該オブジェクトの耐火等級。国で定めた耐火安全等級分類による。"@ja-JP , "耐火等級。当該国の建築法規による。"@ja-JP , "Fire rating for the element. It is given according to the national fire safety classification."@en , "Feuerwiderstandasklasse gemäß der nationalen oder regionalen Brandschutzverordnung."@de-DE , "Fire rating for this object.\nIt is given according to the national fire safety classification."@en , "Fire rating given according to the national fire safety classification."@en , "Fire rating for this object. It is given according to the national fire safety classification."@en , "主要な耐火等級。関連する建築基準法、消防法などの国家基準によって指定される。"@ja-JP , "该构件的防火等级。\n该属性的依据为国家防火安全分级。"@zh-CN ;
        rdfs:label             "ResistanceAuFeu"@fr-FR , "Résistance au feu"@fr-FR , "防火等级"@zh-CN , "fireRating"@en , "Feuerwiderstandsklasse"@de-DE , "耐火等級"@ja-JP ;
        rdfs:range             xsd:string ;
        schema:domainIncludes  <https://w3id.org/product/Window> , <https://w3id.org/product/Slab> , <https://w3id.org/product/BuildingElementProxy> , <https://w3id.org/product/Beam> , <https://w3id.org/product/Stair> , <https://w3id.org/product/Member> , <https://w3id.org/product/Plate> , <https://w3id.org/product/Column> , <https://w3id.org/product/Ramp> , <https://w3id.org/product/Door> , <https://w3id.org/product/Roof> , <https://w3id.org/product/Covering> , <https://w3id.org/product/Wall> , <https://w3id.org/product/Chimney> , <https://w3id.org/product/CurtainWall> .

props:constructionToleranceClass
        a                      owl:DatatypeProperty ;
        rdfs:comment           "Classification designation of the on-site construction tolerances according to local standards."@en , "国の基準が求める現場での製造許容の分類指定。"@ja-JP , "국가 표준이 요구하는 현장에서 제조 허용 범주 지정"@ko-KR ;
        rdfs:label             "constructionToleranceClass"@en , "製造許容クラス"@ja-JP , "제조 허용 클래스"@ko-KR ;
        rdfs:range             xsd:string ;
        schema:domainIncludes  <https://w3id.org/product/BuildingElement> .

props:assetAccountingType
        a                      owl:DatatypeProperty ;
        rdfs:comment           "Identifies the predefined types of risk from which the type required may be set."@en , "会計の定義済み種別。"@ja-JP ;
        rdfs:label             "assetAccountingType"@en , "資産会計種別"@ja-JP ;
        schema:domainIncludes  <https://w3id.org/product/Asset> .

props:cisternHeight  a         owl:DatatypeProperty ;
        rdfs:comment           "Enumeration that identifies the height of the cistern or, if set to 'None' if the urinal has no cistern and is flushed using mains or high pressure water through a flushing valve."@en , "貯水タンクの高さを示す。小便器がフラッシュバルブを使い貯水タンクを持っていない場合は'None'に設定される。"@ja-JP ;
        rdfs:label             "cisternHeight"@en , "貯水タンクの高さ"@ja-JP ;
        schema:domainIncludes  <https://w3id.org/product/SanitaryTerminal%2FCISTERN> .

props:bypassFactor  a          owl:DatatypeProperty ;
        rdfs:comment           "Fraction of air that is bypassed by the coil (0-1)."@en , "Fraction de l'air qui est bypassé par la batterie (0 à 1)."@fr-FR ;
        rdfs:label             "bypassFactor"@en , "FacteurBypass"@fr-FR ;
        rdfs:range             <https://w3id.org/product/NormalisedRatioMeasure> ;
        schema:domainIncludes  <https://w3id.org/product/Coil> .

props:isNeutralPrimaryTerminalAvailable
        a                      owl:DatatypeProperty ;
        rdfs:comment           "An indication of whether the neutral point of the primary winding is available as a terminal (=TRUE) or not (= FALSE)."@en , "一次巻線の中性点がターミナルの場合は（=TRUE）、違う場合は（= FALSE）として表示する"@ja-JP , "1차 권선의 중성점 터미널의 경우 (= TRUE), 다른 경우는 (= FALSE)로 표시"@ko-KR ;
        rdfs:label             "isNeutralPrimaryTerminalAvailable"@en , "中性点第1ターミナルがあるかどうか"@ja-JP , "중성점 제 1 터미널 여부"@ko-KR ;
        rdfs:range             xsd:boolean ;
        schema:domainIncludes  <https://w3id.org/product/Transformer> .

props:actualProductionDate
        a                      owl:DatatypeProperty ;
        rdfs:comment           "Production date (stripped from form)."@en ;
        rdfs:label             "actualProductionDate"@en ;
        rdfs:range             xsd:dateTime ;
        schema:domainIncludes  <https://w3id.org/product/BuildingElement> .

props:valveMechanism  a        owl:DatatypeProperty ;
        rdfs:comment           "The mechanism by which the valve function is achieved where:\n\nBALL: Valve that has a ported ball that can be turned relative to the body seat ports.\nBUTTERFLY: Valve in which a streamlined disc pivots about a diametric axis.\nCONFIGUREDGATE: Screwdown valve in which the closing gate is shaped in a configured manner to have a more precise control of pressure and flow change across the valve.\nGLAND: Valve with a tapered seating, in which a rotatable plug is retained by means of a gland and gland packing.\nGLOBE: Screwdown valve that has a spherical body.\nLUBRICATEDPLUG: Plug valve in which a lubricant is injected under pressure between the plug face and the body.\nNEEDLE: Valve for regulating the flow in or from a pipe, in which a slender cone moves along the axis of flow to close against a fixed conical seat.\nPARALLELSLIDE: Screwdown valve that has a machined plate that slides in formed grooves to form a seal.\nPLUG: Valve that has a ported plug that can be turned relative to the body seat ports.\nWEDGEGATE: Screwdown valve that has a wedge shaped plate fitting into tapered guides to form a seal."@en , "機構により可能な弁機能は以下の通り：\nボール弁(BALL valve)＝本体のシートポートに関連して回転できるポートボールを持つ弁　バタフライ弁(BUTTERFLY valve)＝直径軸あたりに流線型の円板の旋回軸のある弁　CONFIGUREDスクリュー弁(CONFIGUREDGATE Screwdown valve)＝閉鎖ゲートを持つねじ回し式弁。その弁は、弁を通過する時圧力と流量変更をより正確に制御できる方法で形づけられている　グランド弁(GLAND Valve)＝テーパーのついたシートを持った弁。その中に回転プラグがグランドとグランドパッキンによって保持されている　グローブスクリュー弁(GLOBE Screwdown valve)＝ 球形の本体を持つねじ回し式弁　滑プラグ弁(LUBRICATEDPLUG Plug valve)＝プラグ表面と本体との間の圧力を下げるために潤滑油が注入された弁　ニードル弁(NEEDLE Valve)＝管内外の流量を調節する弁。その中に固定した円錐形のシートを閉止ために、流れの軸に沿って動く細長いコーンを持っている　平行スライドスクリュー弁(PARALLELSLIDE Screwdown valve)＝機械加工されたプレートを持つねじ回し式弁。そのプレートはシールを形成するために溝の中を滑る　プラグ弁(PLUG Valve)＝本体のシートポートと関連して回転できる、ポートしたプラグを持つ弁　くさびゲートスクリュー弁(WEDGEGATE Screwdown valve)＝シールを形成するためにテーパーの付いたガイドの中をくさび状の板部品を持つねじ回し式弁"@ja-JP ;
        rdfs:label             "valveMechanism"@en , "弁機構"@ja-JP ;
        schema:domainIncludes  <https://w3id.org/product/Valve> .

props:thermalExpansionCoefficient
        a                      owl:DatatypeProperty ;
        rdfs:comment           "A measure of the expansion coefficient for warming up the material about one Kelvin."@en ;
        rdfs:label             "thermalExpansionCoefficient"@en ;
        rdfs:range             <https://w3id.org/product/ThermalExpansionCoefficientMeasure> ;
        schema:domainIncludes  <https://w3id.org/product/Material> .

props:bladeEdge  a             owl:DatatypeProperty ;
        rdfs:comment           "Blade edge."@en ;
        rdfs:label             "bladeEdge"@en ;
        schema:domainIncludes  <https://w3id.org/product/Damper> .

props:scrapFactor  a           owl:DatatypeProperty ;
        rdfs:comment           "Sheet metal scrap factor."@en , "金属板の廃材率。"@ja-JP , "금속판의 폐재 비율."@ko-KR ;
        rdfs:label             "scrapFactor"@en , "廃材率"@ja-JP , "폐기물 비율"@ko-KR ;
        rdfs:range             xsd:decimal ;
        schema:domainIncludes  <https://w3id.org/product/DistributionSystem%2FVENTILATION> .

props:crossingLowerBarPitch
        a                      owl:DatatypeProperty ;
        rdfs:comment           "The pitch length of the crossing lower bar."@en , "交差する下端筋間隔。"@ja-JP ;
        rdfs:label             "crossingLowerBarPitch"@en , "下端筋間隔"@ja-JP ;
        rdfs:range             <https://w3id.org/product/PositiveLengthMeasure> ;
        schema:domainIncludes  <https://w3id.org/product/Footing> .

props:logarithmicMeanTemperatureDifference
        a                      owl:DatatypeProperty ;
        rdfs:comment           "冷媒と水または空気の対数平均温度差"@ja-JP , "Logarithmic mean temperature difference between refrigerant and water or air."@en ;
        rdfs:label             "対数平均温度差"@ja-JP , "logarithmicMeanTemperatureDifference"@en ;
        schema:domainIncludes  <https://w3id.org/product/Evaporator> , <https://w3id.org/product/Condenser> .

props:primaryApparentPower
        a                      owl:DatatypeProperty ;
        rdfs:comment           "The power in VA (volt ampere) that has been transformed and that runs into the transformer on the primary side."@en , "変圧器の1次側に伝送される電力（VA: アンペア）。"@ja-JP , "변압기 1 차 측에 전송되는 전력 (VA : 암페어)."@ko-KR ;
        rdfs:label             "primaryApparentPower"@en , "第1電力"@ja-JP , "제 1 전력"@ko-KR ;
        rdfs:range             <https://w3id.org/product/PowerMeasure> ;
        schema:domainIncludes  <https://w3id.org/product/Transformer> .

props:requestComments
        a                      owl:DatatypeProperty ;
        rdfs:comment           "Comments that may be made on the request."@en , "要請を作成する人物の名称。"@ja-JP ;
        rdfs:label             "requestComments"@en , "要請ソース名"@ja-JP ;
        rdfs:range             xsd:string ;
        schema:domainIncludes  <https://w3id.org/product/ActionRequest> .

props:dischargePosition
        a                      owl:DatatypeProperty ;
        rdfs:comment           "Centrifugal fan discharge position.\n\nTOPHORIZONTAL: Top horizontal discharge. \nTOPANGULARDOWN: Top angular down discharge. \nDOWNBLAST: Downblast discharge. \nBOTTOMANGULARDOWN: Bottom angular down discharge. \nBOTTOMHORIZONTAL: Bottom horizontal discharge. \nBOTTOMANGULARUP: Bottom angular up discharge. \nUPBLAST: Upblast discharge. \nTOPANGULARUP: Top angular up discharge. \nOTHER: Other type of fan arrangement."@en , "遠心送風機の吐出位置\nTOPHORIZONTAL: 上部水平 \nTOPANGULARDOWN: 上部角度付き下向き \nDOWNBLAST: 下向き\nBOTTOMANGULARDOWN: 下部角度付き下向き\nBOTTOMHORIZONTAL: 下部水平\nBOTTOMANGULARUP: 下部角度付き上向き\nUPBLAST: 上向き\nTOPANGULARUP: 上部角度付き上向き. \nOTHER: その他"@ja-JP ;
        rdfs:label             "dischargePosition"@en , "吐出位置"@ja-JP ;
        schema:domainIncludes  <https://w3id.org/product/Fan%2FCENTRIFUGAL> .

props:serialNumber  a          owl:DatatypeProperty ;
        rdfs:comment           "The manufacturer's serial number for the precast concrete element."@en , "The serial number assigned to an occurrence of a product."@en ;
        rdfs:label             "serialNumber"@en ;
        rdfs:range             xsd:string ;
        schema:domainIncludes  <https://w3id.org/product/BuildingElement> , <https://w3id.org/product/Element> .

props:massDensity  a           owl:DatatypeProperty ;
        rdfs:comment           "Material mass density."@en ;
        rdfs:label             "massDensity"@en ;
        rdfs:range             <https://w3id.org/product/MassDensityMeasure> ;
        schema:domainIncludes  <https://w3id.org/product/Material> .

props:inertWaste  a            owl:DatatypeProperty ;
        rdfs:comment           "生成される安定廃棄物の量。"@ja-JP , "Quantité de déchets inertes générés  [NDT : selon la norme NF P01-010]"@fr-FR , "불활성 폐기물 발생량"@ko-KR , "Quantity of inert waste generated ."@en ;
        rdfs:label             "inertWaste"@en , "불활성 폐기불"@ko-KR , "DechetsInertes"@fr-FR , "安定廃棄物"@ja-JP ;
        rdfs:range             <https://w3id.org/product/MassMeasure> ;
        schema:domainIncludes  <https://w3id.org/product/Element> .

props:fanRotationSpeed
        a                      owl:DatatypeProperty ;
        rdfs:comment           "Fan rotation speed."@en , "回転速度"@ja-JP ;
        rdfs:label             "fanRotationSpeed"@en , "回転速度"@ja-JP ;
        schema:domainIncludes  <https://w3id.org/product/Fan> .

props:edgeDistanceToFirstAxis
        a                      owl:DatatypeProperty ;
        rdfs:comment           "The distance from the left (‘West’) edge of the slab (in the direction of span of the components) to the axis of the first component."@en ;
        rdfs:label             "edgeDistanceToFirstAxis"@en ;
        rdfs:range             <https://w3id.org/product/PositiveLengthMeasure> ;
        schema:domainIncludes  <https://w3id.org/product/Slab> .

props:hasSillExternal
        a                      owl:DatatypeProperty ;
        rdfs:comment           "Indication whether the window opening has an external sill (TRUE) or not (FALSE)."@en , "Angabe, ob dieses Fenster mit einer äußeren Fensterbank ausgestattet ist (JA) under nicht (NEIN)."@de-DE , "Indique si l'ouverture est dotée d'un seuil côté extérieur (VRAI) ou non (FAUX)."@fr-FR ;
        rdfs:label             "hasSillExternal"@en , "Fensterbank aussen"@de-DE , "Seuil côté extérieur"@fr-FR ;
        rdfs:range             xsd:boolean ;
        schema:domainIncludes  <https://w3id.org/product/Window> .

props:releaseCurrentI2tEnd
        a                      owl:DatatypeProperty ;
        rdfs:comment           "The release current in [x In] for the end point of the I2t tripping curve of the G-function, if any. The value of ReleaseCurrentI2tEnd shall be larger than ReleaseCurrentI2tStart."@en , "The release current in [x In] for the end point of the I2t tripping curve of the S-function, if any. The value of ReleaseCurrentI2tEnd shall be larger than ReleaseCurrentI2tStart."@en , "S함수 I2의 특성 곡선의 끝점에서 s를 방류 전류.   I2t 종료 방류 전류가 I2t 시작 방류 전류보다 낮게해야한다. \""@ko-KR , "G 함수 I2의 특성 곡선의 끝점에서 s를 방류 전류.   I2t 종료 방류 전류가 I2t 시작 방류 전류보다 낮게해야한다. \""@ko-KR , "G関数のI2の特性曲線のエンドポイントの[s]を放流電流。 \n  I2tの終了放流電流がI2tの開始放流電流よりも低くしなければならない。"@ja-JP , "S関数のI2の特性曲線のエンドポイントの[s]を放流電流。 \n  I2tの終了放流電流がI2tの開始放流電流よりも低くしなければならない。"@ja-JP ;
        rdfs:label             "releaseCurrentI2tEnd"@en , "I2tの終了放流電流"@ja-JP , "I2t 종료 방류 전류"@ko-KR ;
        rdfs:range             <https://w3id.org/product/ElectricCurrentMeasure> ;
        schema:domainIncludes  <https://w3id.org/product/ProtectiveDeviceTrippingUnit> .

props:weight  a                owl:DatatypeProperty ;
        rdfs:comment           "케이블의 무게"@ko-KR , "코어 kg / km의 무게."@ko-KR , "ケーブルの重量。"@ja-JP , "Weight of filter."@en , "The weight of the humidifier."@en , "The weight of the silencer."@en , "Weight of core kg/km."@en , "コアkg/kmの重量。"@ja-JP , "Weight of cable kg/km."@en , "加湿器の重量"@ja-JP , "サイレンサ重量"@ja-JP ;
        rdfs:label             "weight"@en , "무게"@ko-KR , "重さ"@ja-JP , "重量"@ja-JP ;
        rdfs:range             <https://w3id.org/product/MassMeasure> ;
        schema:domainIncludes  <https://w3id.org/product/Humidifier> , <https://w3id.org/product/Filter> , <https://w3id.org/product/CableSegment%2FCABLESEGMENT> , <https://w3id.org/product/DuctSilencer> , <https://w3id.org/product/CableSegment%2FCORESEGMENT> .

props:hasVisualIndicator
        a                      owl:DatatypeProperty ;
        rdfs:comment           "Indication of whether the tank is provided with a visual indicator (set TRUE) that shows the water level in the tank. If no visual indicator is provided then value is set FALSE."@en , "タンクの水位を示す目視型表示器（TRUEに設定)が備えつけられているかどうかの表示。もし目視型表示器が備えつけられていなければ、値はFALSEと設定される。"@ja-JP ;
        rdfs:label             "hasVisualIndicator"@en , "目視型表示器有り"@ja-JP ;
        rdfs:range             xsd:boolean ;
        schema:domainIncludes  <https://w3id.org/product/Tank> .

props:molecularWeight
        a                      owl:DatatypeProperty ;
        rdfs:comment           "Molecular weight of material (typically gas)."@en ;
        rdfs:label             "molecularWeight"@en ;
        rdfs:range             <https://w3id.org/product/MolecularWeightMeasure> ;
        schema:domainIncludes  <https://w3id.org/product/Material> .

props:process  a               owl:DatatypeProperty ;
        rdfs:comment           "Reference number of the welding process according to ISO 4063, an up to three digits long code"@en ;
        rdfs:label             "process"@en ;
        rdfs:range             xsd:int ;
        schema:domainIncludes  <https://w3id.org/product/Fastener%2FWELD> .

props:plasticShapeFactorZ
        a                      owl:DatatypeProperty ;
        rdfs:comment           "Ratio of plastic versus elastic bending moment capacity about the section analysis axis zs. A dimensionless value."@en ;
        rdfs:label             "plasticShapeFactorZ"@en ;
        rdfs:range             <https://w3id.org/product/PositiveRatioMeasure> ;
        schema:domainIncludes  <https://w3id.org/product/ProfileDef> .

props:tunerFrequency  a        owl:DatatypeProperty ;
        rdfs:comment           "Indicates the tuner frequencies, if applicable."@en , "対応周波数帯を示す。"@ja-JP , "주파수 대역을 나타낸다."@ko-KR ;
        rdfs:label             "tunerFrequency"@en , "周波数"@ja-JP , "주파수 대응"@ko-KR ;
        schema:domainIncludes  <https://w3id.org/product/AudioVisualAppliance%2FTUNER> .

props:nominalCurrentAdjusted
        a                      owl:DatatypeProperty ;
        rdfs:comment           "전류 작동 시간 길이 여부"@ko-KR , "電流によって、動作時間が短かかったり長かったりするかどうか。"@ja-JP , "전류 작동 시간의 여부"@ko-KR , "An indication if the tripping currents of the short time protection is related to the nominal current multiplied with the actual setting of the current adjustment, if any, of the long time protection part of the protective device, or not."@en ;
        rdfs:label             "定格調整電流"@ja-JP , "정격전류조정"@ko-KR , "nominalCurrentAdjusted"@en ;
        rdfs:range             xsd:boolean ;
        schema:domainIncludes  <https://w3id.org/product/ProtectiveDeviceTrippingUnit> .

props:coreSetVertical
        a                      owl:DatatypeProperty ;
        rdfs:comment           "Degree of vertical (in the Y-axis of the LocalPlacement) blade set from the centerline."@en , "垂直翼の中心線からの垂直（ローカル座標のＹ軸）方向の羽根角度"@ja-JP , "Degré d'inclinaison verticale (selon l'axe Y par rapport au positionnement local) de la lame mesuré depuis la ligne médiane."@fr-FR ;
        rdfs:label             "coreSetVertical"@en , "垂直羽根角度"@ja-JP , "PositionVerticalCentre"@fr-FR ;
        rdfs:range             <https://w3id.org/product/PlaneAngleMeasure> ;
        schema:domainIncludes  <https://w3id.org/product/AirTerminal> .

props:description  a           owl:DatatypeProperty ;
        rdfs:comment           "Specific description of this type of furniture."@en , "Description of the reinforcement."@en , "鉄筋の説明。"@ja-JP , "空調方式の説明。"@ja-JP , "The description of the air side system."@en , "공조 방식 설명"@ko-KR ;
        rdfs:label             "description"@en , "説明"@ja-JP , "설명"@ko-KR ;
        rdfs:range             xsd:string ;
        schema:domainIncludes  <https://w3id.org/product/Furniture> , <https://w3id.org/product/Beam> , <https://w3id.org/product/Zone> , <https://w3id.org/product/Slab> , <https://w3id.org/product/Footing> , <https://w3id.org/product/Wall> , <https://w3id.org/product/Space> , <https://w3id.org/product/SpatialZone> , <https://w3id.org/product/Column> .

props:nominalDiameter
        a                      owl:DatatypeProperty ;
        rdfs:comment           "配管の呼び径。"@ja-JP , "Nominal diameter or width of the tubes in the tube bundle."@en , "The nominal diameter of the pipe connection."@en , "チューブ束内のチューブ公称直径又は幅"@ja-JP , "配管部の呼び径、リストに一つの数字しかないとき、この呼び径が全ての管端に当てはまる。一つ以上の数字があるとき、呼び径はリストの表示に対応する管端にあてはまる。"@ja-JP , "The nominal diameter of the pipe segment."@en ;
        rdfs:label             "公称直径"@ja-JP , "nominalDiameter"@en , "呼び径"@ja-JP ;
        rdfs:range             <https://w3id.org/product/PositiveLengthMeasure> ;
        schema:domainIncludes  <https://w3id.org/product/DistributionPort%2FCHEMICAL> , <https://w3id.org/product/TubeBundle> , <https://w3id.org/product/PipeSegment> .

props:equipmentSensible
        a                      owl:DatatypeProperty ;
        rdfs:comment           "Heat gains and losses from equipment."@en , "事務機器からの熱取得と熱ロス。"@ja-JP , "사무기기에서 열 취득 및 손실"@ko-KR ;
        rdfs:label             "equipmentSensible"@en , "事務機器の顕熱"@ja-JP , "사무기기의 현열"@ko-KR ;
        schema:domainIncludes  <https://w3id.org/product/Space> .

props:setPointRadiation
        a                      owl:DatatypeProperty ;
        rdfs:comment           "The radiation power value to be sensed. Use IfcPropertyBoundedValue.SetPointValue to set the set point value."@en , "感知される放射線量。\nセットポイント値を置くために、IfcPropertyBoundedValue.SetPointValueを使用する。"@ja-JP , "감지되는 방사선. 세트 포인트 값을 넣으려면, IfcPropertyBoundedValue.SetPointValue를 사용하십시오."@ko-KR ;
        rdfs:label             "setPointRadiation"@en , "放射線設定値"@ja-JP , "방사선 설정"@ko-KR ;
        schema:domainIncludes  <https://w3id.org/product/Sensor%2FRADIATIONSENSOR> .

props:designLevel  a           owl:DatatypeProperty ;
        rdfs:comment           "Adjustment of the service life resulting from the effect of design level employed."@en ;
        rdfs:label             "designLevel"@en ;
        schema:domainIncludes  <https://w3id.org/product/System> .

props:operation  a             owl:DatatypeProperty ;
        rdfs:comment           "The operational mechanism for the damper operation."@en ;
        rdfs:label             "operation"@en ;
        schema:domainIncludes  <https://w3id.org/product/Damper> .

props:publiclyAccessible
        a                      owl:DatatypeProperty ;
        rdfs:comment           "Indique si l'espace (par exemple des toilettes) est conçu pour être un espace accessible au public (TRUE) ou non (FALSE)."@fr-FR , "가능성이 공간이 공공 액세스 공간 여부를 나타내는 부울 값입니다. 예 : 공공 화장실의 경우 TRUE/ FALSE"@ko-KR , "Indication whether this space (in case of e.g., a toilet) is designed to serve as a publicly accessible space, e.g., for a public toilet (TRUE) or not (FALSE)."@en , "この空間が公共アクセス空間かどうかを示すブーリアン値。例：公共トイレの場合（TRUE）。そうでなければ（FALSE）。"@ja-JP , "Angabe, ob dieser Raum (wie z.B. eine Toilette) öffentlich zugänglich sein soll (JA) oder nicht (NEIN)."@de-DE , "この部屋（空間）が公共アクセス空間かどうかを示すブーリアン値。例：公共トイレの場合TRUE。"@ja-JP , "이 방 (공간)이 공공 액세스 공간 여부를 나타내는 부울 값입니다. 예 : 공공 화장실의 경우 TRUE."@ko-KR ;
        rdfs:label             "公共アクセス可能性"@ja-JP , "AccessibleAuPublic"@fr-FR , "öffentlich zugänglich"@de-DE , "publiclyAccessible"@en , "공공 액세스 가능성"@ko-KR ;
        rdfs:range             xsd:boolean ;
        schema:domainIncludes  <https://w3id.org/product/Zone> , <https://w3id.org/product/Space> .

props:amplifierType  a         owl:DatatypeProperty ;
        rdfs:comment           "Indicates the type of amplifier."@en , "アンプの形式を示す。"@ja-JP , "앰프의 형식을 보여준다."@ko-KR ;
        rdfs:label             "amplifierType"@en , "アンプ形式"@ja-JP , "앰프 형식"@ko-KR ;
        schema:domainIncludes  <https://w3id.org/product/AudioVisualAppliance%2FAMPLIFIER> .

props:surfaceSpreadOfFlame
        a                      owl:DatatypeProperty ;
        rdfs:comment           "Indique comment les flammes se propagent sur une surface. Indication donnée selon le Code National du Bâtiment régissant le comportement au feu des matériaux."@fr-FR , "火炎表面伝播性。当該国の建築法規による。"@ja-JP , "炎がどのように材料の表面を広がるかという指標。材料の炎に対する振る舞いについての国家建築規則に従って提供される。"@ja-JP , "Indication on how the flames spread around the surface,\nIt is given according to the national building code that governs the fire behaviour for materials."@en , "Indication on how the flames spread around the surface, It is given according to the national building code that governs the fire behaviour for materials."@en , "German-description-5"@de-DE , "Beschreibung des Brandverhaltens des Bauteils gemäß der nationalen oder regionalen  Brandschutzverordnung."@de-DE ;
        rdfs:label             "surfaceSpreadOfFlame"@en , "Brandverhalten"@de-DE , "Propagation des flammes en surface"@fr-FR , "火炎表面伝播性"@ja-JP , "火炎伝播性"@ja-JP , "SurfacePropagationFlamme"@fr-FR ;
        rdfs:range             xsd:string ;
        schema:domainIncludes  <https://w3id.org/product/Covering> , <https://w3id.org/product/Slab> , <https://w3id.org/product/Wall> , <https://w3id.org/product/CurtainWall> .

props:tendonRelaxation
        a                      owl:DatatypeProperty ;
        rdfs:comment           "The maximum allowable relaxation of the tendon (usually expressed as %/1000 h).This property applies to prestressed concrete elements only."@en , "緊張材の最大許容リラクセーション（応力弛緩、－係数）。通常、1000時間あたりの割合（%)。この属性はプレストレストコンクリート要素のみに適用される。"@ja-JP ;
        rdfs:label             "tendonRelaxation"@en , "緊張材のリラクセーション"@ja-JP ;
        rdfs:range             <https://w3id.org/product/PositiveRatioMeasure> ;
        schema:domainIncludes  <https://w3id.org/product/BuildingElement> .

props:coilCoolant  a           owl:DatatypeProperty ;
        rdfs:comment           "The fluid used for heating or cooling used by the hydronic coil."@en , "Le fluide utilisé pour chauffer ou refroidir dans la batterie deux tubes."@fr-FR ;
        rdfs:label             "coilCoolant"@en , "RefrigerantBatterie"@fr-FR ;
        schema:domainIncludes  <https://w3id.org/product/Coil> .

props:shapeType  a             owl:DatatypeProperty ;
        rdfs:comment           "Shape of the junction box."@en , "ジヤンクションボックスの形状。"@ja-JP , "지얀 섹션 상자 모양."@ko-KR ;
        rdfs:label             "shapeType"@en , "形状"@ja-JP , "형상"@ko-KR ;
        schema:domainIncludes  <https://w3id.org/product/JunctionBox> .

props:effectiveCapacity
        a                      owl:DatatypeProperty ;
        rdfs:comment           "The total effective or actual volumetric capacity of the tank."@en , "タンクの総有効又は実容量"@ja-JP ;
        rdfs:label             "effectiveCapacity"@en , "有効容量"@ja-JP ;
        rdfs:range             <https://w3id.org/product/VolumeMeasure> ;
        schema:domainIncludes  <https://w3id.org/product/Tank> .

props:buildableArea  a         owl:DatatypeProperty ;
        rdfs:comment           "建築基準により建築可能な最大の面積。"@ja-JP , "bebaubare Fläche als maximale überbaubare Fläche des Grundstücks."@de-DE , "Surface constructible maximale en fonction des contraintes d'urbanisme."@fr-FR , "속성정의"@ko-KR , "The area of site utilization expressed as a maximum value according to local building codes."@en ;
        rdfs:label             "건축 가능 면적"@ko-KR , "建築可能面積"@ja-JP , "ValeurSurfaceConstructible"@fr-FR , "buildableArea"@en , "bebaubare Fläche"@de-DE ;
        rdfs:range             <https://w3id.org/product/AreaMeasure> ;
        schema:domainIncludes  <https://w3id.org/product/Site> .

props:addressablility
        a                      owl:DatatypeProperty ;
        rdfs:comment           "The type of addressability."@en , "アドレス指定能力のタイプ。"@ja-JP , "주소 지정 능력 타입"@ko-KR ;
        rdfs:label             "addressablility"@en , "アドレス指定能力"@ja-JP , "주소 지정 능력"@ko-KR ;
        schema:domainIncludes  <https://w3id.org/product/LightFixture%2FSECURITYLIGHTING> .

props:uACurve  a               owl:DatatypeProperty ;
        rdfs:comment           "UA curve as function of ambient temperature and surface temperature; UA = f (Tambient, Tsurface)"@en , "周囲温度と表面温度との関数のUA曲線"@ja-JP , "UA value as a  function of fan speed at certain water flow rate, UA = f ( fan speed)."@en ;
        rdfs:label             "UA曲線"@ja-JP , "uACurve"@en ;
        schema:domainIncludes  <https://w3id.org/product/SpaceHeater> , <https://w3id.org/product/CoolingTower> .

props:dustHoldingCapacity
        a                      owl:DatatypeProperty ;
        rdfs:comment           "Maximum filter dust holding capacity."@en ;
        rdfs:label             "dustHoldingCapacity"@en ;
        rdfs:range             <https://w3id.org/product/MassMeasure> ;
        schema:domainIncludes  <https://w3id.org/product/Filter%2FAIRPARTICLEFILTER> .

props:maintenaceType  a        owl:DatatypeProperty ;
        rdfs:comment           "Identifies the predefined types of maintenance that can be done from which the type that generates the maintenance work order may be set where:\n\nConditionBased: generated as a result of the condition of an asset or artefact being less than a determined value.\nCorrective: generated as a result of an immediate and urgent need for maintenance action.\nPlannedCorrective: generated as a result of immediate corrective action being needed but with sufficient time available for the work order to be included in maintenance planning.\nScheduled: generated as a result of a fixed, periodic maintenance requirement."@en ;
        rdfs:label             "maintenaceType"@en ;
        schema:domainIncludes  <https://w3id.org/product/ProjectOrder%2FMAINTENANCEWORKORDER> .

props:clearHeight  a           owl:DatatypeProperty ;
        rdfs:comment           "Clear height of the object (elevator).  \nThe shape information is provided in addition to the shape representation and the geometric parameters used within. In cases of inconsistency between the geometric parameters and the shape properties, provided in the attached property, the geometric parameters take precedence."@en , "オブジェクト（エレベータ）の高さ。エレベータドアの内部の床面から天井までの距離を示す。\n形状表現は、Shape representation（IFCの幾何形状表現）およびそこで設定されている幾何形状パラメータにより与えられる。もし、幾何形状パラメータと形状プロパティ情報が一致しない場合は、形状パラメータの値を優先する。"@ja-JP , "Hauteur du passage de l'ascenseur. Cette propriété est donnée en complément de la représentation de la forme de l'élément et des paramètres géométriques qui la déterminent. En cas d'incohérence entre ces paramètres géométriques et cette propriété, ce sont les paramètres géométriques qui priment."@fr-FR ;
        rdfs:label             "clearHeight"@en , "高さ"@ja-JP , "Hauteur de passage"@fr-FR ;
        rdfs:range             <https://w3id.org/product/PositiveLengthMeasure> ;
        schema:domainIncludes  <https://w3id.org/product/TransportElement%2FELEVATOR> .

props:severity  a              owl:DatatypeProperty ;
        rdfs:comment           "Indicates alarm severity over time, where the scale of values is determined by the control system configuration.  A zero value indicates no present alarm."@en ;
        rdfs:label             "severity"@en ;
        schema:domainIncludes  <https://w3id.org/product/Alarm> .

props:coverMaterial  a         owl:DatatypeProperty ;
        rdfs:comment           "Material from which the cover or grating is constructed."@en , "カバーか格子の材質。"@ja-JP ;
        rdfs:label             "coverMaterial"@en , "カバー材質"@ja-JP ;
        schema:domainIncludes  <https://w3id.org/product/WasteTerminal%2FFLOORTRAP> .

props:horizontalSpacing
        a                      owl:DatatypeProperty ;
        rdfs:comment           "Horizontal spacing between tubes in the tube bundle."@en , "チューブ束内のチューブ間水平間隔"@ja-JP ;
        rdfs:label             "horizontalSpacing"@en , "水平間隔"@ja-JP ;
        rdfs:range             <https://w3id.org/product/PositiveLengthMeasure> ;
        schema:domainIncludes  <https://w3id.org/product/TubeBundle> .

props:buildingHeightLimit
        a                      owl:DatatypeProperty ;
        rdfs:comment           "Allowed maximum height of buildings on this site - according to local building codes."@en , "TotalArea / BuildableArea로 표시되는 이용 가능한 비율의 최대값입니다."@ko-KR , "Maximale Bebauungshöhe die auf diesem Grundstück zulässig ist."@de-DE , "Hauteur maximale des bâtiments autorisée sur ce site."@fr-FR , "各地域の建築基準により許可される建物の高さの最大値。"@ja-JP ;
        rdfs:label             "HauteurMaximale"@fr-FR , "maximale Bebauungshöhe"@de-DE , "建物高さ制限"@ja-JP , "건물 높이 제한"@ko-KR , "buildingHeightLimit"@en ;
        rdfs:range             <https://w3id.org/product/PositiveLengthMeasure> ;
        schema:domainIncludes  <https://w3id.org/product/Site> .

props:idealShaftPower
        a                      owl:DatatypeProperty ;
        rdfs:comment           "Compressor shaft power under ideal conditions."@en , "Puissance au niveau de l'arbre du compresseur sous conditions idéales."@fr-FR ;
        rdfs:label             "idealShaftPower"@en , "PuissanceArbreMaximale"@fr-FR ;
        rdfs:range             <https://w3id.org/product/PowerMeasure> ;
        schema:domainIncludes  <https://w3id.org/product/Compressor> .

props:productDescription
        a                      owl:DatatypeProperty ;
        rdfs:comment           "A textual description of the products that require the work."@en ;
        rdfs:label             "productDescription"@en ;
        rdfs:range             xsd:string ;
        schema:domainIncludes  <https://w3id.org/product/ProjectOrder%2FWORKORDER> , <https://w3id.org/product/ProjectOrder%2FMAINTENANCEWORKORDER> .

props:setPointContact
        a                      owl:DatatypeProperty ;
        rdfs:comment           "The contact value to be sensed. Use IfcPropertyBoundedValue.SetPointValue to set the set point value."@en , "感知される接触状態。\nセットポイント値を置くために、IfcPropertyBoundedValue.SetPointValueを使用する。"@ja-JP , "감지되는 접촉 상태. 세트 포인트 값을 넣으려면, IfcPropertyBoundedValue.SetPointValue를 사용하십시오."@ko-KR ;
        rdfs:label             "setPointContact"@en , "接触状態設定値"@ja-JP , "접촉 상태 설정"@ko-KR ;
        schema:domainIncludes  <https://w3id.org/product/Sensor%2FCONTACTSENSOR> .

props:coolingDryBulb  a        owl:DatatypeProperty ;
        rdfs:comment           "냉방 설계의 실내 디자인 건구 온도"@ko-KR , "냉방용 설계 외기건구 온도"@ko-KR , "Inside dry bulb temperature for cooling design."@en , "冷房設計における室内設計乾球温度。"@ja-JP , "Outside dry bulb temperature for cooling design."@en , "冷房用設計用外気乾球温度。"@ja-JP ;
        rdfs:label             "냉방 설계온도"@ko-KR , "冷房用設計外気乾球温度"@ja-JP , "냉방용 설계 외기건구 온도"@ko-KR , "coolingDryBulb"@en , "冷房設計温度"@ja-JP ;
        rdfs:range             <https://w3id.org/product/ThermodynamicTemperatureMeasure> ;
        schema:domainIncludes  <https://w3id.org/product/Space> , <https://w3id.org/product/Building> .

props:enabled  a               owl:DatatypeProperty ;
        rdfs:comment           "Indicates whether alarm is enabled or disabled over time."@en ;
        rdfs:label             "enabled"@en ;
        schema:domainIncludes  <https://w3id.org/product/Alarm> .

props:hoseLength  a            owl:DatatypeProperty ;
        rdfs:comment           "Notional length of the hose fitted to the hose reel when fully extended."@en , "ホースホースリールに装着されたホースの公称長さ（全て伸ばされたときの）。"@ja-JP ;
        rdfs:label             "hoseLength"@en , "ホースの長さ"@ja-JP ;
        rdfs:range             <https://w3id.org/product/PositiveLengthMeasure> ;
        schema:domainIncludes  <https://w3id.org/product/FireSuppressionTerminal%2FHOSEREEL> .

props:location2Local  a        owl:DatatypeProperty ;
        rdfs:comment           "Local x,y coordinates of the point in which Thickness2 is given"@en ;
        rdfs:label             "location2Local"@en ;
        schema:domainIncludes  <https://w3id.org/product/StructuralSurfaceMemberVarying> .

props:numberOfCircuits
        a                      owl:DatatypeProperty ;
        rdfs:comment           "Number of parallel fluid tube circuits."@en , "平行流チューブ回路数"@ja-JP ;
        rdfs:label             "numberOfCircuits"@en , "平行流回路数"@ja-JP ;
        rdfs:range             xsd:int ;
        schema:domainIncludes  <https://w3id.org/product/TubeBundle> .

props:renewableEnergyConsumptionPerUnit
        a                      owl:DatatypeProperty ;
        rdfs:comment           "ISO21930:2007で定義される再生可能エネルギーの使用量。"@ja-JP , "ISO21930 : 2007에 정의된 재생 가능 에너지 사용량"@ko-KR , "Quantity of renewable energy used as defined in ISO21930:2007"@en , "Consommation d'énergie renouvelable telle que définie dans la norme ISO21930:2007 [NDT : et dans la norme NF P01-010]"@fr-FR ;
        rdfs:label             "단위당 재생 에너지 소비"@ko-KR , "単位あたり再生可能エネルギ消費"@ja-JP , "ConsommationEnergieRenouvelableParUnite"@fr-FR , "renewableEnergyConsumptionPerUnit"@en ;
        rdfs:range             <https://w3id.org/product/EnergyMeasure> ;
        schema:domainIncludes  <https://w3id.org/product/Element> .

props:version  a               owl:DatatypeProperty ;
        rdfs:comment           "The version number of the agreement that is identified."@en ;
        rdfs:label             "version"@en ;
        rdfs:range             xsd:string ;
        schema:domainIncludes  <https://w3id.org/product/SpatialStructureElement> .

props:visibleReflectanceBack
        a                      owl:DatatypeProperty ;
        rdfs:comment           "Reflectance at normal incidence (visible): back side. Defines the fraction of the solar ray in the visible spectrum that is reflected and not transmitted when the ray passes from one medium into another, at the \"back\" side of the other material, perpendicular to the surface. Dependent on material and surface characteristics."@en ;
        rdfs:label             "visibleReflectanceBack"@en ;
        rdfs:range             <https://w3id.org/product/PositiveRatioMeasure> ;
        schema:domainIncludes  <https://w3id.org/product/Material> .

props:momentaryType  a         owl:DatatypeProperty ;
        rdfs:comment           "A list of the available types of momentary switch from which that required may be selected."@en , "選択が必要となる、自動復帰スイッチの一覧リスト。"@ja-JP , "선택이 필요한 자동 복귀 스위치 목록"@ko-KR ;
        rdfs:label             "momentaryType"@en , "瞬時スイッチタイプ"@ja-JP , "순간스위치 유형"@ko-KR ;
        schema:domainIncludes  <https://w3id.org/product/SwitchingDevice%2FMOMENTARYSWITCH> .

props:internalSurfaceArea
        a                      owl:DatatypeProperty ;
        rdfs:comment           "内部表面積"@ja-JP , "Internal surface area."@en ;
        rdfs:label             "内表面積"@ja-JP , "internalSurfaceArea"@en ;
        rdfs:range             <https://w3id.org/product/AreaMeasure> ;
        schema:domainIncludes  <https://w3id.org/product/Evaporator> , <https://w3id.org/product/Condenser> .

props:fullLoadRatio  a         owl:DatatypeProperty ;
        rdfs:comment           "Ratio of actual power to full load power as a quadratic function of part load, at certain condensing and evaporating temperature, FracFullLoadPower = f ( PartLoadRatio)."@en , "Rapport entre puissance actuelle sur la puissance à pleine charge, comme fonction quadratique de la charge partielle, à une température de condensation et une température d'évaporation donnée, FracFullLoadPower = f (RapportChargePartielle)."@fr-FR ;
        rdfs:label             "fullLoadRatio"@en , "CoefficientChargeTotale"@fr-FR ;
        schema:domainIncludes  <https://w3id.org/product/Compressor> .

props:shearCentreY  a          owl:DatatypeProperty ;
        rdfs:comment           "Location of the profile's shear centre, measured along ys."@en ;
        rdfs:label             "shearCentreY"@en ;
        rdfs:range             <https://w3id.org/product/LengthMeasure> ;
        schema:domainIncludes  <https://w3id.org/product/ProfileDef> .

props:downstreamPressure
        a                      owl:DatatypeProperty ;
        rdfs:comment           "The operating pressure of the fluid downstream of the pressure reducing valve."@en , "減圧弁の下流の流体運転圧力"@ja-JP ;
        rdfs:label             "downstreamPressure"@en , "下流圧力"@ja-JP ;
        rdfs:range             <https://w3id.org/product/PressureMeasure> ;
        schema:domainIncludes  <https://w3id.org/product/Valve%2FPRESSUREREDUCING> .

props:infiltrationDiversityWinter
        a                      owl:DatatypeProperty ;
        rdfs:comment           "冬期すき間換気率。"@ja-JP , "겨울철 틈새 환기 비율."@ko-KR , "겨울철 틈새 환기 비율"@ko-KR , "Diversity factor for Winter infiltration."@en ;
        rdfs:label             "겨울철 틈새 환기비율"@ko-KR , "infiltrationDiversityWinter"@en , "冬期すき間換気率"@ja-JP , "겨울철 틈새 환기 비율"@ko-KR ;
        rdfs:range             <https://w3id.org/product/PositiveRatioMeasure> ;
        schema:domainIncludes  <https://w3id.org/product/Space> , <https://w3id.org/product/Zone> , <https://w3id.org/product/SpatialElement> , <https://w3id.org/product/SpatialZone> .

props:temperatureRating
        a                      owl:DatatypeProperty ;
        rdfs:comment           "Temperature rating."@en ;
        rdfs:label             "temperatureRating"@en ;
        rdfs:range             <https://w3id.org/product/ThermodynamicTemperatureMeasure> ;
        schema:domainIncludes  <https://w3id.org/product/Damper> .

props:capacityControl
        a                      owl:DatatypeProperty ;
        rdfs:comment           "FanCycling: Fan is cycled on and off to control duty.\nTwoSpeedFan: Fan is switched between low and high speed to control duty.\nVariableSpeedFan: Fan speed is varied to control duty.\nDampersControl: Dampers modulate the air flow to control duty.\nBypassValveControl: Bypass valve modulates the water flow to control duty.\nMultipleSeriesPumps: Turn on/off multiple series pump to control duty.\nTwoSpeedPump: Switch between high/low pump speed to control duty.\nVariableSpeedPump: vary pump speed to control duty."@en ;
        rdfs:label             "capacityControl"@en ;
        schema:domainIncludes  <https://w3id.org/product/CoolingTower> .

props:accessCoverLoadRating
        a                      owl:DatatypeProperty ;
        rdfs:comment           "The load rating of the access cover (which may be a value or an alphanumerically defined class rating)."@en , "사용 (체크) 커버 하중 (숫자 혹은 알파벳에서 정의됨)"@ko-KR , "アクセス（点検）カバーの耐荷重（数字或いはアルファベットで定義する）。"@ja-JP ;
        rdfs:label             "사용 (체크)커버 하중"@ko-KR , "accessCoverLoadRating"@en , "アクセス（点検）カバーの耐荷重"@ja-JP , "사용(체크)커버 하중"@ko-KR ;
        rdfs:range             xsd:string ;
        schema:domainIncludes  <https://w3id.org/product/DistributionChamberElement%2FMANHOLE> , <https://w3id.org/product/DistributionChamberElement%2FFORMEDDUCT> , <https://w3id.org/product/DistributionChamberElement%2FINSPECTIONCHAMBER> .

props:tileWidth  a             owl:DatatypeProperty ;
        rdfs:comment           "Breite der Unterdeckenplatten, oder -panele, die zur Verkleidung verwendet werden."@de-DE , "Largeur des carreaux de plafond. Cette propriété est donnée en complément de la représentation de la forme et des paramètres géométriques qui la déterminent. En cas d'incohérence entre ces paramètres géométriques et cette propriété, ce sont les paramètres géométriques qui priment."@fr-FR , "天花板面砖的宽度。\n该属性所提供的尺寸信息是对内部形状描述和几何参数的补充。如果几何参数与该属性所提供的尺寸属性不符，应以几何参数为准。"@zh-CN , "Width of ceiling tiles. The size information is provided in addition to the shape representation and the geometric parameters used within. In cases of inconsistency between the geometric parameters and the size properties, provided in the attached property set, the geometric parameters take precedence."@en ;
        rdfs:label             "Deckenplattenbreite"@de-DE , "Largeur des carreaux"@fr-FR , "tileWidth"@en , "面砖宽度"@zh-CN ;
        rdfs:range             <https://w3id.org/product/PositiveLengthMeasure> ;
        schema:domainIncludes  <https://w3id.org/product/Covering%2FCEILING> .

props:arrangementType
        a                      owl:DatatypeProperty ;
        rdfs:comment           "Terminal box arrangement.\nSingleDuct: Terminal box receives warm or cold air from a single air supply duct.\nDualDuct: Terminal box receives warm and cold air from separate air supply ducts."@en , "ターミナルボックスの形式。\n単一ダクト：単一のダクトから、温風または冷風を受け取る\nデュアルダクト：温風、冷風を分離されたダクトから受け取る"@ja-JP , "Configuration du registre terminal.\nConduit unique: le registre terminal reçoit de l'air chaud ou froid depuis un conduit unique d'amenée d'air"@fr-FR ;
        rdfs:label             "arrangementType"@en , "ターミナル形式"@ja-JP , "Type de configuration"@fr-FR ;
        schema:domainIncludes  <https://w3id.org/product/AirTerminalBox> .

props:signalFactor  a          owl:DatatypeProperty ;
        rdfs:comment           "Factor multiplied onto offset signal."@en , "인자는 오프셋 신호 곱셈"@ko-KR ;
        rdfs:label             "signalFactor"@en , "요소"@ko-KR ;
        rdfs:range             xsd:decimal ;
        schema:domainIncludes  <https://w3id.org/product/Controller%2FFLOATING> .

props:drainConnectionSize
        a                      owl:DatatypeProperty ;
        rdfs:comment           "Size of the drain connection inlet to the waste disposal unit."@en , "ゴミ処理装置の吸入口配管接続口サイズ。"@ja-JP ;
        rdfs:label             "drainConnectionSize"@en , "配管接続口サイズ"@ja-JP ;
        rdfs:range             <https://w3id.org/product/PositiveLengthMeasure> ;
        schema:domainIncludes  <https://w3id.org/product/WasteTerminal%2FWASTEDISPOSALUNIT> .

props:frictionHeatGain
        a                      owl:DatatypeProperty ;
        rdfs:comment           "Friction heat gain."@en , "Gain thermique par friction."@fr-FR ;
        rdfs:label             "frictionHeatGain"@en , "GainThermiqueFriction"@fr-FR ;
        schema:domainIncludes  <https://w3id.org/product/Compressor> .

props:ratedTemperature
        a                      owl:DatatypeProperty ;
        rdfs:comment           "使用できることが許可されている許容温度。"@ja-JP , "장치를 사용할 보장된 온도 상한은 최대."@ko-KR , "사용할 수있는 권한이있는 허용 온도"@ko-KR , "The range of allowed temerature that a device is certified to handle. The upper bound of this value is the maximum."@en , "機器を使用できる保障された温度。上限値は最大値。"@ja-JP ;
        rdfs:label             "定格温度"@ja-JP , "정격 온도"@ko-KR , "ratedTemperature"@en ;
        schema:domainIncludes  <https://w3id.org/product/CableSegment%2FCABLESEGMENT> , <https://w3id.org/product/CableSegment%2FCORESEGMENT> .

props:ventilationOutdoorAir
        a                      owl:DatatypeProperty ;
        rdfs:comment           "Ventilation loads from outdoor air."@en , "外気による熱負荷。"@ja-JP , "외기에한 열부하"@ko-KR ;
        rdfs:label             "ventilationOutdoorAir"@en , "外気量"@ja-JP , "외기량"@ko-KR ;
        schema:domainIncludes  <https://w3id.org/product/Space> .

props:motorDriveType  a        owl:DatatypeProperty ;
        rdfs:comment           "Motor drive type:\nDIRECTDRIVE: Direct drive. \nBELTDRIVE: Belt drive. \nCOUPLING: Coupling. \nOTHER: Other type of motor drive. \nUNKNOWN: Unknown motor drive type."@en , "モーター駆動種類\nDIRECTDRIVE: ダイレクトドライブ\nBELTDRIVE: ベルトドライブ\nCOUPLING: カップリング\nOTHER: その他"@ja-JP ;
        rdfs:label             "motorDriveType"@en , "モーター駆動種類"@ja-JP ;
        schema:domainIncludes  <https://w3id.org/product/Fan> .

props:workFinishTime  a        owl:DatatypeProperty ;
        rdfs:comment           "The default time of day a task is scheduled to finish. For presentation purposes, if the finish time of a task matches the WorkFinishTime, then applications may choose to display the date only. Conversely when entering dates without specifying time, applications may automatically append the WorkFinishTime."@en , "作業が終了するスケジュールのデフォルト時刻。"@ja-JP ;
        rdfs:label             "workFinishTime"@en , "作業終了時間"@ja-JP ;
        rdfs:range             xsd:time ;
        schema:domainIncludes  <https://w3id.org/product/WorkControl> .

props:fullLoadRatioCurve
        a                      owl:DatatypeProperty ;
        rdfs:comment           "Ratio of actual power to full load power as a quadratic function of part load, at certain condensing and evaporating temperature, FracFullLoadPower = f ( PartLoadRatio)."@en , "Rapport entre la puissance instantanée et la puissance à pleine charge comme fonction quadratique de charge partielle, pour une certaine température de condensation et une température d'évaporation, FracFullLoadPower= f (CoefficientChargePartielle)"@fr-FR ;
        rdfs:label             "fullLoadRatioCurve"@en , "CourbeFonctionnementPleineCharge"@fr-FR ;
        schema:domainIncludes  <https://w3id.org/product/Chiller> .

props:d  a                     owl:DatatypeProperty ;
        rdfs:comment           "Measure d according to ISO 2553"@en ;
        rdfs:label             "d"@en ;
        rdfs:range             <https://w3id.org/product/PositiveLengthMeasure> ;
        schema:domainIncludes  <https://w3id.org/product/Fastener%2FWELD> .

props:spaceHumidity  a         owl:DatatypeProperty ;
        rdfs:comment           "Humidity of the space or zone that is required from user/designer view point.  If no summer or winter space humidity requirements are given, it applies all year, otherwise for the intermediate period. Provide this property, if no humidity range (Min-Max) is available."@en , "Humidité relative de l'espace ou de la zone spécifiée par l'usager ou le concepteur. Si les valeurs pour l'été et l'hiver ne sont pas connues, cette température s'applique toute l'année, sinon seulement en demi-saison. A fournir si les valeurs maximale et minimale ne sont pas connues."@fr-FR , "Geforderte Luftfeuchtigkeit für diesen Raum, gilt als ganzjährige Anforderung unabhängig vom Heizungs-, oder Kühlungsfall. Es wird angegeben, wenn kein geforderter Luftfeuchtigkeitsbereich (Min - Max)  vorhanden ist."@de-DE , "空間またはゾーンの湿度。利用者/設計者の視点から要求される。もし夏季または冬季の室内湿度要求が与えられないと、それは通年に、さもなければ中間季に適用される。"@ja-JP ;
        rdfs:label             "Humidité relative"@fr-FR , "室内湿度"@ja-JP , "Luftfeuchtigkeit"@de-DE , "spaceHumidity"@en ;
        rdfs:range             <https://w3id.org/product/RatioMeasure> ;
        schema:domainIncludes  <https://w3id.org/product/cSpatialZone> , <https://w3id.org/product/cZone> , <https://w3id.org/product/Space> .

props:riskRating  a            owl:DatatypeProperty ;
        rdfs:comment           "A general rating of the risk that may be determined from a combination of the risk assessment and risk consequence."@en ;
        rdfs:label             "riskRating"@en ;
        schema:domainIncludes  <https://w3id.org/product/Process> .

props:finalResistance
        a                      owl:DatatypeProperty ;
        rdfs:comment           "Filter fluid resistance when replacement is required (i.e., Pressure drop at the maximum air flowrate across the filter when the filter needs replacement per ASHRAE Standard 52.1)."@en ;
        rdfs:label             "finalResistance"@en ;
        rdfs:range             <https://w3id.org/product/PressureMeasure> ;
        schema:domainIncludes  <https://w3id.org/product/Filter> .

props:correctionFactorForHeating
        a                      owl:DatatypeProperty ;
        rdfs:comment           "Correction factor k as a function of water flow rate (used to calculate heating capacity)."@en ;
        rdfs:label             "correctionFactorForHeating"@en ;
        schema:domainIncludes  <https://w3id.org/product/CooledBeam> .

props:minimumHeight  a         owl:DatatypeProperty ;
        rdfs:comment           "The minimum duct height for rectangular, oval or round duct."@en , "矩形、円形或いは楕円形ダクトの最小高さ。"@ja-JP , "사각형, 원형 또는 타원형 덕트의 최소 높이입니다."@ko-KR ;
        rdfs:label             "minimumHeight"@en , "最小高さ"@ja-JP , "최소 높이"@ko-KR ;
        rdfs:range             <https://w3id.org/product/PositiveLengthMeasure> ;
        schema:domainIncludes  <https://w3id.org/product/DistributionSystem%2FVENTILATION> .

props:showerHeadDescription
        a                      owl:DatatypeProperty ;
        rdfs:comment           "A description of the shower head(s) that emit the spray of water."@en , "シャワーヘッドが排出する水の放射の表現。"@ja-JP ;
        rdfs:label             "showerHeadDescription"@en , "シャワーヘッド表現"@ja-JP ;
        rdfs:range             xsd:string ;
        schema:domainIncludes  <https://w3id.org/product/SanitaryTerminal%2FSHOWER> .

props:compressorTotalHeatGain
        a                      owl:DatatypeProperty ;
        rdfs:comment           "Compressor total heat gain."@en , "Gain thermique total au niveau du compresseur."@fr-FR ;
        rdfs:label             "compressorTotalHeatGain"@en , "GainThermiqueTotalCompresseur"@fr-FR ;
        schema:domainIncludes  <https://w3id.org/product/Compressor> .

props:fireRiskFactor  a        owl:DatatypeProperty ;
        rdfs:comment           "地域の建築規則に従って空間に割り当てられた火災危険要因\n火災のいくつかのレベルにおける空間の火災危険度を定義する。"@ja-JP , "Fire Risk factor assigned to the space according to local building regulations. It defines the fire risk of the space at several levels of fire hazard."@en , "지역 건축 규칙에 따라 공간에 할당된 화재 위험 요인 화재 어느 정도의 공간의 화재 위험도를 정의한다. \""@ko-KR , "Facteur de risque incendie attribué à l'espace, selon la réglementation locale en matière de construction."@fr-FR , "Brandgefahrenklasse des Raums, angegeben nach der nationalen oder regionalen Brandschutzverordnung."@de-DE ;
        rdfs:label             "火災危険度要因"@ja-JP , "화재 위험 요인"@ko-KR , "fireRiskFactor"@en , "Brandgefahrenklasse"@de-DE , "FacteurRisqueIncendie"@fr-FR ;
        rdfs:range             xsd:string ;
        schema:domainIncludes  <https://w3id.org/product/cSpatialZone> , <https://w3id.org/product/Space> , <https://w3id.org/product/cZone> .

props:isolatingPurpose
        a                      owl:DatatypeProperty ;
        rdfs:comment           "Defines the purpose for which the isolating valve is used since the way in which the valve is identified as an isolating valve may be in the context of its use. Note that unless there is a contextual name for the isolating valve (as in the case of a Landing Valve on a rising fire main), then the value assigned shoulkd be UNSET."@en , "その使用の前後関係から遮断弁として使われる弁があるようであれば、遮断弁が使われている理由を定義します。\n注：燃え上がる火の上のランディング弁のように、遮断弁に前後関係から別な名前がつく場合は別です。このようなとき値は定まらない。"@ja-JP ;
        rdfs:label             "isolatingPurpose"@en , "遮断目的"@ja-JP ;
        schema:domainIncludes  <https://w3id.org/product/Valve%2FISOLATING> .

props:moldingHeight  a         owl:DatatypeProperty ;
        rdfs:comment           "Height of the molding.\n\nThe height information is provided in absence of an IfcCovering (type=MOLDING) object with own shape representation and material assignment. In case of inconsistency the height assigned to IfcCovering elements takes precedence."@en , "Angabe der  Höhe des umlaufenden Gesims (Deckenkante). \n\nDer Höhenparameter wird übernommen, wenn kein eigenes Bekleidungsobjekt (IfcCovering mit PredefinedType = MOLDING) für das Gesims dem Raum zugeordnet ist. Bei Inkonsistenzen (wenn beides gegeben ist), hat die Höhe des zugeordneten Bekleidungsobjekts Priorität."@de-DE , "部屋の廻縁の高さ。\n\n形状表現を持つIfcCovering(type=MOLDING)オブジェクトが存在しない場合に与えられる厚さ情報。IfcCoveringの幾何形状パラメータとこのプロパティ値が一致しない場合、幾何形状パラメータの値を優先する。"@ja-JP ;
        rdfs:label             "廻縁高"@ja-JP , "Hauteur de la moulure"@fr-FR , "Höhe des Gesims"@de-DE , "moldingHeight"@en ;
        rdfs:range             <https://w3id.org/product/PositiveLengthMeasure> ;
        schema:domainIncludes  <https://w3id.org/product/Space> .

props:setPointFlow  a          owl:DatatypeProperty ;
        rdfs:comment           "The volumetric flow value to be sensed. Use IfcPropertyBoundedValue.SetPointValue to set the set point value."@en , "感知される流量。\nセットポイント値を置くために、IfcPropertyBoundedValue.SetPointValueを使用する。"@ja-JP , "감지되는 유량. 세트 포인트 값을 넣으려면, IfcPropertyBoundedValue.SetPointValue를 사용하십시오."@ko-KR ;
        rdfs:label             "setPointFlow"@en , "流量設定値"@ja-JP , "유량 설정"@ko-KR ;
        schema:domainIncludes  <https://w3id.org/product/Sensor%2FFLOWSENSOR> .

props:illuminance  a           owl:DatatypeProperty ;
        rdfs:comment           "Geforderte durchschnittliche Beleuchtungsstärke in diesem Raum."@de-DE , "Required average illuminance value for this space."@en , "이 공간을 위해 필요한 평균 조도"@ko-KR , "Valeur de l'éclairement attendu pour la pièce."@fr-FR , "領域に対しての必要とされる照度の値の平均値。"@ja-JP ;
        rdfs:label             "illuminance"@en , "조도"@ko-KR , "照度"@ja-JP , "EclairementAttendu"@fr-FR , "Beleuchtungsstärke"@de-DE ;
        rdfs:range             <https://w3id.org/product/IlluminanceMeasure> ;
        schema:domainIncludes  <https://w3id.org/product/Space> , <https://w3id.org/product/cZone> , <https://w3id.org/product/cSpatialZone> .

props:controlDamperOperation
        a                      owl:DatatypeProperty ;
        rdfs:comment           "The inherent characteristic of the control damper operation."@en ;
        rdfs:label             "controlDamperOperation"@en ;
        schema:domainIncludes  <https://w3id.org/product/Damper%2FCONTROLDAMPER> .

props:energyEfficiencyRatio
        a                      owl:DatatypeProperty ;
        rdfs:comment           "L'EER ou Energy Efficiency Ratio est le coefficient d'efficacité frigorifique, rapport entre entre l'énergie utile frigorifique divisée parénergie absorbée au compresseur.\nPar définition, l'unité est le BTU/hour par Watt.\nLa puissance électrique fournie peut être obtenue depuis Pset_DistributionPortHistoryElectrical.RealPower sur le port \"Power\"  du IfcChiller."@fr-FR , "EER, coefficient d'efficacité Thermique"@fr-FR , "The Energy efficiency ratio (EER) is the ratio of net cooling capacity to the total input rate of electric power applied.  By definition, the units are BTU/hour per Watt.\nThe input electric power may be obtained from Pset_DistributionPortPHistoryElectrical.RealPower on the 'Power' port of the IfcChiller."@en , "Energy efficiency ratio (EER)."@en ;
        rdfs:label             "CoefficientEfficacitéThermique"@fr-FR , "energyEfficiencyRatio"@en , "CoefficientEfficacitéEnergétique"@fr-FR ;
        schema:domainIncludes  <https://w3id.org/product/Chiller> , <https://w3id.org/product/Compressor> .

props:skirtingBoard  a         owl:DatatypeProperty ;
        rdfs:comment           "部屋の床の周りにある幅木の材質または施工に関するラベル（識別情報）。ラベル名は部屋リスト情報に使用される。\n\n形状表現を持つIfcCovering (type=SKIRTINGBOARD)オブジェクトが存在しない場合に与えられる材質情報。IfcCoveringの材質情報とこのプロパティ値が一致しない場合、IfcCoveringに与えられている材質情報を優先する。"@ja-JP , "Angabe des Materials für die Sockelleiste. Diese Angabe wird im Raumbuch verwendet.\n\nDie Materialangabe wird übernommen, wenn kein eigenes Bekleidungsobjekt (IfcCovering mit PredefinedType = SKIRTINGBOARD) für die Sockelleiste dem Raum zugeordnet ist. Bei Inkonsistenzen (wenn beides gegeben ist), hat die Materialangabe des zugeordneten Bekleidungsobjekts Priorität."@de-DE , "Label to indicate the material or construction of the skirting board around the space flooring. The label is used for room book information.\n\nThe material information is provided in absence of an IfcCovering (type=SKIRTINGBOARD) object with own shape representation and material assignment. In case of inconsistency the material assigned to IfcCovering elements takes precedence."@en ;
        rdfs:label             "幅木材"@ja-JP , "skirtingBoard"@en , "Sockelleiste"@de-DE , "Matériau de la plinthe"@fr-FR ;
        rdfs:range             xsd:string ;
        schema:domainIncludes  <https://w3id.org/product/Space> .

props:timeToleranceLimit1
        a                      owl:DatatypeProperty ;
        rdfs:comment           "The current limit in [x In] limiting the application of TimeTolerance1, if any. If the value is set to 0, the value of the TimeTolerance1 is valid for the whole time/current-curve."@en , "許容時間1を制限する電流制限値。\n値が0の場合は、制限はない。"@ja-JP , "허용 시간 1를 제한하는 전류 제한. 값이 0이면 제한이 없다"@ko-KR ;
        rdfs:label             "timeToleranceLimit1"@en , "許容限界時間1"@ja-JP , "허용 한계시간1"@ko-KR ;
        rdfs:range             <https://w3id.org/product/ElectricCurrentMeasure> ;
        schema:domainIncludes  <https://w3id.org/product/ProtectiveDeviceTrippingUnit> .

props:hasStrainer  a           owl:DatatypeProperty ;
        rdfs:comment           "溝の防臭弁がろ過装置を備えているかどうかの指示。"@ja-JP , "Indicates whether the gully trap has a strainer (= TRUE) or not (= FALSE)."@en , "溝の防臭弁がろ過装置を備えているかどうか指示する。"@ja-JP ;
        rdfs:label             "hasStrainer"@en , "ろ過装置"@ja-JP ;
        rdfs:range             xsd:boolean ;
        schema:domainIncludes  <https://w3id.org/product/WasteTerminal%2FGULLYTRAP> , <https://w3id.org/product/WasteTerminal%2FFLOORTRAP> .

props:energySource  a          owl:DatatypeProperty ;
        rdfs:comment           "Liste définissant les sources d'énergie ou combustibles pour générer la chaleur."@fr-FR , "列挙型はエネルギー源や燃料該当する場合は熱を発生させる燃焼定義します。注：温水循環式のヒーターはunsetを使用してはならない。デュアル使用すると、温水循環式の電気ヒーターは電気を使用しなければならない。"@ja-JP , "The source of energy."@en , "Enumeration defining the energy source or fuel combusted to generate heat if applicable.  Note: hydronic heaters shall use UNSET; dual-use hydronic/electric heaters shall use ELECTRICITY."@en , "Enumeration defining the energy source or fuel cumbusted to generate heat."@en , "加熱に使用する燃料のエネルギ種類　（石炭、石炭粉末、電気、ガス、油、プロパン、木材、木材チップ、木材ペレット、木粉、他）"@ja-JP , "エネルギー源（ディーゼル、ガソリン、天然ガス、プロパン、バイオディーゼル、下水ガス、水素、バイオ燃料、　他）"@ja-JP ;
        rdfs:label             "SourceEnergie"@fr-FR , "エネルギ種別"@ja-JP , "energySource"@en , "エネルギー源"@ja-JP , "エネルギ源"@ja-JP ;
        schema:domainIncludes  <https://w3id.org/product/SpaceHeater> , <https://w3id.org/product/Burner> , <https://w3id.org/product/Boiler> , <https://w3id.org/product/Engine> .

props:wireLoopLength  a        owl:DatatypeProperty ;
        rdfs:comment           "The length of the fastening loop part of the wire."@en , "ワイヤーの留め具部分の長さ。"@ja-JP , "와이어 클램프 부분의 길이"@ko-KR ;
        rdfs:label             "wireLoopLength"@en , "留め具長さ"@ja-JP , "클램프 길이"@ko-KR ;
        rdfs:range             <https://w3id.org/product/PositiveLengthMeasure> ;
        schema:domainIncludes  <https://w3id.org/product/DiscreteAccessory%2FWire%20loop> .

props:heatExchangeSurfaceArea
        a                      owl:DatatypeProperty ;
        rdfs:comment           "Heat exchange surface area associated with U-value."@en , "Surface d'échange thermique associé à la valeur U."@fr-FR ;
        rdfs:label             "heatExchangeSurfaceArea"@en , "SurfaceEchangeThermique"@fr-FR ;
        rdfs:range             <https://w3id.org/product/AreaMeasure> ;
        schema:domainIncludes  <https://w3id.org/product/Coil> .

props:returnAirFractionRange
        a                      owl:DatatypeProperty ;
        rdfs:comment           "Allowable return air fraction range as a fraction of discharge airflow."@en , "送風量の一部としての許容還気風量"@ja-JP , "Plage possiblede la fraction d'air repris en tant que fraction de l'air rejeté"@fr-FR ;
        rdfs:label             "returnAirFractionRange"@en , "還気風量比"@ja-JP , "Plage pour la fraction d'air repris"@fr-FR ;
        schema:domainIncludes  <https://w3id.org/product/AirTerminalBox> .

props:power  a                 owl:DatatypeProperty ;
        rdfs:comment           "The actual power consumption of the pump."@en , "The actual power and operable range."@en , "ポンプの実動力消費"@ja-JP , "実電力と動作可能範囲。"@ja-JP ;
        rdfs:label             "power"@en , "動力"@ja-JP , "電力"@ja-JP ;
        schema:domainIncludes  <https://w3id.org/product/DistributionPort%2FELECTRICAL> , <https://w3id.org/product/Pump> .

props:discontinuedHeating
        a                      owl:DatatypeProperty ;
        rdfs:comment           "Anfoderung, ob der Raum durch eine diskontinuierliche Heizung versorgt werden soll (WAHR) oder nicht (FALSCH)."@de-DE , "Indique si un chauffage intermittent est requis ou souhaité par l'usager ou le concepteur (VRAI) ou non (FAUX)."@fr-FR , "Indication whether discontinued heating is required/desirable from user/designer view point. (TRUE) if yes, (FALSE) otherwise."@en , "불연속 난방이 이용자 / 설계자의 관점에서 요청 / 요구되는지 여부를 나타내는 부울 값입니다. (TRUE) 필요 (FALSE) 불필요."@ko-KR , "不連続暖房が利用者/設計者の視点から要求/要望されるかどうかを示すブーリアン値。(TRUE)要、(FALSE)不要。"@ja-JP ;
        rdfs:label             "不連続暖房"@ja-JP , "불연속 난방"@ko-KR , "Diskontinuierliche Heizung"@de-DE , "Chauffage intermittent"@fr-FR , "discontinuedHeating"@en ;
        rdfs:range             xsd:boolean ;
        schema:domainIncludes  <https://w3id.org/product/cZone> , <https://w3id.org/product/cSpatialZone> , <https://w3id.org/product/Space> .

props:pressureClass  a         owl:DatatypeProperty ;
        rdfs:comment           "Pressure classification as defined by the authority having jurisdiction (e.g., SMACNA, etc.)."@en , "Nominal pressure rating of the system components. (Data type = PressureMeasure)"@en , "The test or rated pressure classification of the fitting."@en , "덕트 시스템 각 부위의 압력 등급 (측정된 압력)"@ko-KR , "管轄権を持つ当局（SMACNAなど）によって定義された圧力分類"@ja-JP , "ダクトシステム各部位の圧力等級（計測した圧力）。"@ja-JP , "継ぎ手接合部の圧力等級？"@ja-JP ;
        rdfs:label             "pressureClass"@en , "圧力分類"@ja-JP , "圧力クラス"@ja-JP , "圧力等級"@ja-JP , "압력 등급"@ko-KR ;
        rdfs:range             <https://w3id.org/product/PressureMeasure> ;
        schema:domainIncludes  <https://w3id.org/product/PipeFitting> , <https://w3id.org/product/DistributionSystem%2FVENTILATION> , <https://w3id.org/product/DuctFitting> .

props:shape  a                 owl:DatatypeProperty ;
        rdfs:comment           "断面形状：\nこの形状は直管を通じて一定である。変形する形状のためには、かわりに変形継手が使用される。（フラットオーバル、角型、丸型　他）"@ja-JP , "Forme du terminal de ventilation. La fente est généralement un long et étroit appareil d'apport avec un rapport de forme généralement supérieur à 10 pour 1."@fr-FR , "空間の形状を定義します。少なくとも「四角形」、「円」、「未定義」の値を含みます。"@ja-JP , "Anforderung an die Form des Durchbruchs, vordefinierte Werte sind \"Rechteck\", \"Rund\", und \"Nicht definiert\"."@de-DE , "도체의 형상을 표시합니다."@ko-KR , "The shape form of the provision for void, the minimum set of agreed values includes 'Rectangle', 'Round', and 'Undefined'."@en , "空构件的形状，当前得到认可的值至少包括“矩形”、“圆形”及“未定义”。"@zh-CN , "La forme de la réservation. L'ensemble des valeurs autorisées contient au moins \"Rectangle\", \"Round\" et \"Undefined\"."@fr-FR , "Indication of the shape of the conductor."@en , "Cross sectional shape. Note that this shape is uniform throughout the length of the segment. For nonuniform shapes, a transition fitting should be used instead."@en , "ターミナルの形状（円状、四角形、正方形、スロット他）。　スロット（溝状）は一般的にアスペクト比１０以上が典型的である。"@ja-JP , "導体の形状を表示。"@ja-JP , "Shape of the air terminal. Slot is typically a long narrow supply device with an aspect ratio generally greater than 10 to 1."@en ;
        rdfs:label             "Form"@de-DE , "형상"@ko-KR , "Forme"@fr-FR , "shape"@en , "形状"@zh-CN , "形状"@ja-JP ;
        rdfs:range             xsd:string ;
        schema:domainIncludes  <https://w3id.org/product/AirTerminal> , <https://w3id.org/product/BuildingElementProxy%2FPROVISIONFORVOID> , <https://w3id.org/product/DuctSegment> , <https://w3id.org/product/CableSegment%2FCONDUCTORSEGMENT> .

props:surface1  a              owl:DatatypeProperty ;
        rdfs:comment           "Aspect of weld seam surface, i.e. 'plane', 'curved' or 'hollow'.  Combined welds are given by two corresponding symbols analogous to Type1 and Type2."@en ;
        rdfs:label             "surface1"@en ;
        rdfs:range             xsd:string ;
        schema:domainIncludes  <https://w3id.org/product/Fastener%2FWELD> .

props:prevailingWindVelocity
        a                      owl:DatatypeProperty ;
        rdfs:comment           "The design wind velocity coming from the direction specified by the PrevailingWindDirection attribute."@en , "PrevailingWindDirection 属性に示された風向から来た卓越風の風速。"@ja-JP , "PrevailingWindDirection 속성에 지정된 풍향 온 탁월한 바람 바람."@ko-KR ;
        rdfs:label             "prevailingWindVelocity"@en , "卓越風の風速"@ja-JP , "탁월한 바람의 풍속"@ko-KR ;
        rdfs:range             <https://w3id.org/product/LinearVelocityMeasure> ;
        schema:domainIncludes  <https://w3id.org/product/Building> .

props:firstCurvatureRadius
        a                      owl:DatatypeProperty ;
        rdfs:comment           "FirstCurvatureRadius should be defined as the base or left side radius of curvature value."@en , "最初の曲率半径は、基本又は曲率の値の左側の半径として定義する必要があります。"@ja-JP ;
        rdfs:label             "firstCurvatureRadius"@en , "最初の曲率半径"@ja-JP ;
        rdfs:range             <https://w3id.org/product/PositiveLengthMeasure> ;
        schema:domainIncludes  <https://w3id.org/product/Tank%2FPREFORMED> , <https://w3id.org/product/Tank> .

props:concealedCeiling
        a                      owl:DatatypeProperty ;
        rdfs:comment           "Indication whether this space is designed to have a concealed flooring space (TRUE) or not (FALSE). A concealed ceiling space is normally meant to be the space between a slab and a ceiling."@en , "Angabe, ob dieser Raum mit einer Installationsdecke (abhehängten Decke) ausgestattet ist (JA), oder nicht (NEIN)."@de-DE , "Indique si la pièce comprend un faux plafond (VRAI) ou non (FAUX)"@fr-FR , "この部屋（空間）が隠蔽された天井空間を持つように設計されているかどうかを示すブーリアン値。隠蔽された天井空間とは、スラブと天井の間の空間。"@ja-JP ;
        rdfs:label             "隠蔽天井"@ja-JP , "concealedCeiling"@en , "FauxPlafond"@fr-FR , "Installationsdecke"@de-DE ;
        rdfs:range             xsd:boolean ;
        schema:domainIncludes  <https://w3id.org/product/Space> .

props:centerCoreSpacing
        a                      owl:DatatypeProperty ;
        rdfs:comment           "Center core spacing of the profile."@en ;
        rdfs:label             "centerCoreSpacing"@en ;
        rdfs:range             <https://w3id.org/product/PositiveLengthMeasure> ;
        schema:domainIncludes  <https://w3id.org/product/ArbitraryProfileDefWithVoids> .

props:inPlane  a               owl:DatatypeProperty ;
        rdfs:comment           "Mechanical properties with respect to in-plane load, i.e. for function as a membrane."@en , "Mechanical properties with respect to in-plane load, i.e. bending about the strong axis; tension zone of unbalanced layups is stressed in tension."@en ;
        rdfs:label             "inPlane"@en ;
        schema:domainIncludes  <https://w3id.org/product/Material%2FWood> .

props:numberOfLiveConductors
        a                      owl:DatatypeProperty ;
        rdfs:comment           "Number of live conductors within this circuit. Either this property or the ConductorFunction property (if only one) may be asserted."@en ;
        rdfs:label             "numberOfLiveConductors"@en ;
        rdfs:range             xsd:int ;
        schema:domainIncludes  <https://w3id.org/product/DistributionSystem%2FELECTRICAL> .

props:fractionConvectiveHeatTransfer
        a                      owl:DatatypeProperty ;
        rdfs:comment           "Fraction of the total heat transfer rate as the convective heat transfer."@en , "総合熱移動の内対流射熱移動とみなされる部分"@ja-JP ;
        rdfs:label             "fractionConvectiveHeatTransfer"@en , "対流熱移動フラクション"@ja-JP ;
        schema:domainIncludes  <https://w3id.org/product/SpaceHeater> .

props:setPointMovement
        a                      owl:DatatypeProperty ;
        rdfs:comment           "The movement to be sensed."@en ;
        rdfs:label             "setPointMovement"@en ;
        schema:domainIncludes  <https://w3id.org/product/Sensor%2FMOVEMENTSENSOR> .

props:actualCompletion
        a                      owl:DatatypeProperty ;
        rdfs:comment           "The actual completion percentage of the allocation."@en , "実績の完了率。"@ja-JP ;
        rdfs:label             "actualCompletion"@en , "実績完了率"@ja-JP ;
        schema:domainIncludes  <https://w3id.org/product/ConstructionResource> .

props:moistureCapacityThermalGradient
        a                      owl:DatatypeProperty ;
        rdfs:comment           "Thermal gradient coefficient for moisture capacity. Based on water vapor density."@en ;
        rdfs:label             "moistureCapacityThermalGradient"@en ;
        rdfs:range             xsd:decimal ;
        schema:domainIncludes  <https://w3id.org/product/Material> .

props:hasSoundAttenuator
        a                      owl:DatatypeProperty ;
        rdfs:comment           "Terminal box has a sound attenuator."@en , "ターミナルに消音があるか否か　（あればTRUE)"@ja-JP , "If TRUE, the air terminal has sound attenuation."@en , "Si VRAI, le terminal de ventilation possède une correction acoustique."@fr-FR , "Le registre terminal possède une correction acoustique"@fr-FR , "ターミナルに消音が付いている場合に真"@ja-JP ;
        rdfs:label             "hasSoundAttenuator"@en , "消音有無"@ja-JP , "Possède correction acoustique"@fr-FR , "PossèdeCorrectionAcoustique"@fr-FR ;
        rdfs:range             xsd:boolean ;
        schema:domainIncludes  <https://w3id.org/product/AirTerminalBox> , <https://w3id.org/product/AirTerminal> .

props:distanceBetweenParallelCircuits
        a                      owl:DatatypeProperty ;
        rdfs:comment           "Distance measured between parallel circuits."@en ;
        rdfs:label             "distanceBetweenParallelCircuits"@en ;
        rdfs:range             <https://w3id.org/product/LengthMeasure> ;
        schema:domainIncludes  <https://w3id.org/product/CableSegment> .

props:pipeConnectionEnum
        a                      owl:DatatypeProperty ;
        rdfs:comment           "The manner in which the pipe connection is made to the cooled beam."@en ;
        rdfs:label             "pipeConnectionEnum"@en ;
        schema:domainIncludes  <https://w3id.org/product/CooledBeam> .

props:spaceHumiditySummer
        a                      owl:DatatypeProperty ;
        rdfs:comment           "Geforderte Luftfeuchtigkeit für diesen Raum für die Auslegung der Kühlung."@de-DE , "Humidité relative maximale de l'espace ou de la zone  en été. Spécifiée par l'usager ou le concepteur et utilisée comme consigne pour le refroidissement."@fr-FR , "Humidity of the space or zone for the hot (summer) period, that is required from user/designer view point and provided as requirement for cooling."@en , "空間またはゾーンの暑熱季(夏季)の室内湿度。利用者/設計者の視点から要求される。"@ja-JP , "공간이나 영역 혹서 계절 (여름) 실내 습도. 이용자 / 설계자의 관점에서 요구된다."@ko-KR ;
        rdfs:label             "여름철실내 습도"@ko-KR , "Luftfeuchtigkeit Kühlung"@de-DE , "Humidité relative maximale en été"@fr-FR , "spaceHumiditySummer"@en , "夏季室内湿度"@ja-JP ;
        rdfs:range             <https://w3id.org/product/RatioMeasure> ;
        schema:domainIncludes  <https://w3id.org/product/Space> , <https://w3id.org/product/cSpatialZone> , <https://w3id.org/product/cZone> .

props:counterSlope  a          owl:DatatypeProperty ;
        rdfs:comment           "构件的垂线相对于水平（0.0度）方向的坡度角。\n当前设计方案确定的通道行走方向的垂线方向的最大坡度。\n该属性所提供的形状信息是对内部形状描述和几何参数的补充。如果几何参数与该属性所提供的形状属性不符，应以几何参数为准。"@zh-CN , "Sloping angle of the object, measured perpendicular to the slope  - relative to horizontal (0.0 degrees). \nActual maximum slope for the passageway measured perpendicular to the direction of travel according to the current design. The shape information is provided in addition to the shape representation and the geometric parameters used within. In cases of inconsistency between the geometric parameters and the shape properties, provided in the attached property, the geometric parameters take precedence. \nNote: new property in IFC4."@en , "German-description-5"@de-DE , "Angle d'inclinaison de l'objet, mesuré perpendiculairement à la pente. L'horizontale correspond à la valeur 0 degrés. Valeur maximale de la pente de la rampe actuellement projetée, mesurée perpendiculairement à la direction du passage. Cette propriété est donnée en complément de la représentation de la forme de l'élément et des paramètres géométriques qui la déterminent. En cas d'incohérence entre ces paramètres géométriques et cette propriété, ce sont les paramètres géométriques qui priment. Note : nouvelle propriété de la version IFC2x4."@fr-FR , "オブジェクトの傾斜角度（垂直との角度）\n通路のための実際の最大の傾斜は、現在の設計による旅行の方向への垂直を測定しました。形情報は、内側は使用される形表現および幾何学的媒介変数に加えて提供されます。幾何学的媒介変数と形特性の間の矛盾の場合では、付属の特性の中で提供されて、幾何学的媒介変数は先行をとります。\n注:IFC2x4の中の新しいプロパティ"@ja-JP ;
        rdfs:label             "Gegenneigung"@de-DE , "通路の傾斜角度(垂直との角度）"@ja-JP , "ContrePente"@fr-FR , "反向坡度"@zh-CN , "counterSlope"@en ;
        rdfs:range             <https://w3id.org/product/PlaneAngleMeasure> ;
        schema:domainIncludes  <https://w3id.org/product/RampFlight> .

props:measuredFlowRate
        a                      owl:DatatypeProperty ;
        rdfs:comment           "The rate of flow of a fluid measured across the valve."@en , "バルブを通過する流体の計測された流量"@ja-JP ;
        rdfs:label             "measuredFlowRate"@en , "計測流量"@ja-JP ;
        schema:domainIncludes  <https://w3id.org/product/Valve> .

props:marketSubCategoriesAvailableNow
        a                      owl:DatatypeProperty ;
        rdfs:comment           "A list of the sub categories of property that are currently available expressed in terms of IfcLabel."@en , "Liste de sous catégories actuellement disponibles"@fr-FR ;
        rdfs:label             "marketSubCategoriesAvailableNow"@en , "DisponibilitesActuellesParSousCategories"@fr-FR ;
        schema:domainIncludes  <https://w3id.org/product/Building> .

props:partLoadRatio  a         owl:DatatypeProperty ;
        rdfs:comment           "Ratio of the real to the nominal capacity."@en , "設計容量との比"@ja-JP , "Ratio entre capacité effective et capacité nominale"@fr-FR ;
        rdfs:label             "partLoadRatio"@en , "部分負荷比"@ja-JP , "Taux de charge"@fr-FR ;
        schema:domainIncludes  <https://w3id.org/product/Boiler> .

props:totalArea  a             owl:DatatypeProperty ;
        rdfs:comment           "Surface totale brute. Définie en phase de programmation."@fr-FR , "부지에 대한 총 계획 면적. 호텔 공간 계획에 사용됩니다."@ko-KR , "Total planned area for the site. Used for programming the site space."@en , "Gesamte Grundstücksfläche für diese Bauaufgabe."@de-DE , "敷地にたいする延べ計画面積。敷地空間の計画に使用。"@ja-JP ;
        rdfs:label             "연면적"@ko-KR , "Bruttogrundstücksfläche"@de-DE , "totalArea"@en , "SurfaceBruteProgrammee"@fr-FR , "延べ面積"@ja-JP ;
        rdfs:range             <https://w3id.org/product/AreaMeasure> ;
        schema:domainIncludes  <https://w3id.org/product/Site> .

props:cloggingIndicator
        a                      owl:DatatypeProperty ;
        rdfs:comment           "Whether the filter has an indicator to display the degree of clogging of the filter."@en ;
        rdfs:label             "cloggingIndicator"@en ;
        rdfs:range             xsd:boolean ;
        schema:domainIncludes  <https://w3id.org/product/Filter%2FCOMPRESSEDAIRFILTER> .

props:xDirectionUpperBarCount
        a                      owl:DatatypeProperty ;
        rdfs:comment           "The number of bars with X direction upper bar."@en , "X方向の上端筋本数。"@ja-JP ;
        rdfs:label             "xDirectionUpperBarCount"@en , "X方向上端筋本数"@ja-JP ;
        rdfs:range             xsd:int ;
        schema:domainIncludes  <https://w3id.org/product/Footing> .

props:breakerUnitCurve
        a                      owl:DatatypeProperty ;
        rdfs:comment           "A curve that establishes the let through energy of a breaker unit when a particular prospective current is applied.  Note that the breaker unit curve is defined within a Cartesian coordinate system and this fact must be asserted within the property set:\n\n(1) Defining value: ProspectiveCurrent: A list of minimum 2 and maximum 16 numbers providing the currents in [A] for points in the current/I2t log/log coordinate space. The curve is drawn as a straight line between two consecutive points.\n(2) Defined value: LetThroughEnergy: A list of minimum 2 and maximum 16 numbers providing the let-through energy, I2t, in [A2s] for points in the current/I2t log/log coordinate space. The curve is drawn as a straight line between two consecutive points."@en , "適用された電流と通過する遮断機のエネルギーを示した曲線\n （1）定義値：ProspectiveCurrent（固有電流）：\n   電流/I2tで示される最小2から最大8のリストで電流[A]を定義します。\n   カーブが連続する2つの点を結ぶ直線として描かれています。\n\n\n （2）定義値：LetThroughEnergy：\n   電流/I2tで示される最小2から最大8のリストで通過エネルギー電流[[A2s]を定義します。\n   カーブが連続する2つの点を結ぶ直線として描かれています。"@ja-JP , "적용된 전류 통과 차단기의 에너지를 나타낸 곡선  (1) 정의 값 : ProspectiveCurrent (고유 전류) :    전류 / I2t에 표시된 최소 2에서 최대 8 개의 목록에서 전류 [A]를 정의합니다.    커브가 연속되는 두 개의 점을 연결하는 직선으로 그려져 있습니다.  (2) 정의 값 : LetThroughEnergy :    전류 / I2t에 표시된 최소 2에서 최대 8 개의 목록에서 통과 에너지 전류 [A2s을 정의합니다.    커브가 연속되는 두 개의 점을 연결하는 직선으로 그려져 있습니다."@ko-KR ;
        rdfs:label             "breakerUnitCurve"@en , "遮断機曲線"@ja-JP , "차단기 곡선"@ko-KR ;
        schema:domainIncludes  <https://w3id.org/product/ProtectiveDevice> .

props:purpose  a               owl:DatatypeProperty ;
        rdfs:comment           "Indication du motif de l'ouverture (ventilation, accès, etc.)."@fr-FR , "Indication of the purpose for that opening, e.g. 'ventilation', 'access', etc."@en , "開口の目的を示す文字列。例：\"ventilation\"（換気）、\"access\"（通行）など。"@ja-JP , "Enumeration defining the purpose of the flow meter occurrence."@en ;
        rdfs:label             "Motif"@fr-FR , "目的"@ja-JP , "purpose"@en ;
        rdfs:range             xsd:string ;
        schema:domainIncludes  <https://w3id.org/product/OpeningElement> , <https://w3id.org/product/FlowMeter> .

props:setPointLevel  a         owl:DatatypeProperty ;
        rdfs:comment           "The fill level value to be sensed. Use IfcPropertyBoundedValue.SetPointValue to set the set point value."@en , "感知されるレベル。\nセットポイント値を置くために、IfcPropertyBoundedValue.SetPointValueを使用する。"@ja-JP , "감지되는 수준. 세트 포인트 값을 넣으려면, IfcPropertyBoundedValue.SetPointValue를 사용하십시오."@ko-KR ;
        rdfs:label             "setPointLevel"@en , "レベル設定値"@ja-JP , "레벨 설정"@ko-KR ;
        schema:domainIncludes  <https://w3id.org/product/Sensor%2FLEVEL> .

props:hasSoundAttenuation
        a                      owl:DatatypeProperty ;
        rdfs:comment           "TRUE if the coil has sound attenuation, FALSE if it does not."@en , "VRAI si la batterie possède une correction acoustique, FAUX si ce n'est pas le cas."@fr-FR ;
        rdfs:label             "hasSoundAttenuation"@en , "PossedeCorrectionAcoustique"@fr-FR ;
        rdfs:range             xsd:boolean ;
        schema:domainIncludes  <https://w3id.org/product/Coil> .

props:roadVisibleDistanceLeft
        a                      owl:DatatypeProperty ;
        rdfs:comment           "Distance visible to the left of the access."@en , "Distance de visibilité à la gauche de l'accès."@fr-FR , "左側の経路に可視出来る距離。"@ja-JP ;
        rdfs:label             "roadVisibleDistanceLeft"@en , "DistanceVisibiliteCoteGauche"@fr-FR , "左側道路可視距離"@ja-JP ;
        rdfs:range             <https://w3id.org/product/PositiveLengthMeasure> ;
        schema:domainIncludes  <https://w3id.org/product/Annotation%2FLineOfSight> .

props:assetTaxType  a          owl:DatatypeProperty ;
        rdfs:comment           "Identifies the predefined types of taxation group from which the type required may be set."@en , "税の定義済み種別。"@ja-JP ;
        rdfs:label             "assetTaxType"@en , "資産税種別"@ja-JP ;
        schema:domainIncludes  <https://w3id.org/product/Asset> .

props:gullyType  a             owl:DatatypeProperty ;
        rdfs:comment           "設置する予定の溝をあらかじめ定義でタイプを確認します。"@ja-JP , "Identifies the predefined types of gully from which the type required may be set."@en , "必要とされるタイプがセットされる溝の定義されたタイプを確認してください。"@ja-JP ;
        rdfs:label             "防臭弁の種類"@ja-JP , "gullyType"@en , "溝種類"@ja-JP ;
        schema:domainIncludes  <https://w3id.org/product/WasteTerminal%2FGULLYTRAP> , <https://w3id.org/product/WasteTerminal%2FGULLYSUMP> .

props:visibleReflectanceFront
        a                      owl:DatatypeProperty ;
        rdfs:comment           "Reflectance at normal incidence (visible): front side. Defines the fraction of the solar ray in the visible spectrum that is reflected and not transmitted when the ray passes from one medium into another, at the \"front\" side of the other material, perpendicular to the surface. Dependent on material and surface characteristics."@en ;
        rdfs:label             "visibleReflectanceFront"@en ;
        rdfs:range             <https://w3id.org/product/PositiveRatioMeasure> ;
        schema:domainIncludes  <https://w3id.org/product/Material> .

props:centerlineAirVelocity
        a                      owl:DatatypeProperty ;
        rdfs:comment           "Centerline air velocity versus distance from the diffuser and temperature differential; a function of distance from diffuser and temperature difference between supply air and room air."@en , "吹出口かからの距離と温度差に対する中心速度、\n給気と室内空気の間の吹出口かからの距離と温度差の関数"@ja-JP , "Vitesse de l'air en axe central de jet par rapport à la distance entre le diffuseur et la température différentielle; une fonction de la distance entre le diffuseur et la différence de température entre celui de l'air fourni et celui de l'air de la pièce."@fr-FR ;
        rdfs:label             "centerlineAirVelocity"@en , "中心空気速度"@ja-JP , "Vitesse de l'air en axe central de jet"@fr-FR ;
        schema:domainIncludes  <https://w3id.org/product/AirTerminal> .

props:spaceHumidityMax
        a                      owl:DatatypeProperty ;
        rdfs:comment           "공간 또는 영역의 습도. 이용자 / 설계자의 관점에서 요구된다. 만약 여름철 또는 겨울철 실내 습도 요구가 주어지지 않는, 그것은 연중에, 그렇지 않으면 중간 분기별로 적용된다."@ko-KR , "Maximal geforderte Luftfeuchtigkeit für diesen Raum, gilt als ganzjährige Anforderung unabhängig vom Heizungs-, oder Kühlungsfall."@de-DE , "空間またはゾーンの最高湿度。利用者/設計者の視点から要求される。もし夏季または冬季の室内湿度要求が与えられないと、それは通年に、さもなければ中間季に適用される。"@ja-JP , "Humidité relative maximale de l'espace ou de la zone spécifiée par l'usager ou le concepteur. Si les valeurs pour l'été et l'hiver ne sont pas connues, cette température s'applique toute l'année, sinon seulement en demi-saison."@fr-FR , "Maximal permitted humidity of the space or zone that is required from user/designer view point.  If no summer or winter space humidity requirements are given, it applies all year, otherwise for the intermediate period."@en ;
        rdfs:label             "실내습도"@ko-KR , "spaceHumidityMax"@en , "最高室内湿度"@ja-JP , "Humidité relative maximale"@fr-FR , "Luftfeuchtigkeit Maximal"@de-DE ;
        rdfs:range             <https://w3id.org/product/RatioMeasure> ;
        schema:domainIncludes  <https://w3id.org/product/cZone> , <https://w3id.org/product/Space> , <https://w3id.org/product/cSpatialZone> .

props:inUseConditions
        a                      owl:DatatypeProperty ;
        rdfs:comment           "Adjustment of the service life resulting from the effect of the conditions in which components are operating."@en ;
        rdfs:label             "inUseConditions"@en ;
        schema:domainIncludes  <https://w3id.org/product/System> .

props:shortCircuit2PoleMinimumState
        a                      owl:DatatypeProperty ;
        rdfs:comment           "Minimum 2 pole short circuit current provided at the point of supply."@en , "電源供給時点の2極最小短絡電流。"@ja-JP , "전원 공급 시점의 양극 최소 단락 전류."@ko-KR ;
        rdfs:label             "shortCircuit2PoleMinimumState"@en , "2極最小短絡電流"@ja-JP , "2 극 최소 단락 전류"@ko-KR ;
        rdfs:range             <https://w3id.org/product/ElectricCurrentMeasure> ;
        schema:domainIncludes  <https://w3id.org/product/ElectricFlowStorageDevice> .

props:atmosphericAcidificationPerUnit
        a                      owl:DatatypeProperty ;
        rdfs:comment           "SO2で計算される大気の酸性化に影響するガスの量。"@ja-JP , "SO2에 해당 환산된 대기 산성 화의 원인이되는 가스량"@ko-KR , "Quantity of gases responsible for the atmospheric acidification calculated in equivalent SO2"@en , "Quantité de gaz responsables de l'acidification atmosphérique exprimée en Kg d'équivalent SO2 [NDT : selon les normes PrEN15804:2008 et NF P01-010]."@fr-FR ;
        rdfs:label             "단위당 대기 산성화"@ko-KR , "AcidificationAtmospheriqueParUnite"@fr-FR , "atmosphericAcidificationPerUnit"@en , "単位あたり大気酸性化"@ja-JP ;
        rdfs:range             <https://w3id.org/product/MassMeasure> ;
        schema:domainIncludes  <https://w3id.org/product/Element> .

props:faceSurfaceArea
        a                      owl:DatatypeProperty ;
        rdfs:comment           "Face area of filter frame."@en ;
        rdfs:label             "faceSurfaceArea"@en ;
        rdfs:range             <https://w3id.org/product/AreaMeasure> ;
        schema:domainIncludes  <https://w3id.org/product/Filter%2FAIRPARTICLEFILTER> .

props:stratosphericOzoneLayerDestructionPerUnit
        a                      owl:DatatypeProperty ;
        rdfs:comment           "Quantité de gaz destructeurs de la couche d'ozone exprimée en équivalent CFC-R11 tels que définis dans la norme  ISO21930:2007 [NDT : et dans la norme NF P01-010]"@fr-FR , "CFC-R11에 해당 환산된 성층권 오존층 파괴 가스량"@ko-KR , "CFC-R11で計算される成層圏のオゾン層を破壊するガスの量。"@ja-JP , "Quantity of gases destroying the stratospheric ozone layer calculated in equivalent CFC-R11"@en ;
        rdfs:label             "단위당 성층권 오존층 파괴"@ko-KR , "stratosphericOzoneLayerDestructionPerUnit"@en , "単位あたり成層圏オゾン層破壊"@ja-JP , "DestructionCoucheOzoneStartospheriqueParUnite"@fr-FR ;
        rdfs:range             <https://w3id.org/product/MassMeasure> ;
        schema:domainIncludes  <https://w3id.org/product/Element> .

props:response  a              owl:DatatypeProperty ;
        rdfs:comment           "Identifies the predefined methods of sprinkler response from which that required may be set."@en , "あらかじめ定義済みのスプリンクラーの応答方式から必要な方式を設定する識別。"@ja-JP ;
        rdfs:label             "response"@en , "応答"@ja-JP ;
        schema:domainIncludes  <https://w3id.org/product/FireSuppressionTerminal%2FSPRINKLER> .

props:currentContent3rdHarmonic
        a                      owl:DatatypeProperty ;
        rdfs:comment           "The ratio between the third harmonic current and the phase current."@en , "第３高調波電流と相電流の比率。"@ja-JP ;
        rdfs:label             "currentContent3rdHarmonic"@en , "第３高調波電流と相電流の比"@ja-JP ;
        rdfs:range             <https://w3id.org/product/PositiveRatioMeasure> ;
        schema:domainIncludes  <https://w3id.org/product/DistributionPort%2FELECTRICAL> .

props:heatTransferTypeEnum
        a                      owl:DatatypeProperty ;
        rdfs:comment           "Type of heat transfer between the two air streams."@en , "空気間の熱交換の種類（顕熱、潜熱…）"@ja-JP , "Type de transfert de chaleur entre deux flux d'air."@fr-FR ;
        rdfs:label             "heatTransferTypeEnum"@en , "熱交換種類"@ja-JP , "TypeEchangeChaleurEnum"@fr-FR ;
        schema:domainIncludes  <https://w3id.org/product/AirToAirHeatRecovery> .

props:thermalConductivityTemperatureDerivative
        a                      owl:DatatypeProperty ;
        rdfs:comment           "Thermal conductivity temperature derivative."@en ;
        rdfs:label             "thermalConductivityTemperatureDerivative"@en ;
        rdfs:range             xsd:decimal ;
        schema:domainIncludes  <https://w3id.org/product/Material> .

props:hydraulicDiameter
        a                      owl:DatatypeProperty ;
        rdfs:comment           "Hydraulic diameter."@en , "水力直径"@ja-JP ;
        rdfs:label             "hydraulicDiameter"@en , "水力直径"@ja-JP ;
        rdfs:range             <https://w3id.org/product/LengthMeasure> ;
        schema:domainIncludes  <https://w3id.org/product/DuctSilencer> .

props:specialInstructions
        a                      owl:DatatypeProperty ;
        rdfs:comment           "Special instructions that affect the move."@en , "荷造りに関する特記事項。"@ja-JP , "Special instructions for packing."@en , "移動・引っ越しに影響する特別な指示。"@ja-JP ;
        rdfs:label             "特別指示"@ja-JP , "特記事項"@ja-JP , "specialInstructions"@en ;
        rdfs:range             xsd:string ;
        schema:domainIncludes  <https://w3id.org/product/ProjectOrder%2FMOVEORDER> .

props:isHorizontalCable
        a                      owl:DatatypeProperty ;
        rdfs:comment           "Indication of whether the cable occurrences are mounted horizontally (= TRUE) or vertically (= FALSE)."@en ;
        rdfs:label             "isHorizontalCable"@en ;
        rdfs:range             xsd:boolean ;
        schema:domainIncludes  <https://w3id.org/product/CableSegment> .

props:propertyName  a          owl:DatatypeProperty ;
        rdfs:comment           "Addressing details of the property as stated within the agreement."@en ;
        rdfs:label             "propertyName"@en ;
        rdfs:range             xsd:string ;
        schema:domainIncludes  <https://w3id.org/product/SpatialStructureElement> .

props:location3Local  a        owl:DatatypeProperty ;
        rdfs:comment           "Local x,y coordinates of the point in which Thickness3 is given"@en ;
        rdfs:label             "location3Local"@en ;
        schema:domainIncludes  <https://w3id.org/product/StructuralSurfaceMemberVarying> .

props:occupancyTimePerDay
        a                      owl:DatatypeProperty ;
        rdfs:comment           "Durée journalière de l'activité dans cet espace"@fr-FR , "The amount of time during the day that the activity is required within this space."@en , "この空間での活動をするために必要な日中の時間。"@ja-JP , "Durchschnittliche Belegungszeit des Raums pro Tag."@de-DE ;
        rdfs:label             "DureeOccupationJour"@fr-FR , "日毎利用時間"@ja-JP , "Belegungszeit pro Tag"@de-DE , "occupancyTimePerDay"@en ;
        rdfs:range             <https://w3id.org/product/TimeMeasure> ;
        schema:domainIncludes  <https://w3id.org/product/Space> , <https://w3id.org/product/cZone> , <https://w3id.org/product/cSpatialZone> .

props:groundFaultTrippingTime
        a                      owl:DatatypeProperty ;
        rdfs:comment           "Ground fault tripping time. The set value of the ground fault tripping current if adjustable."@en ;
        rdfs:label             "groundFaultTrippingTime"@en ;
        rdfs:range             <https://w3id.org/product/TimeMeasure> ;
        schema:domainIncludes  <https://w3id.org/product/ProtectiveDevice> .

props:meanTimeBetweenFailure
        a                      owl:DatatypeProperty ;
        rdfs:comment           "The average time duration between instances of failure of a product."@en ;
        rdfs:label             "meanTimeBetweenFailure"@en ;
        rdfs:range             xsd:duration ;
        schema:domainIncludes  <https://w3id.org/product/Element> .

props:outsideAirPerPerson
        a                      owl:DatatypeProperty ;
        rdfs:comment           "Design quantity of outside air to be provided per person in the space."@en , "１人あたりの外気量の設計値。"@ja-JP , "당 외기 량의 설계 값."@ko-KR ;
        rdfs:label             "outsideAirPerPerson"@en , "１人あたりの外気量"@ja-JP , "당 외기량"@ko-KR ;
        rdfs:range             <https://w3id.org/product/VolumetricFlowRateMeasure> ;
        schema:domainIncludes  <https://w3id.org/product/SpatialElement> .

props:airPressurization
        a                      owl:DatatypeProperty ;
        rdfs:comment           "空間が加圧することを要求されているかどうかを示すブーリアン値。(TRUE)加圧、(FALSE)非加圧。"@ja-JP , "Indique si l'espace nécessite d'être alimenté en air comprimé (VRAI) ou non (FAUX)"@fr-FR , "Angabe, ob der Raum einen Luftdruckausgleich erfordert (WAHR) oder nicht (FALSCH)."@de-DE , "Indication whether the space is required to have pressurized air (TRUE) or not (FALSE)."@en , "공간이 가압 요구되고 있는지 여부를 나타내는 부울 값입니다. (TRUE) 가압 (FALSE) 비 가압."@ko-KR ;
        rdfs:label             "AirComprimeDisponible"@fr-FR , "空気加圧"@ja-JP , "공기 가압"@ko-KR , "airPressurization"@en , "Luftdruckausgleich"@de-DE ;
        rdfs:range             xsd:boolean ;
        schema:domainIncludes  <https://w3id.org/product/cSpatialZone> , <https://w3id.org/product/cZone> , <https://w3id.org/product/Space> .

props:hazardousWaste  a        owl:DatatypeProperty ;
        rdfs:comment           "Quantité de déchets dangereux générés [NDT : tels que définis dans la norme NF P01-010]"@fr-FR , "Quantity of hazardous waste generated."@en , "유해 폐기물의 발생량"@ko-KR , "生成される有害廃棄物の量。"@ja-JP ;
        rdfs:label             "DechetsDangereux"@fr-FR , "hazardousWaste"@en , "유해 폐기물"@ko-KR , "有害廃棄物"@ja-JP ;
        rdfs:range             <https://w3id.org/product/MassMeasure> ;
        schema:domainIncludes  <https://w3id.org/product/Element> .

props:angleToFirstAxis
        a                      owl:DatatypeProperty ;
        rdfs:comment           "The angle of rotation of the axis of the first component relative to the ‘West’ edge of the slab."@en ;
        rdfs:label             "angleToFirstAxis"@en ;
        rdfs:range             <https://w3id.org/product/PlaneAngleMeasure> ;
        schema:domainIncludes  <https://w3id.org/product/Slab> .

props:n_Protection  a          owl:DatatypeProperty ;
        rdfs:comment           "An indication whether the electronic tripping unit has separate protection for the N conductor, or not."@en , "電磁式トリップ装置がN個の導体を保護するか否かの設定。"@ja-JP , "전자식 트립 장치가 N 개의 도체를 보호 여부 설정."@ko-KR ;
        rdfs:label             "n_Protection"@en , "N_Protection"@ja-JP , "N_Protection"@ko-KR ;
        rdfs:range             xsd:boolean ;
        schema:domainIncludes  <https://w3id.org/product/ProtectiveDeviceTrippingUnit%2FELECTRONIC> .

props:heatingDesignDay
        a                      owl:DatatypeProperty ;
        rdfs:comment           "The month, day and time that has been selected for the heating design calculations."@en , "暖房設計用気象データの日付。"@ja-JP , "난방 설계 기상 데이터의 날짜"@ko-KR ;
        rdfs:label             "heatingDesignDay"@en , "暖房設計基準日"@ja-JP , "난방 설계 기준일"@ko-KR ;
        rdfs:range             xsd:dateTime ;
        schema:domainIncludes  <https://w3id.org/product/Building> .

props:fanPower  a              owl:DatatypeProperty ;
        rdfs:comment           "송풍기 모터의 열 취득"@ko-KR , "Fan motor loads contributing to the cooling load."@en , "送風機モーターからの熱取得。"@ja-JP ;
        rdfs:label             "fanPower"@en , "送風機電力消費量"@ja-JP , "송풍기 소비 전력"@ko-KR ;
        rdfs:range             <https://w3id.org/product/PowerMeasure> ;
        schema:domainIncludes  <https://w3id.org/product/SpatialZone> , <https://w3id.org/product/Space> , <https://w3id.org/product/Zone> .

props:keypadType  a            owl:DatatypeProperty ;
        rdfs:comment           "A list of the available types of keypad switch from which that required may be selected."@en , "選択が必要となる、キーパッドスイッチの一覧リスト。"@ja-JP , "선택이 필요한 키패드 스위치 목록"@ko-KR ;
        rdfs:label             "keypadType"@en , "キーパッドタイプ"@ja-JP , "키패드 유형"@ko-KR ;
        schema:domainIncludes  <https://w3id.org/product/SwitchingDevice%2FKEYPAD> .

props:activationTemperature
        a                      owl:DatatypeProperty ;
        rdfs:comment           "The temperature at which the object is designed to activate."@en , "設計作動温度。"@ja-JP ;
        rdfs:label             "activationTemperature"@en , "作動温度"@ja-JP ;
        rdfs:range             <https://w3id.org/product/ThermodynamicTemperatureMeasure> ;
        schema:domainIncludes  <https://w3id.org/product/FireSuppressionTerminal%2FSPRINKLER> .

props:cO2Content  a            owl:DatatypeProperty ;
        rdfs:comment           "Carbon dioxide (CO2) content of the products of combustion. This is measured in weight of CO2 per unit weight and is therefore unitless."@en ;
        rdfs:label             "cO2Content"@en ;
        rdfs:range             <https://w3id.org/product/PositiveRatioMeasure> ;
        schema:domainIncludes  <https://w3id.org/product/Material> .

props:maximumOperatingTemperature
        a                      owl:DatatypeProperty ;
        rdfs:comment           "The maximum temperature at which a cable or bus is certified to operate."@en , "ケーブルや母線の最大動作温度を示す。"@ja-JP , "케이블과 모선의 최대 작동 온도를 나타낸다."@ko-KR ;
        rdfs:label             "maximumOperatingTemperature"@en , "許容最高温度"@ja-JP , "허용 최고 온도"@ko-KR ;
        rdfs:range             <https://w3id.org/product/ThermodynamicTemperatureMeasure> ;
        schema:domainIncludes  <https://w3id.org/product/CableSegment%2FCABLESEGMENT> .

props:baseChamfer  a           owl:DatatypeProperty ;
        rdfs:comment           "Base chamfer of the profile."@en ;
        rdfs:label             "baseChamfer"@en ;
        rdfs:range             <https://w3id.org/product/NonNegativeLengthMeasure> ;
        schema:domainIncludes  <https://w3id.org/product/ArbitraryProfileDefWithVoids> .

props:hoseDiameter  a          owl:DatatypeProperty ;
        rdfs:comment           "Notional diameter (bore) of the hose."@en , "ホースの公称口径（内径）。"@ja-JP ;
        rdfs:label             "hoseDiameter"@en , "ホース径"@ja-JP ;
        rdfs:range             <https://w3id.org/product/PositiveLengthMeasure> ;
        schema:domainIncludes  <https://w3id.org/product/FireSuppressionTerminal%2FHOSEREEL> .

props:subNatureOfRisk2
        a                      owl:DatatypeProperty ;
        rdfs:comment           "A second subsidiary value that might be assigned to designate a more specific type of risk. An example might be 'o person and property'."@en ;
        rdfs:label             "subNatureOfRisk2"@en ;
        rdfs:range             xsd:string ;
        schema:domainIncludes  <https://w3id.org/product/Process> .

props:refreshRate  a           owl:DatatypeProperty ;
        rdfs:comment           "Indicates the display refresh frequency."@en , "リフレッシュレート周波数範囲を示す。"@ja-JP , "빈도 재생 빈도 주파수 범위를 나타낸다."@ko-KR ;
        rdfs:label             "refreshRate"@en , "リフレッシュレート"@ja-JP , "재생"@ko-KR ;
        rdfs:range             <https://w3id.org/product/FrequencyMeasure> ;
        schema:domainIncludes  <https://w3id.org/product/AudioVisualAppliance%2FDISPLAY> .

props:designName  a            owl:DatatypeProperty ;
        rdfs:comment           "A name for the design values."@en , "設計値の名称。"@ja-JP , "설계 값의 명칭."@ko-KR ;
        rdfs:label             "designName"@en , "設計値名称"@ja-JP , "설계 값이름"@ko-KR ;
        rdfs:range             xsd:string ;
        schema:domainIncludes  <https://w3id.org/product/DistributionSystem%2FVENTILATION> .

props:playerType  a            owl:DatatypeProperty ;
        rdfs:comment           "Indicates the type of player."@en , "再生可能な形式を示す。"@ja-JP , "재생 가능한 형식을 보여준다."@ko-KR ;
        rdfs:label             "playerType"@en , "プレイヤー形式"@ja-JP , "플레이어 형식"@ko-KR ;
        schema:domainIncludes  <https://w3id.org/product/AudioVisualAppliance%2FPLAYER> .

props:ultimateStrain  a        owl:DatatypeProperty ;
        rdfs:comment           "A measure of the (engineering) strain at the state of ultimate stress of the material."@en ;
        rdfs:label             "ultimateStrain"@en ;
        rdfs:range             <https://w3id.org/product/PositiveRatioMeasure> ;
        schema:domainIncludes  <https://w3id.org/product/Material%2FSteel> .

props:toppingType  a           owl:DatatypeProperty ;
        rdfs:comment           "Defines if a topping is applied and what kind. Values are “Full topping”, “Perimeter Wash”, “None”"@en ;
        rdfs:label             "toppingType"@en ;
        rdfs:range             xsd:string ;
        schema:domainIncludes  <https://w3id.org/product/Slab> .

props:modelLabel  a            owl:DatatypeProperty ;
        rdfs:comment           "The descriptive model name of the product model (or product line) as assigned by the manufacturer of the manufactured item."@en ;
        rdfs:label             "modelLabel"@en ;
        rdfs:range             xsd:string ;
        schema:domainIncludes  <https://w3id.org/product/Element> .

props:preventiveMeassures
        a                      owl:DatatypeProperty ;
        rdfs:comment           "Identifies preventive measures to be taken to mitigate risk."@en ;
        rdfs:label             "preventiveMeassures"@en ;
        schema:domainIncludes  <https://w3id.org/product/Process> .

props:conduitShapeType
        a                      owl:DatatypeProperty ;
        rdfs:comment           "The shape of the conduit segment."@en , "電線管の形状タイプ。\n（円筒形,卵形,その他,不明,なし）"@ja-JP , "전선관의 형상 타입. (원통형, 계란 모양, 기타 알 수 없음) \""@ko-KR ;
        rdfs:label             "conduitShapeType"@en , "電線管のタイプ"@ja-JP , "전선관의 유형"@ko-KR ;
        schema:domainIncludes  <https://w3id.org/product/CableCarrierSegment%2FCONDUITSEGMENT> .

props:adjustmentRangeStepValue
        a                      owl:DatatypeProperty ;
        rdfs:comment           "시간 조정 범위를 단계 값을 설정합니다. 목록은 갖고 있지 않은 것을주의."@ko-KR , "時間調整の範囲をステップ値を設定。一覧表ではもっていない事を注意。"@ja-JP , "Step value of current adjustment for an AdjustmentValueType = RANGE. Note that this property should not have a value for an  AdjustmentValueType = LIST."@en , "Step value of time adjustment for an AdjustmentValueType = RANGE. Note that this property should not have a value for an  AdjustmentValueType = LIST."@en ;
        rdfs:label             "조정범위 단계값"@ko-KR , "調整範囲のステップ値"@ja-JP , "adjustmentRangeStepValue"@en ;
        rdfs:range             <https://w3id.org/product/TimeMeasure> , <https://w3id.org/product/ElectricCurrentMeasure> ;
        schema:domainIncludes  <https://w3id.org/product/ProtectiveDeviceTrippingUnit> .

props:spaceHumidityMin
        a                      owl:DatatypeProperty ;
        rdfs:comment           "空間またはゾーンの最低湿度。利用者/設計者の視点から要求される。もし夏季または冬季の室内湿度要求が与えられないと、それは通年に、さもなければ中間季に適用される。"@ja-JP , "Minimal geforderte Luftfeuchtigkeit für diesen Raum, gilt als ganzjährige Anforderung unabhängig vom Heizungs-, oder Kühlungsfall."@de-DE , "Humidité relative minimale de l'espace ou de la zone spécifiée par l'usager ou le concepteur. Si les valeurs pour l'été et l'hiver ne sont pas connues, cette température s'applique toute l'année, sinon seulement en demi-saison."@fr-FR , "Minimal permitted humidity of the space or zone that is required from user/designer view point.  If no summer or winter space humidity requirements are given, it applies all year, otherwise for the intermediate period."@en ;
        rdfs:label             "最低室内湿度"@ja-JP , "Luftfeuchtigkeit Minimal"@de-DE , "spaceHumidityMin"@en , "Humidité relative minimale"@fr-FR ;
        rdfs:range             <https://w3id.org/product/RatioMeasure> ;
        schema:domainIncludes  <https://w3id.org/product/Space> , <https://w3id.org/product/cSpatialZone> , <https://w3id.org/product/cZone> .

props:insetShadingCoefficient
        a                      owl:DatatypeProperty ;
        rdfs:comment           "German-description-3"@de-DE , "玻璃内嵌的遮阳设备的辐射透射系数，符号为b值。无单位。"@zh-CN , "Coefficient de transmission du rayonnement de la protection solaire intégrée au vitrage, symbole \"Valeur-b\". Valeur adimensionnelle."@fr-FR , "Radiation transmission coefficient of the shading device inside the glazing, symbol \"b-value\". It is a value without unit."@en ;
        rdfs:label             "insetShadingCoefficient"@en , "内嵌遮阳系数"@zh-CN , "CoefficientMasqueIntegre"@fr-FR , "German-name-3"@de-DE ;
        rdfs:range             <https://w3id.org/product/PositiveRatioMeasure> ;
        schema:domainIncludes  <https://w3id.org/product/cWindow> , <https://w3id.org/product/Door> .

props:heatingEfficiency
        a                      owl:DatatypeProperty ;
        rdfs:comment           "Heating efficiency under full load heating conditions."@en , "全負荷加熱状態での熱効率"@ja-JP ;
        rdfs:label             "heatingEfficiency"@en , "加熱効率"@ja-JP ;
        rdfs:range             <https://w3id.org/product/PositiveRatioMeasure> ;
        schema:domainIncludes  <https://w3id.org/product/UnitaryEquipment%2FAIRCONDITIONINGUNIT> .

props:worksurfaceArea
        a                      owl:DatatypeProperty ;
        rdfs:comment           "The value of the work surface area of the desk.."@en , "The value of the work surface area of the desk."@en ;
        rdfs:label             "worksurfaceArea"@en ;
        rdfs:range             <https://w3id.org/product/AreaMeasure> ;
        schema:domainIncludes  <https://w3id.org/product/Furniture%2FTABLE> , <https://w3id.org/product/Furniture%2FDESK> .

props:leakageCurve  a          owl:DatatypeProperty ;
        rdfs:comment           "Leakage versus pressure drop; Leakage = f (pressure)."@en , "Leakage per unit length curve versus working pressure. If a scalar is expressed then it represents LeakageClass which is flowrate per unit area at a specified pressure rating (e.g., ASHRAE Fundamentals 2001 34.16.)."@en , "作動圧力に対する単位長さあたりの漏れ曲線。\nスカラー値が表現されている場合は、所定の圧力（例えば、ASHRAE　Fundamentals 200134.16）における単位面積当たりの流量である漏れクラスを表す。"@ja-JP , "配管圧力に対する単位あたり流出量曲線"@ja-JP , "Leakage per unit length curve versus working pressure."@en ;
        rdfs:label             "漏洩曲線"@ja-JP , "leakageCurve"@en , "漏れ曲線"@ja-JP ;
        schema:domainIncludes  <https://w3id.org/product/PipeSegment> , <https://w3id.org/product/DuctSegment> , <https://w3id.org/product/Damper> .

props:assessmentOfRisk
        a                      owl:DatatypeProperty ;
        rdfs:comment           "Likelihood of risk event occurring.\n\nNote  that assessment of risk may frequently be associated with the physical location of the object for which the risk is assessed."@en ;
        rdfs:label             "assessmentOfRisk"@en ;
        schema:domainIncludes  <https://w3id.org/product/Process> .

props:electricActuatorType
        a                      owl:DatatypeProperty ;
        rdfs:comment           "Enumeration that identifies electric actuator as defined by its operational principle."@en , "作動原理によって定義された電気式アクチュエータを識別する一覧。"@ja-JP , "작동 원리에 의해 정의된 전기식 액츄에이터를 식별하는 목록"@ko-KR ;
        rdfs:label             "electricActuatorType"@en , "電気式アクチュエータタイプ"@ja-JP , "전기식 액추에이터 유형"@ko-KR ;
        schema:domainIncludes  <https://w3id.org/product/Actuator%2FELECTRICACTUATOR> .

props:minimumWidth  a          owl:DatatypeProperty ;
        rdfs:comment           "The minimum duct width for oval or rectangular duct."@en , "矩形、円形或いは楕円形ダクトの最小幅。"@ja-JP , "사각형, 원형 또는 타원형 덕트의 최소 폭."@ko-KR ;
        rdfs:label             "minimumWidth"@en , "最小幅"@ja-JP , "최소폭"@ko-KR ;
        rdfs:range             <https://w3id.org/product/PositiveLengthMeasure> ;
        schema:domainIncludes  <https://w3id.org/product/DistributionSystem%2FVENTILATION> .

props:sound  a                 owl:DatatypeProperty ;
        rdfs:comment           "Sound performance."@en , "騒音性能"@ja-JP , "Performance acoustique"@fr-FR ;
        rdfs:label             "sound"@en , "騒音"@ja-JP , "Acoustique"@fr-FR ;
        schema:domainIncludes  <https://w3id.org/product/AirTerminalBox> .

props:nominalSumpDepth
        a                      owl:DatatypeProperty ;
        rdfs:comment           "Nominal or quoted length measured along the z-axis in the local coordinate system of the sump."@en , "局所座標系のZ軸に沿う形で測定され汚水槽の長さ。"@ja-JP ;
        rdfs:label             "nominalSumpDepth"@en , "汚水槽深さ"@ja-JP ;
        rdfs:range             <https://w3id.org/product/PositiveLengthMeasure> ;
        schema:domainIncludes  <https://w3id.org/product/WasteTerminal%2FGULLYSUMP> .

props:finish  a                owl:DatatypeProperty ;
        rdfs:comment           "该构件的表面处理方式。仅供参考。"@zh-CN , "Description of the finish applied to the faucet."@en , "Finish selection for this object.\nHere specification of the surface finish for informational purposes."@en , "水栓に適用される仕上げの説明"@ja-JP , "仕上げ選択に関する情報。表面仕上げに関する仕様。"@ja-JP , "Oberflächenbehandlung oder Oberflächengüte, wie \"poliert\", \"schalungsrau\", imprägniert."@de-DE , "Finition de cet objet. Spécification de la finition donnée à titre informatif."@fr-FR ;
        rdfs:label             "Finition"@fr-FR , "表面处理"@zh-CN , "仕上げ"@ja-JP , "Oberflächengüte"@de-DE , "finish"@en ;
        rdfs:range             xsd:string ;
        schema:domainIncludes  <https://w3id.org/product/Valve%2FFAUCET> , <https://w3id.org/product/Covering> .

props:baseType  a              owl:DatatypeProperty ;
        rdfs:comment           "Defines general types of pump bases.\n\nFRAME: Frame. \nBASE: Base. \nNONE: There is no pump base, such as an inline pump. \nOTHER: Other type of pump base."@en , "ポンプ基礎の一般的な型を定義する(フレーム、(コンクリ)基礎、なし、その他)"@ja-JP ;
        rdfs:label             "baseType"@en , "基礎タイプ"@ja-JP ;
        schema:domainIncludes  <https://w3id.org/product/Pump> .

props:artificialLighting
        a                      owl:DatatypeProperty ;
        rdfs:comment           "Indication si cette pièce a des besoins d'éclairage artificiel (dans la mesure où l'éclairage naturel ne serait pas suffisant). (VRAI) signifie oui, (FAUX) sinon."@fr-FR , "Indication whether this space  requires artificial lighting (as natural lighting would be not sufficient). (TRUE) indicates yes (FALSE) otherwise."@en , "이 공간이 인공 조명을 필요로하는지 여부 (자연 조명이 충분하지 않기 위하여)를 나타내는 부울 값입니다. (TRUE) 필요 (FALSE) 아니오 값."@ko-KR , "Angabe, ob dieser Raum eine künstliche Beleuchtung erfordert (WAHR) oder nicht (FALSCH)"@de-DE , "領域が人工照明を必要とするかどうかの表示（自然光が十分でないとして）　（TRUE）の場合、必要。（FALSE）の場合、不必要。"@ja-JP ;
        rdfs:label             "人工照明"@ja-JP , "künstliche Beleuchtung"@de-DE , "EclairageArtificiel"@fr-FR , "인공 조명"@ko-KR , "artificialLighting"@en ;
        rdfs:range             xsd:boolean ;
        schema:domainIncludes  <https://w3id.org/product/cZone> , <https://w3id.org/product/cSpatialZone> , <https://w3id.org/product/Space> .

props:totalRadiantLoad
        a                      owl:DatatypeProperty ;
        rdfs:comment           "Total electromagnetic energy added or removed by emission or absorption.  If a value is less than zero (negative), then the thermal load is lost from the space. If a value is greater than zero (positive), then the thermal load is a gain to the space."@en , "放射や吸収による放射エネルギーの増加、或いは減少の合計。ゼロより小さい（－）場合、放射エネルギーが減少となる。ゼロより大きい（＋）場合、放射エネルギーが増大となる。"@ja-JP , "방사선 및 흡수에 의한 방사 에너지 증가 또는 감소의 총. 제로보다 작은 (-) 경우 방사 에너지가 감소된다. 제로보다 큰 (+) 경우 방사 에너지가 증대된다."@ko-KR ;
        rdfs:label             "totalRadiantLoad"@en , "放射熱負荷の合計"@ja-JP , "복사열로드 합계"@ko-KR ;
        schema:domainIncludes  <https://w3id.org/product/Space> .

props:n_Protection_50
        a                      owl:DatatypeProperty ;
        rdfs:comment           "An indication whether the electronic tripping unit is tripping if the current in the N conductor is more than 50% of that of the phase conductors. The property is only asserted if the property N_Protection is asserted."@en , "電磁式トリップ装置がN導体の50％以上で保護するか否かの設定。"@ja-JP , "전자식 트립 장치가 N 도체의 50 % 이상으로 보호 여부 설정."@ko-KR ;
        rdfs:label             "n_Protection_50"@en , "N_Protection_50"@ja-JP , "N_Protection_50"@ko-KR ;
        rdfs:range             xsd:boolean ;
        schema:domainIncludes  <https://w3id.org/product/ProtectiveDeviceTrippingUnit%2FELECTRONIC> .

props:keyHeight  a             owl:DatatypeProperty ;
        rdfs:comment           "Key height of the profile."@en ;
        rdfs:label             "keyHeight"@en ;
        rdfs:range             <https://w3id.org/product/NonNegativeLengthMeasure> ;
        schema:domainIncludes  <https://w3id.org/product/ArbitraryProfileDefWithVoids> .

props:secondaryVoltage
        a                      owl:DatatypeProperty ;
        rdfs:comment           "The voltage that has been transformed and is running out of the transformer on the secondary side."@en , "変圧器の2次側へ出力される電圧。"@ja-JP , "변압기 2 차 측에 전송되는 전압."@ko-KR ;
        rdfs:label             "secondaryVoltage"@en , "第2電圧"@ja-JP , "두번째 전압"@ko-KR ;
        rdfs:range             <https://w3id.org/product/ElectricVoltageMeasure> ;
        schema:domainIncludes  <https://w3id.org/product/Transformer> .

props:concreteCoverAtLinks
        a                      owl:DatatypeProperty ;
        rdfs:comment           "国の建築基準に従い、補強筋をコンクリートの被りで保護する。"@ja-JP , "The protective concrete cover at the reinforcement links according to local building regulations."@en , "국가의 건축 기준에 따라 보강근 콘크리트의 입고로 보호"@ko-KR , "Abstand zwischen der Betonoberfläche und der Außenkante der vom Beton umhüllten Bewehrungsverbindungsstäben."@de-DE ;
        rdfs:label             "Betonüberdeckung Verbindungsstäbe"@de-DE , "보강근 콘크리트 입고"@ko-KR , "補強筋のコンクリート被り"@ja-JP , "concreteCoverAtLinks"@en ;
        rdfs:range             <https://w3id.org/product/PositiveLengthMeasure> ;
        schema:domainIncludes  <https://w3id.org/product/BuildingElement> .

props:operatingWeight
        a                      owl:DatatypeProperty ;
        rdfs:comment           "Operating weight of the tank including all of its contents."@en , "中身全部を含んだタンクの運転重量"@ja-JP ;
        rdfs:label             "operatingWeight"@en , "運転重量"@ja-JP ;
        rdfs:range             <https://w3id.org/product/MassMeasure> ;
        schema:domainIncludes  <https://w3id.org/product/Tank> .

props:returnWaterTemperatureCooling
        a                      owl:DatatypeProperty ;
        rdfs:comment           "Return water temperature in cooling mode."@en ;
        rdfs:label             "returnWaterTemperatureCooling"@en ;
        schema:domainIncludes  <https://w3id.org/product/CooledBeam> .

props:prevailingWindDirection
        a                      owl:DatatypeProperty ;
        rdfs:comment           "The prevailing wind angle direction measured from True North (0 degrees) in a clockwise direction."@en , "卓越風の風向、真北は0°、時計回り。"@ja-JP , "탁월한 바람의 풍향, 북쪽은 0 ° 시계 방향."@ko-KR ;
        rdfs:label             "prevailingWindDirection"@en , "卓越風の風向"@ja-JP , "탁월한 방람의 풍향"@ko-KR ;
        rdfs:range             <https://w3id.org/product/PlaneAngleMeasure> ;
        schema:domainIncludes  <https://w3id.org/product/Building> .

props:insulationStandardClass
        a                      owl:DatatypeProperty ;
        rdfs:comment           "Insulation standard classes provides basic protection information against electric shock. Defines levels of insulation required in terms of constructional requirements (creepage and clearance distances) and electrical requirements (compliance with electric strength tests). Basic insulation is considered to be shorted under single fault conditions. The actual values required depend on the working voltage to which the insulation is subjected, as well as other factors. Also indicates whether the electrical device has a protective earth connection."@en ;
        rdfs:label             "insulationStandardClass"@en ;
        schema:domainIncludes  <https://w3id.org/product/DistributionElement> .

props:soundCurve  a            owl:DatatypeProperty ;
        rdfs:comment           "Regenerated sound versus air-flow rate."@en , "オクターブバンド1pW（10^(-12)の音の強さを基準とする音の周波数とデシベル単位で計測した音のエネルギーの一覧表。"@ja-JP , "옥타브 밴드 1pW (10 ^ (-12) 소리의 강도를 기준으로하는 소리의 주파수와 데시벨 단위로 측정하는 소리 에너지의 목록."@ko-KR , "Table of sound frequencies and sound power measured in decibels at a reference power of 1 picowatt(10^(-12) watt) for the referenced octave band frequency."@en , "Son généré par rapport au débit aéraulique."@fr-FR ;
        rdfs:label             "音響（騒音？）曲線"@ja-JP , "음향곡성"@ko-KR , "soundCurve"@en , "CourbeSon"@fr-FR ;
        schema:domainIncludes  <https://w3id.org/product/DistributionFlowElement> , <https://w3id.org/product/Coil> .

props:nominalHeatTransferCoefficient
        a                      owl:DatatypeProperty ;
        rdfs:comment           "設計熱交換面積の全熱交換係数"@ja-JP , "Nominal overall heat transfer coefficient associated with nominal heat transfer area."@en ;
        rdfs:label             "設計熱交換係数"@ja-JP , "nominalHeatTransferCoefficient"@en ;
        rdfs:range             <https://w3id.org/product/ThermalTransmittanceMeasure> ;
        schema:domainIncludes  <https://w3id.org/product/Evaporator> , <https://w3id.org/product/Condenser> .

props:nominalSupplyWaterTemperatureHeating
        a                      owl:DatatypeProperty ;
        rdfs:comment           "Nominal supply water temperature (refers to nominal heating capacity)."@en ;
        rdfs:label             "nominalSupplyWaterTemperatureHeating"@en ;
        rdfs:range             <https://w3id.org/product/ThermodynamicTemperatureMeasure> ;
        schema:domainIncludes  <https://w3id.org/product/CooledBeam> .

props:bodyColor  a             owl:DatatypeProperty ;
        rdfs:comment           "Color of the body of the hydrant.\n\nNote: Consult local fire regulations for statutory colors that may be required for hydrant bodies in particular circumstances."@en , "消火栓本体の色。\n\n注意：特定の状況で消火栓ボディに求められる地域消防規則法定色による。"@ja-JP ;
        rdfs:label             "bodyColor"@en , "本体色"@ja-JP ;
        rdfs:range             xsd:string ;
        schema:domainIncludes  <https://w3id.org/product/FireSuppressionTerminal%2FFIREHYDRANT> .

props:lowerTime1  a            owl:DatatypeProperty ;
        rdfs:comment           "The time in [s], indicating that tripping times of the lower time/current curve lower than LowerTime1 is determined by the I2t part of the L-function."@en , "[s]の時間,下時間より低い特性曲線のトリップ時間は、L-関数ののI2t部分によって決定される。"@ja-JP , "[s] 시간 아래 시간보다 낮은 특성 곡선의 트립 시간은 L-함수의 I2t 부분에 의해 결정된다."@ko-KR ;
        rdfs:label             "lowerTime1"@en , "下時間1"@ja-JP , "하 시간 1"@ko-KR ;
        rdfs:range             <https://w3id.org/product/TimeMeasure> ;
        schema:domainIncludes  <https://w3id.org/product/ProtectiveDeviceTrippingUnit> .

props:exhaustAirFlowrate
        a                      owl:DatatypeProperty ;
        rdfs:comment           "Design exhaust air flow rate for the space."@en , "設計排気量。"@ja-JP , "설계 배기량."@ko-KR ;
        rdfs:label             "exhaustAirFlowrate"@en , "排気量"@ja-JP , "배기량"@ko-KR ;
        rdfs:range             <https://w3id.org/product/VolumetricFlowRateMeasure> ;
        schema:domainIncludes  <https://w3id.org/product/Space> .

props:isNormallyOpen  a        owl:DatatypeProperty ;
        rdfs:comment           "If TRUE, the valve is normally open. If FALSE is is normally closed."@en , "もし、TRUEなら弁はノーマルオープン、もし、FALSEならノーマルクローズ"@ja-JP ;
        rdfs:label             "isNormallyOpen"@en , "ノーマルオープン"@ja-JP ;
        rdfs:range             xsd:boolean ;
        schema:domainIncludes  <https://w3id.org/product/Valve%2FISOLATING> .

props:shortCircuitVoltage
        a                      owl:DatatypeProperty ;
        rdfs:comment           "A complex number that specifies the real and imaginary parts of the short-circuit voltage at rated current of a transformer given in %."@en , "%で与えられる変圧器の定格電流における短絡電圧の実数と虚数を定義する複素数。"@ja-JP , "%에서 주어진 변압기 정격 전류의 단락 전압의 실수와 허수를 정의하는 복소수."@ko-KR ;
        rdfs:label             "shortCircuitVoltage"@en , "短絡電圧"@ja-JP , "단락 전압"@ko-KR ;
        rdfs:range             <https://w3id.org/product/ComplexNumber> ;
        schema:domainIncludes  <https://w3id.org/product/Transformer> .

props:startDate  a             owl:DatatypeProperty ;
        rdfs:comment           "Date and time from which the permit becomes valid."@en ;
        rdfs:label             "startDate"@en ;
        rdfs:range             xsd:dateTime ;
        schema:domainIncludes  <https://w3id.org/product/Permit> .

props:yearOfConstruction
        a                      owl:DatatypeProperty ;
        rdfs:comment           "Year of construction of this building, including expected year of completion."@en , "Année de construction de ce bâtiment, incluant l'année de parfait achèvement."@fr-FR , "시공 년. 준공 예정 년 포함한다."@ko-KR , "Jahr der Errichtung des Gebäudes, einschließliich des Jahres der geplanten Fertigstellung."@de-DE , "施工の年。竣工の予想年も含む。"@ja-JP ;
        rdfs:label             "시공 년"@ko-KR , "施工年"@ja-JP , "AnneeConstruction"@fr-FR , "yearOfConstruction"@en , "Baujahr"@de-DE ;
        rdfs:range             xsd:string ;
        schema:domainIncludes  <https://w3id.org/product/Building> .

props:contributedLuminousFlux
        a                      owl:DatatypeProperty ;
        rdfs:comment           "Luminous flux is a photometric measure of radiant flux, i.e. the volume of light emitted from a light source. Luminous flux is measured either for the interior as a whole or for a part of the interior (partial luminous flux for a solid angle). All other photometric parameters are derivatives of luminous flux. Luminous flux is measured in lumens (lm). The luminous flux is given as a nominal value for each lamp."@en , "光束は放射束を光度測定したもので、たとえば、光源からの発光の量である。光束は全室内、または室内の一部（立体角の部分的な光束）で計測する。\n全ての光度測定の項目は高速の派生である。光束は単位ルーメンで計られる。光束は各ランプからの値で与えられる。"@ja-JP , "광속은 방사들을 광도 측정 것으로, 예를 들어, 광원에서 방출 양이다. 광속은 모든 실내, 실내 일부 (입체 각의 부분적인 광속)로 측정한다.모든 광도 측정 항목은 빠른 파생이다. 광속 단위 루멘으로 정해진다. 광속은 각 램프의 값으로 주어진다."@ko-KR ;
        rdfs:label             "contributedLuminousFlux"@en , "光束"@ja-JP , "광속"@ko-KR ;
        rdfs:range             <https://w3id.org/product/LuminousFluxMeasure> ;
        schema:domainIncludes  <https://w3id.org/product/Lamp> .

props:molding  a               owl:DatatypeProperty ;
        rdfs:comment           "Angabe des Materials für das Gesims (Deckenkante). Diese Angabe wird im Raumbuch verwendet.\n\nDie Materialangabe wird übernommen, wenn kein eigenes Bekleidungsobjekt (IfcCovering mit PredefinedType = MOLDING) für das Gesims dem Raum zugeordnet ist. Bei Inkonsistenzen (wenn beides gegeben ist), hat die Materialangabe des zugeordneten Bekleidungsobjekts Priorität."@de-DE , "部屋の廻縁の材質または施工に関するラベル（識別情報）。ラベル名は部屋リスト情報に使用される。\n\n形状表現を持つIfcCovering (type=MOLDING)オブジェクトが存在しない場合に与えられる材質情報。IfcCoveringの材質情報とこのプロパティ値が一致しない場合、IfcCoveringに与えられている材質情報を優先する。"@ja-JP , "Label to indicate the material or construction of the molding around the space ceiling. The label is used for room book information.\n\nThe material information is provided in absence of an IfcCovering (type=MOLDING) object with own shape representation and material assignment. In case of inconsistency the material assigned to IfcCovering elements takes precedence."@en ;
        rdfs:label             "廻縁"@ja-JP , "molding"@en , "Gesims"@de-DE , "Matériau de la moulure"@fr-FR ;
        rdfs:range             xsd:string ;
        schema:domainIncludes  <https://w3id.org/product/Space> .

props:flangeStandard  a        owl:DatatypeProperty ;
        rdfs:comment           "Designation of the standard describing the flange table."@en , "フランジ規格を記述している基準"@ja-JP ;
        rdfs:label             "flangeStandard"@en , "フランジ規格"@ja-JP ;
        rdfs:range             xsd:string ;
        schema:domainIncludes  <https://w3id.org/product/PipeSegment> .

props:exposureClass  a         owl:DatatypeProperty ;
        rdfs:comment           "Classification of exposure to environmental conditions, usually specified in accordance with the concrete design code which is applied in the project."@en , "Klassifikation der Widerstandsfähigkeit gegenüber chemischen und physikalischen Einwirkungen gemäß der aktuellen, im Projekt angewandten, Norm."@de-DE ;
        rdfs:label             "exposureClass"@en , "Expositionsklasse"@de-DE ;
        rdfs:range             xsd:string ;
        schema:domainIncludes  <https://w3id.org/product/BuildingElement> .

props:flangeTopFillet
        a                      owl:DatatypeProperty ;
        rdfs:comment           "Flange top fillet of the profile."@en ;
        rdfs:label             "flangeTopFillet"@en ;
        rdfs:range             <https://w3id.org/product/NonNegativeLengthMeasure> ;
        schema:domainIncludes  <https://w3id.org/product/ArbitraryClosedProfileDef> .

props:isMain  a                owl:DatatypeProperty ;
        rdfs:comment           "Identifies if the current instance is a main distribution point or topmost level in an electrical distribution hierarchy (= TRUE) or a sub-main distribution point (= FALSE)."@en ;
        rdfs:label             "isMain"@en ;
        rdfs:range             xsd:boolean ;
        schema:domainIncludes  <https://w3id.org/product/ElectricDistributionBoard> .

props:pHLevel  a               owl:DatatypeProperty ;
        rdfs:comment           "Maximum water PH in a range from 0-14."@en ;
        rdfs:label             "pHLevel"@en ;
        rdfs:range             <https://w3id.org/product/PHMeasure> ;
        schema:domainIncludes  <https://w3id.org/product/Material> .

props:halogenProof  a          owl:DatatypeProperty ;
        rdfs:comment           "煙や刺激臭のあるガスの発生が少ないケーブル。"@ja-JP , "Produces small amount of smoke and irritating Deaerator/Gas."@en , "연기와 자극적인 냄새가있는 가스의 발생이 적은 케이블"@ko-KR , "Produces small amount of smoke and irritating deaerator/gas."@en , "少量の煙および刺激する脱気/ガスを生成。"@ja-JP , "소량의 연기와 자극 탈기 / 가스를 생성합니다."@ko-KR ;
        rdfs:label             "에코 케이블"@ko-KR , "ハロゲン証明"@ja-JP , "할로겐 증명"@ko-KR , "エコケーブル"@ja-JP , "halogenProof"@en ;
        rdfs:range             xsd:boolean ;
        schema:domainIncludes  <https://w3id.org/product/CableSegment%2FCORESEGMENT> , <https://w3id.org/product/CableSegment%2FCABLESEGMENT> .

props:manufacturingToleranceClass
        a                      owl:DatatypeProperty ;
        rdfs:comment           "Classification designation of the manufacturing tolerances according to local standards."@en , "ローカルな標準によるメーカーの認可分類。"@ja-JP ;
        rdfs:label             "manufacturingToleranceClass"@en , "メーカーの認可分類"@ja-JP ;
        rdfs:range             xsd:string ;
        schema:domainIncludes  <https://w3id.org/product/BuildingElement> .

props:totalSensibleLoad
        a                      owl:DatatypeProperty ;
        rdfs:comment           "Total energy added or removed from air that affects its temperature.  If a value is less than zero (negative), then the thermal load is lost from the space. If a value is greater than zero (positive), then the thermal load is a gain to the space."@en , "空気温度を上昇・下降させる取得・損失の熱量の合計。ゼロより小さい（－）場合、室内が熱損失となる。ゼロより大きい（＋）場合、室内が熱取得となる。"@ja-JP , "공기 온도를 상승 · 하강하는 취득 · 손실 열량의 총. 제로보다 작은 (-) 경우 실내가 열 손실이된다. 제로보다 큰 (+) 경우 실내가 열을 검색된다."@ko-KR ;
        rdfs:label             "totalSensibleLoad"@en , "顕熱負荷の合計"@ja-JP , "현열부하의 합계"@ko-KR ;
        schema:domainIncludes  <https://w3id.org/product/Space> .

props:columnShoeBasePlateDepth
        a                      owl:DatatypeProperty ;
        rdfs:comment           "The depth of the column shoe base plate."@en , "柱脚ベースプレートの成。"@ja-JP , "기둥 다리 받침판 구성"@ko-KR ;
        rdfs:label             "columnShoeBasePlateDepth"@en , "ベースプレート成"@ja-JP , "베이스 플레이트 구성"@ko-KR ;
        rdfs:range             <https://w3id.org/product/PositiveLengthMeasure> ;
        schema:domainIncludes  <https://w3id.org/product/DiscreteAccessory%2FSHOE> .

props:earthFault1PoleMaximumState
        a                      owl:DatatypeProperty ;
        rdfs:comment           "Maximum 1 pole earth fault current provided at the point of supply i.e. the fault between 1 phase and PE/PEN."@en , "電源供給時点の点1相とPE/PEN間の1極最大地絡電流。"@ja-JP , "전원 공급 시점 점 1 상 및 PE / PEN 사이의 1 극 최대 지락 전류."@ko-KR ;
        rdfs:label             "earthFault1PoleMaximumState"@en , "1極最大地絡電流"@ja-JP , "1 극 최대 지락 전류"@ko-KR ;
        rdfs:range             <https://w3id.org/product/ElectricCurrentMeasure> ;
        schema:domainIncludes  <https://w3id.org/product/ElectricFlowStorageDevice> .

props:spaceAirTemperature
        a                      owl:DatatypeProperty ;
        rdfs:comment           "Dry bulb temperature in the space."@en , "部屋の乾球温度"@ja-JP ;
        rdfs:label             "spaceAirTemperature"@en , "室温"@ja-JP ;
        schema:domainIncludes  <https://w3id.org/product/SpaceHeater> .

props:hasTray  a               owl:DatatypeProperty ;
        rdfs:comment           "Indicates whether the shower has a separate receptacle that catches the water in a shower and directs it to a waste outlet."@en ;
        rdfs:label             "hasTray"@en ;
        rdfs:range             xsd:boolean ;
        schema:domainIncludes  <https://w3id.org/product/SanitaryTerminal%2FSHOWER> .

props:lossCoefficentCurve
        a                      owl:DatatypeProperty ;
        rdfs:comment           "Loss coefficient – blade position angle curve; ratio of pressure drop to velocity pressure versus blade angle; C = f (blade angle position)."@en ;
        rdfs:label             "lossCoefficentCurve"@en ;
        schema:domainIncludes  <https://w3id.org/product/Damper> .

props:isSkilledOperator
        a                      owl:DatatypeProperty ;
        rdfs:comment           "Identifies if the current instance requires a skilled person or instructed person to perform operations on the distribution board (= TRUE) or whether operations may be performed by a person without appropriate skills or instruction (= FALSE)."@en ;
        rdfs:label             "isSkilledOperator"@en ;
        rdfs:range             xsd:boolean ;
        schema:domainIncludes  <https://w3id.org/product/ElectricDistributionBoard> .

props:releaseStrength
        a                      owl:DatatypeProperty ;
        rdfs:comment           "The minimum required compressive strength of the concrete when the tendon stress is released. This property applies to prestressed concrete elements only."@en , "緊張力が解放される時のコンクリートの最小必要圧縮強度。この属性はプレストレストコンクリート要素のみに適用される。"@ja-JP ;
        rdfs:label             "releaseStrength"@en , "リリース強度"@ja-JP ;
        rdfs:range             <https://w3id.org/product/PressureMeasure> ;
        schema:domainIncludes  <https://w3id.org/product/BuildingElement> .

props:startingTime  a          owl:DatatypeProperty ;
        rdfs:comment           "The time (in s) needed for the motor to reach its rated speed with its driven equipment attached, starting from standstill and at the nominal voltage applied at its terminals."@en , "モーターが停止状態から定格電圧を印加し定格速度に到達するまでに必要な時間。"@ja-JP , "모터가 정지 상태에서 정격 전압을인가하여 정격 속도에 도달하는 데 필요한 시간"@ko-KR ;
        rdfs:label             "startingTime"@en , "始動時間"@ja-JP , "시작 시간"@ko-KR ;
        rdfs:range             <https://w3id.org/product/TimeMeasure> ;
        schema:domainIncludes  <https://w3id.org/product/ElectricMotor> .

props:nominalSurroundingTemperatureCooling
        a                      owl:DatatypeProperty ;
        rdfs:comment           "Nominal surrounding temperature (refers to nominal cooling capacity)."@en ;
        rdfs:label             "nominalSurroundingTemperatureCooling"@en ;
        rdfs:range             <https://w3id.org/product/ThermodynamicTemperatureMeasure> ;
        schema:domainIncludes  <https://w3id.org/product/CooledBeam> .

props:flangeDiameter  a        owl:DatatypeProperty ;
        rdfs:comment           "Overall diameter of the flange."@en , "フランジの全直径"@ja-JP ;
        rdfs:label             "flangeDiameter"@en , "フランジの直径"@ja-JP ;
        rdfs:range             <https://w3id.org/product/PositiveLengthMeasure> ;
        schema:domainIncludes  <https://w3id.org/product/PipeSegment> .

props:leakage  a               owl:DatatypeProperty ;
        rdfs:comment           "Air leakage rate."@en ;
        rdfs:label             "leakage"@en ;
        schema:domainIncludes  <https://w3id.org/product/Damper> .

props:lifeCyclePhase  a        owl:DatatypeProperty ;
        rdfs:comment           "Le cycle de vie complet ou seulement une de ses phases pour lequel les les données environnementales sont valides"@fr-FR , "환경 데이터가 유효한지 라이프 사이클 또는 단 하나 주어진 단계"@ko-KR , "The whole life cycle or only a given phase  from which environmental data are valid."@en , "環境データが有効であるライフサイクル全てまたは特定の段階。"@ja-JP ;
        rdfs:label             "lifeCyclePhase"@en , "ライフサイクルフェーズ"@ja-JP , "라이프 사이클 단계"@ko-KR , "PhaseCycleDeVie"@fr-FR ;
        schema:domainIncludes  <https://w3id.org/product/Element> .

props:maximumAirFlowRate
        a                      owl:DatatypeProperty ;
        rdfs:comment           "Maximum allowable air flow rate."@en ;
        rdfs:label             "maximumAirFlowRate"@en ;
        rdfs:range             <https://w3id.org/product/VolumetricFlowRateMeasure> ;
        schema:domainIncludes  <https://w3id.org/product/Damper> .

props:dissolvedSolidsContent
        a                      owl:DatatypeProperty ;
        rdfs:comment           "Fraction of the dissolved solids to the total amount of water. This is measured in weight of dissolved solids per weight of water and is therefore unitless."@en ;
        rdfs:label             "dissolvedSolidsContent"@en ;
        rdfs:range             <https://w3id.org/product/NormalisedRatioMeasure> ;
        schema:domainIncludes  <https://w3id.org/product/Material> .

props:carrierStackNumber
        a                      owl:DatatypeProperty ;
        rdfs:comment           "Number of carrier segments (tray, ladder etc.) that are vertically stacked (vertical is measured as the z-axis of the local coordinate system of the carrier segment)."@en ;
        rdfs:label             "carrierStackNumber"@en ;
        rdfs:range             xsd:int ;
        schema:domainIncludes  <https://w3id.org/product/CableSegment> .

props:proportionalConstant
        a                      owl:DatatypeProperty ;
        rdfs:comment           "The proportional gain factor of the controller (usually referred to as Kp)."@en , "비례 게인 (Kp)"@ko-KR ;
        rdfs:label             "proportionalConstant"@en , "비례 게인 (Kp)"@ko-KR ;
        rdfs:range             xsd:decimal ;
        schema:domainIncludes  <https://w3id.org/product/Controller%2FPROPORTIONAL> .

props:waterFlowControlSystemType
        a                      owl:DatatypeProperty ;
        rdfs:comment           "Factory fitted waterflow control system."@en ;
        rdfs:label             "waterFlowControlSystemType"@en ;
        schema:domainIncludes  <https://w3id.org/product/CooledBeam> .

props:particleAbsorptionCurve
        a                      owl:DatatypeProperty ;
        rdfs:comment           "Ratio of particles that are removed by the filter.  Each entry describes the ratio of particles absorbed greater than equal to the specified size and less than the next specified size.  For example,  given for 3 significant particle sizes >= 0,1 micro m, >= 1 micro m, >= 5 micro m"@en ;
        rdfs:label             "particleAbsorptionCurve"@en ;
        schema:domainIncludes  <https://w3id.org/product/Filter%2FCOMPRESSEDAIRFILTER> .

props:wrappingMaterial
        a             owl:DatatypeProperty ;
        rdfs:comment  "Special requirements for material used to wrap an artefact."@en , "品物の包装に使用される材料に関する特記事項。"@ja-JP ;
        rdfs:label    "wrappingMaterial"@en , "包装材料"@ja-JP .

props:percentageOpen  a        owl:DatatypeProperty ;
        rdfs:comment           "The ratio between the amount that the valve is open to the full open position of the valve."@en , "全開時に対する開度量の比率。"@ja-JP ;
        rdfs:label             "percentageOpen"@en , "パーセント開度"@ja-JP ;
        schema:domainIncludes  <https://w3id.org/product/Valve> .

props:isOneWay  a              owl:DatatypeProperty ;
        rdfs:comment           "Indicates whether the parking aisle is designed for oneway traffic (TRUE) or twoway traffic (FALSE). Should only be provided if the property IsAisle is set to TRUE."@en , "駐車場通路が一方通行(TRUE)か双方向(FALSE)かを示すフラグ。"@ja-JP , "Indique si cette allée du parking est prévue pour être à sens unique (VRAI) ou à double sens (FAUX). A fournir seulement si la propriété \"Est un accès\" est égale à VRAI."@fr-FR ;
        rdfs:label             "isOneWay"@en , "一方通行"@ja-JP , "Sens unique"@fr-FR ;
        rdfs:range             xsd:boolean ;
        schema:domainIncludes  <https://w3id.org/product/Space%2FPARKING> .

props:isWaterStorageHeater
        a                      owl:DatatypeProperty ;
        rdfs:comment           "This is used to identify if the boiler has storage capacity (TRUE). If FALSE, then there is no storage capacity built into the boiler, such as an instantaneous hot water heater."@en , "給湯用の缶体があればTRUE、（瞬間湯沸かし器のように）ボイラにタンクがなければFALSE"@ja-JP , "Utilisé pour identifier si la chaudière une capacité de réserve en eau (VRAI). Si FAUX, alors il n'y a pas de capacité de réserve intégrée dans la chaudière, tel qu'un chauffe-eau instantané."@fr-FR ;
        rdfs:label             "isWaterStorageHeater"@en , "給湯タンク有無"@ja-JP , "AvoirChauffeEau"@fr-FR ;
        rdfs:range             xsd:boolean ;
        schema:domainIncludes  <https://w3id.org/product/Boiler> .

props:controlStrategy
        a                      owl:DatatypeProperty ;
        rdfs:comment           "FixedExitingWaterTemp: The capacity is controlled to maintain a fixed exiting water temperature.\nWetBulbTempReset: The set-point is reset based on the wet-bulb temperature."@en ;
        rdfs:label             "controlStrategy"@en ;
        schema:domainIncludes  <https://w3id.org/product/CoolingTower> .

props:isFreeHanging  a         owl:DatatypeProperty ;
        rdfs:comment           "Is it free hanging type (not mounted in a false ceiling)?"@en ;
        rdfs:label             "isFreeHanging"@en ;
        rdfs:range             xsd:boolean ;
        schema:domainIncludes  <https://w3id.org/product/CooledBeam> .

props:airflowCurve  a          owl:DatatypeProperty ;
        rdfs:comment           "Air flowrate versus damper position relationship;airflow = f ( valve position)."@en , "ダンパ開度と風量の関係　　風量＝f(開度)"@ja-JP , "Relation entre débit d'air par rapport à la position du registre; Débit d'air = f (position du clapet)"@fr-FR ;
        rdfs:label             "airflowCurve"@en , "流量曲線"@ja-JP , "Courbe de débit d'air"@fr-FR ;
        schema:domainIncludes  <https://w3id.org/product/AirTerminalBox> .

props:smokeStop  a             owl:DatatypeProperty ;
        rdfs:comment           "このドアが煙を止める機能を有するかどうかのブーリアン値。"@ja-JP , "Angabe, ob das Fenster einen Rauchschutz gemäß der nationalen oder regionalen Brandschutzverordnung gewährleistet (JA) oder nicht (NEIN)."@de-DE , "Indication whether the object is designed to provide a smoke stop (TRUE) or not (FALSE)."@en , "Indique si la porte est conçue pour une fonction coupe-fumée (VRAI) ou non (FAUX)"@fr-FR , "表示该构件是否设计为防烟。"@zh-CN , "Angabe, ob die Tür einen Rauchschutz gemäß der nationalen oder regionalen Brandschutzverordnung gewährleistet (JA) oder nicht (NEIN). Rauchschutztüren müssen selbstschließend sein."@de-DE ;
        rdfs:label             "煙止め機能区分"@ja-JP , "Rauchschutz"@de-DE , "smokeStop"@en , "CoupeFumee"@fr-FR , "是否防烟"@zh-CN ;
        rdfs:range             xsd:boolean ;
        schema:domainIncludes  <https://w3id.org/product/Window> , <https://w3id.org/product/Door> .

props:n_Protection_100
        a                      owl:DatatypeProperty ;
        rdfs:comment           "An indication whether the electronic tripping unit is tripping if the current in the N conductor is more than 100% of that of the phase conductors. The property is only asserted if the property N_Protection is asserted."@en , "電磁式トリップ装置がN導体の100％以上で保護するか否かの設定。"@ja-JP , "전자식 트립 장치가 N 도체의 100 % 이상으로 보호 여부 설정."@ko-KR ;
        rdfs:label             "n_Protection_100"@en , "N_Protection_100"@ja-JP , "N_Protection_100"@ko-KR ;
        rdfs:range             xsd:boolean ;
        schema:domainIncludes  <https://w3id.org/product/ProtectiveDeviceTrippingUnit%2FELECTRONIC> .

props:ladderTrussLength
        a                      owl:DatatypeProperty ;
        rdfs:comment           "The overall length of the truss connector."@en , "トラス接続部材の全体の長さ。"@ja-JP , "트러스 연결 부재의 전체 길이"@ko-KR ;
        rdfs:label             "ladderTrussLength"@en , "全体長さ"@ja-JP , "전체길이"@ko-KR ;
        rdfs:range             <https://w3id.org/product/PositiveLengthMeasure> ;
        schema:domainIncludes  <https://w3id.org/product/DiscreteAccessory%2FLadder%20truss%20connector> .

props:securityLightingType
        a                      owl:DatatypeProperty ;
        rdfs:comment           "The type of security lighting."@en , "防犯灯のタイプ。"@ja-JP , "방범등 유형"@ko-KR ;
        rdfs:label             "securityLightingType"@en , "防犯灯"@ja-JP , "방범등"@ko-KR ;
        schema:domainIncludes  <https://w3id.org/product/LightFixture%2FSECURITYLIGHTING> .

props:shearDeformationAreaY
        a                      owl:DatatypeProperty ;
        rdfs:comment           "Area of the profile for calculating the shear deformation due to a shear force parallel to ys. For example measured in mm². If given, the shear deformation area ys shall be non-negative."@en ;
        rdfs:label             "shearDeformationAreaY"@en ;
        rdfs:range             <https://w3id.org/product/AreaMeasure> ;
        schema:domainIncludes  <https://w3id.org/product/ProfileDef> .

props:atexVerified  a          owl:DatatypeProperty ;
        rdfs:comment           "An indication whether the tripping_unit is verified to be applied in EX-environment or not."@en , "トリップ装置がEX-環境で適用されるかどうか。"@ja-JP , "트립 장치가 EX-환경에 적용되는지 여부"@ko-KR ;
        rdfs:label             "atexVerified"@en , "アテックス認証"@ja-JP , "EX -환경 인증"@ko-KR ;
        rdfs:range             xsd:boolean ;
        schema:domainIncludes  <https://w3id.org/product/ProtectiveDeviceTrippingUnit> .

props:powerLoss  a             owl:DatatypeProperty ;
        rdfs:comment           "Total loss of power across this cable."@en , "The power loss in [W] of the fuse when the nominal current is flowing through the fuse."@en , "定格電流がヒューズに流れる時の電力損失[W]。"@ja-JP , "정격 전류가 MCB 흐르고있을 때의 MCB 극 당 전력 손실 [W]."@ko-KR , "정격 전류가 퓨즈에 흐르는시 전력 손실 [W]."@ko-KR , "The power loss in [W] per pole of the MCB  when the nominal current is flowing through the MCB."@en , "定格電流がMCBに流れている時のMCBの極当たりの電力損失[W]。"@ja-JP ;
        rdfs:label             "powerLoss"@en , "電力損失"@ja-JP , "전력 손실"@ko-KR ;
        rdfs:range             <https://w3id.org/product/PowerMeasure> , <https://w3id.org/product/ElectricCurrentMeasure> ;
        schema:domainIncludes  <https://w3id.org/product/ProtectiveDevice%2FCIRCUITBREAKER> , <https://w3id.org/product/CableSegment> , <https://w3id.org/product/ProtectiveDevice%2FFUSEDISCONNECTOR> .

props:hasPartWinding  a        owl:DatatypeProperty ;
        rdfs:comment           "Indication of whether the motor is single speed, i.e. has a single winding (= FALSE) or multi-speed i.e.has part winding (= TRUE) ."@en , "モータが単一の速度であるかどうかを示す。例えば、単巻線、マルチスピード、分割巻線。"@ja-JP , "모터가 단일 속도인지 여부를 나타내는 예를 들어, 단일 권선, 다중 속도 분할 권선"@ko-KR ;
        rdfs:label             "hasPartWinding"@en , "巻線　"@ja-JP , "권선"@ko-KR ;
        rdfs:range             xsd:boolean ;
        schema:domainIncludes  <https://w3id.org/product/ElectricMotor> .

props:backflowPreventerType
        a                      owl:DatatypeProperty ;
        rdfs:comment           "Identifies the type of backflow preventer installed to prevent the backflow of contaminated or polluted water from an irrigation/reticulation system to a potable water supply."@en ;
        rdfs:label             "backflowPreventerType"@en ;
        schema:domainIncludes  <https://w3id.org/product/FlowMeter%2FWATERMETER> .

props:dimmerType  a            owl:DatatypeProperty ;
        rdfs:comment           "A list of the available types of dimmer switch from which that required may be selected."@en , "選択が必要となる、ディマースイッチの一覧リスト。"@ja-JP , "선택이 필요한 조광기 스위치 목록"@ko-KR ;
        rdfs:label             "dimmerType"@en , "ディマータイプ"@ja-JP , "조광기 유형"@ko-KR ;
        schema:domainIncludes  <https://w3id.org/product/SwitchingDevice%2FDIMMERSWITCH> .

props:expectedServiceLife
        a                      owl:DatatypeProperty ;
        rdfs:comment           "数年間の期待される耐用年数。"@ja-JP , "Expected service life in years."@en , "Durée de vie typique exprimée en années."@fr-FR , "예상 수명"@ko-KR ;
        rdfs:label             "expectedServiceLife"@en , "DureeDeVieTypique"@fr-FR , "예상수명"@ko-KR , "期待される耐用期間"@ja-JP ;
        rdfs:range             <https://w3id.org/product/TimeMeasure> ;
        schema:domainIncludes  <https://w3id.org/product/Element> .

props:workDayDuration
        a                      owl:DatatypeProperty ;
        rdfs:comment           "The elapsed time within a worktime-based day. For presentation purposes, applications may choose to display IfcTask durations in work days where IfcTaskTime.DurationType=WORKTIME. This value must be less than or equal to 24 hours (an elapsed day); if omitted then 8 hours is assumed."@en , "作業時間を基にした、経過時間の日数。"@ja-JP ;
        rdfs:label             "workDayDuration"@en , "作業日数"@ja-JP ;
        rdfs:range             xsd:duration ;
        schema:domainIncludes  <https://w3id.org/product/WorkControl> .

props:hasLock  a               owl:DatatypeProperty ;
        rdfs:comment           "Indication of whether a switching device has a key operated lock (=TRUE) or not (= FALSE)."@en , "スイッチ装置がキー操作でロックする場合は（TRUE)、そうでない場合は（FALSE)を表す。"@ja-JP , "스위치 장치가 키 조작으로 잠글 경우 (TRUE), 그렇지 않은 경우 (FALSE)을 나타낸다."@ko-KR ;
        rdfs:label             "hasLock"@en , "ロックの可否"@ja-JP , "잠금여부"@ko-KR ;
        rdfs:range             xsd:boolean ;
        schema:domainIncludes  <https://w3id.org/product/SwitchingDevice> .

props:camberAtMidspan
        a                      owl:DatatypeProperty ;
        rdfs:comment           "The camber deflection, measured from the midpoint of a cambered face of a piece to the midpoint of the chord joining the ends of the same face, as shown in the figure below, divided by the original (nominal) straight length of the face of the piece."@en ;
        rdfs:label             "camberAtMidspan"@en ;
        rdfs:range             <https://w3id.org/product/RatioMeasure> ;
        schema:domainIncludes  <https://w3id.org/product/BuildingElement> .

props:backupSupplySystem
        a                      owl:DatatypeProperty ;
        rdfs:comment           "The type of backup supply system."@en , "電源バックアップシステムのタイプ。"@ja-JP , "전원 백업 시스템 유형"@ko-KR ;
        rdfs:label             "backupSupplySystem"@en , "電源バックアップシステム"@ja-JP , "전원백업 시스템"@ko-KR ;
        schema:domainIncludes  <https://w3id.org/product/LightFixture%2FSECURITYLIGHTING> .

props:budgetSource  a          owl:DatatypeProperty ;
        rdfs:comment           "The budget source requested."@en , "要求された予算の出所・源。"@ja-JP ;
        rdfs:label             "budgetSource"@en , "予算源"@ja-JP ;
        rdfs:range             xsd:string ;
        schema:domainIncludes  <https://w3id.org/product/ProjectOrder%2FCHANGEORDER> .

props:sprinklerProtectionAutomatic
        a                      owl:DatatypeProperty ;
        rdfs:comment           "Indication whether this object has an automatic sprinkler protection (TRUE) or not (FALSE)."@en , "스프링 클러 설비가 자동 여부를 나타내는 부울 값입니다. (TRUE) 자동 (FALSE) 비자동. \"스프링 클러 방어\"속성이 TRUE로 설정된 경우에만 주어진다."@ko-KR , "Angabe, ob der Raum durch eine automatische Sprinkleranlage geschützt wird (WAHR) oder nicht (FALSCH).  Dieser Wert soll nur angegeben werden, wenn das Attribut SprinklerProtection auf (WAHR) gesetzt ist."@de-DE , "스프링 클러 설비가 자동 여부를 나타내는 값"@ko-KR , "Indication whether this object has an automatic sprinkler protection (TRUE) or not (FALSE).\nIt should only be given, if the property \"SprinklerProtection\" is set to TRUE."@en , "Indication selon laquelle ce bâtiment bénéficie d'une protection automatique par sprinkler (VRAI) ou non (FAUX)."@fr-FR , "Indication selon laquelle ce bâtiment bénéficie d'une protection automatique par sprinkler (VRAI) ou non (FAUX). Indication à ne fournir que si la propriété \"SprinklerProtection\" est cochée \"VRAI\"."@fr-FR , "Angabe, ob das Geschoss durch eine automatische Sprinkleranlage geschützt wird (WAHR) oder nicht (FALSCH)."@de-DE , "Angabe, ob das Gebäude durch eine automatische Sprinkleranlage geschützt wird (WAHR) oder nicht (FALSCH)."@de-DE , "スプリンクラー設備が自動かどうか示すブーリアン値。(TRUE)自動、(FALSE)非自動。「スプリンクラー防御」プロパティがTRUEに設定された場合のみ、与えられる。"@ja-JP , "スプリンクラー設備が自動かどうか示すブーリアン値。"@ja-JP , "Indication whether the space has an automatic sprinkler protection (TRUE) or not (FALSE).\nIt should only be given, if the property \"SprinklerProtection\" is set to TRUE."@en ;
        rdfs:label             "自動スプリンクラー防御"@ja-JP , "스프링 클러 방어 자동 구분"@ko-KR , "sprinklerProtectionAutomatic"@en , "Sprinklerschutz automatisch"@de-DE , "スプリンクラー防御自動区分"@ja-JP , "ProtectionAutomatiqueParSprinkler"@fr-FR ;
        rdfs:range             xsd:boolean ;
        schema:domainIncludes  <https://w3id.org/product/cZone> , <https://w3id.org/product/Building> , <https://w3id.org/product/cSpatialZone> , <https://w3id.org/product/BuildingStorey> , <https://w3id.org/product/Space> .

props:infiltrationDiversitySummer
        a                      owl:DatatypeProperty ;
        rdfs:comment           "Diversity factor for Summer infiltration."@en , "여름 틈새 환기 비율."@ko-KR , "여름 틈새 환기 비율"@ko-KR , "夏期すき間換気率。"@ja-JP ;
        rdfs:label             "여름 틈새 환기 비율"@ko-KR , "夏期すき間換気率"@ja-JP , "infiltrationDiversitySummer"@en , "여름틈새 환기 비율"@ko-KR ;
        rdfs:range             <https://w3id.org/product/PositiveRatioMeasure> ;
        schema:domainIncludes  <https://w3id.org/product/SpatialElement> , <https://w3id.org/product/SpatialZone> , <https://w3id.org/product/Zone> , <https://w3id.org/product/Space> .

props:setPointIlluminance
        a                      owl:DatatypeProperty ;
        rdfs:comment           "The illuminance value to be sensed. Use IfcPropertyBoundedValue.SetPointValue to set the set point value."@en , "感知される照度。\nセットポイント値を置くために、IfcPropertyBoundedValue.SetPointValueを使用する。"@ja-JP , "감지하는 조도. 세트 포인트 값을 넣으려면, IfcPropertyBoundedValue.SetPointValue를 사용하십시오."@ko-KR ;
        rdfs:label             "setPointIlluminance"@en , "照度設定値"@ja-JP , "조도 설정"@ko-KR ;
        schema:domainIncludes  <https://w3id.org/product/Sensor%2FLIGHTSENSOR> .

props:secondaryCurrent
        a                      owl:DatatypeProperty ;
        rdfs:comment           "The current that has been transformed and is running out of the transformer on the secondary side."@en , "変圧器の2次側へ出力される電流。"@ja-JP , "변압기 2 차 측에 전송되는 전류."@ko-KR ;
        rdfs:label             "secondaryCurrent"@en , "第2電流"@ja-JP , "제 2 전류"@ko-KR ;
        rdfs:range             <https://w3id.org/product/ElectricCurrentMeasure> ;
        schema:domainIncludes  <https://w3id.org/product/Transformer> .

props:numberOfPlates  a        owl:DatatypeProperty ;
        rdfs:comment           "Number of plates used by the plate heat exchanger."@en , "プレート式熱交換器に使われているプレート数"@ja-JP ;
        rdfs:label             "numberOfPlates"@en , "プレート数"@ja-JP ;
        rdfs:range             xsd:int ;
        schema:domainIncludes  <https://w3id.org/product/HeatExchanger%2FPLATE> .

props:backInletPatternType
        a                      owl:DatatypeProperty ;
        rdfs:comment           "Identifies the pattern of inlet connections to a gully trap.\n\nA gulley trap may have 0,1,2,3 or 4 inlet connections and the pattern of their arrangement may vary. The enumeration makes the convention that an outlet is either vertical or is placed at the bottom (south side) of the gully trap (when viewed in plan). Position 1 is to the left (west), position 2 is to the top (north), position 3 is to the right (east) and position 4 is to the bottom (south)."@en , "Identifies the pattern of inlet connections to a gully trap.\n\nA gulley trap may have 0,1,2,3 or 4 inlet connections and the pattern of their arrangement may vary. The enumeration makes the convention that an outlet is either vertical or is placed at the bottom (south side) of the gully trap (when viewed in plan). Position 1 is to the left (west), position 2 is to the top (north), position 3 is to the right (east) and position 4 is to the bottom (south).\n\n               2\n               |\n   ----------------\n   !                       |\n1-|                       |-3\n   !                       |\n   ----------------\n               |\n              4"@en , "溝防臭弁の吸気口パターンを確認してください。\n\n一つの溝防臭弁に0.1.2.3.4.の吸気口接続口とパターンがあるときは変化する可能性があります。表記されるときは、接続口が垂直である様子か、防臭弁の底（南）におかれます。位置1は左(西)に、位置2は上方(北)に、位置3は右(東)に、位置4は下方(南）になります。"@ja-JP ;
        rdfs:label             "backInletPatternType"@en , "背部接続口種類"@ja-JP ;
        schema:domainIncludes  <https://w3id.org/product/WasteTerminal%2FGULLYTRAP> , <https://w3id.org/product/WasteTerminal%2FGULLYSUMP> .

props:videoCaptureInterval
        a                      owl:DatatypeProperty ;
        rdfs:comment           "Indicates video frame capture time intervals."@en , "撮影間隔を示す。"@ja-JP ;
        rdfs:label             "videoCaptureInterval"@en , "撮影間隔"@ja-JP ;
        schema:domainIncludes  <https://w3id.org/product/AudioVisualAppliance%2FCAMERA> .

props:nominalBodyLength
        a                      owl:DatatypeProperty ;
        rdfs:comment           "Nominal or quoted length measured along the x-axis in the local coordinate system or the radius (in the case of a circular shape in plan) of the chamber of the trap."@en , "Nominal or quoted length, measured along the x-axis of the local coordinate system of the object, of the body of the object."@en , "溝防臭弁の半径か局所座標系のＸ軸に沿って測定された呼称もしくは積算された長さ。"@ja-JP , "半径か局所座標系のＸ軸に沿って測定された呼称もしくは積算された配管の長さ。"@ja-JP , "Nominal or quoted length measured along the x-axis in the local coordinate system or the radius (in the case of a circular shape in plan) of the drain."@en , "Nominal or quoted length measured along the x-axis in the local coordinate system or the radius (in the case of a circular shape in plan) of the chamber of the gully trap."@en , "Nominal or quoted length measured along the x-axis in the local coordinate system or the radius (in the case of a circular shape in plan) of the waste."@en , "廃棄物の区画の半径か局所座標系のＸ軸に沿って測定された呼称もしくは積算された長さ。"@ja-JP , "防臭弁の区画の半径か局所座標系のＸ軸に沿って測定された呼称もしくは積算された長さ。"@ja-JP ;
        rdfs:label             "呼称躯体長"@ja-JP , "nominalBodyLength"@en ;
        rdfs:range             <https://w3id.org/product/PositiveLengthMeasure> ;
        schema:domainIncludes  <https://w3id.org/product/WasteTerminal%2FGULLYTRAP> , <https://w3id.org/product/WasteTerminal%2FFLOORWASTE> , <https://w3id.org/product/Interceptor> , <https://w3id.org/product/WasteTerminal%2FFLOORTRAP> , <https://w3id.org/product/WasteTerminal%2FROOFDRAIN> .

props:isOffWhenSFunctionOn
        a                      owl:DatatypeProperty ;
        rdfs:comment           "Indication whether the I-function is automatically switched off when the S-function is switched on."@en ;
        rdfs:label             "isOffWhenSFunctionOn"@en ;
        rdfs:range             xsd:boolean ;
        schema:domainIncludes  <https://w3id.org/product/ProtectiveDeviceTrippingUnit> .

props:nominalWidthOrDiameter
        a                      owl:DatatypeProperty ;
        rdfs:comment           "The nominal width or, in the case of a horizontal cylindrical tank, the nominal diameter of the tank.\n\nNote: Not required for a vertical cylindrical tank."@en , "公称幅又は水平円筒形タンクの場合、タンクの公称直径　　　　　注：垂直円筒形タンクに対しては必須ではない"@ja-JP ;
        rdfs:label             "nominalWidthOrDiameter"@en , "公称幅又は直径"@ja-JP ;
        rdfs:range             <https://w3id.org/product/PositiveLengthMeasure> ;
        schema:domainIncludes  <https://w3id.org/product/Tank> .

props:cornerFixingPlateFlangeWidthInPlaneZ
        a                      owl:DatatypeProperty ;
        rdfs:comment           "The flange width of the L-shaped corner plate in plane Z."@en , "L型コーナープレートのZ面のフランジ幅。"@ja-JP , "L 형 코너 플레이트 Z면 플랜지 폭"@ko-KR ;
        rdfs:label             "cornerFixingPlateFlangeWidthInPlaneZ"@en , "フランジ幅Z"@ja-JP , "플랜지 폭 Z"@ko-KR ;
        rdfs:range             <https://w3id.org/product/PositiveLengthMeasure> ;
        schema:domainIncludes  <https://w3id.org/product/DiscreteAccessory%2FCorner%20fixing%20plate> .

props:withBackdrop  a          owl:DatatypeProperty ;
        rdfs:comment           "Indicates whether the chamber has a backdrop or tumbling bay (TRUE) or not (FALSE)."@en , "ダクトスペースはバックドロップ或いは堰付けかどうか（TRUE或いはFALSE）。"@ja-JP , "덕트 공간 백드롭 혹은 보 표시 여부 (TRUE 또는 FALSE)"@ko-KR ;
        rdfs:label             "バックドロップ付け"@ja-JP , "withBackdrop"@en , "백 드롭 지정"@ko-KR ;
        rdfs:range             xsd:boolean ;
        schema:domainIncludes  <https://w3id.org/product/DistributionChamberElement%2FMANHOLE> , <https://w3id.org/product/DistributionChamberElement%2FINSPECTIONCHAMBER> .

props:setPointPH  a            owl:DatatypeProperty ;
        rdfs:comment           "The fill level value to be sensed. Use IfcPropertyBoundedValue.SetPointValue to set the set point value."@en , "感知される酸性度。\nセットポイント値を置くために、IfcPropertyBoundedValue.SetPointValueを使用する。"@ja-JP , "감지되는 산도. 세트 포인트 값을 넣으려면, IfcPropertyBoundedValue.SetPointValue를 사용하십시오."@ko-KR ;
        rdfs:label             "setPointPH"@en , "酸性度設定値"@ja-JP , "산성도 설정"@ko-KR ;
        schema:domainIncludes  <https://w3id.org/product/Sensor%2FPHSENSOR> .

props:nominalWidth  a          owl:DatatypeProperty ;
        rdfs:comment           "要素の幅。"@ja-JP , "The nominal width or diameter of the duct connection."@en , "The nominal width of the segment."@en , "The nominal width of the system furniture elements of this type. The size information is provided in addition to the shape representation and the geometric parameters used within. In cases of inconsistency between the geometric parameters and the size properties, provided in the attached property set, the geometric parameters take precedence."@en , "公称または引用幅。"@ja-JP , "폭 치수"@ko-KR , "呼び幅寸法。"@ja-JP , "폭 치수."@ko-KR , "Nominal or quoted width of the object."@en ;
        rdfs:label             "공칭 폭"@ko-KR , "呼び幅"@ja-JP , "幅"@ja-JP , "公称幅"@ja-JP , "nominalWidth"@en ;
        rdfs:range             <https://w3id.org/product/PositiveLengthMeasure> ;
        schema:domainIncludes  <https://w3id.org/product/SystemFurnitureElement> , <https://w3id.org/product/DistributionPort%2FAIRCONDITIONING> , <https://w3id.org/product/CableCarrierSegment%2FCONDUITSEGMENT> , <https://w3id.org/product/SanitaryTerminal%2FTOILETPAN> , <https://w3id.org/product/SanitaryTerminal%2FURINAL> , <https://w3id.org/product/SanitaryTerminal%2FBIDET> , <https://w3id.org/product/SanitaryTerminal%2FSINK> , <https://w3id.org/product/CableCarrierSegment%2FCABLETRUNKINGSEGMENT> , <https://w3id.org/product/SanitaryTerminal%2FBATH> , <https://w3id.org/product/SanitaryTerminal%2FSHOWER> , <https://w3id.org/product/CableCarrierSegment%2FCABLELADDERSEGMENT> , <https://w3id.org/product/CableCarrierSegment%2FCABLETRAYSEGMENT> , <https://w3id.org/product/SanitaryTerminal%2FWASHHANDBASIN> , <https://w3id.org/product/SanitaryTerminal%2FSANITARYFOUNTAIN> .

props:occupancyDiversity
        a                      owl:DatatypeProperty ;
        rdfs:comment           "Diversity factor that may be applied to the number of people in the space."@en , "室内居住者の在室率。"@ja-JP , "실내 거주자의 재실 비율."@ko-KR ;
        rdfs:label             "occupancyDiversity"@en , "居住者の在室率"@ja-JP , "거주자의 재실 비율"@ko-KR ;
        rdfs:range             <https://w3id.org/product/PositiveRatioMeasure> ;
        schema:domainIncludes  <https://w3id.org/product/SpatialElement> .

props:currentToleranceLimit1
        a                      owl:DatatypeProperty ;
        rdfs:comment           "The time limit in [s] limiting the application of CurrentTolerance1, if any. If the value is set to 0, the value of the CurrentTolerance1 is valid for the whole time/current-curve."@en , "許容電流1を制限する時間制限。\n値が0の場合は、制限はない。"@ja-JP , "허용 전류 1 제한 시간 제한. 값이 0이면 제한이 없다."@ko-KR ;
        rdfs:label             "currentToleranceLimit1"@en , "許容電流限界1"@ja-JP , "허용전류한계1"@ko-KR ;
        rdfs:range             <https://w3id.org/product/TimeMeasure> ;
        schema:domainIncludes  <https://w3id.org/product/ProtectiveDeviceTrippingUnit> .

props:accuracyOfFireSensor
        a                      owl:DatatypeProperty ;
        rdfs:comment           "The accuracy of the sensor."@en , "センサの精度。"@ja-JP , "센서의 정밀도."@ko-KR ;
        rdfs:label             "accuracyOfFireSensor"@en , "精度"@ja-JP , "정확도"@ko-KR ;
        rdfs:range             <https://w3id.org/product/ThermodynamicTemperatureMeasure> ;
        schema:domainIncludes  <https://w3id.org/product/Sensor%2FFIRESENSOR> .

props:tenureModesAvailableNow
        a                      owl:DatatypeProperty ;
        rdfs:comment           "A list of the tenure modes that are currently available expressed in terms of IfcLabel."@en , "Liste des possibilités d'occupation actuelles."@fr-FR ;
        rdfs:label             "tenureModesAvailableNow"@en , "PossibilitesOccupationActuelles"@fr-FR ;
        schema:domainIncludes  <https://w3id.org/product/Building> .

props:finCorrugatedType
        a                      owl:DatatypeProperty ;
        rdfs:comment           "Description of a fin corrugated type."@en , "コルゲートタイプフィンの実直径"@ja-JP ;
        rdfs:label             "finCorrugatedType"@en , "コルゲートタイプフィン"@ja-JP ;
        rdfs:range             xsd:string ;
        schema:domainIncludes  <https://w3id.org/product/TubeBundle%2FFINNED> .

props:batterAtEnd  a           owl:DatatypeProperty ;
        rdfs:comment           "The angle, in radians, by which the formwork at the ending face of a piece is to be rotated from the vertical in order to compensate for the rotation of the face that will occur once the piece is stripped from its form, inducing camber due to eccentric prestressing."@en ;
        rdfs:label             "batterAtEnd"@en ;
        rdfs:range             <https://w3id.org/product/PlaneAngleMeasure> ;
        schema:domainIncludes  <https://w3id.org/product/BuildingElement> .

props:user  a                  owl:DatatypeProperty ;
        rdfs:comment           "Indicates acknowledging user over time by identification corresponding to IfcPerson.Identification on an IfcActor."@en ;
        rdfs:label             "user"@en ;
        schema:domainIncludes  <https://w3id.org/product/Alarm> .

props:workability  a           owl:DatatypeProperty ;
        rdfs:comment           "Description of the workability of the fresh concrete defined according to local standards."@en ;
        rdfs:label             "workability"@en ;
        rdfs:range             xsd:string ;
        schema:domainIncludes  <https://w3id.org/product/Material%2FConcrete> .

props:supplyAirConnectionType
        a                      owl:DatatypeProperty ;
        rdfs:comment           "The manner in which the pipe connection is made to the cooled beam."@en ;
        rdfs:label             "supplyAirConnectionType"@en ;
        schema:domainIncludes  <https://w3id.org/product/CooledBeam%2FACTIVE> .

props:maximumCurrent  a        owl:DatatypeProperty ;
        rdfs:comment           "The maximum allowed current that a device is certified to handle."@en ;
        rdfs:label             "maximumCurrent"@en ;
        rdfs:range             <https://w3id.org/product/ElectricCurrentMeasure> ;
        schema:domainIncludes  <https://w3id.org/product/FlowMeter%2FENERGYMETER> .

props:treadLength  a           owl:DatatypeProperty ;
        rdfs:comment           "Longueur de giron (largeur de marche), supposée égale pour toutes les marches de l'escalier ou de la volée de marchesle long de la ligne de foulée"@fr-FR , "踏面の前面部分から次の踏面までの水平方向の距離。この踏面長の値は、一連の階段において同じ値と仮定する。"@ja-JP , "German-description-5"@de-DE , "踏板前缘到下一级踏板前缘的水平距离。\n走线方向上楼梯或梯段所有梯级的踏板宽度应当一致。"@zh-CN , "Horizontal distance from the front of the thread to the front of the next tread. \nThe tread length is supposed to be equal for all steps of the stair or stair flight at the walking line."@en ;
        rdfs:label             "踏板长度"@zh-CN , "treadLength"@en , "踏面長"@ja-JP , "LongueurGiron"@fr-FR , "Auftritt"@de-DE ;
        rdfs:range             <https://w3id.org/product/PositiveLengthMeasure> ;
        schema:domainIncludes  <https://w3id.org/product/StairFlight> , <https://w3id.org/product/Stair> .

props:workingPressure
        a                      owl:DatatypeProperty ;
        rdfs:comment           "Pression de fonctionnement de la chaudière."@fr-FR , "ボイラ運転圧力"@ja-JP , "Boiler working pressure."@en , "バルブの通常予想される最高運転圧力"@ja-JP , "Working pressure."@en , "動作圧"@ja-JP , "管轄権を持つ当局（SMACNAなど）によって定義された圧力分類"@ja-JP , "Pressure classification as defined by the authority having jurisdiction (e.g., SMACNA, etc.)."@en , "The normally expected maximum working pressure of the valve."@en ;
        rdfs:label             "運転圧力"@ja-JP , "workingPressure"@en , "圧力クラス"@ja-JP , "動作圧"@ja-JP , "作動圧力"@ja-JP , "PressionFonctionnement"@fr-FR ;
        rdfs:range             <https://w3id.org/product/PressureMeasure> ;
        schema:domainIncludes  <https://w3id.org/product/Valve> , <https://w3id.org/product/DuctSegment> , <https://w3id.org/product/PipeSegment> , <https://w3id.org/product/Boiler> .

props:tunerType  a             owl:DatatypeProperty ;
        rdfs:comment           "Indicates the tuner type."@en , "チューナータイプを示す。"@ja-JP , "튜너 타입을 나타낸다"@ko-KR ;
        rdfs:label             "tunerType"@en , "チューナータイプ"@ja-JP , "튜너 타입"@ko-KR ;
        schema:domainIncludes  <https://w3id.org/product/AudioVisualAppliance%2FTUNER> .

props:switchActivation
        a                      owl:DatatypeProperty ;
        rdfs:comment           "選択が必要となる、トグルスイッチの起動方式の一覧リスト。"@ja-JP , "A list of the available activations for selector switches from which that required may be selected."@en , "스위치 부팅방식의 목록"@ko-KR , "A list of the available activations for toggle switches from which that required may be selected."@en , "선택이 필요한 토글 스위치 부팅 방식의 목록"@ko-KR , "選択が必要となる、切替えスイッチの起動方式の一覧リスト。"@ja-JP ;
        rdfs:label             "기동 방식"@ko-KR , "起動方式"@ja-JP , "switchActivation"@en ;
        schema:domainIncludes  <https://w3id.org/product/SwitchingDevice%2FTOGGLESWITCH> , <https://w3id.org/product/SwitchingDevice%2FSELECTORSWITCH> .

props:n_Protection_Select
        a                      owl:DatatypeProperty ;
        rdfs:comment           "An indication whether the use of the N_Protection can be selected by the user or not. If both the properties N_Protection_50 and N_Protection_100 are asserted, the value of N_Protection_Select property is set to TRUE. The property is only asserted if the property N_Protection is asserted."@en , "どのN_Protectionを使うかユーザが設定できるかどうかを指定する。\nN_Protection_50とN_Protection_100の両方が有効な場合は、TRUEにします。"@ja-JP , "어떤 N_Protection를 사용하거나 사용자가 설정할 수 있는지 여부를 지정합니다. N_Protection_50하면 N_Protection_100를 모두 사용할 경우에는 TRUE합니다."@ko-KR ;
        rdfs:label             "n_Protection_Select"@en , "N_Protectionの選択"@ja-JP , "N_Protection 선택"@ko-KR ;
        rdfs:range             xsd:boolean ;
        schema:domainIncludes  <https://w3id.org/product/ProtectiveDeviceTrippingUnit%2FELECTRONIC> .

props:workingPressureRange
        a                      owl:DatatypeProperty ;
        rdfs:comment           "Allowable minimum and maximum  working pressure (relative to ambient pressure)."@en , "許容最小・最大作動圧力（周囲圧との相対値）"@ja-JP ;
        rdfs:label             "workingPressureRange"@en , "作動圧力範囲"@ja-JP ;
        schema:domainIncludes  <https://w3id.org/product/DuctSilencer> .

props:applicationOfFan
        a                      owl:DatatypeProperty ;
        rdfs:comment           "The functional application of the fan.\n\nSupplyAir: Supply air fan. \nReturnAir: Return air fan. \nExhaustAir: Exhaust air fan. \nOther: Other type of application not defined above."@en , "Fanの系統\nSUPPLYAIR, RETURNAIR, EXHAUSTAIR, COOLINGTOWER, OTHER"@ja-JP ;
        rdfs:label             "applicationOfFan"@en , "Fan用途"@ja-JP ;
        schema:domainIncludes  <https://w3id.org/product/Fan> .

props:faceType  a              owl:DatatypeProperty ;
        rdfs:comment           "Identifies how the terminal face of an AirTerminal is constructed."@en , "ターミナル表面の形式定義"@ja-JP , "Caractérise comment le côté du terminal d'un terminal de ventilation est fabriqué."@fr-FR ;
        rdfs:label             "faceType"@en , "表面タイプ"@ja-JP , "TypeCôté"@fr-FR ;
        schema:domainIncludes  <https://w3id.org/product/AirTerminal> .

props:nominalSupplyVoltage
        a                      owl:DatatypeProperty ;
        rdfs:comment           "The nominal voltage of the supply."@en , "電源の公称電圧。"@ja-JP , "전원 공칭 주파수"@ko-KR ;
        rdfs:label             "nominalSupplyVoltage"@en , "公称電圧"@ja-JP , "공칭 주파수"@ko-KR ;
        rdfs:range             <https://w3id.org/product/ElectricVoltageMeasure> ;
        schema:domainIncludes  <https://w3id.org/product/ElectricFlowStorageDevice> .

props:dimensionalAccuracyClass
        a                      owl:DatatypeProperty ;
        rdfs:comment           "Classification designation of the dimensional accuracy requirement according to local standards."@en , "国の基準が求める寸法精度の分類指定。"@ja-JP , "국가 표준이 요구하는 치수 정밀도의 분류 지정"@ko-KR ;
        rdfs:label             "dimensionalAccuracyClass"@en , "寸法精度クラス"@ja-JP , "치수 정밀도 클래스"@ko-KR ;
        rdfs:range             xsd:string ;
        schema:domainIncludes  <https://w3id.org/product/BuildingElement> .

props:nominalFilterFaceVelocity
        a                      owl:DatatypeProperty ;
        rdfs:comment           "Filter face velocity."@en ;
        rdfs:label             "nominalFilterFaceVelocity"@en ;
        rdfs:range             <https://w3id.org/product/LinearVelocityMeasure> ;
        schema:domainIncludes  <https://w3id.org/product/Filter> .

props:stroke  a                owl:DatatypeProperty ;
        rdfs:comment           "Indicates the maximum distance the actuator must traverse."@en , "アクチュエータが動く最大距離を示す。"@ja-JP , "액츄에이터가 움직이는 최대 거리를 보여준다."@ko-KR ;
        rdfs:label             "stroke"@en , "ストローク"@ja-JP , "입력"@ko-KR ;
        rdfs:range             <https://w3id.org/product/LengthMeasure> ;
        schema:domainIncludes  <https://w3id.org/product/Actuator> .

props:isWired  a               owl:DatatypeProperty ;
        rdfs:comment           "Indique si le verre est un verre armé à maille anti-effraction (VRAI) ou non (FAUX)"@fr-FR , "不法侵入防止の網入りガラスか（TRUE)否か（FALSE）示す。"@ja-JP , "表示玻璃是否具有防断裂的纤维网格。"@zh-CN , "Indication whether the glass includes a contained wire mesh to prevent break-in (TRUE) or not (FALSE)"@en , "German-description-10"@de-DE ;
        rdfs:label             "是否夹丝"@zh-CN , "German-name-10"@de-DE , "網入りガラス"@ja-JP , "VitrageArme"@fr-FR , "isWired"@en ;
        rdfs:range             xsd:boolean ;
        schema:domainIncludes  <https://w3id.org/product/cWindow> , <https://w3id.org/product/Door> .

props:nominalCoolingCapacity
        a                      owl:DatatypeProperty ;
        rdfs:comment           "Nominal cooling capacity."@en ;
        rdfs:label             "nominalCoolingCapacity"@en ;
        rdfs:range             <https://w3id.org/product/PowerMeasure> ;
        schema:domainIncludes  <https://w3id.org/product/CooledBeam> .

props:centerCoreTopHeight
        a                      owl:DatatypeProperty ;
        rdfs:comment           "Center core top height of the profile."@en ;
        rdfs:label             "centerCoreTopHeight"@en ;
        rdfs:range             <https://w3id.org/product/PositiveLengthMeasure> ;
        schema:domainIncludes  <https://w3id.org/product/ArbitraryProfileDefWithVoids> .

props:airPressureRange
        a                      owl:DatatypeProperty ;
        rdfs:comment           "Allowable air static pressure range at the entrance of the air terminal box."@en , "ターミナル入り口での許容静圧範囲"@ja-JP , "Plage admise de la pression statique de l'air à l'entrée du registre terminal de ventilation"@fr-FR ;
        rdfs:label             "airPressureRange"@en , "空気圧範囲"@ja-JP , "Plage de pression d'air"@fr-FR ;
        schema:domainIncludes  <https://w3id.org/product/AirTerminalBox> .

props:fractionOfMotorHeatToAirStream
        a                      owl:DatatypeProperty ;
        rdfs:comment           "Fraction of the motor heat released into the fluid flow."@en , "流体中にモーター発熱が放出される場合にTRUE"@ja-JP ;
        rdfs:label             "fractionOfMotorHeatToAirStream"@en , "モーター排熱"@ja-JP ;
        rdfs:range             <https://w3id.org/product/NormalisedRatioMeasure> ;
        schema:domainIncludes  <https://w3id.org/product/Fan> .

props:dataTransmitted
        a                      owl:DatatypeProperty ;
        rdfs:comment           "For data ports, captures log of data transmitted.  The LIST at IfcTimeSeriesValue.Values may split out data according to Pset_DistributionPortTypeCable.Protocols."@en , "発信データのログ。IfcTimeSeriesValue.Valuesのリスト値にはPset_DistributionPortTypeCable.Protocolsよりデータを送信する。"@ja ;
        rdfs:label             "dataTransmitted"@en , "発信"@ja ;
        schema:domainIncludes  <https://w3id.org/product/DistributionPort%2FELECTRICAL> .

props:ladderTrussCrossBarDiameter
        a                      owl:DatatypeProperty ;
        rdfs:comment           "The nominal diameter of the straight cross-bars."@en , "まっすぐなクロスバーの公称直径。"@ja-JP , "똑바른 크로스바 공칭 지름"@ko-KR ;
        rdfs:label             "ladderTrussCrossBarDiameter"@en , "クロスバー径"@ja-JP , "크로스바 지름"@ko-KR ;
        rdfs:range             <https://w3id.org/product/PositiveLengthMeasure> ;
        schema:domainIncludes  <https://w3id.org/product/DiscreteAccessory%2FLadder%20truss%20connector> .

props:externalShadingCoefficient
        a                      owl:DatatypeProperty ;
        rdfs:comment           "Radiation transmission coefficient of the outside shading device. It is a value without unit."@en , "外部遮阳设备的辐射透射系数。无单位。"@zh-CN , "Coefficient de transmission du rayonnement de la protection solaire extérieure. Valeur adimensionnelle."@fr-FR , "German-description-1"@de-DE ;
        rdfs:label             "外部遮阳系数"@zh-CN , "German-name-1"@de-DE , "CoefficientMasqueExterieur"@fr-FR , "externalShadingCoefficient"@en ;
        rdfs:range             <https://w3id.org/product/PositiveRatioMeasure> ;
        schema:domainIncludes  <https://w3id.org/product/Door> , <https://w3id.org/product/cWindow> .

props:inductionRatio  a        owl:DatatypeProperty ;
        rdfs:comment           "Induction ratio versus distance from the diffuser and its discharge direction; induction ratio (or entrainment ratio) is the ratio of the volumetric flow rate in the jet to the volumetric flow rate at the air terminal."@en , "制気口からの距離とその排出方向に対する誘引比、\n誘導比（または同調比）は、エアターミナルでの体積流量に対する噴流の体積流量の比である。"@ja-JP , "Taux d'induction par rapport à la distance entre le diffuseur et sa direction de rejet;\nLe taux d'induction est le rapport entre  le débit volumique d'air dans le jet sur  le débit volumique d'air au niveau du terminal."@fr-FR ;
        rdfs:label             "inductionRatio"@en , "誘引率"@ja-JP , "Taux d'induction"@fr-FR ;
        schema:domainIncludes  <https://w3id.org/product/AirTerminal> .

props:walkingLineOffset
        a                      owl:DatatypeProperty ;
        rdfs:comment           "German-description-7"@de-DE , "Décalage de la ligne de foulée par rapport au côté intérieur de la volée. Nota : la ligne de foulée peut avoir sa propre représentation. En cas d'incohérences, c'est la valeur déduite de la représentation de la forme qui prime."@fr-FR , "走线到梯段内侧的偏移量。\n注：走线可能有单独的形状描述（如果不一致，应以从形状描述得到的值为准）。"@zh-CN , "Offset of the walking line from the inner side of the flight. \nNote: the walking line may have a own shape representation (in case of inconsistencies, the value derived from the shape representation shall take precedence)."@en ;
        rdfs:label             "走线偏移"@zh-CN , "Abstand der Lauflinie"@de-DE , "walkingLineOffset"@en , "PositionLigneFoulee"@fr-FR ;
        rdfs:range             <https://w3id.org/product/PositiveLengthMeasure> ;
        schema:domainIncludes  <https://w3id.org/product/Stair> , <https://w3id.org/product/StairFlight> .

props:maxAggregateSize
        a                      owl:DatatypeProperty ;
        rdfs:comment           "The maximum aggregate size of the concrete."@en ;
        rdfs:label             "maxAggregateSize"@en ;
        rdfs:range             <https://w3id.org/product/PositiveLengthMeasure> ;
        schema:domainIncludes  <https://w3id.org/product/Material%2FConcrete> .

props:resourceDepletion
        a                      owl:DatatypeProperty ;
        rdfs:comment           "Quantité de ressources consommées exprimée en équivalent Antimoine [NDT : selon la norme NF P01-010]"@fr-FR , "算出されたアンチモンと同等な資源の量。"@ja-JP , "Quantity of resources used calculated in equivalent antimony."@en , "안티몬에 해당 환산된 사용 자원 량"@ko-KR ;
        rdfs:label             "자원 소비"@ko-KR , "EpuisementRessources"@fr-FR , "資源の枯渇"@ja-JP , "resourceDepletion"@en ;
        rdfs:range             <https://w3id.org/product/MassMeasure> ;
        schema:domainIncludes  <https://w3id.org/product/Element> .

props:isCurrentTolerancePositiveOnly
        a                      owl:DatatypeProperty ;
        rdfs:comment           "Indication whether the value of  CurrentTolerance1 is provided as a positive tolereance only  or not. If not, the value is proved as a pluss/minus tolerance."@en , "許容電流限界1の値のみかどうか\n 上記でない場合、電流許容値はプラス/マイナスした値。"@ja-JP , "허용 전류 한계 값 1 만 여부  위의 경우, 전류 허용 값은 플러스 / 마이너스 값."@ko-KR ;
        rdfs:label             "isCurrentTolerancePositiveOnly"@en , "電流許容値"@ja-JP , "전류 허용 값"@ko-KR ;
        rdfs:range             xsd:boolean ;
        schema:domainIncludes  <https://w3id.org/product/ProtectiveDeviceTrippingUnit> .

props:audioAmplification
        a                      owl:DatatypeProperty ;
        rdfs:comment           "Indicates audio amplification frequency ranges."@en , "再生周波数帯域を示す。"@ja-JP , "재생 주파수 대역을 나타낸다."@ko-KR ;
        rdfs:label             "audioAmplification"@en , "オーディオアンプ"@ja-JP , "오디오 앰프"@ko-KR ;
        schema:domainIncludes  <https://w3id.org/product/AudioVisualAppliance%2FRECEIVER> , <https://w3id.org/product/AudioVisualAppliance%2FAMPLIFIER> .

props:audioVolume  a           owl:DatatypeProperty ;
        rdfs:comment           "Indicates discrete audio volume levels and corresponding sound power offsets, if applicable.  Missing values may be interpolated."@en , "Indicates the audio volume level where the integer level corresponds to an entry or interpolation within Pset_AudioVisualApplianceTypeCommon.AudioVolume."@en ;
        rdfs:label             "audioVolume"@en ;
        schema:domainIncludes  <https://w3id.org/product/AudioVisualAppliance> .

props:integralConstant
        a                      owl:DatatypeProperty ;
        rdfs:comment           "The integral gain factor of the controller (usually referred to as Ki).  Asserted where ControlType is PROPORTIONALINTEGRAL or PROPORTIONALINTEGRALDERIVATIVE."@en , "적분 게인 (Ki)"@ko-KR ;
        rdfs:label             "integralConstant"@en , "적분 게인 (Ki)"@ko-KR ;
        rdfs:range             xsd:decimal ;
        schema:domainIncludes  <https://w3id.org/product/Controller%2FPROPORTIONAL> .

props:construction  a          owl:DatatypeProperty ;
        rdfs:comment           "Purpose of informing on how the vonductor is constucted (interwined or solid). I.e. Solid (IEV 461-01-06), stranded (IEV 461-01-07), solid-/finestranded(IEV 461-01-11) (not flexible/flexible)."@en , "導体の構成（より線か単線）の定義。すなわち単線（IEV 461-01-06）、より線（IEV 461-01-07）、フレキシブル導体（IEV 461-01-11）（フレキシブルか否か）で定義。"@ja-JP , "도체 구성 (연선 또는 단선)의 정의 즉 단선 (IEV 461-01-06), 트위스트 (IEV 461-01-07), 플렉서블 도체 (IEV 461-01-11) (유연한 아닌지 가) 정의"@ko-KR ;
        rdfs:label             "construction"@en , "構造"@ja-JP , "구조"@ko-KR ;
        schema:domainIncludes  <https://w3id.org/product/CableSegment%2FCONDUCTORSEGMENT> .

props:tunerMode  a             owl:DatatypeProperty ;
        rdfs:comment           "Indicates the tuner modes (or bands).  For example, 'AnalogCable', 'DigitalAir', 'AM', 'FM'."@en , "受信可能な放送モードを示す。"@ja-JP , "수신 가능한 방송 모드를 나타낸다."@ko-KR ;
        rdfs:label             "tunerMode"@en , "チューナーモード"@ja-JP , "튜너 모드"@ko-KR ;
        schema:domainIncludes  <https://w3id.org/product/AudioVisualAppliance%2FTUNER> .

props:compressiveStrength
        a                      owl:DatatypeProperty ;
        rdfs:comment           "The compressive strength of the concrete."@en ;
        rdfs:label             "compressiveStrength"@en ;
        rdfs:range             <https://w3id.org/product/PressureMeasure> ;
        schema:domainIncludes  <https://w3id.org/product/Material%2FConcrete> .

props:hasCoating  a            owl:DatatypeProperty ;
        rdfs:comment           "TRUE if the fin has a coating, FALSE if it does not."@en , "フィンがコーティング有りの場合 TRUE、無しの場合FALSE"@ja-JP ;
        rdfs:label             "hasCoating"@en , "コーティング有り"@ja-JP ;
        rdfs:range             xsd:boolean ;
        schema:domainIncludes  <https://w3id.org/product/TubeBundle%2FFINNED> .

props:showerType  a            owl:DatatypeProperty ;
        rdfs:comment           "Selection of the type of shower from the enumerated list of types where:-\n\nDrench:  \tShower that rapidly gives a thorough soaking in an emergency.\nIndividual: \tShower unit that is typically enclosed and is for the use of one person at a time.\nTunnel: \tShower that has a succession of shower heads or spreaders that operate simultaneously along its length."@en , "場所からのシャワータイプの選択：\n\n・水浸性：緊急時には素早く水に浸れるシャワー\n・独立性：一度に一人が使え、区切られているシャワーユニット\n・トンネル：シャワーヘッドの連続で設置されているか長さ方向に同時操作となる水散布機型のシャワー"@ja-JP ;
        rdfs:label             "showerType"@en , "シャワータイプ"@ja-JP ;
        schema:domainIncludes  <https://w3id.org/product/SanitaryTerminal%2FSHOWER> .

props:finishing  a             owl:DatatypeProperty ;
        rdfs:comment           "The finishing applied to system furniture elements of this type e.g. walnut, fabric."@en ;
        rdfs:label             "finishing"@en ;
        rdfs:range             xsd:string ;
        schema:domainIncludes  <https://w3id.org/product/SystemFurnitureElement> .

props:acousticRating  a        owl:DatatypeProperty ;
        rdfs:comment           "Schallschutzklasse gemäß der nationalen oder regionalen Schallschutzverordnung."@de-DE , "遮音等級情報。関連する建築基準法を参照。"@ja-JP , "Acoustic rating for this object.\nIt is provided according to the national building code. It indicates the sound transmission resistance of this object by an index ratio (instead of providing full sound absorbtion values)."@en , "Acoustic rating for this object.\nIt is giving according to the national building code. It indicates the sound transmission resistance of this object by an index ration (instead of providing full sound absorbtion values)."@en , "遮音等級。当該国の建築法規による。\nこのオブジェクトの音の透過損失を等級値で示す。"@ja-JP , "该构件的隔音等级。\n该属性的依据为国家建筑规范。为表示该构件隔音效果的比率（而不是完全吸收声音的值）。"@zh-CN , "Schallschutzklasse gemäß der nationalen oder regionalen Richtlinie die als Mindestanforderung für die Schalldämmung der Tür gewährleistet sein muss."@de-DE , "Classement acoustique de cet objet. Donné selon le Code National du Bâtiment. Il indique la résistance à la transmission du son de cet objet par une valeur de référence (au lieu de fournir les valeurs totales d'absorption du son)."@fr-FR , "このオブジェクトの遮音等級。各国の建築基準に従って決められる。このオブジェクトの音響透過を指数であらわす。（実際の吸音値を示すかわりに）"@ja-JP ;
        rdfs:label             "Isolation acoustique"@fr-FR , "IsolationAcoustique"@fr-FR , "隔音等级"@zh-CN , "遮音等級"@ja-JP , "acousticRating"@en , "Schallschutzklasse"@de-DE ;
        rdfs:range             xsd:string ;
        schema:domainIncludes  <https://w3id.org/product/Roof> , <https://w3id.org/product/Covering> , <https://w3id.org/product/Plate> , <https://w3id.org/product/Wall> , <https://w3id.org/product/Window> , <https://w3id.org/product/CurtainWall> , <https://w3id.org/product/Door> , <https://w3id.org/product/Slab> .

props:warpingConstant
        a                      owl:DatatypeProperty ;
        rdfs:comment           "Warping constant of the profile for torsional action. For example measured in mm6."@en ;
        rdfs:label             "warpingConstant"@en ;
        rdfs:range             <https://w3id.org/product/WarpingConstantMeasure> ;
        schema:domainIncludes  <https://w3id.org/product/ProfileDef> .

props:pressureRange  a         owl:DatatypeProperty ;
        rdfs:comment           "許容最大・最小動作圧力（周辺圧力との相対値）"@ja-JP , "許容最大/最小管内圧力(周囲圧力に比較して)"@ja-JP , "許容できる最大/最小管内圧力(周囲圧力に比較して)"@ja-JP , "Allowable maximum and minimum working pressure (relative to ambient pressure)."@en ;
        rdfs:label             "圧力範囲"@ja-JP , "pressureRange"@en ;
        schema:domainIncludes  <https://w3id.org/product/PipeFitting> , <https://w3id.org/product/PipeSegment> , <https://w3id.org/product/DuctSegment> , <https://w3id.org/product/DuctFitting> .

props:hasCaps  a               owl:DatatypeProperty ;
        rdfs:comment           "Does the inlet connection have protective caps."@en , "入口接続が保護キャップを持っているか。"@ja-JP ;
        rdfs:label             "hasCaps"@en , "保護キャップ"@ja-JP ;
        rdfs:range             xsd:boolean ;
        schema:domainIncludes  <https://w3id.org/product/FireSuppressionTerminal%2FBREECHINGINLET> .

props:isUsed  a                owl:DatatypeProperty ;
        rdfs:comment           "Indicates whether the element is being used in a workstation (= TRUE) or not.(= FALSE)."@en ;
        rdfs:label             "isUsed"@en ;
        rdfs:range             xsd:boolean ;
        schema:domainIncludes  <https://w3id.org/product/SystemFurnitureElement> .

props:numberOfStoreys
        a                      owl:DatatypeProperty ;
        rdfs:comment           "The number of storeys within a building.\nCaptured for those cases where the IfcBuildingStorey entity is not used. Note that if IfcBuilingStorey is asserted and the number of storeys in a building can be determined from it, then this approach should be used in preference to setting a property for the number of storeys."@en , "Le nombre de niveaux dans un bâtiment, à indiquer lorsque la classe IfcBuildingStorey n'est pas  utilisée. Il est préférable de créer des instances d'IfcBuildingStorey et d'en déduire le nombre de niveaux plutôt que de saisir cette propriété."@fr-FR , "Anzahl der Vollgeschosse des Gebäudes. \n\nDieses Attribute soll nur dann eingefügt werden, wenn keine Geschosse als Objekte, IfcBuildingStorey, beinhaltet sind. Bei Unstimmigkeiten hat die Anzahl der IfcBuildingStorey Objekte Priorität."@de-DE , "건물 층 수. IfcBuildingStorey 수와 관계없이 취급한다."@ko-KR , "建物階の数。IfcBuildingStoreyの数とは関係なく扱う。"@ja-JP ;
        rdfs:label             "Geschossanzahl"@de-DE , "階数"@ja-JP , "NombreNiveaux"@fr-FR , "층 수"@ko-KR , "numberOfStoreys"@en ;
        rdfs:range             xsd:int ;
        schema:domainIncludes  <https://w3id.org/product/Building> .

props:treadLengthAtOffset
        a                      owl:DatatypeProperty ;
        rdfs:comment           "在指定偏移量处踏板的长度。\n走线位置由“走线偏移”指定。该属性一般应与踏板长度一致，但如果根据建筑规范计算得到的走线偏移量和设计中使用的走线偏移量不同时，应使用该属性。"@zh-CN , "German-description-8"@de-DE , "Longueur du giron le long de la ligne de foulée. La valeur relativement à cette position doit normalement être identique à la propriété \"Longueur du giron\" ; elle peut être indiquée si la valeur de la propriété \"Décalage de la ligne de foulée\" donnée par une règle de calcul est différente de celle utilisée en conception."@fr-FR , "Length of treads at a given offset.\nWalking line position is given by the 'WalkingLineOffset'. The resulting value should normally be identical with TreadLength, it may be given in addition, if the walking line offset for building code calculations is different from that used in design."@en ;
        rdfs:label             "偏移踏板长度"@zh-CN , "LongueurGironSurLigneFoulee"@fr-FR , "treadLengthAtOffset"@en , "Auftritt an der Lauflinie"@de-DE ;
        rdfs:range             <https://w3id.org/product/PositiveLengthMeasure> ;
        schema:domainIncludes  <https://w3id.org/product/Stair> , <https://w3id.org/product/StairFlight> .

props:windSensorType  a        owl:DatatypeProperty ;
        rdfs:comment           "Enumeration that Identifies the types of wind sensors that can be specified."@en , "明示された風センサーのタイプを識別する一覧。"@ja-JP , "명시된 바람 센서 유형을 식별하는 목록."@ko-KR ;
        rdfs:label             "windSensorType"@en , "風センサータイプ"@ja-JP , "바람 센서 타입"@ko-KR ;
        schema:domainIncludes  <https://w3id.org/product/Sensor%2FWINDSENSOR> .

props:panVertical  a           owl:DatatypeProperty ;
        rdfs:comment           "Indicates vertical range for panning."@en , "垂直方向の可動範囲を示す。"@ja-JP ;
        rdfs:label             "panVertical"@en , "パン垂直方向可動範囲"@ja-JP ;
        schema:domainIncludes  <https://w3id.org/product/AudioVisualAppliance%2FCAMERA> .

props:mediaExtendedArea
        a                      owl:DatatypeProperty ;
        rdfs:comment           "Total extended media area."@en ;
        rdfs:label             "mediaExtendedArea"@en ;
        rdfs:range             <https://w3id.org/product/AreaMeasure> ;
        schema:domainIncludes  <https://w3id.org/product/Filter%2FAIRPARTICLEFILTER> .

props:fuseDisconnectorType
        a                      owl:DatatypeProperty ;
        rdfs:comment           "A list of the available types of fuse disconnector from which that required may be selected where:\n\nEngineProtectionDevice: A fuse whose characteristic is specifically designed for the protection of a motor or generator.\nFuseSwitchDisconnector: A switch disconnector in which a fuse link or a fuse carrier with fuse link forms the moving contact,\nHRC: A standard fuse (High Rupturing Capacity)\nOverloadProtectionDevice: A device that disconnects the supply when the operating conditions in an electrically undamaged circuit causes an overcurrent,\nSemiconductorFuse: A fuse whose characteristic is specifically designed for the protection of sem-conductor devices.\nSwitchDisconnectorFuse: A switch disconnector in which one or more poles have a fuse in series in a composite unit."@en , "自家用発電連携側：モータや発電機の保護のために設計されているヒューズ。\n 地絡保護装置：これでヒューズリンクまたはヒューズリンクヒューズキャリアは、可動接点を形成するスイッチ断路器、\n HRC：標準ヒューズ（高連動破壊容量）\n 漏電保護装置：電気的に破損して回路の動作条件は、過電流が発生する電源を切断装置\n 欠相保護付：その特性を具体的にsemが芯デバイスの保護のために設計されているヒューズ。\n 複合ヒューズ保護装置：その内の1つまたは複数の極は、複合ユニットに直列にヒューズを持っているスイッチ断路器。"@ja-JP , "자가용 발전 연계 측면 : 모터 및 발전기 보호를 위해 디자인되는 퓨즈.  지락 보호 장치 : 이제 퓨즈 링크 또는 퓨즈 링크 퓨즈 캐리어는 가동 접점을 형성하는 스위치 단로기,  HRC : 표준 퓨즈 (높이 연동 파괴 용량)  누전 보호 장치 : 전기 손상 회로의 동작 조건은 과전류가 발생하는 전원을 차단 장치  결상 보호 부착 : 그 특성을 구체적으로 sem이 심 장치 보호를 위해 디자인되는 퓨즈.  복합 퓨즈 보호 장치 : 어떤 한 개 이상의 전극은 복합 유닛에 직렬로 퓨즈를 가지고있는 스위치 단로기."@ko-KR ;
        rdfs:label             "fuseDisconnectorType"@en , "ヒューズ遮断機のタイプ"@ja-JP , "퓨즈차단기 유형"@ko-KR ;
        schema:domainIncludes  <https://w3id.org/product/ProtectiveDevice%2FFUSEDISCONNECTOR> .

props:nominalWaterFlowHeating
        a                      owl:DatatypeProperty ;
        rdfs:comment           "Nominal water flow (refers to nominal heating capacity)."@en ;
        rdfs:label             "nominalWaterFlowHeating"@en ;
        rdfs:range             <https://w3id.org/product/VolumetricFlowRateMeasure> ;
        schema:domainIncludes  <https://w3id.org/product/CooledBeam> .

props:realImpedanceRatio
        a                      owl:DatatypeProperty ;
        rdfs:comment           "The ratio between the real part of the zero sequence impedance and the real part of the positive impedance (i.e. real part of the short-circuit voltage) of the transformer.\nUsed for three-phase transformer which includes a N-conductor."@en , "零相インピーダンスと正相インピーダンス（例．短絡電圧の実部）の間の比率。N-コンダクターを含む三相トランスのために使用。"@ja-JP , "영 상 임피던스와 양의 상 임피던스 (예 : 단락 전압의 실제 부분) 사이의 비율. N-지휘자를 포함 삼상 변압기에 사용됩니다."@ko-KR ;
        rdfs:label             "realImpedanceRatio"@en , "インピーダンス実部比率"@ja-JP , "임피던스 실수 부 비율"@ko-KR ;
        rdfs:range             <https://w3id.org/product/RatioMeasure> ;
        schema:domainIncludes  <https://w3id.org/product/Transformer> .

props:system  a                owl:DatatypeProperty ;
        rdfs:comment           "Angabe zu welcher Anlage (oder Anlagen) der Durchbruch benötigt wird."@de-DE , "Le système qui requiert la réservation (exemples : \"Conditionnement d'air\", \"Plomberie\", \"Electricité\")"@fr-FR , "需要空构件的建筑服务系统，例如，“空调”、“给排水”、“电气”等。"@zh-CN , "he building service system that requires the provision for voids, e.g. 'Air Conditioning', 'Plumbing', 'Electro', etc."@en , "空間に提示される建物サービスシステムです。例えば「空調」「配管」「電気」です。"@ja-JP ;
        rdfs:label             "Système"@fr-FR , "Anlage"@de-DE , "系统"@zh-CN , "システム"@ja-JP , "system"@en ;
        rdfs:range             xsd:string ;
        schema:domainIncludes  <https://w3id.org/product/BuildingElementProxy%2FPROVISIONFORVOID> .

props:heatTransferDimension
        a                      owl:DatatypeProperty ;
        rdfs:comment           "Indicates how heat is transmitted according to the shape of the space heater."@en , "室内暖房機の形に従って熱がどう伝えられるかを示します。"@ja-JP ;
        rdfs:label             "heatTransferDimension"@en , "熱伝達値"@ja-JP ;
        schema:domainIncludes  <https://w3id.org/product/SpaceHeater> .

props:overallDiameter
        a                      owl:DatatypeProperty ;
        rdfs:comment           "The overall diameter of a Cable/Bus."@en , "케이블과 모선의 외형 치수 (직경)를 나타낸다."@ko-KR , "전체 직경 (최대 공간)."@ko-KR , "全体の直径（最大スペース）。"@ja-JP , "The overall diameter of a core (maximun space used)."@en , "ケーブルや母線の外形寸法（直径）を示す。"@ja-JP ;
        rdfs:label             "overallDiameter"@en , "全径"@ja-JP , "直径"@ja-JP , "전체 직경"@ko-KR , "직경"@ko-KR ;
        rdfs:range             <https://w3id.org/product/PositiveLengthMeasure> ;
        schema:domainIncludes  <https://w3id.org/product/CableSegment%2FCABLESEGMENT> , <https://w3id.org/product/CableSegment%2FCORESEGMENT> .

props:effectiveness  a         owl:DatatypeProperty ;
        rdfs:comment           "Ratio of the real heat transfer rate to the maximum possible heat transfer rate."@en , "最大可能熱移動量に対する実熱移動量の割合"@ja-JP , "Ratio of the change in dry bulb temperature of the (primary) air stream to the difference between the entering dry bulb temperature of the (primary) air and the wet-bulb temperature of the (secondary) air."@en , "（一次）空気の入力乾球温度と（二次）空気の湿球温度の差に対する（一次）空気の流れの乾球温度の変化の割合。"@ja-JP ;
        rdfs:label             "effectiveness"@en , "効率"@ja-JP ;
        schema:domainIncludes  <https://w3id.org/product/SpaceHeater> , <https://w3id.org/product/EvaporativeCooler> .

props:bladeThickness  a        owl:DatatypeProperty ;
        rdfs:comment           "The thickness of the damper blade."@en ;
        rdfs:label             "bladeThickness"@en ;
        rdfs:range             <https://w3id.org/product/PositiveLengthMeasure> ;
        schema:domainIncludes  <https://w3id.org/product/Damper> .

props:currentTolerance2
        a                      owl:DatatypeProperty ;
        rdfs:comment           "The tolerance for the current of time/current-curve in [%] valid for times above CurrentTolereanceLimit1."@en , "[％]で指定された時間/特性曲線の許容範囲は、上記の許容電流限界1の時間で有効です。"@ja-JP , "[%]로 지정된 시간 / 특성 곡선의 허용 범위는 상기의 허용 전류 한계 1 시간에 유효합니다."@ko-KR ;
        rdfs:label             "currentTolerance2"@en , "許容電流2"@ja-JP , "허용전류 2"@ko-KR ;
        rdfs:range             <https://w3id.org/product/PositiveRatioMeasure> ;
        schema:domainIncludes  <https://w3id.org/product/ProtectiveDeviceTrippingUnit> .

props:lowerCurrent2  a         owl:DatatypeProperty ;
        rdfs:comment           "The current in [x In], indicating the upper current limit of the lower time/current curve of the I2t part of the L-function."@en , "[x In]の電流,電流をトリップするL関数のI2t部分は、特性曲線よりも小さい電流を示す。"@ja-JP , "x In] 전류 전류를 여행하는 L 함수 I2t 부분은 곡선보다 작은 전류를 보여준다."@ko-KR ;
        rdfs:label             "lowerCurrent2"@en , "下電流2"@ja-JP , "하전류 2"@ko-KR ;
        rdfs:range             <https://w3id.org/product/ElectricCurrentMeasure> ;
        schema:domainIncludes  <https://w3id.org/product/ProtectiveDeviceTrippingUnit> .

props:supplyAirTemperatureHeating
        a                      owl:DatatypeProperty ;
        rdfs:comment           "Supply air temperature in heating mode."@en , "暖房時の給気温度"@ja-JP , "Température de l'air soufflé en mode chauffage"@fr-FR ;
        rdfs:label             "supplyAirTemperatureHeating"@en , "暖房給気温度"@ja-JP , "Température de l'air soufflé en chauffage"@fr-FR ;
        schema:domainIncludes  <https://w3id.org/product/AirTerminal> .

props:thermalEfficiency
        a                      owl:DatatypeProperty ;
        rdfs:comment           "Overall Thermal Efficiency is defined as gross energy output of the heat transfer device divided by the energy input."@en , "熱効率：熱伝導装置の総エネルギー出力/エネルギー入力として総合的な熱効率は定義される。"@ja-JP ;
        rdfs:label             "thermalEfficiency"@en , "熱効率"@ja-JP ;
        rdfs:range             <https://w3id.org/product/NormalisedRatioMeasure> ;
        schema:domainIncludes  <https://w3id.org/product/SpaceHeater> .

props:exponent  a              owl:DatatypeProperty ;
        rdfs:comment           "Characteristic exponent, slope of log(heat output) vs log (surface temperature minus environmental temperature)."@en , "特徴的な指数、log(熱出力)log（表面温度マイナス周囲温度）の勾配"@ja-JP ;
        rdfs:label             "exponent"@en , "指数"@ja-JP ;
        schema:domainIncludes  <https://w3id.org/product/SpaceHeater> .

props:numberOfHoseConnections
        a                      owl:DatatypeProperty ;
        rdfs:comment           "The number of hose connections on the hydrant (excluding the pumper connection)."@en , "（ポンプ接続を除く）消火栓のホース接続の数。"@ja-JP ;
        rdfs:label             "numberOfHoseConnections"@en , "ホースの接続の数"@ja-JP ;
        rdfs:range             xsd:int ;
        schema:domainIncludes  <https://w3id.org/product/FireSuppressionTerminal%2FFIREHYDRANT> .

props:nominalHeight  a         owl:DatatypeProperty ;
        rdfs:comment           "ダクト直管の高さ"@ja-JP , "The nominal height of the segment."@en , "呼び高寸法。"@ja-JP , "The nominal height of the duct connection."@en , "The nominal height of the system furniture elements of this type. The size information is provided in addition to the shape representation and the geometric parameters used within. In cases of inconsistency between the geometric parameters and the size properties, provided in the attached property set, the geometric parameters take precedence."@en , "고 치수"@ko-KR , "The nominal height of the furniture of this type. The size information is provided in addition to the shape representation and the geometric parameters used within. In cases of inconsistency between the geometric parameters and the size properties, provided in the attached property set, the geometric parameters take precedence."@en , "고치수"@ko-KR , "The nominal height of the duct segment."@en ;
        rdfs:label             "공칭높이"@ko-KR , "공칭 높이"@ko-KR , "公称高"@ja-JP , "nominalHeight"@en , "呼び高さ"@ja-JP ;
        rdfs:range             <https://w3id.org/product/PositiveLengthMeasure> ;
        schema:domainIncludes  <https://w3id.org/product/CableCarrierSegment%2FCONDUITSEGMENT> , <https://w3id.org/product/CableCarrierSegment%2FCABLELADDERSEGMENT> , <https://w3id.org/product/DuctSegment> , <https://w3id.org/product/Furniture> , <https://w3id.org/product/CableCarrierSegment%2FCABLETRUNKINGSEGMENT> , <https://w3id.org/product/CableCarrierSegment%2FCABLETRAYSEGMENT> , <https://w3id.org/product/SystemFurnitureElement> , <https://w3id.org/product/DistributionPort%2FAIRCONDITIONING> .

props:batterAtStart  a         owl:DatatypeProperty ;
        rdfs:comment           "The angle, in radians, by which the formwork at the starting face of a piece is to be rotated from the vertical in order to compensate for the rotation of the face that will occur once the piece is stripped from its form, inducing camber due to eccentric prestressing."@en ;
        rdfs:label             "batterAtStart"@en ;
        rdfs:range             <https://w3id.org/product/PlaneAngleMeasure> ;
        schema:domainIncludes  <https://w3id.org/product/BuildingElement> .

props:setPointTemperature
        a                      owl:DatatypeProperty ;
        rdfs:comment           "The temperature value to be sensed. Use IfcPropertyBoundedValue.SetPointValue to set the set point value."@en , "感知される温度。\nセットポイント値を置くために、IfcPropertyBoundedValue.SetPointValueを使用する。"@ja-JP , "감지되는 온도. 세트 포인트 값을 넣으려면, IfcPropertyBoundedValue.SetPointValue를 사용하십시오."@ko-KR ;
        rdfs:label             "温度設定値"@ja-JP , "온도 설정"@ko-KR , "setPointTemperature"@en , "온도 성정"@ko-KR ;
        schema:domainIncludes  <https://w3id.org/product/Sensor%2FHEATSENSOR> , <https://w3id.org/product/Sensor%2FTEMPERATURESENSOR> .

props:shearAreaZ  a            owl:DatatypeProperty ;
        rdfs:comment           "Area of the profile for calculating the shear stress due to shear force parallel to the section analysis axis zs. For example measured in mm². If given, the shear area zs shall be non-negative."@en ;
        rdfs:label             "shearAreaZ"@en ;
        rdfs:range             <https://w3id.org/product/AreaMeasure> ;
        schema:domainIncludes  <https://w3id.org/product/ProfileDef> .

props:multipleTarriff
        a                      owl:DatatypeProperty ;
        rdfs:comment           "Indicates whether meter has built-in support for multiple tarriffs (variable energy cost rates)."@en ;
        rdfs:label             "multipleTarriff"@en ;
        rdfs:range             xsd:boolean ;
        schema:domainIncludes  <https://w3id.org/product/FlowMeter%2FENERGYMETER> .

props:selfExtinguishing60332_1
        a                      owl:DatatypeProperty ;
        rdfs:comment           "IEC 60332.1.に規定されている自己消火ケーブル。"@ja-JP , "自動消火ケーブル/コアはIEC 60332.1に準じる。"@ja-JP , "Self Extinguishing cable/core according to IEC 60332.1."@en , "IEC 60332.1.에 규정되어있는 자기 소화 케이블"@ko-KR , "자동 소화 케이블 / 코어는 IEC 60332.1에 준한다"@ko-KR ;
        rdfs:label             "자동 소화 60332_1"@ko-KR , "自己消火ケーブル"@ja-JP , "selfExtinguishing60332_1"@en , "自動消火60332_1"@ja-JP , "자기 소화 케이블"@ko-KR ;
        rdfs:range             xsd:boolean ;
        schema:domainIncludes  <https://w3id.org/product/CableSegment%2FCABLESEGMENT> , <https://w3id.org/product/CableSegment%2FCORESEGMENT> .

props:reinforcementBarType
        a                      owl:DatatypeProperty ;
        rdfs:comment           "Defines the type of the reinforcement bar."@en , "補強筋タイプの定義。"@ja-JP ;
        rdfs:label             "reinforcementBarType"@en , "補強筋タイプ"@ja-JP ;
        schema:domainIncludes  <https://w3id.org/product/Column> .

props:poissonRatio  a          owl:DatatypeProperty ;
        rdfs:comment           "A measure of the lateral deformations in the elastic range."@en ;
        rdfs:label             "poissonRatio"@en ;
        rdfs:range             <https://w3id.org/product/PositiveRatioMeasure> ;
        schema:domainIncludes  <https://w3id.org/product/Material> .

props:xDirectionLowerBarCount
        a                      owl:DatatypeProperty ;
        rdfs:comment           "The number of bars with X direction lower bar."@en , "X方向の下端筋本数。"@ja-JP ;
        rdfs:label             "xDirectionLowerBarCount"@en , "X方向下端筋本数"@ja-JP ;
        rdfs:range             xsd:int ;
        schema:domainIncludes  <https://w3id.org/product/Footing> .

props:deliveryType  a          owl:DatatypeProperty ;
        rdfs:comment           "Determines how the accessory will be delivered to the site."@en ;
        rdfs:label             "deliveryType"@en ;
        schema:domainIncludes  <https://w3id.org/product/ElementComponent> .

props:toiletType  a            owl:DatatypeProperty ;
        rdfs:comment           "Enumeration that defines the types of toilet (water closet) arrangements that may be specified where:-\n\nBedPanWasher: Enclosed soil appliance in which bedpans and urinal bottles are emptied and cleansed.\nChemical: Portable receptacle or soil appliance that receives and retains excrement in either an integral or a separate container, in which it is chemically treated and from which it has to be emptied periodically.\nCloseCoupled: \tToilet suite in which a flushing cistern is connected directly to the water closet pan.\nLooseCoupled: \tToilet arrangement in which a flushing cistern is connected to the water closet pan through a flushing pipe.\nSlopHopper: \tHopper shaped soil appliance with a flushing rim and outlet similar to those of a toilet pan, into which human excrement is emptied for disposal."@en , "トイレ配置は下記に列挙された仕様となります。\n\n便器洗浄機：便器と小便器が空にされ洗浄される周囲が囲まれた電気機器。\nケミカル：別々の容器で排泄物を受けて、保持し、化学的に扱われる、定期的に空にされる携帯用の容器または土機器。\nｼｽﾀｰﾝ直結型：ｼｽﾀｰﾝがが便器に直接密着して設置されたタイプ\nｼｽﾀｰﾝ分離型：ｼｽﾀｰﾝがﾊﾟｲﾌﾟを介して便器につながっているタイプ\n汚物流し：ホッパーは土壌器具にデザイされており、汚物が流され空になります。"@ja-JP ;
        rdfs:label             "toiletType"@en , "トイレ種類"@ja-JP ;
        schema:domainIncludes  <https://w3id.org/product/SanitaryTerminal%2FTOILETPAN> .

props:totalWattage  a          owl:DatatypeProperty ;
        rdfs:comment           "Wattage on whole lightfitting device with all sources intact."@en , "全ての照明器具のワット数。"@ja-JP , "모든 조명기구 와트."@ko-KR ;
        rdfs:label             "totalWattage"@en , "総ワット数"@ja-JP , "총 와트"@ko-KR ;
        rdfs:range             <https://w3id.org/product/PowerMeasure> ;
        schema:domainIncludes  <https://w3id.org/product/LightFixture> .

props:hardeningModule
        a                      owl:DatatypeProperty ;
        rdfs:comment           "A measure of the hardening module of the material (slope of stress versus strain curve after yield range)."@en ;
        rdfs:label             "hardeningModule"@en ;
        rdfs:range             <https://w3id.org/product/ModulusOfElasticityMeasure> ;
        schema:domainIncludes  <https://w3id.org/product/Material%2FSteel> .

props:soundPressure  a         owl:DatatypeProperty ;
        rdfs:comment           "A time series of sound pressure values measured in decibels at a reference pressure of 20 microPascals for the referenced octave band frequency.  Each value in IfcTimeSeries.ListValues is correlated to the sound frequency at the same position within SoundFrequencies."@en , "時系列の音圧、単位はデシベル。オクターブバンドの音の強さ20mPaを基準する。IfcTimeSeriesにリストされた各値は同じ場所で、同じ周波数バントでの温の周波数と関連する。"@ja-JP , "시계열의 음압 단위는 dB. 옥타브 밴드 소리의 강도 20mPa을 기준한다. IfcTimeSeries에 나열된 각 값은 같은 장소에서 같은 주파수 번트에서 온도의 주파수와 관련."@ko-KR ;
        rdfs:label             "soundPressure"@en , "音圧"@ja-JP , "음압"@ko-KR ;
        schema:domainIncludes  <https://w3id.org/product/Annotation%2FSOUND> .

props:thermalIrEmissivityFront
        a                      owl:DatatypeProperty ;
        rdfs:comment           "Thermal IR emissivity: front side. Defines the fraction of thermal energy emitted per unit area to \"blackbody\" at the same temperature, through the \"front\" side of the material."@en ;
        rdfs:label             "thermalIrEmissivityFront"@en ;
        rdfs:range             <https://w3id.org/product/PositiveRatioMeasure> ;
        schema:domainIncludes  <https://w3id.org/product/Material> .

props:tiltAngle  a             owl:DatatypeProperty ;
        rdfs:comment           "The angle of tilt defined in the plane perpendicular to the extrusion axis (X-Axis of the local placement). The angle shall be measured from the orientation of the Z-Axis in the local placement."@en ;
        rdfs:label             "tiltAngle"@en ;
        schema:domainIncludes  <https://w3id.org/product/ShadingDevice> .

props:setPointSpeed  a         owl:DatatypeProperty ;
        rdfs:comment           "The wind speed value to be sensed. Use IfcPropertyBoundedValue.SetPointValue to set the set point value."@en , "感知される風速。\nセットポイント値を置くために、IfcPropertyBoundedValue.SetPointValueを使用する。"@ja-JP , "감지되는 바람. 세트 포인트 값을 넣으려면, IfcPropertyBoundedValue.SetPointValue를 사용하십시오."@ko-KR ;
        rdfs:label             "setPointSpeed"@en , "風速設定値"@ja-JP , "풍속 설정"@ko-KR ;
        rdfs:range             <https://w3id.org/product/LinearVelocityMeasure> ;
        schema:domainIncludes  <https://w3id.org/product/Sensor%2FWINDSENSOR> .

props:vacancyRateInCategoryNow
        a                      owl:DatatypeProperty ;
        rdfs:comment           "Percentage of vacancy found in the particular category currently."@en , "Taux actuel de vacance pour la catégorie."@fr-FR ;
        rdfs:label             "vacancyRateInCategoryNow"@en , "TauxVacanceActuelParCategorie"@fr-FR ;
        rdfs:range             <https://w3id.org/product/PositiveRatioMeasure> ;
        schema:domainIncludes  <https://w3id.org/product/Building> .

props:exhaustAirFlowRate
        a                      owl:DatatypeProperty ;
        rdfs:comment           "Exhaust air flow rate in the space."@en , "室内の排気流量"@ja-JP ;
        rdfs:label             "exhaustAirFlowRate"@en , "排気空気流量"@ja-JP ;
        schema:domainIncludes  <https://w3id.org/product/Space> .

props:firmwareVersion
        a                      owl:DatatypeProperty ;
        rdfs:comment           "Indicates version of device firmware according to device manufacturer."@en , "컨트롤러 펌웨어 버전"@ko-KR ;
        rdfs:label             "firmwareVersion"@en , "펌웨어 버전"@ko-KR ;
        rdfs:range             xsd:string ;
        schema:domainIncludes  <https://w3id.org/product/Controller%2FPROGRAMMABLE> .

props:containerMaterial
        a             owl:DatatypeProperty ;
        rdfs:comment  "Special requirements for material used to contain an artefact."@en , "品物の収容するのに使用される材料に関する特記事項。"@ja-JP ;
        rdfs:label    "containerMaterial"@en , "コンテナー材料"@ja-JP .

props:ductSizingMethod
        a                      owl:DatatypeProperty ;
        rdfs:comment           "Enumeration that identifies the methodology to be used to size system components."@en , "ダクト寸法を決める計算方法。"@ja-JP , "덕트 치수를 결정하는 계산 방법."@ko-KR ;
        rdfs:label             "ductSizingMethod"@en , "ダクト寸法の決め方"@ja-JP , "덕트 치수 결정 방법"@ko-KR ;
        schema:domainIncludes  <https://w3id.org/product/DistributionSystem%2FVENTILATION> .

props:location2Global
        a                      owl:DatatypeProperty ;
        rdfs:comment           "Global X,Y,Z coordinates of the point in which Thickness2 is given"@en ;
        rdfs:label             "location2Global"@en ;
        schema:domainIncludes  <https://w3id.org/product/StructuralSurfaceMemberVarying> .

props:nominalBodyWidth
        a                      owl:DatatypeProperty ;
        rdfs:comment           "Nominal or quoted length measured along the y-axis in the local coordinate system of the chamber of the gully trap."@en , "溝防臭弁の半径か局所座標系のＹ軸に沿って測定された呼称もしくは積算された長さ。"@ja-JP , "Nominal or quoted length measured along the y-axis in the local coordinate system of the drain."@en , "半径か局所座標系のＹ軸に沿って測定された呼称もしくは積算された配管の長さ。"@ja-JP , "Nominal or quoted length measured along the y-axis in the local coordinate system of the waste."@en , "Nominal or quoted length, measured along the y-axis of the local coordinate system of the object, of the body of the object."@en , "Nominal or quoted length measured along the y-axis in the local coordinate system of the chamber of the trap."@en , "廃棄物の半径か局所座標系のＹ軸に沿って測定された呼称もしくは積算された長さ。"@ja-JP , "防臭弁の区画の半径か局所座標系のＹ軸に沿って測定された呼称もしくは積算された長さ。"@ja-JP ;
        rdfs:label             "nominalBodyWidth"@en , "呼称躯体幅"@ja-JP ;
        rdfs:range             <https://w3id.org/product/PositiveLengthMeasure> ;
        schema:domainIncludes  <https://w3id.org/product/WasteTerminal%2FROOFDRAIN> , <https://w3id.org/product/WasteTerminal%2FGULLYTRAP> , <https://w3id.org/product/Interceptor> , <https://w3id.org/product/WasteTerminal%2FFLOORWASTE> , <https://w3id.org/product/WasteTerminal%2FFLOORTRAP> .

props:heat  a                  owl:DatatypeProperty ;
        rdfs:comment           "The amount of heat energy consumed during the period specified in the time series."@en , "특정 기간 동안의 열 소비."@ko-KR ;
        rdfs:label             "heat"@en , "열 소비량"@ko-KR ;
        schema:domainIncludes  <https://w3id.org/product/Building> .

props:plasticShapeFactorY
        a                      owl:DatatypeProperty ;
        rdfs:comment           "Ratio of plastic versus elastic bending moment capacity about the section analysis axis ys. A dimensionless value."@en ;
        rdfs:label             "plasticShapeFactorY"@en ;
        rdfs:range             <https://w3id.org/product/PositiveRatioMeasure> ;
        schema:domainIncludes  <https://w3id.org/product/ProfileDef> .

props:people  a                owl:DatatypeProperty ;
        rdfs:comment           "Heat gains and losses from people."@en , "人員からの熱取得。"@ja-JP , "사람의 열"@ko-KR ;
        rdfs:label             "people"@en , "人員"@ja-JP , "인원"@ko-KR ;
        schema:domainIncludes  <https://w3id.org/product/Space> .

props:polarity  a              owl:DatatypeProperty ;
        rdfs:comment           "True indicates normal polarity; False indicates reverse polarity."@en ;
        rdfs:label             "polarity"@en ;
        rdfs:range             xsd:boolean ;
        schema:domainIncludes  <https://w3id.org/product/Controller%2FTWOPOSITION> .

props:rentalRatesInCategoryFuture
        a                      owl:DatatypeProperty ;
        rdfs:comment           "Range of the cost rates for property expected to be available in the future in the required category."@en , "Prix futur des loyers pour la catégorie considérée."@fr-FR ;
        rdfs:label             "rentalRatesInCategoryFuture"@en , "PrixFuturLoyerParCategorie"@fr-FR ;
        schema:domainIncludes  <https://w3id.org/product/Building> .

props:coilWidth  a             owl:DatatypeProperty ;
        rdfs:comment           "Width of coil."@en ;
        rdfs:label             "coilWidth"@en ;
        rdfs:range             <https://w3id.org/product/PositiveLengthMeasure> ;
        schema:domainIncludes  <https://w3id.org/product/CooledBeam> .

props:waterStorageCapacity
        a                      owl:DatatypeProperty ;
        rdfs:comment           "Water storage capacity."@en , "缶内水量"@ja-JP , "Capacité de réserve en eau"@fr-FR ;
        rdfs:label             "waterStorageCapacity"@en , "缶内水量"@ja-JP , "CapacitéRéservoirEau"@fr-FR ;
        rdfs:range             <https://w3id.org/product/VolumeMeasure> ;
        schema:domainIncludes  <https://w3id.org/product/Boiler> .

props:permeability  a          owl:DatatypeProperty ;
        rdfs:comment           "Ratio of the permeability of the ceiling.\nThe ration can be used to indicate an open ceiling (that enables identification of whether ceiling construction should be considered as impeding distribution of sprinkler water, light etc. from installations within the ceiling area)."@en , "Durchlässigkeit der Unterdecke als Faktor zwischen 0 Undurchlässig und 1 völlig durchlässig. Der Faktor kann zur Abschätzung genutzt werden, ob die Unterdecke zur Decke hin offen und durchlässig (für Licht, Wasser und Sicht) ist."@de-DE , "天花板的渗透比率。\n该比率可用以表示开敞式天花板（表示天花板能否阻隔其内侧的喷淋水、光线等的）。"@zh-CN , "Ratio de perméabilité du plafond. Ce ratio peut être utilisé pour désigner un plafond ouvert (cela permet de savoir si la pose du plafond empêche la distribution de fluides à partir d'installations situées dans le faux plafond)."@fr-FR ;
        rdfs:label             "Durchlässigkeit"@de-DE , "渗透率"@zh-CN , "permeability"@en , "Perméabilité"@fr-FR ;
        rdfs:range             <https://w3id.org/product/NormalisedRatioMeasure> ;
        schema:domainIncludes  <https://w3id.org/product/Covering%2FCEILING> .

props:hasReturnAir  a          owl:DatatypeProperty ;
        rdfs:comment           "Terminal box has return air mixed with supply air from duct work."@en , "ターミナルで還気を混合しているか否か（していればTRUE)"@ja-JP , "Le registre terminal a son air de reprise mélangé avec une amenée d'air issu du réseau de ventilation"@fr-FR ;
        rdfs:label             "hasReturnAir"@en , "還気有無"@ja-JP , "Possède air  repris"@fr-FR ;
        rdfs:range             xsd:boolean ;
        schema:domainIncludes  <https://w3id.org/product/AirTerminalBox> .

props:centerCoreMiddleHeight
        a                      owl:DatatypeProperty ;
        rdfs:comment           "Center core middle height of the profile."@en ;
        rdfs:label             "centerCoreMiddleHeight"@en ;
        rdfs:range             <https://w3id.org/product/PositiveLengthMeasure> ;
        schema:domainIncludes  <https://w3id.org/product/ArbitraryProfileDefWithVoids> .

props:cisternColor  a          owl:DatatypeProperty ;
        rdfs:comment           "Color of the object."@en , "本体色。"@ja-JP ;
        rdfs:label             "cisternColor"@en , "貯水タンクカラー"@ja-JP ;
        rdfs:range             xsd:string ;
        schema:domainIncludes  <https://w3id.org/product/SanitaryTerminal%2FCISTERN> .

props:longOutsideTopBarPitch
        a                      owl:DatatypeProperty ;
        rdfs:comment           "The pitch length of the long outside top bar."@en , "長辺方向・柱列帯・上端の鉄筋間隔。"@ja-JP ;
        rdfs:label             "longOutsideTopBarPitch"@en , "長辺・柱列帯・上端ピッチ"@ja-JP ;
        rdfs:range             <https://w3id.org/product/PositiveLengthMeasure> ;
        schema:domainIncludes  <https://w3id.org/product/Slab> .

props:plasticStrain  a         owl:DatatypeProperty ;
        rdfs:comment           "A measure of the permanent displacement, as in slip or twinning, which remains after the stress has been removed. Currently applied to a strain of 0.2% proportional stress of the material."@en ;
        rdfs:label             "plasticStrain"@en ;
        rdfs:range             <https://w3id.org/product/PositiveRatioMeasure> ;
        schema:domainIncludes  <https://w3id.org/product/Material%2FSteel> .

props:iCS60947  a              owl:DatatypeProperty ;
        rdfs:comment           "IECの60947シリーズに基づいてテスト配線用遮断機またはモータ保護装置のための遮断容量サービスを[A]で設定。"@ja-JP , "IEC의 60947 시리즈를 기반으로 테스트 배선용 차단기 또는 모터 보호 장치를위한 차단 용량 서비스를 [A]로 설정."@ko-KR , "The service breaking capacity in [A] for a circuit breaker or motor protection device tested in accordance with the IEC 60947 series."@en , "IEC60947 시리즈를 기반으로 테스트 배선 차단기 또는 모터 보호 장치를위한 전류 [A]에 견디는 온도  값은 1s 주어진다."@ko-KR , "The service breaking capacity in [A] for an MCB tested in accordance with the IEC 60947 series."@en , "IECの60947シリーズに基づいてテストされたMCBの定格使用短絡遮断容量を[A]で設定。"@ja-JP , "IECの60947シリーズに基づいてテストされた回路遮断機及びモータ保護装置の使用短絡遮断容量[A]。"@ja-JP , "IEC의 60947 시리즈를 기반으로 시험한 MCB의 정격 사용 단락 차단 용량 [A]로 설정."@ko-KR ;
        rdfs:label             "정격사용 단락 차단 용량"@ko-KR , "ICS60947"@ja-JP , "ICS60947"@ko-KR , "iCS60947"@en , "정격 사용 단락 차단 용량"@ko-KR , "定格使用短絡遮断容量"@ja-JP ;
        rdfs:range             <https://w3id.org/product/ElectricCurrentMeasure> ;
        schema:domainIncludes  <https://w3id.org/product/ProtectiveDevice%2FCIRCUITBREAKER> , <https://w3id.org/product/ProtectiveDevice> .

props:escortRequirement
        a                      owl:DatatypeProperty ;
        rdfs:comment           "Indicates whether or not an escort is required to accompany persons carrying out a work order at or to/from the place of work (= TRUE) or not (= FALSE).\n\nNOTE - There are many instances where escorting is required, particularly in a facility that has a high security rating. Escorting may require that persons are escorted to and from the place of work. Alternatively, it may involve the escort remaining at the place of work at all times."@en ;
        rdfs:label             "escortRequirement"@en ;
        rdfs:range             xsd:boolean ;
        schema:domainIncludes  <https://w3id.org/product/Permit> .

props:maximumApparentPower
        a                      owl:DatatypeProperty ;
        rdfs:comment           "Maximum apparent power/capacity in VA (volt ampere)."@en , "皮相電力/容量 の最大値　（VA:アンペア）。"@ja-JP , "피상 전력 / 용량 최대 (VA : 암페어)."@ko-KR ;
        rdfs:label             "maximumApparentPower"@en , "最大電力"@ja-JP , "최대 전력"@ko-KR ;
        rdfs:range             <https://w3id.org/product/PowerMeasure> ;
        schema:domainIncludes  <https://w3id.org/product/Transformer> .

props:hasProtectiveEarth
        a                      owl:DatatypeProperty ;
        rdfs:comment           "各ケーブルは黄色や緑で塗色された絶縁体をもっている。"@ja-JP , "Indicates whether the electrical device has a protective earth connection (=TRUE) or not (= FALSE)."@en , "One core has protective earth marked insulation, Yellow/Green."@en , "각 케이블은 노란색 또는 녹색으로 도색되었다 절연체를 가지고있다."@ko-KR ;
        rdfs:label             "hasProtectiveEarth"@en , "保護用接地の有無"@ja-JP , "보호 접지의 유무"@ko-KR ;
        rdfs:range             xsd:boolean ;
        schema:domainIncludes  <https://w3id.org/product/CableSegment%2FCABLESEGMENT> , <https://w3id.org/product/DistributionElement> .

props:brightness  a            owl:DatatypeProperty ;
        rdfs:comment           "Indicates the display brightness."@en , "明るさ示す。"@ja-JP , "밝기 보여준다"@ko-KR ;
        rdfs:label             "brightness"@en , "明るさ"@ja-JP , "밝기"@ko-KR ;
        rdfs:range             <https://w3id.org/product/IlluminanceMeasure> ;
        schema:domainIncludes  <https://w3id.org/product/AudioVisualAppliance%2FDISPLAY> .

props:t2  a                    owl:DatatypeProperty ;
        rdfs:comment           "열 동식 시험 시간 [s] 관련 시험 전류를 I1과 I2로한다."@ko-KR , "サーマルの試験時間を [s] , 関連する試験電流を I1 と I2　とする。"@ja-JP , "The (thermal) testing time in [s] associated with the testing currents I1 and I2."@en , "열 시험 시간 [s] 관련 시험 전류를 I1과 I2로한다."@ko-KR , "熱動式の試験時間を [s] , 関連する試験電流を I1 と I2　とする。"@ja-JP ;
        rdfs:label             "t2"@en , "T2"@ja-JP , "T2"@ko-KR ;
        rdfs:range             <https://w3id.org/product/TimeMeasure> ;
        schema:domainIncludes  <https://w3id.org/product/ProtectiveDeviceTrippingUnit%2FELECTROMAGNETIC> , <https://w3id.org/product/ProtectiveDeviceTrippingUnit%2FTHERMAL> .

props:numberOfSlots  a         owl:DatatypeProperty ;
        rdfs:comment           "Number of slots."@en , "スロット数"@ja-JP , "Nombre de fentes"@fr-FR ;
        rdfs:label             "numberOfSlots"@en , "スロット数"@ja-JP , "NombreDeFentes"@fr-FR ;
        rdfs:range             xsd:int ;
        schema:domainIncludes  <https://w3id.org/product/AirTerminal> .

props:occupancyType  a         owl:DatatypeProperty ;
        rdfs:comment           "Type d'occupation. Est défini selon le Code National en vigueur."@fr-FR , "このオブジェクトの用途。統括する国の建築法規により定義される。"@ja-JP , "점령 자의 유형. 건축 기준법을 준수합니다."@ko-KR , "Usage type de cet espace. Est défini selon le Code national en vigueur."@fr-FR , "Hauptnutzungsart des Gebäudes (Schulbau. Kaufhaus, etc.). Wird verwendet, wenn keine allgemein anerkanntes Klassifizierungssystem angewandt wird."@de-DE , "Nutzungsart des Raums gemäß der gültigen Raumnutzungstabelle des Raumprogramms."@de-DE , "Occupancy type for this object. It is defined according to the presiding national building code."@en , "Occupancy type for this object.\nIt is defined according to the presiding national building code."@en , "占有者のタイプ。建築基準法に準拠。"@ja-JP ;
        rdfs:label             "점유자 유형"@ko-KR , "占有者タイプ"@ja-JP , "用途"@ja-JP , "TypeOccupation"@fr-FR , "Nutzungsart"@de-DE , "occupancyType"@en ;
        rdfs:range             xsd:string ;
        schema:domainIncludes  <https://w3id.org/product/cSpatialZone> , <https://w3id.org/product/Building> , <https://w3id.org/product/cZone> , <https://w3id.org/product/Space> .

props:layers  a                owl:DatatypeProperty ;
        rdfs:comment           "Number of layers."@en ;
        rdfs:label             "layers"@en ;
        rdfs:range             xsd:int ;
        schema:domainIncludes  <https://w3id.org/product/Material%2FWood> .

props:colorTemperature
        a                      owl:DatatypeProperty ;
        rdfs:comment           "The color temperature of any source of radiation is defined as the temperature (in Kelvin) of a black-body or Planckian radiator whose radiation has the same chromaticity as the source of radiation. Often the values are only approximate color temperatures as the black-body radiator cannot emit radiation of every chromaticity value. The color temperatures of the commonest artificial light sources range from less than 3000K (warm white) to 4000K (intermediate) and over 5000K (daylight)."@en , "放射源の色温度は黒体、または完全放射体の色温度にて定義され、与えられた放射の色度と等しい黒体の温度のこと。与えられた放射の色度が黒体放射軌跡上にない場合に、相対分光分布を黒体放射に近似する。最も一般的な人工光源の色温度の範囲は、3000K以下（暖白）から4000K（中間）で、5000k以上は昼光。"@ja-JP , "방사 원의 색온도는 흑체 또는 흑체의 색온도에서 정의된 주어진 방사의 색도와 동일 흑체의 온도 것. 주어진 방사의 색도가 흑체 복사 궤적에없는 경우 상대 분광 분포를 흑체 복사에 근사한다. 가장 일반적인 인공 광원의 색온도 범위는 3000K 이하 (따뜻한 흰색)에서 4000K (중간)에서 5000k 이상은 일광."@ko-KR ;
        rdfs:label             "colorTemperature"@en , "色温度"@ja-JP , "색온도"@ko-KR ;
        rdfs:range             <https://w3id.org/product/ThermodynamicTemperatureMeasure> ;
        schema:domainIncludes  <https://w3id.org/product/Lamp> .

props:azimuth  a               owl:DatatypeProperty ;
        rdfs:comment           "The azimuth of the outward normal for the outward or upward facing surface."@en ;
        rdfs:label             "azimuth"@en ;
        schema:domainIncludes  <https://w3id.org/product/ShadingDevice> .

props:impellerDiameter
        a                      owl:DatatypeProperty ;
        rdfs:comment           "ファンホイールの直径　-　幾何学的に類似したファンの性能を基準化するために使用。"@ja-JP , "Diameter of fan wheel - used to scale performance of geometrically similar fans."@en , "Diameter of pump impeller - used to scale performance of geometrically similar pumps."@en , "Diameter of compressor impeller - used to scale performance of geometrically similar compressors."@en , "Diamètre du rotor du compresseur - utilisé pour dimensionner les performances des compresseurs géométriquement similaires."@fr-FR , "幾何学的に似たポンプの性能を予測するのに使われる。"@ja-JP ;
        rdfs:label             "羽根径"@ja-JP , "impellerDiameter"@en , "DiametreRotor"@fr-FR , "羽根直径"@ja-JP ;
        rdfs:range             <https://w3id.org/product/PositiveLengthMeasure> ;
        schema:domainIncludes  <https://w3id.org/product/Pump> , <https://w3id.org/product/Fan> , <https://w3id.org/product/Compressor> .

props:skillLevel  a            owl:DatatypeProperty ;
        rdfs:comment           "Skill level exhibited by the actor and which indicates an extent of their capability to perform actions on the artefacts upon which they can act."@en , "関与者が示すスキルレベル（技能・技量段階）、および実行されるアクションへの能力を示すもの。"@ja-JP , "参与者具备的技能的等级，即他们在专业领域内所能展示的能力。"@zh-CN ;
        rdfs:label             "skillLevel"@en , "技能段階"@ja-JP , "技能等级"@zh-CN ;
        rdfs:range             xsd:string ;
        schema:domainIncludes  <https://w3id.org/product/Actor> .

props:exclusions  a            owl:DatatypeProperty ;
        rdfs:comment           "Items, conditions or actions that may be excluded from the warranty or that may cause the warranty to become void."@en ;
        rdfs:label             "exclusions"@en ;
        rdfs:range             xsd:string ;
        schema:domainIncludes  <https://w3id.org/product/Element> .

props:ladderTrussCrossBarSpacing
        a                      owl:DatatypeProperty ;
        rdfs:comment           "The spacing between the straight cross-bars."@en , "まっすぐなのクロスバーの間隔。"@ja-JP , "똑바른 크로스바 간격"@ko-KR ;
        rdfs:label             "ladderTrussCrossBarSpacing"@en , "クロスバー間隔"@ja-JP , "크로스바 간격"@ko-KR ;
        rdfs:range             <https://w3id.org/product/PositiveLengthMeasure> ;
        schema:domainIncludes  <https://w3id.org/product/DiscreteAccessory%2FLadder%20truss%20connector> .

props:longInsideEndLowerBarPitch
        a                      owl:DatatypeProperty ;
        rdfs:comment           "The pitch length of the long inside end lower bar."@en , "長辺方向・柱間帯・下端端部の鉄筋間隔。"@ja-JP ;
        rdfs:label             "longInsideEndLowerBarPitch"@en , "長辺・柱列帯・下端端部ピッチ"@ja-JP ;
        rdfs:range             <https://w3id.org/product/PositiveLengthMeasure> ;
        schema:domainIncludes  <https://w3id.org/product/Slab> .

props:overallDepth  a          owl:DatatypeProperty ;
        rdfs:comment           "Overall depth of the profile."@en ;
        rdfs:label             "overallDepth"@en ;
        rdfs:range             <https://w3id.org/product/PositiveLengthMeasure> ;
        schema:domainIncludes  <https://w3id.org/product/ArbitraryProfileDefWithVoids> , <https://w3id.org/product/ArbitraryClosedProfileDef> .

props:isAutomatic  a           owl:DatatypeProperty ;
        rdfs:comment           "Indication of whether the valve is automatically operated (TRUE) or manually operated (FALSE)."@en , "弁が自動(TRUE)で操作されるか手動(FALSE)で操作されるかの表示"@ja-JP ;
        rdfs:label             "isAutomatic"@en , "自動"@ja-JP ;
        rdfs:range             xsd:boolean ;
        schema:domainIncludes  <https://w3id.org/product/Valve%2FAIRRELEASE> .

props:parkingUnits  a          owl:DatatypeProperty ;
        rdfs:comment           "Indicates the number of transporation units of the type specified by the property ParkingUse that may be accommodated within the space. Generally, this value should default to 1 unit. However, where the parking space is for motorcycles or bicycles, provision may be made for more than one unit in the space."@en , "Nombre d'unités du type de véhicule spécifié dans la propriété TypeVehicule que peut contenir l'espace alloué au parking. Généralement, la valeur par défaut est 1. Elle peut être supérieure pour les deux roues."@fr-FR , "車両種別ごとの駐車台数のユニットごとの指定台数。一般に、この値は1台/1ユニットになるべきです。しかしながら、オートバイまたは自転車向けである場合、数台/1ユニット以上なるかもしれません。"@ja-JP ;
        rdfs:label             "parkingUnits"@en , "TypeVehicule"@fr-FR , "一区画当たりの駐車台数"@ja-JP ;
        rdfs:range             <https://w3id.org/product/CountMeasure> ;
        schema:domainIncludes  <https://w3id.org/product/Space%2FPARKING> .

props:hazardousWastePerUnit
        a                      owl:DatatypeProperty ;
        rdfs:comment           "Quantity of hazardous waste generated"@en , "유해 폐기물의 발생량"@ko-KR , "生成された有害な廃棄量。"@ja-JP , "Quantité de déchets dangereux générés tels que définis dans la norme  ISO21930:2007 [NDT : et dans la norme NF P01-010]."@fr-FR ;
        rdfs:label             "hazardousWastePerUnit"@en , "단위당 유해 폐기물"@ko-KR , "DechetsDangereuxParUnite"@fr-FR , "単位あたり有害廃棄物"@ja-JP ;
        rdfs:range             <https://w3id.org/product/MassMeasure> ;
        schema:domainIncludes  <https://w3id.org/product/Element> .

props:colorCode  a             owl:DatatypeProperty ;
        rdfs:comment           "Name of a color for identifying the connector, if applicable."@en , "コネクタの色。"@ja-JP , "커넥터 고유 이름"@ko-KR ;
        rdfs:label             "colorCode"@en , "色番号"@ja-JP , "색상번호"@ko-KR ;
        rdfs:range             xsd:string ;
        schema:domainIncludes  <https://w3id.org/product/DistributionPort> .

props:releaseTime  a           owl:DatatypeProperty ;
        rdfs:comment           "관련 부분의 초기 여행을위한 [s]가 방출 시간.  이 트립 시간은 릴리스 전류보다 낮은 전류의 경우 지정된 동작 시간보다 길어집니다.  값을 평균으로 주어진다."@ko-KR , "The release time in [s] for the initial tripping of the relevant part. This time indicates that for current lower than the indicated release current, the tripping time will be longer than the indicated release time. The value is given as a mean value."@en , "관련 부분의 초기 여행을위한 [s]가 방출 시간.  이 트립 시간은 릴리스 전류보다 낮은 전류의 경우 지정된 동작 시간보다 길어집니다.  값을 평균으로 주어진다. \""@ko-KR , "関連する部分の初期トリップのための[s]が放出時間。\n このトリップ時間は、リリースの電流よりも低い電流の場合、指定された動作時間よりも長くなります。\n 値が平均値として与えられる。"@ja-JP ;
        rdfs:label             "放出時間"@ja-JP , "방출 시간"@ko-KR , "releaseTime"@en ;
        rdfs:range             <https://w3id.org/product/TimeMeasure> ;
        schema:domainIncludes  <https://w3id.org/product/ProtectiveDeviceTrippingUnit> .

props:thermalConductivity
        a                      owl:DatatypeProperty ;
        rdfs:comment           "The thermal conductivity of the tube."@en , "チューブの熱伝導率"@ja-JP , "フィンの熱伝導率"@ja-JP , "The rate at which thermal energy is transmitted through the material."@en , "The thermal conductivity of the fin."@en ;
        rdfs:label             "thermalConductivity"@en , "熱伝導率"@ja-JP ;
        rdfs:range             <https://w3id.org/product/ThermalConductivityMeasure> ;
        schema:domainIncludes  <https://w3id.org/product/TubeBundle> , <https://w3id.org/product/TubeBundle%2FFINNED> , <https://w3id.org/product/Material> .

props:visibleLightTransmittance
        a                      owl:DatatypeProperty ;
        rdfs:comment           "Fraction du rayonnement visible qui est transmise par la protection solaire sous incidence normale. Valeur sans unité."@fr-FR , "正射时穿透玻璃的可见光比例。无单位。"@zh-CN , "Fraction of the visible light that passes the glazing at normal incidence. It is a value without unit."@en , "German-description-11"@de-DE , "ガラスへ法線入射した可視光の透過率。単位の無い値。"@ja-JP , "Fraction du rayonnement visible qui est transmise par le vitrage sous incidence normale. Valeur sans unité."@fr-FR , "通常の入射における日除け装置を通過する可視光の比率。単位の無い数値。"@ja-JP , "Fraction of the visible light that passes the shading system  at normal incidence. It is a value without unit."@en ;
        rdfs:label             "Transmittance du rayonnement visible"@fr-FR , "Transmissionsgrad für sichtbares Licht"@de-DE , "可见光透射率"@zh-CN , "可視光透過率"@ja-JP , "TransmittanceVisible"@fr-FR , "visibleLightTransmittance"@en ;
        rdfs:range             <https://w3id.org/product/NormalisedRatioMeasure> , <https://w3id.org/product/PositiveRatioMeasure> ;
        schema:domainIncludes  <https://w3id.org/product/Door> , <https://w3id.org/product/cWindow> , <https://w3id.org/product/ShadingDevice> .

props:name  a                  owl:DatatypeProperty ;
        rdfs:comment           "공조 방식의 명칭"@ko-KR , "空調方式の名称。"@ja-JP , "The name of the air side system."@en ;
        rdfs:label             "name"@en , "名前"@ja-JP , "이름"@ko-KR ;
        rdfs:range             xsd:string ;
        schema:domainIncludes  <https://w3id.org/product/Zone> , <https://w3id.org/product/Space> , <https://w3id.org/product/SpatialZone> .

props:setPointMoisture
        a                      owl:DatatypeProperty ;
        rdfs:comment           "The moisture value to be sensed. Use IfcPropertyBoundedValue.SetPointValue to set the set point value."@en , "感知される水分。\nセットポイント値を置くために、IfcPropertyBoundedValue.SetPointValueを使用する。"@ja-JP , "감지되는 수분. 세트 포인트 값을 넣으려면, IfcPropertyBoundedValue.SetPointValue를 사용하십시오."@ko-KR ;
        rdfs:label             "setPointMoisture"@en , "水分設定値"@ja-JP , "수분 설정"@ko-KR ;
        schema:domainIncludes  <https://w3id.org/product/Sensor%2FMOISTURESENSOR> .

props:panHorizontal  a         owl:DatatypeProperty ;
        rdfs:comment           "Indicates horizontal range for panning."@en , "水平方向の可動範囲を示す。"@ja-JP ;
        rdfs:label             "panHorizontal"@en , "パン水平方向可動範囲"@ja-JP ;
        schema:domainIncludes  <https://w3id.org/product/AudioVisualAppliance%2FCAMERA> .

props:length  a                owl:DatatypeProperty ;
        rdfs:comment           "The finished length of the silencer."@en , "サイレンサの仕上げ長さ"@ja-JP , "배수 챔버의 길이"@ko-KR , "피트 길이"@ko-KR , "The length of the pit."@en , "チューブ束のチューブ長さ"@ja-JP , "排水チャンバーの長さ。"@ja-JP , "The length of the sump."@en , "Length of the fin as measured parallel to the direction of airflow."@en , "ピット長さ。"@ja-JP , "Length of the tubes in the tube bundle."@en , "気流方向に平行に計られたフィンの長さ"@ja-JP ;
        rdfs:label             "길이"@ko-KR , "length"@en , "長さ"@ja-JP ;
        rdfs:range             <https://w3id.org/product/LengthMeasure> , <https://w3id.org/product/PositiveLengthMeasure> ;
        schema:domainIncludes  <https://w3id.org/product/TubeBundle> , <https://w3id.org/product/TubeBundle%2FFINNED> , <https://w3id.org/product/DistributionChamberElement%2FINSPECTIONPIT> , <https://w3id.org/product/DuctSilencer> , <https://w3id.org/product/DistributionChamberElement%2FSUMP> .

props:airPressureDropCurve
        a                      owl:DatatypeProperty ;
        rdfs:comment           "Courbe de perte de charge aéraulique, courbe perte de charge/débit."@fr-FR , "風量の関数としての空気圧力降下"@ja-JP , "Air pressure drop curve, pressure drop – flow rate curve, AirPressureDrop = f (AirflowRate)."@en , "Air pressure drop as function of air flow rate."@en , "Air pressure drop versus air-flow rate."@en , "Air pressure drop as a function of air flow rate."@en ;
        rdfs:label             "CourbePerteDeChargeAir"@fr-FR , "airPressureDropCurve"@en , "圧力降下曲線"@ja-JP ;
        schema:domainIncludes  <https://w3id.org/product/DuctSilencer> , <https://w3id.org/product/Coil> , <https://w3id.org/product/EvaporativeCooler> , <https://w3id.org/product/Humidifier> .

props:energyGainSensible
        a                      owl:DatatypeProperty ;
        rdfs:comment           "ピーク時各居室の最大冷房負荷と空調システムの顕熱負荷による最大顕熱負荷。"@ja-JP , "최대 각 거실 최대 냉방 부하 및 공조 시스템의 현열 부하에 의한 최대 현열 부하"@ko-KR , "The sum of total energy gains for the spaces served by the system during the peak cooling conditions, plus any system-level sensible energy gains."@en ;
        rdfs:label             "현열 공조 부하"@ko-KR , "energyGainSensible"@en , "顕熱空調負荷"@ja-JP ;
        rdfs:range             <https://w3id.org/product/PowerMeasure> ;
        schema:domainIncludes  <https://w3id.org/product/Zone> , <https://w3id.org/product/SpatialZone> , <https://w3id.org/product/Space> .

props:hasLadder  a             owl:DatatypeProperty ;
        rdfs:comment           "Indication of whether the tank is provided with a ladder (set TRUE) for access to the top. If no ladder is provided then value is set FALSE.\n\nNote: No indication is given of the type of ladder (gooseneck etc.)"@en , "上部を点検するための梯子(TRUEに設定）をタンクに備えているかどうかの表示　もし、梯子が備え付けられていなければ値はFALSEと設定される。　　注：表示がない場合は梯子のタイプが与えられる（グースネック他）"@ja-JP ;
        rdfs:label             "hasLadder"@en , "梯子有り"@ja-JP ;
        rdfs:range             xsd:boolean ;
        schema:domainIncludes  <https://w3id.org/product/Tank> .

props:maximumSectionModulusZ
        a                      owl:DatatypeProperty ;
        rdfs:comment           "Bending resistance about the zs axis at the point with maximum ys ordinate. For example measured in mm³."@en ;
        rdfs:label             "maximumSectionModulusZ"@en ;
        rdfs:range             <https://w3id.org/product/SectionModulusMeasure> ;
        schema:domainIncludes  <https://w3id.org/product/ProfileDef> .

props:compressorCapacity
        a                      owl:DatatypeProperty ;
        rdfs:comment           "The product of the  ideal capacity and the overall volumetric efficiency of the compressor."@en , "Le produit de la puissance optimale par le rendement global du compresseur."@fr-FR ;
        rdfs:label             "compressorCapacity"@en , "PuissanceCompresseur"@fr-FR ;
        schema:domainIncludes  <https://w3id.org/product/Compressor> .

props:coreSetHorizontal
        a                      owl:DatatypeProperty ;
        rdfs:comment           "Degree of horizontal (in the X-axis of the LocalPlacement) blade set from the centerline."@en , "水平翼の中心線からの水平（ローカル座標のＸ軸）面の羽根角度"@ja-JP , "Degré d'inclinaison horizontale (selon l'axe X par rapport au positionnement local) de la lame mesuré depuis la ligne médiane."@fr-FR ;
        rdfs:label             "coreSetHorizontal"@en , "水平羽根角度"@ja-JP , "PositionHorizontaleCentre"@fr-FR ;
        rdfs:range             <https://w3id.org/product/PlaneAngleMeasure> ;
        schema:domainIncludes  <https://w3id.org/product/AirTerminal> .

props:spaceMeanRadiantTemperature
        a                      owl:DatatypeProperty ;
        rdfs:comment           "Mean radiant temperature in the space."@en , "部屋の平均放射温度"@ja-JP ;
        rdfs:label             "spaceMeanRadiantTemperature"@en , "室平均放射温度"@ja-JP ;
        schema:domainIncludes  <https://w3id.org/product/SpaceHeater> .

props:flowCoefficient
        a                      owl:DatatypeProperty ;
        rdfs:comment           "Flow coefficient (the quantity of fluid that passes through a fully open valve at unit pressure drop), typically expressed as the Kv or Cv value for the valve."@en , "流出係数（全開のバルブを通過する単位圧力損失当たりの流体の量）一般的にバルブのKv又はCv値で表される"@ja-JP ;
        rdfs:label             "flowCoefficient"@en , "流出係数"@ja-JP ;
        rdfs:range             xsd:decimal ;
        schema:domainIncludes  <https://w3id.org/product/Valve> .

props:c  a                     owl:DatatypeProperty ;
        rdfs:comment           "Measure c according to ISO 2553"@en ;
        rdfs:label             "c"@en ;
        rdfs:range             <https://w3id.org/product/PositiveLengthMeasure> ;
        schema:domainIncludes  <https://w3id.org/product/Fastener%2FWELD> .

props:marketSubCategory
        a                      owl:DatatypeProperty ;
        rdfs:comment           "Sous catégorie d'usage."@fr-FR , "Subset of category of use e.g. multi-family, 2 bedroom, low rise."@en , "Sous catégorie d'usage (exemple : collectif, deux pièces,…)"@fr-FR ;
        rdfs:label             "SousCategorieUsage"@fr-FR , "marketSubCategory"@en , "SousCategorieMarche"@fr-FR ;
        rdfs:range             xsd:string ;
        schema:domainIncludes  <https://w3id.org/product/Building> .

props:riskCause  a             owl:DatatypeProperty ;
        rdfs:comment           "A value that may be assigned to capture the cause or trigger for the risk. An example might be 'poor fixing'."@en ;
        rdfs:label             "riskCause"@en ;
        rdfs:range             xsd:string ;
        schema:domainIncludes  <https://w3id.org/product/Process> .

props:gasPressure  a           owl:DatatypeProperty ;
        rdfs:comment           "Fill pressure (e.g. for between-pane gas fills): the pressure exerted by a mass of gas confined in a constant volume."@en ;
        rdfs:label             "gasPressure"@en ;
        rdfs:range             <https://w3id.org/product/PressureMeasure> ;
        schema:domainIncludes  <https://w3id.org/product/Material> .

props:thickness3  a            owl:DatatypeProperty ;
        rdfs:comment           "Third thickness parameter of a surface member with varying thickness"@en ;
        rdfs:label             "thickness3"@en ;
        rdfs:range             <https://w3id.org/product/PositiveLengthMeasure> ;
        schema:domainIncludes  <https://w3id.org/product/StructuralSurfaceMemberVarying> .

props:ladderTrussBaseBarDiameter
        a                      owl:DatatypeProperty ;
        rdfs:comment           "The nominal diameter of the base bar."@en , "ベースバーの公称直径。"@ja-JP , "기반 막대의 공칭 지름"@ko-KR ;
        rdfs:label             "ladderTrussBaseBarDiameter"@en , "ベースバー径"@ja-JP , "기반 막대 지름"@ko-KR ;
        rdfs:range             <https://w3id.org/product/PositiveLengthMeasure> ;
        schema:domainIncludes  <https://w3id.org/product/DiscreteAccessory%2FLadder%20truss%20connector> .

props:internalWaterVolume
        a                      owl:DatatypeProperty ;
        rdfs:comment           "Internal volume of evaporator (water side)."@en , "蒸発器（水側）の内部容積"@ja-JP , "Internal volume of condenser (water side)."@en ;
        rdfs:label             "内部水容積"@ja-JP , "internalWaterVolume"@en ;
        rdfs:range             <https://w3id.org/product/VolumeMeasure> ;
        schema:domainIncludes  <https://w3id.org/product/Evaporator> , <https://w3id.org/product/Condenser> .

props:faceVelocity  a          owl:DatatypeProperty ;
        rdfs:comment           "Air velocity through the coil."@en , "Vitesse de l'air à travers la batterie."@fr-FR ;
        rdfs:label             "faceVelocity"@en , "VitesseFace"@fr-FR ;
        schema:domainIncludes  <https://w3id.org/product/Coil> .

props:hoseConnectionSize
        a                      owl:DatatypeProperty ;
        rdfs:comment           "The size of connections to which a hose may be connected (other than that to be linked to a pumping unit)."@en , "接続ホースのサイズ（ポンプユニット接続以外の）。"@ja-JP ;
        rdfs:label             "hoseConnectionSize"@en , "ホース接続サイズ"@ja-JP ;
        rdfs:range             <https://w3id.org/product/PositiveLengthMeasure> ;
        schema:domainIncludes  <https://w3id.org/product/FireSuppressionTerminal%2FFIREHYDRANT> .

props:isPluggableOutlet
        a                      owl:DatatypeProperty ;
        rdfs:comment           "Indication of whether the outlet accepts a loose plug connection (= TRUE) or whether it is directly connected (= FALSE) or whether the form of connection has not yet been determined (= UNKNOWN)."@en , "差込口が緩いプラグ接続を認めるか、それが直接接続されるかどうか、あるいは接続の形式がまだ決定されていないかを指示する。"@ja-JP , "슬롯이 느슨한 플러그를 인정하거나 그것에 직접 연결되는지 여부, 연결 형식이 아직 결정되지 않았는지 설명한다"@ko-KR ;
        rdfs:label             "isPluggableOutlet"@en , "プラグ接続可否"@ja-JP , "플러그 여부"@ko-KR ;
        rdfs:range             xsd:boolean ;
        schema:domainIncludes  <https://w3id.org/product/Outlet> .

props:projectorType  a         owl:DatatypeProperty ;
        rdfs:comment           "Indicates the type of projector."@en , "プロジェクタの形式を示す。"@ja-JP , "프로젝터의 형식을 보여준다."@ko-KR ;
        rdfs:label             "projectorType"@en , "プロジェクター形式"@ja-JP , "프로젝터 형식"@ko-KR ;
        schema:domainIncludes  <https://w3id.org/product/AudioVisualAppliance%2FPROJECTOR> .

props:panTiltZoomPreset
        a                      owl:DatatypeProperty ;
        rdfs:comment           "Indicates pan/tilt/zoom position presets."@en , "パン・チルト・ズーム機能の初期設定。"@ja-JP ;
        rdfs:label             "panTiltZoomPreset"@en , "パン・チルト・ズーム初期設定"@ja-JP ;
        schema:domainIncludes  <https://w3id.org/product/AudioVisualAppliance%2FCAMERA> .

props:withLock  a              owl:DatatypeProperty ;
        rdfs:comment           "Indicates whether the file cabinet is lockable (= TRUE) or not (= FALSE)."@en ;
        rdfs:label             "withLock"@en ;
        rdfs:range             xsd:boolean ;
        schema:domainIncludes  <https://w3id.org/product/Furniture%2FFILECABINET> .

props:ductSealant  a           owl:DatatypeProperty ;
        rdfs:comment           "Type of sealant used on the duct and fittings."@en , "ダクトと継ぎ手の密閉形式。"@ja-JP , "덕트와 이음새의 밀폐 형식입니다."@ko-KR ;
        rdfs:label             "ductSealant"@en , "ダクトの密閉性"@ja-JP , "덕트 밀폐"@ko-KR ;
        schema:domainIncludes  <https://w3id.org/product/DistributionSystem%2FVENTILATION> .

props:type2  a                 owl:DatatypeProperty ;
        rdfs:comment           "See Type1."@en ;
        rdfs:label             "type2"@en ;
        rdfs:range             xsd:string ;
        schema:domainIncludes  <https://w3id.org/product/Fastener%2FWELD> .

props:hasIntegralControl
        a                      owl:DatatypeProperty ;
        rdfs:comment           "If TRUE, a self powered temperature control is included in the AirTerminal."@en , "もし真なら、ターミナルに自身による温度制御が含まれる"@ja-JP , "Si VRAI, une commande interne de la température est incluse dans le terminal de ventilation."@fr-FR ;
        rdfs:label             "hasIntegralControl"@en , "自己制御有無"@ja-JP , "PossèdeContrôleTotal"@fr-FR ;
        rdfs:range             xsd:boolean ;
        schema:domainIncludes  <https://w3id.org/product/AirTerminal> .

props:fireProtectionClass
        a                      owl:DatatypeProperty ;
        rdfs:comment           "Zugewiesene Gebäudeklasse nach der nationalen Brandschutzverordnung."@de-DE , "主要な防火等級。関連する建築基準法、消防法などの国家基準を参照。"@ja-JP , "Classe principale de protection contre le risque incendie, selon la réglementation nationale."@fr-FR , "주요 방화 등급. 관련 건축 기준법, 소방법 등의 국가 표준을 참조하십시오."@ko-KR , "Main fire protection class for the building which is assigned from the fire protection classification table as given by the relevant national building code."@en ;
        rdfs:label             "耐火等級"@ja-JP , "fireProtectionClass"@en , "방화 등급"@ko-KR , "Gebäudeklasse Brandschutz"@de-DE , "RisqueIncendieUsageSecondaire"@fr-FR ;
        rdfs:range             xsd:string ;
        schema:domainIncludes  <https://w3id.org/product/Building> .

props:isHorizontalBusbar
        a                      owl:DatatypeProperty ;
        rdfs:comment           "Indication of whether the busbar occurrences are routed horizontally (= TRUE) or vertically (= FALSE)."@en , "母線は、水平方向にルーティングされるかどうかを示す（= TRUE）または垂直方向に（= FALSE）を返します。"@ja-JP , "모선은 가로로 라우팅되는지 여부를 나타내는 (= TRUE) 또는 수직 (= FALSE)를 반환합니다."@ko-KR ;
        rdfs:label             "isHorizontalBusbar"@en , "水平母線"@ja-JP , "수평 모선"@ko-KR ;
        rdfs:range             xsd:boolean ;
        schema:domainIncludes  <https://w3id.org/product/CableSegment%2FBUSBARSEGMENT> .

props:flowRateRange  a         owl:DatatypeProperty ;
        rdfs:comment           "Allowable range of volume of fluid being pumped against the resistance specified."@en , "指定された抵抗に対してポンプでくみ上げ可能な流対量の許容範囲"@ja-JP , "Possible range of fluid flowrate that can be delivered."@en ;
        rdfs:label             "流量範囲"@ja-JP , "flowRateRange"@en ;
        schema:domainIncludes  <https://w3id.org/product/Pump> , <https://w3id.org/product/Filter> .

props:releaseTimeI2tStart
        a                      owl:DatatypeProperty ;
        rdfs:comment           "G 함수 특성 곡선 I2t의 시작점 [s]가 시작 방류 시간."@ko-KR , "The release time in [s] for the start point of the I2t tripping curve of the G-function, if any."@en , "The release time in [s] for the start point of the I2t tripping curve of the S-function, if any"@en , "S함수 특성 곡선 I2t의 시작점 [s]가 시작 방류 시간."@ko-KR , "S関数の特性曲線I2tの始点[s]が開始放流時間。"@ja-JP , "G関数の特性曲線I2tの始点[s]が開始放流時間。"@ja-JP ;
        rdfs:label             "I2t 시작 방류 시간"@ko-KR , "releaseTimeI2tStart"@en , "I2tの開始放流時間"@ja-JP ;
        rdfs:range             <https://w3id.org/product/TimeMeasure> ;
        schema:domainIncludes  <https://w3id.org/product/ProtectiveDeviceTrippingUnit> .

props:nominalEfficiency
        a                      owl:DatatypeProperty ;
        rdfs:comment           "Efficactié nominale du groupe froid sous les conditions nominales."@fr-FR , "Efficacité nominale de la chaudière tel que définie par le constructeur.\nPour les chaudières à eau chaude, une fonction de la température en entrée par rapport à la température de sortie.\nRemarque: Comme deux variables sont utilisées ValeurDefinir et ValeursDefinies sont nulles, et les valeurs sont enregistrées dans IfcTable dans l'ordre suivant:\n- TempératureEntrée (IfcThermodynamicTemperatureMeasure) et TempératureSortie (IfcThermodynamicTemperatureMeasure) dans ValeursDefinir , et EfficacitéNominale (IfcNormalisedRatioMeasure) dansValeursDefinies.\nIfcTable est lié à IfcPropertyTableValue qui utilise IfcMetric et IfcPropertyConstraintRelationship."@fr-FR , "Nominal chiller efficiency under nominal conditions."@en , "Efficacité nominale de la chaudière tel que définie par le constructeur.\nPour les chaudières à vapeur, une fonction de la température en entrée par rapport à la pression de vapeur.\nRemarque: Comme deux variables sont utilisées ValeurDefinir et ValeursDefinies sont nulles, et les valeurs sont enregistrées dans IfcTable dans l'ordre suivant:\n- TempératureEntrée (IfcThermodynamicTemperatureMeasure) et TempératureSortie (IfcThermodynamicTemperatureMeasure) dans ValeursDefinir , et EfficacitéNominale (IfcNormalisedRatioMeasure) dansValeursDefinies.\nPar exemple, ValeursDefinir (TempératureEntrée, TempératureSortie), ValeursDefinies (nul, RendementNominal).\nIfcTable est lié à IfcPropertyTableValue qui utilise IfcMetric et IfcPropertyConstraintRelationship."@fr-FR , "The nominal efficiency of the boiler as defined by the manufacturer. For steam boilers, a function of inlet temperature versus steam pressure.  Note: as two variables are used, DefiningValues and DefinedValues are null, and values are stored in IfcTable in the following order: InletTemperature(IfcThermodynamicTemperatureMeasure) and OutletTemperature(IfcThermodynamicTemperatureMeasure) in DefiningValues, and NominalEfficiency(IfcNormalisedRatioMeasure) in DefinedValues. For example, DefininfValues(InletTemp, OutletTemp), DefinedValues(null, NominalEfficiency).  The IfcTable is related to IfcPropertyTableValue using IfcMetric and IfcPropertyConstraintRelationship."@en , "The nominal efficiency of the boiler as defined by the manufacturer. For water boilers, a function of inlet versus outlet temperature. Note: as two variables are used, DefiningValues and DefinedValues are null, and values are stored in IfcTable in the following order: InletTemperature(IfcThermodynamicTemperatureMeasure), OutletTemperature(IfcThermodynamicTemperatureMeasure), NominalEfficiency(IfcNormalizedRatioMeasure).  The IfcTable is related to IfcPropertyTableValue using IfcMetric and IfcPropertyConstraintRelationship."@en ;
        rdfs:label             "EfficacitéNominale"@fr-FR , "nominalEfficiency"@en ;
        rdfs:range             <https://w3id.org/product/PositiveRatioMeasure> ;
        schema:domainIncludes  <https://w3id.org/product/Chiller> , <https://w3id.org/product/Boiler%2FSTEAM> , <https://w3id.org/product/Boiler%2FWATER> .

props:width  a                 owl:DatatypeProperty ;
        rdfs:comment           "排水チャンバーの幅。"@ja-JP , "The width of the trench."@en , "홈의 길이"@ko-KR , "溝の長さ。"@ja-JP , "피트 폭"@ko-KR , "La largeur requise de la réservation (extension horizontale en élévation). Fournie seulement si la propriété Forme a pour valeur \"Rectangle\"."@fr-FR , "Geforderte Breite des Durchbruchs, wird nur dann angegeben, wenn der Wert des Attributes \"Form\" gleich \"Rechteck\" ist."@de-DE , "The width of the sump."@en , "空間の幅（高さにおける水平方向の拡張）を求める定義です。「四角形」の形状プロパティのみ提示されます。"@ja-JP , "The requested width (horizontal extension in elevation) of the provision for void, only provided if the Shape property is set to \"rectangle\"."@en , "The width of the pit."@en , "ピット幅。"@ja-JP , "空构件的宽度（在立面图中水平方向的长度），仅当“形状”属性为“矩形”时适用。"@zh-CN , "배수 챔버의 폭"@ko-KR ;
        rdfs:label             "宽度"@zh-CN , "Largeur"@fr-FR , "Breite"@de-DE , "長さ"@ja-JP , "width"@en , "폭"@ko-KR , "幅"@ja-JP , "길이"@ko-KR ;
        rdfs:range             <https://w3id.org/product/PositiveLengthMeasure> ;
        schema:domainIncludes  <https://w3id.org/product/BuildingElementProxy%2FPROVISIONFORVOID> , <https://w3id.org/product/DistributionChamberElement%2FINSPECTIONPIT> , <https://w3id.org/product/DistributionChamberElement%2FSUMP> , <https://w3id.org/product/DistributionChamberElement%2FTRENCH> .

props:specificHeatTemperatureDerivative
        a                      owl:DatatypeProperty ;
        rdfs:comment           "Specific heat temperature derivative."@en ;
        rdfs:label             "specificHeatTemperatureDerivative"@en ;
        rdfs:range             xsd:decimal ;
        schema:domainIncludes  <https://w3id.org/product/Material> .

props:specificHeatCapacity
        a                      owl:DatatypeProperty ;
        rdfs:comment           "Defines the specific heat of the material: heat energy absorbed per temperature unit."@en , "Specific heat of the products of combustion: heat energy absorbed per temperature unit."@en ;
        rdfs:label             "specificHeatCapacity"@en ;
        rdfs:range             <https://w3id.org/product/SpecificHeatCapacityMeasure> ;
        schema:domainIncludes  <https://w3id.org/product/Material> .

props:partialLoadEfficiencyCurves
        a                      owl:DatatypeProperty ;
        rdfs:comment           "Boiler efficiency as a function of the partial load factor; E = f (partialLaodfactor)."@en , "部分負荷係数の関数としてのボイラ効率　　E=f(部分負荷率）"@ja-JP , "Rendement de la chaudière en fonction de la facteur de charge partielle; E= f(FacteurChargePartielle)."@fr-FR ;
        rdfs:label             "partialLoadEfficiencyCurves"@en , "部分負荷効率曲線"@ja-JP , "CourbesEfficacitéChargePartielle"@fr-FR ;
        schema:domainIncludes  <https://w3id.org/product/Boiler> .

props:foulingFactor  a         owl:DatatypeProperty ;
        rdfs:comment           "Fouling factor of the tubes in the tube bundle."@en , "チューブ束のチューブ汚れ係数"@ja-JP ;
        rdfs:label             "foulingFactor"@en , "汚れ係数"@ja-JP ;
        rdfs:range             <https://w3id.org/product/ThermalResistanceMeasure> ;
        schema:domainIncludes  <https://w3id.org/product/TubeBundle> .

props:accessCoverMaterial
        a                      owl:DatatypeProperty ;
        rdfs:comment           "The material from which the access cover to the chamber is constructed.\nNOTE: It is assumed that chamber walls will be constructed of a single material."@en , "액세스 (체크) 커버의 재질 주 : 챔퍼 공간의 벽은 단층 가정"@ko-KR , "액세스 (체크) 커버의 재질 주 : 바이브 공간의 벽은 단층 가정"@ko-KR , "アクセス（点検）カバーの材質。\n注：バイブスペースの壁は単層と仮定する"@ja-JP ;
        rdfs:label             "사용(체크)커버의 재질"@ko-KR , "アクセス（点検）カバーの材質"@ja-JP , "accessCoverMaterial"@en , "사용 (체크) 커버의 재질"@ko-KR ;
        schema:domainIncludes  <https://w3id.org/product/DistributionChamberElement%2FMETERCHAMBER> , <https://w3id.org/product/DistributionChamberElement%2FMANHOLE> , <https://w3id.org/product/DistributionChamberElement%2FVALVECHAMBER> , <https://w3id.org/product/DistributionChamberElement%2FINSPECTIONCHAMBER> .

props:readOutType  a           owl:DatatypeProperty ;
        rdfs:comment           "Indication of the form that readout from the meter takes. In the case of a dial read out, this may comprise multiple dials that give a cumulative reading and/or a mechanical odometer."@en ;
        rdfs:label             "readOutType"@en ;
        schema:domainIncludes  <https://w3id.org/product/FlowMeter> .

props:totalAirflow  a          owl:DatatypeProperty ;
        rdfs:comment           "난방, 냉방 조건 중 하나 큰 조건에서 요구되는 설계 급기 량"@ko-KR , "The total design supply air flowrate required for the system for either heating or cooling conditions, whichever is greater."@en , "暖房、冷房の条件の、いずれか大きい条件で要求される設計給気量。"@ja-JP ;
        rdfs:label             "totalAirflow"@en , "급기량"@ko-KR , "給気量"@ja-JP ;
        rdfs:range             <https://w3id.org/product/VolumetricFlowRateMeasure> ;
        schema:domainIncludes  <https://w3id.org/product/Space> , <https://w3id.org/product/Zone> , <https://w3id.org/product/SpatialZone> .

props:coolingTemperatureDelta
        a                      owl:DatatypeProperty ;
        rdfs:comment           "Cooling temperature difference for calculating space air flow rates."@en , "空調送風量計算用の冷房給気温度差。"@ja-JP , "에어컨 송풍 량 계산을위한 냉방 급기 온도차"@ko-KR ;
        rdfs:label             "冷房時送風温度差"@ja-JP , "coolingTemperatureDelta"@en , "냉방시 돌풍 온도차"@ko-KR ;
        rdfs:range             <https://w3id.org/product/ThermodynamicTemperatureMeasure> ;
        schema:domainIncludes  <https://w3id.org/product/SpatialZone> , <https://w3id.org/product/Zone> , <https://w3id.org/product/Space> .

props:ifNotAccomplished
        a                      owl:DatatypeProperty ;
        rdfs:comment           "Comments if the job is not accomplished."@en ;
        rdfs:label             "ifNotAccomplished"@en ;
        rdfs:range             xsd:string ;
        schema:domainIncludes  <https://w3id.org/product/ProjectOrder%2FWORKORDER> , <https://w3id.org/product/ProjectOrder%2FMAINTENANCEWORKORDER> .

props:infiltration  a          owl:DatatypeProperty ;
        rdfs:comment           "Luftaustausch über die Fugen des geschlossenen Fensters  (Q-Wert). Gibt die Luftdurchlässigkeit des gesamten Fensters bei einem Luftdruckniveau von 50 Pascal an."@de-DE , "Luftaustausch über die Fugen der geschlossenen Tür  (Q-Wert). Gibt die Luftdurchlässigkeit der gesamten Tür bei einem Luftdruckniveau von 50 Pascal an."@de-DE , "在50帕斯卡压强下填充物面积上外部空气对填充物的渗透流速。在部分接缝的长度未知时应使用该属性。"@zh-CN , "Infiltration flowrate of outside air for the filler object based on the area of the filler object at a pressure level of 50 Pascals. It shall be used, if the length of all joints is unknown."@en , "Taux d'infiltration de l'air extérieur lorsqu'on soumet la porte à une pression de 50 pascals. Cette valeur sera utilisée si la longueur des joints n'est pas connue."@fr-FR , "隙間風の流量値。"@ja-JP ;
        rdfs:label             "渗风量"@zh-CN , "TauxInfiltration"@fr-FR , "隙間風"@ja-JP , "Luftdurchlässigkeit"@de-DE , "infiltration"@en ;
        rdfs:range             <https://w3id.org/product/VolumetricFlowRateMeasure> ;
        schema:domainIncludes  <https://w3id.org/product/Window> , <https://w3id.org/product/Door> .

props:clearWidth  a            owl:DatatypeProperty ;
        rdfs:comment           "オブジェクト（エレベータ）の幅。エレベータ昇降機内部表面の左から右の距離を示す。\n形状表現は、Shape representation（IFCの幾何形状表現）およびそこで設定されている幾何形状パラメータにより与えられる。もし、幾何形状パラメータと形状プロパティ情報が一致しない場合は、形状パラメータの値を優先する。"@ja-JP , "덕트 공간 폭"@ko-KR , "Largeur du passage. Mesure de la distance entre les deux rampes ou entre le mur et la rampe. Cette propriété est donnée en complément de la représentation de la forme de l'élément et des paramètres géométriques qui la déterminent. En cas d'incohérence entre ces paramètres géométriques et cette propriété, ce sont les paramètres géométriques qui priment."@fr-FR , "通道入口和出口实际测量的净宽度，以两侧扶手之间或墙与坡道扶手之间的距离为准。\n该属性所提供的形状信息是对内部形状描述和几何参数的补充。如果几何参数与该属性所提供的形状属性不符，应以几何参数为准。"@zh-CN , "The width of the formed space in the duct."@en , "Largeur du passage de l'ascenseur. Elle indique la distance entre les surfaces intérieures gauche et droite de la cabine depuis la porte de l'ascenseur. Cette propriété est donnée en complément de la représentation de la forme de l'élément et des paramètres géométriques qui la déterminent. En cas d'incohérence entre ces paramètres géométriques et cette propriété, ce sont les paramètres géométriques qui priment."@fr-FR , "ダクトスペースの幅。"@ja-JP , "Actual clear width measured as the clear space for accessibility and egress; it is a measured distance betwen the two handrails or the wall and a handrail on a ramp.\nThe shape information is provided in addition to the shape representation and the geometric parameters used within. In cases of inconsistency between the geometric parameters and the shape properties, provided in the attached property, the geometric parameters take precedence."@en , "実際の通路の有効幅\n形情報は、内側は使用される形表現および幾何学的媒介変数に加えて提供されます。幾何学的媒介変数と形特性の間の矛盾の場合では、付属の特性の中で提供されて、幾何学的媒介変数は先行をとります。\""@ja-JP , "Clear width of the object (elevator). It indicates the distance from the inner surfaces of the elevator car left and right from the elevator door. \nThe shape information is provided in addition to the shape representation and the geometric parameters used within. In cases of inconsistency between the geometric parameters and the shape properties, provided in the attached property, the geometric parameters take precedence."@en , "German-description-3"@de-DE ;
        rdfs:label             "clearWidth"@en , "Lichte Breite"@de-DE , "通路有効寸法"@ja-JP , "Largeur du passage"@fr-FR , "LargeurPassage"@fr-FR , "폭"@ko-KR , "净宽"@zh-CN , "幅員"@ja-JP ;
        rdfs:range             <https://w3id.org/product/PositiveLengthMeasure> ;
        schema:domainIncludes  <https://w3id.org/product/DistributionChamberElement%2FFORMEDDUCT> , <https://w3id.org/product/RampFlight> , <https://w3id.org/product/TransportElement%2FELEVATOR> .

props:userCorrectionFactor
        a                      owl:DatatypeProperty ;
        rdfs:comment           "An arbitrary correction factor that may be applied by the user."@en ;
        rdfs:label             "userCorrectionFactor"@en ;
        rdfs:range             xsd:decimal ;
        schema:domainIncludes  <https://w3id.org/product/CableSegment> .

props:breechingInletType
        a                      owl:DatatypeProperty ;
        rdfs:comment           "Defines the type of breeching inlet."@en , "送水口タイプの定義。"@ja-JP ;
        rdfs:label             "breechingInletType"@en , "送水口タイプ"@ja-JP ;
        schema:domainIncludes  <https://w3id.org/product/FireSuppressionTerminal%2FBREECHINGINLET> .

props:weightedEfficiencyCurve
        a                      owl:DatatypeProperty ;
        rdfs:comment           "Weighted efficiency curve as a function of dust holding weight, efficiency = f (dust holding weight)."@en ;
        rdfs:label             "weightedEfficiencyCurve"@en ;
        schema:domainIncludes  <https://w3id.org/product/Filter%2FAIRPARTICLEFILTER> .

props:heatingCapacity
        a                      owl:DatatypeProperty ;
        rdfs:comment           "Heating capacity."@en , "加熱容量"@ja-JP ;
        rdfs:label             "heatingCapacity"@en , "加熱容量"@ja-JP ;
        rdfs:range             <https://w3id.org/product/PowerMeasure> ;
        schema:domainIncludes  <https://w3id.org/product/UnitaryEquipment%2FAIRCONDITIONINGUNIT> .

props:exhaustAir  a            owl:DatatypeProperty ;
        rdfs:comment           "Loads from exhaust air."@en , "排気による熱負荷。"@ja-JP , "배기에 의한 열부하"@ko-KR ;
        rdfs:label             "exhaustAir"@en , "排気"@ja-JP , "배기"@ko-KR ;
        schema:domainIncludes  <https://w3id.org/product/Space> .

props:bathType  a              owl:DatatypeProperty ;
        rdfs:comment           "The property enumeration defines the types of bath that may be specified within the property set where.\n\nDomestic: \tBath, for one person at a time, into which the whole body can be easily immersed.\nDomesticCorner: \tBath, for one person at a time, into which the whole body can be easily immersed and in which the immersion trough is at an angle.\nFoot: \tShallow bath for washing the feet.\nJacuzzi: \tWhirlpool bath for more than one person\nPlunge: \tBath, usually for more than one person at a time, into which the whole body can be easily immersed.\nSitz: \tBath in which a bather sits as in a chair.\nTreatment: \tBath used for hydrotherapy purposes.\nWhirlpool: \tBath in which an integrated device agitates the water by pumped circulation or induction of water and/or air."@en , "列挙するプロパティは、プロパティセット内で指定することができるバスの種類の定義：\n\n家庭用：全身を簡単に浸漬することができる一度に1人の人間が入るバス。\n\n家庭用Corner：浸漬トラフが傾いていて、全身を簡単に浸漬することができる一度に1人の人間が入るバス。\n\nフットバス：足を洗う浅いバス。\n\nジャグジー：複数の人のための渦のバス\n\nプランジバス：通常は全身を簡単に浸漬することができまる一度に複数の人の入るバス。\n\n座バス：水浴を椅子のように座って行うバス。\n\n治療バス：水浴セラピーの目的に使用されるバス。\n\n渦バス：ポンプによる水の循環や、水や空気の誘引により水を攪拌する統合された装置としてのバス。"@ja-JP ;
        rdfs:label             "bathType"@en , "バスタイプ"@ja-JP ;
        schema:domainIncludes  <https://w3id.org/product/SanitaryTerminal%2FBATH> .

props:viscosityTemperatureDerivative
        a                      owl:DatatypeProperty ;
        rdfs:comment           "Viscosity temperature derivative."@en ;
        rdfs:label             "viscosityTemperatureDerivative"@en ;
        rdfs:range             xsd:decimal ;
        schema:domainIncludes  <https://w3id.org/product/Material> .

props:capacityWeight  a        owl:DatatypeProperty ;
        rdfs:comment           "Capacité de transport de l'élément mesurée par le poids."@fr-FR , "Capacity of the transport element measured by weight."@en , "Kapazität nach Gewicht, das maximal befördert werden kann."@de-DE , "搬送要素の重さに関する容量。"@ja-JP ;
        rdfs:label             "capacityWeight"@en , "搭載重量"@ja-JP , "Lastkapazität"@de-DE , "Capacité en poids"@fr-FR ;
        rdfs:range             <https://w3id.org/product/MassMeasure> ;
        schema:domainIncludes  <https://w3id.org/product/TransportElement> .

props:coolingWetBulb  a        owl:DatatypeProperty ;
        rdfs:comment           "Outside wet bulb temperature for cooling design."@en , "冷房用設計用外気湿球温度。"@ja-JP , "냉방용 설계외기 습구온도"@ko-KR ;
        rdfs:label             "coolingWetBulb"@en , "冷房用設計外気湿球温度"@ja-JP , "냉방용 설계외기 습구온도"@ko-KR ;
        rdfs:range             <https://w3id.org/product/ThermodynamicTemperatureMeasure> ;
        schema:domainIncludes  <https://w3id.org/product/Building> .

props:designAmbientTemperature
        a                      owl:DatatypeProperty ;
        rdfs:comment           "The highest and lowest local ambient temperature likely to be encountered."@en ;
        rdfs:label             "designAmbientTemperature"@en ;
        schema:domainIncludes  <https://w3id.org/product/CableSegment> .

props:electricCookerType
        a                      owl:DatatypeProperty ;
        rdfs:comment           "Type of electric cooker."@en , "電気調理器のタイプ。"@ja-JP , "전자 조리기의 유형."@ko-KR ;
        rdfs:label             "electricCookerType"@en , "電気調理器のタイプ"@ja-JP , "전기 밥솥의 종류"@ko-KR ;
        schema:domainIncludes  <https://w3id.org/product/ElectricAppliance%2FELECTRICCOOKER> .

props:coreTopWidth  a          owl:DatatypeProperty ;
        rdfs:comment           "Core top width of the profile."@en ;
        rdfs:label             "coreTopWidth"@en ;
        rdfs:range             <https://w3id.org/product/PositiveLengthMeasure> ;
        schema:domainIncludes  <https://w3id.org/product/ArbitraryProfileDefWithVoids> .

props:standardFixingPlateWidth
        a                      owl:DatatypeProperty ;
        rdfs:comment           "The width of the standard fixing plate."@en , "標準的な固定プレートの幅。"@ja-JP , "표준 고정 플레이트의 폭"@ko-KR ;
        rdfs:label             "standardFixingPlateWidth"@en , "幅"@ja-JP , "폭"@ko-KR ;
        rdfs:range             <https://w3id.org/product/PositiveLengthMeasure> ;
        schema:domainIncludes  <https://w3id.org/product/DiscreteAccessory%2FStandard%20fixing%20plate> .

props:minimumPlateThickness
        a                      owl:DatatypeProperty ;
        rdfs:comment           "This value may be needed for stress analysis and to handle buckling problems. It can also be derived from the given profile geometry or classification and therefore it is only an optional feature allowing for an explicit description. For example measured in mm."@en ;
        rdfs:label             "minimumPlateThickness"@en ;
        rdfs:range             <https://w3id.org/product/PositiveLengthMeasure> ;
        schema:domainIncludes  <https://w3id.org/product/ProfileDef> .

props:conductorFunction
        a                      owl:DatatypeProperty ;
        rdfs:comment           "Function of a line conductor to which a device  is intended to be connected where L1, L2 and L3 represent the phase lines according to IEC 60446 notation (sometimes phase lines may be referenced by color [Red, Blue, Yellow] or by number [1, 2, 3] etc). Protective Earth is sometimes also known as CPC or common protective conductor. Note that for an electrical device, a set of line conductor functions may be applied."@en , "For ports distributing power, indicates function of the conductors to which the load is connected."@en , "電気負荷と連結する電線種類。"@ja-JP ;
        rdfs:label             "conductorFunction"@en , "電線種類"@ja-JP ;
        schema:domainIncludes  <https://w3id.org/product/DistributionElement> , <https://w3id.org/product/DistributionPort%2FELECTRICAL> .

props:playerMediaEject
        a                      owl:DatatypeProperty ;
        rdfs:comment           "Indicates whether the media can be ejected from the player (if physical media)."@en , "メディアを取り出すことができるかどうかを示す。"@ja-JP , "미디어를 꺼낼 수 있는지 여부를 나타낸다."@ko-KR ;
        rdfs:label             "playerMediaEject"@en , "メディア取り出し可否"@ja-JP , "미디어 꺼내기 여부"@ko-KR ;
        rdfs:range             xsd:boolean ;
        schema:domainIncludes  <https://w3id.org/product/AudioVisualAppliance%2FPLAYER> .

props:thermalMassHeatCapacity
        a                      owl:DatatypeProperty ;
        rdfs:comment           "Product of component mass and specific heat."@en , "質量あたりの熱容量"@ja-JP ;
        rdfs:label             "thermalMassHeatCapacity"@en , "保有熱容量"@ja-JP ;
        rdfs:range             xsd:decimal ;
        schema:domainIncludes  <https://w3id.org/product/SpaceHeater> .

props:style  a                 owl:DatatypeProperty ;
        rdfs:comment           "Description of the furniture style."@en ;
        rdfs:label             "style"@en ;
        rdfs:range             xsd:string ;
        schema:domainIncludes  <https://w3id.org/product/Furniture> .

props:mediaContent  a          owl:DatatypeProperty ;
        rdfs:comment           "Indicates the media content storage location, such as URLs to camera footage within particular time periods."@en ;
        rdfs:label             "mediaContent"@en ;
        schema:domainIncludes  <https://w3id.org/product/AudioVisualAppliance> .

props:portNumber  a            owl:DatatypeProperty ;
        rdfs:comment           "The port index for logically ordering the port within the containing element or element type."@en , "ポートに含まれる要素、種類を示す番号。"@ja-JP , "포트에 포함되는 요소 유형을 나타내는 숫자"@ko-KR ;
        rdfs:label             "portNumber"@en , "ポート番号"@ja-JP , "포트 번호"@ko-KR ;
        rdfs:range             xsd:int ;
        schema:domainIncludes  <https://w3id.org/product/DistributionPort> .

props:reactivePower  a         owl:DatatypeProperty ;
        rdfs:comment           "Reactive power."@en , "無効電力。"@ja-JP ;
        rdfs:label             "reactivePower"@en , "無効電力"@ja-JP ;
        schema:domainIncludes  <https://w3id.org/product/DistributionPort%2FELECTRICAL> .

props:airExchangeRate
        a                      owl:DatatypeProperty ;
        rdfs:comment           "Loads from the air exchange rate."@en , "換気による熱負荷。"@ja-JP , "환기에 의한 열부하"@ko-KR ;
        rdfs:label             "airExchangeRate"@en , "換気回数"@ja-JP , "환기회수"@ko-KR ;
        schema:domainIncludes  <https://w3id.org/product/Space> .

props:damperPosition  a        owl:DatatypeProperty ;
        rdfs:comment           "Position de contrôle du registre, compris entre 0 et 1."@fr-FR , "制御ダンパの開度（０～１）"@ja-JP , "Damper position (0-1); damper position ( 0=closed=90deg position angle, 1=open=0deg position angle."@en , "Control damper position, ranging from 0 to 1."@en ;
        rdfs:label             "Position du registre"@fr-FR , "damperPosition"@en , "ダンパ開度"@ja-JP ;
        schema:domainIncludes  <https://w3id.org/product/AirTerminalBox> , <https://w3id.org/product/Damper> .

props:mediaSource  a           owl:DatatypeProperty ;
        rdfs:comment           "Indicates media sources and corresponding names of ports (IfcDistributionPort with FlowDirection=SINK and PredefinedType=AUDIOVISUAL) or aggregated audio/video components (IfcAudioVisualAppliance)."@en , "メディアソースと定義済みタイプ(IfcDistributionPort with FlowDirection=SINK and PredefinedType=AUDIOVISUAL)及びaudio/videoを構成する集合に対応する名前。"@ja-JP , "미디어 소스 정의된 유형 (IfcDistributionPort with FlowDirection = SINK and PredefinedType = AUDIOVISUAL) 및 audio / video 구성 집합에 해당하는 이름."@ko-KR , "Indicates the media source where the identifier corresponds to an entry within the table of available media sources on Pset_AudioVisualApplianceTypeCommon.MediaSource."@en ;
        rdfs:label             "メディアソース"@ja-JP , "미디어 소스"@ko-KR , "mediaSource"@en ;
        schema:domainIncludes  <https://w3id.org/product/AudioVisualAppliance> .

props:commencementDate
        a                      owl:DatatypeProperty ;
        rdfs:comment           "Date on which the agreement commences."@en ;
        rdfs:label             "commencementDate"@en ;
        rdfs:range             xsd:date ;
        schema:domainIncludes  <https://w3id.org/product/SpatialStructureElement> .

props:edgeFixingPlateFlangeWidthInPlaneX
        a                      owl:DatatypeProperty ;
        rdfs:comment           "The flange width of the L-shaped edge plate in plane X."@en , "L型端部プレートのX面フランジ幅。"@ja-JP , "L 형 단부 플레이트 X면 플랜지 폭"@ko-KR ;
        rdfs:label             "edgeFixingPlateFlangeWidthInPlaneX"@en , "フランジ幅X"@ja-JP , "플랜지 폭 X"@ko-KR ;
        rdfs:range             <https://w3id.org/product/PositiveLengthMeasure> ;
        schema:domainIncludes  <https://w3id.org/product/DiscreteAccessory%2FEdge%20fixing%20plate> .

props:teTime  a                owl:DatatypeProperty ;
        rdfs:comment           "The maximum time (in s) at which the motor could run with locked rotor when the motor is used in an EX-environment. The time indicates that a protective device should trip before this time when the starting current of the motor is slowing through the device."@en , "モーターがEX環境でローターロックされて使用きる最大時間。\nモーター始動電流が機器を介して減速している時間より前に保護装置で停止する時間を示す。"@ja-JP , "모터가 EX 환경 로터 잠겨 사용 수있는 최대 시간. 모터 기동 전류가 장비를 통해 감속하고있다 시간 전에 보호 장치 중지 시간을 보여준다"@ko-KR ;
        rdfs:label             "teTime"@en , "最大時間"@ja-JP , "최대 시간"@ko-KR ;
        rdfs:range             <https://w3id.org/product/TimeMeasure> ;
        schema:domainIncludes  <https://w3id.org/product/ElectricMotor> .

props:remainingWork  a         owl:DatatypeProperty ;
        rdfs:comment           "The remaining work on behalf of the resource allocation."@en , "資源配分のための残存している作業。"@ja-JP ;
        rdfs:label             "remainingWork"@en , "残存作業時間"@ja-JP ;
        schema:domainIncludes  <https://w3id.org/product/ConstructionResource> .

props:temperatureFactor
        a                      owl:DatatypeProperty ;
        rdfs:comment           "열 전류 / 시간 미리 정의된 온도에 의해 주어진 값과 다른 경우 주위 온도에 맞추기위한 보정 계수 (% / deg K로 측정한다)."@ko-KR , "The correction factor (typically measured as %/deg K) for adjusting the thermal current/time to an ambient temperature different from the value given by the defined temperature."@en , "熱の電流/時間を、定義済みの温度によって与えられる値と異なる場合に周囲温度に合わせるための補正係数（%/deg K で計測する）。"@ja-JP ;
        rdfs:label             "温度係数"@ja-JP , "온도 계수"@ko-KR , "temperatureFactor"@en ;
        rdfs:range             <https://w3id.org/product/RatioMeasure> ;
        schema:domainIncludes  <https://w3id.org/product/ProtectiveDeviceTrippingUnit%2FTHERMAL> , <https://w3id.org/product/ProtectiveDeviceTrippingUnit%2FELECTROMAGNETIC> .

props:porosity  a              owl:DatatypeProperty ;
        rdfs:comment           "The void fraction of the total volume occupied by material (Vbr - Vnet)/Vbr."@en ;
        rdfs:label             "porosity"@en ;
        rdfs:range             <https://w3id.org/product/NormalisedRatioMeasure> ;
        schema:domainIncludes  <https://w3id.org/product/Material> .

props:keyOffset  a             owl:DatatypeProperty ;
        rdfs:comment           "Key offset of the profile."@en ;
        rdfs:label             "keyOffset"@en ;
        rdfs:range             <https://w3id.org/product/NonNegativeLengthMeasure> ;
        schema:domainIncludes  <https://w3id.org/product/ArbitraryProfileDefWithVoids> .

props:insideDiameter  a        owl:DatatypeProperty ;
        rdfs:comment           "Actual inner diameter of the tube in the tube bundle."@en , "チューブ束内のチューブ実内径"@ja-JP ;
        rdfs:label             "insideDiameter"@en , "内径"@ja-JP ;
        rdfs:range             <https://w3id.org/product/PositiveLengthMeasure> ;
        schema:domainIncludes  <https://w3id.org/product/TubeBundle> .

props:regeneratedSoundCurve
        a                      owl:DatatypeProperty ;
        rdfs:comment           "Regenerated sound versus air flow rate."@en ;
        rdfs:label             "regeneratedSoundCurve"@en ;
        schema:domainIncludes  <https://w3id.org/product/Damper> .

props:faucetType  a            owl:DatatypeProperty ;
        rdfs:comment           "Defines the range of faucet types that may be specified where:\n\nBib:\t Faucet with a horizontal inlet and a nozzle that discharges downwards.\nGlobe:\t Faucet fitted through the end of a bath, with a horizontal inlet, a partially spherical body and a vertical nozzle.\nDiverter: \tCombination faucet assembly with a valve to enable the flow of mixed water to be transferred to a showerhead.\nDividedFlowCombination:\t Combination faucet assembly in which hot and cold water are kept separate until emerging from a common nozzle\n.\nPillar:\t Faucet that has a vertical inlet and a nozzle that discharges downwards\n.\nSingleOutletCombination =\t Combination faucet assembly in which hot and cold water mix before emerging from a common nozzle\n.\nSpray:\t Faucet with a spray outlet\n.\nSprayMixing:\t Spray faucet connected to hot and cold water supplies that delivers water at a temperature determined during use."@en , "水栓タイプの範囲をここに明確に定義する\nBib = 入口が水平で、下に吐出するノズルの水栓　Globe =浴槽の端に付けられ、入口が水平で、本体が部分的に球形で、ノズルが垂直な水栓　Diverter =シャワーヘッドへの混合水の流れを変えられる弁を持った組合せ水栓　DividedFlowCombination = 共通のノズルから出るまで水と湯が分かれたままになっている組合せ水栓　Pillar =垂直な入口と下へ吐出するノズルを持った水栓　SingleOutletCombination =共通のノズルから出る前に水と湯が混合する組合せ水栓　Spray =スプレー状の吐出口を持った水栓　SprayMixing =使用中決められた温度で供給する給水と給湯に接続されたスプレー水栓"@ja-JP ;
        rdfs:label             "faucetType"@en , "水栓タイプ"@ja-JP ;
        schema:domainIncludes  <https://w3id.org/product/Valve%2FFAUCET> .

props:hasLiner  a              owl:DatatypeProperty ;
        rdfs:comment           "TRUE if the fitting has interior duct insulating lining, FALSE if it does not."@en , "内貼り保温ダクト内面にあるときにTRUE。無い時にFALSE"@ja-JP ;
        rdfs:label             "hasLiner"@en , "内張り有無"@ja-JP ;
        rdfs:range             xsd:boolean ;
        schema:domainIncludes  <https://w3id.org/product/DuctSegment> , <https://w3id.org/product/DuctFitting> .

props:perimeter  a             owl:DatatypeProperty ;
        rdfs:comment           "Perimeter of the profile for calculating the surface area. For example measured in mm."@en ;
        rdfs:label             "perimeter"@en ;
        rdfs:range             <https://w3id.org/product/PositiveLengthMeasure> ;
        schema:domainIncludes  <https://w3id.org/product/ProfileDef> .

props:ratedVoltage  a          owl:DatatypeProperty ;
        rdfs:comment           "The voltage that a device is designed to handle."@en , "사용할 수있는 권한이있는 허용 전압."@ko-KR , "使用できることが許可されている許容電圧。"@ja-JP , "장치를 사용할 보장된 전압. 상한은 최대."@ko-KR , "機器を使用できる保障された電圧。上限値は最大値。"@ja-JP , "The range of allowed voltage that a device is certified to handle. The upper bound of this value is the maximum."@en ;
        rdfs:label             "정격 전압"@ko-KR , "ratedVoltage"@en , "定格電圧"@ja-JP ;
        schema:domainIncludes  <https://w3id.org/product/DistributionElement> , <https://w3id.org/product/CableSegment%2FCABLESEGMENT> , <https://w3id.org/product/CableSegment%2FCORESEGMENT> .

props:supportDuringTransportDescription
        a                      owl:DatatypeProperty ;
        rdfs:comment           "Textual description of how the concrete element is supported during transportation."@en , "プレキャストコンクリート要素が輸送中における支持方法について書かれたテキスト文書。"@ja-JP ;
        rdfs:label             "supportDuringTransportDescription"@en , "輸送中の支持に関する記述"@ja-JP ;
        rdfs:range             xsd:string ;
        schema:domainIncludes  <https://w3id.org/product/BuildingElement> .

props:poleUsage  a             owl:DatatypeProperty ;
        rdfs:comment           "Pole usage."@en ;
        rdfs:label             "poleUsage"@en ;
        schema:domainIncludes  <https://w3id.org/product/ProtectiveDevice> .

props:relativeHumidity
        a                      owl:DatatypeProperty ;
        rdfs:comment           "Loads from the relative humidity."@en , "相対湿度による熱負荷。"@ja-JP , "상대습도에 의한 열부하"@ko-KR ;
        rdfs:label             "relativeHumidity"@en , "相対湿度"@ja-JP , "상대습도"@ko-KR ;
        schema:domainIncludes  <https://w3id.org/product/Space> .

props:isExtendedWarranty
        a                      owl:DatatypeProperty ;
        rdfs:comment           "Indication of whether this is an extended warranty whose duration is greater than that normally assigned to an artefact (=TRUE) or not (= FALSE)."@en ;
        rdfs:label             "isExtendedWarranty"@en ;
        rdfs:range             xsd:boolean ;
        schema:domainIncludes  <https://w3id.org/product/Element> .

props:flowRating  a            owl:DatatypeProperty ;
        rdfs:comment           "Actual flow capacity for the gutter. Value of 0.00 means this value has not been set."@en , "実際の排水流量　　０.00値はこの値がｾｯﾄされていないことを意味する　"@ja-JP ;
        rdfs:label             "flowRating"@en , "流量"@ja-JP ;
        rdfs:range             <https://w3id.org/product/VolumetricFlowRateMeasure> ;
        schema:domainIncludes  <https://w3id.org/product/PipeSegment%2FGUTTER> .

props:thermalTrippingUnitType
        a                      owl:DatatypeProperty ;
        rdfs:comment           "A list of the available types of thermal tripping unit  from which that required may be selected."@en , "選択を必要とするときのためのサーマルトリップ装置の選択リスト。"@ja-JP , "선택을 필요로하는 경우를위한 열 트립 장치 선택 목록."@ko-KR ;
        rdfs:label             "thermalTrippingUnitType"@en , "サーマルトリップ装置タイプ"@ja-JP , "열 트립 장치 유형"@ko-KR ;
        schema:domainIncludes  <https://w3id.org/product/ProtectiveDeviceTrippingUnit%2FTHERMAL> .

props:type  a                  owl:DatatypeProperty ;
        rdfs:comment           "Defines the allowed values for selection of the flow meter operation type."@en ;
        rdfs:label             "type"@en ;
        schema:domainIncludes  <https://w3id.org/product/FlowMeter%2FWATERMETER> .

props:solarRefractionIndex
        a                      owl:DatatypeProperty ;
        rdfs:comment           "Index of refraction (solar) defines the \"bending\" of the solar ray when it passes from one medium into another."@en ;
        rdfs:label             "solarRefractionIndex"@en ;
        rdfs:range             xsd:decimal ;
        schema:domainIncludes  <https://w3id.org/product/Material> .

props:placementType  a         owl:DatatypeProperty ;
        rdfs:comment           "暖房用ヒーターが置かれるようにどう設計されているかを示します。"@ja-JP , "Indicates how the space heater is designed to be placed."@en , "Indicates the placement of the coil.  \nFLOOR indicates an under floor heater (if coil type is WATERHEATINGCOIL or ELECTRICHEATINGCOIL); \nCEILING indicates a cooling ceiling (if coil type is WATERCOOLINGCOIL);\nUNIT indicates that the coil is part of a cooling or heating unit, like cooled beam, etc."@en , "Précise l'implantation de la batterie.\nPLANCHER indique que c'est un plancher chauffant (si le type de batterie is BATTERIEEAUCHAUDE ou CABLECHAUFFANTLECTRIQUE);\nPLAFOND indique un plafond rafraïchissant (si le type de la batterie est BATTERIEEAUFROIDE); UNITE indique que la batterie fait partie d'une unité de chauffage ou de refroidissement, tel que poutre froide, etc."@fr-FR ;
        rdfs:label             "TypeImplantation"@fr-FR , "プレースメントタイプ"@ja-JP , "placementType"@en ;
        schema:domainIncludes  <https://w3id.org/product/Coil> , <https://w3id.org/product/SpaceHeater> .

props:junctionRightAngle
        a                      owl:DatatypeProperty ;
        rdfs:comment           "The change of direction of flow for the right junction where 0 indicates straight segment."@en , "右継ぎ手の流れの方向の変化"@ja-JP ;
        rdfs:label             "junctionRightAngle"@en , "右継ぎ手角度"@ja-JP ;
        rdfs:range             <https://w3id.org/product/PositivePlaneAngleMeasure> ;
        schema:domainIncludes  <https://w3id.org/product/PipeFitting%2FJUNCTION> .

props:dischargePressureLoss
        a                      owl:DatatypeProperty ;
        rdfs:comment           "Fan discharge pressure loss associated with the discharge arrangement."@en , "吐出部に関連した吐出圧力損失"@ja-JP ;
        rdfs:label             "dischargePressureLoss"@en , "吐出圧力損失"@ja-JP ;
        schema:domainIncludes  <https://w3id.org/product/Fan> .

props:externalSurfaceArea
        a                      owl:DatatypeProperty ;
        rdfs:comment           "外表面積（一次・二次の両面積）"@ja-JP , "External surface area (both primary and secondary area)."@en ;
        rdfs:label             "外表面積"@ja-JP , "externalSurfaceArea"@en ;
        rdfs:range             <https://w3id.org/product/AreaMeasure> ;
        schema:domainIncludes  <https://w3id.org/product/Evaporator> , <https://w3id.org/product/Condenser> .

props:nominalSurroundingHumidityCooling
        a                      owl:DatatypeProperty ;
        rdfs:comment           "Nominal surrounding humidity (refers to nominal cooling capacity)."@en ;
        rdfs:label             "nominalSurroundingHumidityCooling"@en ;
        rdfs:range             <https://w3id.org/product/NormalisedRatioMeasure> ;
        schema:domainIncludes  <https://w3id.org/product/CooledBeam> .

props:softwareVersion
        a                      owl:DatatypeProperty ;
        rdfs:comment           "Indicates version of application software according to systems integrator."@en , "컨트롤러 소프트웨어 버전"@ko-KR ;
        rdfs:label             "softwareVersion"@en , "소프트웨어 버전"@ko-KR ;
        rdfs:range             xsd:string ;
        schema:domainIncludes  <https://w3id.org/product/Controller%2FPROGRAMMABLE> .

props:waterPressDropCurve
        a                      owl:DatatypeProperty ;
        rdfs:comment           "Water pressure drop as function of water flow rate."@en ;
        rdfs:label             "waterPressDropCurve"@en ;
        schema:domainIncludes  <https://w3id.org/product/EvaporativeCooler> .

props:flowArrangement
        a                      owl:DatatypeProperty ;
        rdfs:comment           "CounterFlow: Air and water flow enter in different directions.\n\nCrossFlow: Air and water flow are perpendicular.\nParallelFlow: Air and water flow enter in same directions."@en , "カウンタフロー：空気と水の流れが逆方向で入る\nクロスフロー：空気と「水の流れが垂直\n平行流：空気と水の流れが同じ方向で入る"@ja-JP , "CounterFlow: Air and water flow enter in different directions.\nCrossFlow: Air and water flow are perpendicular.\nParallelFlow: air and water flow enter in same directions."@en ;
        rdfs:label             "流れ種類"@ja-JP , "flowArrangement"@en ;
        schema:domainIncludes  <https://w3id.org/product/EvaporativeCooler> , <https://w3id.org/product/CoolingTower> .

props:airSideSystemDistributionType
        a                      owl:DatatypeProperty ;
        rdfs:comment           "基本的な空調方式（単一ダクト、二重ダクト、マルチゾーン等）。"@ja-JP , "This enumeration defines the basic types of air side systems (e.g., SingleDuct, DualDuct, Multizone, etc.)."@en , "기본적인 공조 방식 (단일 덕트, 이중 덕트, 멀티존 등)"@ko-KR ;
        rdfs:label             "airSideSystemDistributionType"@en , "搬送方式"@ja-JP , "반송방식"@ko-KR ;
        schema:domainIncludes  <https://w3id.org/product/Zone> , <https://w3id.org/product/SpatialZone> , <https://w3id.org/product/Space> .

props:airHandlerFanCoilArrangement
        a                      owl:DatatypeProperty ;
        rdfs:comment           "Enumeration defining the arrangement of the supply air fan and the cooling coil."@en , "給気ファンと冷却コイルの配置の定義列挙"@ja-JP ;
        rdfs:label             "airHandlerFanCoilArrangement"@en , "空調機ファン・コイル配列"@ja-JP ;
        schema:domainIncludes  <https://w3id.org/product/UnitaryEquipment%2FAIRHANDLER> .

props:waterFilterType
        a                      owl:DatatypeProperty ;
        rdfs:comment           "Further qualifies the type of water filter.  Filtration removes undissolved matter; Purification removes dissolved matter; Softening replaces dissolved matter."@en ;
        rdfs:label             "waterFilterType"@en ;
        schema:domainIncludes  <https://w3id.org/product/Filter%2FWATERFILTER> .

props:ventilation  a           owl:DatatypeProperty ;
        rdfs:comment           "要求された外気量。"@ja-JP , "요청한 외기 량"@ko-KR , "Required outside air ventilation."@en ;
        rdfs:label             "ventilation"@en , "외기량"@ko-KR , "外気量"@ja-JP ;
        rdfs:range             <https://w3id.org/product/VolumetricFlowRateMeasure> ;
        schema:domainIncludes  <https://w3id.org/product/SpatialZone> , <https://w3id.org/product/Space> , <https://w3id.org/product/Zone> .

props:flowClass  a             owl:DatatypeProperty ;
        rdfs:comment           "Alphanumeric indication of the flow class of a hydrant (may be used in connection with or instead of the FlowRate property)."@en , "消火栓流量クラスの英数字表示（流量属性と一緒に、または代わりに用いられる）。"@ja-JP ;
        rdfs:label             "flowClass"@en , "流量クラス"@ja-JP ;
        rdfs:range             xsd:string ;
        schema:domainIncludes  <https://w3id.org/product/FireSuppressionTerminal%2FFIREHYDRANT> .

props:admixturesDescription
        a                      owl:DatatypeProperty ;
        rdfs:comment           "Description of the admixtures added to the concrete mix."@en ;
        rdfs:label             "admixturesDescription"@en ;
        rdfs:range             xsd:string ;
        schema:domainIncludes  <https://w3id.org/product/Material%2FConcrete> .

props:subNatureOfRisk1
        a                      owl:DatatypeProperty ;
        rdfs:comment           "A first subsidiary value that might be assigned to designate a more specific type of risk.\n\nNOTE: Nature of risk may be identified in various ways depending upon the place where risk assessment takes place and according to local agreement. This property set allows for a generic nature of risk and up to two subsidiary natures. An example might be 'causing injury and damage'."@en ;
        rdfs:label             "subNatureOfRisk1"@en ;
        rdfs:range             xsd:string ;
        schema:domainIncludes  <https://w3id.org/product/Process> .

props:primaryCurrent  a        owl:DatatypeProperty ;
        rdfs:comment           "The current that is going to be transformed and that runs into the transformer on the primary side."@en , "変圧器の1次側に伝送される電流。"@ja-JP , "변압기 1 차 측에 전송되는 전류."@ko-KR ;
        rdfs:label             "primaryCurrent"@en , "第1電流"@ja-JP , "제 1 전류"@ko-KR ;
        rdfs:range             <https://w3id.org/product/ElectricCurrentMeasure> ;
        schema:domainIncludes  <https://w3id.org/product/Transformer> .

props:stemBaseWidth  a         owl:DatatypeProperty ;
        rdfs:comment           "Stem base width of the profile."@en ;
        rdfs:label             "stemBaseWidth"@en ;
        rdfs:range             <https://w3id.org/product/PositiveLengthMeasure> ;
        schema:domainIncludes  <https://w3id.org/product/ArbitraryClosedProfileDef> .

props:hasOpening  a            owl:DatatypeProperty ;
        rdfs:comment           "indicates whether the panel has an opening (= TRUE) or not (= FALSE)."@en ;
        rdfs:label             "hasOpening"@en ;
        rdfs:range             xsd:boolean ;
        schema:domainIncludes  <https://w3id.org/product/SystemFurnitureElement%2FPANEL> .

props:mode  a                  owl:DatatypeProperty ;
        rdfs:comment           "Table mapping operation mode identifiers to descriptive labels, which may be used for interpreting Pset_UnitaryControlElementPHistory.Mode."@en , "Indicates operation mode corresponding to Pset_UnitaryControlTypeCommon.Mode.  For example, 'HEAT', 'COOL', 'AUTO'."@en ;
        rdfs:label             "mode"@en ;
        schema:domainIncludes  <https://w3id.org/product/UnitaryControlElement> .

props:glassColor  a            owl:DatatypeProperty ;
        rdfs:comment           "Color (tint) selection for this glazing. It is given for information purposes only."@en , "Choix de la couleur (teinte) du vitrage. Donné à titre informatif seulement."@fr-FR , "ガラスの色合い。これは情報目的専用に提供される。"@ja-JP , "German-description-6"@de-DE , "玻璃（贴膜）的颜色。仅供参考。"@zh-CN ;
        rdfs:label             "玻璃颜色"@zh-CN , "German-name-6"@de-DE , "glassColor"@en , "ガラス色"@ja-JP , "CouleurVitrage"@fr-FR ;
        rdfs:range             xsd:string ;
        schema:domainIncludes  <https://w3id.org/product/cWindow> , <https://w3id.org/product/Door> .

props:ultimateStress  a        owl:DatatypeProperty ;
        rdfs:comment           "A measure of the ultimate stress of the material."@en ;
        rdfs:label             "ultimateStress"@en ;
        rdfs:range             <https://w3id.org/product/PressureMeasure> ;
        schema:domainIncludes  <https://w3id.org/product/Material%2FSteel> .

props:slope  a                 owl:DatatypeProperty ;
        rdfs:comment           "オブジェクト傾斜角度（水平が0.0度)\n現在の設計による通路のための実際の最大の傾斜。形情報は、内側は使用される形表現および幾何学的媒介変数に加えて提供されます。幾何学的媒介変数と形特性の間の矛盾の場合では、付属の特性の中で提供されて、幾何学的媒介変数は先行をとります。\""@ja-JP , "Angle d'inclinaison avec l'horizontale (0 degrés). Cette propriété est donnée en complément de la représentation de la forme de l'élément et des paramètres géométriques qui la déterminent. En cas d'incohérence entre ces paramètres géométriques et cette propriété, ce sont les paramètres géométriques qui priment."@fr-FR , "傾斜角度。水平を0度とする。"@ja-JP , "German-description-4"@de-DE , "傾斜角度。水平を0度とする。\n\nその形状（傾斜梁）情報は、表示のための形状に内部で使用される幾何学的パラメータを加えて提供される。形状情報と内部の幾何学的パラメータに矛盾が生じた場合は、幾何学的パラメータが優先される。幾何学的パラメ－タ編集アプリケーションでは、CADと同様に、この値は書き込み専用とする。"@ja-JP , "Angle of the gutter to allow for drainage."@en , "Slope angle - relative to horizontal (0.0 degrees).\n\nThe shape information is provided in addition to the shape representation and the geometric parameters used within. In cases of inconsistency between the geometric parameters and the shape properties, provided in the attached property, the geometric parameters take precedence.   For geometry editing applications, like CAD: this value should be write-only."@en , "Slope angle - relative to horizontal (0.0 degrees).\nThe shape information is provided in addition to the shape representation and the geometric parameters used within. In cases of inconsistency between the geometric parameters and the shape properties, provided in the attached property, the geometric parameters take precedence."@en , "排水に必要な溝の角度（傾斜）"@ja-JP , "Angle d'inclinaison avec l'horizontale (0 degrés). Cette propriété  est donnée en complément de la représentation de la forme et des paramètres géométriques qui la déterminent. En cas d'incohérence entre ces paramètres géométriques et cette propriété, ce sont les paramètres géométriques qui priment. Les applications qui déterminent la géométrie comme les logiciels de CAO ne doivent pas autoriser la modification de cette propriété"@fr-FR , "Angle d'inclinaison relativement à l'horizontale correspondant à la valeur 0 degrés. Valeur maximale de l'inclinaison actuellement projetée. Cette propriété est donnée en complément de la représentation de la forme de l'élément et des paramètres géométriques qui la déterminent. En cas d'incohérence entre ces paramètres géométriques et cette propriété, ce sont les paramètres géométriques qui priment."@fr-FR , "Angle d'inclinaison avec l'horizontale (0 degrés). Cette propriété est donnée en complément de la représentation de la forme et des paramètres géométriques qui la déterminent. En cas d'incohérence entre ces paramètres géométriques et cette propriété, ce sont les paramètres géométriques qui priment."@fr-FR , "相对于水平（0.0度）方向的坡度角。\n该属性所提供的形状信息是对内部形状描述和几何参数的补充。如果几何参数与该属性所提供的形状属性不符，应以几何参数为准。对CAD等几何编辑程序，该属性应为只写类型。"@zh-CN , "Slope angle - relative to horizontal (0.0 degrees).\n\nThe shape information is provided in addition to the shape representation and the geometric parameters used within. In cases of inconsistency between the geometric parameters and the shape properties, provided in the attached property, the geometric parameters take precedence.  For geometry editing applications, like CAD: this value should be write-only."@en , "German-description-3"@de-DE , "Neigungswinkel des Balkens relative zur Horizontalen (0 Grad).\n\nDieser Parameter wird zusätzlich zur geometrischen Repräsentation bereitgestellt. Im Fall der Inkonsistenz zwischen dem Parameter und der Geometrie hat die geometrische Repräsention Priorität. Dieser Parameter ist für CAD Software write-only."@de-DE , "构件相对于水平（0.0度）方向的实际坡度角。\n当前设计方案确定的通道的最大坡度。\n该属性所提供的形状信息是对内部形状描述和几何参数的补充。如果几何参数与该属性所提供的形状属性不符，应以几何参数为准。"@zh-CN , "Neigungswinkel der Stütze relative zur Horizontalen (0 Grad).\n\nDieser Parameter wird zusätzlich zur geometrischen Repräsentation bereitgestellt. Im Fall der Inkonsistenz zwischen dem Parameter und der Geometrie hat die geometrische Repräsention Priorität. Dieser Parameter ist für CAD Software write-only."@de-DE , "Sloping angle of the object  - relative to horizontal (0.0 degrees). \nActual maximum slope for the passageway according to the current design.\nThe shape information is provided in addition to the shape representation and the geometric parameters used within. In cases of inconsistency between the geometric parameters and the shape properties, provided in the attached property, the geometric parameters take precedence."@en ;
        rdfs:label             "通路の傾斜角度(水平からの角度）"@ja-JP , "Neigungswinkel"@de-DE , "Pente"@fr-FR , "slope"@en , "勾配"@ja-JP , "Inclinaison"@fr-FR , "傾斜"@ja-JP , "坡度"@zh-CN , "Neigung"@de-DE ;
        rdfs:range             <https://w3id.org/product/PlaneAngleMeasure> ;
        schema:domainIncludes  <https://w3id.org/product/PipeSegment%2FGUTTER> , <https://w3id.org/product/Beam> , <https://w3id.org/product/Column> , <https://w3id.org/product/Member> , <https://w3id.org/product/RampFlight> .

props:assessmentDate  a        owl:DatatypeProperty ;
        rdfs:comment           "Date on which the overall condition is assessed"@en , "全体状況を評価した日。"@ja-JP ;
        rdfs:label             "assessmentDate"@en , "評価日"@ja-JP ;
        rdfs:range             xsd:date ;
        schema:domainIncludes  <https://w3id.org/product/Element> .

props:wheelTipSpeed  a         owl:DatatypeProperty ;
        rdfs:comment           "Fan blade tip speed, typically defined as the linear speed of the tip of the fan blade furthest from the shaft."@en , "ファンブレード先端速度\n通常、軸から最も遠いファンブレードの先端の直線速度として定義されている"@ja-JP ;
        rdfs:label             "wheelTipSpeed"@en , "ホイール先端速度"@ja-JP ;
        schema:domainIncludes  <https://w3id.org/product/Fan> .

props:riskConsequence
        a                      owl:DatatypeProperty ;
        rdfs:comment           "Indicates the level of severity of the consequences that the risk would have in case it happens."@en ;
        rdfs:label             "riskConsequence"@en ;
        schema:domainIncludes  <https://w3id.org/product/Process> .

props:centerCoreBaseWidth
        a                      owl:DatatypeProperty ;
        rdfs:comment           "Center core base width of the profile."@en ;
        rdfs:label             "centerCoreBaseWidth"@en ;
        rdfs:range             <https://w3id.org/product/PositiveLengthMeasure> ;
        schema:domainIncludes  <https://w3id.org/product/ArbitraryProfileDefWithVoids> .

props:powerFactor  a           owl:DatatypeProperty ;
        rdfs:comment           "The ratio between the rated electrical power and the product of the rated current and rated voltage"@en , "Power factor."@en , "パワーファクタ。"@ja-JP ;
        rdfs:label             "powerFactor"@en , "パワーファクタ"@ja-JP ;
        rdfs:range             <https://w3id.org/product/NormalisedRatioMeasure> ;
        schema:domainIncludes  <https://w3id.org/product/DistributionElement> , <https://w3id.org/product/DistributionPort%2FELECTRICAL> .

props:crossingUpperBarPitch
        a                      owl:DatatypeProperty ;
        rdfs:comment           "The pitch length of the crossing upper bar."@en , "交差する上端筋間隔。"@ja-JP ;
        rdfs:label             "crossingUpperBarPitch"@en , "上端筋間隔"@ja-JP ;
        rdfs:range             <https://w3id.org/product/PositiveLengthMeasure> ;
        schema:domainIncludes  <https://w3id.org/product/Footing> .

props:nominalFlowrate
        a                      owl:DatatypeProperty ;
        rdfs:comment           "Nominal fluid flow rate through the filter."@en ;
        rdfs:label             "nominalFlowrate"@en ;
        rdfs:range             <https://w3id.org/product/VolumetricFlowRateMeasure> ;
        schema:domainIncludes  <https://w3id.org/product/Filter> .

props:speakerType  a           owl:DatatypeProperty ;
        rdfs:comment           "Indicates the type of speaker."@en , "スピーカーのタイプを示す。"@ja-JP , "스피커의 타입을 나타낸다."@ko-KR ;
        rdfs:label             "speakerType"@en , "スピーカータイプ"@ja-JP , "스피커 타입"@ko-KR ;
        schema:domainIncludes  <https://w3id.org/product/AudioVisualAppliance%2FSPEAKER> .

props:nominalRotationSpeed
        a                      owl:DatatypeProperty ;
        rdfs:comment           "多目的な状況の下でのポンプの回転速度"@ja-JP , "Nominal fan wheel speed."@en , "設計ホイール速度"@ja-JP , "Pump rotational speed under nominal conditions."@en ;
        rdfs:label             "設計回転速度"@ja-JP , "通常の回転速度"@ja-JP , "nominalRotationSpeed"@en ;
        rdfs:range             <https://w3id.org/product/RotationalFrequencyMeasure> ;
        schema:domainIncludes  <https://w3id.org/product/Pump> , <https://w3id.org/product/Fan> .

props:assessmentDescription
        a                      owl:DatatypeProperty ;
        rdfs:comment           "Qualitative description of the condition."@en , "状態に関する定性的な記述。"@ja-JP ;
        rdfs:label             "assessmentDescription"@en , "評価記述"@ja-JP ;
        rdfs:range             xsd:string ;
        schema:domainIncludes  <https://w3id.org/product/Element> .

props:treadLengthAtInnerSide
        a                      owl:DatatypeProperty ;
        rdfs:comment           "Longueur minimum des girons du côté intérieur de l'enroulement. Pertinent seulement pour les escaliers tournants car pour une volée droite, la valeur est donnée par la propriété \"Longueur du giron\". C'est une valeur précalculée. En cas d'incohérence, c'est la valeur dérivée de la représentation de la forme qui prime."@fr-FR , "German-description-9"@de-DE , "Minimum length of treads at the inner side of the winder. \nOnly relevant in case of winding flights, for straight flights it is identical with IfcStairFlight.TreadLength. It is a pre-calculated value, in case of inconsistencies, the value derived from the shape representation shall take precedence."@en , "螺旋楼梯踏板内侧的最小长度。\n该属性仅适用于螺旋楼梯。对直跑楼梯，该属性与IfcStairFlight.TreadLength一致。该属性为预设值，若有冲突，应以从形状描述得到的值为准。"@zh-CN ;
        rdfs:label             "LongueurGironCoteInterieur"@fr-FR , "minimaler Auftritt an der Innenseite"@de-DE , "内侧踏板长度"@zh-CN , "treadLengthAtInnerSide"@en ;
        rdfs:range             <https://w3id.org/product/PositiveLengthMeasure> ;
        schema:domainIncludes  <https://w3id.org/product/StairFlight> , <https://w3id.org/product/Stair> .

props:connectionGender
        a                      owl:DatatypeProperty ;
        rdfs:comment           "The physical connection gender."@en , "形状的な接続ジェンダー（オス、メス、その他、未知、未設定）。"@ja-JP ;
        rdfs:label             "connectionGender"@en , "接続ジェンダー"@ja-JP ;
        schema:domainIncludes  <https://w3id.org/product/DistributionPort%2FELECTRICAL> .

props:waterContent  a          owl:DatatypeProperty ;
        rdfs:comment           "Weight of water content within the heater."@en , "ヒーター内部の水分の重み"@ja-JP ;
        rdfs:label             "waterContent"@en , "水含量"@ja-JP ;
        rdfs:range             <https://w3id.org/product/MassMeasure> ;
        schema:domainIncludes  <https://w3id.org/product/SpaceHeater%2FRADIATOR> .

props:intermittent  a          owl:DatatypeProperty ;
        rdfs:comment           "If fillet weld, intermittent or not"@en ;
        rdfs:label             "intermittent"@en ;
        rdfs:range             xsd:boolean ;
        schema:domainIncludes  <https://w3id.org/product/Fastener%2FWELD> .

props:frequencyResponse
        a                      owl:DatatypeProperty ;
        rdfs:comment           "Indicates the output over a specified range of frequencies."@en , "周波数範囲での出力を示す。"@ja-JP , "주파수 범위에서 출력을 보여준다."@ko-KR ;
        rdfs:label             "frequencyResponse"@en , "周波数応答"@ja-JP , "주파수 응답"@ko-KR ;
        schema:domainIncludes  <https://w3id.org/product/AudioVisualAppliance%2FSPEAKER> .

props:radioactiveWastePerUnit
        a                      owl:DatatypeProperty ;
        rdfs:comment           "방사성 폐기물 발생량"@ko-KR , "Quantité de déchets radioactifs générés [NDT : selon la norme NF P01-010]"@fr-FR , "生成された放射性廃棄物の量。"@ja-JP , "Quantity of radioactive waste generated"@en ;
        rdfs:label             "単位あたり放射性廃棄物"@ja-JP , "DechetsRadioactifsParUnite"@fr-FR , "단위당 방사성 폐기물"@ko-KR , "radioactiveWastePerUnit"@en ;
        rdfs:range             <https://w3id.org/product/MassMeasure> ;
        schema:domainIncludes  <https://w3id.org/product/Element> .

props:evaporatorMeanVoidFraction
        a                      owl:DatatypeProperty ;
        rdfs:comment           "Mean void fraction in evaporator."@en , "蒸発器の平均の空隙率"@ja-JP ;
        rdfs:label             "evaporatorMeanVoidFraction"@en , "蒸発器平均空隙率"@ja-JP ;
        schema:domainIncludes  <https://w3id.org/product/Evaporator> .

props:selfTestFunction
        a                      owl:DatatypeProperty ;
        rdfs:comment           "The type of self test function."@en , "自己診断機能のタイプ。"@ja-JP , "자기 진단 기능의 유형"@ko-KR ;
        rdfs:label             "selfTestFunction"@en , "自己診断機能"@ja-JP , "자기 진단 기능"@ko-KR ;
        schema:domainIncludes  <https://w3id.org/product/LightFixture%2FSECURITYLIGHTING> .

props:accessLengthOrRadius
        a                      owl:DatatypeProperty ;
        rdfs:comment           "The length of the chamber access cover or, where the plan shape of the cover is circular, the radius."@en , "사용 (체크) 덮개 길이, 혹은 원형 커버 반경"@ko-KR , "アクセス（点検）カバーの長さ、或いは円形カバーの半径。"@ja-JP ;
        rdfs:label             "アクセス（点検）カバーの長さ或いは半径"@ja-JP , "accessLengthOrRadius"@en , "사용(체크)덮개 길이 혹은 반경"@ko-KR ;
        rdfs:range             <https://w3id.org/product/PositiveLengthMeasure> ;
        schema:domainIncludes  <https://w3id.org/product/DistributionChamberElement%2FMANHOLE> , <https://w3id.org/product/DistributionChamberElement%2FINSPECTIONCHAMBER> .

props:dischargeCoefficient
        a                      owl:DatatypeProperty ;
        rdfs:comment           "The coefficient of flow at the sprinkler."@en , "スプリンクラーの流れの係数。"@ja-JP ;
        rdfs:label             "dischargeCoefficient"@en , "流量係数"@ja-JP ;
        rdfs:range             xsd:decimal ;
        schema:domainIncludes  <https://w3id.org/product/FireSuppressionTerminal%2FSPRINKLER> .

props:specialConstruction
        a                      owl:DatatypeProperty ;
        rdfs:comment           "Special construction capabilities like self-supporting, flat devidable cable or bus flat non devidable cable or bus supporting elements inside (steal, textile, concentric conductor). Note that materials used should be agreed between exchange participants before use."@en , "特殊な構造を備えた性能－たとえば、平型フレキシブルケーブルあるいは硬い平型母線ケーブル、あるいは母線で内部に鉄製、繊維、同心導体で構成されているサポートを持っている。\n注記）使用する材料は、使用前に交流参加者間で合意すること。"@ja-JP , "특수한 구조를 갖춘 성능 - 예를 들어, 평형 플렉시블 케이블 또는 딱딱한 평형 모선 케이블 또는 모선 내부에 철제, 섬유, 동심 도체로 구성되어있는 지원이있다. 주) 사용하는 재료는 사용 전에 교류 참가자 사이에 동의한다."@ko-KR ;
        rdfs:label             "specialConstruction"@en , "特別な施工方法"@ja-JP , "특별한 시공 방법"@ko-KR ;
        rdfs:range             xsd:string ;
        schema:domainIncludes  <https://w3id.org/product/CableSegment%2FCABLESEGMENT> .

props:hardness  a              owl:DatatypeProperty ;
        rdfs:comment           "Water hardness as positive, multivalent ion concentration in the water (usually concentrations of calcium and magnesium ions in terms of calcium carbonate)."@en ;
        rdfs:label             "hardness"@en ;
        rdfs:range             <https://w3id.org/product/IonConcentrationMeasure> ;
        schema:domainIncludes  <https://w3id.org/product/Material> .

props:motorEnclosureType
        a                      owl:DatatypeProperty ;
        rdfs:comment           "A list of the available types of motor enclosure from which that required may be selected."@en , "モーターに必要な筐体を使用可能なタイプのリストから選択。"@ja-JP , "모터에 필요한 케이스를 사용 가능한 종류 목록에서 선택합니다."@ko-KR ;
        rdfs:label             "motorEnclosureType"@en , "モーター保護構造"@ja-JP , "모터 보호구조"@ko-KR ;
        schema:domainIncludes  <https://w3id.org/product/ElectricMotor> .

props:dualDeck  a              owl:DatatypeProperty ;
        rdfs:comment           "Does the AirHandler have a dual deck? TRUE = Yes, FALSE = No."@en , "空調機は2層になっているか\nTRUE=はい、FALSE=Iいいえ"@ja-JP ;
        rdfs:label             "dualDeck"@en , "2層"@ja-JP ;
        rdfs:range             xsd:boolean ;
        schema:domainIncludes  <https://w3id.org/product/UnitaryEquipment%2FAIRHANDLER> .

props:columnShoeBasePlateThickness
        a                      owl:DatatypeProperty ;
        rdfs:comment           "The thickness of the column shoe base plate."@en , "柱脚ベースプレートの板厚。"@ja-JP , "기둥 다리베이스 플레이트의 두께"@ko-KR ;
        rdfs:label             "columnShoeBasePlateThickness"@en , "ベースプレート厚"@ja-JP , "베이스 플레이트 두께"@ko-KR ;
        rdfs:range             <https://w3id.org/product/PositiveLengthMeasure> ;
        schema:domainIncludes  <https://w3id.org/product/DiscreteAccessory%2FSHOE> .

props:openPressureDrop
        a                      owl:DatatypeProperty ;
        rdfs:comment           "Total pressure drop across damper."@en ;
        rdfs:label             "openPressureDrop"@en ;
        rdfs:range             <https://w3id.org/product/PressureMeasure> ;
        schema:domainIncludes  <https://w3id.org/product/Damper> .

props:heatingTemperatureDelta
        a                      owl:DatatypeProperty ;
        rdfs:comment           "에어컨 송풍 량 계산을위한 난방 급기 온도차"@ko-KR , "空調送風量計算用の暖房給気温度差。"@ja-JP , "Heating temperature difference for calculating space air flow rates."@en ;
        rdfs:label             "暖房時送風温度差"@ja-JP , "난방시 돌풍 온도차"@ko-KR , "heatingTemperatureDelta"@en ;
        rdfs:range             <https://w3id.org/product/ThermodynamicTemperatureMeasure> ;
        schema:domainIncludes  <https://w3id.org/product/Space> , <https://w3id.org/product/SpatialZone> , <https://w3id.org/product/Zone> .

props:soffitLevel  a           owl:DatatypeProperty ;
        rdfs:comment           "Level of the highest internal part of the cross section as measured from ground level."@en , "단면의 가장 높은 부분의 깊이 (지상에서)"@ko-KR , "断面の最も高い部分の深さ（地面から）。"@ja-JP ;
        rdfs:label             "최소깊이"@ko-KR , "最小深さ"@ja-JP , "soffitLevel"@en ;
        rdfs:range             <https://w3id.org/product/LengthMeasure> ;
        schema:domainIncludes  <https://w3id.org/product/DistributionChamberElement%2FMANHOLE> , <https://w3id.org/product/DistributionChamberElement%2FINSPECTIONCHAMBER> .

props:thermalTransmittanceWinter
        a                      owl:DatatypeProperty ;
        rdfs:comment           "Thermal transmittance coefficient (U-Value) of a material.\nWinter thermal transmittance coefficient of the glazing only, often referred to as (U-value)."@en , "Coefficient de transmission thermique (U) d'un matériau. Coefficient de transmission thermique en hiver du vitrage seul, souvent désigné comme étant Uw."@fr-FR , "German-description-18"@de-DE , "素材の熱透過係数（U値）。夏期のガラスの熱透過係数だけ、U値として参照される。"@ja-JP , "材料的导热系数（U值）。\n仅玻璃的冬季导热系数，常以U值表示。"@zh-CN ;
        rdfs:label             "TransmittanceThermiqueHiver"@fr-FR , "冬季导热系数"@zh-CN , "German-name-16"@de-DE , "thermalTransmittanceWinter"@en , "冬季の熱透過係数"@ja-JP ;
        rdfs:range             <https://w3id.org/product/ThermalTransmittanceMeasure> ;
        schema:domainIncludes  <https://w3id.org/product/Door> , <https://w3id.org/product/cWindow> .

props:nutsCount  a             owl:DatatypeProperty ;
        rdfs:comment           "Count of nuts to be mounted on one bolt"@en ;
        rdfs:label             "nutsCount"@en ;
        rdfs:range             <https://w3id.org/product/CountMeasure> ;
        schema:domainIncludes  <https://w3id.org/product/MechanicalFastener%2FBOLT> .

props:isIlluminated  a         owl:DatatypeProperty ;
        rdfs:comment           "An indication of whether there is an illuminated indicator to show that the switch is on (=TRUE) or not (= FALSE)."@en , "イルミネーション型（自照型）表示機でスイッチのオン（TRUE）やオフ（FALSE）を示す。"@ja-JP , "일루미 네이션 형 (자조 형) 표시기 스위치를 켜거나 (TRUE) 또는 오프 (FALSE)를 나타낸다."@ko-KR ;
        rdfs:label             "isIlluminated"@en , "自照型"@ja-JP , "스위치 조명표시기"@ko-KR ;
        rdfs:range             xsd:boolean ;
        schema:domainIncludes  <https://w3id.org/product/SwitchingDevice> .

props:compressedAirFilterType
        a                      owl:DatatypeProperty ;
        rdfs:comment           "ACTIVATEDCARBON: absorbs oil vapor and odor; PARTICLE_FILTER: used to absorb solid particles of medium size; COALESCENSE_FILTER: used to absorb fine solid, oil, and water particles, also called micro filter"@en ;
        rdfs:label             "compressedAirFilterType"@en ;
        schema:domainIncludes  <https://w3id.org/product/Filter%2FCOMPRESSEDAIRFILTER> .

props:acquisitionDate
        a                      owl:DatatypeProperty ;
        rdfs:comment           "The date that the manufactured item was purchased."@en ;
        rdfs:label             "acquisitionDate"@en ;
        rdfs:range             xsd:date ;
        schema:domainIncludes  <https://w3id.org/product/Element> .

props:durabilityRating
        a                      owl:DatatypeProperty ;
        rdfs:comment           "Durability against mechanical stress. It is given according to the national code or regulation."@en , "Mechanische Widerstandsfähigkeit gegen immer wiederkehrende Bewegungen und Einflüsse gemäß der nationalen oder regionalen Richtlinie."@de-DE , "Durabilité au stress mécanique, selon une classification ou règlementation nationale."@fr-FR ;
        rdfs:label             "durabilityRating"@en , "Beanspruchungsklasse"@de-DE , "Durabilité"@fr-FR ;
        rdfs:range             xsd:string ;
        schema:domainIncludes  <https://w3id.org/product/Door> .

props:shortCircuit1PoleMaximumState
        a                      owl:DatatypeProperty ;
        rdfs:comment           "Maximum 1 pole short circuit current provided at the point of supply i.e. the fault between 1 phase and N."@en , "電源供給時点の点1相とN間の1極最大短絡電流。"@ja-JP , "전원 공급 시점 점 1 단계와 N 사이의 1 극 최대 단락 전류 역률."@ko-KR ;
        rdfs:label             "shortCircuit1PoleMaximumState"@en , "1極最大短絡電流"@ja-JP , "1 극 최대 단락 전류"@ko-KR ;
        rdfs:range             <https://w3id.org/product/ElectricCurrentMeasure> ;
        schema:domainIncludes  <https://w3id.org/product/ElectricFlowStorageDevice> .

props:surfaceColor  a          owl:DatatypeProperty ;
        rdfs:comment           "La couleur de la surface"@fr-FR , "The color of the surface."@en , "表面の色を示す文字列情報。"@ja-JP ;
        rdfs:label             "Oberflächenfarbe"@de-DE , "表面色"@ja-JP , "Couleur surface"@fr-FR , "surfaceColor"@en ;
        rdfs:range             xsd:string ;
        schema:domainIncludes  <https://w3id.org/product/ShadingDevice> .

props:flowResistanceRange
        a                      owl:DatatypeProperty ;
        rdfs:comment           "Allowable range of frictional resistance against which the fluid is being pumped."@en , "流体をポンプでくみ上げる際の摩擦抵抗の許容範囲"@ja-JP ;
        rdfs:label             "flowResistanceRange"@en , "流体抵抗の範囲"@ja-JP ;
        schema:domainIncludes  <https://w3id.org/product/Pump> .

props:pictogramEscapeDirection
        a                      owl:DatatypeProperty ;
        rdfs:comment           "The direction of escape pictogram."@en , "避難標識の向き。"@ja-JP , "피난 표지판 방향"@ko-KR ;
        rdfs:label             "pictogramEscapeDirection"@en , "避難標識の向き"@ja-JP , "피난 표지판 방향"@ko-KR ;
        schema:domainIncludes  <https://w3id.org/product/LightFixture%2FSECURITYLIGHTING> .

props:iCW60947  a              owl:DatatypeProperty ;
        rdfs:comment           "IEC60947シリーズに基づいてテストした配線遮断機またはモータ保護装置のための電流[A]に耐える温度。\n 値は、1sで与えられる。"@ja-JP , "IEC60947 시리즈를 기반으로 테스트 배선 차단기 또는 모터 보호 장치를위한 전류 [A]에 견디는 온도  값은 1s 주어진다."@ko-KR , "The thermal withstand current in [A] for a circuit breaker or motor protection device tested in accordance with the IEC 60947 series. The value shall be related to 1 s."@en ;
        rdfs:label             "iCW60947"@en , "ICW60947"@ja-JP , "ICW60947"@ko-KR ;
        rdfs:range             <https://w3id.org/product/ElectricCurrentMeasure> ;
        schema:domainIncludes  <https://w3id.org/product/ProtectiveDevice> , <https://w3id.org/product/ProtectiveDevice%2FCIRCUITBREAKER> .

props:requestSourceLabel
        a                      owl:DatatypeProperty ;
        rdfs:comment           "A specific name or label that further qualifies the identity of a request source. In the event of an email, this may be the email address."@en , "要請がなされる源のあらかじめ定義されたタイプの識別子。"@ja-JP ;
        rdfs:label             "requestSourceLabel"@en , "要請ソースタイプ"@ja-JP ;
        rdfs:range             xsd:string ;
        schema:domainIncludes  <https://w3id.org/product/ActionRequest> .

props:ambientDesignWetBulbTemperature
        a                      owl:DatatypeProperty ;
        rdfs:comment           "Ambient design wet bulb temperature used for selecting the cooling tower."@en ;
        rdfs:label             "ambientDesignWetBulbTemperature"@en ;
        rdfs:range             <https://w3id.org/product/ThermodynamicTemperatureMeasure> ;
        schema:domainIncludes  <https://w3id.org/product/CoolingTower> .

props:compressorSpeed
        a                      owl:DatatypeProperty ;
        rdfs:comment           "Compressor speed."@en , "Vitesse du compresseur"@fr-FR ;
        rdfs:label             "compressorSpeed"@en , "VitesseCompresseur"@fr-FR ;
        rdfs:range             <https://w3id.org/product/RotationalFrequencyMeasure> ;
        schema:domainIncludes  <https://w3id.org/product/Compressor> .

props:basinReserveVolume
        a                      owl:DatatypeProperty ;
        rdfs:comment           "Volume between operating and overflow levels in cooling tower basin."@en ;
        rdfs:label             "basinReserveVolume"@en ;
        rdfs:range             <https://w3id.org/product/VolumeMeasure> ;
        schema:domainIncludes  <https://w3id.org/product/CoolingTower> .

props:neckArea  a              owl:DatatypeProperty ;
        rdfs:comment           "Neck area of the air terminal."@en , "ターミナルのネック面積"@ja-JP , "Partie la plus étroite du terminal de ventilation."@fr-FR ;
        rdfs:label             "neckArea"@en , "ネック面積"@ja-JP , "ZoneReduction"@fr-FR ;
        rdfs:range             <https://w3id.org/product/AreaMeasure> ;
        schema:domainIncludes  <https://w3id.org/product/AirTerminal> .

props:inLineRowSpacing
        a                      owl:DatatypeProperty ;
        rdfs:comment           "In-line tube row spacing."@en , "インラインチューブ列間隔"@ja-JP ;
        rdfs:label             "inLineRowSpacing"@en , "インライン列間隔"@ja-JP ;
        rdfs:range             <https://w3id.org/product/PositiveLengthMeasure> ;
        schema:domainIncludes  <https://w3id.org/product/TubeBundle> .

props:shaftPowerRate  a        owl:DatatypeProperty ;
        rdfs:comment           "Fan shaft power."@en , "ファン軸動力"@ja-JP ;
        rdfs:label             "shaftPowerRate"@en , "軸動力量"@ja-JP ;
        schema:domainIncludes  <https://w3id.org/product/Fan> .

props:pressureRegulatorSetting
        a                      owl:DatatypeProperty ;
        rdfs:comment           "Pressure that is automatically maintained in the tank."@en , "タンク内で自動的に維持される圧力"@ja-JP ;
        rdfs:label             "pressureRegulatorSetting"@en , "圧力調整設定"@ja-JP ;
        rdfs:range             <https://w3id.org/product/PressureMeasure> ;
        schema:domainIncludes  <https://w3id.org/product/Tank%2FPRESSUREVESSEL> , <https://w3id.org/product/Tank%2FEXPANSION> .

props:flangeBaseFillet
        a                      owl:DatatypeProperty ;
        rdfs:comment           "Flange base fillet of the profile."@en ;
        rdfs:label             "flangeBaseFillet"@en ;
        rdfs:range             <https://w3id.org/product/NonNegativeLengthMeasure> ;
        schema:domainIncludes  <https://w3id.org/product/ArbitraryClosedProfileDef> .

props:arrangement  a           owl:DatatypeProperty ;
        rdfs:comment           "Defines the basic flow arrangements for the heat exchanger:\n\nCOUNTERFLOW: Counterflow heat exchanger arrangement. \nCROSSFLOW: Crossflow heat exchanger arrangement. \nPARALLELFLOW: Parallel flow heat exchanger arrangement. \nMULTIPASS: Multipass flow heat exchanger arrangement. \nOTHER: Other type of heat exchanger flow arrangement not defined above."@en , "熱交換器の流れの基本的配置(カウンターフロー、クロスフロー。パラレルフロー、マルチパス、その他)"@ja-JP , "Defines the fan and motor drive arrangement as defined by AMCA.\n\nARRANGEMENT1: Arrangement 1. \nARRANGEMENT2: Arrangement 2. \nARRANGEMENT3: Arrangement 3. \nARRANGEMENT4: Arrangement 4. \nARRANGEMENT7: Arrangement 7. \nARRANGEMENT8: Arrangement 8. \nARRANGEMENT9: Arrangement 9. \nARRANGEMENT10: Arrangement 10. \nOTHER: Other type of fan drive arrangement."@en , "ファンとモーターの配置（AMCAによる定義）\nARRANGEMENT1, ARRANGEMENT2, ARRANGEMENT3, ARRANGEMENT4, ARRANGEMENT7, ARRANGEMENT8, ARRANGEMENT9, ARRANGEMENT10, OTHER, NOTKNOWN, UNSET"@ja-JP ;
        rdfs:label             "arrangement"@en , "配置"@ja-JP ;
        schema:domainIncludes  <https://w3id.org/product/HeatExchanger> , <https://w3id.org/product/Fan%2FCENTRIFUGAL> .

props:anchorBoltLength
        a                      owl:DatatypeProperty ;
        rdfs:comment           "The length of the anchor bolt."@en , "アンカーボルトの長さ。"@ja-JP , "앵커 볼트의 길이"@ko-KR ;
        rdfs:label             "anchorBoltLength"@en , "長さ"@ja-JP , "길이"@ko-KR ;
        rdfs:range             <https://w3id.org/product/PositiveLengthMeasure> ;
        schema:domainIncludes  <https://w3id.org/product/MechanicalFastener%2FANCHORBOLT> .

props:shortTimeCurrentSetValue
        a                      owl:DatatypeProperty ;
        rdfs:comment           "Short time current set value. The set value of the long time tripping current if adjustable."@en ;
        rdfs:label             "shortTimeCurrentSetValue"@en ;
        rdfs:range             <https://w3id.org/product/ElectricCurrentMeasure> ;
        schema:domainIncludes  <https://w3id.org/product/ProtectiveDevice> .

props:protocols  a             owl:DatatypeProperty ;
        rdfs:comment           "For data ports, identifies the protocols used as defined by the Open System Interconnection (OSI) Basic Reference Model (ISO 7498).  Layers include: 1. Physical; 2. DataLink; 3. Network; 4. Transport; 5. Session; 6. Presentation; 7. Application.  Example: 3:IP, 4:TCP, 5:HTTP"@en , "OSIのオープンシステム相互接続用基本プロトコル(ISO 7498)：\n1. 物理層; 2.データリンク層; 3. ネットワーク層; 4. トランスポート層; 5. セッション層; 6.プレゼンテーション層 ; 7. アプリケーション層. \n例: 3:IP, 4:TCP, 5:HTTP"@ja ;
        rdfs:label             "protocols"@en , "プロトコル"@ja ;
        schema:domainIncludes  <https://w3id.org/product/DistributionPort%2FELECTRICAL> .

props:flowCondition  a         owl:DatatypeProperty ;
        rdfs:comment           "断面の充満率で流動状態を定義する。"@ja-JP , "Defines the flow condition as a percentage of the cross-sectional area."@en ;
        rdfs:label             "流動状態"@ja-JP , "flowCondition"@en ;
        schema:domainIncludes  <https://w3id.org/product/DistributionPort%2FCHEMICAL> , <https://w3id.org/product/DistributionPort%2FAIRCONDITIONING> .

props:edgeFixingPlateLength
        a                      owl:DatatypeProperty ;
        rdfs:comment           "The length of the L-shaped edge plate."@en , "L型端部プレートの長さ。"@ja-JP , "L 형 단부 플레이트의 길이"@ko-KR ;
        rdfs:label             "edgeFixingPlateLength"@en , "長さ"@ja-JP , "길이"@ko-KR ;
        rdfs:range             <https://w3id.org/product/PositiveLengthMeasure> ;
        schema:domainIncludes  <https://w3id.org/product/DiscreteAccessory%2FEdge%20fixing%20plate> .

props:interiorHeatTransferCoefficient
        a                      owl:DatatypeProperty ;
        rdfs:comment           "内面に関連づけられた内面熱交換係数"@ja-JP , "Interior heat transfer coefficient associated with interior surface area."@en ;
        rdfs:label             "内面熱交換係数"@ja-JP , "interiorHeatTransferCoefficient"@en ;
        schema:domainIncludes  <https://w3id.org/product/Evaporator> , <https://w3id.org/product/Condenser> .

props:separationType  a        owl:DatatypeProperty ;
        rdfs:comment           "Air particulate filter media separation type."@en ;
        rdfs:label             "separationType"@en ;
        schema:domainIncludes  <https://w3id.org/product/Filter%2FAIRPARTICLEFILTER> .

props:totalCoolingCapacity
        a                      owl:DatatypeProperty ;
        rdfs:comment           "Total cooling capacity. This includes cooling capacity of beam and cooling capacity of supply air."@en ;
        rdfs:label             "totalCoolingCapacity"@en ;
        schema:domainIncludes  <https://w3id.org/product/CooledBeam> .

props:accessType  a            owl:DatatypeProperty ;
        rdfs:comment           "Defines the types of access (or cover) to a tank that may be specified.\n\nNote that covers are generally specified for rectangular tanks. For cylindrical tanks, access will normally be via a manhole."@en , "タンクの点検口（又はカバー)のタイプの定義は明示される。カバーは一般的に矩形タンクについて明示されていることに注意。円筒形タンクの点検は通常のマンホールを通る"@ja-JP ;
        rdfs:label             "accessType"@en , "点検タイプ"@ja-JP ;
        schema:domainIncludes  <https://w3id.org/product/Tank> .

props:groundFaulti2tFunction
        a                      owl:DatatypeProperty ;
        rdfs:comment           "Applying ground fault i2t function. A flag indicating that the I2t ground fault function of the device is used. The value should be set to TRUE only if the I2t function is explicitly selected for the device."@en ;
        rdfs:label             "groundFaulti2tFunction"@en ;
        rdfs:range             xsd:boolean ;
        schema:domainIncludes  <https://w3id.org/product/ProtectiveDevice> .

props:residualFlowingPressure
        a                      owl:DatatypeProperty ;
        rdfs:comment           "The residual flowing pressure in the pipeline at which the discharge flow rate is determined."@en , "吐出流量が確保される、パイプラインの流れ時残留圧力。"@ja-JP ;
        rdfs:label             "residualFlowingPressure"@en , "残留流動圧力"@ja-JP ;
        rdfs:range             <https://w3id.org/product/PressureMeasure> ;
        schema:domainIncludes  <https://w3id.org/product/FireSuppressionTerminal%2FSPRINKLER> .

props:ventilationAirFlowRate
        a                      owl:DatatypeProperty ;
        rdfs:comment           "Ventilation air flow rate in the space."@en , "室内の換気空気流量"@ja-JP ;
        rdfs:label             "ventilationAirFlowRate"@en , "換気気流速度"@ja-JP ;
        schema:domainIncludes  <https://w3id.org/product/Space> .

props:airConditioningCentral
        a                      owl:DatatypeProperty ;
        rdfs:comment           "Indique si l'espace requiert un conditionnement d'air centralisé (VRAI) ou non (FAUX). A fournir si la propriété \"Conditionnement d'air\" est VRAI."@fr-FR , "Anforderung, ob die Klimaanlage zentral gesteuert werden soll (WAHR), oder nicht (FALSCH). Soll nur angegeben werden, wenn die Eigenschaft \"Klimaanlage\" mit WAHR gegeben ist."@de-DE , "空間が中央式空調を要求するかどうかを示すブーリアン値。「空調」プロパティがTRUEに設定された場合のみ、与えられる。"@ja-JP , "Indication whether the space  requires a central air conditioning provided (TRUE) or not (FALSE).\nIt should only be given, if the property \"AirConditioning\" is set to TRUE."@en , "공간이 중앙 식 공조를 요청할지 여부를 나타내는 부울 값입니다. \"공조\"속성이 TRUE로 설정된 경우에만 주어진다."@ko-KR ;
        rdfs:label             "Klimaanlage zentral"@de-DE , "중앙식 에어컨"@ko-KR , "Conditionnement d'air centralisé"@fr-FR , "airConditioningCentral"@en , "中央式空調"@ja-JP ;
        rdfs:range             xsd:boolean ;
        schema:domainIncludes  <https://w3id.org/product/cSpatialZone> , <https://w3id.org/product/Space> , <https://w3id.org/product/cZone> .

props:nominalSupplyWaterTemperatureCooling
        a                      owl:DatatypeProperty ;
        rdfs:comment           "Nominal supply water temperature (refers to nominal cooling capacity)."@en ;
        rdfs:label             "nominalSupplyWaterTemperatureCooling"@en ;
        rdfs:range             <https://w3id.org/product/ThermodynamicTemperatureMeasure> ;
        schema:domainIncludes  <https://w3id.org/product/CooledBeam> .

props:refrigerantType
        a                      owl:DatatypeProperty ;
        rdfs:comment           "冷媒材質"@ja-JP , "Refrigerant material."@en , "Type de réfrigérant"@fr-FR ;
        rdfs:label             "冷媒種類"@ja-JP , "refrigerantType"@en , "TypeRéfrigérant"@fr-FR ;
        schema:domainIncludes  <https://w3id.org/product/Evaporator> , <https://w3id.org/product/Compressor> .

props:fixingSocketThreadLength
        a                      owl:DatatypeProperty ;
        rdfs:comment           "The length of the threaded part of the fixing socket."@en , "固定ソケットの全体長さねじ部の長さ。"@ja-JP , "고정 소켓의 전체 길이 나사부의 길이"@ko-KR ;
        rdfs:label             "fixingSocketThreadLength"@en , "ねじ部長さ"@ja-JP , "나사부 길이"@ko-KR ;
        rdfs:range             <https://w3id.org/product/PositiveLengthMeasure> ;
        schema:domainIncludes  <https://w3id.org/product/DiscreteAccessory%2FFixing%20socket> .

props:endDate  a               owl:DatatypeProperty ;
        rdfs:comment           "Date and time at which the permit ceases to be valid."@en ;
        rdfs:label             "endDate"@en ;
        rdfs:range             xsd:dateTime ;
        schema:domainIncludes  <https://w3id.org/product/Permit> .

props:latentHeatTransferRate
        a                      owl:DatatypeProperty ;
        rdfs:comment           "潜熱交換量"@ja-JP , "Puissance thermique latente"@fr-FR , "Latent heat transfer rate to primary air flow."@en , "Latent heat transfer rate."@en , "一次空気流の潜熱交換量"@ja-JP ;
        rdfs:label             "latentHeatTransferRate"@en , "潜熱交換量"@ja-JP , "PuissanceThermiqueLatente"@fr-FR ;
        schema:domainIncludes  <https://w3id.org/product/AirToAirHeatRecovery> , <https://w3id.org/product/EvaporativeCooler> .

props:earthFault1PoleMinimumState
        a                      owl:DatatypeProperty ;
        rdfs:comment           "Minimum 1 pole earth fault current provided at the point of supply i.e. the fault between 1 phase and PE/PEN."@en , "電源供給時点の点1相とPE/PEN間の1極最小地絡電流。"@ja-JP , "전원 공급 시점 점 1 상 및 PE / PEN 사이의 1 극 최소 지락 전류"@ko-KR ;
        rdfs:label             "earthFault1PoleMinimumState"@en , "1極最小地絡電流"@ja-JP , "1 극 최소 지락 전류"@ko-KR ;
        rdfs:range             <https://w3id.org/product/ElectricCurrentMeasure> ;
        schema:domainIncludes  <https://w3id.org/product/ElectricFlowStorageDevice> .

props:surfaceTemperature
        a                      owl:DatatypeProperty ;
        rdfs:comment           "Average surface temperature of the component."@en , "構成要素の平均表面温度"@ja-JP ;
        rdfs:label             "surfaceTemperature"@en , "表面温度"@ja-JP ;
        schema:domainIncludes  <https://w3id.org/product/SpaceHeater> .

props:nominalFrequencyRange
        a                      owl:DatatypeProperty ;
        rdfs:comment           "The upper and lower limits of frequency for which the operation of the device is certified."@en ;
        rdfs:label             "nominalFrequencyRange"@en ;
        schema:domainIncludes  <https://w3id.org/product/DistributionElement> .

props:nominalMoistureGain
        a                      owl:DatatypeProperty ;
        rdfs:comment           "Nominal rate of water vapor added into the airstream."@en , "気流に加わった水蒸気の平均量"@ja-JP ;
        rdfs:label             "nominalMoistureGain"@en , "加湿量の平均"@ja-JP ;
        rdfs:range             <https://w3id.org/product/MassFlowRateMeasure> ;
        schema:domainIncludes  <https://w3id.org/product/Humidifier> .

props:gradient  a              owl:DatatypeProperty ;
        rdfs:comment           "The gradient of the pipe segment."@en , "配管部の勾配"@ja-JP ;
        rdfs:label             "gradient"@en , "勾配"@ja-JP ;
        rdfs:range             <https://w3id.org/product/PositiveRatioMeasure> ;
        schema:domainIncludes  <https://w3id.org/product/PipeSegment> .

props:isSwitch  a              owl:DatatypeProperty ;
        rdfs:comment           "Identifies if the sensor also functions as a switch at the set point (=TRUE) or not (= FALSE)."@en , "センサーが設定値でスイッチとして機能する（TRUE)か、否か（FALSE)を識別する。"@ja-JP , "센서 설정에서 스위치 역할 (TRUE) 또는 여부 (FALSE)를 확인한다."@ko-KR ;
        rdfs:label             "isSwitch"@en , "スイッチ機能の有無"@ja-JP , "스위치 기능의 유무"@ko-KR ;
        rdfs:range             xsd:boolean ;
        schema:domainIncludes  <https://w3id.org/product/Sensor%2FPRESSURESENSOR> .

props:oldDevice  a             owl:DatatypeProperty ;
        rdfs:comment           "Indication whether the protection_ unit is out-dated or not. If not out-dated, the device is still for sale."@en , "基準に適合されていて販売されているかどうか。"@ja-JP , "기준에 적합하여 판매하는지에 대한 여부"@ko-KR ;
        rdfs:label             "oldDevice"@en , "販売中止装置"@ja-JP , "판매중지 장치"@ko-KR ;
        rdfs:range             xsd:boolean ;
        schema:domainIncludes  <https://w3id.org/product/ProtectiveDeviceTrippingUnit> .

props:setPoint  a              owl:DatatypeProperty ;
        rdfs:comment           "Indicates the temperature setpoint.  For thermostats with setbacks or separate high and low setpoints, then the time series may contain a pair of values at each entry where the first value is the heating setpoint (low) and the second value is the cooling setpoint (high)."@en , "Indicates the setpoint and label.  For toggle switches, there are two positions, 0 for off and 1 for on.  For dimmer switches, the values may indicate the fully-off and full-on positions, where missing integer values in between are interpolated.   For selector switches, the range indicates the available positions.  \nAn IfcTable may be attached (using IfcMetric and IfcPropertyConstraintRelationship) containing columns of the specified header names and types:\n'Position' (IfcInteger): The discrete setpoint level.\n'Sink' (IfcLabel): The Name of the switched input port (IfcDistributionPort with FlowDirection=SINK).\n'Source' (IfcLabel): The Name of the switched output port (IfcDistributionPort with FlowDirection=SOURCE).\n'Ratio' (IfcNormalizedRatioMeasure): The ratio of power at the setpoint where 0.0 is off and 1.0 is fully on."@en , "입력 포트 이름 (IfcDistributionPort 및 FlowDirection = SINK), Maps SetPoint 위치. 회로가 어떤 경로를 추적할지를 나타낸다."@ko-KR , "Indicates the switch position over time according to Pset_SwitchingDeviceTypeCommon.SetPoint."@en , "設定ポイントと範囲を示す。トグルスイッチは2つのポジションがある：0 は オフ(OFF)、1 は オン(ON)。ディマースイッチは、全閉(fully-off) または　全開(fully-on) の他に、その間で取得可能な値をオプションで示す。選択型スイッチは選択可能なポジションの範囲を示す。"@ja-JP ;
        rdfs:label             "設定ポイント"@ja-JP , "setPoint"@en , "스위치 포트 싱크"@ko-KR ;
        schema:domainIncludes  <https://w3id.org/product/UnitaryControlElement> , <https://w3id.org/product/SwitchingDevice> .

props:electricMotorEfficiency
        a                      owl:DatatypeProperty ;
        rdfs:comment           "The ratio of output capacity to intake capacity."@en , "出力容量と入力容量の比率。"@ja-JP , "출력 용량을 입력 용량의 비율."@ko-KR ;
        rdfs:label             "electricMotorEfficiency"@en , "出力効率"@ja-JP , "출력 효율"@ko-KR ;
        rdfs:range             <https://w3id.org/product/PositiveRatioMeasure> ;
        schema:domainIncludes  <https://w3id.org/product/ElectricMotor> .

props:totalPrimaryEnergyConsumptionPerUnit
        a                      owl:DatatypeProperty ;
        rdfs:comment           "Consommation d'énergie primaire utilisée, telle que définie dans la norme ISO21930:2007 [NDT : et dans la norme NF P01-010]"@fr-FR , "ISO21930 : 2007에서 정의된 에너지 사용량"@ko-KR , "Quantity of energy used as defined in ISO21930:2007."@en , "ISO21930:2007で定義されたエネルギー消費量。"@ja-JP ;
        rdfs:label             "ConsommationTotaleEnergiePrimaireParUnite"@fr-FR , "totalPrimaryEnergyConsumptionPerUnit"@en , "단위당 모든 차 에너지 소비"@ko-KR , "単位あたり全一次エネルギ消費"@ja-JP ;
        rdfs:range             <https://w3id.org/product/EnergyMeasure> ;
        schema:domainIncludes  <https://w3id.org/product/Element> .

props:heatOutputRate  a        owl:DatatypeProperty ;
        rdfs:comment           "Overall heat transfer rate."@en , "総合熱移動率"@ja-JP ;
        rdfs:label             "heatOutputRate"@en , "熱出力比"@ja-JP ;
        schema:domainIncludes  <https://w3id.org/product/SpaceHeater> .

props:glassThickness3
        a                      owl:DatatypeProperty ;
        rdfs:comment           "3番目（外側）のガラスの厚み。"@ja-JP , "Thickness of the third (outer) glass layer."@en , "第三层（外侧）玻璃的厚度。"@zh-CN , "German-description-4"@de-DE , "Epaisseur de la troisième couche de verre (côté extérieur)"@fr-FR ;
        rdfs:label             "玻璃厚度3"@zh-CN , "glassThickness3"@en , "ガラス厚3"@ja-JP , "German-name-4"@de-DE , "EpaisseurVitrage3"@fr-FR ;
        rdfs:range             <https://w3id.org/product/PositiveLengthMeasure> ;
        schema:domainIncludes  <https://w3id.org/product/cWindow> , <https://w3id.org/product/Door> .

props:staggeredRowSpacing
        a                      owl:DatatypeProperty ;
        rdfs:comment           "Staggered tube row spacing."@en , "互い違いのチューブ列間隔"@ja-JP ;
        rdfs:label             "staggeredRowSpacing"@en , "互い違いの列間隔"@ja-JP ;
        rdfs:range             <https://w3id.org/product/PositiveLengthMeasure> ;
        schema:domainIncludes  <https://w3id.org/product/TubeBundle> .

props:reference  a             owl:DatatypeProperty ;
        rdfs:comment           "Reference ID for this specified type in this project"@en , "Référence à l'identifiant d'un type spécifié dans le contexte du projet (exemple : \"type A1\"). A fournir s'il n'y a pas de référence à une classification en usage."@fr-FR , "当プロジェクトにおけるこの指定型式のためのリファレンスID。（たとえは、'A-1'型)"@ja-JP , "Bezeichnung zur Zusammenfassung gleichartiger Komponenten zu einem Komponententyp (auch Konstruktionstyp genannt). Alternativ zum Namen des \"Typobjekts\", insbesondere wenn die Software keine Typen unterstützt."@de-DE , "使用される認識分類システムで分類基準がない場合、プロジェクトで指定された型（タイプ'Ａ-1'など）で提供されるレファレンスID。"@ja-JP , "Référence à l'identifiant d'un type spécifié dans le contexte du projet (exemple : \"type A1\") pour désigner un \"type de construction\". Une alternative au nom d'un objet type lorsque les objets types ne sont pas gérés par le logiciel."@fr-FR , "Reference ID for this specified type in this project (e.g. type 'A-1'). Used to store the non-classification driven internal construction type."@en , "参照するID番号。"@ja-JP , "프로젝트의 참조 ID (예 : A-1). 분류 코드가 아닌 내부에서 사용되는 프로젝트 형식으로 사용됩니다."@ko-KR , "このプロジェクトのための参照記号。"@ja-JP , "해당 프로젝트에서 사용이 유형에 대한 참조 ID (예 : 'A-1') ※ 기본이있는 경우 그 기호를 사용"@ko-KR , "当該プロジェクトで定義する形式の参照ID（例：A-1)、承認された分類に存在しないときに使用される。"@ja-JP , "空調システム、或いはサブシステムの参照ID（例えば、'WWS/VS1'はWWS系統のVSI/400サブ系統）。IDは当該地域技術基準より決められる。"@ja-JP , "Reference ID for this specific instance (e.g.  'WWS/VS1/400/001', which indicates the occurrence belongs to system WWS, subsystems VSI/400, and has the component number 001)."@en , "该项目中该类型构件的参考编号（例如，类型A-1）。"@zh-CN , "若未采用已知的分类系统，则该属性为该项目中该类型构件的参考编号（例如，类型A-1）。"@zh-CN , "Identifikator der projektinternen Referenz für dieses Grundstück, z.B. nach der Grundstückklassifizierung des Bauherrn. Wird verwendet, wenn keine allgemein anerkanntes Klassifizierungssystem angewandt wird."@de-DE , "Kennzeichen für diese bauliche System in dem Projekt (z.B. 'TRA/EL1'). Die Kennzeichensystematik hängt von den jeweiligen nationalen/regionalen Regelungen ab."@de-DE , "해당프로젝트에 정의도니 형식의 참조ID (예 : A-1) 승인된 분류에 존재하지 않을 때 사용된다."@ko-KR , "このプロジェクトにおける建物システムの指定されたインスタンスの参照記号"@ja-JP , "A descriptive label for the general reinforcement type."@en , "一般的な鉄筋タイプの説明ラベル。"@ja-JP , "一般的な鉄筋タイプの説明ラベル。\n（例えば、壁の外側・内側で鉄筋間隔が異なる場合に、\"Outside\",\"Inside\"を記述する）"@ja-JP , "해당 프로젝트에 정의된 형식의 참조 ID (예 : A-1) 승인된 분류에 존재하지 않을 때 사용된다. 참조"@ko-KR , "Bezeichnung zur Zusammenfassung gleichartiger Bauteile zu einem Bauteiltyp (auch Konstruktionstyp genannt). Alternativ zum Namen des \"Typobjekts\", insbesondere wenn die Software keine Typen unterstützt."@de-DE , "このプロジェクト (例． 'A-1'　タイプなど)で指定された参照ID。認められた分類体系の分類参照が存在しない場合に適用される。"@ja-JP , "이 프로젝트 (예 : 'A-1'유형 등) 지정된 참조 ID. 인정 분류 체계의 분류 참조가없는 경우에 적용된다."@ko-KR , "Wird verwendet, wenn keine allgemein anerkanntes Klassifizierungssystem angewandt wird."@de-DE , "認識された分類体系で参照する分類がない場合にこのプロジェクト固有の参照記号（例：タイプ'A-1'）が与えられる。"@ja-JP , "Reference ID for this specific instance of a distribution system, or sub-system (e.g. 'WWS/VS1', which indicates the system to be WWS, subsystems VSI/400). The reference values depend on the local code of practice."@en , "Reference ID for this specified type in this project (e.g. type 'A-1'). Used to store the non-classification driven internal project type."@en , "具体的な参照ID（例えば、“WWS/VS1/400/001”はWWS系統、VS1/400サブシステム001番部品）。"@ja-JP , "このプロジェクトにおける参照記号(例：A-1)"@ja-JP , "Référence à l'identifiant d'un type spécifié dans le contexte de ce projet."@fr-FR , "この規格(例、Ａ－1)で特定のタイプの参照ＩＤが割り当てられ、等級がなければ等級システムを使って割り当てられます。"@ja-JP , "Bezeichnung zur Zusammenfassung gleichartiger Räume zu einem Raumtyp (auch Funktionstyp genannt). Alternativ zum Namen des \"Typobjekts\", insbesondere wenn die Software keine Raumtypen als Typobjekte unterstützt."@de-DE , "Reference ID for this specified type in this project (e.g. type 'A-1')."@en , "Reference ID for this specified instance of building system in this project (e.g. 'TRA/EL1'), The reference values depend on the local code of practice."@en , "Identifikator der projektinternen Referenz für dieses Geschoss, z.B. nach der Geschossklassifizierung des Bauherrn. Wird verwendet, wenn keine allgemein anerkanntes Klassifizierungssystem angewandt wird."@de-DE , "프로젝트 (예 : 'A-1'유형 등) 지정된 참조 ID. 인정 분류 체계의 분류 참조가없는 경우에 적용된다."@ko-KR , "このプロジェクトにおける参照記号(例：A-1)。分類コードではなく内部で使用されるプロジェクトタイプとして使用されるもの。"@ja-JP , "一般的な鉄筋タイプの説明ラベル。\n（例えば、梁の両端・中央で肋筋や巾止筋の間隔が異なる場合に、\"Start\",\"Center\",\"End\"を記述する）"@ja-JP , "参照記号でプロジェクトでのタイプとして使用されるもの。"@ja-JP , "해당 프로젝트에 정의된 형식의 참조 ID (예 : A-1) 승인된 분류에 존재하지 않을 때 사용된다."@ko-KR , "Reference ID for this specified type in this project (e.g. type 'A-1'), Also referred to as \"construction type\". It should be provided as an alternative to the name of the \"object type\", if the software does not support object types."@en , "Identification de référence pour ce type spécifique à ce projet, c'est-à-dire type'A-1', fourni à partir du moment où, s'il n'y a pas de référence de classification par rapport à un système de classification reconnu et en usage."@fr-FR , "Identifikator der projektinternen Referenz für dieses Gebäude, z.B. nach der Gebäudelassifizierung des Bauherrn. Wird verwendet, wenn keine allgemein anerkanntes Klassifizierungssystem angewandt wird."@de-DE , "이 프로젝트에서 여기에 특정한 형식에 대한 참조 ID"@ko-KR , "공조 시스템 혹은 서브 시스템의 참조 ID (예 : 'WWS/VS1'는 WWS 계통의 VSI/400 하위 계통). ID는 해당 지역 기술 기준보다 결정된다."@ko-KR , "해당 프로젝트에 정의된 형식의 참조 ID (예 : A-1) 승인된 분류에 존재하지 않을 때 사용된다"@ko-KR , "Reference ID for this specified type in this project (e.g. type 'A-1'), provided, if there is no classification reference to a recognized classification system used."@en , "구체적인 참조 ID (예 : \"WWS/VS1/400/001\"는 WWS 계통, VS1/400 서브 시스템 001 번 부품)"@ko-KR , "이 프로젝트의 참조 ID (예 : A-1). 분류 코드가 아닌 내부에서 사용되는 프로젝트 형식으로 사용됩니다."@ko-KR , "该项目中该特定建筑系统实例的参考编号（例如，“TRA/EL1”）。该属性值由当地编码规范决定。"@zh-CN , "Bemusterungstyp, wird als Attribute angegeben, wenn keine allgemein anerkanntes Klassifizierungssystem angewandt wird."@de-DE , "Référence à l'identifiant d'un type spécifié dans le contexte du projet (exemple : \"type A1\"). Utilisé pour enregistrer un type sans recourir à une classification."@fr-FR , "Référence à l'identifiant d'un type spécifié dans le contexte de ce projet (exemple : \"type A1\"). A fournir s'il n'y a pas de référence à une classification en usage."@fr-FR , "一般的な鉄筋タイプの説明ラベル。\n（例えば、柱の柱頭・柱脚で帯筋や巾止筋の間隔・本数が異なる場合に、\"Top\",\"Bottom\"を記述する）"@ja-JP ;
        rdfs:label             "참조 ID"@ko-KR , "Référence"@fr-FR , "Referenz ID"@de-DE , "参照記号"@ja-JP , "참조 기호"@ko-KR , "참조기호"@ko-KR , "Reference"@fr-FR , "Bemusterungstyp"@de-DE , "reference"@en , "参考号"@zh-CN , "참조"@ko-KR , "Raumtyp"@de-DE , "Kennzeichen"@de-DE , "참조ID"@ko-KR , "Komponententyp"@de-DE , "参照"@ja-JP , "Bauteiltyp"@de-DE ;
        rdfs:range             xsd:string ;
        schema:domainIncludes  <https://w3id.org/product/ElectricGenerator> , <https://w3id.org/product/Element> , <https://w3id.org/product/FlowInstrument> , <https://w3id.org/product/ProtectiveDeviceTrippingUnit> , <https://w3id.org/product/Space> , <https://w3id.org/product/FireSuppressionTerminal> , <https://w3id.org/product/CableCarrierSegment> , <https://w3id.org/product/AirTerminalBox> , <https://w3id.org/product/CableSegment> , <https://w3id.org/product/BuildingStorey> , <https://w3id.org/product/CooledBeam> , <https://w3id.org/product/Engine> , <https://w3id.org/product/LightFixture> , <https://w3id.org/product/AudioVisualAppliance> , <https://w3id.org/product/SanitaryTerminal> , <https://w3id.org/product/ElectricMotor> , <https://w3id.org/product/WasteTerminal> , <https://w3id.org/product/DuctSegment> , <https://w3id.org/product/AirTerminal> , <https://w3id.org/product/Humidifier> , <https://w3id.org/product/Outlet> , <https://w3id.org/product/CableFitting> , <https://w3id.org/product/Stair> , <https://w3id.org/product/Covering> , <https://w3id.org/product/UnitaryControlElement> , <https://w3id.org/product/CoolingTower> , <https://w3id.org/product/Footing> , <https://w3id.org/product/CableCarrierFitting> , <https://w3id.org/product/TubeBundle> , <https://w3id.org/product/ProtectiveDevice> , <https://w3id.org/product/PipeFitting> , <https://w3id.org/product/Building> , <https://w3id.org/product/AirToAirHeatRecovery> , <https://w3id.org/product/Column> , <https://w3id.org/product/Pump> , <https://w3id.org/product/Site> , <https://w3id.org/product/OpeningElement> , <https://w3id.org/product/Ramp> , <https://w3id.org/product/Beam> , <https://w3id.org/product/SolarDevice> , <https://w3id.org/product/Railing> , <https://w3id.org/product/Transformer> , <https://w3id.org/product/Boiler> , <https://w3id.org/product/ElectricAppliance> , <https://w3id.org/product/ElectricDistributionBoard> , <https://w3id.org/product/StackTerminal> , <https://w3id.org/product/Door> , <https://w3id.org/product/ElectricTimeControl> , <https://w3id.org/product/Evaporator> , <https://w3id.org/product/Window> , <https://w3id.org/product/Chiller> , <https://w3id.org/product/ShadingDevice> , <https://w3id.org/product/FlowMeter> , <https://w3id.org/product/DistributionChamberElement> , <https://w3id.org/product/Coil> , <https://w3id.org/product/SpaceHeater> , <https://w3id.org/product/Chimney> , <https://w3id.org/product/Zone> , <https://w3id.org/product/Interceptor> , <https://w3id.org/product/UnitaryEquipment> , <https://w3id.org/product/MedicalDevice> , <https://w3id.org/product/Lamp> , <https://w3id.org/product/StairFlight> , <https://w3id.org/product/Roof> , <https://w3id.org/product/CurtainWall> , <https://w3id.org/product/CommunicationsAppliance> , <https://w3id.org/product/Sensor> , <https://w3id.org/product/BuildingElementProxy> , <https://w3id.org/product/Fan> , <https://w3id.org/product/Alarm> , <https://w3id.org/product/Member> , <https://w3id.org/product/Damper> , <https://w3id.org/product/Filter> , <https://w3id.org/product/ElementComponent> , <https://w3id.org/product/Condenser> , <https://w3id.org/product/DuctSilencer> , <https://w3id.org/product/BuildingSystem> , <https://w3id.org/product/DuctFitting> , <https://w3id.org/product/JunctionBox> , <https://w3id.org/product/Burner> , <https://w3id.org/product/SwitchingDevice> , <https://w3id.org/product/ElectricFlowStorageDevice> , <https://w3id.org/product/Pile> , <https://w3id.org/product/Compressor> , <https://w3id.org/product/MotorConnection> , <https://w3id.org/product/DistributionSystem> , <https://w3id.org/product/Valve> , <https://w3id.org/product/Tank> , <https://w3id.org/product/VibrationIsolator> , <https://w3id.org/product/TransportElement> , <https://w3id.org/product/Plate> , <https://w3id.org/product/RampFlight> , <https://w3id.org/product/Wall> , <https://w3id.org/product/PipeSegment> , <https://w3id.org/product/EvaporativeCooler> , <https://w3id.org/product/Controller> , <https://w3id.org/product/Slab> , <https://w3id.org/product/HeatExchanger> , <https://w3id.org/product/Actuator> .

props:outerDiameter  a         owl:DatatypeProperty ;
        rdfs:comment           "配管の実外径(リストの複数の数字の解釈については呼び径参照)"@ja-JP , "The actual outer diameter of the pipe."@en , "配管の実外径。"@ja-JP ;
        rdfs:label             "outerDiameter"@en , "外径"@ja-JP ;
        rdfs:range             <https://w3id.org/product/PositiveLengthMeasure> ;
        schema:domainIncludes  <https://w3id.org/product/PipeSegment> , <https://w3id.org/product/DistributionPort%2FCHEMICAL> .

props:rateOfTemperatureRise
        a                      owl:DatatypeProperty ;
        rdfs:comment           "The rate of temperature rise that is to be sensed as being hazardous."@en , "危険であるとして感じられることになっている温度上昇率。"@ja-JP , "위험 것으로 느껴지게하는 온도 상승률."@ko-KR ;
        rdfs:label             "rateOfTemperatureRise"@en , "温度上昇率"@ja-JP , "온도 상승률"@ko-KR ;
        rdfs:range             <https://w3id.org/product/TemperatureRateOfChangeMeasure> ;
        schema:domainIncludes  <https://w3id.org/product/Sensor%2FHEATSENSOR> .

props:workStartTime  a         owl:DatatypeProperty ;
        rdfs:comment           "The default time of day a task is scheduled to start. For presentation purposes, if the start time of a task matches the WorkStartTime, then applications may choose to display the date only. Conversely when entering dates without specifying time, applications may automatically append the WorkStartTime."@en , "仕事開始予定のデフォルト時刻。プレゼンテーション目的のために、仕事の開始時間がWorkStartTimeと一致するならば、アプリケーションは日付だけを表示するほうを選ぶことが出来る。逆に、時間を指定することなく日付を入力した際、アプリケーションはWorkStartTimeを自動的に追加することが出来る。"@ja-JP ;
        rdfs:label             "workStartTime"@en , "作業開始時間"@ja-JP ;
        rdfs:range             xsd:time ;
        schema:domainIncludes  <https://w3id.org/product/WorkControl> .

props:usePurpose  a            owl:DatatypeProperty ;
        rdfs:comment           "The principal purpose for which the work surface is intended to be used e.g. writing/reading, computer, meeting, printer, reference files, etc."@en ;
        rdfs:label             "usePurpose"@en ;
        rdfs:range             xsd:string ;
        schema:domainIncludes  <https://w3id.org/product/SystemFurnitureElement%2FWORKSURFACE> .

props:sprayType  a             owl:DatatypeProperty ;
        rdfs:comment           "SprayFilled: Water is sprayed into airflow.\nSplashTypeFill: water cascades over successive rows of splash bars.\nFilmTypeFill: water flows in a thin layer over closely spaced sheets."@en ;
        rdfs:label             "sprayType"@en ;
        schema:domainIncludes  <https://w3id.org/product/CoolingTower> .

props:switchFunction  a        owl:DatatypeProperty ;
        rdfs:comment           "Indicates types of switches which differs in functionality."@en , "機能ごとに異なるスイッチのタイプを示す"@ja-JP , "기능마다 다른 스위치 타입을 나타낸다."@ko-KR ;
        rdfs:label             "switchFunction"@en , "スイッチタイプ"@ja-JP , "스위치 유형"@ko-KR ;
        schema:domainIncludes  <https://w3id.org/product/SwitchingDevice> .

props:mechanicalVentilationRate
        a                      owl:DatatypeProperty ;
        rdfs:comment           "Geforderte Luftwechselzahl (in Wechsel per Stunde) im Fall der künstlichen Lüftung."@de-DE , "特定の機械換気率の要求指標。1時間あたりの換気回数で与えられる。"@ja-JP , "Spécification du taux de ventilation mécanique exprimé en volumes par heure."@fr-FR , "Indication of the requirement of a particular mechanical air ventilation rate, given in air changes per hour."@en , "특정 기계 환기 비율 요구 지표. 시간 당 환기 회수로 주어진다."@ko-KR ;
        rdfs:label             "Taux ventilation mécanique"@fr-FR , "mechanicalVentilationRate"@en , "기계환기 비율"@ko-KR , "機械換気率"@ja-JP , "Künstliche Luftwechselzahl"@de-DE ;
        rdfs:range             <https://w3id.org/product/CountMeasure> ;
        schema:domainIncludes  <https://w3id.org/product/cSpatialZone> , <https://w3id.org/product/Space> , <https://w3id.org/product/cZone> .

props:solarReflectance
        a                      owl:DatatypeProperty ;
        rdfs:comment           "(Rsol)：日除けシステムにより反射される日射の率。注： Asol + Rsol + Tsol = 1　という方程式が成り立つ。"@ja-JP , "German-description-14"@de-DE , "(Rsol). Ratio du rayonnement solaire incident qui est réfléchi par le vitrage. Noter l'équation suivante : Asol + Rsol + Tsol = 1."@fr-FR , "(Rsol): The ratio of incident solar radiation that is reflected by a glazing system (also named ρe). Note the following equation Asol + Rsol + Tsol = 1"@en , "(Rsol): The ratio of incident solar radiation that is reflected by a shading system (also named ρe). Note the following equation Asol + Rsol + Tsol = 1"@en , "（Rsol）ガラスで反射する日射の比率（ρeとも表わされる）。以下の方程式に注意。Asol + Rsol + Tsol = 1"@ja-JP , "（Rsol）被玻璃系统反射的太阳入射辐射的比率（也可用ρe表示）。注：以下等式成立Asol + Rsol + Tsol = 1"@zh-CN , "(Rsol). Ratio du rayonnement solaire incident qui est réfléchi par la protection solaire. Noter l'équation suivante : Asol + Rsol + Tsol = 1."@fr-FR ;
        rdfs:label             "solarReflectance"@en , "太阳能反射率"@zh-CN , "Reflexion du rayonnement solaire"@fr-FR , "ReflexionRayonnementSolaire"@fr-FR , "日射反射率"@ja-JP , "Strahlungsreflectionsgrad"@de-DE ;
        rdfs:range             <https://w3id.org/product/NormalisedRatioMeasure> , <https://w3id.org/product/PositiveRatioMeasure> ;
        schema:domainIncludes  <https://w3id.org/product/Door> , <https://w3id.org/product/cWindow> , <https://w3id.org/product/ShadingDevice> .

props:minimumPartLoadRatio
        a                      owl:DatatypeProperty ;
        rdfs:comment           "Minimum part load ratio as a fraction of nominal capacity."@en , "Coefficient minimum de charge partielle en tant que fraction de la puissance nominale."@fr-FR ;
        rdfs:label             "minimumPartLoadRatio"@en , "CoefficientMinimalChargePartielle"@fr-FR ;
        rdfs:range             <https://w3id.org/product/PositiveRatioMeasure> ;
        schema:domainIncludes  <https://w3id.org/product/Compressor> .

props:tenureModesAvailableFuture
        a                      owl:DatatypeProperty ;
        rdfs:comment           "A list of the tenure modes that are expected to be available in the future expressed in terms of IfcLabel."@en , "Liste des possibilités d'occupation futures."@fr-FR ;
        rdfs:label             "tenureModesAvailableFuture"@en , "PossibilitesOccupationFutures"@fr-FR ;
        schema:domainIncludes  <https://w3id.org/product/Building> .

props:outOfPlane  a            owl:DatatypeProperty ;
        rdfs:comment           "Mechanical properties with respect to out-of-plane load, i.e. for function as a plate; tension zone of unbalanced layups is stressed in tension."@en , "Mechanical properties with respect to out-of-plane load, i.e. bending about the weak axis."@en ;
        rdfs:label             "outOfPlane"@en ;
        schema:domainIncludes  <https://w3id.org/product/Material%2FWood> .

props:temperatureSetPoint
        a                      owl:DatatypeProperty ;
        rdfs:comment           "The temperature setpoint range and default setpoint."@en ;
        rdfs:label             "temperatureSetPoint"@en ;
        schema:domainIncludes  <https://w3id.org/product/UnitaryControlElement%2FTHERMOSTAT> .

props:flangeDraft  a           owl:DatatypeProperty ;
        rdfs:comment           "Flange draft of the profile."@en ;
        rdfs:label             "flangeDraft"@en ;
        rdfs:range             <https://w3id.org/product/NonNegativeLengthMeasure> ;
        schema:domainIncludes  <https://w3id.org/product/ArbitraryClosedProfileDef> .

props:stratosphericOzoneLayerDestruction
        a                      owl:DatatypeProperty ;
        rdfs:comment           "算出された CFC-R11と等しい大気オゾン層を破壊するガスの量。"@ja-JP , "Quantity of gases destroying the stratospheric ozone layer calculated in equivalent CFC-R11."@en , "CFC-R11에 해당 환산된 성층권 오존층 파괴 가스량"@ko-KR , "Quantité de gaz destructeurs de la couche d'ozone exprimée en équivalent CFC-R11  [NDT : selon la norme NF P01-010]"@fr-FR ;
        rdfs:label             "DestructionCoucheOzoneStartospherique"@fr-FR , "stratosphericOzoneLayerDestruction"@en , "성층권 오존층 파괴"@ko-KR , "大気オゾン層破壊"@ja-JP ;
        rdfs:range             <https://w3id.org/product/MassMeasure> ;
        schema:domainIncludes  <https://w3id.org/product/Element> .

props:internalRefrigerantVolume
        a                      owl:DatatypeProperty ;
        rdfs:comment           "Internal volume of evaporator (refrigerant side)."@en , "蒸発器（冷媒側）の内部容積"@ja-JP , "Internal volume of condenser (refrigerant side)."@en ;
        rdfs:label             "内部冷媒容積"@ja-JP , "internalRefrigerantVolume"@en ;
        rdfs:range             <https://w3id.org/product/VolumeMeasure> ;
        schema:domainIncludes  <https://w3id.org/product/Evaporator> , <https://w3id.org/product/Condenser> .

props:groundFaultFunction
        a                      owl:DatatypeProperty ;
        rdfs:comment           "Applying ground fault function. A flag indicating that the ground fault function of the device is used. The value should be set to FALSE for devices not having a ground fault function, or if the ground fault function is not selected to be used."@en ;
        rdfs:label             "groundFaultFunction"@en ;
        rdfs:range             xsd:boolean ;
        schema:domainIncludes  <https://w3id.org/product/ProtectiveDevice> .

props:riskType  a              owl:DatatypeProperty ;
        rdfs:comment           "Identifies the predefined types of risk from which the type required may be set."@en ;
        rdfs:label             "riskType"@en ;
        schema:domainIncludes  <https://w3id.org/product/Process> .

props:instantaneousCurrentSetValue
        a                      owl:DatatypeProperty ;
        rdfs:comment           "Instantaneous current set value. The set value of the instantaneous tripping current if adjustable."@en ;
        rdfs:label             "instantaneousCurrentSetValue"@en ;
        rdfs:range             <https://w3id.org/product/ElectricCurrentMeasure> ;
        schema:domainIncludes  <https://w3id.org/product/ProtectiveDevice> .

props:waterPressureDropCurves
        a                      owl:DatatypeProperty ;
        rdfs:comment           "Water pressure drop as function of water flow rate."@en ;
        rdfs:label             "waterPressureDropCurves"@en ;
        schema:domainIncludes  <https://w3id.org/product/CooledBeam> .

props:maximumAllowedVoltageDrop
        a                      owl:DatatypeProperty ;
        rdfs:comment           "The maximum voltage drop across the circuit that must not be exceeded. \nThere are two  voltage drop limit settings that may be applied; one for sub-main circuits, and one in each Distribution Board or Consumer Unit for final circuits connected to that board. The settings should limit the overall voltage drop to the required level. Default settings of 1.5% for sub-main circuits and 2.5% for final circuits, giving an overall limit of 4% may be applied.\nNOTE: This value may also be specified as a constraint within an IFC model if required but is included within the property set at this stage pending implementation of the required capabilities within software applications."@en , "電気回路での電圧降下は最大電圧降下を超えないように。二種類の電圧降下限度があり、一つは分岐－主回路、もう一つは各分電盤或いは末端回路の電気需要装置と接続電気盤である。総電圧下降を使用範囲以内に制限する。デフォルト値は分岐－主回路1.5％、末端回路2.5％、合計総電圧4％である。\n注：この値はIFCモデルでの制約値と指定されているが、現段階ではプロプティセットに設定する。将来的には必要な性能として各ソフトアプリケションに利用する。"@ja-JP , "전기 회로에서 전압 강하는 최대 전압 강하를 초과하지 않도록. 두 종류의 전압 강하 한도가 있는데 하나는 분기 - 주회로, 다른 하나는 각 분전반 혹은 말단 회로의 전기 수요 장치와 연결 전기 판이다. 총 전압 하강을 사용 범위 이내로 제한한다. 기본값은 분기 - 주회로 1.5 %, 말단 회로 2.5 %, 합계 총 전압 4 %이다. 참고 :이 값은 IFC 모델에 따라 제한 값이 지정되어 있지만, 현 단계에서는 프로 쁘띠 세트로 설정한다. 미래에 필요한 성능으로 각 소프트웨어 어플 리케이션에 이용한다."@ko-KR ;
        rdfs:label             "maximumAllowedVoltageDrop"@en , "最大許容電圧降下"@ja-JP , "최대허용전압강하"@ko-KR ;
        rdfs:range             <https://w3id.org/product/ElectricVoltageMeasure> ;
        schema:domainIncludes  <https://w3id.org/product/DistributionSystem%2FELECTRICAL> .

props:nominalDamperDiameter
        a                      owl:DatatypeProperty ;
        rdfs:comment           "Nominal damper diameter."@en , "ダンパ直径の設計値"@ja-JP , "Diamètre nominal clapet"@fr-FR ;
        rdfs:label             "nominalDamperDiameter"@en , "設計ダンパ直径"@ja-JP , "Diamètre nominal clapet"@fr-FR ;
        rdfs:range             <https://w3id.org/product/PositiveLengthMeasure> ;
        schema:domainIncludes  <https://w3id.org/product/AirTerminalBox> .

props:photochemicalOzoneFormationPerUnit
        a                      owl:DatatypeProperty ;
        rdfs:comment           "Quantité de gaz producteurs d'ozone photochimique exprimée en équivalent ethylène tels que définis dans la norme  ISO21930:2007 [NDT : et dans la norme NF P01-010]"@fr-FR , "エチレンで計算される光化学物質オゾンを生成するガスの量。"@ja-JP , "Quantity of gases creating the photochemical ozone calculated in equivalent ethylene"@en , "에틸렌에 해당 환산된 광화학 오존 생성 끊 가스량"@ko-KR ;
        rdfs:label             "FormationOzonePhotochimiqueParUnite"@fr-FR , "단위당 광화학 오존 생성"@ko-KR , "photochemicalOzoneFormationPerUnit"@en , "単位あたり光化学オゾン生成"@ja-JP ;
        rdfs:range             <https://w3id.org/product/MassMeasure> ;
        schema:domainIncludes  <https://w3id.org/product/Element> .

props:qualityOfComponents
        a                      owl:DatatypeProperty ;
        rdfs:comment           "Adjustment of the service life resulting from the effect of the quality of components used."@en ;
        rdfs:label             "qualityOfComponents"@en ;
        schema:domainIncludes  <https://w3id.org/product/System> .

props:conditionTermination
        a                      owl:DatatypeProperty ;
        rdfs:comment           "Condition of property required on termination of the agreement e.g. cold shell, warm lit shell, broom clean, turn-key."@en ;
        rdfs:label             "conditionTermination"@en ;
        rdfs:range             xsd:string ;
        schema:domainIncludes  <https://w3id.org/product/SpatialStructureElement> .

props:shadingCoefficient
        a                      owl:DatatypeProperty ;
        rdfs:comment           "German-description-0"@de-DE , "采用遮阳设备后玻璃的太阳能得热系数（SHGC值，在欧洲等于g值）的折减，又称为Fc（或z值）。总辐射透射率\ng<total> = g*Fc。\n折减系数为一个大于0小于1的无单位数，该值越小表示传递的太阳热量越小。"@zh-CN , "(SC): ガラスの太陽熱伝導の基準、3mm（1/8インチ）透明の一枚ガラスの性能との比。遮蔽係数は太陽熱利得係数(SHGC)に移行し、段階的に廃止、SHGC×1.15とほとんど等しい。遮蔽係数は０から１までの単位無しの値。"@ja-JP , "（SC）玻璃传递太阳热量能力的度量，以3mm（1/8英寸）透明双倍强度单层玻璃为基准。遮阳系数有被太阳能得热系数（SHGC）取代的趋势，其值约为SHGC的1.15倍。遮阳系数以大于0小于1的无单位数表示。"@zh-CN , "Réduction du coefficient de transmission énergétique solaire du vitrage (SHGC, noté g en Europe) du fait de l'application d'un pare-soleil. Communément appelé Fc (ou précédemment Valeur-z). Coefficient de transmission du rayonnement total g<total> = g * Fc. Le coefficient de réduction est adimensionnel et sa valeur est comprise entre 0 et 1 ; plus la valeur de SC est petite, plus faible est la transmission d'énergie solaire."@fr-FR , "Reduction of the Solar Heat Gain Coefficient (SHGC) value (equal to the g-value in Europe) of the glazing by applying a shading device. Commonly known as Fc (or previously z-Value). The total Radiation Transmittance g<total> = g * Fc. The reduction coefficient is given as a unitless value between 0 and 1; the lower the shading coefficient (SC) the less solar heat it transmits."@en , "Das Verhältnis aus g-Wert der jeweiligen Verglasung und dem g-Wert eines Zweischeiben-Normalglasfensters.\nDer g-Wert dieses Zweischeiben-Normalglasfensters wird als Konstante mit 80 % angesetzt. Bei Einfachglas beträgt die Konstante 87 %, Auch \"Shading coefficient\" genannt."@de-DE , "(SC): Mesure de la capacité d'un vitrage à transmettre l'énergie solaire comparativement à un simple vitrage clair, de 3 mm (double renfort). Le coefficient d'atténuation est supprimé progressivement en faveur du coefficient d'apport solaire (SHGC) et est approximativement égal au SHGC multiplié par 1,15. Le coefficient d'atténuation est exprimé comme nombre sans unités entre 0 et 1."@fr-FR , "(SC): The measure of the ability of a glazing to transmit solar heat, relative to that ability for 3 mm (1/8-inch) clear, double-strength, single glass. Shading coefficient is being phased out in favor of the solar heat gain coefficient (SHGC), and is approximately equal to the SHGC multiplied by 1.15. The shading coefficient is expressed as a number without units between 0 and 1."@en ;
        rdfs:label             "CoefficientOmbrage"@fr-FR , "遮蔽係数"@ja-JP , "shadingCoefficient"@en , "German-name-0"@de-DE , "折减系数"@zh-CN , "FacteurSolaire"@fr-FR , "mittlere Durchlassfaktor b"@de-DE , "遮阳系数"@zh-CN ;
        rdfs:range             <https://w3id.org/product/NormalisedRatioMeasure> ;
        schema:domainIncludes  <https://w3id.org/product/cWindow> , <https://w3id.org/product/Door> .

props:voltage  a               owl:DatatypeProperty ;
        rdfs:comment           "The actual voltage and operable range."@en , "実電圧と動作可能範囲。"@ja-JP , "Log of electrical voltage."@en , "電圧のログ。"@ja-JP ;
        rdfs:label             "voltage"@en , "電圧"@ja-JP ;
        schema:domainIncludes  <https://w3id.org/product/DistributionPort%2FELECTRICAL> .

props:placingType  a           owl:DatatypeProperty ;
        rdfs:comment           "Location at which the type of junction box can be located."@en , "ジヤンクションボックスの配置場所。"@ja-JP , "지얀 섹션 보트 상자 설치 방법."@ko-KR ;
        rdfs:label             "placingType"@en , "位置"@ja-JP , "위치"@ko-KR ;
        schema:domainIncludes  <https://w3id.org/product/JunctionBox> .

props:derivativeConstant
        a                      owl:DatatypeProperty ;
        rdfs:comment           "The derivative gain factor of the controller (usually referred to as Kd).  Asserted where ControlType is PROPORTIONALINTEGRALDERIVATIVE."@en , "미분 게인 (Kd)"@ko-KR ;
        rdfs:label             "derivativeConstant"@en , "미분 게인 (Kd)"@ko-KR ;
        rdfs:range             xsd:decimal ;
        schema:domainIncludes  <https://w3id.org/product/Controller%2FPROPORTIONAL> .

props:force  a                 owl:DatatypeProperty ;
        rdfs:comment           "Indicates the maximum close-off force for the actuator."@en , "アクチュエータの最大締め切り力を示す。"@ja-JP , "액츄에이터의 최대 마감 힘을 보여준다."@ko-KR ;
        rdfs:label             "force"@en , "最大推力"@ja-JP , "최대추력"@ko-KR ;
        rdfs:range             <https://w3id.org/product/ForceMeasure> ;
        schema:domainIncludes  <https://w3id.org/product/Actuator> .

props:nonRenewableEnergyConsumption
        a                      owl:DatatypeProperty ;
        rdfs:comment           "Quantity of non-renewable energy used as defined in ISO21930:2007"@en , "ISO21930:2007 で定義されている継続不可能なエネルギー消費量。"@ja-JP , "ISO21930 : 2007에 정의된 재생 불가 에너지 사용량"@ko-KR , "Consommation d'énergie non renouvelable telle que définie dans les normes ISO21930:2007 [NDT : ou NF P01-010]"@fr-FR ;
        rdfs:label             "ConsommationEnergieNonRenouvelable"@fr-FR , "継続不可能なエネルギー消費量"@ja-JP , "재생 불가 에너지 소비"@ko-KR , "nonRenewableEnergyConsumption"@en ;
        rdfs:range             <https://w3id.org/product/EnergyMeasure> ;
        schema:domainIncludes  <https://w3id.org/product/Element> .

props:closeOffRating  a        owl:DatatypeProperty ;
        rdfs:comment           "クローズオフレーティング"@ja-JP , "Close off rating."@en ;
        rdfs:label             "クローズオフレーティング"@ja-JP , "closeOffRating"@en ;
        rdfs:range             <https://w3id.org/product/PressureMeasure> ;
        schema:domainIncludes  <https://w3id.org/product/Valve> , <https://w3id.org/product/Damper> .

props:accessWidth  a           owl:DatatypeProperty ;
        rdfs:comment           "アクセス（点検）カバーの幅。"@ja-JP , "사용 (체크) 커버 폭"@ko-KR , "The width of the chamber access cover where the plan shape of the cover is not circular."@en ;
        rdfs:label             "アクセス（点検）カバーの幅"@ja-JP , "accessWidth"@en , "사용 (체크)커버 폭"@ko-KR ;
        rdfs:range             <https://w3id.org/product/PositiveLengthMeasure> ;
        schema:domainIncludes  <https://w3id.org/product/DistributionChamberElement%2FINSPECTIONCHAMBER> , <https://w3id.org/product/DistributionChamberElement%2FMANHOLE> .

props:chamberLengthOrRadius
        a                      owl:DatatypeProperty ;
        rdfs:comment           "Length or, in the event of the shape being circular in plan, the radius of the chamber."@en , "챔버의 길이 또는 원형 챔버의 반경"@ko-KR , "チャンバーの長さあるいは円形チャンバーの半径。"@ja-JP ;
        rdfs:label             "챔버 (파이프 공간)의 길이 또는 반경"@ko-KR , "chamberLengthOrRadius"@en , "チャンバーの長さあるいは半径"@ja-JP , "チャンバー（バイブスペース？）の長さあるいは半径"@ja-JP , "챔버의 길이 또는 반경"@ko-KR ;
        rdfs:range             <https://w3id.org/product/PositiveLengthMeasure> ;
        schema:domainIncludes  <https://w3id.org/product/DistributionChamberElement%2FMETERCHAMBER> , <https://w3id.org/product/DistributionChamberElement%2FINSPECTIONCHAMBER> , <https://w3id.org/product/DistributionChamberElement%2FVALVECHAMBER> .

props:sensibleEffectivenessTable
        a                      owl:DatatypeProperty ;
        rdfs:comment           "Sensible heat transfer effectiveness curve as a function of the primary and secondary air flow rate."@en , "一次と二次空気量の関数としての顕熱交換効率曲線"@ja-JP , "Courbe d'efficacité d'échange thermique sensible, en tant que fonction du débit d'air au primaire et débit d'air au secondaire"@fr-FR ;
        rdfs:label             "sensibleEffectivenessTable"@en , "顕熱効率テーブル"@ja-JP , "DiagrammeEfficacitéSensible"@fr-FR ;
        schema:domainIncludes  <https://w3id.org/product/AirToAirHeatRecovery> .

props:reliefValveSetting
        a                      owl:DatatypeProperty ;
        rdfs:comment           "Pressure at which the relief valve activates."@en , "安全弁が作動する圧力"@ja-JP ;
        rdfs:label             "reliefValveSetting"@en , "安全弁設定"@ja-JP ;
        rdfs:range             <https://w3id.org/product/PressureMeasure> ;
        schema:domainIncludes  <https://w3id.org/product/Tank%2FPRESSUREVESSEL> , <https://w3id.org/product/Tank%2FEXPANSION> .

props:hangingHeight  a         owl:DatatypeProperty ;
        rdfs:comment           "The hanging height of the worksurface."@en ;
        rdfs:label             "hangingHeight"@en ;
        rdfs:range             <https://w3id.org/product/PositiveLengthMeasure> ;
        schema:domainIncludes  <https://w3id.org/product/SystemFurnitureElement%2FWORKSURFACE> .

props:waterImpermeability
        a                      owl:DatatypeProperty ;
        rdfs:comment           "Description of the water impermeability denoting the water repelling properties."@en ;
        rdfs:label             "waterImpermeability"@en ;
        rdfs:range             xsd:string ;
        schema:domainIncludes  <https://w3id.org/product/Material%2FConcrete> .

props:nominalInletAirPressure
        a                      owl:DatatypeProperty ;
        rdfs:comment           "Nominal airflow inlet static pressure."@en , "入口静圧の設計値"@ja-JP , "Pression statique en débit d'air nominal à l'entrée"@fr-FR ;
        rdfs:label             "nominalInletAirPressure"@en , "設計入口空気圧"@ja-JP , "Pression nominale à l'entrée d'air"@fr-FR ;
        rdfs:range             <https://w3id.org/product/PressureMeasure> ;
        schema:domainIncludes  <https://w3id.org/product/AirTerminalBox> .

props:carbonContent  a         owl:DatatypeProperty ;
        rdfs:comment           "The carbon content in the fuel. This is measured in weight of carbon per unit weight of fuel and is therefore unitless."@en ;
        rdfs:label             "carbonContent"@en ;
        rdfs:range             <https://w3id.org/product/PositiveRatioMeasure> ;
        schema:domainIncludes  <https://w3id.org/product/Material> .

props:nominalLength  a         owl:DatatypeProperty ;
        rdfs:comment           "The nominal length of the furniture of this type. The size information is provided in addition to the shape representation and the geometric parameters used within. In cases of inconsistency between the geometric parameters and the size properties, provided in the attached property set, the geometric parameters take precedence."@en , "要素の長さ。"@ja-JP , "公称または引用長さ。"@ja-JP , "Nominal or quoted length of the object."@en ;
        rdfs:label             "呼び長さ"@ja-JP , "長さ"@ja-JP , "nominalLength"@en ;
        rdfs:range             <https://w3id.org/product/PositiveLengthMeasure> ;
        schema:domainIncludes  <https://w3id.org/product/SanitaryTerminal%2FBATH> , <https://w3id.org/product/SanitaryTerminal%2FSINK> , <https://w3id.org/product/Furniture> , <https://w3id.org/product/SanitaryTerminal%2FURINAL> , <https://w3id.org/product/SanitaryTerminal%2FSHOWER> , <https://w3id.org/product/SanitaryTerminal%2FSANITARYFOUNTAIN> , <https://w3id.org/product/SanitaryTerminal%2FBIDET> , <https://w3id.org/product/SanitaryTerminal%2FTOILETPAN> , <https://w3id.org/product/SanitaryTerminal%2FWASHHANDBASIN> .

props:ambientDesignDryBulbTemperature
        a                      owl:DatatypeProperty ;
        rdfs:comment           "Ambient design dry bulb temperature used for selecting the cooling tower."@en ;
        rdfs:label             "ambientDesignDryBulbTemperature"@en ;
        rdfs:range             <https://w3id.org/product/ThermodynamicTemperatureMeasure> ;
        schema:domainIncludes  <https://w3id.org/product/CoolingTower> .

props:ventilatingPipeSize
        a                      owl:DatatypeProperty ;
        rdfs:comment           "Size of the ventilating pipe(s)."@en ;
        rdfs:label             "ventilatingPipeSize"@en ;
        rdfs:range             <https://w3id.org/product/PositiveLengthMeasure> ;
        schema:domainIncludes  <https://w3id.org/product/Interceptor> .

props:impedence  a             owl:DatatypeProperty ;
        rdfs:comment           "Indicates the speaker impedence."@en , "インピーダンス値を示す。"@ja-JP , "임피던스 값을 나타낸다."@ko-KR ;
        rdfs:label             "impedence"@en , "インピーダンス値"@ja-JP , "임피던스"@ko-KR ;
        rdfs:range             <https://w3id.org/product/FrequencyMeasure> ;
        schema:domainIncludes  <https://w3id.org/product/AudioVisualAppliance%2FSPEAKER> .

props:fluidFlowLeakage
        a                      owl:DatatypeProperty ;
        rdfs:comment           "漏洩量"@ja-JP , "Volumetric leakage flow rate."@en , "体積漏れ流量"@ja-JP ;
        rdfs:label             "流体漏洩量"@ja-JP , "fluidFlowLeakage"@en , "漏れ量"@ja-JP ;
        schema:domainIncludes  <https://w3id.org/product/PipeSegment> , <https://w3id.org/product/DuctSegment> .

props:leftFlangeWidth
        a                      owl:DatatypeProperty ;
        rdfs:comment           "Left flange width of the profile."@en ;
        rdfs:label             "leftFlangeWidth"@en ;
        rdfs:range             <https://w3id.org/product/PositiveLengthMeasure> ;
        schema:domainIncludes  <https://w3id.org/product/ArbitraryClosedProfileDef> .

props:isForSullageWater
        a                      owl:DatatypeProperty ;
        rdfs:comment           "Indicates if the purpose of the floor trap is to receive sullage water, or if that is amongst its purposes (= TRUE), or not (= FALSE). Note that if TRUE, it is expected that an upstand or kerb will be placed around the floor trap to prevent the ingress of surface water runoff; the provision of the upstand or kerb is not dealt with in this property set."@en , "床排水防臭弁の目的が、汚水を受けることの可（=true)否(=false)を示す。\n注意：TRUEの場合、水の流入を防ぐための床防臭弁の周りに直立壁か縁石が配置され、このプロパティセットにおいては直立壁や縁石の提供は処理されない。"@ja-JP ;
        rdfs:label             "isForSullageWater"@en , "汚水用"@ja-JP ;
        rdfs:range             xsd:boolean ;
        schema:domainIncludes  <https://w3id.org/product/WasteTerminal%2FFLOORTRAP> .

props:wasteTrapType  a         owl:DatatypeProperty ;
        rdfs:comment           "Identifies the predefined types of trap from which the type required may be set."@en , "必要とされるタイプがセットされる防臭弁の定義されたタイプを確認してください。"@ja-JP ;
        rdfs:label             "wasteTrapType"@en , "廃棄物防臭弁種類"@ja-JP ;
        schema:domainIncludes  <https://w3id.org/product/WasteTerminal%2FWASTETRAP> .

props:coolingRelativeHumidity
        a                      owl:DatatypeProperty ;
        rdfs:comment           "Inside relative humidity for cooling design."@en , "冷房設計における室内設計相対湿度。"@ja-JP , "냉방 설계의 실내 디자인 상대 습도."@ko-KR ;
        rdfs:label             "coolingRelativeHumidity"@en , "冷房設計相対湿度"@ja-JP , "냉방 설계 상대습도"@ko-KR ;
        rdfs:range             <https://w3id.org/product/PositiveRatioMeasure> ;
        schema:domainIncludes  <https://w3id.org/product/Space> .

props:currentForTimeDelay
        a                      owl:DatatypeProperty ;
        rdfs:comment           "The tripping current in [x In] at which the time delay is specified. A value for this property should only be asserted for time delay of L-function, and for I2t of the S and G function."@en , "時延[x]ののトリップ電流は、L関数の遅延時間、およびSとG関数のI2tを指定。"@ja-JP , "시간 연장 [x]의 트립 전류는 L 함수의 지연 시간 및 S와 G 함수 I2t를 지정합니다."@ko-KR ;
        rdfs:label             "currentForTimeDelay"@en , "時延電流"@ja-JP , "시간연장 전류"@ko-KR ;
        rdfs:range             <https://w3id.org/product/TimeMeasure> ;
        schema:domainIncludes  <https://w3id.org/product/ProtectiveDeviceTrippingUnit> .

props:sumpHeaterPower
        a                      owl:DatatypeProperty ;
        rdfs:comment           "Electrical heat power of sump heater."@en ;
        rdfs:label             "sumpHeaterPower"@en ;
        schema:domainIncludes  <https://w3id.org/product/CoolingTower> .

props:inputPower  a            owl:DatatypeProperty ;
        rdfs:comment           "Input power to the compressor motor."@en , "Puissance fournie au moteur du compresseur."@fr-FR ;
        rdfs:label             "inputPower"@en , "PuissanceEntréeMoteur"@fr-FR ;
        schema:domainIncludes  <https://w3id.org/product/Compressor> .

props:hoseNozzleType  a        owl:DatatypeProperty ;
        rdfs:comment           "Identifies the predefined types of nozzle (in terms of spray pattern) fitted to the end of the hose from which the type required may be set."@en , "あらかじめ定義済みのホースの先端に取り付けられるノズルの型（放出パターンの観点から）から必要な型を設定する識別。"@ja-JP ;
        rdfs:label             "hoseNozzleType"@en , "ホースノズルタイプ"@ja-JP ;
        schema:domainIncludes  <https://w3id.org/product/FireSuppressionTerminal%2FHOSEREEL> .

props:location1Global
        a                      owl:DatatypeProperty ;
        rdfs:comment           "Global X,Y,Z coordinates of the point in which Thickness1 is given"@en ;
        rdfs:label             "location1Global"@en ;
        schema:domainIncludes  <https://w3id.org/product/StructuralSurfaceMemberVarying> .

props:sensibleHeatTransferRate
        a                      owl:DatatypeProperty ;
        rdfs:comment           "Puissance thermique sensible"@fr-FR , "顕熱交換量"@ja-JP , "Sensible heat transfer rate to primary air flow."@en , "Sensible heat transfer rate."@en , "一次空気流の顕熱交換量"@ja-JP ;
        rdfs:label             "sensibleHeatTransferRate"@en , "顕熱交換量"@ja-JP , "PuissanceThermiqueSensible"@fr-FR ;
        schema:domainIncludes  <https://w3id.org/product/AirToAirHeatRecovery> , <https://w3id.org/product/EvaporativeCooler> .

props:rangeAngle  a            owl:DatatypeProperty ;
        rdfs:comment           "Indicates the maximum rotation the actuator must traverse."@en , "アクチュエータが動く最大回転角を示す。"@ja-JP , "액츄에이터가 움직이는 최대 회전각을 나타낸다."@ko-KR ;
        rdfs:label             "rangeAngle"@en , "最大回転角"@ja-JP , "최대 회전각"@ko-KR ;
        rdfs:range             <https://w3id.org/product/PlaneAngleMeasure> ;
        schema:domainIncludes  <https://w3id.org/product/Actuator> .

props:isTimeTolerancePositiveOnly
        a                      owl:DatatypeProperty ;
        rdfs:comment           "Indication whether the value of  TimeTolerance1 is provided as a positive tolereance only  or not. If not, the value is proved as a pluss/minus tolerance."@en , "許容時間1の値のみかどうか\n 上記でない場合、時間許容値は、プラス/マイナスした値。"@ja-JP , "허용 시간 1 값만 여부  위의 경우 시간 허용치는 플러스 / 마이너스 값."@ko-KR , "許容時間1の値のみかどうか。\n 上記でない場合、時間許容値は、プラス/マイナスした値。"@ja-JP ;
        rdfs:label             "isTimeTolerancePositiveOnly"@en , "時間許容値"@ja-JP , "시간 허용치"@ko-KR ;
        rdfs:range             xsd:boolean ;
        schema:domainIncludes  <https://w3id.org/product/ProtectiveDeviceTrippingUnit> .

props:ventilationIndoorAir
        a                      owl:DatatypeProperty ;
        rdfs:comment           "Ventilation loads from indoor air."@en , "室内の換気による熱負荷。"@ja-JP , "실내 환기에 의한 열 부하"@ko-KR ;
        rdfs:label             "ventilationIndoorAir"@en , "室内の換気量"@ja-JP , "실내 환기량"@ko-KR ;
        schema:domainIncludes  <https://w3id.org/product/Space> .

props:lowerHeatingValue
        a                      owl:DatatypeProperty ;
        rdfs:comment           "Lower Heating Value is defined as the amount of energy released (MJ/kg) when a fuel is burned completely, and H2O is in vapor form in the combustion products."@en ;
        rdfs:label             "lowerHeatingValue"@en ;
        rdfs:range             <https://w3id.org/product/HeatingValueMeasure> ;
        schema:domainIncludes  <https://w3id.org/product/Material> .

props:interiorRoughnessCoefficient
        a                      owl:DatatypeProperty ;
        rdfs:comment           "The interior roughness coefficient of the pipe segment."@en , "配管部の内部粗度係数"@ja-JP , "The interior roughness of the duct fitting material."@en , "ダクト継手材料の内面粗さ"@ja-JP ;
        rdfs:label             "interiorRoughnessCoefficient"@en , "内部粗度係数"@ja-JP , "内面粗さ係数"@ja-JP ;
        rdfs:range             <https://w3id.org/product/PositiveLengthMeasure> ;
        schema:domainIncludes  <https://w3id.org/product/PipeFitting> , <https://w3id.org/product/DuctSegment> , <https://w3id.org/product/DuctFitting> , <https://w3id.org/product/PipeSegment> .

props:overallEfficiency
        a                      owl:DatatypeProperty ;
        rdfs:comment           "ポンプとモーターの運用全効率"@ja-JP , "Total efficiency of motor and fan."@en , "モーターとファンの全体効率"@ja-JP , "The pump and motor overall operational efficiency."@en ;
        rdfs:label             "overallEfficiency"@en , "全体効率"@ja-JP , "全効率"@ja-JP ;
        schema:domainIncludes  <https://w3id.org/product/Fan> , <https://w3id.org/product/Pump> .

props:keyDepth  a              owl:DatatypeProperty ;
        rdfs:comment           "Key depth of the profile."@en ;
        rdfs:label             "keyDepth"@en ;
        rdfs:range             <https://w3id.org/product/NonNegativeLengthMeasure> ;
        schema:domainIncludes  <https://w3id.org/product/ArbitraryProfileDefWithVoids> .

props:shortCircuit3PoleMaximumState
        a                      owl:DatatypeProperty ;
        rdfs:comment           "Maximum 3 pole short circuit current provided at the point of supply."@en , "電源供給時点の3極最大短絡電流。"@ja-JP , "전원 공급 시점의 3 극 최대 단락 전류."@ko-KR ;
        rdfs:label             "shortCircuit3PoleMaximumState"@en , "3極最大短絡電流"@ja-JP , "3 극 최대 단락 전류"@ko-KR ;
        rdfs:range             <https://w3id.org/product/ElectricCurrentMeasure> ;
        schema:domainIncludes  <https://w3id.org/product/ElectricFlowStorageDevice> .

props:flangeThickness
        a                      owl:DatatypeProperty ;
        rdfs:comment           "Thickness of the material from which the pipe bend is constructed."@en , "パイプをつなぐ材料の厚み"@ja-JP ;
        rdfs:label             "flangeThickness"@en , "フランジの厚さ"@ja-JP ;
        rdfs:range             <https://w3id.org/product/PositiveLengthMeasure> ;
        schema:domainIncludes  <https://w3id.org/product/PipeSegment> .

props:faceArea  a              owl:DatatypeProperty ;
        rdfs:comment           "Face area open to the airstream."@en ;
        rdfs:label             "faceArea"@en ;
        rdfs:range             <https://w3id.org/product/AreaMeasure> ;
        schema:domainIncludes  <https://w3id.org/product/Damper> .

props:nominalSumpWidth
        a                      owl:DatatypeProperty ;
        rdfs:comment           "Nominal or quoted length measured along the y-axis in the local coordinate system of the sump."@en , "局所座標系のY軸に沿う形で測定され汚水槽の長さ。"@ja-JP ;
        rdfs:label             "nominalSumpWidth"@en , "汚水槽幅"@ja-JP ;
        rdfs:range             <https://w3id.org/product/PositiveLengthMeasure> ;
        schema:domainIncludes  <https://w3id.org/product/WasteTerminal%2FGULLYSUMP> .

props:shapeDescription
        a                      owl:DatatypeProperty ;
        rdfs:comment           "A description of the shape of the work surface e.g. corner square, rectangle, etc."@en ;
        rdfs:label             "shapeDescription"@en ;
        rdfs:range             xsd:string ;
        schema:domainIncludes  <https://w3id.org/product/SystemFurnitureElement%2FWORKSURFACE> .

props:photochemicalOzoneFormation
        a                      owl:DatatypeProperty ;
        rdfs:comment           "Quantity of gases creating the photochemical ozone calculated in equivalent ethylene."@en , "Quantité de gaz producteurs d'ozone photochimique exprimée en équivalent ethylène  [NDT : selon la norme NF P01-010]"@fr-FR , "算出された エチレンと等しい光化学オゾン層を生成するガスの量。"@ja-JP , "에틸렌에 해당 환산된 광화학 오존 생성 끊 가스량"@ko-KR ;
        rdfs:label             "photochemicalOzoneFormation"@en , "광화학 오존 생성"@ko-KR , "光化学オゾン生成"@ja-JP , "FormationOzonePhotochimique"@fr-FR ;
        rdfs:range             <https://w3id.org/product/MassMeasure> ;
        schema:domainIncludes  <https://w3id.org/product/Element> .

props:adjustmentRange
        a                      owl:DatatypeProperty ;
        rdfs:comment           "Upper and lower time adjustment limits for an AdjustmentValueType = RANGE. Note that this property should not have a value for an  AdjustmentValueType = LIST."@en , "Upper and lower current adjustment limits for an AdjustmentValueType = RANGE. Note that this property should not have a value for an  AdjustmentValueType = LIST."@en , "時間調整の範囲の上限値と下限値を設定。一覧表ではもっていない事を注意。"@ja-JP , "시간 조정 범위의 상한 치와 하한 치를 설정합니다. 목록은 갖고 있지 않은 것을주의."@ko-KR ;
        rdfs:label             "adjustmentRange"@en , "調整範囲"@ja-JP , "조정 범위"@ko-KR ;
        schema:domainIncludes  <https://w3id.org/product/ProtectiveDeviceTrippingUnit> .

props:yDirectionUpperBarCount
        a                      owl:DatatypeProperty ;
        rdfs:comment           "The number of bars with Y direction upper bar."@en , "Y方向の上端筋本数。"@ja-JP ;
        rdfs:label             "yDirectionUpperBarCount"@en , "Y方向上端筋本数"@ja-JP ;
        rdfs:range             xsd:int ;
        schema:domainIncludes  <https://w3id.org/product/Footing> .

props:narrativeText  a         owl:DatatypeProperty ;
        rdfs:comment           "Information sur l'usage des bâtiments voisins"@fr-FR , "Added information relating to the adjacent building use that is not appropriate to the general descriptive text associated with an entity through the inherited IfcRoot.Description."@en , "Information relative aux bâtiments voisins qui n'est pas appropriée au texte d'ordre général que l'on peut saisir dans l'attribut hérité IfcRoot.Description."@fr-FR ;
        rdfs:label             "CommentaireUsage"@fr-FR , "narrativeText"@en , "TexteLibre"@fr-FR ;
        rdfs:range             xsd:string ;
        schema:domainIncludes  <https://w3id.org/product/Building> .

props:i2  a                    owl:DatatypeProperty ;
        rdfs:comment           "サーマルの高試験電流限界値を [x In], 電流は I2 よりも高い値を示す。トリップ時間は関連する T2 の時間よりも短い。"@ja-JP , "열 동식 높은 시험 전류 한계를 [x In], 전류 I2보다 높은 값을 나타낸다. 트립 시간은 관련 T2 시간보다 짧다."@ko-KR , "열 높은 시험 전류 한계를 [x In], 전류 I2보다 높은 값을 나타낸다. 트립 시간은 관련 T2 시간보다 짧다."@ko-KR , "The (thermal) upper testing current limit in [x In], indicating that for currents larger than I2, the tripping time shall be shorter than the associated tripping time, T2."@en , "熱動式の高試験電流限界値を [x In], 電流は I2 よりも高い値を示す。トリップ時間は関連する T2 の時間よりも短い。"@ja-JP ;
        rdfs:label             "I2"@ko-KR , "I2"@ja-JP , "i2"@en ;
        rdfs:range             xsd:decimal ;
        schema:domainIncludes  <https://w3id.org/product/ProtectiveDeviceTrippingUnit%2FELECTROMAGNETIC> , <https://w3id.org/product/ProtectiveDeviceTrippingUnit%2FTHERMAL> .

props:inletConnectionSize
        a                      owl:DatatypeProperty ;
        rdfs:comment           "Size of the inlet connection(s), where used, of the inlet connections.\n\nNote that all inlet connections are assumed to be the same size."@en , "吸気口接続口のサイズ。\n\n注意：同サイズの吸気接続口がないものとします。"@ja-JP , "ホースリールへの入口接続のサイズ。"@ja-JP , "吸気口接続口のサイズ\n\n注意：同サイズの吸気口接続口がないものとする。"@ja-JP , "Size of the inlet connection to the hose reel."@en , "吸気口接続口のサイズ。\n\n注意：同サイズの吸気口接続口がないものとします。"@ja-JP , "Size of the inlet connection."@en ;
        rdfs:label             "インレット接続サイズ"@ja-JP , "inletConnectionSize"@en , "吸気口接続口サイズ"@ja-JP , "吸気口サイズ"@ja-JP ;
        rdfs:range             <https://w3id.org/product/PositiveLengthMeasure> ;
        schema:domainIncludes  <https://w3id.org/product/WasteTerminal%2FGULLYTRAP> , <https://w3id.org/product/WasteTerminal%2FFLOORTRAP> , <https://w3id.org/product/WasteTerminal%2FWASTETRAP> , <https://w3id.org/product/Interceptor> , <https://w3id.org/product/FireSuppressionTerminal%2FHOSEREEL> , <https://w3id.org/product/WasteTerminal%2FGULLYSUMP> .

props:climateChange  a         owl:DatatypeProperty ;
        rdfs:comment           "Quantity of greenhouse gases emitted calculated in equivalent CO2."@en , "算出されたCO2と等しい放出される温室効果ガスの量。"@ja-JP , "Quantité d'émissions de gaz à effet de serre exprimée en Kg d'équivalent CO2, selon les normes PrEN15804:2008 [NDT : ou NF P01-010]"@fr-FR , "CO2 등가 환산되는 온실 가스 발생량"@ko-KR ;
        rdfs:label             "기후변화"@ko-KR , "ChangementClimatique"@fr-FR , "気候変化"@ja-JP , "climateChange"@en ;
        rdfs:range             <https://w3id.org/product/MassMeasure> ;
        schema:domainIncludes  <https://w3id.org/product/Element> .

props:l  a                     owl:DatatypeProperty ;
        rdfs:comment           "Measure l according to ISO 2553"@en ;
        rdfs:label             "l"@en ;
        rdfs:range             <https://w3id.org/product/PositiveLengthMeasure> ;
        schema:domainIncludes  <https://w3id.org/product/Fastener%2FWELD> .

props:waterRequirement
        a                      owl:DatatypeProperty ;
        rdfs:comment           "Make-up water requirement."@en , "補給水の必要量"@ja-JP , "水の要件"@ja-JP , "Make-up water requirements."@en ;
        rdfs:label             "水必要量"@ja-JP , "水要件"@ja-JP , "waterRequirement"@en ;
        rdfs:range             <https://w3id.org/product/VolumetricFlowRateMeasure> ;
        schema:domainIncludes  <https://w3id.org/product/EvaporativeCooler> , <https://w3id.org/product/CoolingTower> , <https://w3id.org/product/Humidifier> .

props:uAcurves  a              owl:DatatypeProperty ;
        rdfs:comment           "UV=ｆ（V外面、V内面）、UVは、入り口での内面・外面流体速度の関数"@ja-JP , "UV = f (VExterior, VInterior), UV as a function of interior and exterior fluid flow velocity at the entrance."@en ;
        rdfs:label             "UA曲線"@ja-JP , "uAcurves"@en ;
        schema:domainIncludes  <https://w3id.org/product/Evaporator> , <https://w3id.org/product/Condenser> .

props:apparentPower  a         owl:DatatypeProperty ;
        rdfs:comment           "Apparent power."@en , "皮相電力。"@ja-JP ;
        rdfs:label             "apparentPower"@en , "皮相電力"@ja-JP ;
        schema:domainIncludes  <https://w3id.org/product/DistributionPort%2FELECTRICAL> .

props:minimumAllowableSupportLength
        a                      owl:DatatypeProperty ;
        rdfs:comment           "The minimum allowable support length."@en , "最小許容支持長さ。"@ja-JP ;
        rdfs:label             "minimumAllowableSupportLength"@en , "最小許容支持長さ"@ja-JP ;
        rdfs:range             <https://w3id.org/product/PositiveLengthMeasure> ;
        schema:domainIncludes  <https://w3id.org/product/BuildingElement> .

props:internalControl
        a                      owl:DatatypeProperty ;
        rdfs:comment           "Internal modulation control."@en , "内部調整の制御"@ja-JP ;
        rdfs:label             "internalControl"@en , "内部制御"@ja-JP ;
        schema:domainIncludes  <https://w3id.org/product/Humidifier> .

props:powerSource  a           owl:DatatypeProperty ;
        rdfs:comment           "Type of power driving the compressor."@en , "Type de puissance fournie au compresseur"@fr-FR ;
        rdfs:label             "powerSource"@en , "SourcePuissance"@fr-FR ;
        schema:domainIncludes  <https://w3id.org/product/Compressor> .

props:totalUACurves  a         owl:DatatypeProperty ;
        rdfs:comment           "Total UA curves, UA - air and water velocities, UA = [(C1 * AirFlowRate^0.8)^-1 + (C2 * WaterFlowRate^0.8)^-1]^-1.  Note: as two variables are used, DefiningValues and DefinedValues are null, and values are stored in IfcTable in the following order: AirFlowRate,WaterFlowRate,UA.  The IfcTable is related to IfcPropertyTableValue using IfcMetric and IfcPropertyConstraintRelationship."@en , "Courbes de coefficient de transmission thermique total - vitesses de l'eau et de l'air, U.S = [(C1*DébitAéraulique^0,8)^-1 + (C2*DébitHydraulique^0,8)^-1]^-1.\nRemarque: comme deux variables sont utilisées, ValeursDefinir et ValeursDéfinies sont nulles, et les valeurs sont enregistrées dans IfcTable dans l'ordre suivant:\nDébitAéraulique, DebitHydraulique, U.S.\nLe IfcTable est lié à IfcPropertyTableValue en utilisant IfcMetric et IfcPropertyConstraintRelationship."@fr-FR ;
        rdfs:label             "totalUACurves"@en , "CourbesCoefficientTransmissionThermiqueTotal"@fr-FR ;
        schema:domainIncludes  <https://w3id.org/product/Coil> .

props:nominalCondensingTemperature
        a                      owl:DatatypeProperty ;
        rdfs:comment           "Chiller condensing temperature."@en , "Température de condensation du groupe froid."@fr-FR ;
        rdfs:label             "nominalCondensingTemperature"@en , "TemperatureCondensationNominale"@fr-FR ;
        rdfs:range             <https://w3id.org/product/ThermodynamicTemperatureMeasure> ;
        schema:domainIncludes  <https://w3id.org/product/Chiller> .

props:useInDiscrimination
        a                      owl:DatatypeProperty ;
        rdfs:comment           "An indication whether the time/current tripping information can be applied in a discrimination\nanalysis or not."@en , "トリップ情報を時間か電流かどちらで判断するか。"@ja-JP , "트립 정보를 시간 또는 전류가 어디에서 결정하는가?"@ko-KR ;
        rdfs:label             "useInDiscrimination"@en , "使用方法"@ja-JP , "사용방법"@ko-KR ;
        rdfs:range             xsd:boolean ;
        schema:domainIncludes  <https://w3id.org/product/ProtectiveDeviceTrippingUnit> .

props:bodyMass  a              owl:DatatypeProperty ;
        rdfs:comment           "Overall body mass of the heater."@en , "ヒーターの全体的な質量"@ja-JP ;
        rdfs:label             "bodyMass"@en , "本体重量"@ja-JP ;
        rdfs:range             <https://w3id.org/product/MassMeasure> ;
        schema:domainIncludes  <https://w3id.org/product/SpaceHeater> .

props:pressureCurve  a         owl:DatatypeProperty ;
        rdfs:comment           "Pressure rise = f (flow rate)."@en ;
        rdfs:label             "pressureCurve"@en ;
        schema:domainIncludes  <https://w3id.org/product/Fan> .

props:cornerChamfer  a         owl:DatatypeProperty ;
        rdfs:comment           "The chamfer in the corners of the precast element. The chamfer is presumed to be equal in both directions."@en , "プレキャストコンクリート要素の面取り。面取りは両方向で等しいものとする。"@ja-JP ;
        rdfs:label             "cornerChamfer"@en , "面取り"@ja-JP ;
        rdfs:range             <https://w3id.org/product/PositiveLengthMeasure> ;
        schema:domainIncludes  <https://w3id.org/product/BuildingElement> .

props:currentTolerance1
        a                      owl:DatatypeProperty ;
        rdfs:comment           "The tolerance for the current of time/current-curve in [%]."@en , "時間/特性曲線の許容範囲を[％]で指定。"@ja-JP , "시간 / 특성 곡선의 허용 범위를 [%]로 지정합니다."@ko-KR ;
        rdfs:label             "currentTolerance1"@en , "許容電流1"@ja-JP , "허용 전류1"@ko-KR ;
        rdfs:range             <https://w3id.org/product/PositiveRatioMeasure> ;
        schema:domainIncludes  <https://w3id.org/product/ProtectiveDeviceTrippingUnit> .

props:lowerCurrent1  a         owl:DatatypeProperty ;
        rdfs:comment           "The current in [x In], indicating that for currents smaller than LowerCurrent1 the I2t part of the L-function will not trip the current,"@en , "[x In]の電流,電流をトリップするL関数のI2t部分は、下電流1よりも小さい電流を示す。"@ja-JP , "[x In] 전류 전류를 여행하는 L 함수 I2t 부분은 아래 전류 1보다 작은 전류를 보여준다."@ko-KR ;
        rdfs:label             "lowerCurrent1"@en , "下電流1"@ja-JP , "하전류 1"@ko-KR ;
        rdfs:range             <https://w3id.org/product/ElectricCurrentMeasure> ;
        schema:domainIncludes  <https://w3id.org/product/ProtectiveDeviceTrippingUnit> .

props:nominalStaticPressure
        a                      owl:DatatypeProperty ;
        rdfs:comment           "The static pressure within the air stream that the fan must overcome to insure designed circulation of air."@en , "設計空気循環量を保証するためにファンが克服しなければならない気流中の静圧"@ja-JP ;
        rdfs:label             "nominalStaticPressure"@en , "設計静圧"@ja-JP ;
        rdfs:range             <https://w3id.org/product/PressureMeasure> ;
        schema:domainIncludes  <https://w3id.org/product/Fan> .

props:maximumOutletPressure
        a                      owl:DatatypeProperty ;
        rdfs:comment           "Maximum steam outlet pressure."@en , "最大出口蒸気圧力"@ja-JP , "Pression vapeur en sortie maximale"@fr-FR ;
        rdfs:label             "maximumOutletPressure"@en , "最大出口圧力"@ja-JP , "PressionSortieAdmissible"@fr-FR ;
        rdfs:range             xsd:string ;
        schema:domainIncludes  <https://w3id.org/product/Boiler%2FSTEAM> .

props:loadBearingCapacity
        a                      owl:DatatypeProperty ;
        rdfs:comment           "Maximum load bearing capacity of the floor structure throughtout the storey as designed."@en , "Maximale Deckentragfähigkeit in diesem Geschoss."@de-DE , "Capacité porteuse maximale de la structure du plancher tel que conçu pour cet étage."@fr-FR ;
        rdfs:label             "loadBearingCapacity"@en , "Deckentragfähigkeit"@de-DE , "Capacité porteuse"@fr-FR ;
        rdfs:range             <https://w3id.org/product/PlanarForceMeasure> ;
        schema:domainIncludes  <https://w3id.org/product/BuildingStorey> .

props:numberOfCores  a         owl:DatatypeProperty ;
        rdfs:comment           "케이블과 모선의 심수 보여준다."@ko-KR , "The number of cores in Cable/Bus."@en , "Number of cores."@en , "ケーブルや母線の芯数を示す。"@ja-JP ;
        rdfs:label             "numberOfCores"@en , "심수"@ko-KR , "芯数"@ja-JP ;
        rdfs:range             xsd:int , <https://w3id.org/product/CountMeasure> ;
        schema:domainIncludes  <https://w3id.org/product/CableSegment%2FCABLESEGMENT> , <https://w3id.org/product/ArbitraryProfileDefWithVoids> .

props:articleNumber  a         owl:DatatypeProperty ;
        rdfs:comment           "Article number or reference that is be applied to a configured product according to a standard scheme for article number definition as defined by the manufacturer. It is often used as the purchasing number."@en ;
        rdfs:label             "articleNumber"@en ;
        rdfs:range             xsd:string ;
        schema:domainIncludes  <https://w3id.org/product/Element> .

props:liftElevationDifference
        a                      owl:DatatypeProperty ;
        rdfs:comment           "Elevation difference between cooling tower sump and the top of the tower."@en ;
        rdfs:label             "liftElevationDifference"@en ;
        rdfs:range             <https://w3id.org/product/PositiveLengthMeasure> ;
        schema:domainIncludes  <https://w3id.org/product/CoolingTower> .

props:naturalVentilationRate
        a                      owl:DatatypeProperty ;
        rdfs:comment           "Taux de ventilation naturelle exprimé en volumes par heure."@fr-FR , "特定の自然換気率の要求指標。1時間あたりの換気回数で与えられる。"@ja-JP , "특정 자연 환기 율의 요구 지표. 시간 당 환기 회수로 주어진다."@ko-KR , "Indication of the requirement of a particular natural air ventilation rate, given in air changes per hour."@en , "Geforderte Luftwechselzahl (in Wechsel per Stunde) im Fall der natürlichen Lüftung."@de-DE ;
        rdfs:label             "自然換気率"@ja-JP , "자연환기 비율"@ko-KR , "Taux ventilation naturelle"@fr-FR , "naturalVentilationRate"@en , "Natürliche Luftwechselzahl"@de-DE ;
        rdfs:range             <https://w3id.org/product/CountMeasure> ;
        schema:domainIncludes  <https://w3id.org/product/Space> , <https://w3id.org/product/cZone> , <https://w3id.org/product/cSpatialZone> .

props:legend  a                owl:DatatypeProperty ;
        rdfs:comment           "A text inscribed or applied to the switch as a legend to indicate purpose or function."@en , "目的または機能を示す凡例など、スイッチに適用されるテキスト。"@ja-JP , "목적이나 기능을 나타내는 범례와 같은 스위치에 적용되는 텍스트입니다."@ko-KR ;
        rdfs:label             "legend"@en , "凡例"@ja-JP , "범례"@ko-KR ;
        rdfs:range             xsd:string ;
        schema:domainIncludes  <https://w3id.org/product/SwitchingDevice> .

props:ladderConfiguration
        a                      owl:DatatypeProperty ;
        rdfs:comment           "Description of the configuration of the ladder structure used."@en , "使用されるはしご構造の概要説明。"@ja-JP , "사용되는 사다리 구조의 개요 설명."@ko-KR ;
        rdfs:label             "ladderConfiguration"@en , "梯子設定"@ja-JP , "사다리 설정"@ko-KR ;
        rdfs:range             xsd:string ;
        schema:domainIncludes  <https://w3id.org/product/CableCarrierSegment%2FCABLELADDERSEGMENT> .

props:standard  a              owl:DatatypeProperty ;
        rdfs:comment           "使用されるケーブル、busbarの定義のために使用される標準仕様。"@ja-JP , "使用するコアの定義に適用される基準の指定。"@ja-JP , "The designation of the standard applicable for the definition of the core used."@en , "사용되는 케이블, busbar의 정의를 위해 사용되는 표준."@ko-KR , "The designation of the standard applicable for the definition of the characteristics of the\ntripping_unit."@en , "The designation of the standard applicable for the definition of the Cable/Bus used."@en , "토릿삔구 장치의 특성 정의에 대한 표준 적용 지정."@ko-KR , "사용하는 코어의 정의에 적용되는 기준 지정"@ko-KR , "トリッピング装置の特性定義のための標準的な適用の指定。"@ja-JP ;
        rdfs:label             "基準"@ja-JP , "特性定義"@ja-JP , "標準"@ja-JP , "특성 정의"@ko-KR , "기준"@ko-KR , "standard"@en , "표준"@ko-KR ;
        rdfs:range             xsd:string ;
        schema:domainIncludes  <https://w3id.org/product/ProtectiveDeviceTrippingUnit> , <https://w3id.org/product/CableSegment%2FCABLESEGMENT> , <https://w3id.org/product/CableSegment%2FCORESEGMENT> .

props:hoseReelType  a          owl:DatatypeProperty ;
        rdfs:comment           "Identifies the predefined types of hose arrangement from which the type required may be set."@en , "あらかじめ定義済みのホース構成の型から必要な型を設定する識別。"@ja-JP ;
        rdfs:label             "hoseReelType"@en , "ホースリールタイプ"@ja-JP ;
        schema:domainIncludes  <https://w3id.org/product/FireSuppressionTerminal%2FHOSEREEL> .

props:shearAreaY  a            owl:DatatypeProperty ;
        rdfs:comment           "Area of the profile for calculating the shear stress due to shear force parallel to the section analysis axis ys. For example measured in mm². If given, the shear area ys shall be non-negative."@en ;
        rdfs:label             "shearAreaY"@en ;
        rdfs:range             <https://w3id.org/product/AreaMeasure> ;
        schema:domainIncludes  <https://w3id.org/product/ProfileDef> .

props:driveConnectionType
        a                      owl:DatatypeProperty ;
        rdfs:comment           "The way the pump drive mechanism is connected to the pump.\n\nDIRECTDRIVE: Direct drive. \nBELTDRIVE: Belt drive. \nCOUPLING: Coupling. \nOTHER: Other type of drive connection."@en , "ポンプの動力機械がポンプに接続される方法(直動、ベルト、カップリング、その他)"@ja-JP ;
        rdfs:label             "driveConnectionType"@en , "駆動接続タイプ"@ja-JP ;
        schema:domainIncludes  <https://w3id.org/product/Pump> .

props:loadBearing  a           owl:DatatypeProperty ;
        rdfs:comment           "荷重に関係している部材かどうかを示すブーリアン値。"@ja-JP , "オブジェクトが荷重を保持するか（TRUE）、保持しないか（FALSE）を示す。"@ja-JP , "Indicates whether the object is intended to carry loads (TRUE) or not (FALSE)."@en , "Angabe, ob dieses Bauteil tragend ist (JA) oder nichttragend (NEIN)"@de-DE , "Indique si l'objet est censé porter des charges (VRAI) ou non (FAUX)."@fr-FR , "Indique si l'objet est supposé porter des charges (VRAI) ou non (FAUX)."@fr-FR , "表示该对象是否需要承重。"@zh-CN ;
        rdfs:label             "耐力部材"@ja-JP , "loadBearing"@en , "Tragendes Bauteil"@de-DE , "Porteur"@fr-FR , "是否承重"@zh-CN ;
        rdfs:range             xsd:boolean ;
        schema:domainIncludes  <https://w3id.org/product/Plate> , <https://w3id.org/product/Chimney> , <https://w3id.org/product/BuildingElementProxy> , <https://w3id.org/product/Beam> , <https://w3id.org/product/Slab> , <https://w3id.org/product/Column> , <https://w3id.org/product/Member> , <https://w3id.org/product/Wall> .

props:iP_Code  a               owl:DatatypeProperty ;
        rdfs:comment           "인클로저에 의한 국제 보호 등급 (IP 코드)."@ko-KR , "IEC 60529 (1989) Classification of degrees of protection provided by enclosures (IP Code)."@en , "エンクロージャによる国際保護等級（IPコード）。"@ja-JP ;
        rdfs:label             "기밀성 인클로저 등급"@ko-KR , "iP_Code"@en , "機密性エンクロージャ等級"@ja-JP ;
        rdfs:range             xsd:string ;
        schema:domainIncludes  <https://w3id.org/product/DistributionElement> , <https://w3id.org/product/JunctionBox> .

props:thermometerType
        a                      owl:DatatypeProperty ;
        rdfs:comment           "Identifies the means by which temperature is displayed."@en , "温度が表示される手段を識別する。"@ja-JP , "온도가 표시되는 방법을 확인한다."@ko-KR ;
        rdfs:label             "thermometerType"@en , "温度計タイプ"@ja-JP , "온도계 유형"@ko-KR ;
        schema:domainIncludes  <https://w3id.org/product/FlowInstrument%2FTHERMOMETER> .

props:marketSubCategoriesAvailableFuture
        a                      owl:DatatypeProperty ;
        rdfs:comment           "A list of the sub categories of property that are expected to be available in the future expressed in terms of IfcLabel."@en , "Liste de sous catégories disponibles dans le futur."@fr-FR ;
        rdfs:label             "marketSubCategoriesAvailableFuture"@en , "DisponibilitesFuturesParSousCategories"@fr-FR ;
        schema:domainIncludes  <https://w3id.org/product/Building> .

props:neckAirVelocity
        a                      owl:DatatypeProperty ;
        rdfs:comment           "Air velocity at the neck."@en , "ネックの風速"@ja-JP , "Vitesse de l'air au point le plus étroit"@fr-FR ;
        rdfs:label             "neckAirVelocity"@en , "ネック風速"@ja-JP , "Vitesse de l'air au point le plus étroit"@fr-FR ;
        schema:domainIncludes  <https://w3id.org/product/AirTerminal> .

props:scheduleCompletion
        a                      owl:DatatypeProperty ;
        rdfs:comment           "The scheduled completion percentage of the allocation."@en , "予定された完了率。"@ja-JP ;
        rdfs:label             "scheduleCompletion"@en , "予定完了率"@ja-JP ;
        schema:domainIncludes  <https://w3id.org/product/ConstructionResource> .

props:anchorBoltDiameter
        a                      owl:DatatypeProperty ;
        rdfs:comment           "The nominal diameter of the anchor bolt bar(s)."@en , "アンカーボルトの直径。"@ja-JP , "앵커 볼트의 공칭 직경"@ko-KR ;
        rdfs:label             "anchorBoltDiameter"@en , "直径"@ja-JP , "지름"@ko-KR ;
        rdfs:range             <https://w3id.org/product/PositiveLengthMeasure> ;
        schema:domainIncludes  <https://w3id.org/product/MechanicalFastener%2FANCHORBOLT> .

props:spectrum  a              owl:DatatypeProperty ;
        rdfs:comment           "The spectrum of radiation describes its composition with regard to wavelength. Light, for example, as the portion of electromagnetic radiation that is visible to the human eye, is radiation with wavelengths in the range of approx. 380 to 780 nm (1 nm = 10 m). The corresponding range of colours varies from violet to indigo, blue, green, yellow, orange, and red. These colours form a continuous spectrum, in which the various spectral sectors merge into each other."@en , "波長を考慮して合成することを放射スペクトルで表現する。\n光は可視の電磁波の一種で、訳380～780nmの範囲の波長の放射である。\n色の変化は紫から藍色、青、緑、黄色、オレンジ、赤の範囲に相当する。これらの色は連続する波長で、お互いに合成した波長領域である。"@ja-JP ;
        rdfs:label             "spectrum"@en , "波長域"@ja-JP , "파장"@ko-KR ;
        schema:domainIncludes  <https://w3id.org/product/Lamp> .

props:inputPressure  a         owl:DatatypeProperty ;
        rdfs:comment           "アクチュエータへの最大設計圧力。"@ja-JP , "Maximum input control air pressure requirement."@en , "Maximum design pressure for the actuator."@en , "최대 제어 공압"@ko-KR , "最大制御空気圧。"@ja-JP , "액츄에이터의 최대 설계 압력"@ko-KR ;
        rdfs:label             "inputPressure"@en , "入力圧力"@ja-JP , "입력 압력"@ko-KR ;
        rdfs:range             <https://w3id.org/product/PressureMeasure> ;
        schema:domainIncludes  <https://w3id.org/product/Actuator%2FPNEUMATICACTUATOR> , <https://w3id.org/product/Actuator%2FHYDRAULICACTUATOR> .

props:shortCircuit2PolePowerFactorMinimumState
        a                      owl:DatatypeProperty ;
        rdfs:comment           "Power factor of the minimum 2 pole short circuit current provided at the point of supply."@en , "電源供給時点の2極最小短絡電流力率。"@ja-JP , "전원 공급 시점의 양극 최소 단락 전류 역률."@ko-KR ;
        rdfs:label             "shortCircuit2PolePowerFactorMinimumState"@en , "2極最小短絡電流力率"@ja-JP , "2 극 최소 단락 전류 역률"@ko-KR ;
        rdfs:range             xsd:decimal ;
        schema:domainIncludes  <https://w3id.org/product/ElectricFlowStorageDevice> .

props:wireDiameter  a          owl:DatatypeProperty ;
        rdfs:comment           "The nominal diameter of the wire."@en , "ワイヤーの公称直径。"@ja-JP , "와이어의 공칭 지름"@ko-KR ;
        rdfs:label             "wireDiameter"@en , "ワイヤー径"@ja-JP , "와이어 지름"@ko-KR ;
        rdfs:range             <https://w3id.org/product/PositiveLengthMeasure> ;
        schema:domainIncludes  <https://w3id.org/product/DiscreteAccessory%2FWire%20loop> .

props:torsionalSectionModulus
        a                      owl:DatatypeProperty ;
        rdfs:comment           "Torsional resistance (about xs). For example measured in mm³."@en ;
        rdfs:label             "torsionalSectionModulus"@en ;
        rdfs:range             <https://w3id.org/product/SectionModulusMeasure> ;
        schema:domainIncludes  <https://w3id.org/product/ProfileDef> .

props:diameter  a              owl:DatatypeProperty ;
        rdfs:comment           "German-description-3"@de-DE , "空构件的直径（在立面图中），仅当“形状”属性为“圆形”时适用。"@zh-CN , "构件的直径。栏杆扶手的直径。\n该属性所提供的形状信息是对内部形状描述和几何参数的补充。如果几何参数与该属性所提供的形状属性不符，应以几何参数为准。\n此处为栏杆内侧扶手或护栏的直径。"@zh-CN , "Geforderte Durchmesser des Durchbruchs, wird nur dann angegeben, wenn der Wert des Attributes \"Form\" gleich \"Rund\" ist."@de-DE , "Diameter of the object. It is the diameter of the handrail of the railing.\nThe size information is provided in addition to the shape representation and the geometric parameters used within. In cases of inconsistency between the geometric parameters and the size properties, provided in the attached property set, the geometric parameters take precedence.\nHere the diameter of the hand or guardrail within the railing."@en , "The requested diameter (in elevation) of the provision for void, only provided if the Shape property is set to \"round\"."@en , "Diamètre de la rampe du garde-corps. Cette propriété est donnée en complément de la représentation de la forme et des paramètres géométriques qui la déterminent. En cas d'incohérence entre ces paramètres géométriques et cette propriété, ce sont les paramètres géométriques qui priment."@fr-FR , "Actual diameter of a fin for circular fins only."@en , "オブジェクトの直径。"@ja-JP , "円形フィンのみ、フィンの実直径"@ja-JP , "空間における直径（高さにおける）を求める定義です。「円」形状プロパティのみに提示されます。"@ja-JP , "Le diamètre requis de la réservation (en élévation). Fournie seulement si la propriété Forme a pour valeur \"Round\"."@fr-FR ;
        rdfs:label             "直径"@ja-JP , "直径"@zh-CN , "Diamètre"@fr-FR , "Diametre"@fr-FR , "diameter"@en , "Durchmesser"@de-DE , "Handlaufdurchmesser"@de-DE ;
        rdfs:range             <https://w3id.org/product/PositiveLengthMeasure> ;
        schema:domainIncludes  <https://w3id.org/product/Railing> , <https://w3id.org/product/TubeBundle%2FFINNED> , <https://w3id.org/product/BuildingElementProxy%2FPROVISIONFORVOID> .

props:actualErectionDate
        a                      owl:DatatypeProperty ;
        rdfs:comment           "Date erected."@en ;
        rdfs:label             "actualErectionDate"@en ;
        rdfs:range             xsd:dateTime ;
        schema:domainIncludes  <https://w3id.org/product/BuildingElement> .

props:controlType  a           owl:DatatypeProperty ;
        rdfs:comment           "The type of signal modification.\nPROPORTIONAL: Output is proportional to the control error. The gain of a proportional control (Kp) will have the effect of reducing the rise time and reducing , but never eliminating, the steady-state error of the variable controlled. \nPROPORTIONALINTEGRAL: Part of the output is proportional to the control error and part is proportional to the time integral of the control error. Adding the gain of an integral control (Ki) will have the effect of eliminating the steady-state error of the variable controlled, but it may make the transient response worse. \nPROPORTIONALINTEGRALDERIVATIVE: Part of the output is proportional to the control error, part is proportional to the time integral of the control error and part is proportional to the time derivative of the control error. Adding the gain of a derivative control (Kd) will have the effect of increasing the stability of the system, reducing the overshoot, and improving the transient response of the variable controlled."@en , "신호 변경 유형   P (비례), I (적분), D (미분)의 조합 PROPORTIONAL :   P (비례) 제어 PROPORTIONALINTEGRAL :   PI (비례 적분) 제어 PROPORTIONALINTEGRALDERIVATIVE :   PID (비례 적분 미분) 제어"@ko-KR , "The type of signal modification effected and applicable ports:\n\nINPUT: Controller element is a dedicated input.\nOUTPUT: Controller element is a dedicated output.\nVARIABLE: Controller element is an in-memory variable."@en , "The type of discrete digital controller: \n\nPRIMARY: Controller has built-in communication interface for PC connection, may manage secondary controllers.\nSECONDARY: Controller communicates with primary controller and its own managed devices."@en , "컨트롤러는 항상 하나의 출력 포트와 가변 입력 포트 유형에 따라있는 한결 : output = SignalOffset 수정자 : output = input * SignalFactor + SignalOffset 절대치 : output = | input | 역수 : output = 1.0 / input 지연 : output = 지연 (input, SignalTime 후) 이동 평균 : output = 평균 (inputN, SignalTime 사이) 미분 : output = 미분 (inputN, SignalTime 사이) 적분 : output = 적분 (inputN, SignalTime 사이) 바이너리 : output = SignalOffset ※ input = TRUE의 경우 누적 : output = accumulator       ※ accumulator = 펄스 카운트 * SignalOffset       ※ if (accumulator> SignalFactor) accumulator - = SignalFactor       ??? 펄스 카운터 : output = input * SignalMultiplier       ※ input 펄스 카운트, SignalMultiplier은 원인 불명       ??? 총 : output = input1 + input2 뺄셈 : output = input1 - input2 적립 : output = input1 * input2 나누기 : output = input1 / input2 평균 : output = (input1 + input2) / 2 최대 : output = input1 or input2 ※보다 큰 최소 : output = input1 or input2 ※보다 작은"@ko-KR , "The type of signal modification effected and applicable ports:\n\nLOWERLIMITSWITCH: Single analog input is read and if less than Value.LowerBound then True is written to the output value.\nUPPERLIMITSWITCH: Single analog input is read and if more than Value.UpperBound then True is written to the output value.\nLOWERBANDSWITCH: Single analog input is read and if less than Value.LowerBound+BandWidth then True is written to the output value.\nUPPERBANDSWITCH: Single analog input is read and if more than Value.UpperBound-BandWidth then True is written to the output value.\nNOT: Single binary input is read and the opposite value is written to the output value.\nAND: Two binary inputs are read and if both are True then True is written to the output value.\nOR: Two binary inputs are read and if either is True then True is written to the output value.\nXOR: Two binary inputs are read and if one is true then True is written to the output value.\nCALENDAR: No inputs; the current time is compared with an IfcWorkCalendar to which the IfcController is assigned and True is written if active.\nINPUT: Controller element is a dedicated input.\nOUTPUT: Controller element is a dedicated output.\nVARIABLE: Controller element is an in-memory variable."@en , "The type of control used to operate the damper (e.g., Open/Closed Indicator, Resetable Temperature Sensor, Temperature Override, etc.) ."@en , "신호 변경 유형 리미트 스위치가 범위를 Pset_ControllerTypeValue 값을 묶여 속성에 의해 결정 하한 : if (Value.LowerBound> Input) output = TRUE 상한 : if (Value.UpperBound <Input) output = TRUE 하한 + 불감대 : if (Value.LowerBound + BandWidth> Input) output = TRUE 최대 - 불감대 : if (Value.UpperBound - BandWidth <Input) output = TRUE 논리 부정 : output = NOT (input) 논리적 : output = AND (input1, input2) 논리합 : output = OR (input, input2) 배타적 논리합 : output = XOR (input, input2) 달력 : output = TRUE ※ 컨트롤러에 입력없이하고 IfcWorkCalendar 컨트롤러가 할당되어 현재 시간인 경우"@ko-KR , "The type of control used to operate the damper (e.g., Open/Closed Indicator, Resetable Temperature Sensor, Temperature Override, etc.)."@en , "The type of signal modification effected and applicable ports: \n\nCONSTANT: No inputs; SignalOffset is written to the output value.\nMODIFIER: Single analog input is read, added to SignalOffset, multiplied by SignalFactor, and written to the output value.\nABSOLUTE: Single analog input is read and absolute value is written to the output value.\nINVERSE: Single analog input is read, 1.0 is divided by the input value and written to the output value.\nHYSTERISIS: Single analog input is read, delayed according to SignalTime, and written to the output value.\nRUNNINGAVERAGE: Single analog input is read, averaged over SignalTime, and written to the output value.\nDERIVATIVE: Single analog input is read and the rate of change during the SignalTime is written to the output value.\nINTEGRAL: Single analog input is read and the average value during the SignalTime is written to the output value.\nBINARY: Single binary input is read and SignalOffset is written to the output value if True.\nACCUMULATOR: Single binary input is read, and for each pulse the SignalOffset is added to the accumulator, and while the accumulator is greater than the SignalFactor, the accumulator is decremented by SignalFactor and the integer result is incremented by one.\nPULSECONVERTER: Single integer input is read, and for each increment the SignalMultiplier is added and written to the output value.\nSUM: Two analog inputs are read, added, and written to the output value.\nSUBTRACT: Two analog inputs are read, subtracted, and written to the output value.\nPRODUCT: Two analog inputs are read, multiplied, and written to the output value.\nDIVIDE: Two analog inputs are read, divided, and written to the output value.\nAVERAGE: Two analog inputs are read and the average is written to the output value.\nMAXIMUM: Two analog inputs are read and the maximum is written to the output value.\nMINIMUM: Two analog inputs are read and the minimum is written to the output value..\nINPUT: Controller element is a dedicated input.\nOUTPUT: Controller element is a dedicated output.\nVARIABLE: Controller element is an in-memory variable."@en ;
        rdfs:label             "controlType"@en , "PROPORTIONAL 유형"@ko-KR , "FLOATING 유형"@ko-KR , "TWOPOSITION 유형"@ko-KR ;
        rdfs:range             xsd:string ;
        schema:domainIncludes  <https://w3id.org/product/Controller%2FPROGRAMMABLE> , <https://w3id.org/product/Controller%2FMULTIPOSITION> , <https://w3id.org/product/Damper%2FFIRESMOKEDAMPER> , <https://w3id.org/product/Damper%2FSMOKEDAMPER> , <https://w3id.org/product/Controller%2FPROPORTIONAL> , <https://w3id.org/product/Controller%2FTWOPOSITION> , <https://w3id.org/product/Controller%2FFLOATING> .

props:breakerUnitFuseBreakingingCurve
        a                      owl:DatatypeProperty ;
        rdfs:comment           "A curve that establishes the let through breaking energy of a breaker unit when a particular prospective breaking current is applied.  Note that the breaker unit fuse breaking curve is defined within a Cartesian coordinate system and this fact must be:\n\n(1) Defining value: ProspectiveCurrentBreaking: A list of minimum 2 and maximum 8 numbers providing the currents in [A] for points in the\ncurrent/breaking energy log/log coordinate space. The curve is drawn as a straight line between two consecutive points.\n(2) Defined value: LetThroughBreakingEnergy: A list of minimum 2 and maximum 8 numbers providing the breaking energy whereby the fuse has provided a break, I2t, in [A2s] for points in the current/breakting_energy log/log coordinate space. The curve is drawn as a straight line between two consecutive."@en , "想定外の電流が流れた時に遮断機のフューズを溶かすために必要なエネルギーを表す曲線。\n  想定外の電流が流れた時に遮断機のフューズを溶かすために必要なエネルギーを表す曲線。\n\n  （1）定義値：融解電流：電流/ 融解エネルギーで示される最小2から最大8のリストで電流[A]を定義します。\n   カーブが連続する2つの点を結ぶ直線として描かれています。\n  （2）定義値：融解エネルギー：/電流/融解エネルギーの位置[A2s]で示される2～16の想定されるフューズが溶解始める電流[A2s]を定義します。カーブが連続する2つの点を結ぶ直線として描かれています。"@ja-JP , "예상치 못한 전류가 흐를 때 차단기의 퓨즈를 녹이는 데 필요한 에너지를 나타내는 곡선.   예상외의 전류가 흘렀을 때에 차단기의 퓨즈를 녹이는 데 필요한 에너지를 나타내는 곡선.   (1) 정의 값 : 융해 전류 : 전류 / 융해 에너지에 표시된 최소 2에서 최대 8 개의 목록에서 전류 [A]를 정의합니다.    커브가 연속되는 두 개의 점을 연결하는 직선으로 그려져 있습니다.   (2) 정의 값 : 융해 에너지 :/ 전류 / 융해 에너지의 위치 [A2s에서 나타나는 2 ~ 16 예상되는 퓨즈가 용해 시작 전류 [A2s을 정의합니다. 커브가 연속되는 두 개의 점을 연결하는 직선으로 그려져 있습니다."@ko-KR ;
        rdfs:label             "breakerUnitFuseBreakingingCurve"@en , "フューズ遮断機融解曲線"@ja-JP , "퓨즈 차단기 융해 곡선"@ko-KR ;
        schema:domainIncludes  <https://w3id.org/product/ProtectiveDevice> .

props:barAllocationType
        a                      owl:DatatypeProperty ;
        rdfs:comment           "Defines the type of the reinforcement bar allocation."@en , "配筋タイプの定義。"@ja-JP ;
        rdfs:label             "barAllocationType"@en , "配筋タイプ"@ja-JP ;
        schema:domainIncludes  <https://w3id.org/product/Wall> .

props:radiatorType  a          owl:DatatypeProperty ;
        rdfs:comment           "Indicates the type of radiator."@en , "ラジエーターの種類"@ja-JP ;
        rdfs:label             "radiatorType"@en , "ラジエータータイプ"@ja-JP ;
        schema:domainIncludes  <https://w3id.org/product/SpaceHeater%2FRADIATOR> .

props:weightedEfficiency
        a                      owl:DatatypeProperty ;
        rdfs:comment           "Filter efficiency based the particle weight concentration before and after filter against particles with certain size distribution."@en ;
        rdfs:label             "weightedEfficiency"@en ;
        schema:domainIncludes  <https://w3id.org/product/Filter> .

props:evaporatorMediumType
        a                      owl:DatatypeProperty ;
        rdfs:comment           "ColdLiquid: Evaporator is using liquid type of fluid to exchange heat with refrigerant.\nColdAir: Evaporator is using air to exchange heat with refrigerant."@en , "ColdLiquidは：蒸発器は、冷媒と熱交換するために液状の流体を使用しています。\nColdAir：蒸発器は、冷媒と熱交換するために空気を使用している。"@ja-JP ;
        rdfs:label             "evaporatorMediumType"@en , "蒸発媒体"@ja-JP ;
        schema:domainIncludes  <https://w3id.org/product/Evaporator> .

props:nominalWaterFlowCooling
        a                      owl:DatatypeProperty ;
        rdfs:comment           "Nominal water flow (refers to nominal cooling capacity)."@en ;
        rdfs:label             "nominalWaterFlowCooling"@en ;
        rdfs:range             <https://w3id.org/product/VolumetricFlowRateMeasure> ;
        schema:domainIncludes  <https://w3id.org/product/CooledBeam> .

props:airPressureDropCurves
        a                      owl:DatatypeProperty ;
        rdfs:comment           "Air pressure drop as function of air flow rate."@en , "風量の関数としての空気圧力降下"@ja-JP , "Perte de charge aéraulique fonction du débit d'air"@fr-FR ;
        rdfs:label             "airPressureDropCurves"@en , "空気圧力降下曲線"@ja-JP , "CourbesPerteChargeAir"@fr-FR ;
        schema:domainIncludes  <https://w3id.org/product/CooledBeam%2FACTIVE> , <https://w3id.org/product/AirToAirHeatRecovery> .

props:cOContent  a             owl:DatatypeProperty ;
        rdfs:comment           "Carbon monoxide (CO) content of the products of combustion. This is measured in weight of CO per unit weight and is therefore unitless."@en ;
        rdfs:label             "cOContent"@en ;
        rdfs:range             <https://w3id.org/product/PositiveRatioMeasure> ;
        schema:domainIncludes  <https://w3id.org/product/Material> .

props:species  a               owl:DatatypeProperty ;
        rdfs:comment           "Wood species of a solid wood or laminated wood product."@en ;
        rdfs:label             "species"@en ;
        rdfs:range             xsd:string ;
        schema:domainIncludes  <https://w3id.org/product/Material%2FWood> .

props:anchorBoltThreadLength
        a                      owl:DatatypeProperty ;
        rdfs:comment           "The length of the threaded part of the anchor bolt."@en , "앵커 볼트의 나사 부분의 길이"@ko-KR ;
        rdfs:label             "anchorBoltThreadLength"@en , "나사부 길이"@ko-KR ;
        rdfs:range             <https://w3id.org/product/PositiveLengthMeasure> ;
        schema:domainIncludes  <https://w3id.org/product/MechanicalFastener%2FANCHORBOLT> .

props:trippingCurve  a         owl:DatatypeProperty ;
        rdfs:comment           "A curve that establishes the release time of a tripping unit when a particular prospective current is applied.  Note that the tripping curve is defined within a Cartesian coordinate system and this fact must be asserted within the property set: \n\n(1) Defining value is the Prospective Current which is a list of minimum 2 and maximum 16 numbers providing the currents in [x In] for points in the current/time log/log coordinate space. The curve is drawn as a straight line between two consecutive points.\n(2) Defined value is a list of minimum 2 and maximum 16 numbers providing the release_time in [s] for points in the current/time log/log coordinate space. The curve is drawn as a straight line between two consecutive points. Note that a defined interpolation."@en , "(1)電流/時間の位置[x In]で示される2～16の想定される電流値を定義する。\n(2)定義された値は、電流/時間の位置[ｓ]で示される2～16の想定される放電時間。"@ja-JP , "(1) 전류 / 시간 위치 [x In에서 나타나는 2 ~ 16 예상되는 전류 값을 정의한다. (2) 정의된 값은 전류 / 시간 위치 [s]로 표시되는 2 ~ 16 예상되는 방전 시간."@ko-KR ;
        rdfs:label             "trippingCurve"@en , "動作特性曲線"@ja-JP , "동작 특성 곡선"@ko-KR ;
        schema:domainIncludes  <https://w3id.org/product/ProtectiveDevice> .

props:radioactiveWaste
        a                      owl:DatatypeProperty ;
        rdfs:comment           "Quantity of radioactive waste generated."@en , "방사성 폐기물 발생량"@ko-KR , "生成される放射性廃棄物の量。"@ja-JP , "Quantité de déchets radioactifs générés [NDT : selon la norme NF P01-010]"@fr-FR ;
        rdfs:label             "radioactiveWaste"@en , "DechetsRadioactifs"@fr-FR , "방사성 폐기물"@ko-KR , "放射性廃棄物"@ja-JP ;
        rdfs:range             <https://w3id.org/product/MassMeasure> ;
        schema:domainIncludes  <https://w3id.org/product/Element> .

props:diagonalTrussCrossBarSpacing
        a                      owl:DatatypeProperty ;
        rdfs:comment           "The spacing between diagonal cross-bar sections."@en , "斜めのクロスバーの間隔。"@ja-JP , "대각선 크로스바 간격"@ko-KR ;
        rdfs:label             "diagonalTrussCrossBarSpacing"@en , "クロスバー間隔"@ja-JP , "크로스바 간격"@ko-KR ;
        rdfs:range             <https://w3id.org/product/PositiveLengthMeasure> ;
        schema:domainIncludes  <https://w3id.org/product/DiscreteAccessory%2FDiagonal%20truss%20connector> .

props:angleBetweenComponentAxes
        a                      owl:DatatypeProperty ;
        rdfs:comment           "The angle between the axes of each pair of components."@en ;
        rdfs:label             "angleBetweenComponentAxes"@en ;
        rdfs:range             <https://w3id.org/product/PlaneAngleMeasure> ;
        schema:domainIncludes  <https://w3id.org/product/Slab> .

props:mountingMethod  a        owl:DatatypeProperty ;
        rdfs:comment           "The method of mounting cable segment occurrences on a cable carrier occurrence from which the method required can be selected. This is for the purpose of carrying out 'worst case' cable sizing calculations and may be a conceptual requirement rather than a statement of the physical occurrences of cable and carrier segments."@en ;
        rdfs:label             "mountingMethod"@en ;
        schema:domainIncludes  <https://w3id.org/product/CableSegment> .

props:invertLevel  a           owl:DatatypeProperty ;
        rdfs:comment           "단면의 가장 낮은 부분의 깊이 (지상에서)"@ko-KR , "단면의 가장 낮은 부분의 깊이 (지상)"@ko-KR , "The lowest point in the cross section of the sump."@en , "Level of the lowest part of the cross section as measured from ground level."@en , "断面の最も低い部分の深さ（地面から）。"@ja-JP ;
        rdfs:label             "invertLevel"@en , "最大深さ"@ja-JP , "최대 깊이"@ko-KR ;
        rdfs:range             <https://w3id.org/product/PositiveLengthMeasure> , <https://w3id.org/product/LengthMeasure> ;
        schema:domainIncludes  <https://w3id.org/product/DistributionChamberElement%2FSUMP> , <https://w3id.org/product/DistributionChamberElement%2FMANHOLE> , <https://w3id.org/product/DistributionChamberElement%2FTRENCH> , <https://w3id.org/product/DistributionChamberElement%2FINSPECTIONCHAMBER> .

props:maximumPressureLoss
        a                      owl:DatatypeProperty ;
        rdfs:comment           "Pressure loss expected across the meter under conditions of maximum flow."@en ;
        rdfs:label             "maximumPressureLoss"@en ;
        rdfs:range             <https://w3id.org/product/PressureMeasure> ;
        schema:domainIncludes  <https://w3id.org/product/FlowMeter%2FWATERMETER> , <https://w3id.org/product/FlowMeter%2FGASMETER> .

props:horizontalBarPitch
        a                      owl:DatatypeProperty ;
        rdfs:comment           "The pitch length of the horizontal bar."@en , "水平方向の補強筋の間隔。"@ja-JP ;
        rdfs:label             "horizontalBarPitch"@en , "横筋ピッチ"@ja-JP ;
        rdfs:range             <https://w3id.org/product/PositiveLengthMeasure> ;
        schema:domainIncludes  <https://w3id.org/product/Wall> .

props:infiltrationSensible
        a                      owl:DatatypeProperty ;
        rdfs:comment           "Heat gains and losses from infiltration."@en , "すき間風からの熱負荷と熱ロス。"@ja-JP , "열 부하및 열손실"@ko-KR ;
        rdfs:label             "infiltrationSensible"@en , "すき間風の顕熱"@ja-JP , "열취득 및 손실"@ko-KR ;
        schema:domainIncludes  <https://w3id.org/product/Space> .

props:maximumFlowRate
        a                      owl:DatatypeProperty ;
        rdfs:comment           "Maximum rate of flow which the meter is expected to pass."@en ;
        rdfs:label             "maximumFlowRate"@en ;
        rdfs:range             <https://w3id.org/product/VolumetricFlowRateMeasure> ;
        schema:domainIncludes  <https://w3id.org/product/FlowMeter%2FWATERMETER> , <https://w3id.org/product/FlowMeter%2FOILMETER> , <https://w3id.org/product/FlowMeter%2FGASMETER> .

props:numberofBlades  a        owl:DatatypeProperty ;
        rdfs:comment           "Number of blades."@en ;
        rdfs:label             "numberofBlades"@en ;
        rdfs:range             xsd:int ;
        schema:domainIncludes  <https://w3id.org/product/Damper> .

props:slotLength  a            owl:DatatypeProperty ;
        rdfs:comment           "Slot length."@en , "スロット長"@ja-JP , "Longueur de la fente"@fr-FR ;
        rdfs:label             "slotLength"@en , "スロット長"@ja-JP , "ElongueurFente"@fr-FR ;
        rdfs:range             <https://w3id.org/product/PositiveLengthMeasure> ;
        schema:domainIncludes  <https://w3id.org/product/AirTerminal> .

props:nominalReturnWaterTemperatureHeating
        a                      owl:DatatypeProperty ;
        rdfs:comment           "Nominal return water temperature (refers to nominal heating capacity)."@en ;
        rdfs:label             "nominalReturnWaterTemperatureHeating"@en ;
        rdfs:range             <https://w3id.org/product/ThermodynamicTemperatureMeasure> ;
        schema:domainIncludes  <https://w3id.org/product/CooledBeam> .

props:lowerVaporResistanceFactor
        a                      owl:DatatypeProperty ;
        rdfs:comment           "The vapor permeability relationship of air/material (typically value > 1), measured in low relative humidity (typically in 0/50 % RH)."@en ;
        rdfs:label             "lowerVaporResistanceFactor"@en ;
        rdfs:range             <https://w3id.org/product/PositiveRatioMeasure> ;
        schema:domainIncludes  <https://w3id.org/product/Material> .

props:bladeShape  a            owl:DatatypeProperty ;
        rdfs:comment           "Blade shape. Flat means triple V-groove."@en ;
        rdfs:label             "bladeShape"@en ;
        schema:domainIncludes  <https://w3id.org/product/Damper> .

props:videoResolutionWidth
        a                      owl:DatatypeProperty ;
        rdfs:comment           "水平方向のピクセル数。"@ja-JP , "水平方向のピクセル数を示す。"@ja-JP , "가로 픽셀 수입니다."@ko-KR , "가로 픽셀 수를 나타낸다."@ko-KR , "Indicates the number of horizontal pixels, e.g. 1920."@en , "Indicates the number of horizontal pixels (the largest native video resolution width)."@en ;
        rdfs:label             "videoResolutionWidth"@en , "水平解像度"@ja-JP , "수평 해상도"@ko-KR ;
        rdfs:range             xsd:int ;
        schema:domainIncludes  <https://w3id.org/product/AudioVisualAppliance%2FPROJECTOR> , <https://w3id.org/product/AudioVisualAppliance%2FDISPLAY> , <https://w3id.org/product/AudioVisualAppliance%2FCAMERA> .

props:duration  a              owl:DatatypeProperty ;
        rdfs:comment           "The period of time for the lease."@en ;
        rdfs:label             "duration"@en ;
        rdfs:range             xsd:duration ;
        schema:domainIncludes  <https://w3id.org/product/SpatialStructureElement> .

props:timeTolerance2  a        owl:DatatypeProperty ;
        rdfs:comment           "The tolerance for the time of the time/current-curve in [%] valid for currents above TimeToleranceLimit1."@en , "[％]で指定された時間/特性曲線の許容範囲は、上記の許容電流限界1の電流で有効です。"@ja-JP , "[%]로 지정된 시간 / 특성 곡선의 허용 범위는 상기의 허용 전류 한계 1의 전류로 사용할 수 있습니다."@ko-KR ;
        rdfs:label             "timeTolerance2"@en , "許容時間2"@ja-JP , "허용시간 2"@ko-KR ;
        rdfs:range             <https://w3id.org/product/PositiveRatioMeasure> ;
        schema:domainIncludes  <https://w3id.org/product/ProtectiveDeviceTrippingUnit> .

props:flangeDepth  a           owl:DatatypeProperty ;
        rdfs:comment           "Flange depth of the profile."@en ;
        rdfs:label             "flangeDepth"@en ;
        rdfs:range             <https://w3id.org/product/PositiveLengthMeasure> ;
        schema:domainIncludes  <https://w3id.org/product/ArbitraryClosedProfileDef> .

props:ladderTrussSecondaryBarDiameter
        a                      owl:DatatypeProperty ;
        rdfs:comment           "The nominal diameter of the secondary bar."@en , "二次バーの公称直径。"@ja-JP , "보조 막대의 공칭 지름"@ko-KR ;
        rdfs:label             "ladderTrussSecondaryBarDiameter"@en , "二次バー径"@ja-JP , "보조막대 지름"@ko-KR ;
        rdfs:range             <https://w3id.org/product/PositiveLengthMeasure> ;
        schema:domainIncludes  <https://w3id.org/product/DiscreteAccessory%2FLadder%20truss%20connector> .

props:imaginaryImpedanceRatio
        a                      owl:DatatypeProperty ;
        rdfs:comment           "The ratio between the imaginary part of the zero sequence impedance and the imaginary part of the positive impedance (i.e. imaginary part of the short-circuit voltage) of the transformer.\nUsed for three-phase transformer which includes a N-conductor."@en , "零相インピーダンスと正相インピーダンス（例．短絡電圧の虚部）の間の比率。N-コンダクターを含む三相トランスのために使用。"@ja-JP , "영 상 임피던스와 양의 상 임피던스 (예 : 단락 전압 국소 부) 사이의 비율. N-지휘자를 포함 삼상 변압기에 사용됩니다."@ko-KR ;
        rdfs:label             "imaginaryImpedanceRatio"@en , "インピーダンス虚部比率"@ja-JP , "임피던스 허수 부 비율"@ko-KR ;
        rdfs:range             <https://w3id.org/product/RatioMeasure> ;
        schema:domainIncludes  <https://w3id.org/product/Transformer> .

props:airFlowrateVersusFlowControlElement
        a                      owl:DatatypeProperty ;
        rdfs:comment           "Air flowrate versus flow control element position at nominal pressure drop."@en , "標準の圧力低下における流量制御装置の位置に対する流量"@ja-JP , "Débit d'air par rapport à la position de l'élément de contrôle du flux en perte de charge nominale"@fr-FR ;
        rdfs:label             "airFlowrateVersusFlowControlElement"@en , "流量制御特性"@ja-JP , "DébitAirContreElementControleFlux"@fr-FR ;
        schema:domainIncludes  <https://w3id.org/product/AirTerminal> .

props:coolingWaterFlowRate
        a                      owl:DatatypeProperty ;
        rdfs:comment           "Water flow rate for cooling."@en ;
        rdfs:label             "coolingWaterFlowRate"@en ;
        schema:domainIncludes  <https://w3id.org/product/CooledBeam> .

props:planningControlStatus
        a                      owl:DatatypeProperty ;
        rdfs:comment           "Label of zoning category or class, or planning control category for the site or facility."@en , "Catégorie de zone ou classe, ou catégorie relativement à un planning de contrôle pour le site ou l'ensemble immobilier."@fr-FR ;
        rdfs:label             "planningControlStatus"@en , "EtatPlanningControle"@fr-FR ;
        rdfs:range             xsd:string ;
        schema:domainIncludes  <https://w3id.org/product/Building> .

props:hasSteps  a              owl:DatatypeProperty ;
        rdfs:comment           "Indicates whether the chamber has steps (TRUE) or not (FALSE)."@en , "ダクトスペースは階段付けかどうか（TRUE或いはFALSE）。"@ja-JP , "덕트 공간은 계단 표시 여부 (TRUE 또는 FALSE)"@ko-KR ;
        rdfs:label             "hasSteps"@en , "階段付け"@ja-JP , "계단 지정"@ko-KR ;
        rdfs:range             xsd:boolean ;
        schema:domainIncludes  <https://w3id.org/product/DistributionChamberElement%2FMANHOLE> .

props:workWeekDuration
        a                      owl:DatatypeProperty ;
        rdfs:comment           "The elapsed time within a worktime-based week. For presentation purposes, applications may choose to display IfcTask durations in work weeks where IfcTaskTime.DurationType=WORKTIME. This value must be less than or equal to 168 hours (an elapsed week); if omitted then 40 hours is assumed."@en , "作業時間を基にした経過時間の週数。"@ja-JP ;
        rdfs:label             "workWeekDuration"@en , "作業週数"@ja-JP ;
        rdfs:range             xsd:duration ;
        schema:domainIncludes  <https://w3id.org/product/WorkControl> .

props:connectionSubType
        a                      owl:DatatypeProperty ;
        rdfs:comment           "物理ポート接続のサブタイプ。接続タイプ以外の情報を設定する場合に使用。下記の値を設定：\n\n- DSub: DA15, DB25, DC37, DD50, DE9, DE15 \n- Radio: IEEE802.11g, IEEE802.11n\n- RJ: 4P4C, 6P2C, 8P8C \n- USB: A, B, MiniA, MiniB, MicroA, MicroB"@ja-JP , "The physical port connection subtype that further qualifies the ConnectionType."@en ;
        rdfs:label             "接続サブタイプ"@ja-JP , "connectionSubType"@en ;
        rdfs:range             xsd:string ;
        schema:domainIncludes  <https://w3id.org/product/DistributionPort%2FCHEMICAL> , <https://w3id.org/product/DistributionPort%2FAIRCONDITIONING> .

props:heatingRelativeHumidity
        a                      owl:DatatypeProperty ;
        rdfs:comment           "Inside relative humidity for heating design."@en , "暖房設計における室内設計相対湿度。"@ja-JP , "난방 설계의 실내 디자인 상대 습도."@ko-KR ;
        rdfs:label             "heatingRelativeHumidity"@en , "暖房設計相対湿度"@ja-JP , "난방 설계 상대습도"@ko-KR ;
        rdfs:range             <https://w3id.org/product/PositiveRatioMeasure> ;
        schema:domainIncludes  <https://w3id.org/product/Space> .

props:glazingAreaFraction
        a                      owl:DatatypeProperty ;
        rdfs:comment           "Anteil der verglasten Fläche an der Gesamtfläche der Tür."@de-DE , "Rapport de la surface de vitrage à la surface totale de l'ouverture. Cette propriété sera utilisée si la surface de vitrage n'est pas donnée séparément pour tous les panneaux occupant l'ouverture."@fr-FR , "Anteil der verglasten Fläche an der Gesamtfläche des Fensters. Es ist der Reziprokwert des Rahmenanteils."@de-DE , "Part de surface de vitrage par rapport à la surface totale de l'élément de remplissage. Doit être utilisée si la surface de vitrage n'est pas donnée séparément pour tous les panneaux occupant l'ouverture."@fr-FR , "Fraction of the glazing area relative to the total area of the filling element. \nIt shall be used, if the glazing area is not given separately for all panels within the filling element."@en , "外壁の総面積に対するガラスの面積の比率。\nガラスの面積が外壁に含まれる全てのパネルと分離されていないときに、使用されます。"@ja-JP ;
        rdfs:label             "ガラス率"@ja-JP , "Glasflächenanteil"@de-DE , "glazingAreaFraction"@en , "FractionSurfaceVitree"@fr-FR ;
        rdfs:range             <https://w3id.org/product/PositiveRatioMeasure> ;
        schema:domainIncludes  <https://w3id.org/product/Door> , <https://w3id.org/product/Window> .

props:lampBallastType
        a                      owl:DatatypeProperty ;
        rdfs:comment           "The type of ballast used to stabilise gas discharge by limiting the current during operation and to deliver the necessary striking voltage for starting. Ballasts are needed to operate Discharge Lamps such as Fluorescent, Compact Fluorescent, High-pressure Mercury, Metal Halide and High-pressure Sodium Lamps. \nMagnetic ballasts are chokes which limit the current passing through a lamp connected in series on the principle of self-induction. The resultant current and power are decisive for the efficient operation of the lamp. A specially designed ballast is required for every type of lamp to comply with lamp rating in terms of Luminous Flux, Color Appearance and service life. The two types of magnetic ballasts for fluorescent lamps are KVG Conventional   (EC-A series) and VVG Low-loss ballasts (EC-B series). Low-loss ballasts have a higher efficiency, which means reduced ballast losses and a lower thermal load. Electronic ballasts are used to run fluorescent lamps at high frequencies (approx. 35 - 40 kHz)."@en , "安定器は使用中の過電流を抑え、蛍光ランプの起動に必要な高い電圧を供給し、ガス放電を安定させる。安定器は蛍光灯、水銀灯、メタルハライドランプ、高圧ナトリウムランプ等の放電灯使用する時に必要となる。\n磁気式安定器はランプに流れる電流の制限のために、直列に接続された自己誘導の手法を用いている電流と出力から照明の効率運用の結果がわかる。\n特別な設計の安定器は全ての照明の光束、色の見え方、寿命の要求に答える。\n蛍光灯用の磁気式安定器にはKVG従来型とVVG省電力型の2種類がある。\n省電力型安定器は光効率で、安定器での損失の低減及び低熱負荷になっている。電子式安定器は蛍光灯を高周波で安定的に点灯させる。"@ja-JP , "안정기는 사용중인 서지를 억제하고, 형광 램프 시작하는 데 필요한 높은 전압을 공급하여 가스 방전을 안정시킨다. 안정기는 형광등, 수은등, 메탈 할라이드 램프, 고압 나트륨 램프 등의 방전등 사용 때 필요하다. 마그네틱 안정기는 램프에 흐르는 전류의 제한을 위해 직렬로 연결된 자기 유도 방법을 사용하는 전류 출력에서 조명 효율 운영 결과 알 수있다. 특별한 디자인의 안정기는 모든 조명의 광속, 색상의 외관 수명의 요구에 반응한다. 형광 등용 자기 식 안정기에 KVG 기존과 VVG 절전 형의 2 종류가있다. 에너지 절약형 안정기는 조명 효율에서 안정기의 손실 감소 및 낮은 열 부하되어있다. 전자식 안정기는 형광등 고주파에서 안정적으로 점등한다."@ko-KR ;
        rdfs:label             "lampBallastType"@en , "安定期のタイプ"@ja-JP , "안정기의 종류"@ko-KR ;
        schema:domainIncludes  <https://w3id.org/product/Lamp> .

props:connectedConductorFunction
        a                      owl:DatatypeProperty ;
        rdfs:comment           "Function of the conductors to which the load is connected."@en , "導体の機能は負荷が接続された状態。"@ja-JP , "도체의 기능은 부하가 연결된 상태."@ko-KR ;
        rdfs:label             "connectedConductorFunction"@en , "接続導体機能"@ja-JP , "연결 도체 기능"@ko-KR ;
        schema:domainIncludes  <https://w3id.org/product/ElectricFlowStorageDevice> .

props:measuredPressureDrop
        a                      owl:DatatypeProperty ;
        rdfs:comment           "The actual pressure drop in the fluid measured across the valve."@en , "バルブを通過する際の計測された圧力降下"@ja-JP ;
        rdfs:label             "measuredPressureDrop"@en , "計測圧力降下"@ja-JP ;
        schema:domainIncludes  <https://w3id.org/product/Valve> .

props:heatingAirFlowRate
        a                      owl:DatatypeProperty ;
        rdfs:comment           "Heating air flow rate in the space."@en , "室内の暖房空気流量"@ja-JP ;
        rdfs:label             "heatingAirFlowRate"@en , "暖房空気流量"@ja-JP ;
        schema:domainIncludes  <https://w3id.org/product/Space> .

props:hasGrabHandles  a        owl:DatatypeProperty ;
        rdfs:comment           "Indicates whether the bath is fitted with handles that provide assistance to a bather in entering or leaving the bath."@en , "風呂の出入りを補助する手すりが取り付けられているかどうかを示す。"@ja-JP ;
        rdfs:label             "hasGrabHandles"@en , "手すりの有無"@ja-JP ;
        rdfs:range             xsd:boolean ;
        schema:domainIncludes  <https://w3id.org/product/SanitaryTerminal%2FBATH> .

props:fanEfficiency  a         owl:DatatypeProperty ;
        rdfs:comment           "Fan mechanical efficiency."@en , "ファン機械効率"@ja-JP ;
        rdfs:label             "fanEfficiency"@en , "Fan効率"@ja-JP ;
        schema:domainIncludes  <https://w3id.org/product/Fan> .

props:visibleAngleRight
        a                      owl:DatatypeProperty ;
        rdfs:comment           "Angle of visibility to the right of the access."@en , "Angle de visibilité à la droite de l'accès."@fr-FR , "右側の経路に可視出来る角度。"@ja-JP ;
        rdfs:label             "visibleAngleRight"@en , "VisibiliteAngleDroit"@fr-FR , "右側可視角度"@ja-JP ;
        rdfs:range             <https://w3id.org/product/PositivePlaneAngleMeasure> ;
        schema:domainIncludes  <https://w3id.org/product/Annotation%2FLineOfSight> .

props:isShallow  a             owl:DatatypeProperty ;
        rdfs:comment           "Indicates whether the chamber has been designed as being shallow (TRUE) or deep (FALSE)."@en , "ダクトスペースは浅いかどうか（TRUE或いはFALSE）。"@ja-JP , "덕트 공간이 얕은 여부 (TRUE 또는 FALSE)"@ko-KR ;
        rdfs:label             "isShallow"@en , "浅いか"@ja-JP , "덕트공간"@ko-KR ;
        rdfs:range             xsd:boolean ;
        schema:domainIncludes  <https://w3id.org/product/DistributionChamberElement%2FMANHOLE> .

props:maximumSectionModulusY
        a                      owl:DatatypeProperty ;
        rdfs:comment           "Bending resistance about the ys axis at the point with maximum zs ordinate. For example measured in mm³."@en ;
        rdfs:label             "maximumSectionModulusY"@en ;
        rdfs:range             <https://w3id.org/product/SectionModulusMeasure> ;
        schema:domainIncludes  <https://w3id.org/product/ProfileDef> .

props:fountainType  a          owl:DatatypeProperty ;
        rdfs:comment           "Selection of the type of fountain from the enumerated list of types where:-\n\nDrinkingWater: \tSanitary appliance that provides a low pressure jet of drinking water.\nEyewash: \tWaste water appliance, usually installed in work places where there is a risk of injury to eyes by solid particles or dangerous liquids, with which the user can wash the eyes without touching them."@en , "噴水タイプの選択：\n\n・飲用水：飲用水を低圧で供給するための衛生器具\n・洗眼器：廃水器具で、通常は個体の粒子か危険な液体による眼への障害の危険がある作業場所に設置され、使用者はそれらに触れずに目を洗うことができる。"@ja-JP ;
        rdfs:label             "fountainType"@en , "噴水タイプ"@ja-JP ;
        schema:domainIncludes  <https://w3id.org/product/SanitaryTerminal%2FSANITARYFOUNTAIN> .

props:outletDiameter  a        owl:DatatypeProperty ;
        rdfs:comment           "The outlet diameter of the breeching inlet."@en , "出口の直径。"@ja-JP ;
        rdfs:label             "outletDiameter"@en , "出口口径"@ja-JP ;
        rdfs:range             <https://w3id.org/product/PositiveLengthMeasure> ;
        schema:domainIncludes  <https://w3id.org/product/FireSuppressionTerminal%2FBREECHINGINLET> .

props:stirrupBarPitch
        a                      owl:DatatypeProperty ;
        rdfs:comment           "The pitch length of the stirrup bar."@en , "肋筋の間隔。"@ja-JP ;
        rdfs:label             "stirrupBarPitch"@en , "肋筋間隔"@ja-JP ;
        rdfs:range             <https://w3id.org/product/PositiveLengthMeasure> ;
        schema:domainIncludes  <https://w3id.org/product/Beam> .

props:loadDisconnectionType
        a                      owl:DatatypeProperty ;
        rdfs:comment           "A list of the available types of load disconnection from which that required may be selected."@en , "選択が必要となる、負荷開閉器タイプの一覧リスト。"@ja-JP ;
        rdfs:label             "loadDisconnectionType"@en , "切断タイプ"@ja-JP ;
        schema:domainIncludes  <https://w3id.org/product/SwitchingDevice%2FSWITCHDISCONNECTOR> .

props:setPointPressure
        a                      owl:DatatypeProperty ;
        rdfs:comment           "The pressure value to be sensed. Use IfcPropertyBoundedValue.SetPointValue to set the set point value."@en , "感知される圧力。\nセットポイント値を置くために、IfcPropertyBoundedValue.SetPointValueを使用する。"@ja-JP , "감지되는 압력. 세트 포인트 값을 넣으려면, IfcPropertyBoundedValue.SetPointValue를 사용하십시오."@ko-KR ;
        rdfs:label             "setPointPressure"@en , "圧力設定値"@ja-JP , "압력 설정"@ko-KR ;
        schema:domainIncludes  <https://w3id.org/product/Sensor%2FPRESSURESENSOR> .

props:coolingAirFlowRate
        a                      owl:DatatypeProperty ;
        rdfs:comment           "Cooling air flow rate in the space."@en , "室内の冷却空気流量"@ja-JP ;
        rdfs:label             "coolingAirFlowRate"@en , "冷却空気流量"@ja-JP ;
        schema:domainIncludes  <https://w3id.org/product/Space> .

props:thickness2  a            owl:DatatypeProperty ;
        rdfs:comment           "Second thickness parameter of a surface member with varying thickness"@en ;
        rdfs:label             "thickness2"@en ;
        rdfs:range             <https://w3id.org/product/PositiveLengthMeasure> ;
        schema:domainIncludes  <https://w3id.org/product/StructuralSurfaceMemberVarying> .

props:numberOfBoltholes
        a                      owl:DatatypeProperty ;
        rdfs:comment           "Number of boltholes in the flange."@en , "フランジにあるボルト穴の数"@ja-JP ;
        rdfs:label             "numberOfBoltholes"@en , "ボルト穴の数"@ja-JP ;
        rdfs:range             xsd:int ;
        schema:domainIncludes  <https://w3id.org/product/PipeSegment> .

props:wallMaterial  a          owl:DatatypeProperty ;
        rdfs:comment           "The material from which the wall of the chamber is constructed.\nNOTE: It is assumed that chamber walls will be constructed of a single material."@en , "덕트 공간 벽의 재질 참고 : 덕트 공간의 벽은 단층 가정"@ko-KR , "ダクトスペース壁の材質。\n注：ダクトスペースの壁は単層と仮定する"@ja-JP ;
        rdfs:label             "wallMaterial"@en , "벽의 재질"@ko-KR , "壁の材質"@ja-JP ;
        schema:domainIncludes  <https://w3id.org/product/DistributionChamberElement%2FMANHOLE> , <https://w3id.org/product/DistributionChamberElement%2FVALVECHAMBER> , <https://w3id.org/product/DistributionChamberElement%2FINSPECTIONCHAMBER> , <https://w3id.org/product/DistributionChamberElement%2FMETERCHAMBER> .

props:wallCoveringThickness
        a                      owl:DatatypeProperty ;
        rdfs:comment           "Angabe der Dicke der Materialschichten für die Wandbekleidung. \n\nDer Dickenparameter wird übernommen, wenn kein eigenes Bekleidungsobjekt (IfcCovering mit PredefinedType = CLADDING) für die Wandbekleidung dem Raum zugeordnet ist. Bei Inkonsistenzen (wenn beides gegeben ist), hat die Materialdicke des zugeordneten Bekleidungsobjekts Priorität."@de-DE , "Epaisseur de la couche de matériau constituant le revêtement de mur. Cette information sur le matériau est fournie en l'absence d'un objet de la classe IfcCovering (Type=CLADDING) avec sa propre représentation de forme. En cas d'incohérence entre les paramètres géométriques de l'instance de IfcCovering et cette propriété, ce sont les paramètres géométriques qui priment."@fr-FR , "Thickness of the material layer(s) for the space cladding.  \n\nThe thickness information is provided in absence of an IfcCovering (type=CLADDING) object with own shape representation. In cases of inconsistency between the geometric parameters of an assigned IfcCovering and this attached property, the geometric parameters take precedence."@en , "部屋の壁に関する材質層の厚さ。\n\n形状表現を持つIfcCovering(type=CLADDING)オブジェクトが存在しない場合に与えられる厚さ情報。IfcCoveringの幾何形状パラメータとこのプロパティ値が一致しない場合、幾何形状パラメータの値を優先する。"@ja-JP ;
        rdfs:label             "壁仕上げ厚"@ja-JP , "Epaisseur du revêtement de mur"@fr-FR , "Dicke der Wandbekleidung"@de-DE , "wallCoveringThickness"@en ;
        rdfs:range             <https://w3id.org/product/PositiveLengthMeasure> ;
        schema:domainIncludes  <https://w3id.org/product/Space> .

props:visibleAngleLeft
        a                      owl:DatatypeProperty ;
        rdfs:comment           "Angle of visibility to the left of the access."@en , "Angle de visibilité à la gauche de l'accès."@fr-FR , "左側の経路に可視出来る角度。"@ja-JP ;
        rdfs:label             "visibleAngleLeft"@en , "VisibiliteAngleGauche"@fr-FR , "左側可視角度"@ja-JP ;
        rdfs:range             <https://w3id.org/product/PositivePlaneAngleMeasure> ;
        schema:domainIncludes  <https://w3id.org/product/Annotation%2FLineOfSight> .

props:refrigerantClass
        a                      owl:DatatypeProperty ;
        rdfs:comment           "Refrigerant class used by the condenser.\n\nCFC: Chlorofluorocarbons.\nHCFC: Hydrochlorofluorocarbons.\nHFC: Hydrofluorocarbons."@en , "Refrigerant class used by the compressor.\n\nCFC: Chlorofluorocarbons.\nHCFC: Hydrochlorofluorocarbons.\nHFC: Hydrofluorocarbons."@en , "Classe de réfrigérant utilisé par le compresseur.\n\nCFC\nHCFC\nHFC"@fr-FR , "圧縮機で使用される冷媒種類\nCFC: Chlorofluorocarbons.\nHCFC: Hydrochlorofluorocarbons.\nHFC: Hydrofluorocarbons.\n（CFC, HCFC, HFC, HYDROCARBONS, AMMONIA, CO2, H2O, その他）"@ja-JP , "Refrigerant class used by the compressor.\nCFC: Chlorofluorocarbons.\nHCFC: Hydrochlorofluorocarbons.\nHFC: Hydrofluorocarbons."@en ;
        rdfs:label             "冷媒分類"@ja-JP , "refrigerantClass"@en , "ClasseRéfrigérant"@fr-FR ;
        schema:domainIncludes  <https://w3id.org/product/Evaporator> , <https://w3id.org/product/Condenser> , <https://w3id.org/product/Compressor> .

props:nominalAirFlowRate
        a                      owl:DatatypeProperty ;
        rdfs:comment           "Nominal airflow rate."@en , "Débit d'air nominal"@fr-FR , "設計風量"@ja-JP , "設計風量範囲"@ja-JP , "Nominal air flow rate."@en , "加湿される気流の平均量"@ja-JP , "Nominal rate of air flow into which water vapor is added."@en ;
        rdfs:label             "設計風量"@ja-JP , "nominalAirFlowRate"@en , "気流量の平均"@ja-JP , "設計風量範囲"@ja-JP , "Débit d'air nominal"@fr-FR ;
        rdfs:range             <https://w3id.org/product/VolumetricFlowRateMeasure> ;
        schema:domainIncludes  <https://w3id.org/product/AirTerminalBox> , <https://w3id.org/product/Fan> , <https://w3id.org/product/Humidifier> , <https://w3id.org/product/Damper> .

props:receptacleLoadIntensity
        a                      owl:DatatypeProperty ;
        rdfs:comment           "Average power use intensity of appliances and other non-HVAC equipment in the space per unit area.(PowerMeasure/IfcAreaMeasure)."@en , "単位面積あたり事務機器など非空調設備の平均電力消費量。\n（PowerMeasure/IfcAreaMeasure）"@ja-JP , "단위 면적 당 사무 기기 등 비 공조 설비의 평균 전력 소비. (PowerMeasure / IfcAreaMeasure)"@ko-KR ;
        rdfs:label             "receptacleLoadIntensity"@en , "単位面積あたり事務機器の平均電力消費量"@ja-JP , "단위면적 당 사무기기 평균 전력 소비량"@ko-KR ;
        rdfs:range             xsd:decimal ;
        schema:domainIncludes  <https://w3id.org/product/SpatialElement> .

props:netImpedance  a          owl:DatatypeProperty ;
        rdfs:comment           "The maximum earth loop impedance upstream of a circuit (typically stated as the variable Zs). This value is for 55o C (130oF) Celsius usage."@en , "電気回路での最大接地インピーダンス（一般はZsで表示）。55℃ (130°F)での数値。"@ja-JP , "전기 회로에서 최대 접지 임피던스 (일반은 Zs로 표시). 55 ℃ (130 ° F)의 숫자."@ko-KR ;
        rdfs:label             "netImpedance"@en , "ネットインピーダンス"@ja-JP , "인터넷 임피던스"@ko-KR ;
        rdfs:range             <https://w3id.org/product/ElectricResistanceMeasure> ;
        schema:domainIncludes  <https://w3id.org/product/DistributionSystem%2FELECTRICAL> .

props:type1  a                 owl:DatatypeProperty ;
        rdfs:comment           "Type of weld seam according to ISO 2553.  Note, combined welds are given by two corresponding symbols in the direction of the normal axis of the coordinate system.  For example, an X weld is specified by Type1 = 'V' and Type2 = 'V'."@en ;
        rdfs:label             "type1"@en ;
        rdfs:range             xsd:string ;
        schema:domainIncludes  <https://w3id.org/product/Fastener%2FWELD> .

props:ceilingCoveringThickness
        a                      owl:DatatypeProperty ;
        rdfs:comment           "Angabe der  Dicke der Materialschichten für die Deckenbekleidung. \n\nDer Dickenparameter wird übernommen, wenn kein eigenes Bekleidungsobjekt (IfcCovering mit PredefinedType = CEILING) für die Deckenbekleidung dem Raum zugeordnet ist. Bei Inkonsistenzen (wenn beides gegeben ist), hat die Materialdicke des zugeordneten Bekleidungsobjekts Priorität."@de-DE , "部屋の天井に関する材質層の厚さ。\n\n形状表現を持つIfcCovering(type=CEILING)オブジェクトが存在しない場合に与えられる厚さ情報。IfcCoveringの幾何形状パラメータとこのプロパティ値が一致しない場合、幾何形状パラメータの値を優先する。"@ja-JP , "Epaisseur de la couche de matériau constituant le revêtement de sol. Cette information sur le matériau est fournie en l'absence d'un objet de la classe IfcCovering (Type=CEILING) avec sa propre représentation de forme. En cas d'incohérence entre les paramètres géométriques de l'instance de IfcCovering et cette propriété, ce sont les paramètres géométriques qui priment."@fr-FR , "Thickness of the material layer(s) for the space ceiling.  \n\nThe thickness information is provided in absence of an IfcCovering (type=CEILING) object with own shape representation. In cases of inconsistency between the geometric parameters of an assigned IfcCovering and this attached property, the geometric parameters take precedence."@en ;
        rdfs:label             "Epaisseur du revêtement de plafond"@fr-FR , "ceilingCoveringThickness"@en , "Dicke der Deckenbekleidung"@de-DE , "天井仕上げ厚"@ja-JP ;
        rdfs:range             <https://w3id.org/product/PositiveLengthMeasure> ;
        schema:domainIncludes  <https://w3id.org/product/Space> .

props:dataReceived  a          owl:DatatypeProperty ;
        rdfs:comment           "For data ports, captures log of data received.  The LIST at IfcTimeSeriesValue.Values may split out data according to Pset_DistributionPortTypeCable.Protocols."@en , "受信データのログ。IfcTimeSeriesValue.Valuesのリスト値にはPset_DistributionPortTypeCable.Protocolsよりデータを受信する。"@ja ;
        rdfs:label             "dataReceived"@en , "受信"@ja ;
        schema:domainIncludes  <https://w3id.org/product/DistributionPort%2FELECTRICAL> .

props:outletConnectionSize
        a                      owl:DatatypeProperty ;
        rdfs:comment           "Size of the outlet connection from the object."@en , "混合弁の配管接続サイズ"@ja-JP , "要素からの接続口サイズ。"@ja-JP , "要素からの接続口口径。"@ja-JP , "Size of the outlet connection from the waste disposal unit."@en , "The size of the pipework connection from the mixing valve."@en , "要素からの排気口接続口のサイズ。"@ja-JP , "要素からの排気口サイズ。"@ja-JP , "ゴミ処理装置の排出口接続口サイズ。"@ja-JP , "Size of the outlet connection."@en ;
        rdfs:label             "outletConnectionSize"@en , "排気口サイズ"@ja-JP , "排出口接続口サイズ"@ja-JP , "出力側接続口径"@ja-JP , "接続口口径"@ja-JP , "排気口接続口サイズ"@ja-JP , "排気口接続口"@ja-JP ;
        rdfs:range             <https://w3id.org/product/PositiveLengthMeasure> ;
        schema:domainIncludes  <https://w3id.org/product/WasteTerminal%2FGULLYSUMP> , <https://w3id.org/product/WasteTerminal%2FGULLYTRAP> , <https://w3id.org/product/WasteTerminal%2FROOFDRAIN> , <https://w3id.org/product/Valve%2FMIXING> , <https://w3id.org/product/WasteTerminal%2FFLOORWASTE> , <https://w3id.org/product/Interceptor> , <https://w3id.org/product/WasteTerminal%2FWASTETRAP> , <https://w3id.org/product/WasteTerminal%2FFLOORTRAP> , <https://w3id.org/product/WasteTerminal%2FWASTEDISPOSALUNIT> .

props:auxiliaryEnergySourceConsumption
        a                      owl:DatatypeProperty ;
        rdfs:comment           "Auxiliary energy source consumption."@en , "補助エネルギー源使用量"@ja-JP ;
        rdfs:label             "auxiliaryEnergySourceConsumption"@en , "補助エネルギー源使用量"@ja-JP ;
        schema:domainIncludes  <https://w3id.org/product/SpaceHeater> .

props:category  a              owl:DatatypeProperty ;
        rdfs:comment           "Designation of the category into which the actors in the population belong."@en , "母集団の中の関与者のカテゴリー（部門・分野）の指定。"@ja-JP , "该组参与者所属的类别。"@zh-CN ;
        rdfs:label             "category"@en , "部門"@ja-JP , "类别"@zh-CN ;
        rdfs:range             xsd:string ;
        schema:domainIncludes  <https://w3id.org/product/Actor> .

props:airConditioning
        a                      owl:DatatypeProperty ;
        rdfs:comment           "Anforderung, ob der Raum mit einer Klimaanlage ausgestattet werden soll (WAHR), oder nicht (Falsch)."@de-DE , "이 공간이 공조를 요청할지 여부를 나타내는 부울 값입니다. (TRUE) 필요 (FALSE) 불필요."@ko-KR , "Indique si l'espace requiert un conditionnement d'air  (VRAI) ou non (FAUX)."@fr-FR , "この空間が空調を要求するかどうかを示すブーリアン値。(TRUE)要、(FALSE)不要。"@ja-JP , "Indication whether this space requires air conditioning provided (TRUE) or not (FALSE)."@en ;
        rdfs:label             "공조"@ko-KR , "airConditioning"@en , "空調"@ja-JP , "Conditionnement d'air"@fr-FR , "Klimaanlage"@de-DE ;
        rdfs:range             xsd:boolean ;
        schema:domainIncludes  <https://w3id.org/product/cSpatialZone> , <https://w3id.org/product/Space> , <https://w3id.org/product/cZone> .

props:valveOperation  a        owl:DatatypeProperty ;
        rdfs:comment           "The method of valve operation where:\n\nDROPWEIGHT: A valve that is closed by the action of a weighted lever being released, the weight normally being prevented from dropping by being held by a wire, the closure normally being made by the action of heat on a fusible link in the wire\nFLOAT: A valve that is opened and closed by the action of a float that rises and falls with water level. The float may be a ball attached to a lever or other mechanism\nHYDRAULIC: A valve that is opened and closed by hydraulic actuation\nLEVER: A valve that is opened and closed by the action of a lever rotating the gate within the valve.\nLOCKSHIELD: A valve that requires the use of a special lockshield key for opening and closing, the operating mechanism being protected by a shroud during normal operation.\nMOTORIZED: A valve that is opened and closed by the action of an electric motor on an actuator\nPNEUMATIC: A valve that is opened and closed by pneumatic actuation\nSOLENOID: A valve that is normally held open by a magnetic field in a coil acting on the gate but that is closed immediately if the electrical current generating the magnetic field is removed. \nSPRING: A valve that is normally held in position by the pressure of a spring on a plate but that may be caused to open if the pressure of the fluid is sufficient to overcome the spring pressure. \nTHERMOSTATIC: A valve in which the ports are opened or closed to maintain a required predetermined temperature.\nWHEEL: A valve that is opened and closed by the action of a wheel moving the gate within the valve."@en , "The method of valve operation where:弁操作方法は以下の通り：\nおもり(DROPWEIGHT)＝おもりを付けられたレバーが外される動作で閉まる弁　浮き(FLOAT)＝水位と共に上下する浮きの動作で開閉する弁。浮きはレバーに付けたボール又は他の機構　水力(HYDRAULIC)＝水力アクチュエータで開閉する弁　レバー(LEVER)＝弁内のゲートを回転させるレバーの動作で開閉する弁　ロックシールド(LOCKSHIELD)＝開閉のために特別のロックシールドキーの使用を要求する弁。操作機構は通常の操作の間は覆いで保護されている　電動化(MOTORIZED)＝アクチュエータに付けられた電動モータの動作で開閉する弁　空気圧(PNEUMATIC)＝圧縮空気で動くアクチュエータで開閉する弁　筒型コイル(SOLENOID)＝ゲートに付けられ作動しているコイルの磁界で通常は開に保たれている弁。しかし、もし磁界を発生している電流が消されたらただちに閉まる　ばね(SPRING)＝板に付けられたばねの圧力で、通常は位置を保たれている弁。しかし、もし流体の圧力が、ばねの圧力より十分大きければ開いてしまう。　自動温度調節(THERMOSTATIC)＝前もって決められた要求温度を維持するために、中のポートが開閉する弁　ハンドル(WHEEL)＝弁内のゲートを動かすハンドルの動作で開閉する弁"@ja-JP ;
        rdfs:label             "valveOperation"@en , "弁操作"@ja-JP ;
        schema:domainIncludes  <https://w3id.org/product/Valve> .

props:spaceTemperatureMax
        a                      owl:DatatypeProperty ;
        rdfs:comment           "공간 또는 영역의 최고 온도. 이용자 / 설계자의 관점에서 요구된다. 만약 여름철 또는 겨울철 실내 온도 요구가 주어지지 않는, 그것은 연중에, 그렇지 않으면 중간 분기별로 적용된다."@ko-KR , "Maximale geforderte Raumtemperatur, die nicht überschritten werden darf, gilt als ganzjährige Anforderung unabhängig vom Heizungs-, oder Kühlungsfall."@de-DE , "空間またはゾーンの最高温度。利用者/設計者の視点から要求される。もし夏季または冬季の室内温度要求が与えられないと、それは通年に、さもなければ中間季に適用される。"@ja-JP , "Température maximale de l'espace ou de la zone spécifiée par l'usager ou le concepteur. Si les valeurs pour l'été et l'hiver ne sont pas connues, cette température s'applique toute l'année, sinon seulement en demi-saison."@fr-FR , "Maximal temperature of the space or zone, that is required from user/designer view point.  If no summer or winter space temperature requirements are given, it applies all year, otherwise for the intermediate period."@en ;
        rdfs:label             "最高室内温度"@ja-JP , "spaceTemperatureMax"@en , "Température maximale"@fr-FR , "최고 온도"@ko-KR , "Raumtemperatur Maximal"@de-DE ;
        rdfs:range             <https://w3id.org/product/ThermodynamicTemperatureMeasure> ;
        schema:domainIncludes  <https://w3id.org/product/cZone> , <https://w3id.org/product/Space> , <https://w3id.org/product/cSpatialZone> .

props:rightFlangeWidth
        a                      owl:DatatypeProperty ;
        rdfs:comment           "Right flange width of the profile."@en ;
        rdfs:label             "rightFlangeWidth"@en ;
        rdfs:range             <https://w3id.org/product/PositiveLengthMeasure> ;
        schema:domainIncludes  <https://w3id.org/product/ArbitraryClosedProfileDef> .

props:longitudinalSeam
        a                      owl:DatatypeProperty ;
        rdfs:comment           "The type of seam to be used along the longitudinal axis of the duct segment."@en , "ハゼの種類は、ダクト直管の縦方向に使用するハゼの種類"@ja-JP ;
        rdfs:label             "longitudinalSeam"@en , "ハゼ"@ja-JP ;
        rdfs:range             xsd:string ;
        schema:domainIncludes  <https://w3id.org/product/DuctSegment> .

props:appearanceGrade
        a                      owl:DatatypeProperty ;
        rdfs:comment           "Grade with respect to visual quality."@en ;
        rdfs:label             "appearanceGrade"@en ;
        rdfs:range             xsd:string ;
        schema:domainIncludes  <https://w3id.org/product/Material%2FWood> .

props:mounting  a              owl:DatatypeProperty ;
        rdfs:comment           "Selection of the form of mounting from the enumerated list of mountings where:-\n\nBackToWall =\tA pedestal mounted sanitary terminal that fits flush to the wall at the rear to cover its service connections\nPedestal =\tA floor mounted sanitary terminal that has an integral base\nCounterTop =\tA sanitary terminal that is installed into a horizontal surface that is installed into a horizontal surface. Note: When applied to a wash hand basin, the term more normally used is ‘vanity’. See also Wash Hand Basin Type specification.\nWallHung =\tA sanitary terminal cantilevered clear of the floor\n.\n\nNote that BackToWall, Pedestal and WallHung are allowable values for a urinal."@en , "下記の設置方法より選択\n\n\n・床置き壁排出：接続口の後部に出水口を合わせること。\n・台：床置きの衛生器具には基礎があること。\n・カウンター：衛生器具の表層が水平に設置されていること。※手洗い台として設置された場合「化粧台」として扱うこと。また、洗面台種類の規格表を参照のこと。\n・壁掛け型：衛生器具は片側固定がされ床から離れていること。\n\n床置き壁排出型・台座と壁掛け型は便器と同等とされます。"@ja-JP , "Selection of the form of mounting from the enumerated list of mountings where:-\n\nBackToWall: \tA pedestal mounted sanitary terminal that fits flush to the wall at the rear to cover its service connections.\nPedestal: \tA floor mounted sanitary terminal that has an integral base\nCounterTop: \tA sanitary terminal that is installed into a horizontal surface that is installed into a horizontal surface. Note: When applied to a wash hand basin, the term more normally used is ‘vanity’. See also Wash Hand Basin Type specification.\nWallHung: \tA sanitary terminal cantilevered clear of the floor."@en , "Selection of the form of mounting of the fountain from the enumerated list of mountings where:-\n\nBackToWall: \tA pedestal mounted sanitary terminal that fits flush to the wall at the rear to cover its service connections.\nPedestal: \tA floor mounted sanitary terminal that has an integral base\n.\nCounterTop: \tA sanitary terminal that is installed into a horizontal surface that is installed into a horizontal surface. Note: When applied to a wash hand basin, the term more normally used is ‘vanity’. See also Wash Hand Basin Type specification.\nWallHung: \tA sanitary terminal cantilevered clear of the floor."@en , "設置場所の選択\n\n・床置き壁排出：接続口の後部に出水口を合わせること。\n・台：床置きの衛生器具には基礎があること。\n・調理台：衛生器具の表層が水平に設置されていること。※手洗い台として設置された場合「化粧台」として扱うこと。また、洗面台種類の規格表を参照のこと。\n・壁掛け型：衛生器具は片側固定がされ床から離れていること。"@ja-JP , "The property enumeration Pset_SanitaryMountingEnum defines the forms of mounting or fixing of the sanitary terminal that may be specified within property sets used to define sanitary terminals (WC’s, basins, sinks, etc.) where:-\n\nBackToWall: \tA pedestal mounted sanitary terminal that fits flush to the wall at the rear to cover its service connections\n.\nPedestal: \tA floor mounted sanitary terminal that has an integral base\n.\nCounterTop: \tA sanitary terminal that is installed into a horizontal surface that is installed into a horizontal surface. Note: When applied to a wash hand basin, the term more normally used is ‘vanity’. See also Wash Hand Basin Type specification.\nWallHung: \tA sanitary terminal cantilevered clear of the floor.\n\nNote that BackToWall, Pedestal and WallHung are allowable values for a bidet."@en , "列挙するプロパティはPset_SanitaryMountingEnumでは（トイレの、洗面台、シンクなど）、衛生配管への装着法で定義される：\n\n床置き壁排水：台座は、カバーの背面の壁にあるフラッシュバルブに接続される。\n\n床置き：床の衛生配管に装着される。\n\nカウンター：水平面に設置された衛生配管に接続します。注：手洗器があると、通常は'化粧'が使用される。手洗器を参照。\n\n壁掛け：衛生配管は壁から出され床には何もなくなる。。\n\n床置き壁排水、床置き、壁掛けは、ビデの許容値であることに注意。"@ja-JP , "設置場所の選択：\n\n・床置き壁排出：接続口の後部に出水口を合わせること。\n・台：床置きの衛生器具には基礎があること。\n・調理台：衛生器具の表層が水平に設置されていること。※手洗い台として設置された場合「化粧台」として扱うこと。また、洗面台種類の規格表を参照のこと。\n・壁掛け型：衛生器具は片側固定がされ床から離れていること。"@ja-JP , "Selection of the form of mounting of the sink from the enumerated list of mountings where:-\n\nBackToWall: A pedestal mounted sanitary terminal that fits flush to the wall at the rear to cover its service connections.\nPedestal: \tA floor mounted sanitary terminal that has an integral base.\nCounterTop: \tA sanitary terminal that is installed into a horizontal surface that is installed into a horizontal surface. Note: When applied to a wash hand basin, the term more normally used is ‘vanity’. See also Wash Hand Basin Type specification.\nWallHung: \tA sanitary terminal cantilevered clear of the floor."@en , "以下のリストから設置方法を選択\n\n\n・床置き壁排出：接続口の後部に出水口を合わせること。\n・台：床置きの衛生器具には基礎があること。\n・カウンター：衛生器具の表層が水平に設置されていること。※手洗い台として設置された場合「化粧台」として扱うこと。また、洗面台種類の規格表を参照のこと。\n・壁掛け型：衛生器具は片側固定がされ床から離れていること。"@ja-JP ;
        rdfs:label             "設置"@ja-JP , "mounting"@en , "装着"@ja-JP ;
        schema:domainIncludes  <https://w3id.org/product/SanitaryTerminal%2FSINK> , <https://w3id.org/product/SanitaryTerminal%2FWASHHANDBASIN> , <https://w3id.org/product/SanitaryTerminal%2FBIDET> , <https://w3id.org/product/SanitaryTerminal%2FSANITARYFOUNTAIN> , <https://w3id.org/product/SanitaryTerminal%2FURINAL> .

props:torqueRange  a           owl:DatatypeProperty ;
        rdfs:comment           "Torque range: minimum operational torque to maximum allowable torque."@en ;
        rdfs:label             "torqueRange"@en ;
        schema:domainIncludes  <https://w3id.org/product/Damper%2FCONTROLDAMPER> .

props:maximumPlenumSensibleLoad
        a                      owl:DatatypeProperty ;
        rdfs:comment           "Maximum or Peak sensible thermal load contributed to the conditioned space by the light fixture."@en ;
        rdfs:label             "maximumPlenumSensibleLoad"@en ;
        rdfs:range             <https://w3id.org/product/PowerMeasure> ;
        schema:domainIncludes  <https://w3id.org/product/LightFixture> .

props:coreTopHeight  a         owl:DatatypeProperty ;
        rdfs:comment           "Core top height of the profile."@en ;
        rdfs:label             "coreTopHeight"@en ;
        rdfs:range             <https://w3id.org/product/PositiveLengthMeasure> ;
        schema:domainIncludes  <https://w3id.org/product/ArbitraryProfileDefWithVoids> .

props:nominalCurrents
        a                      owl:DatatypeProperty ;
        rdfs:comment           "A set of nominal currents in [A] for which the data of this instance is valid. At least one value shall be provided. Any value in the set shall not exceed the value of the \nUltimateRatedCurrent associated with the same breaker unit."@en , "정격 전류 [A]를 적어도 2 개의 값을 설정해야한다.   동일한 차단기부와 연결된 정격전류는세트 내의 임의의 값은 초과할 수 없다."@ko-KR , "トリップ装置が対応する定格電流。"@ja-JP , "定格電流[A]を少なくても1つ値をセットしなければならない。\n セット内の任意の値の値を超えてはならない。\n 定格電流は、同じブレーカ部に関連付けられている。"@ja-JP , "트립 장치가 지원하는 정격 전류."@ko-KR , "A set of values providing information on available modules (chips) for setting the nominal current of the protective device. If\nthe set is empty, no nominal current modules are available for the tripping unit."@en ;
        rdfs:label             "nominalCurrents"@en , "정격전류"@ko-KR , "정격 전류"@ko-KR , "定格電流"@ja-JP ;
        schema:domainIncludes  <https://w3id.org/product/ProtectiveDevice%2FCIRCUITBREAKER> , <https://w3id.org/product/ProtectiveDeviceTrippingUnit%2FELECTRONIC> .

props:patternType  a           owl:DatatypeProperty ;
        rdfs:comment           "定義　パターンのタイプ（又はタンクの形状）が明示される。"@ja-JP , "Defines the types of pattern (or shape of a tank that may be specified."@en , "定義　パターンのタイプ（又はタンクの形状)が明示される"@ja-JP ;
        rdfs:label             "patternType"@en , "パターンタイプ"@ja-JP ;
        schema:domainIncludes  <https://w3id.org/product/Tank%2FPREFORMED> , <https://w3id.org/product/Tank> .

props:diagonalTrussSecondaryBarDiameter
        a                      owl:DatatypeProperty ;
        rdfs:comment           "The nominal diameter of the secondary bar."@en , "二次バーの公称直径。"@ja-JP , "보조 막대의 공칭 지름"@ko-KR ;
        rdfs:label             "diagonalTrussSecondaryBarDiameter"@en , "二次バー径"@ja-JP , "보조 막대 지름"@ko-KR ;
        rdfs:range             <https://w3id.org/product/PositiveLengthMeasure> ;
        schema:domainIncludes  <https://w3id.org/product/DiscreteAccessory%2FDiagonal%20truss%20connector> .

props:isExternal  a            owl:DatatypeProperty ;
        rdfs:comment           "ジャンクションボックスが外部露出の許可がされているかどうかを表示（外部露出が許可されている場合は設定）。"@ja-JP , "表示该图元是否设计为外部构件。若是，则该图元为外部图元，朝向建筑物的外部。"@zh-CN , "外部の部材かどうかを示すブーリアン値。もしTRUEの場合、外部の部材で建物の外側に面している。"@ja-JP , "Angabe, ob dieser Bekleidung eine Außenbekleidung ist (JA) oder ein Innenbekleidung (NEIN)."@de-DE , "表示该构件是否设计为外部构件。若是，则该构件为外部构件，朝向建筑物的外侧。"@zh-CN , "この要素が外部に用いられるか（TRUE）、否か（FALSE）を示す。（TRUE)の場合、これは外部要素で、建物の外部に面している。"@ja-JP , "Indique si l'élément est conçu pour être utilisé à l'extérieur (VRAI) ou non (FAUX). Si VRAI, c'est un élément extérieur qui donne sur l'extérieur du bâtiment."@fr-FR , "Indication whether the element is designed for use in the exterior (TRUE) or not (FALSE). If (TRUE) it is an external element and faces the outside of the building."@en , "Indication of whether the junction box type is allowed for exposure to outdoor elements (set TRUE where external exposure is allowed)."@en , "Indication whether the element is designed for use in the exterior (TRUE) or not (FALSE). If (TRUE) it is an external zone at the outside of the building."@en , "Angabe, ob dieses Bauteil ein Aussenbauteil ist (JA) oder ein Innenbauteil (NEIN). Als Aussenbauteil grenzt es an den Aussenraum (oder Erdreich, oder Wasser)."@de-DE , "정션 박스 외부 노출의 허가가되어 있는지 여부를 표시 (외부 노출이 허용되는 경우 설정)."@ko-KR , "Angabe, ob dieser Raum ein Aussenaum ist (JA) oder ein Innenraum (NEIN)."@de-DE ;
        rdfs:label             "外部"@ja-JP , "外部露出"@ja-JP , "Außenbauteil"@de-DE , "외부노출"@ko-KR , "IstAußenraum"@de-DE , "EstExterieur"@fr-FR , "外部区分"@ja-JP , "isExternal"@en , "是否外部构件"@zh-CN , "Est extérieur"@fr-FR ;
        rdfs:range             xsd:boolean ;
        schema:domainIncludes  <https://w3id.org/product/Ramp> , <https://w3id.org/product/BuildingElementProxy> , <https://w3id.org/product/ShadingDevice> , <https://w3id.org/product/Wall> , <https://w3id.org/product/Stair> , <https://w3id.org/product/Window> , <https://w3id.org/product/Column> , <https://w3id.org/product/Zone> , <https://w3id.org/product/Slab> , <https://w3id.org/product/Member> , <https://w3id.org/product/Beam> , <https://w3id.org/product/Door> , <https://w3id.org/product/Railing> , <https://w3id.org/product/Chimney> , <https://w3id.org/product/Roof> , <https://w3id.org/product/CurtainWall> , <https://w3id.org/product/Covering> , <https://w3id.org/product/Plate> , <https://w3id.org/product/Space> , <https://w3id.org/product/JunctionBox> .

props:pressureRating  a        owl:DatatypeProperty ;
        rdfs:comment           "管轄組織により設定されたボイラの常用圧力"@ja-JP , "最大圧力、消火栓の耐圧。"@ja-JP , "Nominal pressure rating of the boiler as rated by the agency having jurisdiction."@en , "Maximum pressure that the hydrant is manufactured to withstand."@en , "Pression nominale admissible de la chaudière comme classée par l'organisme qui fait autorité."@fr-FR ;
        rdfs:label             "圧力"@ja-JP , "常用圧力"@ja-JP , "PressionAdmissibleNominale"@fr-FR , "pressureRating"@en ;
        rdfs:range             <https://w3id.org/product/PressureMeasure> ;
        schema:domainIncludes  <https://w3id.org/product/Boiler> , <https://w3id.org/product/FireSuppressionTerminal%2FFIREHYDRANT> .

props:connectionType  a        owl:DatatypeProperty ;
        rdfs:comment           "物理ポート接続：\n\n- Coaxial: 同軸コネクタ.\n- DSub: D-Subコネクタ.\n- Infrared:赤外線\n- RJ: 登録済みジャック.\n- Radio: 無線\n- USB: USB."@ja-JP , "The end-style treatment of the duct port:\n\nBEADEDSLEEVE: Beaded Sleeve. \nCOMPRESSION: Compression. \nCRIMP: Crimp. \nDRAWBAND: Drawband. \nDRIVESLIP: Drive slip. \nFLANGED: Flanged. \nOUTSIDESLEEVE: Outside Sleeve. \nSLIPON: Slipon. \nSOLDERED: Soldered. \nSSLIP: S-Slip. \nSTANDINGSEAM: Standing seam. \nSWEDGE: Swedge. \nWELDED: Welded. \nOTHER: Another type of end-style has been applied.\nNONE: No end-style has been applied."@en , "The physical port connection:\n\nACPLUG: AC plug\nDCPLUG: DC plug\nCRIMP: bare wire"@en , "物理ポート接続：\n\n- ACPLUG: AC プラグ\n- DCPLUG: DC プラグ\n- CRIMP: 裸線"@ja-JP , "The end-style treatment of the pipe port:\n\nBRAZED: Brazed. \nCOMPRESSION: Compression. \nFLANGED: Flanged. \nGROOVED: Grooved. \nOUTSIDESLEEVE: Outside Sleeve. \nSOLDERED: Soldered. \nSWEDGE: Swedge. \nTHREADED: Threaded. \nWELDED: Welded. \nOTHER: Another type of end-style has been applied.\nNONE: No end-style has been applied.\nUSERDEFINED: User-defined port connection type. \nNOTDEFINED: Undefined port connection type."@en ;
        rdfs:label             "接続タイプ"@ja-JP , "connectionType"@en ;
        schema:domainIncludes  <https://w3id.org/product/DistributionPort%2FAIRCONDITIONING> , <https://w3id.org/product/DistributionPort%2FCHEMICAL> , <https://w3id.org/product/DistributionPort%2FELECTRICAL> .

props:locationPriorityType
        a                      owl:DatatypeProperty ;
        rdfs:comment           "Identifies the predefined types of priority that can be assigned from which the type may be set where:\n\nHigh: action is required urgently.\nMedium: action can occur within a reasonable period of time.\nLow: action can occur when convenient."@en ;
        rdfs:label             "locationPriorityType"@en ;
        schema:domainIncludes  <https://w3id.org/product/ProjectOrder%2FMAINTENANCEWORKORDER> .

props:reliefPressure  a        owl:DatatypeProperty ;
        rdfs:comment           "The pressure at which the spring or weight in the valve is set to discharge fluid."@en , "バルブのバネやおもりが流体を放出する作動するときの圧力。"@ja-JP ;
        rdfs:label             "reliefPressure"@en , "リリーフ圧力"@ja-JP ;
        rdfs:range             <https://w3id.org/product/PressureMeasure> ;
        schema:domainIncludes  <https://w3id.org/product/Valve%2FPRESSURERELIEF> .

props:capacityPeople  a        owl:DatatypeProperty ;
        rdfs:comment           "Kapazität nach Anzahl der Personen, die maximal befördert werden können."@de-DE , "搬送要素の人数に関する容量。"@ja-JP , "Capacity of the transportation element measured in numbers of person."@en , "Capacité de transport de l'élément mesurée en nombre de personnes."@fr-FR ;
        rdfs:label             "Personenkapazität"@de-DE , "Capacité en nombre de personnes"@fr-FR , "搭乗人数定員"@ja-JP , "capacityPeople"@en ;
        rdfs:range             <https://w3id.org/product/CountMeasure> ;
        schema:domainIncludes  <https://w3id.org/product/TransportElement> .

props:screenDiameter  a        owl:DatatypeProperty ;
        rdfs:comment           "遮へい層の径、厚さ。"@ja-JP , "The diameter of the screen around a cable or bus segment (if present)."@en , "코어 부분 (있는 경우)의 측면에 지름."@ko-KR , "The diameter of the screen around a core segment (if present)."@en , "차폐 층의 직경, 두께."@ko-KR , "コア部分（存在する場合）の面の直径。"@ja-JP ;
        rdfs:label             "스크린 지름"@ko-KR , "screenDiameter"@en , "スクリーン径"@ja-JP , "실드 직경"@ko-KR , "シールド径"@ja-JP ;
        rdfs:range             <https://w3id.org/product/PositiveLengthMeasure> ;
        schema:domainIncludes  <https://w3id.org/product/CableSegment%2FCABLESEGMENT> , <https://w3id.org/product/CableSegment%2FCORESEGMENT> .

props:keyShape  a              owl:DatatypeProperty ;
        rdfs:comment           "If applicable, shape of the head's slot, e.g. 'Slot', 'Allen'"@en ;
        rdfs:label             "keyShape"@en ;
        rdfs:range             xsd:string ;
        schema:domainIncludes  <https://w3id.org/product/MechanicalFastener%2FBOLT> .

props:switchOperation
        a                      owl:DatatypeProperty ;
        rdfs:comment           "Indicates operation of emergency stop switch."@en , "緊急停止スイッチの操作を示す。"@ja-JP , "비상 정지 스위치의 조작을 보여준다."@ko-KR ;
        rdfs:label             "switchOperation"@en , "スイッチ操作"@ja-JP , "스위치 조작"@ko-KR ;
        schema:domainIncludes  <https://w3id.org/product/SwitchingDevice%2FEMERGENCYSTOP> .

props:toiletPanType  a         owl:DatatypeProperty ;
        rdfs:comment           "The property enumeration Pset_ToiletPanTypeEnum defines the types of toilet pan that may be specified within the property set Pset_Toilet:-\n\nSiphonic: \tToilet pan in which excrement is removed by siphonage induced by the flushing water.\nSquat: \tToilet pan with an elongated bowl installed with its top edge at or near floor level, so that the user has to squat.\nWashDown: \tToilet pan in which excrement is removed by the momentum of the flushing water.\nWashOut: \tA washdown toilet pan in which excrement falls first into a shallow water filled bowl."@en , "Pset_SanitaryMountingEnumは下記に列挙された便器タイプとして定義されます。\n\nサイホン式：流水を含むサイホンにより汚物が廃棄される便器\n和式：便器が床面か淵の高さと同じに配置された便器。使用者はしゃがまなければならない。\nウォッシュダウン式：勢いよく洗い流すことにより便器をきれいにします\n洗浄式便器：まず汚物が落ちその後、便器に水が流れます"@ja-JP ;
        rdfs:label             "toiletPanType"@en , "便器タイプ"@ja-JP ;
        schema:domainIncludes  <https://w3id.org/product/SanitaryTerminal%2FTOILETPAN> .

props:hoopBarPitch  a          owl:DatatypeProperty ;
        rdfs:comment           "The pitch length of the hoop bar."@en , "帯筋の間隔。"@ja-JP ;
        rdfs:label             "hoopBarPitch"@en , "帯筋間隔"@ja-JP ;
        rdfs:range             <https://w3id.org/product/PositiveLengthMeasure> ;
        schema:domainIncludes  <https://w3id.org/product/Column> .

props:couplingType  a          owl:DatatypeProperty ;
        rdfs:comment           "Defines the type coupling on the inlet of the breeching inlet."@en , "送水口入口のカップリングタイプ。"@ja-JP ;
        rdfs:label             "couplingType"@en , "カップリングタイプ"@ja-JP ;
        schema:domainIncludes  <https://w3id.org/product/FireSuppressionTerminal%2FBREECHINGINLET> .

props:pointOfContact  a        owl:DatatypeProperty ;
        rdfs:comment           "The organization that should be contacted for action under the terms of the warranty. Note that the role of the organization (manufacturer, supplier, installer etc.) is determined by the IfcActorRole attribute of IfcOrganization."@en ;
        rdfs:label             "pointOfContact"@en ;
        schema:domainIncludes  <https://w3id.org/product/Element> .

props:chargePressure  a        owl:DatatypeProperty ;
        rdfs:comment           "Nominal or design operating pressure of the tank."@en , "タンクの公称又は設計運転圧力"@ja-JP ;
        rdfs:label             "chargePressure"@en , "加圧力"@ja-JP ;
        rdfs:range             <https://w3id.org/product/PressureMeasure> ;
        schema:domainIncludes  <https://w3id.org/product/Tank%2FPRESSUREVESSEL> , <https://w3id.org/product/Tank%2FEXPANSION> .

props:coreBaseHeight  a        owl:DatatypeProperty ;
        rdfs:comment           "Core base height of the profile."@en ;
        rdfs:label             "coreBaseHeight"@en ;
        rdfs:range             <https://w3id.org/product/PositiveLengthMeasure> ;
        schema:domainIncludes  <https://w3id.org/product/ArbitraryProfileDefWithVoids> .

props:pressureGaugeType
        a                      owl:DatatypeProperty ;
        rdfs:comment           "Identifies the means by which pressure is displayed."@en , "圧力が表示される手段を識別する。"@ja-JP , "압력이 표시되는 방법을 확인한다."@ko-KR ;
        rdfs:label             "pressureGaugeType"@en , "圧力計タイプ"@ja-JP , "압력계 유형"@ko-KR ;
        schema:domainIncludes  <https://w3id.org/product/FlowInstrument%2FPRESSUREGAUGE> .

props:coreType  a              owl:DatatypeProperty ;
        rdfs:comment           "Identifies the way the core of the AirTerminal is constructed."@en , "取り付けられたターミナルのコアの定義方法（SHUTTERBLADE, CURVEDBLADE, REMOVABLE, REVERSIBLEなど）"@ja-JP , "Caractérise comment la partie centrale du terminal de ventilation est fabriquée."@fr-FR ;
        rdfs:label             "coreType"@en , "コア形式"@ja-JP , "TypePartieCentrale"@fr-FR ;
        schema:domainIncludes  <https://w3id.org/product/AirTerminal> .

props:shortTimei2tFunction
        a                      owl:DatatypeProperty ;
        rdfs:comment           "Applying short time i2t function. A flag indicating that the I2t short time function of the device is used. The value should be set to TRUE only if the I2t function  is explicitly selected for the device."@en ;
        rdfs:label             "shortTimei2tFunction"@en ;
        rdfs:range             xsd:boolean ;
        schema:domainIncludes  <https://w3id.org/product/ProtectiveDevice> .

props:dischargeType  a         owl:DatatypeProperty ;
        rdfs:comment           "Defines the type of connection at the fan discharge.\n\nDuct: Discharge into ductwork.\nScreen: Discharge into screen outlet.\nLouver: Discharge into a louver.\nDamper: Discharge into a damper."@en , "送風機出口の接続形式定義\nDuct：ダクトへの吐き出し\nScreen:SCREEN内への吐き出し\nLouver:ルーバーへの吐き出し"@ja-JP ;
        rdfs:label             "dischargeType"@en , "吐出形式"@ja-JP ;
        schema:domainIncludes  <https://w3id.org/product/Fan> .

props:airFlowRate  a           owl:DatatypeProperty ;
        rdfs:comment           "The actual airflow rate as designed."@en , "Air flow rate."@en , "Volumetric flow rate."@en , "体積風量"@ja-JP , "Volumetric air flow rate."@en , "Débit d'air volumique"@fr-FR , "送風量"@ja-JP ;
        rdfs:label             "airFlowRate"@en , "風量"@ja-JP , "Débit d'air"@fr-FR ;
        rdfs:range             <https://w3id.org/product/VolumetricFlowRateMeasure> ;
        schema:domainIncludes  <https://w3id.org/product/AirTerminal> , <https://w3id.org/product/CooledBeam%2FACTIVE> , <https://w3id.org/product/Damper> , <https://w3id.org/product/DuctSilencer> .

props:siteCoverageRatio
        a                      owl:DatatypeProperty ;
        rdfs:comment           "The ratio of the utilization,  TotalArea / BuildableArea, expressed as a maximum value. The ratio value may be used to derive BuildableArea."@en , "Grundflächenzahl als Verhältnis der bebaubaren Fläche zur Bruttogrundstücksfläche."@de-DE , "建築基準により最大となる、敷地面積(IfcElementQuantity)と建築面積(IfcBuildingのIfcElementQuantity)の比率。"@ja-JP , "TotalArea / BuildableArea로 표시되는 이용 가능한 비율의 최대값입니다."@ko-KR , "Valeur maximale de la surface constructible exprimée en ratio. La valeur du ratio peut être utilisée pour déterminer la surface constructible."@fr-FR ;
        rdfs:label             "建蔽率"@ja-JP , "건폐율"@ko-KR , "Grundflächenzahl"@de-DE , "siteCoverageRatio"@en , "RatioSurfaceConstructible"@fr-FR ;
        rdfs:range             <https://w3id.org/product/PositiveRatioMeasure> ;
        schema:domainIncludes  <https://w3id.org/product/Site> .

props:trapType  a              owl:DatatypeProperty ;
        rdfs:comment           "必要とされるタイプがセットされる防臭弁の定義されたタイプを確認してください。"@ja-JP , "Identifies the predefined types of waste trap used in combination with the floor trap from which the type required may be set."@en , "セットされる予定の防臭弁のあらかじめ定義されたタイプを確認します。"@ja-JP , "セットされる予定の床の防臭弁と組み合わせて使われる廃棄物の防臭弁のあらかじめ定義されたタイプの識別情報。"@ja-JP , "Identifies the predefined types of trap from which the type required may be set."@en ;
        rdfs:label             "防臭弁の種類"@ja-JP , "trapType"@en , "防臭弁種類"@ja-JP ;
        schema:domainIncludes  <https://w3id.org/product/WasteTerminal%2FGULLYTRAP> , <https://w3id.org/product/WasteTerminal%2FGULLYSUMP> , <https://w3id.org/product/WasteTerminal%2FFLOORTRAP> .

props:trippingCurveType
        a                      owl:DatatypeProperty ;
        rdfs:comment           "The type of tripping curve that is represented by the property set."@en , "動作特性曲線のタイプを指定。"@ja-JP , "동작 특성 곡선의 유형을 지정합니다."@ko-KR ;
        rdfs:label             "trippingCurveType"@en , "動作特性曲線のタイプ"@ja-JP , "동작 특성 곡선의 유형"@ko-KR ;
        schema:domainIncludes  <https://w3id.org/product/ProtectiveDevice> .

props:visibleLightReflectance
        a                      owl:DatatypeProperty ;
        rdfs:comment           "Fraction du rayonnement visible qui est réfléchi par la protection solaire sous incidence normale. Valeur sans unité."@fr-FR , "Fraction of the visible light that is reflected by the glazing at normal incidence. It is a value without unit."@en , "ガラスへ法線入射した可視光の反射率。単位の無い値。"@ja-JP , "Fraction du rayonnement visible qui est réfléchi par le vitrage sous incidence normale. Valeur sans unité."@fr-FR , "正射时被玻璃反射的可见光比例。无单位。"@zh-CN , "通常の入射における日除け装置により反射される可視光の比率。単位の無い数値。"@ja-JP , "German-description-12"@de-DE ;
        rdfs:label             "Reflexion du rayonnement visible"@fr-FR , "Reflektionsgrad für sichtbares Licht"@de-DE , "ReflexionVisible"@fr-FR , "可见光反射率"@zh-CN , "visibleLightReflectance"@en , "可視光反射率"@ja-JP ;
        rdfs:range             <https://w3id.org/product/NormalisedRatioMeasure> , <https://w3id.org/product/PositiveRatioMeasure> ;
        schema:domainIncludes  <https://w3id.org/product/Door> , <https://w3id.org/product/ShadingDevice> , <https://w3id.org/product/cWindow> .

props:beamCoolingCapacity
        a                      owl:DatatypeProperty ;
        rdfs:comment           "Cooling capacity of beam. This excludes cooling capacity of supply air."@en ;
        rdfs:label             "beamCoolingCapacity"@en ;
        schema:domainIncludes  <https://w3id.org/product/CooledBeam> .

props:lubricantPumpHeatGain
        a                      owl:DatatypeProperty ;
        rdfs:comment           "Lubricant pump heat gain."@en , "Gain thermique par lubrification de la pompe à chaleur."@fr-FR ;
        rdfs:label             "lubricantPumpHeatGain"@en , "GainThermiqueLubrifiantPompe"@fr-FR ;
        schema:domainIncludes  <https://w3id.org/product/Compressor> .

props:nominalEnergyConsumption
        a                      owl:DatatypeProperty ;
        rdfs:comment           "Nominal fuel consumption rate required to produce the total boiler heat output."@en , "ボイラ最大能力時の設計燃料消費量"@ja-JP , "Consommation nominale de combustible correspondant à la production nominale totale de la chaudière."@fr-FR ;
        rdfs:label             "nominalEnergyConsumption"@en , "設計エネルギー消費量"@ja-JP , "Consommation nominale d'energie"@fr-FR ;
        rdfs:range             <https://w3id.org/product/PowerMeasure> ;
        schema:domainIncludes  <https://w3id.org/product/Boiler> .

props:lossCoefficient
        a                      owl:DatatypeProperty ;
        rdfs:comment           "無次元数的な損失係数で、ある断面において、動圧に対する全圧損失の割合を表す流れ抵抗を計算するのに使われる。"@ja-JP , "Dimensionless loss coefficient used for calculating fluid resistance representing the ratio of total pressure loss to velocity pressure at a referenced cross-section."@en , "参照された断面での動圧に対する全圧損失の比を表わす流体抵抗の計算に使用される無次元の損失係数"@ja-JP ;
        rdfs:label             "lossCoefficient"@en , "損失係数"@ja-JP ;
        schema:domainIncludes  <https://w3id.org/product/PipeFitting> , <https://w3id.org/product/DuctSegment> , <https://w3id.org/product/DuctFitting> .

props:bendAngle  a             owl:DatatypeProperty ;
        rdfs:comment           "The change of direction of flow."@en , "流れの方向を変える"@ja-JP ;
        rdfs:label             "bendAngle"@en , "曲がり角度"@ja-JP ;
        rdfs:range             <https://w3id.org/product/PositivePlaneAngleMeasure> ;
        schema:domainIncludes  <https://w3id.org/product/PipeFitting%2FBEND> .

props:failPosition  a          owl:DatatypeProperty ;
        rdfs:comment           "Specifies the required fail-safe position of the actuator."@en , "要求されたアクチュエータのフェールセーフタイプを示す。"@ja-JP , "대체 기능으로 수동 조작이 제공되는지 (= TRUE) 여부 (= FALSE)를 확인한다. 수동으로 조작하는 액츄에이터의 경우는이 값을 기본값으로 FALSE로 설정해야하므로주의한다."@ko-KR ;
        rdfs:label             "failPosition"@en , "フェールセーフタイプ"@ja-JP , "재정 기능의 유무"@ko-KR ;
        schema:domainIncludes  <https://w3id.org/product/Actuator> .

props:terminationDate
        a                      owl:DatatypeProperty ;
        rdfs:comment           "Date on which the agreement terminates."@en ;
        rdfs:label             "terminationDate"@en ;
        rdfs:range             xsd:date ;
        schema:domainIncludes  <https://w3id.org/product/SpatialStructureElement> .

props:compressorEvaporatorPressureDrop
        a                      owl:DatatypeProperty ;
        rdfs:comment           "Pressure drop between the evaporator outlet and the compressor inlet."@en , "蒸発器出口と圧縮機入口間の圧力降下"@ja-JP ;
        rdfs:label             "compressorEvaporatorPressureDrop"@en , "圧縮機・蒸発器圧力降下"@ja-JP ;
        schema:domainIncludes  <https://w3id.org/product/Evaporator> .

props:numberOfCells  a         owl:DatatypeProperty ;
        rdfs:comment           "Number of cells in one cooling tower unit."@en ;
        rdfs:label             "numberOfCells"@en ;
        rdfs:range             xsd:int ;
        schema:domainIncludes  <https://w3id.org/product/CoolingTower> .

props:fan  a                   owl:DatatypeProperty ;
        rdfs:comment           "Indicates fan operation where True is on, False is off, and Unknown is automatic."@en ;
        rdfs:label             "fan"@en ;
        schema:domainIncludes  <https://w3id.org/product/UnitaryControlElement> .

props:nominalUA  a             owl:DatatypeProperty ;
        rdfs:comment           "Nominal UA value."@en , "Valeur nominale du coefficient de transmission thermique totale."@fr-FR ;
        rdfs:label             "nominalUA"@en , "UANominale"@fr-FR ;
        rdfs:range             xsd:decimal ;
        schema:domainIncludes  <https://w3id.org/product/Coil> .

props:flushRate  a             owl:DatatypeProperty ;
        rdfs:comment           "The minimum and maximum volume of water used at each flush. Where a single flush is used, the value of upper bound and lower bound should be equal. For a dual flush toilet, the lower bound should be used for the lesser flush rate and the upper bound for the greater flush rate. Where flush is achieved using mains pressure water through a flush valve, the value of upper and lower bound should be equal and should be the same as the flush rate property of the flush valve (see relevant valve property set). Alternatively, in this case, do not assert the flush rate property; refer to the flush rate of the flush valve."@en , "各フラッシュで使用される水量の最小値と最大値。単一フラッシュが使用されている場合、上下限値は同じ。デュアルフラッシュトイレについては、下限が低いフラッシュレート、上限に大きいフラッシュ率を使用する。ここで、洗浄はフラッシュバルブを通した水の水圧を用いて達成されるので、フラッシュレートとフラッシュバルブの上下限値と等しくなければなりません（関連バルブプロパティセットを参照してください）。また、この場合には、フラッシュレートのプロパティを設定しない。フラッシュバルブのフラッシュレートを参照。"@ja-JP ;
        rdfs:label             "flushRate"@en , "フラッシュレート"@ja-JP ;
        schema:domainIncludes  <https://w3id.org/product/SanitaryTerminal%2FCISTERN> .

props:nominalBodyDepth
        a                      owl:DatatypeProperty ;
        rdfs:comment           "Nominal or quoted length measured along the z-axis in the local coordinate system of the chamber of the gully trap."@en , "廃棄物の半径か局所座標系のZ軸に沿って測定された呼称もしくは積算された長さ。"@ja-JP , "溝防臭弁の半径か局所座標系のZ軸に沿って測定された呼称もしくは積算された長さ。"@ja-JP , "Nominal or quoted =length, measured along the z-axis of the local coordinate system of the object, of the body of the object."@en , "Nominal or quoted length measured along the z-axis in the local coordinate system of the chamber of the  trap."@en , "Nominal or quoted length measured along the z-axis in the local coordinate system of the waste."@en , "半径か局所座標系のZ軸に沿って測定された呼称もしくは積算された配管の長さ。"@ja-JP , "Nominal or quoted length measured along the z-axis in the local coordinate system of the drain."@en , "防臭弁の区画の半径か局所座標系のZ軸に沿って測定された呼称もしくは積算された長さ。"@ja-JP ;
        rdfs:label             "呼称躯体深さ"@ja-JP , "nominalBodyDepth"@en ;
        rdfs:range             <https://w3id.org/product/PositiveLengthMeasure> ;
        schema:domainIncludes  <https://w3id.org/product/WasteTerminal%2FGULLYTRAP> , <https://w3id.org/product/Interceptor> , <https://w3id.org/product/WasteTerminal%2FROOFDRAIN> , <https://w3id.org/product/WasteTerminal%2FFLOORWASTE> , <https://w3id.org/product/WasteTerminal%2FFLOORTRAP> .

props:totalPrimaryEnergyConsumption
        a                      owl:DatatypeProperty ;
        rdfs:comment           "Consommation d'énergie primaire utilisée, telle que définie dans les normes ISO21930:2007 [NDT : ou NF P01-010]"@fr-FR , "ISO21930 : 2007에서 정의된 에너지 사용량"@ko-KR , "Quantity of energy used as defined in ISO21930:2007."@en , "ISO21930:2007.で定義されているエネルギー量。"@ja-JP ;
        rdfs:label             "主なエネルギー消費の総量"@ja-JP , "ConsommationTotaleEnergiePrimaire"@fr-FR , "totalPrimaryEnergyConsumption"@en , "모든 차 에너지 소비"@ko-KR ;
        rdfs:range             <https://w3id.org/product/EnergyMeasure> ;
        schema:domainIncludes  <https://w3id.org/product/Element> .

props:spaceTemperatureMin
        a                      owl:DatatypeProperty ;
        rdfs:comment           "공간 또는 영역의 최저 온도 이용자 / 설계자의 관점에서 요구된다. 만약 여름철 또는 겨울철 실내 온도 요구가 주어지지 않는, 그것은 연중에, 그렇지 않으면 중간 분기별로 적용된다."@ko-KR , "Minimal temperature of the space or zone, that is required from user/designer view point. If no summer or winter space temperature requirements are given, it applies all year, otherwise for the intermediate period."@en , "Température minimale de l'espace ou de la zone spécifiée par l'usager ou le concepteur. Si les valeurs pour l'été et l'hiver ne sont pas connues, cette température s'applique toute l'année, sinon seulement en demi-saison."@fr-FR , "Minimale geforderte Raumtemperatur, die nicht unterschritten werden darf, gilt als ganzjährige Anforderung unabhängig vom Heizungs-, oder Kühlungsfall."@de-DE , "空間またはゾーンの最低温度。利用者/設計者の視点から要求される。もし夏季または冬季の室内温度要求が与えられないと、それは通年に、さもなければ中間季に適用される。"@ja-JP ;
        rdfs:label             "최저온도"@ko-KR , "最低室内温度"@ja-JP , "spaceTemperatureMin"@en , "Température minimale"@fr-FR , "Raumtemperatur Minimal"@de-DE ;
        rdfs:range             <https://w3id.org/product/ThermodynamicTemperatureMeasure> ;
        schema:domainIncludes  <https://w3id.org/product/cZone> , <https://w3id.org/product/cSpatialZone> , <https://w3id.org/product/Space> .

props:inertWastePerUnit
        a                      owl:DatatypeProperty ;
        rdfs:comment           "Quantity of inert waste generated"@en , "Quantité de déchets inertes générés [NDT : selon la norme NF P01-010]"@fr-FR , "生成された安定廃棄物の量。"@ja-JP , "불활성 폐기물 발생량"@ko-KR ;
        rdfs:label             "단위당 불황성 폐기물"@ko-KR , "DechetsInertesParUnite"@fr-FR , "inertWastePerUnit"@en , "単位あたり不活性廃棄物"@ja-JP ;
        rdfs:range             <https://w3id.org/product/MassMeasure> ;
        schema:domainIncludes  <https://w3id.org/product/Element> .

props:entranceLevel  a         owl:DatatypeProperty ;
        rdfs:comment           "Angabe, ob der Gebäudeeingang sich in diesem Geschoss befinded (WAHR), oder nicht (FALSCH)."@de-DE , "Indication si l'étage est au niveau d'une entrée (VRAI) ou non (FAUX)"@fr-FR , "Indication whether this building storey is an entrance level to the building (TRUE), or (FALSE) if otherwise."@en , "エントランスレベルかどうかを示すブーリアン値。"@ja-JP , "입구 레벨 여부를 나타내는 값"@ko-KR ;
        rdfs:label             "입구 레벨"@ko-KR , "Eingangsebene"@de-DE , "entranceLevel"@en , "エントランスレベル"@ja-JP , "NiveauEntrée"@fr-FR ;
        rdfs:range             xsd:boolean ;
        schema:domainIncludes  <https://w3id.org/product/BuildingStorey> .

props:defrostTemperatureEffectiveness
        a                      owl:DatatypeProperty ;
        rdfs:comment           "Temperature heat transfer effectiveness when defrosting is active."@en , "デフロスト作動時の温度熱交換効率"@ja-JP , "Efficacité thermique sensible lorsque le mode dégel est actif"@fr-FR ;
        rdfs:label             "defrostTemperatureEffectiveness"@en , "デフロスト温度効率"@ja-JP , "EfficacitéTemperatureDégel"@fr-FR ;
        schema:domainIncludes  <https://w3id.org/product/AirToAirHeatRecovery> .

props:sheathColors  a          owl:DatatypeProperty ;
        rdfs:comment           "Colour of the core (derived from IEC 60757). Note that the combined color 'GreenAndYellow' shall be used only as Protective Earth (PE) conductors according to the requirements of IEC 60446."@en , "コア色（IEC60757による）。緑と黄色の混合色の保護接地（PE）の導体は、IEC60446の要件に応じて注意して使用。"@ja-JP , "녹색과 노란색 혼합 색상의 보호 접지 (PE) 도체는 IEC60446의 요구에 따라주의하여 사용."@ko-KR ;
        rdfs:label             "sheathColors"@en , "シース色"@ja-JP , "코어 색"@ko-KR ;
        schema:domainIncludes  <https://w3id.org/product/CableSegment%2FCORESEGMENT> .

props:primaryEnergyConsumption
        a                      owl:DatatypeProperty ;
        rdfs:comment           "Boiler primary energy source consumption (i.e., the fuel consumed for changing the thermodynamic state of the fluid)."@en , "ボイラ一次エネルギ消費量（つまり流体の熱力学状態変更のために消費された燃料）"@ja-JP , "Consommation d'énergie primaire de la chaudière(c'est-à-dire le combustible consommé pour le changement d'état thermodynamique du fluide)."@fr-FR ;
        rdfs:label             "primaryEnergyConsumption"@en , "一次エネルギ消費量"@ja-JP , "ConsommationEnergiePrimaire"@fr-FR ;
        schema:domainIncludes  <https://w3id.org/product/Boiler> .

props:floorCovering  a         owl:DatatypeProperty ;
        rdfs:comment           "部屋の床材質または仕上げに関するラベル（識別情報）。このラベル名は部屋リスト情報や部屋情報表示の際に利用される。"@ja-JP , "Indication sur la nature du revêtement de sol […]. L'information sur le matériau est fournie en l'absence d'un objet de la classe IfcCovering (Type=FLOORING) avec sa propre représentation de forme et une assignation à un matériau. En cas d'incohérence, c'est le matériau assigné à l'instance de IfcCovering qui prime."@fr-FR , "Label to indicate the material or finish of the space flooring. The label is used for room book information and often displayed in room stamp.\n\nThe material information is provided in absence of an IfcCovering (type=FLOORING) object with own shape representation and material assignment. In case of inconsistency the material assigned to IfcCovering elements takes precedence."@en , "Angabe des Materials für den Bodenbelag. Diese Angabe wird im Raumbuch verwendet und oft im Raumstempel angezeigt.\n\nDie Materialangabe wird übernommen, wenn kein eigenes Bekleidungsobjekt (IfcCovering mit PredefinedType = FLOORING) für den Bodenbelag dem Raum zugeordnet ist. Bei Inkonsistenzen (wenn beides gegeben ist), hat die Materialangabe des zugeordneten Bekleidungsobjekts Priorität."@de-DE ;
        rdfs:label             "Bodenbelag"@de-DE , "床仕上げ"@ja-JP , "floorCovering"@en , "RevetementSol"@fr-FR ;
        rdfs:range             xsd:string ;
        schema:domainIncludes  <https://w3id.org/product/Space> .

props:nominalFrequency
        a                      owl:DatatypeProperty ;
        rdfs:comment           "The nominal frequency of the supply."@en , "電源の公称周波数。"@ja-JP , "전원 공칭 주파수."@ko-KR ;
        rdfs:label             "nominalFrequency"@en , "公称周波数"@ja-JP , "공칭 주파수"@ko-KR ;
        rdfs:range             <https://w3id.org/product/FrequencyMeasure> ;
        schema:domainIncludes  <https://w3id.org/product/ElectricFlowStorageDevice> .

props:warrantyContent
        a                      owl:DatatypeProperty ;
        rdfs:comment           "The content of the warranty."@en ;
        rdfs:label             "warrantyContent"@en ;
        rdfs:range             xsd:string ;
        schema:domainIncludes  <https://w3id.org/product/Element> .

props:contractualType
        a                      owl:DatatypeProperty ;
        rdfs:comment           "The contractual type of the work."@en ;
        rdfs:label             "contractualType"@en ;
        rdfs:range             xsd:string ;
        schema:domainIncludes  <https://w3id.org/product/ProjectOrder%2FWORKORDER> , <https://w3id.org/product/ProjectOrder%2FMAINTENANCEWORKORDER> .

props:baseThickness  a         owl:DatatypeProperty ;
        rdfs:comment           "ダクトスペース床面の厚さ。\n注：ダクトスペースの床は単層と仮定する"@ja-JP , "The thickness of the duct base construction\nNOTE: It is assumed that duct base will be constructed at a single thickness."@en , "The thickness of the chamber base construction.\nNOTE: It is assumed that chamber base will be constructed at a single thickness."@en , "덕트 공간 바닥의 두께 참고 : 덕트 공간의 바닥은 단층 가정"@ko-KR , "The thickness of the chamber base construction\nNOTE: It is assumed that chamber base will be constructed at a single thickness."@en ;
        rdfs:label             "baseThickness"@en , "바닥두께"@ko-KR , "基部の厚さ"@ja-JP , "床の厚さ"@ja-JP , "바닥의 두께"@ko-KR ;
        rdfs:range             <https://w3id.org/product/PositiveLengthMeasure> ;
        schema:domainIncludes  <https://w3id.org/product/DistributionChamberElement%2FMANHOLE> , <https://w3id.org/product/DistributionChamberElement%2FMETERCHAMBER> , <https://w3id.org/product/DistributionChamberElement%2FFORMEDDUCT> , <https://w3id.org/product/DistributionChamberElement%2FINSPECTIONCHAMBER> , <https://w3id.org/product/DistributionChamberElement%2FVALVECHAMBER> .

props:proportionalStress
        a                      owl:DatatypeProperty ;
        rdfs:comment           "A measure of the proportional stress of the material. It describes the stress before the first plastic deformation occurs and is commonly measured at a deformation of 0.01%."@en ;
        rdfs:label             "proportionalStress"@en ;
        rdfs:range             <https://w3id.org/product/PressureMeasure> ;
        schema:domainIncludes  <https://w3id.org/product/Material%2FSteel> .

props:numberOfSections
        a                      owl:DatatypeProperty ;
        rdfs:comment           "タンクの製作に使用されているセクションの数　既定は1つ　　注：全てのセクションは同サイズと考える"@ja-JP , "流れ方向で測定した垂直方向のセクションの数"@ja-JP , "タンクの製作に使用されているセクションの数\n注：全てのセクションは同サイズと考える"@ja-JP , "Number of sections used in the construction of the tank\n\nNote: All sections assumed to be the same size."@en , "Number of vertical sections, measured in the direction of flow."@en , "Number of sections used in the construction of the tank. Default is 1.\n\nNote: All sections assumed to be the same size."@en ;
        rdfs:label             "numberOfSections"@en , "セクションの数"@ja-JP ;
        rdfs:range             xsd:int ;
        schema:domainIncludes  <https://w3id.org/product/Tank> , <https://w3id.org/product/Tank%2FSECTIONAL> , <https://w3id.org/product/SpaceHeater> .

props:size  a                  owl:DatatypeProperty ;
        rdfs:comment           "The size of the connection to the valve (or to each connection for faucets, mixing valves, etc.)."@en , "弁（又は、水栓、混合弁等の接続）接続サイズ"@ja-JP ;
        rdfs:label             "size"@en , "サイズ"@ja-JP ;
        rdfs:range             <https://w3id.org/product/PositiveLengthMeasure> ;
        schema:domainIncludes  <https://w3id.org/product/Valve> .

props:sectionWidth  a          owl:DatatypeProperty ;
        rdfs:comment           "The width of a section used in the construction of the tank."@en , "タンクの製作に使用されているセクションの幅"@ja-JP ;
        rdfs:label             "sectionWidth"@en , "セクションの幅"@ja-JP ;
        rdfs:range             <https://w3id.org/product/PositiveLengthMeasure> ;
        schema:domainIncludes  <https://w3id.org/product/Tank%2FSECTIONAL> .

props:nominalSupplyVoltageOffset
        a                      owl:DatatypeProperty ;
        rdfs:comment           "The maximum and minimum allowed voltage of the supply e.g. boundaries of 380V/440V may be applied for a nominal voltage of 400V."@en , "電源の最大値と最小許容電圧。たとえば380V/440Vの境界は400Vの公称電圧に適用される。"@ja-JP , "전원 최대 및 최소 허용 전압 예 : 380V/440V 경계는 400V의 정격 전압에 적용된다."@ko-KR ;
        rdfs:label             "nominalSupplyVoltageOffset"@en , "オフセット公称電圧"@ja-JP , "옵셋 공칭 전압"@ko-KR ;
        schema:domainIncludes  <https://w3id.org/product/ElectricFlowStorageDevice> .

props:waterPressureDropCurve
        a                      owl:DatatypeProperty ;
        rdfs:comment           "Water pressure drop curve, pressure drop – flow rate curve, WaterPressureDrop = f(WaterflowRate)."@en , "Courbe de perte de charge hydraulique, courbe perte de charge - débit, perte de charge = f(DébitHydraulique)."@fr-FR ;
        rdfs:label             "waterPressureDropCurve"@en , "CourbePerteChargeHydraulique"@fr-FR ;
        schema:domainIncludes  <https://w3id.org/product/Coil> .

props:definedTemperature
        a                      owl:DatatypeProperty ;
        rdfs:comment           "この保護装置が定める温度・電流/時間-カーブに関連する周囲温度"@ja-JP , "The ambient temperature at which the thermal current/time-curve associated with this protection device is defined."@en , "이 보호 장치가 정한 온도 · 전류 / 시간 - 곡선과 관련된 주위 온도."@ko-KR , "이 보호 장치가 정한 온도 · 전류 / 시간 - 곡선과 관련된 주위 온도"@ko-KR , "この保護装置が定める温度・電流/時間-カーブに関連する周囲温度。"@ja-JP ;
        rdfs:label             "設定温度"@ja-JP , "definedTemperature"@en , "설정 온도"@ko-KR ;
        rdfs:range             <https://w3id.org/product/ThermodynamicTemperatureMeasure> ;
        schema:domainIncludes  <https://w3id.org/product/ProtectiveDeviceTrippingUnit%2FELECTROMAGNETIC> , <https://w3id.org/product/ProtectiveDeviceTrippingUnit%2FTHERMAL> .

props:isentropicEfficiency
        a                      owl:DatatypeProperty ;
        rdfs:comment           "Ratio of the work required for isentropic compression of the gas to work input to the compressor shaft."@en , "Rapport entre le travail requis pour une compression isentropique du gaz et le travail fourni à l'arbre du compresseur."@fr-FR ;
        rdfs:label             "isentropicEfficiency"@en , "RendementIsentropique"@fr-FR ;
        schema:domainIncludes  <https://w3id.org/product/Compressor> .

props:strengthGrade  a         owl:DatatypeProperty ;
        rdfs:comment           "Grade with respect to mechanical strength and stiffness."@en ;
        rdfs:label             "strengthGrade"@en ;
        rdfs:range             xsd:string ;
        schema:domainIncludes  <https://w3id.org/product/Material%2FWood> .

props:inletDiameter  a         owl:DatatypeProperty ;
        rdfs:comment           "The inlet diameter of the breeching inlet."@en , "入口の直径。"@ja-JP ;
        rdfs:label             "inletDiameter"@en , "入口口径"@ja-JP ;
        rdfs:range             <https://w3id.org/product/PositiveLengthMeasure> ;
        schema:domainIncludes  <https://w3id.org/product/FireSuppressionTerminal%2FBREECHINGINLET> .

props:nominalHeatingCapacity
        a                      owl:DatatypeProperty ;
        rdfs:comment           "Nominal heating capacity."@en ;
        rdfs:label             "nominalHeatingCapacity"@en ;
        rdfs:range             <https://w3id.org/product/PowerMeasure> ;
        schema:domainIncludes  <https://w3id.org/product/CooledBeam> .

props:coefficientOfPerformance
        a                      owl:DatatypeProperty ;
        rdfs:comment           "Coefficient of performance (COP)."@en , "Coefficient de performance (COP)."@fr-FR , "The Coefficient of performance (COP) is the ratio of heat removed to energy input. \nThe energy input may be obtained by multiplying \nPset_DistributionPortPHistoryGas.FlowRate on the 'Fuel' port of the IfcChiller by Pset_MaterialFuel.LowerHeatingValue.  \nThe IfcDistributionPort for fuel has an associated IfcMaterial with fuel properties and is assigned to an IfcPerformanceHistory object nested within this IfcPerformanceHistory object."@en , "Le coefficient de performance (COP) est le rapport entre l'énergie calorifique fournie sur l'énergie abosrbée.\nL'énergie fournie peut être obtenue en multipliant Pset_DistributionPortHistoryGas.flowRate depuis le port du IfcChiller par Pset_MaterialFuel.LowerHeatingValue.\nLe IfcDistributionPort pour combustible est associé à IfcMaterial pour les propriétés du combustible et est atrribué à l'objet IfcPerformanceHistory situé à l'intérieur même de cet objet IfcPerformanceHistory."@fr-FR ;
        rdfs:label             "coefficientOfPerformance"@en , "CoefficientDePerformance"@fr-FR , "CoefficientPerformance"@fr-FR ;
        schema:domainIncludes  <https://w3id.org/product/Compressor> , <https://w3id.org/product/Chiller> .

props:soundFrequency  a        owl:DatatypeProperty ;
        rdfs:comment           "List of nominal sound frequencies, correlated to the SoundPressure time series values (IfcTimeSeries.ListValues)"@en , "代表的な周波数リスト、時系列音圧値と関連する。（IfcTimeSeriesにリストされた値）"@ja-JP , "대표적인 주파수 목록 시계열 소리 圧値과 관련된다. (IfcTimeSeries에 나열된 값)"@ko-KR ;
        rdfs:label             "soundFrequency"@en , "音の周波数"@ja-JP , "소리의 주파수"@ko-KR ;
        schema:domainIncludes  <https://w3id.org/product/Annotation%2FSOUND> .

props:waterSumpTemperature
        a                      owl:DatatypeProperty ;
        rdfs:comment           "Water sump temperature."@en , "液温度　（水溜り温度）"@ja-JP ;
        rdfs:label             "waterSumpTemperature"@en , "液温度"@ja-JP ;
        schema:domainIncludes  <https://w3id.org/product/EvaporativeCooler> .

props:spaceHumidityWinter
        a                      owl:DatatypeProperty ;
        rdfs:comment           "Humidity of the space or zone for the cold (winter) period that is required from user/designer view point and provided as requirement for heating."@en , "공간이나 영역 추운 계절 (동절기) 실내 습도. 이용자 / 설계자의 관점에서 요구된다."@ko-KR , "空間またはゾーンの寒冷季(冬季)の室内湿度。利用者/設計者の視点から要求される。"@ja-JP , "Humidité relative minimale de l'espace ou de la zone  en été. Spécifiée par l'usager ou le concepteur et utilisée comme consigne pour le refroidissement."@fr-FR , "Geforderte Luftfeuchtigkeit für diesen Raum für die Auslegung der Heizung."@de-DE ;
        rdfs:label             "冬季室内湿度"@ja-JP , "겨울철실내 습도"@ko-KR , "Luftfeuchtigkeit Heizung"@de-DE , "spaceHumidityWinter"@en , "Humidité relative minimale en été"@fr-FR ;
        rdfs:range             <https://w3id.org/product/RatioMeasure> ;
        schema:domainIncludes  <https://w3id.org/product/cSpatialZone> , <https://w3id.org/product/cZone> , <https://w3id.org/product/Space> .

props:affectsSurroundings
        a                      owl:DatatypeProperty ;
        rdfs:comment           "Indicates wether the risk affects only to the person assigned to that task (FALSE) or if it can also affect to the people in the surroundings (TRUE).\n\nFor example, the process of painting would affect all the people in the vicinity of the process."@en ;
        rdfs:label             "affectsSurroundings"@en ;
        rdfs:range             xsd:boolean ;
        schema:domainIncludes  <https://w3id.org/product/Process> .

props:floorCoveringThickness
        a                      owl:DatatypeProperty ;
        rdfs:comment           "Epaisseur de la couche de matériau constituant le revêtement de sol. Cette information sur le matériau est fournie en l'absence d'un objet de la classe IfcCovering (Type=FLOORING) avec sa propre représentation de forme. En cas d'incohérence entre les paramètres géométriques de l'instance de IfcCovering et cette propriété, ce sont les paramètres géométriques qui priment."@fr-FR , "Thickness of the material layer(s) for the space flooring.  \n\nThe thickness information is provided in absence of an IfcCovering (type=FLOORING) object with own shape representation. In cases of inconsistency between the geometric parameters of an assigned IfcCovering and this attached property, the geometric parameters take precedence."@en , "部屋の床に関する材質層の厚さ。\n\n形状表現を持つIfcCovering(type=FLOORING)オブジェクトが存在しない場合に与えられる厚さ情報。IfcCoveringの幾何形状パラメータとこのプロパティ値が一致しない場合、幾何形状パラメータの値を優先する。"@ja-JP , "Angabe der Dicke der Materialschichten für den Bodenbelag. \n\nDer Dickenparameter wird übernommen, wenn kein eigenes Bekleidungsobjekt (IfcCovering mit PredefinedType = FLOORING) für den Bodenbelag dem Raum zugeordnet ist. Bei Inkonsistenzen (wenn beides gegeben ist), hat die Materialdicke des zugeordneten Bekleidungsobjekts Priorität."@de-DE ;
        rdfs:label             "床仕上げ材厚"@ja-JP , "floorCoveringThickness"@en , "Dicke des Bodenbelags"@de-DE , "Epaisseur du revêtement de sol"@fr-FR ;
        rdfs:range             <https://w3id.org/product/PositiveLengthMeasure> ;
        schema:domainIncludes  <https://w3id.org/product/Space> .

props:cisternCapacity
        a                      owl:DatatypeProperty ;
        rdfs:comment           "Volumetric capacity of the cistern"@en , "貯水タンクの体積容量。"@ja-JP ;
        rdfs:label             "cisternCapacity"@en , "貯水タンク容量"@ja-JP ;
        rdfs:range             <https://w3id.org/product/VolumeMeasure> ;
        schema:domainIncludes  <https://w3id.org/product/SanitaryTerminal%2FCISTERN> .

props:upperCurrent2  a         owl:DatatypeProperty ;
        rdfs:comment           "The current in [x In], indicating the upper current limit of the upper time/current curve of the I2t part of the L-function."@en , "[x In]の電流,電流をトリップするL関数のI2t部分は、上限時間/特性曲線よりも大きい電流を示す。"@ja-JP , "[x In] 전류 전류를 여행하는 L 함수 I2t 부분은 제한 시간 / 특성 곡선보다 큰 전류를 보여준다."@ko-KR ;
        rdfs:label             "upperCurrent2"@en , "上電流2"@ja-JP , "상전류2"@ko-KR ;
        rdfs:range             <https://w3id.org/product/ElectricCurrentMeasure> ;
        schema:domainIncludes  <https://w3id.org/product/ProtectiveDeviceTrippingUnit> .

props:receiverType  a          owl:DatatypeProperty ;
        rdfs:comment           "Indicates the type of receiver."@en , "受信機の形式を示す。"@ja-JP , "수신기의 형식을 보여준다."@ko-KR ;
        rdfs:label             "receiverType"@en , "受信機形式"@ja-JP , "수신기 형식"@ko-KR ;
        schema:domainIncludes  <https://w3id.org/product/AudioVisualAppliance%2FRECEIVER> .

props:heatingWaterFlowRate
        a                      owl:DatatypeProperty ;
        rdfs:comment           "Water flow rate for heating."@en ;
        rdfs:label             "heatingWaterFlowRate"@en ;
        schema:domainIncludes  <https://w3id.org/product/CooledBeam> .

props:mechanicalOperated
        a                      owl:DatatypeProperty ;
        rdfs:comment           "機械的操作が可能かどうかを示すブーリアン値。可能な場合TRUE、手動の場合FALSE。"@ja-JP , "Angabe, ob dieses Bauteil  mechanisch bewegt oder angetrieben wird (JA) oder manuell (NEIN). Diese Eigenschaft wird nur für beweglichen Sonnenschutz angegeben."@de-DE , "Indique si l'élément est actionné mécaniquement (VRAI) ou manuellement (FAUX)."@fr-FR , "Indication whether the element is operated machanically (TRUE) or not, i.e. manually  (FALSE)."@en ;
        rdfs:label             "機械的操作"@ja-JP , "mechanicalOperated"@en , "Actionné mécaniquement"@fr-FR , "Mechanisch"@de-DE ;
        rdfs:range             xsd:boolean ;
        schema:domainIncludes  <https://w3id.org/product/ShadingDevice> .

props:edgeDraft  a             owl:DatatypeProperty ;
        rdfs:comment           "Edge draft of the profile."@en ;
        rdfs:label             "edgeDraft"@en ;
        rdfs:range             <https://w3id.org/product/NonNegativeLengthMeasure> ;
        schema:domainIncludes  <https://w3id.org/product/ArbitraryProfileDefWithVoids> .

props:ceilingRAPlenum
        a                      owl:DatatypeProperty ;
        rdfs:comment           "Ceiling plenum used for return air or not. TRUE = Yes, FALSE = No."@en , "天井裏還気（リタンあり・なし）　TRUE=あり、FALSE=なし。"@ja-JP , "천장 환 기 (리탄있어 · 없음) TRUE = 있고 FALSE = 없음."@ko-KR ;
        rdfs:label             "ceilingRAPlenum"@en , "天井裏還気"@ja-JP , "천장환원주의"@ko-KR ;
        rdfs:range             xsd:boolean ;
        schema:domainIncludes  <https://w3id.org/product/Space> .

props:globalTradeItemNumber
        a                      owl:DatatypeProperty ;
        rdfs:comment           "The Global Trade Item Number (GTIN) is an identifier for trade items developed by GS1 (www.gs1.org)."@en ;
        rdfs:label             "globalTradeItemNumber"@en ;
        rdfs:range             xsd:string ;
        schema:domainIncludes  <https://w3id.org/product/Element> .

props:pressure  a              owl:DatatypeProperty ;
        rdfs:comment           "燃料の圧力。"@ja-JP , "The pressure of the fluid."@en , "流体の圧力。"@ja-JP , "The pressure of the fuel."@en ;
        rdfs:label             "pressure"@en , "圧力"@ja-JP ;
        schema:domainIncludes  <https://w3id.org/product/DistributionPort%2FGAS> , <https://w3id.org/product/DistributionPort%2FAIRCONDITIONING> , <https://w3id.org/product/DistributionPort%2FCHEMICAL> .

props:drivePowerLoss  a        owl:DatatypeProperty ;
        rdfs:comment           "Fan drive power losses associated with the type of connection between the motor and the fan wheel."@en , "ファン駆動力損失は、モータとファンホイールとの間の接続の種類に関連付けられている。"@ja-JP ;
        rdfs:label             "drivePowerLoss"@en , "駆動電力損失"@ja-JP ;
        schema:domainIncludes  <https://w3id.org/product/Fan> .

props:overallWidth  a          owl:DatatypeProperty ;
        rdfs:comment           "Overall width of the profile."@en ;
        rdfs:label             "overallWidth"@en ;
        rdfs:range             <https://w3id.org/product/PositiveLengthMeasure> ;
        schema:domainIncludes  <https://w3id.org/product/ArbitraryProfileDefWithVoids> , <https://w3id.org/product/ArbitraryClosedProfileDef> .

props:solarTransmittance
        a                      owl:DatatypeProperty ;
        rdfs:comment           "(Tsol)：日除けシステムを直接透過する日射の率。注： Asol + Rsol + Tsol = 1　という方程式が成り立つ。"@ja-JP , "(Tsol). Ratio du rayonnement solaire incident qui est transmis directement par le vitrage. Noter l'équation suivante : Asol + Rsol + Tsol = 1."@fr-FR , "(Tsol): The ratio of incident solar radiation that directly passes through a glazing system (also named τe). Note the following equation Asol + Rsol + Tsol = 1"@en , "（Tsol）ガラスを透過する日射の比率（τeとも表わされる）。以下の方程式に注意。Asol + Rsol + Tsol = 1"@ja-JP , "（Tsol）透过玻璃系统的太阳入射辐射的比率（也可用τe表示）。注：以下等式成立Asol + Rsol + Tsol = 1"@zh-CN , "(Tsol). Ratio du rayonnement solaire incident qui est transmis directement par la protection solaire. Noter l'équation suivante : Asol + Rsol + Tsol = 1."@fr-FR , "(Tsol): The ratio of incident solar radiation that directly passes through a shading system (also named τe). Note the following equation Asol + Rsol + Tsol = 1"@en , "German-description-15"@de-DE , "Transmittance at normal incidence (solar). Defines the fraction of solar radiation that passes through per unit area, perpendicular to the surface."@en ;
        rdfs:label             "太阳能透射率"@zh-CN , "日射透過率"@ja-JP , "Transmission du rayonnement solaire"@fr-FR , "TransmissionRayonnementSolaire"@fr-FR , "Strahlungstransmissionsgrad"@de-DE , "solarTransmittance"@en ;
        rdfs:range             <https://w3id.org/product/PositiveRatioMeasure> , <https://w3id.org/product/NormalisedRatioMeasure> ;
        schema:domainIncludes  <https://w3id.org/product/cWindow> , <https://w3id.org/product/ShadingDevice> , <https://w3id.org/product/Door> , <https://w3id.org/product/Material> .

props:z  a                     owl:DatatypeProperty ;
        rdfs:comment           "Measure z according to ISO 2553"@en ;
        rdfs:label             "z"@en ;
        rdfs:range             <https://w3id.org/product/PositiveLengthMeasure> ;
        schema:domainIncludes  <https://w3id.org/product/Fastener%2FWELD> .

props:anchorBoltProtrusionLength
        a                      owl:DatatypeProperty ;
        rdfs:comment           "The length of the protruding part of the anchor bolt."@en , "앵커 볼트의 돌출 부분의 길이"@ko-KR ;
        rdfs:label             "anchorBoltProtrusionLength"@en , "돌출부 길이"@ko-KR ;
        rdfs:range             <https://w3id.org/product/PositiveLengthMeasure> ;
        schema:domainIncludes  <https://w3id.org/product/MechanicalFastener%2FANCHORBOLT> .

props:auxiliaryEnergyConsumption
        a                      owl:DatatypeProperty ;
        rdfs:comment           "Boiler secondary energy source consumption (i.e., the electricity consumed by electrical devices such as fans and pumps)."@en , "ボイラ補助エネルギ消費量（つまりファンおよびポンプのような電気装置によって消費される電気）"@ja-JP , "Consommation d'énergie secondaire de la chaudière(c'est-à-dire l'électricité consommée pour les équipements électriques tels que ventilateurs et circulateurs)."@fr-FR ;
        rdfs:label             "auxiliaryEnergyConsumption"@en , "補助エネルギ消費量"@ja-JP , "ConsommationEnergieAuxiliaire"@fr-FR ;
        schema:domainIncludes  <https://w3id.org/product/Boiler> .

props:hasAntiStaticSurface
        a                      owl:DatatypeProperty ;
        rdfs:comment           "Indique si la finition est conçue pour être anti statique (VRAI) ou non (FAUX)."@fr-FR , "Indication whether the surface finish is designed to prevent electrostatic charge (TRUE) or not (FALSE)."@en , "表示表面处理是否设计为防静电的。"@zh-CN , "Angabe, ob der Bodenbelag eine antistatische Oberfläche hat (JA), oder nicht (NEIN)."@de-DE ;
        rdfs:label             "表面是否防静电"@zh-CN , "Antistatische Oberfläche"@de-DE , "Anti statique"@fr-FR , "hasAntiStaticSurface"@en ;
        rdfs:range             xsd:boolean ;
        schema:domainIncludes  <https://w3id.org/product/Covering%2FFLOORING> .

props:distanceBetweenComponentAxes
        a                      owl:DatatypeProperty ;
        rdfs:comment           "The distance between the axes of the components, measured along the ‘South’ edge of the slab."@en ;
        rdfs:label             "distanceBetweenComponentAxes"@en ;
        rdfs:range             <https://w3id.org/product/PositiveLengthMeasure> ;
        schema:domainIncludes  <https://w3id.org/product/Slab> .

props:maximumSupportedWeight
        a                      owl:DatatypeProperty ;
        rdfs:comment           "The maximum weight that can be carried by the vibration isolator."@en , "振動絶縁材で支えられる最高重量"@ja-JP ;
        rdfs:label             "maximumSupportedWeight"@en , "最高支持重量"@ja-JP ;
        rdfs:range             <https://w3id.org/product/MassMeasure> ;
        schema:domainIncludes  <https://w3id.org/product/VibrationIsolator> .

props:diagonalTrussLength
        a                      owl:DatatypeProperty ;
        rdfs:comment           "The overall length of the truss connector."@en , "トラス接続部材の全体の長さ。"@ja-JP , "트러스 연결 부재의 전체 길이"@ko-KR ;
        rdfs:label             "diagonalTrussLength"@en , "全体長さ"@ja-JP , "전체 길이"@ko-KR ;
        rdfs:range             <https://w3id.org/product/PositiveLengthMeasure> ;
        schema:domainIncludes  <https://w3id.org/product/DiscreteAccessory%2FDiagonal%20truss%20connector> .

props:fireSensorSetPoint
        a                      owl:DatatypeProperty ;
        rdfs:comment           "The temperature value to be sensed to indicate the presence of fire."@en , "炎の存在を示すために感知される温度値。"@ja-JP , "불꽃의 존재를 보여주기 위하여 감지되는 온도 값."@ko-KR ;
        rdfs:label             "fireSensorSetPoint"@en , "感知温度"@ja-JP , "감지 온도"@ko-KR ;
        rdfs:range             <https://w3id.org/product/ThermodynamicTemperatureMeasure> ;
        schema:domainIncludes  <https://w3id.org/product/Sensor%2FFIRESENSOR> .

props:isolatorStaticDeflection
        a                      owl:DatatypeProperty ;
        rdfs:comment           "Static deflection of the vibration isolator."@en , "振動絶縁材の静的たわみ"@ja-JP ;
        rdfs:label             "isolatorStaticDeflection"@en , "振動絶縁材静的たわみ"@ja-JP ;
        rdfs:range             <https://w3id.org/product/LengthMeasure> ;
        schema:domainIncludes  <https://w3id.org/product/VibrationIsolator> .

props:reinforcementStrengthClass
        a                      owl:DatatypeProperty ;
        rdfs:comment           "Classification of the reinforcement strength in accordance with the concrete design code which is applied in the project. The reinforcing strength class often combines strength and ductility."@en ;
        rdfs:label             "reinforcementStrengthClass"@en ;
        rdfs:range             xsd:string ;
        schema:domainIncludes  <https://w3id.org/product/BuildingElement> .

props:coverLength  a           owl:DatatypeProperty ;
        rdfs:comment           "The length measured along the x-axis in the local coordinate system or the radius (in the case of a circular shape in plan) of the cover of the waste."@en , "局所座標系のX軸に沿うか、半径（円状の形の場合）で測定された配管カバーの長さ。"@ja-JP , "局所座標系のX軸に沿うか、半径（円状の形の場合）で測定された防臭弁カバーの長さ。"@ja-JP , "局所座標系のX軸に沿うか、半径（円状の形の場合）で測定された溝防臭弁カバーの長さ。"@ja-JP , "The length measured along the x-axis in the local coordinate system or the radius (in the case of a circular shape in plan) of the cover of the trap."@en , "The length measured along the x-axis in the local coordinate system or the radius (in the case of a circular shape in plan) of the cover of the oil interceptor."@en , "The length measured along the x-axis in the local coordinate system or the radius (in the case of a circular shape in plan) of the cover of the drain."@en , "The length measured along the x-axis in the local coordinate system or the radius (in the case of a circular shape in plan) of the cover of the gully trap."@en ;
        rdfs:label             "カバーの長さ"@ja-JP , "coverLength"@en , "カバー長さ"@ja-JP ;
        rdfs:range             <https://w3id.org/product/PositiveLengthMeasure> ;
        schema:domainIncludes  <https://w3id.org/product/WasteTerminal%2FFLOORTRAP> , <https://w3id.org/product/WasteTerminal%2FROOFDRAIN> , <https://w3id.org/product/WasteTerminal%2FGULLYSUMP> , <https://w3id.org/product/Interceptor> , <https://w3id.org/product/WasteTerminal%2FFLOORWASTE> , <https://w3id.org/product/WasteTerminal%2FGULLYTRAP> .

props:soundScale  a            owl:DatatypeProperty ;
        rdfs:comment           "The reference sound scale.  \n\nDBA: Decibels in an A-weighted scale\nDBB: Decibels in an B-weighted scale\nDBC: Decibels in an C-weighted scale\nNC: Noise criteria\nNR: Noise rating"@en , "騒音の単位：\n\n- DBA: dB(A)\n- DBB: dB(B)\n- DBC:dB(C)\n- NC:騒音基準\n- NR:騒音評価"@ja-JP , "소음 단위. DBA : dB (A) DBB : dB (B) DBC : dB (C) NC : 소음 기준 NR : 소음 평가"@ko-KR ;
        rdfs:label             "soundScale"@en , "騒音の単位"@ja-JP , "소음단위"@ko-KR ;
        schema:domainIncludes  <https://w3id.org/product/Annotation%2FSOUND> .

props:throwLength  a           owl:DatatypeProperty ;
        rdfs:comment           "The horizontal or vertical axial distance an airstream travels after leaving an AirTerminal before the maximum stream velocity is reduced to a specified terminal velocity under isothermal conditions at the upper value of the AirFlowrateRange."@en , "ターミナルからの水平または垂直の到達距離\n流量範囲の最大値での吐き出し速度が設定された流速に減速するまでの上限値"@ja-JP , "La distance axiale horizontale ou verticale un jet d'air parcourt après avoir quitté un terminal de ventilation avant que la vittesse d'éjection maximale est réduite à une vitessedu terminal spécifique dans des conditions isothermes pour la valeur la plus élevée de la plage de débit d'air."@fr-FR ;
        rdfs:label             "throwLength"@en , "到達距離"@ja-JP , "Longueur de jet"@fr-FR ;
        rdfs:range             <https://w3id.org/product/LengthMeasure> ;
        schema:domainIncludes  <https://w3id.org/product/AirTerminal> .

props:nominalHeatRejectionRate
        a                      owl:DatatypeProperty ;
        rdfs:comment           "Sum of the refrigeration effect and the heat equivalent of the power input to the compressor."@en , "Somme de l'effet de réfrigération et de la chaleur équivalente à la puisssance absorbée par le compresseur."@fr-FR ;
        rdfs:label             "nominalHeatRejectionRate"@en , "CoefficientEvacuationNominaleChaleur"@fr-FR ;
        rdfs:range             <https://w3id.org/product/PowerMeasure> ;
        schema:domainIncludes  <https://w3id.org/product/Chiller> .

props:workTypeRequested
        a                      owl:DatatypeProperty ;
        rdfs:comment           "Work type requested in circumstances where there are categorizations of types of work task. It could be used to identify a remedial task, minor work task, electrical task etc."@en ;
        rdfs:label             "workTypeRequested"@en ;
        rdfs:range             xsd:string ;
        schema:domainIncludes  <https://w3id.org/product/ProjectOrder%2FWORKORDER> , <https://w3id.org/product/ProjectOrder%2FMAINTENANCEWORKORDER> .

props:ladderTrussHeight
        a                      owl:DatatypeProperty ;
        rdfs:comment           "The overall height of the truss connector."@en , "トラス接続部材の全体の高さ。"@ja-JP , "트러스 연결 부재의 전체 높이"@ko-KR ;
        rdfs:label             "ladderTrussHeight"@en , "全体高さ"@ja-JP , "전체 높이"@ko-KR ;
        rdfs:range             <https://w3id.org/product/PositiveLengthMeasure> ;
        schema:domainIncludes  <https://w3id.org/product/DiscreteAccessory%2FLadder%20truss%20connector> .

props:sensibleHeatRatio
        a                      owl:DatatypeProperty ;
        rdfs:comment           "Air-side sensible heat ratio, or fraction of sensible heat transfer to the total heat transfer."@en , "Ratio de chaleur sensible, ou fraction d'échange thermique sensible sur la chaleur thermique totale échangée."@fr-FR ;
        rdfs:label             "sensibleHeatRatio"@en , "RatioChaleurSensible"@fr-FR ;
        rdfs:range             <https://w3id.org/product/NormalisedRatioMeasure> ;
        schema:domainIncludes  <https://w3id.org/product/Coil> .

props:yDirectionLowerBarCount
        a                      owl:DatatypeProperty ;
        rdfs:comment           "The number of bars with Y direction lower bar."@en , "Y方向の下端筋本数。"@ja-JP ;
        rdfs:label             "yDirectionLowerBarCount"@en , "Y方向下端筋本数"@ja-JP ;
        rdfs:range             xsd:int ;
        schema:domainIncludes  <https://w3id.org/product/Footing> .

props:hasThermalInsulation
        a                      owl:DatatypeProperty ;
        rdfs:comment           "If TRUE, the air terminal has thermal insulation."@en , "ターミナルに断熱がある場合に真"@ja-JP , "Si VRAI, le terminal de ventilation possède une isolation thermique."@fr-FR ;
        rdfs:label             "hasThermalInsulation"@en , "断熱有無"@ja-JP , "PossèdeIsolationThermique"@fr-FR ;
        rdfs:range             xsd:boolean ;
        schema:domainIncludes  <https://w3id.org/product/AirTerminal> .

props:gasType  a               owl:DatatypeProperty ;
        rdfs:comment           "Defines the types of gas that may be specified."@en ;
        rdfs:label             "gasType"@en ;
        schema:domainIncludes  <https://w3id.org/product/FlowMeter%2FGASMETER> .

props:landID  a                owl:DatatypeProperty ;
        rdfs:comment           "Identification number assigned by the statutory registration authority to a land parcel."@en , "등기의 ID입니다."@ko-KR , "登記における識別番号。"@ja-JP , "Identifiant numérique de la parcelle attribué par une autorité [NDT : exemple : DGI]"@fr-FR ;
        rdfs:label             "敷地ID"@ja-JP , "IdParcelle"@fr-FR , "landID"@en , "부지 ID"@ko-KR ;
        rdfs:range             xsd:string ;
        schema:domainIncludes  <https://w3id.org/product/Site> .

props:dischargeDirection
        a                      owl:DatatypeProperty ;
        rdfs:comment           "Discharge direction of the air terminal.\n\nParallel: discharges parallel to mounting surface designed so that flow attaches to the surface.\nPerpendicular:  discharges away from mounting surface.\nAdjustable: both parallel and perpendicular discharge."@en , "ターミナルの吐き出し方向\n水平：取り付け面と水平に吐き出し\n垂直：取り付け面から離れた方向に吐き出し\n調節可能：水平・垂直方向両方に調整"@ja-JP , "Direction d'émission du terminal de ventilation.\n\nParallèle: émission parallèle à la surface de fixation conçu de façon à ce que le flux se colle à la surface.\nPerpendiculaire: émission s'éloignant de la surface de fixation.\nRéglable: émission parallèle et aussi s'éloignant de la surface de fixation."@fr-FR ;
        rdfs:label             "dischargeDirection"@en , "吐き出し方向"@ja-JP , "DirectionEmission"@fr-FR ;
        schema:domainIncludes  <https://w3id.org/product/AirTerminal> .

props:nosingLength  a          owl:DatatypeProperty ;
        rdfs:comment           "Horizontal distance from the front of the tread to the riser underneath. It is the overhang of the tread."@en , "German-description-6"@de-DE , "Longueur du nez de marche."@fr-FR , "Hauteur de passage (échappée) requise selon le Code en vigueur ou des spécifications additionnelles."@fr-FR , "踏板前边沿到下级踢板的水平距离，即踏板悬挑部分的长度。"@zh-CN ;
        rdfs:label             "LongueurNez"@fr-FR , "nosingLength"@en , "踏板前缘长度"@zh-CN , "Hauteur de passage requise"@fr-FR , "Überstand"@de-DE ;
        rdfs:range             <https://w3id.org/product/LengthMeasure> ;
        schema:domainIncludes  <https://w3id.org/product/Stair> , <https://w3id.org/product/StairFlight> .

props:aboveGround  a           owl:DatatypeProperty ;
        rdfs:comment           "Angabe, ob dieses Geschoss vollständig überhalb oberirdisch ist (WAHR), vollständig unterirdisch (FALSCH), oder teilweise unter- und überirdisch (UNKNOWN)."@de-DE , "이 건물 층이 지상 (TRUE), 지하 (FALSE), 일부 지하 부분 (UNKOWN) 여부를 나타내는 논리 값."@ko-KR , "この建物階が地上(TRUE)、地下(FALSE)、一部が地下部分(UNKOWN)かどうかを示すロジカル値。"@ja-JP , "Indication whether this building storey is fully above ground (TRUE), or below ground (FALSE), or partially above and below ground (UNKNOWN) - as in sloped terrain."@en , "Indication si l'étage est complètement au dessus du niveau du sol (VRAI), au dessous du niveau du sol (FAUX) ou partiellement enterré (INCONNU) comme dans le cas d'un terrain en pente."@fr-FR ;
        rdfs:label             "地上判別"@ja-JP , "AuDessusSol"@fr-FR , "Oberirdisches Geschoss"@de-DE , "aboveGround"@en , "지상 여부"@ko-KR ;
        rdfs:range             xsd:boolean ;
        schema:domainIncludes  <https://w3id.org/product/BuildingStorey> .

props:location1Local  a        owl:DatatypeProperty ;
        rdfs:comment           "Local x,y coordinates of the point in which Thickness1 is given"@en ;
        rdfs:label             "location1Local"@en ;
        schema:domainIncludes  <https://w3id.org/product/StructuralSurfaceMemberVarying> .

props:waistThickness  a        owl:DatatypeProperty ;
        rdfs:comment           "楼梯梯段的最小厚度，即踢板和踏板所成的内角到梯段斜面的垂线长度。该属性为预设值，若有冲突，应以从形状描述得到的值为准。"@zh-CN , "Epaisseur minimum de la volée mesurée perpendiculairement à la pente de la volée jusqu'au coin intérieur formé par la marche et la contremarche. C'est une valeur précalculée. En cas d'incohérence, c'est la valeur dérivée de la représentation de la forme qui prime."@fr-FR , "Minimum thickness of the stair flight, measured perpendicular to the slope of the flight to the inner corner of riser and tread. It is a pre-calculated value, in case of inconsistencies, the value derived from the shape representation shall take precedence."@en , "German-description-11"@de-DE ;
        rdfs:label             "Epaisseur"@fr-FR , "腰部厚度"@zh-CN , "waistThickness"@en , "minimale Dicke des Treppenplatte"@de-DE ;
        rdfs:range             <https://w3id.org/product/PositiveLengthMeasure> ;
        schema:domainIncludes  <https://w3id.org/product/StairFlight> , <https://w3id.org/product/Stair> .

props:depth  a                 owl:DatatypeProperty ;
        rdfs:comment           "La profondeur requise ou épaisseur de la réservation."@fr-FR , "ピット深さ。"@ja-JP , "구덩이 깊이"@ko-KR , "空間の厚さに対しての深さが提示されます。"@ja-JP , "溝の幅。"@ja-JP , "The depth of the pit."@en , "空构件的深度或厚度。"@zh-CN , "The depth of the trench."@en , "Geforderte Tiefe des Durchbruchs für eine Nische oder Aussparung. Wenn nicht angegeben, dann ist der geforderte Durchbruch eine Durchbruchsöffnung."@de-DE , "The requested depth or thickness of the provision for void."@en , "홈의 폭"@ko-KR ;
        rdfs:label             "深度"@zh-CN , "폭"@ko-KR , "Profondeur"@fr-FR , "深さ"@ja-JP , "깊이"@ko-KR , "Tiefe"@de-DE , "幅"@ja-JP , "depth"@en ;
        rdfs:range             <https://w3id.org/product/PositiveLengthMeasure> ;
        schema:domainIncludes  <https://w3id.org/product/DistributionChamberElement%2FINSPECTIONPIT> , <https://w3id.org/product/DistributionChamberElement%2FTRENCH> , <https://w3id.org/product/BuildingElementProxy%2FPROVISIONFORVOID> .

props:minimumSectionModulusZ
        a                      owl:DatatypeProperty ;
        rdfs:comment           "Bending resistance about the zs axis at the point with minimum ys ordinate. For example measured in mm³."@en ;
        rdfs:label             "minimumSectionModulusZ"@en ;
        rdfs:range             <https://w3id.org/product/SectionModulusMeasure> ;
        schema:domainIncludes  <https://w3id.org/product/ProfileDef> .

props:velocity  a              owl:DatatypeProperty ;
        rdfs:comment           "流体の速度。"@ja-JP , "The velocity of the fluid."@en ;
        rdfs:label             "速度"@ja-JP , "velocity"@en ;
        schema:domainIncludes  <https://w3id.org/product/DistributionPort%2FCHEMICAL> , <https://w3id.org/product/DistributionPort%2FAIRCONDITIONING> .

props:constructionMethod
        a                      owl:DatatypeProperty ;
        rdfs:comment           "The type of construction action to the building, the project deals with, e.g. new construction, renovation, refurbishment, etc."@en , "Designator for whether the concrete element is constructed on site or prefabricated. Allowed values are: 'In-Situ' vs 'Precast'."@en , "Angabe, ob dieses Betonbauteil als Ortbeton (\"In-Situ\") oder als Fertigteil (\"Precast\") ausgeführt werden soll."@de-DE , "Le type d'intervention sur le bâtiment : construction neuve, rénovation, réhabilitation, etc."@fr-FR , "공사의 유형. 예 : 신축 리노베이션 · 개장 등."@ko-KR , "工事におけるタイプ。例：新築・リノベーション・改装等。"@ja-JP , "Wesentliche Konstruktionsart des Gebäudes (Stahlbeton, Stahlbau, Holzfachwerk, etc.)"@de-DE ;
        rdfs:label             "constructionMethod"@en , "工事種別"@ja-JP , "Ausführung"@de-DE , "RisqueIncendieUsagePrincipal"@fr-FR , "공사 종류"@ko-KR , "Konstruktionsart"@de-DE ;
        rdfs:range             xsd:string ;
        schema:domainIncludes  <https://w3id.org/product/BuildingElement> , <https://w3id.org/product/Building> .

props:staggered  a             owl:DatatypeProperty ;
        rdfs:comment           "If intermittent weld, staggered or not"@en ;
        rdfs:label             "staggered"@en ;
        rdfs:range             xsd:boolean ;
        schema:domainIncludes  <https://w3id.org/product/Fastener%2FWELD> .

props:temperature  a           owl:DatatypeProperty ;
        rdfs:comment           "燃料の温度。"@ja-JP , "流体の温度。"@ja-JP , "Temperature of the fluid. For air this value represents the dry bulb temperature."@en , "Temperature of the fluid."@en , "Indicates the current measured temperature."@en , "The temperature of the fuel."@en ;
        rdfs:label             "温度"@ja-JP , "temperature"@en ;
        schema:domainIncludes  <https://w3id.org/product/DistributionPort%2FGAS> , <https://w3id.org/product/UnitaryControlElement> , <https://w3id.org/product/DistributionPort%2FAIRCONDITIONING> , <https://w3id.org/product/DistributionPort%2FCHEMICAL> .

props:roadVisibleDistanceRight
        a                      owl:DatatypeProperty ;
        rdfs:comment           "Distance visible to the right of the access."@en , "Distance de visibilité à la droite de l'accès."@fr-FR , "右側の経路に可視出来る距離。"@ja-JP ;
        rdfs:label             "roadVisibleDistanceRight"@en , "DistanceVisibiliteCoteDroit"@fr-FR , "右側道路可視距離"@ja-JP ;
        rdfs:range             <https://w3id.org/product/PositiveLengthMeasure> ;
        schema:domainIncludes  <https://w3id.org/product/Annotation%2FLineOfSight> .

props:lightingDiversity
        a                      owl:DatatypeProperty ;
        rdfs:comment           "조명 부하 계수."@ko-KR , "Lighting diversity."@en , "조명 부하 계수"@ko-KR , "照明負荷係数。"@ja-JP ;
        rdfs:label             "조명 부하계수"@ko-KR , "照明負荷係数"@ja-JP , "lightingDiversity"@en , "조명부하계수"@ko-KR ;
        rdfs:range             <https://w3id.org/product/PositiveRatioMeasure> ;
        schema:domainIncludes  <https://w3id.org/product/SpatialZone> , <https://w3id.org/product/Space> , <https://w3id.org/product/Zone> , <https://w3id.org/product/SpatialElement> .

props:clearDepth  a            owl:DatatypeProperty ;
        rdfs:comment           "덕트 공간의 깊이"@ko-KR , "Profondeur de l'ascenseur. Elle indique la distance entre la face intérieure de la porte et la face opposée de la cabine de l'ascenseur. Cette propriété est donnée en complément de la représentation de la forme de l'élément et des paramètres géométriques qui la déterminent. En cas d'incohérence entre ces paramètres géométriques et cette propriété, ce sont les paramètres géométriques qui priment."@fr-FR , "ジヤンクションボックスにケーブルを収められる深さ。"@ja-JP , "Clear unobstructed depth available for cable inclusion within the junction box."@en , "지얀 섹션 상자에 케이블을 거둘 깊이."@ko-KR , "ダクトスペースの深さ。"@ja-JP , "The depth of the formed space in the duct."@en , "The clear depth of the culvert."@en , "オブジェクト（エレベータ）の奥行き。エレベータドアの内部表面から、反対側の表面までの距離を示す。\n形状表現は、Shape representation（IFCの幾何形状表現）およびそこで設定されている幾何形状パラメータにより与えられる。もし、幾何形状パラメータと形状プロパティ情報が一致しない場合は、形状パラメータの値を優先する。"@ja-JP , "Clear depth of the object (elevator). It indicates the distance from the inner surface of the elevator door to the opposite surface of the elevator car. \nThe shape information is provided in addition to the shape representation and the geometric parameters used within. In cases of inconsistency between the geometric parameters and the shape properties, provided in the attached property, the geometric parameters take precedence."@en , "暗渠管の許容(安全)深さ"@ja-JP ;
        rdfs:label             "許容深さ"@ja-JP , "깊이"@ko-KR , "clearDepth"@en , "明確な深さ"@ja-JP , "深さ"@ja-JP , "奥行き"@ja-JP , "명확한 깊이"@ko-KR , "Profondeur de passage"@fr-FR ;
        rdfs:range             <https://w3id.org/product/PositiveLengthMeasure> , <https://w3id.org/product/LengthMeasure> ;
        schema:domainIncludes  <https://w3id.org/product/PipeSegment%2FCULVERT> , <https://w3id.org/product/DistributionChamberElement%2FFORMEDDUCT> , <https://w3id.org/product/TransportElement%2FELEVATOR> , <https://w3id.org/product/JunctionBox> .

props:electricGeneratorEfficiency
        a                      owl:DatatypeProperty ;
        rdfs:comment           "The ratio of output capacity to intake capacity."@en , "出力容量と入力容量の比率。"@ja-JP , "출력 용량을 입력 용량의 비율"@ko-KR ;
        rdfs:label             "electricGeneratorEfficiency"@en , "発電効率"@ja-JP , "발전 효율"@ko-KR ;
        rdfs:range             <https://w3id.org/product/PositiveRatioMeasure> ;
        schema:domainIncludes  <https://w3id.org/product/ElectricGenerator> .

props:numberOfCompartments
        a                      owl:DatatypeProperty ;
        rdfs:comment           "The number of separate internal compartments within the trunking."@en , "管の区別される内部区画の個数。"@ja-JP , "관 구분되는 내부 파티션 개수"@ko-KR ;
        rdfs:label             "numberOfCompartments"@en , "区画数"@ja-JP , "구획 수"@ko-KR ;
        rdfs:range             xsd:int ;
        schema:domainIncludes  <https://w3id.org/product/CableCarrierSegment%2FCABLETRUNKINGSEGMENT> .

props:direction  a             owl:DatatypeProperty ;
        rdfs:comment           "Indicates sensed direction for sensors capturing magnitude and direction measured from True North (0 degrees) in a clockwise direction."@en ;
        rdfs:label             "direction"@en ;
        schema:domainIncludes  <https://w3id.org/product/Sensor> .

props:solarHeatGainTransmittance
        a                      owl:DatatypeProperty ;
        rdfs:comment           "（SHGC）导致室内取得热量的入射太阳辐射比率，该值为透射太阳辐射（Tsol或τe）与分配到室内的吸收太阳辐射（qi）的和。SHGC也被称为g值（g = τe + qi）。"@zh-CN , "(SHGC):室内の熱利得の原因となる日射の比率。ガラスの透過分(Tsol or τe)と吸収分の内、室内側(qi)への分配分の和。SHGCは、g値（g = τe + qi）としても参照される。"@ja-JP , "(SHGC): The ratio of incident solar radiation that contributes to the heat gain of the interior, it is the solar radiation that directly passes (Tsol or τe) plus the part of the absorbed radiation that is distributed to the interior (qi). The SHGC is refered to also as g-value (g = τe + qi)."@en , "German-description-16"@de-DE , "(SHGC): Ratio du rayonnement solaire incident qui contribue aux apports solaires récupérés. Rayonnemment transmis directement (Tsol ou Te), plus la part de rayonnement absorbé restitué à l'intérieur (qi). Le SHGC est également appelé valeur-g (g = Te + qi)."@fr-FR ;
        rdfs:label             "太阳能得热系数"@zh-CN , "solarHeatGainTransmittance"@en , "ApportsSolaires"@fr-FR , "Gesamtenergiedurchlassgrad"@de-DE , "透過太陽熱利得係数"@ja-JP ;
        rdfs:range             <https://w3id.org/product/NormalisedRatioMeasure> ;
        schema:domainIncludes  <https://w3id.org/product/Door> , <https://w3id.org/product/cWindow> .

props:frameType  a             owl:DatatypeProperty ;
        rdfs:comment           "The type of frame used by the damper (e.g., Standard, Single Flange, Single Reversed Flange, Double Flange, etc.)."@en ;
        rdfs:label             "frameType"@en ;
        rdfs:range             xsd:string ;
        schema:domainIncludes  <https://w3id.org/product/Damper> .

props:lampCompensationType
        a                      owl:DatatypeProperty ;
        rdfs:comment           "Identifies the form of compensation used for power factor correction and radio suppression."@en , "力率の改善と高調波の抑制のために使用される補正"@ja-JP ;
        rdfs:label             "lampCompensationType"@en , "ランプ補正"@ja-JP , "램프보정"@ko-KR ;
        schema:domainIncludes  <https://w3id.org/product/Lamp> .

props:standardFixingPlateDepth
        a                      owl:DatatypeProperty ;
        rdfs:comment           "The depth of the standard fixing plate."@en , "標準的な固定プレートの成。"@ja-JP , "표준 고정 플레이트 구성"@ko-KR ;
        rdfs:label             "standardFixingPlateDepth"@en , "成"@ja-JP , "구성"@ko-KR ;
        rdfs:range             <https://w3id.org/product/PositiveLengthMeasure> ;
        schema:domainIncludes  <https://w3id.org/product/DiscreteAccessory%2FStandard%20fixing%20plate> .

props:hasCover  a              owl:DatatypeProperty ;
        rdfs:comment           "Indication of whether the cable tray has a cover (=TRUE) or not (= FALSE). By default, this value should be set to FALSE.."@en , "カバー付かどうか。"@ja-JP , "커버 유무"@ko-KR ;
        rdfs:label             "hasCover"@en , "カバー"@ja-JP , "커버"@ko-KR ;
        rdfs:range             xsd:boolean ;
        schema:domainIncludes  <https://w3id.org/product/CableCarrierSegment%2FCABLETRAYSEGMENT> .

props:shipMethod  a            owl:DatatypeProperty ;
        rdfs:comment           "Method of shipping that will be used for goods or services."@en ;
        rdfs:label             "shipMethod"@en ;
        rdfs:range             xsd:string ;
        schema:domainIncludes  <https://w3id.org/product/ProjectOrder%2FPURCHASEORDER> .

props:wireLoopBasePlateLength
        a                      owl:DatatypeProperty ;
        rdfs:comment           "The length of the base plate."@en , "ベースプレートの長さ。"@ja-JP , "플레이트 길이"@ko-KR ;
        rdfs:label             "wireLoopBasePlateLength"@en , "ベースプレート長さ"@ja-JP , "플레이트 길이"@ko-KR ;
        rdfs:range             <https://w3id.org/product/PositiveLengthMeasure> ;
        schema:domainIncludes  <https://w3id.org/product/DiscreteAccessory%2FWire%20loop> .

props:switchUsage  a           owl:DatatypeProperty ;
        rdfs:comment           "A list of the available usages for toggle switches from which that required may be selected."@en , "A list of the available usages for selector switches from which that required may be selected."@en , "選択が必要となる、切替えスイッチの使用法の一覧リスト。"@ja-JP , "選択が必要となる、トグルスイッチの使用法の一覧リスト。"@ja-JP , "선택이 필요한 토글 스위치 사용목록"@ko-KR , "전환스위치 사용 목록"@ko-KR ;
        rdfs:label             "スイッチの使用法"@ja-JP , "스위치 사용"@ko-KR , "switchUsage"@en ;
        schema:domainIncludes  <https://w3id.org/product/SwitchingDevice%2FTOGGLESWITCH> , <https://w3id.org/product/SwitchingDevice%2FSELECTORSWITCH> .

props:shortCircuit1PoleMinimumState
        a                      owl:DatatypeProperty ;
        rdfs:comment           "Minimum 1 pole short circuit current provided at the point of supply i.e. the fault between 1 phase and N."@en , "電源供給時点の点1相とN間の1極最小短絡電流。"@ja-JP , "전원 공급 시점 점 1 단계와 N 사이의 1 극 최소 단락 전류."@ko-KR ;
        rdfs:label             "shortCircuit1PoleMinimumState"@en , "1極最小短絡電流"@ja-JP , "1 극 최소 단락 전류"@ko-KR ;
        rdfs:range             <https://w3id.org/product/ElectricCurrentMeasure> ;
        schema:domainIncludes  <https://w3id.org/product/ElectricFlowStorageDevice> .

props:totalEffectiveness
        a                      owl:DatatypeProperty ;
        rdfs:comment           "Total heat transfer effectiveness: The ratio of heat transfer to the maximum possible heat transfer."@en , "全熱効率\n最大可能熱交換に対する熱交換の比率"@ja-JP , "Rendement thermique: rapport entre la chaleur effective échangée et l'échange maximum possible."@fr-FR ;
        rdfs:label             "totalEffectiveness"@en , "全熱効率"@ja-JP , "Rendement thermique"@fr-FR ;
        schema:domainIncludes  <https://w3id.org/product/AirToAirHeatRecovery> .

props:nominalPowerConsumption
        a                      owl:DatatypeProperty ;
        rdfs:comment           "Nominal total power consumption."@en , "Puissance de consommation totale nominale."@fr-FR ;
        rdfs:label             "nominalPowerConsumption"@en , "ConsommationPuissanceNominale"@fr-FR ;
        rdfs:range             <https://w3id.org/product/PowerMeasure> ;
        schema:domainIncludes  <https://w3id.org/product/Chiller> .

props:latentCoolingCapacity
        a                      owl:DatatypeProperty ;
        rdfs:comment           "Latent cooling capacity."@en , "潜熱冷却能力"@ja-JP ;
        rdfs:label             "latentCoolingCapacity"@en , "潜熱冷却能力"@ja-JP ;
        rdfs:range             <https://w3id.org/product/PowerMeasure> ;
        schema:domainIncludes  <https://w3id.org/product/UnitaryEquipment%2FAIRCONDITIONINGUNIT> .

props:longInsideCenterTopBarPitch
        a                      owl:DatatypeProperty ;
        rdfs:comment           "The pitch length of the long inside center top bar."@en , "長辺方向・柱間帯・上端中央の鉄筋間隔。"@ja-JP ;
        rdfs:label             "longInsideCenterTopBarPitch"@en , "長辺・柱列帯・上端中央ピッチ"@ja-JP ;
        rdfs:range             <https://w3id.org/product/PositiveLengthMeasure> ;
        schema:domainIncludes  <https://w3id.org/product/Slab> .

props:nominalMediaSurfaceVelocity
        a                      owl:DatatypeProperty ;
        rdfs:comment           "Average fluid velocity at the media surface."@en ;
        rdfs:label             "nominalMediaSurfaceVelocity"@en ;
        rdfs:range             <https://w3id.org/product/LinearVelocityMeasure> ;
        schema:domainIncludes  <https://w3id.org/product/Filter> .

props:coilFaceArea  a          owl:DatatypeProperty ;
        rdfs:comment           "Coil face area in the direction against air the flow."@en , "Surface d'échange de la batterie dans la direction contraire du jet."@fr-FR ;
        rdfs:label             "coilFaceArea"@en , "SurfaceEchangeBatterie"@fr-FR ;
        rdfs:range             <https://w3id.org/product/AreaMeasure> ;
        schema:domainIncludes  <https://w3id.org/product/Coil> .

props:airFlowLeakage  a        owl:DatatypeProperty ;
        rdfs:comment           "Volumetric leakage flow rate."@en , "体積漏れ流量"@ja-JP ;
        rdfs:label             "airFlowLeakage"@en , "漏れ量"@ja-JP ;
        schema:domainIncludes  <https://w3id.org/product/DuctFitting> .

props:rotationSpeed  a         owl:DatatypeProperty ;
        rdfs:comment           "Pump rotational speed."@en , "ポンプ回転速度"@ja-JP ;
        rdfs:label             "rotationSpeed"@en , "回転速度"@ja-JP ;
        schema:domainIncludes  <https://w3id.org/product/Pump> .

props:flammableStorage
        a                      owl:DatatypeProperty ;
        rdfs:comment           "空間が可燃物(建築基準を管理することによりそのように考慮される)の倉庫として使われることを意図されているかどうかを示すブーリアン値。(TRUE)はい、(FALSE)いいえ。"@ja-JP , "Indique si l'espace est destiné au stockage de matières inflammables (considérées comme telles par le Code de la Construction en vigueur). (VRAI) signifie oui, (FAUX) sinon."@fr-FR , "Indication whether the space is intended to serve as a storage of flammable material (which is regarded as such by the presiding building code. (TRUE) indicates yes, (FALSE) otherwise."@en , "Angabe, ob der Raum zur Lagerung der Produktion von brennbaren Stoffen genutzt wird (WHAHR) oder nicht (FALSCH). Die Angabe erfolgt nach der nationalen oder regionalen Brandschutzverordnung."@de-DE , "공간이 가연물 (건축 기준을 관리함으로써 그렇게 여겨지는)의 창고로 사용되는 것을 의도하고 있는지 여부를 나타내는 부울 값입니다. (TRUE) 예 (FALSE) 아니오. \"이 물체가 화재의 경우 출구로 사용되도록 설계되었는지 여부를 나타내는  (TRUE) 예 (FALSE) 아니오 값"@ko-KR ;
        rdfs:label             "Lagerung brennbarer Stoffe"@de-DE , "flammableStorage"@en , "可燃物保管区分"@ja-JP , "StockageCombustible"@fr-FR , "가연성 물질 창고"@ko-KR ;
        rdfs:range             xsd:boolean ;
        schema:domainIncludes  <https://w3id.org/product/cZone> , <https://w3id.org/product/Space> , <https://w3id.org/product/cSpatialZone> .

props:secondaryFrequency
        a                      owl:DatatypeProperty ;
        rdfs:comment           "The frequency that has been transformed and is running out of the transformer on the secondary side."@en , "変圧器の2次側に出力される周波数。"@ja-JP , "변압기 2 차 측에 전송되는 주파수."@ko-KR ;
        rdfs:label             "secondaryFrequency"@en , "第2周波数"@ja-JP , "제 2 주파수"@ko-KR ;
        rdfs:range             <https://w3id.org/product/FrequencyMeasure> ;
        schema:domainIncludes  <https://w3id.org/product/Transformer> .

props:effectivenessTable
        a                      owl:DatatypeProperty ;
        rdfs:comment           "Total heat transfer effectiveness curve as a function of the primary air flow rate."@en ;
        rdfs:label             "effectivenessTable"@en ;
        schema:domainIncludes  <https://w3id.org/product/EvaporativeCooler> .

props:signalTime  a            owl:DatatypeProperty ;
        rdfs:comment           "Time factor used for integral and running average controllers."@en , "시간 요소는 INTEGRAL (적분)과 AVERAGE ((이동) 평균) 컨트롤러에 사용됨"@ko-KR ;
        rdfs:label             "signalTime"@en , "시간 요소"@ko-KR ;
        rdfs:range             <https://w3id.org/product/TimeMeasure> ;
        schema:domainIncludes  <https://w3id.org/product/Controller%2FFLOATING> .

props:impuritiesContent
        a                      owl:DatatypeProperty ;
        rdfs:comment           "Fraction of impurities such as dust to the total amount of water. This is measured in weight of impurities per weight of water and is therefore unitless."@en ;
        rdfs:label             "impuritiesContent"@en ;
        rdfs:range             <https://w3id.org/product/NormalisedRatioMeasure> ;
        schema:domainIncludes  <https://w3id.org/product/Material> .

props:baseMaterial  a          owl:DatatypeProperty ;
        rdfs:comment           "The material from which the base of the chamber is constructed.\nNOTE: It is assumed that chamber base will be constructed of a single material."@en , "덕트 공간 바닥의 재질 참고 : 덕트 공간의 바닥은 단층 가정"@ko-KR , "ダクトスペース床面の材質。\n注：ダクトスペースの床は単層と仮定する"@ja-JP ;
        rdfs:label             "바닥의 ​​재질"@ko-KR , "床の材質"@ja-JP , "baseMaterial"@en , "바닥의 재질"@ko-KR ;
        schema:domainIncludes  <https://w3id.org/product/DistributionChamberElement%2FMETERCHAMBER> , <https://w3id.org/product/DistributionChamberElement%2FMANHOLE> , <https://w3id.org/product/DistributionChamberElement%2FINSPECTIONCHAMBER> , <https://w3id.org/product/DistributionChamberElement%2FVALVECHAMBER> .

props:waterFoulingResistance
        a                      owl:DatatypeProperty ;
        rdfs:comment           "水／空気面の汚れ抵抗"@ja-JP , "Fouling resistance on water/air side."@en ;
        rdfs:label             "水側汚れ抵抗"@ja-JP , "waterFoulingResistance"@en ;
        schema:domainIncludes  <https://w3id.org/product/Evaporator> , <https://w3id.org/product/Condenser> .

props:powerState  a            owl:DatatypeProperty ;
        rdfs:comment           "Indicates the power state of the device where True is on and False is off."@en , "機器の電源オンオフの時間ごとの状態を示す。"@ja-JP ;
        rdfs:label             "powerState"@en , "電源状態"@ja-JP ;
        schema:domainIncludes  <https://w3id.org/product/ElectricAppliance> , <https://w3id.org/product/CommunicationsAppliance> , <https://w3id.org/product/AudioVisualAppliance> .

props:iCM60947  a              owl:DatatypeProperty ;
        rdfs:comment           "IEC의 60947 시리즈를 기반으로 테스트 배선 차단기 또는 모터 보호 장치를위한 만드는 능력 [A]. \""@ko-KR , "IECの60947シリーズに基づいてテストした配線遮断機またはモータ保護装置のためので作る能力[A]。"@ja-JP , "IEC의 60947 시리즈를 기반으로 테스트 회로 차단 기나 모터 보호 장치의 능력 [A]."@ko-KR , "IECの60947シリーズに基づいてテストされた回路遮断機またはモータ保護装置の能力[A]。"@ja-JP , "The making capacity in [A] for a circuit breaker or motor protection device tested in accordance with the IEC 60947 series."@en ;
        rdfs:label             "iCM60947"@en , "ICM60947"@ja-JP , "ICM60947"@ko-KR ;
        rdfs:range             <https://w3id.org/product/ElectricCurrentMeasure> ;
        schema:domainIncludes  <https://w3id.org/product/ProtectiveDevice> , <https://w3id.org/product/ProtectiveDevice%2FCIRCUITBREAKER> .

props:installationMethod
        a                      owl:DatatypeProperty ;
        rdfs:comment           "Method of installation of cable/conductor. Installation methods are typically defined by reference in standards such as IEC 60364-5-52, table 52A-1 or BS7871 Appendix 4 Table 4A1 etc. Selection of the value to be used should be determined from such a standard according to local usage."@en ;
        rdfs:label             "installationMethod"@en ;
        rdfs:range             xsd:string ;
        schema:domainIncludes  <https://w3id.org/product/CableSegment> .

props:releaseCurrentI2tStart
        a                      owl:DatatypeProperty ;
        rdfs:comment           "S 함수 특성 곡선 I2t의 시작점 [x In]가 시작 방류 전류."@ko-KR , "G 함수 특성 곡선 I2t의 시작점 [x In]가 시작 방류 전류."@ko-KR , "The release current in [x In] for the start point of the I2t tripping curve of the G-function, if any."@en , "G関数の特性曲線I2tの始点[x In]が開始放流電流。"@ja-JP , "The release current in [x In] for the start point of the I2t tripping curve of the S-function, if any."@en , "S関数の特性曲線I2tの始点[x In]が開始放流電流。"@ja-JP ;
        rdfs:label             "I2t 시작 방류 전류"@ko-KR , "releaseCurrentI2tStart"@en , "I2tの開始放流電流"@ja-JP ;
        rdfs:range             <https://w3id.org/product/ElectricCurrentMeasure> ;
        schema:domainIncludes  <https://w3id.org/product/ProtectiveDeviceTrippingUnit> .

props:energySourceConsumption
        a                      owl:DatatypeProperty ;
        rdfs:comment           "Energy consumption."@en , "エネルギ消費量"@ja-JP , "Consommation d'énergie."@fr-FR ;
        rdfs:label             "energySourceConsumption"@en , "エネルギ消費量"@ja-JP , "ConsommationSourceEnergie."@fr-FR ;
        schema:domainIncludes  <https://w3id.org/product/Boiler> .

props:hasDefrost  a            owl:DatatypeProperty ;
        rdfs:comment           "has the heat exchanger has defrost function or not."@en , "熱交換器のデフロスト機能有無"@ja-JP , "Possède ou non une fonction dégel sur l'échangeur de chaleur"@fr-FR ;
        rdfs:label             "hasDefrost"@en , "デフロスト有無"@ja-JP , "PossèdeDégel"@fr-FR ;
        rdfs:range             xsd:boolean ;
        schema:domainIncludes  <https://w3id.org/product/AirToAirHeatRecovery> .

props:circuitType  a           owl:DatatypeProperty ;
        rdfs:comment           "OpenCircuit: Exposes water directly to the cooling atmosphere.\nCloseCircuit: The fluid is separated from the atmosphere by a heat exchanger.\nWet: The air stream or the heat exchange surface is evaporatively cooled.\nDry: No evaporation into the air stream.\nDryWet: A combination of a dry tower and a wet tower."@en ;
        rdfs:label             "circuitType"@en ;
        schema:domainIncludes  <https://w3id.org/product/CoolingTower> .

props:vibrationTransmissibility
        a                      owl:DatatypeProperty ;
        rdfs:comment           "The vibration transmissibility percentage."@en , "振動伝達割合"@ja-JP ;
        rdfs:label             "vibrationTransmissibility"@en , "振動伝達"@ja-JP ;
        rdfs:range             <https://w3id.org/product/PositiveRatioMeasure> ;
        schema:domainIncludes  <https://w3id.org/product/VibrationIsolator> .

props:tiltVertical  a          owl:DatatypeProperty ;
        rdfs:comment           "Indicates vertical range for pivoting, where 0.0 is level, +90 degrees is looking up, -90 degrees is looking down."@en , "チルト垂直の可動角度を示す。"@ja-JP ;
        rdfs:label             "tiltVertical"@en , "チルト垂直方向可動角度"@ja-JP ;
        schema:domainIncludes  <https://w3id.org/product/AudioVisualAppliance%2FCAMERA> .

props:initialResistance
        a                      owl:DatatypeProperty ;
        rdfs:comment           "Initial new filter fluid resistance (i.e., pressure drop at the maximum air flowrate across the filter when the filter is new per ASHRAE Standard 52.1)."@en ;
        rdfs:label             "initialResistance"@en ;
        rdfs:range             <https://w3id.org/product/PressureMeasure> ;
        schema:domainIncludes  <https://w3id.org/product/Filter> .

props:glassThickness2
        a                      owl:DatatypeProperty ;
        rdfs:comment           "第二层（中间或外侧）玻璃的厚度。"@zh-CN , "Epaisseur de la deuxième couche de verre (intermédiaire ou côté extérieur)"@fr-FR , "German-description-3"@de-DE , "2番目（中間、あるいは外側）のガラスの厚み。"@ja-JP , "Thickness of the second (intermediate or outer) glass layer."@en ;
        rdfs:label             "German-name-3"@de-DE , "玻璃厚度2"@zh-CN , "EpaisseurVitrage2"@fr-FR , "glassThickness2"@en , "ガラス厚2"@ja-JP ;
        rdfs:range             <https://w3id.org/product/PositiveLengthMeasure> ;
        schema:domainIncludes  <https://w3id.org/product/cWindow> , <https://w3id.org/product/Door> .

props:maximumCableLength
        a                      owl:DatatypeProperty ;
        rdfs:comment           "Maximum cable length based on voltagedrop. NOTE: This value may also be specified as a constraint within an IFC model if required but is included within the property set at this stage pending implementation of the required capabilities within software applications."@en ;
        rdfs:label             "maximumCableLength"@en ;
        rdfs:range             <https://w3id.org/product/LengthMeasure> ;
        schema:domainIncludes  <https://w3id.org/product/CableSegment> .

props:groundFaultCurrentSetValue
        a                      owl:DatatypeProperty ;
        rdfs:comment           "Ground fault current set value. The set value of the ground tripping current if adjustable."@en ;
        rdfs:label             "groundFaultCurrentSetValue"@en ;
        rdfs:range             <https://w3id.org/product/ElectricCurrentMeasure> ;
        schema:domainIncludes  <https://w3id.org/product/ProtectiveDevice> .

props:condenserFlowrate
        a                      owl:DatatypeProperty ;
        rdfs:comment           "Flow rate of fluid through the condenser."@en , "凝縮器を通る流体の流量"@ja-JP ;
        rdfs:label             "condenserFlowrate"@en , "凝縮器流量"@ja-JP ;
        rdfs:range             <https://w3id.org/product/VolumetricFlowRateMeasure> ;
        schema:domainIncludes  <https://w3id.org/product/UnitaryEquipment%2FAIRCONDITIONINGUNIT> .

props:secondaryAirflowRateRange
        a                      owl:DatatypeProperty ;
        rdfs:comment           "possible range of secondary airflow that can be delivered."@en , "二次側の送風可能範囲"@ja-JP , "Plage possible de débit d'air au secondaire qui peut être fourni."@fr-FR ;
        rdfs:label             "secondaryAirflowRateRange"@en , "二次側風量範囲"@ja-JP , "PlageDébitAirSecondaire"@fr-FR ;
        schema:domainIncludes  <https://w3id.org/product/AirToAirHeatRecovery> .

props:transportationStrength
        a                      owl:DatatypeProperty ;
        rdfs:comment           "The minimum required compressive strength of the concrete required for transportation."@en , "輸送に必要なコンクリートの最小必要圧縮強度。"@ja-JP ;
        rdfs:label             "transportationStrength"@en , "輸送強度"@ja-JP ;
        rdfs:range             <https://w3id.org/product/PressureMeasure> ;
        schema:domainIncludes  <https://w3id.org/product/BuildingElement> .

props:moistureContent
        a                      owl:DatatypeProperty ;
        rdfs:comment           "Total weight of moisture relative to oven-dried weight of the wood."@en ;
        rdfs:label             "moistureContent"@en ;
        rdfs:range             <https://w3id.org/product/PositiveRatioMeasure> ;
        schema:domainIncludes  <https://w3id.org/product/Material%2FWood> .

props:asBuiltLocationNumber
        a                      owl:DatatypeProperty ;
        rdfs:comment           "Defines a unique location within a structure, the ‘slot’ into which the piece was installed. Where pieces share the same piece mark, they can be interchanged. The value is only known after erection."@en ;
        rdfs:label             "asBuiltLocationNumber"@en ;
        rdfs:range             xsd:string ;
        schema:domainIncludes  <https://w3id.org/product/BuildingElement> .

props:totalSensibleHeatGain
        a                      owl:DatatypeProperty ;
        rdfs:comment           "The total sensible heat or energy gained by the space during the peak cooling conditions."@en , "ピーク時の冷房条件で取得した顕熱或いはエネルギー。"@ja-JP , "피크 냉방 조건에서 얻은 현열 또는 에너지."@ko-KR ;
        rdfs:label             "totalSensibleHeatGain"@en , "顕熱負荷の合計"@ja-JP , "현열 부하의 합계"@ko-KR ;
        rdfs:range             <https://w3id.org/product/PowerMeasure> ;
        schema:domainIncludes  <https://w3id.org/product/Space> .

props:compressorEvaporatorHeatGain
        a                      owl:DatatypeProperty ;
        rdfs:comment           "Heat gain between the evaporator outlet and the compressor inlet."@en , "蒸発器出口と圧縮機入口間の熱取得"@ja-JP ;
        rdfs:label             "compressorEvaporatorHeatGain"@en , "圧縮機・蒸発器熱取得"@ja-JP ;
        schema:domainIncludes  <https://w3id.org/product/Evaporator> .

props:compressorTotalEfficiency
        a                      owl:DatatypeProperty ;
        rdfs:comment           "Ratio of the thermal cooling capacity to electrical input."@en , "Rapport entre la puissance frigorifique et l'énergie électrique absorbée."@fr-FR ;
        rdfs:label             "compressorTotalEfficiency"@en , "RendementGlobalIsentropique"@fr-FR ;
        schema:domainIncludes  <https://w3id.org/product/Compressor> .

props:yieldStress  a           owl:DatatypeProperty ;
        rdfs:comment           "A measure of the yield stress (or characteristic 0.2 percent proof stress) of the material."@en ;
        rdfs:label             "yieldStress"@en ;
        rdfs:range             <https://w3id.org/product/PressureMeasure> ;
        schema:domainIncludes  <https://w3id.org/product/Material%2FSteel> .

props:effectiveArea  a         owl:DatatypeProperty ;
        rdfs:comment           "Effective discharge area of the air terminal."@en , "ターミナルの有効吹き出し範囲"@ja-JP , "Zone d'émission efficace du terminal de ventilation."@fr-FR ;
        rdfs:label             "effectiveArea"@en , "有効面積"@ja-JP , "ZoneEfficace"@fr-FR ;
        rdfs:range             <https://w3id.org/product/AreaMeasure> ;
        schema:domainIncludes  <https://w3id.org/product/AirTerminal> .

props:boundaryAreaHeatLoss
        a                      owl:DatatypeProperty ;
        rdfs:comment           "Heat loss per unit area for the boundary object. This is a design input value for use in the absence of calculated load data."@en , "単位面積ありた周辺関連設備の熱ロス。空調負荷計算値以外の設計設定値。"@ja-JP , "단위 면적이 주변 관련 설비의 열 손실. 공조 부하 계산 이외의 디자인 설정."@ko-KR ;
        rdfs:label             "boundaryAreaHeatLoss"@en , "周辺関連設備の熱ロス"@ja-JP , "주변 관련 설비의 열 손실"@ko-KR ;
        rdfs:range             <https://w3id.org/product/HeatFluxDensityMeasure> ;
        schema:domainIncludes  <https://w3id.org/product/Space> .

props:cornerFixingPlateFlangeWidthInPlaneX
        a                      owl:DatatypeProperty ;
        rdfs:comment           "The flange width of the L-shaped corner plate in plane X."@en , "L型コーナープレートのX面のフランジ幅。"@ja-JP , "L 형 코너 플레이트 X면 플랜지 폭"@ko-KR ;
        rdfs:label             "cornerFixingPlateFlangeWidthInPlaneX"@en , "フランジ幅X"@ja-JP , "플랜지 폭 X"@ko-KR ;
        rdfs:range             <https://w3id.org/product/PositiveLengthMeasure> ;
        schema:domainIncludes  <https://w3id.org/product/DiscreteAccessory%2FCorner%20fixing%20plate> .

props:productionLotId
        a                      owl:DatatypeProperty ;
        rdfs:comment           "The manufacturer's production lot identifier."@en ;
        rdfs:label             "productionLotId"@en ;
        rdfs:range             xsd:string ;
        schema:domainIncludes  <https://w3id.org/product/BuildingElement> .

props:junctionRightRadius
        a                      owl:DatatypeProperty ;
        rdfs:comment           "The radius of bending for the right junction where 0 indicates sharp bend."@en , "右継ぎ手の曲がりの半径(ゼロは鋭い曲がりを意味する)"@ja-JP ;
        rdfs:label             "junctionRightRadius"@en , "右継ぎ手半径"@ja-JP ;
        rdfs:range             <https://w3id.org/product/PositiveLengthMeasure> ;
        schema:domainIncludes  <https://w3id.org/product/PipeFitting%2FJUNCTION> .

props:motorPosition  a         owl:DatatypeProperty ;
        rdfs:comment           "Defines the location of the motor relative to the air stream.\n\nInAirStream: Fan motor is in the air stream.\nOutOfAirStream: Fan motor is out of the air stream."@en , "空気流路と相対的なモーターの位置定義\n流路内、流路外　その他"@ja-JP ;
        rdfs:label             "motorPosition"@en , "モーター位置"@ja-JP ;
        schema:domainIncludes  <https://w3id.org/product/Fan> .

props:colorAppearance
        a                      owl:DatatypeProperty ;
        rdfs:comment           "In both the DIN and CIE standards, artificial light sources are classified in terms of their color appearance. To the human eye they all appear to be white; the difference can only be detected by direct comparison. Visual performance is not directly affected by differences in color appearance."@en , "DIN（ドイツ規格協会）とCIE（国際照明委員会）の両方の規格で、人工照明は色の見え方で分類される。\n人の目には全て白く見えてくる、その差異は直接比較することにより判別することが可能である。視機能は色の見え方の差異に直接影響はしない。"@ja-JP ;
        rdfs:label             "colorAppearance"@en , "色の見え方"@ja-JP , "색상의 외관"@ko-KR ;
        rdfs:range             xsd:string ;
        schema:domainIncludes  <https://w3id.org/product/Lamp> .

props:maxAdjustmentX_ICS
        a                      owl:DatatypeProperty ;
        rdfs:comment           "Provides the maximum setting value for the available current adjustment in relation to the\nIcs breaking capacity of the protection device of which the actual tripping unit is a part of. The value is not asserted unless the instantaneous time protection is."@en , "実際のトリップ装置の一部である保護装置のIcs 遮断容量に関連して利用可能な電流の最大調整値。"@ja-JP , "실제 트립 장치의 일부인 보호자 Ics 차단 용량과 관련하여 사용 가능한 전류의 최대 조정 값"@ko-KR ;
        rdfs:label             "maxAdjustmentX_ICS"@en , "最大調整X_ICS"@ja-JP , "최대 조정 X_ICS"@ko-KR ;
        rdfs:range             <https://w3id.org/product/ElectricCurrentMeasure> ;
        schema:domainIncludes  <https://w3id.org/product/ProtectiveDeviceTrippingUnit> .

props:condenserMeanVoidFraction
        a                      owl:DatatypeProperty ;
        rdfs:comment           "Mean void fraction in condenser."@en ;
        rdfs:label             "condenserMeanVoidFraction"@en ;
        schema:domainIncludes  <https://w3id.org/product/Condenser> .

props:isLaminated  a           owl:DatatypeProperty ;
        rdfs:comment           "表示玻璃是否具有含其他材料的夹层。"@zh-CN , "ガラス以外の素材が重ねられているか（TRUE）否か（FALSE)示す。"@ja-JP , "Indication whether the glass is layered with other materials (TRUE) or not (FALSE)."@en , "German-description-8"@de-DE , "Indique si le verre est feuilleté (VRAI) ou non (FAUX)."@fr-FR ;
        rdfs:label             "VitrageFeuillete"@fr-FR , "German-name-8"@de-DE , "皮膜を被せたガラス"@ja-JP , "是否夹层"@zh-CN , "isLaminated"@en ;
        rdfs:range             xsd:boolean ;
        schema:domainIncludes  <https://w3id.org/product/Door> , <https://w3id.org/product/cWindow> .

props:supplyWaterTemperatureHeating
        a                      owl:DatatypeProperty ;
        rdfs:comment           "Supply water temperature in heating mode."@en ;
        rdfs:label             "supplyWaterTemperatureHeating"@en ;
        schema:domainIncludes  <https://w3id.org/product/CooledBeam> .

props:restrictions  a          owl:DatatypeProperty ;
        rdfs:comment           "Restrictions that may be placed by a  competent authority."@en ;
        rdfs:label             "restrictions"@en ;
        rdfs:range             xsd:string ;
        schema:domainIncludes  <https://w3id.org/product/SpatialStructureElement> .

props:dischargeFlowRate
        a                      owl:DatatypeProperty ;
        rdfs:comment           "The volumetric rate of fluid discharge."@en , "吐出流体の体積流量。"@ja-JP , "放水液体の体積。"@ja-JP ;
        rdfs:label             "吐出流量"@ja-JP , "放水流量"@ja-JP , "dischargeFlowRate"@en ;
        rdfs:range             <https://w3id.org/product/VolumetricFlowRateMeasure> ;
        schema:domainIncludes  <https://w3id.org/product/FireSuppressionTerminal%2FSPRINKLER> , <https://w3id.org/product/FireSuppressionTerminal%2FFIREHYDRANT> .

props:waterConsumptionPerUnit
        a                      owl:DatatypeProperty ;
        rdfs:comment           "リットル単位で表現された水の消費量。"@ja-JP , "사용 수량의 리터 수"@ko-KR , "Quantité d'eau utilisée telle que définie dans la norme ISO21930:2007 [NDT : et dans la norme NF P01-010]. Exprimée en litres."@fr-FR , "Quantity of water used."@en ;
        rdfs:label             "単位あたり水使用"@ja-JP , "waterConsumptionPerUnit"@en , "단위 당 물 사용"@ko-KR , "ConsommationEauParUnite"@fr-FR ;
        rdfs:range             <https://w3id.org/product/VolumeMeasure> ;
        schema:domainIncludes  <https://w3id.org/product/Element> .

props:visibleRefractionIndex
        a                      owl:DatatypeProperty ;
        rdfs:comment           "Index of refraction (visible) defines the \"bending\" of the sola! r ray in the visible spectrum when it passes from one medium into another."@en ;
        rdfs:label             "visibleRefractionIndex"@en ;
        rdfs:range             xsd:decimal ;
        schema:domainIncludes  <https://w3id.org/product/Material> .

props:coolingDesignDay
        a                      owl:DatatypeProperty ;
        rdfs:comment           "The month, day  and time that has been selected for the cooling design calculations."@en , "冷房設計用気象データの日時（月、日、時刻）。"@ja-JP , "냉방 설계 기상 데이터의 시간 (월, 일, 시간)."@ko-KR ;
        rdfs:label             "coolingDesignDay"@en , "冷房設計基準日"@ja-JP , "냉방설계 기준일"@ko-KR ;
        rdfs:range             xsd:dateTime ;
        schema:domainIncludes  <https://w3id.org/product/Building> .

props:particleMassHolding
        a                      owl:DatatypeProperty ;
        rdfs:comment           "Mass of particle holding in the filter."@en ;
        rdfs:label             "particleMassHolding"@en ;
        schema:domainIncludes  <https://w3id.org/product/Filter> .

props:outsideAirFlowrate
        a                      owl:DatatypeProperty ;
        rdfs:comment           "Flow rate of outside air entering the unit."@en , "ユニットに入る外気流量"@ja-JP ;
        rdfs:label             "outsideAirFlowrate"@en , "外気流量"@ja-JP ;
        rdfs:range             <https://w3id.org/product/VolumetricFlowRateMeasure> ;
        schema:domainIncludes  <https://w3id.org/product/UnitaryEquipment%2FAIRCONDITIONINGUNIT> .

props:operationalTemperatureRange
        a                      owl:DatatypeProperty ;
        rdfs:comment           "Allowable operation ambient air temperature range."@en , "Opération admise sur la plage de température de l'air ambiant"@fr-FR , "動作を許容する周囲温度の範囲"@ja-JP , "Allowable operational air temperature range."@en , "Plage de température fonctionnelle admissible."@fr-FR ;
        rdfs:label             "動作温度範囲"@ja-JP , "operationalTemperatureRange"@en , "PlageTemperatureFonctionnelle"@fr-FR , "PlageTempératureOpérationelle"@fr-FR ;
        schema:domainIncludes  <https://w3id.org/product/AirToAirHeatRecovery> , <https://w3id.org/product/Coil> .

props:operationPressureMax
        a                      owl:DatatypeProperty ;
        rdfs:comment           "Maximum pressure under normal operating conditions."@en ;
        rdfs:label             "operationPressureMax"@en ;
        rdfs:range             <https://w3id.org/product/PressureMeasure> ;
        schema:domainIncludes  <https://w3id.org/product/Filter%2FCOMPRESSEDAIRFILTER> .

props:releaseTimeI2tEnd
        a                      owl:DatatypeProperty ;
        rdfs:comment           "G 함수 I2의 특성 곡선의 끝점에서 s를 방류 시간.  I2t 종료 방류 전류 시간이 I2t 시작 방류 시간보다 낮게해야한다"@ko-KR , "G関数のI2の特性曲線のエンドポイントの[s]を放流時間。 \n I2tの終了放流電流時間がI2tの開始放流時間よりも低くしなければならない。"@ja-JP , "The release time in [s] for the end point of the I2 tripping curve of the S-function, if any. The value of ReleaseTimeI2tEnd shall be lower than ReleaseTimeI2tStart."@en , "The release time in [s] for the end point of the I2 tripping curve of the G-function, if any. The value of ReleaseTimeI2tEnd shall be lower than ReleaseTimeI2tStart."@en , "S関数のI2の特性曲線のエンドポイントの[s]を放流時間。 \n I2tの終了放流電流時間がI2tの開始放流時間よりも低くしなければならない。"@ja-JP , "S함수 I2의 특성 곡선의 끝점에서 s를 방류 시간.  I2t 종료 방류 전류 시간이 I2t 시작 방류 시간보다 낮게해야한다"@ko-KR ;
        rdfs:label             "I2tの終了放流時間"@ja-JP , "I2t 종료 방류 시간"@ko-KR , "releaseTimeI2tEnd"@en ;
        rdfs:range             <https://w3id.org/product/TimeMeasure> ;
        schema:domainIncludes  <https://w3id.org/product/ProtectiveDeviceTrippingUnit> .

props:identifier  a            owl:DatatypeProperty ;
        rdfs:comment           "The identifier assigned to the agreement for the purposes of tracking."@en ;
        rdfs:label             "identifier"@en ;
        rdfs:range             xsd:string ;
        schema:domainIncludes  <https://w3id.org/product/SpatialStructureElement> .

props:buildingID  a            owl:DatatypeProperty ;
        rdfs:comment           "Gebäudekennzeichen dieses Gebäudes. Während der Baueingabe ist es das temporäre Kennzeichnen des Bauantrags."@de-DE , "건물에 부여되는 고유 식별자이다. 계획 요청시 사용되는 초기 임시 식별자이다. 이 임시 식별자는 건물이 정식으로 등록된 경우에 영구적인 식별자로 변경된다."@ko-KR , "Un identifiant unique attribué au bâtiment. Un identifiant temporaire est attribué au moment de la programmation. Il est ensuite remplacé par un identifiant permanent lorsque le bâtiment est enregistré dans une base de données de nature règlementaire."@fr-FR , "建物に付与されるユニークな識別子。計画要請の際に使用される初期の一時的な識別子。この一時的な識別子は、建物が正式に登録された際に恒久的な識別子へと変更される。"@ja-JP , "A unique identifier assigned to a building. A temporary identifier is initially assigned at the time of making a planning application. This temporary identifier is changed to a permanent identifier when the building is registered into a statutory buildings and properties database."@en ;
        rdfs:label             "buildingID"@en , "IdBatiment"@fr-FR , "建物記号"@ja-JP , "Gebäudekennzeichen"@de-DE , "건물 ID"@ko-KR ;
        rdfs:range             xsd:string ;
        schema:domainIncludes  <https://w3id.org/product/Building> .

props:orientation  a           owl:DatatypeProperty ;
        rdfs:comment           "The intended orientation for the damper as specified by the manufacturer."@en ;
        rdfs:label             "orientation"@en ;
        schema:domainIncludes  <https://w3id.org/product/Damper> .

props:fanPowerRate  a          owl:DatatypeProperty ;
        rdfs:comment           "Fan power consumption."@en , "ファン消費電力"@ja-JP ;
        rdfs:label             "fanPowerRate"@en , "Fan効率動力量"@ja-JP ;
        schema:domainIncludes  <https://w3id.org/product/Fan> .

props:centerCoreBaseHeight
        a                      owl:DatatypeProperty ;
        rdfs:comment           "Center core base height of the profile."@en ;
        rdfs:label             "centerCoreBaseHeight"@en ;
        rdfs:range             <https://w3id.org/product/PositiveLengthMeasure> ;
        schema:domainIncludes  <https://w3id.org/product/ArbitraryProfileDefWithVoids> .

props:upstreamPressure
        a                      owl:DatatypeProperty ;
        rdfs:comment           "The operating pressure of the fluid upstream of the pressure reducing valve."@en , "減圧弁の上流の流体運転圧力"@ja-JP ;
        rdfs:label             "upstreamPressure"@en , "上流圧力"@ja-JP ;
        rdfs:range             <https://w3id.org/product/PressureMeasure> ;
        schema:domainIncludes  <https://w3id.org/product/Valve%2FPRESSUREREDUCING> .

props:remainingCost  a         owl:DatatypeProperty ;
        rdfs:comment           "The remaining cost on behalf of the resource allocation."@en , "資源配分のための残存しているコスト。"@ja-JP ;
        rdfs:label             "remainingCost"@en , "残存コスト"@ja-JP ;
        schema:domainIncludes  <https://w3id.org/product/ConstructionResource> .

props:temperatureRange
        a                      owl:DatatypeProperty ;
        rdfs:comment           "Allowable maximum and minimum temperature."@en , "Allowable operational range of the fluid temperature."@en , "許容できる最大/最小温度"@ja-JP , "Temperature range within which the air terminal is designed to operate."@en , "許容最大/最小温度"@ja-JP , "Plage de température dans laquelle le terminal de ventilation est prévu de fonctionner."@fr-FR , "Allowable minimum and maximum temperature."@en , "Temperature range."@en , "流体温度の許容範囲"@ja-JP , "許容最低・最高温度"@ja-JP , "許容最高・最低温度"@ja-JP , "操作されるターミナルの温度範囲"@ja-JP ;
        rdfs:label             "temperatureRange"@en , "温度範囲"@ja-JP , "PlageTemperature"@fr-FR ;
        schema:domainIncludes  <https://w3id.org/product/PipeSegment> , <https://w3id.org/product/AirTerminal> , <https://w3id.org/product/DuctSegment> , <https://w3id.org/product/Damper> , <https://w3id.org/product/Pump> , <https://w3id.org/product/DuctFitting> , <https://w3id.org/product/DuctSilencer> , <https://w3id.org/product/PipeFitting> .

props:sprinklerType  a         owl:DatatypeProperty ;
        rdfs:comment           "Identifies the predefined types of sprinkler  from which the type required may be set."@en , "あらかじめ定義済みのスプリンクラーの型から必要な型を設定する識別。"@ja-JP ;
        rdfs:label             "sprinklerType"@en , "スプリンクラータイプ"@ja-JP ;
        schema:domainIncludes  <https://w3id.org/product/FireSuppressionTerminal%2FSPRINKLER> .

props:centreOfGravityInY
        a                      owl:DatatypeProperty ;
        rdfs:comment           "Location of the profile's centre of gravity (geometric centroid), measured along yp."@en ;
        rdfs:label             "centreOfGravityInY"@en ;
        rdfs:range             <https://w3id.org/product/LengthMeasure> ;
        schema:domainIncludes  <https://w3id.org/product/ProfileDef> .

props:standardFixingPlateThickness
        a                      owl:DatatypeProperty ;
        rdfs:comment           "The thickness of the standard fixing plate."@en , "標準的な固定プレートの板厚。"@ja-JP , "표준 고정 플레이트의 두께"@ko-KR ;
        rdfs:label             "standardFixingPlateThickness"@en , "板厚"@ja-JP , "두께"@ko-KR ;
        rdfs:range             <https://w3id.org/product/PositiveLengthMeasure> ;
        schema:domainIncludes  <https://w3id.org/product/DiscreteAccessory%2FStandard%20fixing%20plate> .

props:batchReference  a        owl:DatatypeProperty ;
        rdfs:comment           "The identity of the batch reference from which an occurrence of a product is taken."@en ;
        rdfs:label             "batchReference"@en ;
        rdfs:range             xsd:string ;
        schema:domainIncludes  <https://w3id.org/product/Element> .

props:spaceTemperatureWinterMax
        a                      owl:DatatypeProperty ;
        rdfs:comment           "空間またはゾーンの寒冷季(冬季)の最高温度。利用者/設計者の視点から要求される。"@ja-JP , "Maximal temperature of the space or zone for the cold (winter) period, that is required from user/designer view point and provided as requirement for heating."@en , "공간이나 영역 추운 계절 (겨울) 최고 온도 이용자 / 설계자의 관점에서 요구된다."@ko-KR , "Maximal geforderte Raumtemperatur für die Auslegung der Raumheizung."@de-DE , "Température maximale de l'espace ou de la zone en hiver. Spécifiée par l'usager ou le concepteur et utilisée comme consigne pour le chauffage."@fr-FR ;
        rdfs:label             "spaceTemperatureWinterMax"@en , "冬季最高室内温度"@ja-JP , "Température maximale en hiver"@fr-FR , "겨울최고온도"@ko-KR , "Raumtemperatur Heizung Maximal"@de-DE ;
        rdfs:range             <https://w3id.org/product/ThermodynamicTemperatureMeasure> ;
        schema:domainIncludes  <https://w3id.org/product/cZone> , <https://w3id.org/product/cSpatialZone> , <https://w3id.org/product/Space> .

props:pressureRise  a          owl:DatatypeProperty ;
        rdfs:comment           "The developed pressure."@en , "上がった圧力"@ja-JP ;
        rdfs:label             "pressureRise"@en , "昇圧"@ja-JP ;
        schema:domainIncludes  <https://w3id.org/product/Pump> .

props:starterType  a           owl:DatatypeProperty ;
        rdfs:comment           "A list of the available types of starter from which that required may be selected where:\n\nAutoTransformer: A starter for an induction motor which uses for starting one or more reduced voltages derived from an auto transformer. (IEC 441-14-45)\nManual: A starter in which the force for closing the main contacts is provided exclusively by manual energy. (IEC 441-14-39)\nDirectOnLine: A starter which connects the line voltage across the motor terminals in one step. (IEC 441-14-40)\nFrequency: A starter in which the frequency of the power supply is progressively increased until the normal operation frequency is attained.\nnStep: A starter in which there are (n-1) intermediate accelerating positions between the off and full on positions. (IEC 441-14-41)\nRheostatic: A starter using one or several resistors for obtaining, during starting, stated motor torque characteristics and for limiting the current. (IEC 441-14-425)\nStarDelta: A starter for a 3 phase induction motor such that in the starting position the stator windings are connected in star and in the final running position they are connected in delta. (IEC 441-14-44)"@en , "以下より選択が必要となる、始動の一覧リスト：\n\n自動： 自動トランスから引き出された１つ以上の低下した電圧でスタートするために使用する誘導電動機用のスターター (IEC 441-14-45)\n手動： メインのコンタクトから強制的に分離されたところにあり、手動によりエネルギーが供給される (IEC 441-14-39)\nじか入れ: ワンステップでモーター・ターミナル間の線間電圧をつなぐスターター (IEC 441-14-40)\n振動：電源の振動数が通常の操作振動まで次第に増大して行くスターター\nnStep: オフ（OFF)とオン（ON）の間で、（n-1）の中間の加速度的な位置であるスターター。 (IEC 441-14-41)\n抵抗：モータのトルク特性の取得、開始、そして安定する間に、電流を制限するために 1 つまたはいくつかの抵抗を利用したスターター (IEC 441-14-425) \nスターデルタ：開始位置では固定小巻線（スターターワインディング）が星状で接続され、その後、最終の実行状態ではデルタ状に接続されるという3相誘導モーター用のスターター。（IEC 441-14-44）"@ja-JP , "아래에서 선택이 필요한 시동 목록 목록 : 자동 : 자동 트랜스에서 가져온 하나 이상의 저하 전압으로 시작하는 데 사용하는 유도 전동기의 스타터 (IEC 441-14-45) 수동 : 기본 연락처에서 강제로 격리된 거리에 있으며, 수동으로 에너지가 공급되는 (IEC 441-14-39) 글자 하나 입력 : 한 번에 모터 터미널 사이의 선간 전압을 연결 스타터 (IEC 441-14-40) 진동 : 전원의 진동수가 정상 작동 진동까지 점차 증대 해가는 스타터 nStep : 꺼짐 (OFF)과 켜짐 (ON) 사이에서 (n-1) 사이의 가속도적인 위치이다 스타터. (IEC 441-14-41) 저항 : 모터의 토크 특성 가져오기 시작, 그리고 안정 사이에 전류를 제한하기 위해 하나 또는 몇 가지 저항을 이용한 스타터 (IEC 441-14-425) 스타 델타 : 시작 위치는 고정 小巻 선 (초보 와인)이 소행성에 연결된 후, 최종 상태에서는 델타 모양으로 연결된다 3 상 유도 모터의 스타터. (IEC 441-14-44)"@ko-KR ;
        rdfs:label             "starterType"@en , "始動タイプ"@ja-JP , "시작 유형"@ko-KR ;
        schema:domainIncludes  <https://w3id.org/product/SwitchingDevice%2FSTARTER> .

props:protectivePoreRatio
        a                      owl:DatatypeProperty ;
        rdfs:comment           "The protective pore ratio indicating the frost-resistance of the concrete."@en ;
        rdfs:label             "protectivePoreRatio"@en ;
        rdfs:range             <https://w3id.org/product/NormalisedRatioMeasure> ;
        schema:domainIncludes  <https://w3id.org/product/Material%2FConcrete> .

props:airflowSensible
        a                      owl:DatatypeProperty ;
        rdfs:comment           "最大潜熱負荷に対応する給気量。"@ja-JP , "The air flowrate required to satisfy the sensible peak loads."@en , "최대 잠열 부하에 대한 급기 량"@ko-KR ;
        rdfs:label             "顕熱空調給気量"@ja-JP , "airflowSensible"@en , "현열 공조 급기 량"@ko-KR ;
        rdfs:range             <https://w3id.org/product/VolumetricFlowRateMeasure> ;
        schema:domainIncludes  <https://w3id.org/product/Zone> , <https://w3id.org/product/SpatialZone> , <https://w3id.org/product/Space> .

props:extendToStructure
        a                      owl:DatatypeProperty ;
        rdfs:comment           "Indicates whether the object extend to the structure above (TRUE) or not (FALSE)."@en , "Angabe , ob diese Wand raumhoch ist (WAHR), oder nicht (FALSCH)."@de-DE , "Indique si l'objet s'étend à la structure au-dessus (VRAI) ou non (FAUX)."@fr-FR ;
        rdfs:label             "extendToStructure"@en , "Raumhohe Wand"@de-DE , "ExtensionStructure"@fr-FR ;
        rdfs:range             xsd:boolean ;
        schema:domainIncludes  <https://w3id.org/product/Wall> .

props:videoScaleMode  a        owl:DatatypeProperty ;
        rdfs:comment           "비디오 크기 조정모드를 나타낸다."@ko-KR , "Indicates video scaling modes."@en , "ビデオスケーリングモードを示す。"@ja-JP , "비디오 크기 조정 모드를 나타낸다."@ko-KR ;
        rdfs:label             "비디오 스케일 모드"@ko-KR , "videoScaleMode"@en , "비디오 스케일"@ko-KR , "ビデオスケールモード"@ja-JP ;
        schema:domainIncludes  <https://w3id.org/product/AudioVisualAppliance%2FDISPLAY> , <https://w3id.org/product/AudioVisualAppliance%2FPROJECTOR> .

props:maximumWorkingPressure
        a                      owl:DatatypeProperty ;
        rdfs:comment           "Maximum pressure that the object is manufactured to withstand."@en , "最大圧力、製造耐圧。"@ja-JP , "Maximum working pressure."@en ;
        rdfs:label             "最大作動圧力"@ja-JP , "maximumWorkingPressure"@en ;
        rdfs:range             <https://w3id.org/product/PressureMeasure> ;
        schema:domainIncludes  <https://w3id.org/product/FireSuppressionTerminal%2FSPRINKLER> , <https://w3id.org/product/Damper> .

props:setPointConcentration
        a                      owl:DatatypeProperty ;
        rdfs:comment           "感知される煙濃度。\nセットポイント値を置くために、IfcPropertyBoundedValue.SetPointValueを使用する。"@ja-JP , "The ion concentration value to be sensed. Use IfcPropertyBoundedValue.SetPointValue to set the set point value."@en , "감지되는 이온 농도. 세트 포인트 값을 넣으려면, IfcPropertyBoundedValue.SetPointValue를 사용하십시오."@ko-KR , "The gas concentration value to be sensed. Use IfcPropertyBoundedValue.SetPointValue to set the set point value."@en , "감지되는 연기 농도. 세트 포인트 값을 넣으려면, IfcPropertyBoundedValue.SetPointValue를 사용하십시오."@ko-KR , "The smoke concentration value to be sensed. Use IfcPropertyBoundedValue.SetPointValue to set the set point value."@en , "感知されるイオン濃度。\nセットポイント値を置くために、IfcPropertyBoundedValue.SetPointValueを使用する。"@ja-JP , "感知されるガス濃度。\nセットポイント値を置くために、IfcPropertyBoundedValue.SetPointValueを使用する。"@ja-JP ;
        rdfs:label             "setPointConcentration"@en , "煙濃度設定値"@ja-JP , "이온 농도 설정"@ko-KR , "ガス濃度設定値"@ja-JP , "イオン濃度設定値"@ja-JP , "연기 농도 설정"@ko-KR ;
        schema:domainIncludes  <https://w3id.org/product/Sensor%2FIONCONCENTRATIONSENSOR> , <https://w3id.org/product/Sensor%2FSMOKESENSOR> , <https://w3id.org/product/Sensor%2FGASSENSOR> .

props:dynamicViscosity
        a                      owl:DatatypeProperty ;
        rdfs:comment           "A measure of the viscous resistance of the material."@en ;
        rdfs:label             "dynamicViscosity"@en ;
        rdfs:range             <https://w3id.org/product/DynamicViscosityMeasure> ;
        schema:domainIncludes  <https://w3id.org/product/Material> .

props:nominalPressureDrop
        a                      owl:DatatypeProperty ;
        rdfs:comment           "Total pressure drop across the filter."@en ;
        rdfs:label             "nominalPressureDrop"@en ;
        rdfs:range             <https://w3id.org/product/PressureMeasure> ;
        schema:domainIncludes  <https://w3id.org/product/Filter> .

props:location3Global
        a                      owl:DatatypeProperty ;
        rdfs:comment           "Global X,Y,Z coordinates of the point in which Thickness3 is given"@en ;
        rdfs:label             "location3Global"@en ;
        schema:domainIncludes  <https://w3id.org/product/StructuralSurfaceMemberVarying> .

props:coreBaseWidth  a         owl:DatatypeProperty ;
        rdfs:comment           "Core base width of the profile."@en ;
        rdfs:label             "coreBaseWidth"@en ;
        rdfs:range             <https://w3id.org/product/PositiveLengthMeasure> ;
        schema:domainIncludes  <https://w3id.org/product/ArbitraryProfileDefWithVoids> .

props:fuel  a                  owl:DatatypeProperty ;
        rdfs:comment           "The amount of fuel consumed during the period specified in the time series."@en , "특정 기간 동안의 연료 소비."@ko-KR ;
        rdfs:label             "fuel"@en , "연료 소비량"@ko-KR ;
        schema:domainIncludes  <https://w3id.org/product/Building> .

props:nominalTotalPressure
        a                      owl:DatatypeProperty ;
        rdfs:comment           "Nominal total pressure rise across the fan."@en , "ファンでの設計全圧上昇"@ja-JP ;
        rdfs:label             "nominalTotalPressure"@en , "設計全圧"@ja-JP ;
        rdfs:range             <https://w3id.org/product/PressureMeasure> ;
        schema:domainIncludes  <https://w3id.org/product/Fan> .

props:volumetricEfficiency
        a                      owl:DatatypeProperty ;
        rdfs:comment           "Ratio of the actual volume of gas entering the compressor to the theoretical displacement of the compressor."@en , "Rapport entre le volume effectif de gaz rentrant dans le compresseur et le volume déplacé théorique du compresseur."@fr-FR ;
        rdfs:label             "volumetricEfficiency"@en , "RendementVolumétrique"@fr-FR ;
        schema:domainIncludes  <https://w3id.org/product/Compressor> .

props:signalTimeIncrease
        a                      owl:DatatypeProperty ;
        rdfs:comment           "Time factor used for exponential increase."@en , "적분 시간 (Ti)"@ko-KR ;
        rdfs:label             "signalTimeIncrease"@en , "적분 시간 (Ti)"@ko-KR ;
        rdfs:range             <https://w3id.org/product/TimeMeasure> ;
        schema:domainIncludes  <https://w3id.org/product/Controller%2FPROPORTIONAL> .

props:remoteReading  a         owl:DatatypeProperty ;
        rdfs:comment           "Indicates whether the meter has a connection for remote reading through connection of a communication device (set TRUE) or not (set FALSE)."@en ;
        rdfs:label             "remoteReading"@en ;
        rdfs:range             xsd:boolean ;
        schema:domainIncludes  <https://w3id.org/product/FlowMeter> .

props:wireEmbeddingLength
        a                      owl:DatatypeProperty ;
        rdfs:comment           "The length of the part of wire which is embedded in the precast concrete element."@en , "プレキャストコンクリート部材の中に埋め込まれたワイヤーの長さ。"@ja-JP , "프리 캐스트 콘크리트 부재속에 묻힌 철사의 길이"@ko-KR ;
        rdfs:label             "wireEmbeddingLength"@en , "埋め込み長さ"@ja-JP , "포함 길이"@ko-KR ;
        rdfs:range             <https://w3id.org/product/PositiveLengthMeasure> ;
        schema:domainIncludes  <https://w3id.org/product/DiscreteAccessory%2FWire%20loop> .

props:coilConnectionDirection
        a                      owl:DatatypeProperty ;
        rdfs:comment           "Coil connection direction (facing into the air stream)."@en , "Direction de la connexion à la batterie (en face du jet d'air)"@fr-FR ;
        rdfs:label             "coilConnectionDirection"@en , "DirectionConnexionBatterie"@fr-FR ;
        schema:domainIncludes  <https://w3id.org/product/Coil> .

props:i1  a                    owl:DatatypeProperty ;
        rdfs:comment           "The (thermal) lower testing current limit in [x In], indicating that for currents lower than I1, the tripping time shall be longer than the associated tripping time, T2."@en , "熱動式の低試験電流限界値を [x In]、電流は I1　よりも低い値を示す。トリップ時間は関連する T2 の時間よりも長い。"@ja-JP , "열 동식 낮은 시험 전류 한계를 [x In] 전류는 I1보다 낮은 값을 나타낸다. 트립 시간은 관련 T2 시간보다 길다."@ko-KR , "サーマルの低試験電流限界値を [x In]、電流は I1　よりも低い値を示す。トリップ時間は関連する T2 の時間よりも長い。"@ja-JP , "열 낮은 시험 전류 한계를 [x In] 전류는 I1보다 낮은 값을 나타낸다. 트립 시간은 관련 T2 시간보다 길다."@ko-KR ;
        rdfs:label             "i1"@en , "I1"@ko-KR , "I1"@ja-JP ;
        rdfs:range             xsd:decimal ;
        schema:domainIncludes  <https://w3id.org/product/ProtectiveDeviceTrippingUnit%2FTHERMAL> , <https://w3id.org/product/ProtectiveDeviceTrippingUnit%2FELECTROMAGNETIC> .

props:condenserLeavingTemperature
        a                      owl:DatatypeProperty ;
        rdfs:comment           "Termperature of fluid leaving condenser."@en , "凝縮器出口流体温度"@ja-JP ;
        rdfs:label             "condenserLeavingTemperature"@en , "凝縮器出口温度"@ja-JP ;
        rdfs:range             <https://w3id.org/product/ThermodynamicTemperatureMeasure> ;
        schema:domainIncludes  <https://w3id.org/product/UnitaryEquipment%2FAIRCONDITIONINGUNIT> .

props:timeConstant  a          owl:DatatypeProperty ;
        rdfs:comment           "The time constant of the sensor."@en , "センサの時定数。"@ja-JP , "센서의 시정."@ko-KR ;
        rdfs:label             "timeConstant"@en , "時定数"@ja-JP , "시정"@ko-KR ;
        rdfs:range             <https://w3id.org/product/TimeMeasure> ;
        schema:domainIncludes  <https://w3id.org/product/Sensor%2FFIRESENSOR> .

props:outputCapacity  a        owl:DatatypeProperty ;
        rdfs:comment           "Total nominal heat output as listed by the manufacturer."@en , "メーカーによりリストアップされた公称熱出力"@ja-JP ;
        rdfs:label             "outputCapacity"@en , "出力"@ja-JP ;
        rdfs:range             <https://w3id.org/product/PowerMeasure> ;
        schema:domainIncludes  <https://w3id.org/product/SpaceHeater> .

props:accuracyQualityObtained
        a                      owl:DatatypeProperty ;
        rdfs:comment           "A measure of the accuracy quality of survey points as obtained expressed in percentage terms."@en , "Mesure de la précision obtenue des points de relevé, exprimée en pourcentage."@fr-FR ;
        rdfs:label             "accuracyQualityObtained"@en , "PrecisionObtenue"@fr-FR ;
        rdfs:range             <https://w3id.org/product/RatioMeasure> ;
        schema:domainIncludes  <https://w3id.org/product/Annotation%2FSurveyArea> .

props:airParticleFilterType
        a                      owl:DatatypeProperty ;
        rdfs:comment           "A panel dry type extended surface filter is a dry-type air filter with random fiber mats or blankets in the forms of pockets, V-shaped or radial pleats, and include the following:\n\nCoarseFilter: Filter with a efficiency lower than 30% for atmosphere dust-spot.\nCoarseMetalScreen: Filter made of metal screen.\nCoarseCellFoams: Filter made of cell foams.\nCoarseSpunGlass: Filter made of spun glass.\nMediumFilter: Filter with an efficiency between 30-98% for atmosphere dust-spot.\nMediumElectretFilter: Filter with fine electret synthetic fibers.\nMediumNaturalFiberFilter: Filter with natural fibers.\nHEPAFilter: High efficiency particulate air filter.\nULPAFilter: Ultra low penetration air filter.\nMembraneFilters: Filter made of membrane for certain pore diameters in flat sheet and pleated form.\nA renewable media with a moving curtain viscous filter are random-fiber media coated with viscous substance in roll form or curtain where fresh media is fed across the face of the filter and the dirty media is rewound onto a roll at the bottom or to into a reservoir:\nRollForm: Viscous filter used in roll form.\nAdhesiveReservoir: Viscous filter used in moving curtain form.\nA renewable moving curtain dry media filter is a random-fiber dry media of relatively high porosity used in moving-curtain(roll) filters.\nAn electrical filter uses electrostatic precipitation to remove and collect particulate contaminants."@en ;
        rdfs:label             "airParticleFilterType"@en ;
        schema:domainIncludes  <https://w3id.org/product/Filter%2FAIRPARTICLEFILTER> .

props:iC60269  a               owl:DatatypeProperty ;
        rdfs:comment           "The breaking capacity in [A] for fuses in accordance with the IEC 60269 series."@en , "IECの60269シリーズに応じたヒューズの遮断容量[A]。"@ja-JP , "IEC의 60269 시리즈에 따라 퓨즈의 차단 용량 [A]."@ko-KR ;
        rdfs:label             "iC60269"@en , "IC60269"@ja-JP , "IC60269"@ko-KR ;
        rdfs:range             <https://w3id.org/product/ElectricCurrentMeasure> ;
        schema:domainIncludes  <https://w3id.org/product/ProtectiveDevice%2FFUSEDISCONNECTOR> .

props:hygrothermalRating
        a                      owl:DatatypeProperty ;
        rdfs:comment           "Resistence against hygrothermal impact from different temperatures and humidities inside and outside. It is given according to the national code or regulation."@en , "Hygrothermische Widerstandsfähigkeit gegen Temperatur- und Feuchteunterschiede gemäß der nationalen oder regionalen Richtlinie als Mindestanforderung gegen die Verformung der Tür."@de-DE , "Résistance à l'impact hygrothermique des différences de température et d'humidité entre l'intérieur et l'extérieur, selon une classification ou règlementation nationale."@fr-FR ;
        rdfs:label             "hygrothermalRating"@en , "Klimaklasse"@de-DE , "Résistance hygrothermique"@fr-FR ;
        rdfs:range             xsd:string ;
        schema:domainIncludes  <https://w3id.org/product/Door> .

props:evaporatorCoolant
        a                      owl:DatatypeProperty ;
        rdfs:comment           "The fluid used for the coolant in the evaporator."@en , "蒸発器で使用する流体（水、ブライン、グリコール、　他）"@ja-JP ;
        rdfs:label             "evaporatorCoolant"@en , "蒸発器冷却剤"@ja-JP ;
        schema:domainIncludes  <https://w3id.org/product/Evaporator> .

props:i2TApplicability
        a                      owl:DatatypeProperty ;
        rdfs:comment           "The applicability of the time adjustment related to the tripping function."@en , "トリップ機能の時延を求める時に適用する関数。"@ja-JP , "트립 기능 시간 연장을 요구할 때 적용하는 함수입니다."@ko-KR ;
        rdfs:label             "i2TApplicability"@en , "I2Tの適用"@ja-JP , "12 T적용"@ko-KR ;
        schema:domainIncludes  <https://w3id.org/product/ProtectiveDeviceTrippingUnit> .

props:lightFixturePlacingType
        a                      owl:DatatypeProperty ;
        rdfs:comment           "A list of the available types of placing specification for light fixtures from which that required may be selected."@en , "照明器具の取付場所をリストから選択。"@ja-JP , "조명기구의 설치 장소를 목록에서 선택합니다."@ko-KR ;
        rdfs:label             "lightFixturePlacingType"@en , "照明器具取付場所"@ja-JP , "조명기구 설치 장소"@ko-KR ;
        schema:domainIncludes  <https://w3id.org/product/LightFixture> .

props:slotWidth  a             owl:DatatypeProperty ;
        rdfs:comment           "Slot width."@en , "スロット巾"@ja-JP , "Epaisseur de la fente"@fr-FR ;
        rdfs:label             "slotWidth"@en , "スロット巾"@ja-JP , "EpaisseurFente"@fr-FR ;
        rdfs:range             <https://w3id.org/product/PositiveLengthMeasure> ;
        schema:domainIncludes  <https://w3id.org/product/AirTerminal> .

props:efficiencyCurve
        a                      owl:DatatypeProperty ;
        rdfs:comment           "Fan efficiency =f (flow rate)."@en ;
        rdfs:label             "efficiencyCurve"@en ;
        schema:domainIncludes  <https://w3id.org/product/Fan> .

props:hasFan  a                owl:DatatypeProperty ;
        rdfs:comment           "Terminal box has a fan inside (fan powered box)."@en , "内部に送風機を持つ時にTRUE"@ja-JP , "Le registre terminal possède dans son  intérieur un ventilateur (registre motorisé)"@fr-FR ;
        rdfs:label             "hasFan"@en , "送風機有無"@ja-JP , "Possède ventilateur"@fr-FR ;
        rdfs:range             xsd:boolean ;
        schema:domainIncludes  <https://w3id.org/product/AirTerminalBox> .

props:stemTopChamfer  a        owl:DatatypeProperty ;
        rdfs:comment           "Stem top chamfer of the profile."@en ;
        rdfs:label             "stemTopChamfer"@en ;
        rdfs:range             <https://w3id.org/product/NonNegativeLengthMeasure> ;
        schema:domainIncludes  <https://w3id.org/product/ArbitraryClosedProfileDef> .

props:t5  a                    owl:DatatypeProperty ;
        rdfs:comment           "The electromagnetic testing time in [s] associated with the testing currents I4 and I5, i.e. electromagnetic tripping time"@en , "電磁の試験時間を [s] , 関連する試験電流を I4 と I5　とする。"@ja-JP , "전자 시험 시간 [s] 관련 시험 전류를 I4하면 I5한다."@ko-KR ;
        rdfs:label             "t5"@en , "T5"@ja-JP , "T5"@ko-KR ;
        rdfs:range             <https://w3id.org/product/TimeMeasure> ;
        schema:domainIncludes  <https://w3id.org/product/ProtectiveDeviceTrippingUnit%2FELECTROMAGNETIC> .

props:washersCount  a          owl:DatatypeProperty ;
        rdfs:comment           "Count of washers to be mounted on one bolt"@en ;
        rdfs:label             "washersCount"@en ;
        rdfs:range             <https://w3id.org/product/CountMeasure> ;
        schema:domainIncludes  <https://w3id.org/product/MechanicalFastener%2FBOLT> .

props:natureOfRisk  a          owl:DatatypeProperty ;
        rdfs:comment           "An indication of the generic nature of the risk that might be encountered. \n\nNOTE: It is anticipated that there will be a local agreement that constrains the values that might be assigned to this property. An example might be 'Fall'  or 'Fall of grille unit' causing injury and damage to person and property."@en ;
        rdfs:label             "natureOfRisk"@en ;
        rdfs:range             xsd:string ;
        schema:domainIncludes  <https://w3id.org/product/Process> .

props:fixtureHeight  a         owl:DatatypeProperty ;
        rdfs:comment           "The height of the fixture, such as the text height of an exit sign."@en , "出口標識などの器具の高さ。"@ja-JP , "출구 표지판 등의기구의 높이"@ko-KR ;
        rdfs:label             "fixtureHeight"@en , "器具の高さ"@ja-JP , "기구의 높이"@ko-KR ;
        rdfs:range             <https://w3id.org/product/PositiveLengthMeasure> ;
        schema:domainIncludes  <https://w3id.org/product/LightFixture%2FSECURITYLIGHTING> .

props:airflowRateRange
        a                      owl:DatatypeProperty ;
        rdfs:comment           "Range of airflow that can be delivered."@en , "Possible range of airflow that can be delivered."@en , "Plage possible de débit aéraulique pouvant être délivré. Pour les cas où il n'y a pas de débit à travers la batterie (par ex. batterie électrique en plancher), alors la valeur est zéro."@fr-FR , "送風できる風量の範囲"@ja-JP , "Plage de débit d'air pouvant être fourni."@fr-FR , "Possible range of airflow that can be delivered.  For cases where there is no airflow across the coil (e.g. electric coil in a floor slab), then the value is zero."@en ;
        rdfs:label             "PlageDébitAéraulique"@fr-FR , "風量範囲"@ja-JP , "Domaine de débit d'air"@fr-FR , "airflowRateRange"@en ;
        schema:domainIncludes  <https://w3id.org/product/CooledBeam%2FACTIVE> , <https://w3id.org/product/AirTerminalBox> , <https://w3id.org/product/Coil> .

props:inputFlowrate  a         owl:DatatypeProperty ;
        rdfs:comment           "Maximum hydraulic flowrate requirement."@en , "최대 제어 공기 유량"@ko-KR , "Maximum input control air flowrate requirement."@en , "最大流量。"@ja-JP , "最大制御空気流量。"@ja-JP , "최대 유량"@ko-KR ;
        rdfs:label             "入力流量"@ja-JP , "입력 유량"@ko-KR , "inputFlowrate"@en ;
        rdfs:range             <https://w3id.org/product/VolumetricFlowRateMeasure> ;
        schema:domainIncludes  <https://w3id.org/product/Actuator%2FPNEUMATICACTUATOR> , <https://w3id.org/product/Actuator%2FHYDRAULICACTUATOR> .

props:occupancyNumber
        a                      owl:DatatypeProperty ;
        rdfs:comment           "Nombre d'occupants concernés par l'activité dans cet espace."@fr-FR , "Number of people required for the activity assigned to this space."@en , "Durchschnittliche Anzahl der Personen für deren  Aktivitäten der Raum vorgesehen ist."@de-DE , "この空間に割り当てられた活動を遂行するために必要な人数。"@ja-JP ;
        rdfs:label             "利用人数"@ja-JP , "occupancyNumber"@en , "Belegung"@de-DE , "NombreOccupants"@fr-FR ;
        rdfs:range             <https://w3id.org/product/CountMeasure> ;
        schema:domainIncludes  <https://w3id.org/product/Space> , <https://w3id.org/product/cSpatialZone> , <https://w3id.org/product/cZone> .

props:supportType  a           owl:DatatypeProperty ;
        rdfs:comment           "Available support types from which that required may be selected."@en ;
        rdfs:label             "supportType"@en ;
        schema:domainIncludes  <https://w3id.org/product/SystemFurnitureElement%2FWORKSURFACE> .

props:longTimeFunction
        a                      owl:DatatypeProperty ;
        rdfs:comment           "Applying long time function\nA flag indicating that the long time function (i.e. the thermal tripping) of the device is used. The value should be set to TRUE for all devices except those that allows the Long time function of the device not to be used."@en ;
        rdfs:label             "longTimeFunction"@en ;
        rdfs:range             xsd:boolean ;
        schema:domainIncludes  <https://w3id.org/product/ProtectiveDevice> .

props:heatTransferCoefficient
        a                      owl:DatatypeProperty ;
        rdfs:comment           "Heat transfer coefficient-area product."@en ;
        rdfs:label             "heatTransferCoefficient"@en ;
        schema:domainIncludes  <https://w3id.org/product/CoolingTower> .

props:sensibleCoolingCapacity
        a                      owl:DatatypeProperty ;
        rdfs:comment           "Sensible cooling capacity."@en , "顕熱冷却能力"@ja-JP ;
        rdfs:label             "sensibleCoolingCapacity"@en , "顕熱冷却能力"@ja-JP ;
        rdfs:range             <https://w3id.org/product/PowerMeasure> ;
        schema:domainIncludes  <https://w3id.org/product/UnitaryEquipment%2FAIRCONDITIONINGUNIT> .

props:requiredHeadroom
        a                      owl:DatatypeProperty ;
        rdfs:comment           "German-description-2"@de-DE , "Hauteur de passage (échappée) requise selon la réglementation en vigueur ou des spécifications additionnelles."@fr-FR , "Required headroom clearance for the passageway according to the applicable building code or additional requirements."@en , "German-description-6"@de-DE , "Hauteur de passage (échappée) requise selon le Code en vigueur ou des spécifications additionnelles."@fr-FR , "要求される頭高余裕。関連する建築基準法を参照。"@ja-JP , "建筑规范或其他规定要求的通道净空高度。"@zh-CN ;
        rdfs:label             "requiredHeadroom"@en , "所需净空"@zh-CN , "要求頭高余裕"@ja-JP , "HauteurPassageRequise"@fr-FR , "erforderliche Durchgangshöhe"@de-DE ;
        rdfs:range             <https://w3id.org/product/PositiveLengthMeasure> ;
        schema:domainIncludes  <https://w3id.org/product/Ramp> , <https://w3id.org/product/Stair> .

props:longInsideEndTopBarPitch
        a                      owl:DatatypeProperty ;
        rdfs:comment           "The pitch length of the long inside end top bar."@en , "長辺方向・柱間帯・上端端部の鉄筋間隔。"@ja-JP ;
        rdfs:label             "longInsideEndTopBarPitch"@en , "長辺・柱列帯・上端端部ピッチ"@ja-JP ;
        rdfs:range             <https://w3id.org/product/PositiveLengthMeasure> ;
        schema:domainIncludes  <https://w3id.org/product/Slab> .

props:upperTime2  a            owl:DatatypeProperty ;
        rdfs:comment           "The time in [s], indicating the tripping times of the upper time/current curve at the UpperCurrent2."@en , "[s]の時間,上電流2より上部の特性曲線のトリップ時間を示す"@ja-JP , "[s]의 시간에 전류 2보다 상단의 특성 곡선의 트립 시간을 나타냄"@ko-KR ;
        rdfs:label             "upperTime2"@en , "上時間2"@ja-JP , "상시간2"@ko-KR ;
        rdfs:range             <https://w3id.org/product/TimeMeasure> ;
        schema:domainIncludes  <https://w3id.org/product/ProtectiveDeviceTrippingUnit> .

props:acknowledge  a           owl:DatatypeProperty ;
        rdfs:comment           "Indicates acknowledgement status where False indicates acknowlegement is required and outstanding, True indicates condition has been acknowedged, and Unknown indicates no acknowledgement is required.  Upon resetting the condition, then acknowledgement reverts to Unknown."@en ;
        rdfs:label             "acknowledge"@en ;
        schema:domainIncludes  <https://w3id.org/product/Alarm> .

props:pumperConnectionSize
        a                      owl:DatatypeProperty ;
        rdfs:comment           "The size of a connection to which a fire hose may be connected that is then linked to a pumping unit."@en , "ポンプユニットに接続されであろう消防ホースの接続サイズ。"@ja-JP ;
        rdfs:label             "pumperConnectionSize"@en , "ポンプ接続サイズ"@ja-JP ;
        rdfs:range             <https://w3id.org/product/PositiveLengthMeasure> ;
        schema:domainIncludes  <https://w3id.org/product/FireSuppressionTerminal%2FFIREHYDRANT> .

props:material  a              owl:DatatypeProperty ;
        rdfs:comment           "Type of material from which the conductor is constructed."@en , "導体を構成する材料のタイプ。"@ja-JP , "도체를 구성하는 재료의 종류."@ko-KR ;
        rdfs:label             "material"@en , "材料"@ja-JP , "도체의 기능 유형."@ko-KR ;
        schema:domainIncludes  <https://w3id.org/product/CableSegment%2FCONDUCTORSEGMENT> .

props:setPointHumidity
        a                      owl:DatatypeProperty ;
        rdfs:comment           "The humidity value to be sensed. Use IfcPropertyBoundedValue.SetPointValue to set the set point value."@en , "感知される湿度。\nセットポイント値を置くために、IfcPropertyBoundedValue.SetPointValueを使用する。"@ja-JP , "감지되는 습도. 세트 포인트 값을 넣으려면, IfcPropertyBoundedValue.SetPointValue를 사용하십시오."@ko-KR ;
        rdfs:label             "setPointHumidity"@en , "湿度設定値"@ja-JP , "습도 설정"@ko-KR ;
        schema:domainIncludes  <https://w3id.org/product/Sensor%2FHUMIDITYSENSOR> .

props:spaceTemperatureWinterMin
        a                      owl:DatatypeProperty ;
        rdfs:comment           "Température minimale de l'espace ou de la zone en hiver. Spécifiée par l'usager ou le concepteur et utilisée comme consigne pour le chauffage."@fr-FR , "Minimal geforderte Raumtemperatur für die Auslegung der Raumheizung."@de-DE , "Minimal temperature of the space or zone for the cold (winter) period, that is required from user/designer view point and provided as requirement for heating."@en , "공간이나 영역 추운 계절 (겨울)의 최저 온도. 이용자 / 설계자의 관점에서 요구된다."@ko-KR , "空間またはゾーンの寒冷季(冬季)の最低温度。利用者/設計者の視点から要求される。"@ja-JP ;
        rdfs:label             "겨울철 최저온도"@ko-KR , "Raumtemperatur Heizung Minimal"@de-DE , "冬季最低室内温度"@ja-JP , "spaceTemperatureWinterMin"@en , "Température minimale en hiver"@fr-FR ;
        rdfs:range             <https://w3id.org/product/ThermodynamicTemperatureMeasure> ;
        schema:domainIncludes  <https://w3id.org/product/cSpatialZone> , <https://w3id.org/product/Space> , <https://w3id.org/product/cZone> .

props:manualOverride  a        owl:DatatypeProperty ;
        rdfs:comment           "Identifies whether hand-operated operation is provided as an override (= TRUE) or not (= FALSE). Note that this value should be set to FALSE by default in the case of a Hand Operated Actuator."@en , "オーバーライド機能として手動操作が提供されるか (= TRUE) 、否か （= FALSE)を識別する。手動で操作するアクチュエータの場合は、この値をデフォルトとしてFALSEに設定する必要があるので注意すること。"@ja-JP ;
        rdfs:label             "manualOverride"@en , "オーバーライド機能の有無"@ja-JP ;
        rdfs:range             xsd:boolean ;
        schema:domainIncludes  <https://w3id.org/product/Actuator> .

props:pieceMark  a             owl:DatatypeProperty ;
        rdfs:comment           "Defines a unique piece for production purposes. All pieces with the same piece mark value are identical and interchangeable. The piece mark may be composed of sub-parts that have specific locally defined meaning (e.g. B-1A may denote a beam, of generic type ‘1’ and specific shape ‘A’)."@en ;
        rdfs:label             "pieceMark"@en ;
        rdfs:range             xsd:string ;
        schema:domainIncludes  <https://w3id.org/product/BuildingElement> .

props:mechanicalEfficiency
        a                      owl:DatatypeProperty ;
        rdfs:comment           "ポンプの稼動時の機械効率"@ja-JP , "The pumps operational mechanical efficiency."@en , "Ratio of the work (as measured) delivered to the gas to the work input to the compressor shaft."@en , "Rapport entre le travail fourni (tel que mesuré) au gaz et le travail fourni à l'arbre du compresseur."@fr-FR ;
        rdfs:label             "機械効率"@ja-JP , "mechanicalEfficiency"@en , "RendementMécanique"@fr-FR ;
        schema:domainIncludes  <https://w3id.org/product/Pump> , <https://w3id.org/product/Compressor> .

props:fusibleLinkTemperature
        a                      owl:DatatypeProperty ;
        rdfs:comment           "The temperature that the fusible link melts."@en ;
        rdfs:label             "fusibleLinkTemperature"@en ;
        rdfs:range             <https://w3id.org/product/ThermodynamicTemperatureMeasure> ;
        schema:domainIncludes  <https://w3id.org/product/Damper%2FFIRESMOKEDAMPER> , <https://w3id.org/product/Damper%2FFIREDAMPER> .

props:groupCode  a             owl:DatatypeProperty ;
        rdfs:comment           "e.g. panels, worksurfaces, storage, etc."@en ;
        rdfs:label             "groupCode"@en ;
        rdfs:range             xsd:string ;
        schema:domainIncludes  <https://w3id.org/product/SystemFurnitureElement> .

props:tiltHorizontal  a        owl:DatatypeProperty ;
        rdfs:comment           "Indicates horizontal range for pivoting, where positive values indicate the camera rotating clockwise,"@en , "チルト水平の可動角度を示す。"@ja-JP ;
        rdfs:label             "tiltHorizontal"@en , "チルト水平方向可動角度"@ja-JP ;
        schema:domainIncludes  <https://w3id.org/product/AudioVisualAppliance%2FCAMERA> .

props:finishColor  a           owl:DatatypeProperty ;
        rdfs:comment           "La couleur de finition du terminal de ventilation."@fr-FR , "ターミナルの仕上げ色"@ja-JP , "The finish color for the air terminal."@en , "Finish color for cooled beam."@en ;
        rdfs:label             "finishColor"@en , "仕上げ色"@ja-JP , "CouleurFinition"@fr-FR ;
        rdfs:range             xsd:string ;
        schema:domainIncludes  <https://w3id.org/product/AirTerminal> , <https://w3id.org/product/CooledBeam> .

props:height  a                owl:DatatypeProperty ;
        rdfs:comment           "German-description-2"@de-DE , "空間の高さ（高さにおける垂直方向の拡張）を求める定義です。「四角形」の形状プロパティのみ提示されます。"@ja-JP , "The requested height (vertical extension in elevation) of the provision for void\", only provided if the Shape property is set to \"rectangle\"."@en , "負荷を掛ける前の振動絶縁材の高さ"@ja-JP , "Height of the object. It is the upper hight of the railing above the floor or stair.\nThe size information is provided in addition to the shape representation and the geometric parameters used within. In cases of inconsistency between the geometric parameters and the size properties, provided in the attached property set, the geometric parameters take precedence."@en , "Hauteur du garde-corps. C'est la plus grande hauteur du garde-corps relativement au plancher ou à l'escalier. Cette propriété est donnée en complément de la représentation de la forme et des paramètres géométriques qui la déterminent. En cas d'incohérence entre ces paramètres géométriques et cette propriété, ce sont les paramètres géométriques qui priment."@fr-FR , "Height of the vibration isolator before tha application of load."@en , "Geforderte Höhe des Durchbruchs, wird nur dann angegeben, wenn der Wert des Attributes \"Form\" gleich \"Rechteck\" ist."@de-DE , "La hauteur requise de la réservation (extension verticale en élévation). Fournie seulement si la propriété Forme a pour valeur \"Rectangle\"."@fr-FR , "空构件的高度（在立面图中竖直方向的长度），仅当“形状”属性为“矩形”时适用。"@zh-CN , "気流方向に垂直に計られたフィンの長さ"@ja-JP , "构件的高度。该属性为栏杆在地板或楼梯以上部分的高度。\n该属性所提供的形状信息是对内部形状描述和几何参数的补充。如果几何参数与该属性所提供的形状属性不符，应以几何参数为准。"@zh-CN , "オブジェクトの高さ。床または会談から手すりの上部までの高さ。"@ja-JP , "Length of the fin as measured perpendicular to the direction of airflow."@en ;
        rdfs:label             "Hauteur"@fr-FR , "Höhe"@de-DE , "高さ"@ja-JP , "高度"@zh-CN , "height"@en ;
        rdfs:range             <https://w3id.org/product/PositiveLengthMeasure> ;
        schema:domainIncludes  <https://w3id.org/product/TubeBundle%2FFINNED> , <https://w3id.org/product/VibrationIsolator> , <https://w3id.org/product/BuildingElementProxy%2FPROVISIONFORVOID> , <https://w3id.org/product/Railing> .

props:hasBuiltInAlarm
        a                      owl:DatatypeProperty ;
        rdfs:comment           "Indicates whether the smoke sensor is included as an element within a smoke alarm/sensor unit (TRUE) or not (FALSE)."@en , "煙センサーが煙警報センサユニットの中に要素として含まれているか(TRUE)、否か(FALSE)を識別する。"@ja-JP , "연기 센서가 화재 경보 센서 유닛의 요소로 포함되어 있는지 (TRUE) 여부 (FALSE)를 확인한다."@ko-KR ;
        rdfs:label             "hasBuiltInAlarm"@en , "煙警報器に含まれているか"@ja-JP , "연기 경보기에 포함여부"@ko-KR ;
        rdfs:range             xsd:boolean ;
        schema:domainIncludes  <https://w3id.org/product/Sensor%2FSMOKESENSOR> .

props:energyGainTotal
        a                      owl:DatatypeProperty ;
        rdfs:comment           "居室の最大冷房負荷と空調システム（機器等）の再熱負荷による最大熱負荷。"@ja-JP , "거실 최대 냉방 부하 및 공조 시스템 (장비 등) 재열 부하에 의한 최대 열부하."@ko-KR , "The total amount of energy gains for the spaces served by the system during the peak cooling conditions, plus any system-level total energy gains."@en ;
        rdfs:label             "総熱取得"@ja-JP , "energyGainTotal"@en , "총 열 검색"@ko-KR ;
        rdfs:range             <https://w3id.org/product/PowerMeasure> ;
        schema:domainIncludes  <https://w3id.org/product/Space> , <https://w3id.org/product/Zone> , <https://w3id.org/product/SpatialZone> .

props:videoResolutionMode
        a                      owl:DatatypeProperty ;
        rdfs:comment           "ビデオ解像度モードを示す。"@ja-JP , "解像度モードを示す。"@ja-JP , "비디오 해상도를 보여준다."@ko-KR , "Indicates video resolution modes."@en , "해상도를 보여준다"@ko-KR , "모드해상도를 보여준다"@ko-KR ;
        rdfs:label             "비디오 해상도 모드"@ko-KR , "videoResolutionMode"@en , "解像度モード"@ja-JP , "ビデオ解像度モード"@ja-JP , "디스플레이 모드"@ko-KR ;
        schema:domainIncludes  <https://w3id.org/product/AudioVisualAppliance%2FCAMERA> , <https://w3id.org/product/AudioVisualAppliance%2FPROJECTOR> , <https://w3id.org/product/AudioVisualAppliance%2FDISPLAY> .

props:varistorType  a          owl:DatatypeProperty ;
        rdfs:comment           "A list of the available types of varistor  from which that required may be selected."@en , "選択が必要となる、バリスターの一覧リスト。"@ja-JP , "선택된 varistor(소자)의 유용한 유형목록"@ko-KR ;
        rdfs:label             "varistorType"@en , "保護タイプ"@ja-JP , "보호 종류"@ko-KR ;
        schema:domainIncludes  <https://w3id.org/product/ProtectiveDevice%2FVARISTOR> .

props:nominalDiameterOrWidth
        a                      owl:DatatypeProperty ;
        rdfs:comment           "The nominal diameter or width of the duct segment."@en , "ダクト直管の呼び径またはダクト巾"@ja-JP ;
        rdfs:label             "nominalDiameterOrWidth"@en , "呼び径・巾"@ja-JP ;
        rdfs:range             <https://w3id.org/product/PositiveLengthMeasure> ;
        schema:domainIncludes  <https://w3id.org/product/DuctSegment> .

props:reheatType  a            owl:DatatypeProperty ;
        rdfs:comment           "Terminal box reheat type."@en , "ターミナルの再熱方式\n（電気、水コイル、蒸気コイル、ガス加熱．．．）"@ja-JP , "Type de réchauffage d'un registre terminal de ventilation"@fr-FR ;
        rdfs:label             "reheatType"@en , "再熱形式"@ja-JP , "Type de réchauffage"@fr-FR ;
        schema:domainIncludes  <https://w3id.org/product/AirTerminalBox> .

props:warrantyIdentifier
        a                      owl:DatatypeProperty ;
        rdfs:comment           "The identifier assigned to a warranty."@en ;
        rdfs:label             "warrantyIdentifier"@en ;
        rdfs:range             xsd:string ;
        schema:domainIncludes  <https://w3id.org/product/Element> .

props:operationTemperatureRange
        a                      owl:DatatypeProperty ;
        rdfs:comment           "許容動作周囲温度範囲"@ja-JP , "許容周囲温度範囲"@ja-JP , "許容作動周囲空気温度範囲"@ja-JP , "Allowable operational range of the ambient air temperature."@en , "Allowable operation ambient air temperature range."@en , "Allowable operation ambient fluid temperature range."@en , "Plage opérationnelle possible de la température de l'air ambiant"@fr-FR ;
        rdfs:label             "動作温度範囲"@ja-JP , "Plage de température d'exploitation"@fr-FR , "operationTemperatureRange"@en ;
        rdfs:range             <https://w3id.org/product/ThermodynamicTemperatureMeasure> ;
        schema:domainIncludes  <https://w3id.org/product/EvaporativeCooler> , <https://w3id.org/product/AirTerminalBox> , <https://w3id.org/product/Fan> , <https://w3id.org/product/CoolingTower> , <https://w3id.org/product/Filter> .

props:throw  a                 owl:DatatypeProperty ;
        rdfs:comment           "Distance cooled beam throws the air."@en ;
        rdfs:label             "throw"@en ;
        schema:domainIncludes  <https://w3id.org/product/CooledBeam%2FACTIVE> .

props:valvePattern  a          owl:DatatypeProperty ;
        rdfs:comment           "The configuration of the ports of a valve according to either the linear route taken by a fluid flowing through the valve or by the number of ports where:\n\nSINGLEPORT: Valve that has a single entry port from the system that it serves, the exit port being to the surrounding environment.\nANGLED_2_PORT: Valve in which the direction of flow is changed through 90 degrees.\nSTRAIGHT_2_PORT: Valve in which the flow is straight through.\nSTRAIGHT_3_PORT: Valve with three separate ports.\nCROSSOVER_4_PORT: Valve with 4 separate ports."@en , "単一ポートSINGLEPORT()=システムで単一入口ポートを持ち、出口ポートは周囲環境である　2ポート直角型(ANGLED_2_PORT)＝中で流れ方向が完全に90度変わる弁　2ポート直行型(STRAIGHT_2_PORT)＝中で流れが真っ直ぐな弁　3ポート直行型(STRAIGHT_3_PORT)＝3つの別々のポートを持つ　4ポート交差型(CROSSOVER_4_PORT)＝4つの別々のポートを持つ"@ja-JP ;
        rdfs:label             "valvePattern"@en , "弁の形"@ja-JP ;
        schema:domainIncludes  <https://w3id.org/product/Valve> .

props:quality  a               owl:DatatypeProperty ;
        rdfs:comment           "計測の品質を示す値。"@ja-JP , "요청한 액츄에이터의 안전 장치 유형을 표시"@ko-KR , "시간이 지남에 값을 나타내는 Pset_ControllerTypeValue.Value에 대응 ※ 설정 가능한 정보는 IfcTimeSeries 속성 참조"@ko-KR , "Indicates the quality of measurement or failure condition, which may be further qualified by the Status.  True: measured values are considered reliable; False: measured values are considered not reliable (i.e. a fault has been detected); Unknown: reliability of values is uncertain."@en ;
        rdfs:label             "페일 세이프 유형"@ko-KR , "기본 출력 시계열 상수"@ko-KR , "quality"@en , "品質"@ja-JP ;
        schema:domainIncludes  <https://w3id.org/product/Controller> , <https://w3id.org/product/FlowInstrument> , <https://w3id.org/product/Actuator> , <https://w3id.org/product/Sensor> .

props:shortCircuit3PolePowerFactorMaximumState
        a                      owl:DatatypeProperty ;
        rdfs:comment           "Power factor of the maximum 3 pole short circuit current provided at the point of supply."@en , "電源供給時点の3極最大短絡電流力率。"@ja-JP , "전원 공급 시점의 3 극 최대 단락 전류 역률."@ko-KR ;
        rdfs:label             "shortCircuit3PolePowerFactorMaximumState"@en , "3極最大短絡電流力率"@ja-JP , "3 극 최대 단락 전류 역률"@ko-KR ;
        rdfs:range             xsd:decimal ;
        schema:domainIncludes  <https://w3id.org/product/ElectricFlowStorageDevice> .

props:fanMountingType
        a                      owl:DatatypeProperty ;
        rdfs:comment           "Defines the method of mounting the fan in the building."@en , "建物へのFan設置方法定義\nMANUFACTUREDCURB, FIELDERECTEDCURB, CONCRETEPAD, SUSPENDED, WALLMOUNTED, DUCTMOUNTED"@ja-JP ;
        rdfs:label             "fanMountingType"@en , "Fan設置タイプ"@ja-JP ;
        schema:domainIncludes  <https://w3id.org/product/Fan> .

props:buildingThermalExposure
        a                      owl:DatatypeProperty ;
        rdfs:comment           "The thermal exposure expected by the building based on surrounding site conditions."@en , "周囲環境から建物への熱放射強度。"@ja-JP , "주위 환경​​에서 건물의 열 방사 강도."@ko-KR ;
        rdfs:label             "buildingThermalExposure"@en , "周囲環境からの熱放射強度"@ja-JP , "주위환경에서 열의 방사강도"@ko-KR ;
        schema:domainIncludes  <https://w3id.org/product/Building> .

props:water  a                 owl:DatatypeProperty ;
        rdfs:comment           "The amount of water consumed during the period specified in the time series."@en , "특정 기간 동안 물 소비."@ko-KR ;
        rdfs:label             "water"@en , "물소비"@ko-KR ;
        schema:domainIncludes  <https://w3id.org/product/Building> .

props:verticalSpacing
        a                      owl:DatatypeProperty ;
        rdfs:comment           "Vertical spacing between tubes in the tube bundle."@en , "チューブ束内のチューブ間垂直間隔"@ja-JP ;
        rdfs:label             "verticalSpacing"@en , "垂直間隔"@ja-JP ;
        rdfs:range             <https://w3id.org/product/PositiveLengthMeasure> ;
        schema:domainIncludes  <https://w3id.org/product/TubeBundle> .

props:status  a                owl:DatatypeProperty ;
        rdfs:comment           "エラーコードまたはIDを示す。例：'ConfigurationError', 'NotConnected', 'DeviceFailure', 'SensorFailure', 'LastKnown, 'CommunicationsFailure', 'OutOfService'."@ja-JP , "Indicates an error code or identifier, whose meaning is specific to the particular automation system.  Example values include: 'ConfigurationError', 'NotConnected', 'DeviceFailure', 'SensorFailure', 'LastKnown, 'CommunicationsFailure', 'OutOfService'."@en , "대체 기능으로 수동 조작이 제공되는지 (= TRUE) 여부 (= FALSE)를 확인한다. 수동으로 조작하는 액츄에이터의 경우는이 값을 기본값으로 FALSE로 설정해야하므로주의한다."@ko-KR , "Etat de l'élément, utilisé avant tout pour les projets de rénovation et réaménagement. L'état assigné peut être \"Nouveau\" - l'élément prévu pour du neuf, \"Existant\" - l'élément existait et est maintenu, \"Démoli\" - l'élément existait mais doit être démoli/supprimé, \"Provisoire\" - l'élément existera à titre provisoire seulement (comme un support structurel par exemple)."@fr-FR , "Status of the element, predominately used in renovation or retrofitting projects. The status can be assigned to as \"New\" - element designed as new addition, \"Existing\" - element exists and remains, \"Demolish\" - element existed but is to be demolished,  \"Temporary\" - element will exists only temporary (like a temporary support structure)."@en , "Statut de l'élément, principalement utilisé dans les projets de rénovation et de réhabilitation. Le statut a pour valeur NOUVEAU pour un nouvel élément, EXISTANT pour un élément existant qui est conservé, DEMOLI pour un élément existant à démolir et TEMPORAIRE pour un élément temporaire (comme une structure support provisoire)."@fr-FR , "Status bzw. Phase des Bauteils insbesondere beim Bauen im Bestand. \"Neu\" (new) neues Bauteil als Ergänzung, \"Bestand\" (existing) bestehendes Bauteil, dass erhalten bleibt, \"Abbruch\" (demolish) Bauteil, das abgebrochen wird, \"Temporär\" (temporary) Bauteil und andere Bauelemente, die vorübergehend eingebaut werden (wie Abstützungen, etc.)"@de-DE , "要素（主にリノベーションまたは改修プロジェクトにおいて）の状態。 状態は、「新規(New)」－新しく追加される要素。「既存」－要素は存在し、かつ残りもの。「破壊」－要素は存在したが、廃棄されるもの。「一時的」－一時的に存在する要素（一時的にサポートしている構造のようなもの）。"@ja-JP , "요청한 액츄에이터의 안전 장치 유형을 표시"@ko-KR , "현재 전원 상태를 나타냄"@ko-KR ;
        rdfs:label             "状態"@ja-JP , "재정 기능의 유무"@ko-KR , "Etat"@fr-FR , "Status"@de-DE , "전원 상태"@ko-KR , "status"@en , "Statut"@fr-FR , "페일 세이프 유형"@ko-KR ;
        schema:domainIncludes  <https://w3id.org/product/Ramp> , <https://w3id.org/product/Slab> , <https://w3id.org/product/SolarDevice> , <https://w3id.org/product/Beam> , <https://w3id.org/product/CableFitting> , <https://w3id.org/product/ElectricDistributionBoard> , <https://w3id.org/product/ElectricMotor> , <https://w3id.org/product/StackTerminal> , <https://w3id.org/product/Sensor> , <https://w3id.org/product/Chiller> , <https://w3id.org/product/CurtainWall> , <https://w3id.org/product/ProtectiveDevice> , <https://w3id.org/product/BuildingElementProxy> , <https://w3id.org/product/Lamp> , <https://w3id.org/product/ProtectiveDeviceTrippingUnit> , <https://w3id.org/product/AudioVisualAppliance> , <https://w3id.org/product/Filter> , <https://w3id.org/product/Stair> , <https://w3id.org/product/FlowMeter> , <https://w3id.org/product/Pump> , <https://w3id.org/product/FireSuppressionTerminal> , <https://w3id.org/product/CableSegment> , <https://w3id.org/product/TubeBundle> , <https://w3id.org/product/UnitaryControlElement> , <https://w3id.org/product/TransportElement> , <https://w3id.org/product/Door> , <https://w3id.org/product/Coil> , <https://w3id.org/product/LightFixture> , <https://w3id.org/product/HeatExchanger> , <https://w3id.org/product/Compressor> , <https://w3id.org/product/Tank> , <https://w3id.org/product/Alarm> , <https://w3id.org/product/MedicalDevice> , <https://w3id.org/product/Footing> , <https://w3id.org/product/Actuator> , <https://w3id.org/product/Wall> , <https://w3id.org/product/Pile> , <https://w3id.org/product/Burner> , <https://w3id.org/product/ElectricTimeControl> , <https://w3id.org/product/MotorConnection> , <https://w3id.org/product/Member> , <https://w3id.org/product/AirTerminalBox> , <https://w3id.org/product/CoolingTower> , <https://w3id.org/product/WasteTerminal> , <https://w3id.org/product/AirToAirHeatRecovery> , <https://w3id.org/product/Window> , <https://w3id.org/product/Covering> , <https://w3id.org/product/Damper> , <https://w3id.org/product/Column> , <https://w3id.org/product/Transformer> , <https://w3id.org/product/ElectricGenerator> , <https://w3id.org/product/JunctionBox> , <https://w3id.org/product/Humidifier> , <https://w3id.org/product/ShadingDevice> , <https://w3id.org/product/CommunicationsAppliance> , <https://w3id.org/product/Controller> , <https://w3id.org/product/CableCarrierFitting> , <https://w3id.org/product/Evaporator> , <https://w3id.org/product/Roof> , <https://w3id.org/product/RampFlight> , <https://w3id.org/product/Plate> , <https://w3id.org/product/Interceptor> , <https://w3id.org/product/ElementComponent> , <https://w3id.org/product/Chimney> , <https://w3id.org/product/UnitaryEquipment> , <https://w3id.org/product/DuctSilencer> , <https://w3id.org/product/PipeSegment> , <https://w3id.org/product/StairFlight> , <https://w3id.org/product/Outlet> , <https://w3id.org/product/PipeFitting> , <https://w3id.org/product/CableCarrierSegment> , <https://w3id.org/product/Boiler> , <https://w3id.org/product/OpeningElement> , <https://w3id.org/product/Fan> , <https://w3id.org/product/DuctSegment> , <https://w3id.org/product/EvaporativeCooler> , <https://w3id.org/product/ElectricFlowStorageDevice> , <https://w3id.org/product/CooledBeam> , <https://w3id.org/product/AirTerminal> , <https://w3id.org/product/FlowInstrument> , <https://w3id.org/product/Engine> , <https://w3id.org/product/Railing> , <https://w3id.org/product/SwitchingDevice> , <https://w3id.org/product/SpaceHeater> , <https://w3id.org/product/DuctFitting> , <https://w3id.org/product/DistributionChamberElement> , <https://w3id.org/product/ElectricAppliance> .

props:movementSensingType
        a                      owl:DatatypeProperty ;
        rdfs:comment           "Enumeration that identifies the type of movement sensing mechanism."@en ;
        rdfs:label             "movementSensingType"@en ;
        schema:domainIncludes  <https://w3id.org/product/Sensor%2FMOVEMENTSENSOR> .

props:classOfService  a        owl:DatatypeProperty ;
        rdfs:comment           "A classification of usage of the hose reel that may be applied."@en , "適用されるホースリールの使用方法の分類。"@ja-JP ;
        rdfs:label             "classOfService"@en , "サービスクラス"@ja-JP ;
        rdfs:range             xsd:string ;
        schema:domainIncludes  <https://w3id.org/product/FireSuppressionTerminal%2FHOSEREEL> .

props:manufacturer  a          owl:DatatypeProperty ;
        rdfs:comment           "The organization that manufactured and/or assembled the item."@en ;
        rdfs:label             "manufacturer"@en ;
        rdfs:range             xsd:string ;
        schema:domainIncludes  <https://w3id.org/product/Element> .

props:energyLoss  a            owl:DatatypeProperty ;
        rdfs:comment           "ピーク時空調システム最大暖房負荷を提供する際の熱ロス。"@ja-JP , "The sum of energy losses for the spaces served by the system during the peak heating conditions."@en , "최대 공조 시스템 최대 난방 부하를 제공할 수있는 열 손실"@ko-KR ;
        rdfs:label             "열(에너지)로스"@ko-KR , "energyLoss"@en , "熱（エネルギー）ロス"@ja-JP ;
        rdfs:range             <https://w3id.org/product/PowerMeasure> ;
        schema:domainIncludes  <https://w3id.org/product/SpatialZone> , <https://w3id.org/product/Space> , <https://w3id.org/product/Zone> .

props:coefficientOfPerformanceCurve
        a                      owl:DatatypeProperty ;
        rdfs:comment           "Chiller coefficient of performance (COP) is function of condensing temperature and evaporating temperature, data is in table form, COP= f (TempCon, TempEvp), COP = a2+b2*Tei+c2*Tei^2+d2*Tci+e2*Tci^2+f2*Tei*Tci. \nThis table uses multiple input variables; to represent, both DefiningValues and DefinedValues lists are null and IfcTable is attached using IfcPropertyConstraintRelationship and IfcMetric.  Columns are specified in the following order: \n1.IfcPositiveRatioMeasure:CoefficientOfPerformance\n2.IfcThermodynamicTemperatureMeasure:CondensingTemperature\n3.IfcThermodynamicTemperatureMeasure:EvaporatingTemperature"@en , "Coefficient de Performance (COP) du groupe froid qui est une fonction de la température de condensation et de la température d'évaporation, les informations sont sous la forme d'un tableau, COP = f(TempCon,TempEvp), COP = a2+b1*Tei+c2*Tei^2+d2*Tci+e2*Tci^2+f2*Tei*Tci.\nCe tableau utilises plusieurs entrées variables; pour la  représenter, DefiningValues et DefinedValues sont pour les deux nulles et IfcTable est attachée en utilisant IfcPropertyConstraintRelationship et IfcMetric. Les colonnes sont indiquées dans l'ordre suivant:\n1. IfcPowerMeasureCapacity\n2. IfcThermodynamicTemperatureMeasure: CondensingTemperature\n3. IfcThermodynamicTemperatureMeasure: EvaporatingTemperature"@fr-FR ;
        rdfs:label             "coefficientOfPerformanceCurve"@en , "CourbeCOP"@fr-FR ;
        schema:domainIncludes  <https://w3id.org/product/Chiller> .

props:isMountedFlatCable
        a                      owl:DatatypeProperty ;
        rdfs:comment           "Indication of whether the cable occurrences are mounted flat (= TRUE) or in a trefoil pattern (= FALSE)."@en ;
        rdfs:label             "isMountedFlatCable"@en ;
        rdfs:range             xsd:boolean ;
        schema:domainIncludes  <https://w3id.org/product/CableSegment> .

props:endShapeType  a          owl:DatatypeProperty ;
        rdfs:comment           "Defines the types of end shapes that can be used for preformed tanks. The convention for reading these enumerated values is that for a vertical cylinder, the first value is the base and the second is the top; for a horizontal cylinder, the order of reading should be left to right. For a speherical tank, the value UNSET should be used."@en , "定義　予めタンクに使用することができる端形状の種類を示す。これらの列挙された値を読み取るための規則は、垂直円筒に関しては、最初の値はベースです、そして、2番目は先端です。水平円筒に関しては、値は左から右に読む必要があります。球形タンクの場合、値はUNSETを使用する必要があります。"@ja-JP ;
        rdfs:label             "endShapeType"@en , "末端形状タイプ"@ja-JP ;
        schema:domainIncludes  <https://w3id.org/product/Tank%2FPREFORMED> , <https://w3id.org/product/Tank> .

props:visibleTransmittance
        a                      owl:DatatypeProperty ;
        rdfs:comment           "Transmittance at normal incidence (visible). Defines the fraction of the visible spectrum of solar radiation that passes through per unit area, perpendicular to the surface."@en ;
        rdfs:label             "visibleTransmittance"@en ;
        rdfs:range             <https://w3id.org/product/PositiveRatioMeasure> ;
        schema:domainIncludes  <https://w3id.org/product/Material> .

props:heatRejectionRate
        a                      owl:DatatypeProperty ;
        rdfs:comment           "冷凍効果と圧縮機への電源入力の相当熱量の合計"@ja-JP , "Sum of the refrigeration effect and the heat equivalent of the power input to the compressor."@en ;
        rdfs:label             "排熱量"@ja-JP , "heatRejectionRate"@en ;
        schema:domainIncludes  <https://w3id.org/product/Evaporator> , <https://w3id.org/product/Condenser> .

props:securityRating  a        owl:DatatypeProperty ;
        rdfs:comment           "表示安全程度的参考性等级。\n该属性的依据为国家建筑规范。"@zh-CN , "Index based rating system indicating security level.\nIt is giving according to the national building code."@en , "Widerstandsklasse für den Einbruchschutz gemäß der nationalen oder regionalen Richtlinie die als Mindestanforderung für die Einbruchhemmung der Tür gewährleistet sein muss."@de-DE , "Système de classification par indices, indiquant le niveau de sécurité."@fr-FR , "防犯等級情報。関連する基準を参照。"@ja-JP , "Sicherheitsklasse gemäß der nationalen oder regionalen Gebäudesicherheitsverordnung."@de-DE ;
        rdfs:label             "NiveauSecurite"@fr-FR , "安全等级"@zh-CN , "Widerstandsklasse"@de-DE , "Sicherheitsklasse"@de-DE , "securityRating"@en , "防犯等級"@ja-JP ;
        rdfs:range             xsd:string ;
        schema:domainIncludes  <https://w3id.org/product/Door> , <https://w3id.org/product/Window> .

props:hasNonSkidSurface
        a                      owl:DatatypeProperty ;
        rdfs:comment           "German-description-11"@de-DE , "Indique si le revêtement de surface est anti dérapant (VRAI) ou non (FAUX)"@fr-FR , "スリップ防止のための表面仕上げをしているかどうかのブーリアン値。"@ja-JP , "表示表面处理是否设计为防滑的。"@zh-CN , "Angabe, ob der Bodenbelag eine nichtrutschende Oberfläche hat (JA), oder nicht (NEIN)."@de-DE , "Indique si le revêtement de surface est anti dérapant (VRAI) ou non (FALSE)"@fr-FR , "German-description-8"@de-DE , "Indication whether the surface finish is designed to prevent slippery (TRUE) or not (FALSE)."@en , "Indique si la finition est conçue pour être anti dérapante (VRAI) ou non (FAUX)."@fr-FR ;
        rdfs:label             "Anti dérapant"@fr-FR , "hasNonSkidSurface"@en , "AntiDerapant"@fr-FR , "滑り止め表面加工区分"@ja-JP , "表面是否防滑"@zh-CN , "Nichtrutschende Oberfläche"@de-DE ;
        rdfs:range             xsd:boolean ;
        schema:domainIncludes  <https://w3id.org/product/Stair> , <https://w3id.org/product/Covering%2FFLOORING> , <https://w3id.org/product/Ramp> .

props:spaceRelativeHumidity
        a                      owl:DatatypeProperty ;
        rdfs:comment           "The relative humidity of the space."@en , "室内の相対湿度"@ja-JP ;
        rdfs:label             "spaceRelativeHumidity"@en , "室内相対湿度"@ja-JP ;
        schema:domainIncludes  <https://w3id.org/product/Space> .

props:airFlowrateRange
        a                      owl:DatatypeProperty ;
        rdfs:comment           "操作されるターミナル内の空気流の範囲"@ja-JP , "Possible range of airflow that can be delivered."@en , "Air flowrate range within which the air terminal is designed to operate."@en , "Plage de débit de ventilation dans laquelle le terminal de ventilation est prévu de fonctionner."@fr-FR , "送風可能な風量範囲"@ja-JP ;
        rdfs:label             "流量範囲"@ja-JP , "PlageDébitVentilation"@fr-FR , "airFlowrateRange"@en ;
        schema:domainIncludes  <https://w3id.org/product/DuctSilencer> , <https://w3id.org/product/AirTerminal> .

props:timeTolerance1  a        owl:DatatypeProperty ;
        rdfs:comment           "[%] 시간 / 특성 곡선의 허용 시간을 설정"@ko-KR , "The tolerance for the time of time/current-curve in [%]."@en , "[％]で時間/特性曲線の許容時間を設定"@ja-JP , "[％]で時間/特性曲線の許容時間を設定。"@ja-JP ;
        rdfs:label             "timeTolerance1"@en , "許容時間1"@ja-JP , "허용 시간1"@ko-KR ;
        rdfs:range             <https://w3id.org/product/PositiveRatioMeasure> ;
        schema:domainIncludes  <https://w3id.org/product/ProtectiveDeviceTrippingUnit> .

props:skirtingBoardHeight
        a                      owl:DatatypeProperty ;
        rdfs:comment           "Angabe der  Höhe der umlaufenden Sockelleiste. \n\nDer Höhenparameter wird übernommen, wenn kein eigenes Bekleidungsobjekt (IfcCovering mit PredefinedType = SKIRTINGBOARD) für die Sockelleiste dem Raum zugeordnet ist. Bei Inkonsistenzen (wenn beides gegeben ist), hat die Höhe des zugeordneten Bekleidungsobjekts Priorität."@de-DE , "Height of the skirting board.\n\nThe height information is provided in absence of an IfcCovering (type=SKIRTINGBOARD) object with own shape representation and material assignment. In case of inconsistency the height assigned to IfcCovering elements takes precedence."@en , "部屋の幅木の高さ。\n\n形状表現を持つIfcCovering(type=SKIRTINGBOARD)オブジェクトが存在しない場合に与えられる厚さ情報。IfcCoveringの幾何形状パラメータとこのプロパティ値が一致しない場合、幾何形状パラメータの値を優先する。"@ja-JP ;
        rdfs:label             "skirtingBoardHeight"@en , "Höhe der Sockelleite"@de-DE , "幅木材高"@ja-JP , "Hauteur de la plinthe"@fr-FR ;
        rdfs:range             <https://w3id.org/product/PositiveLengthMeasure> ;
        schema:domainIncludes  <https://w3id.org/product/Space> .

props:junctionType  a          owl:DatatypeProperty ;
        rdfs:comment           "The type of junction. TEE=3 ports, CROSS = 4 ports."@en , "接合のタイプ　(T継ぎ手は3本　十字継ぎ手は4本)"@ja-JP ;
        rdfs:label             "junctionType"@en , "継ぎ手タイプ"@ja-JP ;
        schema:domainIncludes  <https://w3id.org/product/PipeFitting%2FJUNCTION> .

props:landTitleID  a           owl:DatatypeProperty ;
        rdfs:comment           "Identification number assigned by the statutory registration authority to the title to a land parcel."@en , "등기소의 ID입니다."@ko-KR , "登記所による識別番号。"@ja-JP , "Identifiant numérique du titre de la parcelle attribué par une autorité."@fr-FR ;
        rdfs:label             "IdTitreParcelle"@fr-FR , "landTitleID"@en , "부지 번호 ID"@ko-KR , "敷地番号ID"@ja-JP ;
        rdfs:range             xsd:string ;
        schema:domainIncludes  <https://w3id.org/product/Site> .

props:crossSectionalArea
        a                      owl:DatatypeProperty ;
        rdfs:comment           "Cross section area of the phase(s) lead(s)."@en , "位相、リードの断面積。"@ja-JP , "리드 단면적."@ko-KR ;
        rdfs:label             "crossSectionalArea"@en , "断面積"@ja-JP , "단면적 영역"@ko-KR ;
        rdfs:range             <https://w3id.org/product/AreaMeasure> ;
        schema:domainIncludes  <https://w3id.org/product/CableSegment%2FCONDUCTORSEGMENT> .

props:designLocationNumber
        a                      owl:DatatypeProperty ;
        rdfs:comment           "Defines a unique location within a structure, the ‘slot’ for which the piece was designed."@en ;
        rdfs:label             "designLocationNumber"@en ;
        rdfs:range             xsd:string ;
        schema:domainIncludes  <https://w3id.org/product/BuildingElement> .

props:outletTemperatureRange
        a                      owl:DatatypeProperty ;
        rdfs:comment           "Allowable outlet temperature of either the water or the steam."@en , "水または蒸気のどちらかの許容出口温度"@ja-JP , "Température admissible de sortie de l'eau ou de la vapeur"@fr-FR ;
        rdfs:label             "outletTemperatureRange"@en , "出口温度範囲"@ja-JP , "PlageTempératureSortie"@fr-FR ;
        schema:domainIncludes  <https://w3id.org/product/Boiler> .

props:hollowCorePlugging
        a                      owl:DatatypeProperty ;
        rdfs:comment           "A descriptive label for how the hollow core ends are treated: they may be left open, closed with a plug, or sealed with cast concrete. Values would be, for example: 'Unplugged', 'Plugged', 'SealedWithConcrete'. This property applies to  hollow core slabs only."@en , "（定着部の？）くぼみをどのように扱うのかについて書かれたラベル：開けたままにするか、プラグで塞ぐ、または後詰めコンクリートで塞ぐ。例えば、「塞がない」、「塞ぐ」、「コンクリートで塞ぐ」と書かれるだろう。この属性はスラブに開けられたくぼみにも適用される。"@ja-JP ;
        rdfs:label             "hollowCorePlugging"@en , "くぼみの充填"@ja-JP ;
        rdfs:range             xsd:string ;
        schema:domainIncludes  <https://w3id.org/product/BuildingElement> .

props:value  a                 owl:DatatypeProperty ;
        rdfs:comment           "The expected range and default value.  While the property data type is IfcReal (to support all cases including when the units are unknown), a unit may optionally be provided to indicate the measure and unit.  The LowerLimitValue and UpperLimitValue must fall within the physical Range and may be used to determine extents when charting Pset_ControllerPHistory.Value."@en , "Indicates measured values over time which may be recorded continuously or only when changed beyond a particular deadband."@en , "The default value such as normally-closed or normally-open."@en , "The expected range and default value.  While the property data type is IfcReal (to support all cases including when the units are unknown), a unit may optionally be provided to indicate the measure and unit."@en , "시간이 지남에 오류 상태를 나타내는 Pset_ControllerTypeValue.Fault에 대응 ※ 설정 가능한 정보는 IfcTimeSeries 속성 참조"@ko-KR , "Indicates sensed values over time which may be recorded continuously or only when changed beyond a particular deadband.  The range of possible values is defined by the SetPoint property of the corresponding sensor type property set."@en , "Indicates values over time which may be recorded continuously or only when changed beyond a particular deadband.  The range of possible values is defined by the Value property on the corresponding occurrence property set (Pset_ControllerTypeFloating, Pset_ControllerTypeProportional, Pset_ControllerTypeMultiPosition, or Pset_ControllerTypeTwoPosition)."@en , "時間とともに値を示す。\nPset_ControllerTypeValue.Valueに対応\n※ 設定可能情報は IfcTimeSeriesプロパティ参照"@ja-JP , "The expected range and default value.  The LowerLimitValue and UpperLimitValue must fall within the physical Range."@en ;
        rdfs:label             "value"@en , "이상 출력 시계열 상수"@ko-KR , "デフォルト出力時系列定数"@ja-JP ;
        rdfs:range             xsd:boolean ;
        schema:domainIncludes  <https://w3id.org/product/Controller%2FMULTIPOSITION> , <https://w3id.org/product/Controller%2FFLOATING> , <https://w3id.org/product/Controller> , <https://w3id.org/product/Controller%2FPROPORTIONAL> , <https://w3id.org/product/Sensor> , <https://w3id.org/product/Controller%2FTWOPOSITION> , <https://w3id.org/product/FlowInstrument> .

props:contrastRatio  a         owl:DatatypeProperty ;
        rdfs:comment           "Indicates the display contrast ratio."@en , "コントラスト比を示す。"@ja-JP , "명암비를 보여준다"@ko-KR ;
        rdfs:label             "contrastRatio"@en , "コントラスト比"@ja-JP , "명암비"@ko-KR ;
        rdfs:range             <https://w3id.org/product/PositiveRatioMeasure> ;
        schema:domainIncludes  <https://w3id.org/product/AudioVisualAppliance%2FDISPLAY> .

props:actualCost  a            owl:DatatypeProperty ;
        rdfs:comment           "The actual cost on behalf of the resource allocation."@en , "資源配分のための実績のコスト。"@ja-JP ;
        rdfs:label             "actualCost"@en , "実績コスト"@ja-JP ;
        schema:domainIncludes  <https://w3id.org/product/ConstructionResource> .

props:nominalHeatTransferArea
        a                      owl:DatatypeProperty ;
        rdfs:comment           "設計全熱交換係数の設計熱交換面積"@ja-JP , "Nominal heat transfer surface area associated with nominal overall heat transfer coefficient."@en ;
        rdfs:label             "設計熱交換面積"@ja-JP , "nominalHeatTransferArea"@en ;
        rdfs:range             <https://w3id.org/product/AreaMeasure> ;
        schema:domainIncludes  <https://w3id.org/product/Evaporator> , <https://w3id.org/product/Condenser> .

props:numberOfTreads  a        owl:DatatypeProperty ;
        rdfs:comment           "Total number of treads included in the stair flight."@en , "Nombre total de girons de l'escalier"@fr-FR , "階段の踏面数。"@ja-JP , "该梯段所包含的踏板总数。"@zh-CN , "German-description-3"@de-DE , "该楼梯所包含的踏板总数。"@zh-CN , "Total number of treads included in the stair."@en ;
        rdfs:label             "Anzahl der Auftritte"@de-DE , "踏板数"@zh-CN , "踏面数"@ja-JP , "NombreGirons"@fr-FR , "numberOfTreads"@en ;
        rdfs:range             <https://w3id.org/product/CountMeasure> ;
        schema:domainIncludes  <https://w3id.org/product/StairFlight> , <https://w3id.org/product/Stair> .

props:primarySurfaceArea
        a                      owl:DatatypeProperty ;
        rdfs:comment           "Primary heat transfer surface area of the tubes and headers."@en , "Surface d'échange thermique au primaire des tubes et aux collecteurs."@fr-FR ;
        rdfs:label             "primarySurfaceArea"@en , "SurfaceEchangePrimaire"@fr-FR ;
        rdfs:range             <https://w3id.org/product/AreaMeasure> ;
        schema:domainIncludes  <https://w3id.org/product/Coil> .

props:gasDetected  a           owl:DatatypeProperty ;
        rdfs:comment           "Identification of the gas that is being detected, according to chemical formula.  For example, carbon monoxide is 'CO', carbon dioxide is 'CO2', oxygen is 'O2'."@en , "検出されているガスの識別。"@ja-JP ;
        rdfs:label             "gasDetected"@en , "対象ガス"@ja-JP ;
        rdfs:range             xsd:string ;
        schema:domainIncludes  <https://w3id.org/product/Sensor%2FGASSENSOR> .

props:isRigid  a               owl:DatatypeProperty ;
        rdfs:comment           "Indication of whether the conduit is rigid (= TRUE) or flexible (= FALSE)."@en , "鋼管か否か。"@ja-JP ;
        rdfs:label             "isRigid"@en , "鋼管"@ja-JP , "강관"@ko-KR ;
        rdfs:range             xsd:boolean ;
        schema:domainIncludes  <https://w3id.org/product/CableCarrierSegment%2FCONDUITSEGMENT> .

props:operatingMode  a         owl:DatatypeProperty ;
        rdfs:comment           "Identifies the operating mode of the boiler."@en , "ボイラの動作モードのID　（固定、２段階、比例．．．）"@ja-JP , "Identifie le mode de fonctionnement de la chaudière."@fr-FR ;
        rdfs:label             "operatingMode"@en , "動作モード"@ja-JP , "ModeFonctionnement"@fr-FR ;
        schema:domainIncludes  <https://w3id.org/product/Boiler> .

props:junctionLeftRadius
        a                      owl:DatatypeProperty ;
        rdfs:comment           "The radius of bending for the left junction."@en , "左継ぎ手の曲がりの半径"@ja-JP ;
        rdfs:label             "junctionLeftRadius"@en , "左継ぎ手半径"@ja-JP ;
        rdfs:range             <https://w3id.org/product/PositiveLengthMeasure> ;
        schema:domainIncludes  <https://w3id.org/product/PipeFitting%2FJUNCTION> .

props:assessmentCondition
        a                      owl:DatatypeProperty ;
        rdfs:comment           "The overall condition of a product based on an assessment of the contributions to the overall condition made by the various criteria considered. The meanings given to the values of assessed condition should be agreed and documented by local agreements. For instance, is overall condition measured on a scale of 1 - 10 or by assigning names such as Good, OK, Poor."@en , "様々な基準を用いた評価による製品に関する全体的な状態。評価された状態値の意味は、ローカル協定によって同意され、文書化されなければならない。例えば、状態を1から10の値で計測したり、Good, Ok, Poor等で表す。"@ja-JP ;
        rdfs:label             "assessmentCondition"@en , "評価状態"@ja-JP ;
        rdfs:range             xsd:string ;
        schema:domainIncludes  <https://w3id.org/product/Element> .

props:twisting  a              owl:DatatypeProperty ;
        rdfs:comment           "The angle, in radians, through which the end face of a precast piece is rotated with respect to its starting face, along its longitudinal axis, as a result of non-aligned supports. This measure is also termed the ‘warping’ angle."@en ;
        rdfs:label             "twisting"@en ;
        rdfs:range             <https://w3id.org/product/PlaneAngleMeasure> ;
        schema:domainIncludes  <https://w3id.org/product/BuildingElement> .

props:condenserEnteringTemperature
        a                      owl:DatatypeProperty ;
        rdfs:comment           "Temperature of fluid entering condenser."@en , "凝縮器入口流体温度"@ja-JP ;
        rdfs:label             "condenserEnteringTemperature"@en , "凝縮器入口温度"@ja-JP ;
        rdfs:range             <https://w3id.org/product/ThermodynamicTemperatureMeasure> ;
        schema:domainIncludes  <https://w3id.org/product/UnitaryEquipment%2FAIRCONDITIONINGUNIT> .

props:a  a                     owl:DatatypeProperty ;
        rdfs:comment           "Measure a according to ISO 2553"@en ;
        rdfs:label             "a"@en ;
        rdfs:range             <https://w3id.org/product/PositiveLengthMeasure> ;
        schema:domainIncludes  <https://w3id.org/product/Fastener%2FWELD> .

props:nominalReturnWaterTemperatureCooling
        a                      owl:DatatypeProperty ;
        rdfs:comment           "Nominal return water temperature (refers to nominal cooling capacity)."@en ;
        rdfs:label             "nominalReturnWaterTemperatureCooling"@en ;
        rdfs:range             <https://w3id.org/product/ThermodynamicTemperatureMeasure> ;
        schema:domainIncludes  <https://w3id.org/product/CooledBeam> .

props:headroom  a              owl:DatatypeProperty ;
        rdfs:comment           "Actual headroom clearance for the passageway according to the current design. \nThe shape information is provided in addition to the shape representation and the geometric parameters used within. In cases of inconsistency between the geometric parameters and the shape properties, provided in the attached property, the geometric parameters take precedence."@en , "現状の設計に一致した斜路の実際の頭上スペース高\n形状の情報は、内側は使用される形表現および幾何パラメータ学的媒介変数に加えて提供されます。\n幾何パラメータと形状プロパティが矛盾する場合は、付属のプロパティで提供されている、幾何パラメータを優先する。"@ja-JP , "当前设计方案确定的通道实际净空高度。\n该属性所提供的形状信息是对内部形状描述和几何参数的补充。如果几何参数与该属性所提供的形状属性不符，应以几何参数为准。"@zh-CN , "German-description-2"@de-DE , "German-description-10"@de-DE , "Hauteur de passage (échappée) actuellement projetée. Cette propriété est donnée en complément de la représentation de la forme de l'élément et des paramètres géométriques qui la déterminent. En cas d'incohérence entre ces paramètres géométriques et cette propriété, ce sont les paramètres géométriques qui priment."@fr-FR ;
        rdfs:label             "頭上スペース"@ja-JP , "headroom"@en , "净空"@zh-CN , "HauteurPassage"@fr-FR , "Durchgangshöhe"@de-DE ;
        rdfs:range             <https://w3id.org/product/PositiveLengthMeasure> ;
        schema:domainIncludes  <https://w3id.org/product/RampFlight> , <https://w3id.org/product/StairFlight> .

props:productionYear  a        owl:DatatypeProperty ;
        rdfs:comment           "The year of production of the manufactured item."@en ;
        rdfs:label             "productionYear"@en ;
        rdfs:range             xsd:string ;
        schema:domainIncludes  <https://w3id.org/product/Element> .

props:yearOfLastRefurbishment
        a                      owl:DatatypeProperty ;
        rdfs:comment           "Year of last major refurbishment, or reconstruction, of the building (applies to reconstruction works)."@en , "Jahr der letzten Renovierung des Gebäudes."@de-DE , "Année de la dernière rénovation majeure ou de la reconstruction du bâtiment."@fr-FR ;
        rdfs:label             "yearOfLastRefurbishment"@en , "letztes Renovierungsjahr"@de-DE , "Année de la dernière rénovation"@fr-FR ;
        rdfs:range             xsd:string ;
        schema:domainIncludes  <https://w3id.org/product/Building> .

props:nominalParticleGeometricStandardDeviation
        a                      owl:DatatypeProperty ;
        rdfs:comment           "Particle geometric standard deviation associated with nominal efficiency."@en ;
        rdfs:label             "nominalParticleGeometricStandardDeviation"@en ;
        rdfs:range             xsd:decimal ;
        schema:domainIncludes  <https://w3id.org/product/Filter> .

props:operationalCriteria
        a                      owl:DatatypeProperty ;
        rdfs:comment           "Time of operation at maximum operational ambient air temperature."@en , "最大動作周囲温度での動作の時間"@ja-JP ;
        rdfs:label             "operationalCriteria"@en , "動作環境"@ja-JP ;
        rdfs:range             <https://w3id.org/product/TimeMeasure> ;
        schema:domainIncludes  <https://w3id.org/product/Fan> .

props:thickness1  a            owl:DatatypeProperty ;
        rdfs:comment           "First thickness parameter of a surface member with varying thickness"@en ;
        rdfs:label             "thickness1"@en ;
        rdfs:range             <https://w3id.org/product/PositiveLengthMeasure> ;
        schema:domainIncludes  <https://w3id.org/product/StructuralSurfaceMemberVarying> .

props:transformerVectorGroup
        a                      owl:DatatypeProperty ;
        rdfs:comment           "List of the possible vector groups for the transformer from which that required may be set. Values in the enumeration list follow a standard international code where the first letter  describes how the primary windings are connected,\nthe second letter describes how the secondary windings are connected, and the numbers describe the rotation of voltages and currents from the primary to the secondary side in multiples of 30 degrees.\n\nD: means that the windings are delta-connected.\nY: means that the windings are star-connected. \nZ: means that the windings are zig-zag connected (a special start-connected providing low reactance of the transformer); \nThe connectivity is only relevant for three-phase transformers."@en ;
        rdfs:label             "transformerVectorGroup"@en ;
        schema:domainIncludes  <https://w3id.org/product/Transformer> .

props:adjustmentValueType
        a                      owl:DatatypeProperty ;
        rdfs:comment           "The type of adjustment value that is applied through the property set. This determines the properties that should be asserted (see below)."@en , "調整値のタイプを設定。"@ja-JP , "조정 값 유형을 설정합니다."@ko-KR ;
        rdfs:label             "adjustmentValueType"@en , "調整値の型"@ja-JP , "조정 형식"@ko-KR ;
        schema:domainIncludes  <https://w3id.org/product/ProtectiveDeviceTrippingUnit> .

props:position  a              owl:DatatypeProperty ;
        rdfs:comment           "Indicates position of the actuator over time where 0.0 is fully closed and 1.0 is fully open."@en , "アクチュエータの時間ごとの位置を示す値。0.0が完全に閉じられた状態で、1.0が完全に開いた状態。"@ja-JP , "해당 프로젝트에서 사용이 유형에 대한 참조 ID (예 : 'A-1') ※ 기본이있는 경우 그 기호를 사용"@ko-KR ;
        rdfs:label             "position"@en , "位置"@ja-JP , "참조 ID"@ko-KR ;
        schema:domainIncludes  <https://w3id.org/product/Actuator> .

props:setPointConductance
        a                      owl:DatatypeProperty ;
        rdfs:comment           "The fill level value to be sensed. Use IfcPropertyBoundedValue.SetPointValue to set the set point value."@en , "感知される電気伝導率。\nセットポイント値を置くために、IfcPropertyBoundedValue.SetPointValueを使用する。"@ja-JP , "감지되는 전기 전도율. 세트 포인트 값을 넣으려면, IfcPropertyBoundedValue.SetPointValue를 사용하십시오."@ko-KR ;
        rdfs:label             "setPointConductance"@en , "電気伝導率設定値"@ja-JP , "전기 전도율 설정"@ko-KR ;
        schema:domainIncludes  <https://w3id.org/product/Sensor%2FCONDUCTANCESENSOR> .

props:electricity  a           owl:DatatypeProperty ;
        rdfs:comment           "The amount of electricity consumed during the period specified in the time series."@en , "특정 기간 동안의 전력 소비."@ko-KR ;
        rdfs:label             "electricity"@en , "전력 소비량"@ko-KR ;
        schema:domainIncludes  <https://w3id.org/product/Building> .

props:waterConsumption
        a                      owl:DatatypeProperty ;
        rdfs:comment           "사용 수량의 리터 수"@ko-KR , "Quantité d'eau utilisée [NDT : telle que définie dans la norme NF P01-010]"@fr-FR , "Quantity of water used."@en , "水の消費量。"@ja-JP ;
        rdfs:label             "물 사용"@ko-KR , "waterConsumption"@en , "水消費量"@ja-JP , "ConsommationEau"@fr-FR ;
        rdfs:range             <https://w3id.org/product/VolumeMeasure> ;
        schema:domainIncludes  <https://w3id.org/product/Element> .

props:compartmentation
        a                      owl:DatatypeProperty ;
        rdfs:comment           "Angabe, ob dieses Bauteil einen Brandabschnitt begrenzt (WAHR), oder nicht (FALSCH)."@de-DE , "部材が防火区画として用いられるかどうかを示すブーリアン値（TRUE or False)。"@ja-JP , "Indication whether the object is designed to serve as a fire compartmentation (TRUE) or not (FALSE)."@en , "Indique si l'objet est conçu  pour assurer un compartimentage contre l'incendie (VRAI) ou non (FAUX)."@fr-FR , "防火区画を考慮した部材かどうかを示すブーリアン値"@ja-JP ;
        rdfs:label             "compartmentation"@en , "Brandabschnittsdefinierendes Bauteil"@de-DE , "Compartimentage"@fr-FR , "防火区画"@ja-JP ;
        rdfs:range             xsd:boolean ;
        schema:domainIncludes  <https://w3id.org/product/Wall> , <https://w3id.org/product/Slab> .

props:lightEmitterNominalPower
        a                      owl:DatatypeProperty ;
        rdfs:comment           "Light emitter nominal power."@en , "発光するための定格ワット数"@ja-JP , "발광하는 정격 와트"@ko-KR ;
        rdfs:label             "lightEmitterNominalPower"@en , "照明器具ワット数"@ja-JP , "조명기구 와트"@ko-KR ;
        rdfs:range             <https://w3id.org/product/PowerMeasure> ;
        schema:domainIncludes  <https://w3id.org/product/Lamp> .

props:appliancePercentLoadToRadiant
        a                      owl:DatatypeProperty ;
        rdfs:comment           "Percent of sensible load to radiant heat."@en , "放射熱のうち顕熱分負荷の割合。"@ja-JP , "복사열 중 현열 분 부하의 비율."@ko-KR ;
        rdfs:label             "appliancePercentLoadToRadiant"@en , "放射熱のうち顕熱分の割合"@ja-JP , "복사열 중 현열 분의 비율"@ko-KR ;
        rdfs:range             <https://w3id.org/product/PositiveRatioMeasure> ;
        schema:domainIncludes  <https://w3id.org/product/SpatialElement> .

props:fluidPressureRange
        a                      owl:DatatypeProperty ;
        rdfs:comment           "Allowable water working pressure range inside the tube."@en , "Plage de pression hydraulique fonctionnelle admissible dans le tube."@fr-FR ;
        rdfs:label             "fluidPressureRange"@en , "PlagePressionFluide"@fr-FR ;
        schema:domainIncludes  <https://w3id.org/product/Coil> .

props:electricalSystemType
        a                      owl:DatatypeProperty ;
        rdfs:comment           "For certain purposes of electrical regulations, IEC 60364 defines types of system using type identifiers. Assignment of identifiers depends upon the relationship of the source, and of exposed conductive parts of the installation, to Ground (Earth).   Identifiers that may be assigned through IEC 60364 are: \n\n•TN type system, a system having one or more points of the source of energy directly earthed, the exposed conductive parts of the installation being connected to that point by protective conductors, \n•TN C type system, a TN type system in which neutral and protective functions are combined in a single conductor throughout the system, \n•TN S type system, a TN type system having separate neutral and protective conductors throughout the system, \n•TN C S type system, a TN type system in which neutral and protective functions are combined in a single conductor in part of the system, \n•TT type system, a system having one point of the source of energy directly earthed, the exposed conductive parts of the installation being connected to earth electrodes electrically independent of the earth electrodes of the source, \n•IT type system, a system having no direct connection between live parts and Earth, the exposed conductive parts of the electrical installation being earthed."@en , "IEC60364電気基準に定義した電気接地の方式。電気設備の種類、接地電極と設備の導電性部分の種類で決められる。具体的なには、IEC60364に下記のような方法がある：\n\n\n- TNシステム：電気設備は一点或いは多点の接地点を持ち、直接接地されるシステム。設備と接地極の導電性部分は保護されていること。\n- TN　Cシステム：系統の全てにわたって、中性線と保護導体が一つの導体のTNシステム。\n- TN　Sシステム：系統の全てにわたって、独立の中性線と保護導体を有するTNシステム。\n- TN　C　Sシステム：系統の一部では、中性線と保護導体が一つの導体のTNシステム。\n- TTシステム：一点を大地に直接接続し、電力系統の接地とは無関係に、設備の露出導電性部分を大地に直接接地すること。\n- ITシステム：電力システムを大地(接地)から絶縁する、設備の露出導電性部分を大地に直接接地すること。"@ja-JP , "IEC60364 전기 기준으로 정의한 전기 접지 방식. 전기 설비의 종류, 접지 전극 시설의 도전성 부분 유형에 결정된다. 구체적인에는 IEC60364에 다음과 같은 방법이있다. · TN 시스템 : 전기 설비는한데 또는 다점 접지 점을 가지고 직접 접지되는 시스템. 시설과 접지극의 도전성 부분을 보호하는 것. · TN C 시스템 : 계통의 모든 걸쳐 중성선과 보호 도체가 하나의 도체 TN 시스템. · TN S 시스템 : 계통의 모든 걸쳐 독립 중성선과 보호 도체가있는 TN 시스템. · TN C S 시스템 : 계통의 일부가, 중성선과 보호 도체가 하나의 도체 TN 시스템. · TT 시스템 : 한 점을 대지에 직접 연결하여 전력 계통의 접지와는 상관없이 설비의 노출 도전성 부분을 대지에 직접 접지한다. · IT 시스템 : 전력 시스템을 대지 (접지)로부터 절연하는 설비의 노출 도전성 부분을 대지에 직접 접지한다."@ko-KR ;
        rdfs:label             "electricalSystemType"@en , "電気システム方式"@ja-JP , "전기 시스템 방식"@ko-KR ;
        schema:domainIncludes  <https://w3id.org/product/DistributionSystem%2FELECTRICAL> .

props:totalHeatingCapacity
        a                      owl:DatatypeProperty ;
        rdfs:comment           "Total heating capacity. This includes heating capacity of beam and heating capacity of supply air."@en ;
        rdfs:label             "totalHeatingCapacity"@en ;
        schema:domainIncludes  <https://w3id.org/product/CooledBeam> .

props:contactorType  a         owl:DatatypeProperty ;
        rdfs:comment           "A list of the available types of contactor from which that required may be selected where:\n\nCapacitorSwitching: for switching 3 phase single or multi-step capacitor banks.\nLowCurrent: requires the use of low resistance contacts.\nMagneticLatching: enables the contactor to remain in the on position when the coil is no longer energized.\nMechanicalLatching: requires that the contactor is mechanically retained in the on position.\nModular: are totally enclosed and self contained.\nReversing: has a double set of contactors that are prewired.\nStandard: is a generic device that controls the flow of power in a circuit on or off."@en , "以下より選択が必要となる、接触器の一覧リスト：\n\nコンデンサスイッチ：3つのシングルフェーズまたは複数のコンデンサバンクで切り替える。\n低流：低い抵抗接触の使用が必要\nマグネット式：コイルのエネルギーが無くなった時に切替をONポジションにして有効にする\nMechanicalLatching：切替器がONポジションを維持するために機械的な仕組みが必要。\nモジュール式：閉鎖されている自働型切替器。\nリバース：2つの切替器をワイヤーで接続したもの。\n標準：回路で電力潮流をオンまたはオフでコントロールする一般的な装置。"@ja-JP , "다음에서 선택이 필요하다, 접촉기  목록 : 콘덴서 스위치 : 3 개의 단일 위상 이상의 커패시터 뱅크를 전환합니다. 낮은여 : 낮은 저항 접촉 사용해야 마그네틱 : 코일의 에너지가 분실된 때 전환을 ON 위치로하여 사용 MechanicalLatching : 판을 ON 위치를 유지하기 위해 기계적인 구조가 필요합니다. 모듈형 : 폐쇄되어있는 자신 동형 판. 리버스 : 두 판을 와이어로 연결한 것. 표준 : 회로에서 전력 조류를 켜지거나 꺼지지 컨트롤하는 일반적인 장치"@ko-KR ;
        rdfs:label             "contactorType"@en , "接触器タイプ"@ja-JP , "접촉기 유형"@ko-KR ;
        schema:domainIncludes  <https://w3id.org/product/SwitchingDevice%2FCONTACTOR> .

props:hoseReelMountingType
        a                      owl:DatatypeProperty ;
        rdfs:comment           "Identifies the predefined types of hose reel mounting from which the type required may be set."@en , "あらかじめ定義済みの取り付けホースリールの型から必要な型を設定する識別。"@ja-JP ;
        rdfs:label             "hoseReelMountingType"@en , "ホースリール装着タイプ"@ja-JP ;
        schema:domainIncludes  <https://w3id.org/product/FireSuppressionTerminal%2FHOSEREEL> .

props:vaporPermeability
        a                      owl:DatatypeProperty ;
        rdfs:comment           "The rate of water vapor transmission per unit area per unit of vapor pressure differential under test conditions."@en ;
        rdfs:label             "vaporPermeability"@en ;
        rdfs:range             <https://w3id.org/product/VaporPermeabilityMeasure> ;
        schema:domainIncludes  <https://w3id.org/product/Material> .

props:hasIntegralShutOffDevice
        a                      owl:DatatypeProperty ;
        rdfs:comment           "Indication of whether the flushing valve has an integral shut off device fitted (set TRUE) or not (set FALSE)."@en , "フラッシュ弁に全体閉止装置がついているかどうかの表示（付きTRUE）又は（無しFALSE）"@ja-JP ;
        rdfs:label             "hasIntegralShutOffDevice"@en , "全体閉止装置がついているかどうか"@ja-JP ;
        rdfs:range             xsd:boolean ;
        schema:domainIncludes  <https://w3id.org/product/Valve%2FFLUSHING> .

props:serviceLifeDuration
        a                      owl:DatatypeProperty ;
        rdfs:comment           "The length or duration of a service life.  \n\nThe lower bound indicates pessimistic service life, the upper bound indicates optimistic service life, and the setpoint indicates the typical service life."@en ;
        rdfs:label             "serviceLifeDuration"@en ;
        schema:domainIncludes  <https://w3id.org/product/Element> .

props:momentOfInertiaZ
        a                      owl:DatatypeProperty ;
        rdfs:comment           "Moment of inertia about zs (second moment of area, about zs). For example measured in mm4"@en ;
        rdfs:label             "momentOfInertiaZ"@en ;
        rdfs:range             <https://w3id.org/product/MomentOfInertiaMeasure> ;
        schema:domainIncludes  <https://w3id.org/product/ProfileDef> .

props:inletPatternType
        a                      owl:DatatypeProperty ;
        rdfs:comment           "Identifies the pattern of inlet connections to a trap.\n\nA trap may have 0,1,2,3 or 4 inlet connections and the pattern of their arrangement may vary. The enumeration makes the convention that an outlet is either vertical or is placed at the bottom (south side) of the trap (when viewed in plan). Position 1 is to the left (west), position 2 is to the top (north), position 3 is to the right (east) and position 4 is to the bottom (south)."@en , "防臭弁の吸気口接続口の識別情報。\n\n一つの防臭弁に0.1.2.3.4.の吸気口接続口とパターンがあるときは変化する可能性があります。羅列されるとき、接続口が垂直である様子か、防臭弁の底（南）におかれます。位置1は左(西)に、位置2は上方(北)に、位置3は右(東)に、位置4は下方(南）になる。"@ja-JP ;
        rdfs:label             "inletPatternType"@en , "吸気口種類"@ja-JP ;
        schema:domainIncludes  <https://w3id.org/product/WasteTerminal%2FFLOORTRAP> .

props:inPlaneNegative
        a                      owl:DatatypeProperty ;
        rdfs:comment           "Mechanical properties with respect to in-plane load, i.e. bending about the strong axis; compression zone of unbalanced layups is stressed in tension."@en ;
        rdfs:label             "inPlaneNegative"@en ;
        schema:domainIncludes  <https://w3id.org/product/Material%2FWood> .

props:shortInsideCenterTopBarPitch
        a                      owl:DatatypeProperty ;
        rdfs:comment           "The pitch length of the short inside center top bar."@en , "短辺方向・柱間帯・上端中央の鉄筋間隔。"@ja-JP ;
        rdfs:label             "shortInsideCenterTopBarPitch"@en , "短辺・柱列帯・上端中央ピッチ"@ja-JP ;
        rdfs:range             <https://w3id.org/product/PositiveLengthMeasure> ;
        schema:domainIncludes  <https://w3id.org/product/Slab> .

props:shortInsideEndTopBarPitch
        a                      owl:DatatypeProperty ;
        rdfs:comment           "The pitch length of the short inside end top bar."@en , "短辺方向・柱間帯・上端端部の鉄筋間隔。"@ja-JP ;
        rdfs:label             "shortInsideEndTopBarPitch"@en , "短辺・柱列帯・上端端部ピッチ"@ja-JP ;
        rdfs:range             <https://w3id.org/product/PositiveLengthMeasure> ;
        schema:domainIncludes  <https://w3id.org/product/Slab> .

props:columnShoeCasingDepth
        a                      owl:DatatypeProperty ;
        rdfs:comment           "The depth of the column shoe casing."@en , "柱脚ケーシングの成。"@ja-JP , "기둥 다리 케이스의 구성"@ko-KR ;
        rdfs:label             "columnShoeCasingDepth"@en , "ケーシング成"@ja-JP , "케이스 구성"@ko-KR ;
        rdfs:range             <https://w3id.org/product/PositiveLengthMeasure> ;
        schema:domainIncludes  <https://w3id.org/product/DiscreteAccessory%2FSHOE> .

props:connectionSize  a        owl:DatatypeProperty ;
        rdfs:comment           "ポンプの入出の接続サイズ"@ja-JP , "Defines the size of inlet and outlet pipe connections to the meter."@en , "Duct connection diameter."@en , "Size of the inlet connection to the sprinkler."@en , "The connection size of the to and from the pump."@en , "スプリンクラーへの入口接続のサイズ。"@ja-JP ;
        rdfs:label             "接続サイズ"@ja-JP , "connectionSize"@en ;
        rdfs:range             <https://w3id.org/product/PositiveLengthMeasure> , <https://w3id.org/product/LengthMeasure> ;
        schema:domainIncludes  <https://w3id.org/product/CooledBeam%2FACTIVE> , <https://w3id.org/product/FireSuppressionTerminal%2FSPRINKLER> , <https://w3id.org/product/FlowMeter%2FGASMETER> , <https://w3id.org/product/FlowMeter%2FWATERMETER> , <https://w3id.org/product/Pump> , <https://w3id.org/product/FlowMeter%2FOILMETER> .

props:activation  a            owl:DatatypeProperty ;
        rdfs:comment           "Identifies the predefined methods of sprinkler activation from which that required may be set."@en , "あらかじめ定義済みのスプリンクラーの作動方式から必要な方式を設定する識別。"@ja-JP ;
        rdfs:label             "activation"@en , "作動"@ja-JP ;
        schema:domainIncludes  <https://w3id.org/product/FireSuppressionTerminal%2FSPRINKLER> .

props:longTimeCurrentSetValue
        a                      owl:DatatypeProperty ;
        rdfs:comment           "Long time current set value. The set value of the long time tripping current if adjustable."@en ;
        rdfs:label             "longTimeCurrentSetValue"@en ;
        rdfs:range             <https://w3id.org/product/ElectricCurrentMeasure> ;
        schema:domainIncludes  <https://w3id.org/product/ProtectiveDevice> .

props:isFOB  a                 owl:DatatypeProperty ;
        rdfs:comment           "Indication of whether contents of the purchase order are delivered 'Free on Board' (= True) or not (= False). FOB is a shipping term which indicates that the supplier pays the shipping costs (and usually also the insurance costs) from the point of manufacture to a specified destination, at which point the buyer takes responsibility."@en ;
        rdfs:label             "isFOB"@en ;
        rdfs:range             xsd:boolean ;
        schema:domainIncludes  <https://w3id.org/product/ProjectOrder%2FPURCHASEORDER> .

props:outdoorEnvironment
        a                      owl:DatatypeProperty ;
        rdfs:comment           "Adjustment of the service life resulting from the effect of the outdoor environment (where appropriate)"@en ;
        rdfs:label             "outdoorEnvironment"@en ;
        schema:domainIncludes  <https://w3id.org/product/System> .

props:spacingBarPitch
        a                      owl:DatatypeProperty ;
        rdfs:comment           "The pitch length of the spacing bar."@en , "巾止筋の間隔。"@ja-JP ;
        rdfs:label             "巾止筋ピッチ"@ja-JP , "spacingBarPitch"@en , "幅止筋間隔"@ja-JP ;
        rdfs:range             <https://w3id.org/product/PositiveLengthMeasure> ;
        schema:domainIncludes  <https://w3id.org/product/Wall> , <https://w3id.org/product/Beam> .

props:steam  a                 owl:DatatypeProperty ;
        rdfs:comment           "The amount of steam consumed during the period specified in the time series."@en , "특정 기간 동안 증기 소비."@ko-KR ;
        rdfs:label             "steam"@en , "증기소비량"@ko-KR ;
        schema:domainIncludes  <https://w3id.org/product/Building> .

props:lockedRotorCurrent
        a                      owl:DatatypeProperty ;
        rdfs:comment           "Input current when a motor armature is energized but not rotating."@en , "モーターの電機子に電圧を印加しロータが回っていない時の入力電流。"@ja-JP , "모터의 전기자 전압을인가 로터가 회전하지 않을 때 입력 전류."@ko-KR ;
        rdfs:label             "lockedRotorCurrent"@en , "拘束ロータ電流"@ja-JP , "구속 회전자 전류"@ko-KR ;
        rdfs:range             <https://w3id.org/product/ElectricCurrentMeasure> ;
        schema:domainIncludes  <https://w3id.org/product/ElectricMotor> .

props:barCode  a               owl:DatatypeProperty ;
        rdfs:comment           "The identity of the bar code given to an occurrence of the product."@en ;
        rdfs:label             "barCode"@en ;
        rdfs:range             xsd:string ;
        schema:domainIncludes  <https://w3id.org/product/Element> .

props:boltholePitch  a         owl:DatatypeProperty ;
        rdfs:comment           "Diameter of the circle along which the boltholes are placed."@en , "ボルト穴がある円の直径"@ja-JP ;
        rdfs:label             "boltholePitch"@en , "ボルト穴ピッチ"@ja-JP ;
        rdfs:range             <https://w3id.org/product/PositiveLengthMeasure> ;
        schema:domainIncludes  <https://w3id.org/product/PipeSegment> .

props:displayType  a           owl:DatatypeProperty ;
        rdfs:comment           "Indicates the type of display."@en , "画面の種類を示す。"@ja-JP , "화면 종류를 나타낸다"@ko-KR ;
        rdfs:label             "displayType"@en , "画面種類"@ja-JP , "화면 유형"@ko-KR ;
        schema:domainIncludes  <https://w3id.org/product/AudioVisualAppliance%2FDISPLAY> .

props:acidityConcentration
        a                      owl:DatatypeProperty ;
        rdfs:comment           "Maximum CaCO3 equivalent that would neutralize the acid."@en ;
        rdfs:label             "acidityConcentration"@en ;
        rdfs:range             <https://w3id.org/product/IonConcentrationMeasure> ;
        schema:domainIncludes  <https://w3id.org/product/Material> .

props:hasSillInternal
        a                      owl:DatatypeProperty ;
        rdfs:comment           "Indication whether the window opening has an internal sill (TRUE) or not (FALSE)."@en , "Angabe, ob dieses Fenster mit einer inneren Fensterbank ausgestattet ist (JA) under nicht (NEIN)."@de-DE , "Indique si l'ouverture est dotée d'un seuil côté intérieur (VRAI) ou non (FAUX)."@fr-FR ;
        rdfs:label             "hasSillInternal"@en , "Fensterbank innen"@de-DE , "Seuil côté intérieur"@fr-FR ;
        rdfs:range             xsd:boolean ;
        schema:domainIncludes  <https://w3id.org/product/Window> .

props:performance  a           owl:DatatypeProperty ;
        rdfs:comment           "Water temperature change as a function of wet-bulb temperature, water entering temperature, water flow rate, air flow rate, Tdiff = f ( Twet-bulb, Twater,in, mwater, mair)."@en ;
        rdfs:label             "performance"@en ;
        schema:domainIncludes  <https://w3id.org/product/CoolingTower> .

props:coilFluidArrangement
        a                      owl:DatatypeProperty ;
        rdfs:comment           "Fluid flow arrangement of the coil.\n\nCrossCounterFlow: Air and water flow enter in different directions.\nCrossFlow: Air and water flow are perpendicular.\nCrossParallelFlow: Air and water flow enter in same directions."@en , "Disposition du flux du fluide dans la batterie."@fr-FR ;
        rdfs:label             "coilFluidArrangement"@en , "DispositionFluideBatterie"@fr-FR ;
        schema:domainIncludes  <https://w3id.org/product/Coil> .

props:secondCurvatureRadius
        a                      owl:DatatypeProperty ;
        rdfs:comment           "SecondCurvatureRadius should be defined as the top or right side radius of curvature value."@en , "2番目の曲率半径は、曲率の値の先頭又は右側の半径として定義する必要があります。"@ja-JP ;
        rdfs:label             "secondCurvatureRadius"@en , "2番目の曲率半径"@ja-JP ;
        rdfs:range             <https://w3id.org/product/PositiveLengthMeasure> ;
        schema:domainIncludes  <https://w3id.org/product/Tank%2FPREFORMED> , <https://w3id.org/product/Tank> .

props:hasDeflector  a          owl:DatatypeProperty ;
        rdfs:comment           "Indication of whether the sprinkler has a deflector (baffle) fitted to diffuse the discharge on activation (= TRUE) or not (= FALSE)."@en , "スプリンクラー作動時、放水を拡散させる偏向器（バッフル）取り付けているかどうかの表示（= TRUE）そうでないか（= FALSE）を返します。"@ja-JP ;
        rdfs:label             "hasDeflector"@en , "ディフレクターの有無"@ja-JP ;
        rdfs:range             xsd:boolean ;
        schema:domainIncludes  <https://w3id.org/product/FireSuppressionTerminal%2FSPRINKLER> .

props:coreMiddleHeight
        a                      owl:DatatypeProperty ;
        rdfs:comment           "Core middle height of the profile."@en ;
        rdfs:label             "coreMiddleHeight"@en ;
        rdfs:range             <https://w3id.org/product/PositiveLengthMeasure> ;
        schema:domainIncludes  <https://w3id.org/product/ArbitraryProfileDefWithVoids> .

props:trippingUnitReleaseCurrent
        a                      owl:DatatypeProperty ;
        rdfs:comment           "The value of tripping or residual current for which the device has the possibility to be equipped. The values are given in mA."@en , "漏電ブレーカの感度電流値（mA）。"@ja-JP , "누전 차단기의 감도 전류 (mA)."@ko-KR ;
        rdfs:label             "trippingUnitReleaseCurrent"@en , "定格感度電流"@ja-JP , "정격 감도 전류"@ko-KR ;
        schema:domainIncludes  <https://w3id.org/product/ProtectiveDeviceTrippingUnit%2FRESIDUALCURRENT> .

props:wireLoopBasePlateThickness
        a                      owl:DatatypeProperty ;
        rdfs:comment           "The thickness of the base plate."@en , "ベースプレートの板厚。"@ja-JP , "베이스 플레이트 두께"@ko-KR ;
        rdfs:label             "wireLoopBasePlateThickness"@en , "ベースプレート厚"@ja-JP , "베이스 플레이트 두께"@ko-KR ;
        rdfs:range             <https://w3id.org/product/PositiveLengthMeasure> ;
        schema:domainIncludes  <https://w3id.org/product/DiscreteAccessory%2FWire%20loop> .

props:longInsideCenterLowerBarPitch
        a                      owl:DatatypeProperty ;
        rdfs:comment           "The pitch length of the long inside center lower bar."@en , "長辺方向・柱間帯・下端中央の鉄筋間隔。"@ja-JP ;
        rdfs:label             "longInsideCenterLowerBarPitch"@en , "長辺・柱列帯・下端中央ピッチ"@ja-JP ;
        rdfs:range             <https://w3id.org/product/PositiveLengthMeasure> ;
        schema:domainIncludes  <https://w3id.org/product/Slab> .

props:automaticCondensateDischarge
        a                      owl:DatatypeProperty ;
        rdfs:comment           "Whether or not the condensing water or oil is discharged automatically from the filter."@en ;
        rdfs:label             "automaticCondensateDischarge"@en ;
        rdfs:range             xsd:boolean ;
        schema:domainIncludes  <https://w3id.org/product/Filter%2FCOMPRESSEDAIRFILTER> .

props:adjustmentDesignation
        a                      owl:DatatypeProperty ;
        rdfs:comment           "The desgnation on the device for the adjustment."@en , "調整する装置の指定。"@ja-JP , "조정하는 장치를 지정합니다."@ko-KR ;
        rdfs:label             "adjustmentDesignation"@en , "調整の指定"@ja-JP , "조정지정"@ko-KR ;
        rdfs:range             xsd:string ;
        schema:domainIncludes  <https://w3id.org/product/ProtectiveDeviceTrippingUnit> .

props:nonHazardousWaste
        a                      owl:DatatypeProperty ;
        rdfs:comment           "Quantity of non hazardous waste generated."@en , "비 유해 폐기물의 발생량"@ko-KR , "生成される一般廃棄物の量。"@ja-JP , "Quantité de déchets non dangereux générés [NDT : tels que définis dans la norme NF P01-010]"@fr-FR ;
        rdfs:label             "nonHazardousWaste"@en , "비 유해 폐기물"@ko-KR , "一般廃棄物"@ja-JP , "DechetsNonDangereux"@fr-FR ;
        rdfs:range             <https://w3id.org/product/MassMeasure> ;
        schema:domainIncludes  <https://w3id.org/product/Element> .

props:lighting  a              owl:DatatypeProperty ;
        rdfs:comment           "Lighting loads."@en , "照明負荷。"@ja-JP , "조명 부하"@ko-KR ;
        rdfs:label             "lighting"@en , "照明"@ja-JP , "조명"@ko-KR ;
        schema:domainIncludes  <https://w3id.org/product/Space> .

props:fixingSocketTypeReference
        a                      owl:DatatypeProperty ;
        rdfs:comment           "Type reference for the fixing socket according to local standards."@en , "固定ソケットが参照するローカル標準。"@ja-JP , "고정 소켓이 참조하는 로컬 표준"@ko-KR ;
        rdfs:label             "fixingSocketTypeReference"@en , "参照基準"@ja-JP , "참조 기준"@ko-KR ;
        schema:domainIncludes  <https://w3id.org/product/DiscreteAccessory%2FFixing%20socket> .

props:isBuiltIn  a             owl:DatatypeProperty ;
        rdfs:comment           "Indicates whether the furniture type is intended to be 'built in' i.e. physically attached to a building or facility (= TRUE) or not i.e. Loose and movable (= FALSE)."@en ;
        rdfs:label             "isBuiltIn"@en ;
        rdfs:range             xsd:boolean ;
        schema:domainIncludes  <https://w3id.org/product/Furniture> .

props:performanceClasses
        a                      owl:DatatypeProperty ;
        rdfs:comment           "모터 보호하는 개폐 장치는 능력이 다른 최대 7 종류가있다. 이름의 예로는, B, C, N, S, H, L, V가 포함된다."@ko-KR , "モータ保護を行う開閉装置は、能力が違う最大7種類がある。名称の例として、B, C, N, S, H, L, Vが含まれる。"@ja-JP , "A set of designations of performance classes for the breaker unit for which the data of this instance is valid. A breaker unit being a motor protection device may be\nconstructed for different levels of breaking capacities. A maximum of 7 different\nperformance classes may be provided. Examples of performance classes that may be specified include B, C, N, S, H, L, V."@en , "A set of designations of performance classes for the breaker unit for which the data of this instance is valid. A breaker unit being a circuit breaker may be\nconstructed for different levels of breaking capacities. A maximum of 7 different\nperformance classes may be provided. Examples of performance classes that may be specified include B, C, N, S, H, L, V."@en ;
        rdfs:label             "performanceClasses"@en , "능력 클래스"@ko-KR , "能力クラス"@ja-JP , "능력클래스"@ko-KR ;
        schema:domainIncludes  <https://w3id.org/product/ProtectiveDevice> , <https://w3id.org/product/ProtectiveDevice%2FCIRCUITBREAKER> .

props:nominalThickness
        a                      owl:DatatypeProperty ;
        rdfs:comment           "The nominal thickness of the work surface."@en , "The nominal thickness of the panel."@en , "The nominal overall thickness of the slab."@en ;
        rdfs:label             "nominalThickness"@en ;
        rdfs:range             <https://w3id.org/product/PositiveLengthMeasure> ;
        schema:domainIncludes  <https://w3id.org/product/SystemFurnitureElement%2FWORKSURFACE> , <https://w3id.org/product/SystemFurnitureElement%2FPANEL> , <https://w3id.org/product/Slab> .

props:refrigerantMaterial
        a                      owl:DatatypeProperty ;
        rdfs:comment           "The refrigerant material used for heat transfer purposes."@en ;
        rdfs:label             "refrigerantMaterial"@en ;
        schema:domainIncludes  <https://w3id.org/product/Condenser> .

props:chamberWidth  a          owl:DatatypeProperty ;
        rdfs:comment           "비원 챔버의 폭"@ko-KR , "非円形チャンバーの幅。"@ja-JP , "Width, in the event of the shape being non circular in plan."@en ;
        rdfs:label             "챔버의 너비"@ko-KR , "チャンバー（バイブスペース？）の幅"@ja-JP , "챔버 (파이프 공간)의 너비"@ko-KR , "チャンバー幅"@ja-JP , "チャンバーの幅"@ja-JP , "chamberWidth"@en , "챔버의 폭"@ko-KR ;
        rdfs:range             <https://w3id.org/product/PositiveLengthMeasure> ;
        schema:domainIncludes  <https://w3id.org/product/DistributionChamberElement%2FVALVECHAMBER> , <https://w3id.org/product/DistributionChamberElement%2FMETERCHAMBER> , <https://w3id.org/product/DistributionChamberElement%2FINSPECTIONCHAMBER> .

props:iCN60898  a              owl:DatatypeProperty ;
        rdfs:comment           "The nominal breaking capacity in [A] for an MCB tested in accordance with the IEC 60898 series."@en , "IECの60898シリーズに基づいてテストされたMCBの定格遮断容量を[A]で設定。"@ja-JP , "IEC의 60898 시리즈를 기반으로 시험한 MCB의 정격 차단 용량 [A]로 설정."@ko-KR ;
        rdfs:label             "iCN60898"@en , "ICN60898"@ja-JP , "ICN60898"@ko-KR ;
        rdfs:range             <https://w3id.org/product/ElectricCurrentMeasure> ;
        schema:domainIncludes  <https://w3id.org/product/ProtectiveDevice%2FCIRCUITBREAKER> .

props:alkalinityConcentration
        a                      owl:DatatypeProperty ;
        rdfs:comment           "Maximum alkalinity concentration (maximum sum of concentrations of each of the negative ions substances measured as CaCO3)."@en ;
        rdfs:label             "alkalinityConcentration"@en ;
        rdfs:range             <https://w3id.org/product/IonConcentrationMeasure> ;
        schema:domainIncludes  <https://w3id.org/product/Material> .

props:hasTurbulator  a         owl:DatatypeProperty ;
        rdfs:comment           "TRUE if the tube has a turbulator, FALSE if it does not."@en , "かくはん器有りの時 TRUE、無しの時 FALSE"@ja-JP ;
        rdfs:label             "hasTurbulator"@en , "かくはん器有り"@ja-JP ;
        rdfs:range             xsd:boolean ;
        schema:domainIncludes  <https://w3id.org/product/TubeBundle> .

props:totalLatentLoad
        a                      owl:DatatypeProperty ;
        rdfs:comment           "Total energy added or removed from air that affects its humidity or concentration of water vapor.  If a value is less than zero (negative), then the thermal load is lost from the space. If a value is greater than zero (positive), then the thermal load is a gain to the space."@en , "空気湿度（水蒸気量）を上昇・下降させる取得・損失の熱量の合計。ゼロより小さい（－）場合、室内の水蒸気が減少となる。ゼロより大きい（＋）場合、室内の水蒸気が増大となる。"@ja-JP , "습도 (수증기량)을 상승 · 하강하는 취득 · 손실 열량의 총. 제로보다 작은 (-) 경우 실내의 수증기가 감소된다. 제로보다 큰 (+) 경우 실내의 수증기가 증가된다."@ko-KR ;
        rdfs:label             "totalLatentLoad"@en , "潜熱負荷の合計"@ja-JP , "잠열부하의 합계"@ko-KR ;
        schema:domainIncludes  <https://w3id.org/product/Space> .

props:assetInsuranceType
        a                      owl:DatatypeProperty ;
        rdfs:comment           "Identifies the predefined types of insurance rating from which the type required may be set."@en , "保険の定義済み種別。"@ja-JP ;
        rdfs:label             "assetInsuranceType"@en , "資産保険種別"@ja-JP ;
        schema:domainIncludes  <https://w3id.org/product/Asset> .

props:electronicTrippingUnitType
        a                      owl:DatatypeProperty ;
        rdfs:comment           "A list of the available types of electronic tripping unit  from which that required may be selected."@en , "電磁式の装置タイプをリストから選択。"@ja-JP , "전자식 장치 유형을 목록에서 선택합니다."@ko-KR ;
        rdfs:label             "electronicTrippingUnitType"@en , "電磁式の装置タイプ"@ja-JP , "전자식 장치 유형"@ko-KR ;
        schema:domainIncludes  <https://w3id.org/product/ProtectiveDeviceTrippingUnit%2FELECTRONIC> .

props:applicableStructuralDesignMethod
        a                      owl:DatatypeProperty ;
        rdfs:comment           "Determines whether mechanical material properties are applicable to 'ASD' = allowable stress design (working stress design), 'LSD' = limit state design, or 'LRFD' = load and resistance factor design."@en ;
        rdfs:label             "applicableStructuralDesignMethod"@en ;
        rdfs:range             xsd:string ;
        schema:domainIncludes  <https://w3id.org/product/Material%2FWood> .

props:touchScreen  a           owl:DatatypeProperty ;
        rdfs:comment           "Indicates touchscreen support."@en , "タッチスクリーンのサポートを示す。"@ja-JP , "터치 스크린 지원을 보여준다"@ko-KR ;
        rdfs:label             "touchScreen"@en , "タッチスクリーン"@ja-JP , "터치 스크린"@ko-KR ;
        schema:domainIncludes  <https://w3id.org/product/AudioVisualAppliance%2FDISPLAY> .

props:externalAdjusted
        a                      owl:DatatypeProperty ;
        rdfs:comment           "An indication if the ground fault protection may be adjusted according to an external current coil or not."@en , "外部調整が可能かどうか。"@ja-JP , "외부 조정이 가능합니까?"@ko-KR ;
        rdfs:label             "externalAdjusted"@en , "外部調整"@ja-JP , "외부조정"@ko-KR ;
        rdfs:range             xsd:boolean ;
        schema:domainIncludes  <https://w3id.org/product/ProtectiveDeviceTrippingUnit> .

props:isTempered  a            owl:DatatypeProperty ;
        rdfs:comment           "German-description-7"@de-DE , "Indique si le verre est trempé (VRAI) ou non (FAUX)."@fr-FR , "表示玻璃是否经过强化处理。"@zh-CN , "強化ガラスか（TRUE）否か(FALSE)を示す。"@ja-JP , "Indication whether the glass is tempered (TRUE) or not (FALSE) ."@en ;
        rdfs:label             "German-name-7"@de-DE , "是否钢化"@zh-CN , "VitrageTrempe"@fr-FR , "isTempered"@en , "強化ガラス"@ja-JP ;
        rdfs:range             xsd:boolean ;
        schema:domainIncludes  <https://w3id.org/product/Door> , <https://w3id.org/product/cWindow> .

props:pitchAngle  a            owl:DatatypeProperty ;
        rdfs:comment           "Angle of the slab to the horizontal when used as a component for the roof (specified as 0 degrees or not asserted for cases where the slab is not used as a roof component).      \n\nThe shape information is provided in addition to the shape representation and the geometric parameters used within. In cases of inconsistency between the geometric parameters and the shape properties, provided in the attached property, the geometric parameters take precedence.  For geometry editing applications, like CAD: this value should be write-only."@en , "コンポーネントが屋根として使用される場合の、水平に対するスラブの角度（スラブが屋根として使用されない場合は、0度と指定されるか、定義されない）。\n\n形状情報は形状の表現として追加され、幾何学的なパラメータが使用される。幾何学的なパラメータと追加された形状プロパティが矛盾する場合、幾何学的なパラメータが優先される。CADのような、幾何学操作アプリケーションにとって、この値は、書き込み専用であるべきだ。"@ja-JP , "Angle de la dalle avec l'horizontale quand elle est utilisée comme un élément de la couverture (valeur 0 ou non définie lorsque la dalle ne participe pas à la couverture). Cette propriété  est donnée en complément de la représentation de la forme et des paramètres géométriques qui la déterminent. En cas d'incohérence entre ces paramètres géométriques et cette propriété, ce sont les paramètres géométriques qui priment. Les applications qui déterminent la géométrie comme les logiciels de CAO ne doivent pas autoriser la modification de cette propriété."@fr-FR , "Neigungswinkel der Decke gegenüber der Horizontalen wenn es sich um eine Dachfläche handelt. Angabe 0 Grad definiert eine horizontale Fläche.\n\nDieser Parameter wird zusätzlich zur geometrischen Repräsentation bereitgestellt. Im Fall der Inkonsistenz zwischen dem Parameter und der Geometrie hat die geometrische Repräsention Priorität. Dieser Parameter ist für CAD Software write-only."@de-DE ;
        rdfs:label             "AngleInclinaison"@fr-FR , "勾配角度"@ja-JP , "pitchAngle"@en , "Dachflächenneigung"@de-DE ;
        rdfs:range             <https://w3id.org/product/PlaneAngleMeasure> ;
        schema:domainIncludes  <https://w3id.org/product/Slab> .

props:heatingWetBulb  a        owl:DatatypeProperty ;
        rdfs:comment           "Outside wet bulb temperature for heating design."@en , "暖房用設計用外気湿球温度。"@ja-JP , "난방 설계 외기 습구온도"@ko-KR ;
        rdfs:label             "heatingWetBulb"@en , "暖房用設計外気湿球温度"@ja-JP , "난방 설계 외기 습구온도"@ko-KR ;
        rdfs:range             <https://w3id.org/product/ThermodynamicTemperatureMeasure> ;
        schema:domainIncludes  <https://w3id.org/product/Building> .

props:isSelectable  a          owl:DatatypeProperty ;
        rdfs:comment           "Indication whether the S-function can be switched off or not."@en , "Indication whether the L-function can be switched off or not."@en , "장치의 \"ON-OFF\"상태를 전기적으로 표시가 교체 가능합니까?"@ko-KR , "장치\"ON-OFF \"상태를 전기적으로 표시가 교체 가능합니까?"@ko-KR , "装置の “ON-OFF”状態を電気的表示が切り替え可能かどうか。"@ja-JP ;
        rdfs:label             "전환"@ko-KR , "isSelectable"@en , "切り替え"@ja-JP ;
        rdfs:range             xsd:boolean ;
        schema:domainIncludes  <https://w3id.org/product/ProtectiveDeviceTrippingUnit> .

props:nominalEvaporatingTemperature
        a                      owl:DatatypeProperty ;
        rdfs:comment           "Chiller evaporating temperature."@en , "Température d'évaporation du groupe froid."@fr-FR ;
        rdfs:label             "nominalEvaporatingTemperature"@en , "TempératureEvaporationNominale"@fr-FR ;
        rdfs:range             <https://w3id.org/product/ThermodynamicTemperatureMeasure> ;
        schema:domainIncludes  <https://w3id.org/product/Chiller> .

props:lightingPercentLoadToReturnAir
        a                      owl:DatatypeProperty ;
        rdfs:comment           "Percent of lighting load to the return air plenum."@en , "照明機器からリタン空気（天井裏）への放熱率。"@ja-JP , "조명 기기에서 폴리탄 공기 (천장)의 방열 속도."@ko-KR ;
        rdfs:label             "lightingPercentLoadToReturnAir"@en , "リタン空気への照明機器の放熱率"@ja-JP , "리탄 공기에 조명 기기의 방열 비율"@ko-KR ;
        rdfs:range             <https://w3id.org/product/PositiveRatioMeasure> ;
        schema:domainIncludes  <https://w3id.org/product/SpatialElement> .

props:packingCareType
        a             owl:DatatypeProperty ;
        rdfs:comment  "Identifies the predefined types of care that may be required when handling the artefact during a move where:\n\nFragile: artefact may be broken during a move through careless handling.\nHandleWithCare: artefact may be damaged during a move through careless handling."@en , "引越しの最中の品物の取り扱いに要求される、あらかじめ定義されている注意タイプの識別子：\n\nFragile: 注意深い取り扱いをしないと壊れる品物。\nHandleWithCare: 注意深い取り扱いでしないと損害を受ける品物。"@ja-JP ;
        rdfs:label    "packingCareType"@en , "荷造り注意タイプ"@ja-JP .

props:flowrate  a              owl:DatatypeProperty ;
        rdfs:comment           "The actual operational fluid flowrate."@en , "実際の運用流量"@ja-JP , "The flowrate of the fuel."@en , "燃料の流速。"@ja-JP ;
        rdfs:label             "flowrate"@en , "流量"@ja-JP ;
        schema:domainIncludes  <https://w3id.org/product/Pump> , <https://w3id.org/product/DistributionPort%2FGAS> .

props:capacityControlType
        a                      owl:DatatypeProperty ;
        rdfs:comment           "InletVane: Control by adjusting inlet vane.\nVariableSpeedDrive: Control by variable speed drive. \nBladePitchAngle: Control by adjusting blade pitch angle.\nTwoSpeed: Control by switch between high and low speed.\nDischargeDamper: Control by modulating discharge damper."@en , "InletVane: インレットベーン\nVariableSpeedDrive: 変速駆動 \nBladePitchAngle: 羽根ピッチ制御\nTwoSpeed: 二速制御\nDischargeDamper: 吐出ダンパ制御"@ja-JP ;
        rdfs:label             "capacityControlType"@en , "容量制御方式"@ja-JP ;
        schema:domainIncludes  <https://w3id.org/product/Fan> .

props:upperCurrent1  a         owl:DatatypeProperty ;
        rdfs:comment           "The current in [x In], indicating that for currents larger than UpperCurrent1 the I2t part of the L-function will trip the current."@en , "[x In]の電流,電流をトリップするL関数のI2t部分は、上限電流1よりも大きい電流を示す。"@ja-JP , "x In] 전류 전류를 여행하는 L 함수 I2t 부분은 최대 전류 1보다 큰 전류를 보여준다."@ko-KR ;
        rdfs:label             "upperCurrent1"@en , "上電流1"@ja-JP , "상전류1"@ko-KR ;
        rdfs:range             <https://w3id.org/product/ElectricCurrentMeasure> ;
        schema:domainIncludes  <https://w3id.org/product/ProtectiveDeviceTrippingUnit> .

props:dishwasherType  a        owl:DatatypeProperty ;
        rdfs:comment           "Type of dishwasher."@en , "食器洗浄機のタイプ。"@ja-JP , "식기 세척기의 유형"@ko-KR ;
        rdfs:label             "dishwasherType"@en , "食器洗浄機のタイプ"@ja-JP , "식기 세척기의 유형"@ko-KR ;
        schema:domainIncludes  <https://w3id.org/product/ElectricAppliance%2FDISHWASHER> .

props:compressorCondenserPressureDrop
        a                      owl:DatatypeProperty ;
        rdfs:comment           "Pressure drop between condenser inlet and compressor outlet."@en ;
        rdfs:label             "compressorCondenserPressureDrop"@en ;
        schema:domainIncludes  <https://w3id.org/product/Condenser> .

props:correctionFactorForCooling
        a                      owl:DatatypeProperty ;
        rdfs:comment           "Correction factor k as a function of water flow rate (used to calculate cooling capacity)."@en ;
        rdfs:label             "correctionFactorForCooling"@en ;
        schema:domainIncludes  <https://w3id.org/product/CooledBeam> .

props:eutrophicationPerUnit
        a                      owl:DatatypeProperty ;
        rdfs:comment           "PO4 (인산)에 상응하는 환산되는 부영 양화 성분 물량"@ko-KR , "PO4で計算される富栄養化する化合物の量。"@ja-JP , "Quantity of eutrophicating compounds calculated in equivalent PO4"@en , "Quantité de composés responsables de l'eutrophisation exprimée en équivalent P04 tels que définis dans la norme  ISO21930:2007 [NDT : et dans la norme PrEN15804:2008]"@fr-FR ;
        rdfs:label             "eutrophicationPerUnit"@en , "EutrophisationParUnite"@fr-FR , "단위당 부영양화"@ko-KR , "単位あたり富栄養化"@ja-JP ;
        rdfs:range             <https://w3id.org/product/MassMeasure> ;
        schema:domainIncludes  <https://w3id.org/product/Element> .

props:numberOfActors  a        owl:DatatypeProperty ;
        rdfs:comment           "The number of actors that are to be dealt with together in the population."@en , "母集団において取り扱われる関与者の数。"@ja-JP , "该组参与者的总数。"@zh-CN ;
        rdfs:label             "numberOfActors"@en , "関与者数"@ja-JP , "参与者数"@zh-CN ;
        rdfs:range             <https://w3id.org/product/CountMeasure> ;
        schema:domainIncludes  <https://w3id.org/product/Actor> .

props:maximumVelocity
        a                      owl:DatatypeProperty ;
        rdfs:comment           "The maximum design velocity of the air in the duct or fitting."@en , "ダクト或いは継ぎ手の最大設計風速。"@ja-JP , "덕트 또는 이음새의 최대 설계 바람."@ko-KR ;
        rdfs:label             "maximumVelocity"@en , "最大速度"@ja-JP , "최대 속도"@ko-KR ;
        rdfs:range             <https://w3id.org/product/LinearVelocityMeasure> ;
        schema:domainIncludes  <https://w3id.org/product/DistributionSystem%2FVENTILATION> .

props:liftingStrength
        a                      owl:DatatypeProperty ;
        rdfs:comment           "The minimum required compressive strength of the concrete when the concrete element is lifted."@en , "コンクリート要素が吊り上げられる時のコンクリートの最小必要圧縮強度。"@ja-JP ;
        rdfs:label             "liftingStrength"@en , "吊り上げ強度"@ja-JP ;
        rdfs:range             <https://w3id.org/product/PressureMeasure> ;
        schema:domainIncludes  <https://w3id.org/product/BuildingElement> .

props:combustionTemperature
        a                      owl:DatatypeProperty ;
        rdfs:comment           "燃焼室平均温度"@ja-JP , "Average combustion chamber temperature."@en , "Combustion temperature of the material when air is at 298 K and 100 kPa."@en , "Température de combustion moyenne au foyer."@fr-FR ;
        rdfs:label             "TempératureCombustion"@fr-FR , "燃焼温度"@ja-JP , "combustionTemperature"@en ;
        rdfs:range             <https://w3id.org/product/ThermodynamicTemperatureMeasure> ;
        schema:domainIncludes  <https://w3id.org/product/Boiler> , <https://w3id.org/product/Material> .

props:fireExit  a              owl:DatatypeProperty ;
        rdfs:comment           "이 물체가 화재의 경우 출구로 사용되도록 설계되었는지 여부를 나타내는 부울 값입니다. 여기에 공간 (예 복도), 예를 들면 화재 피난 목적을 위해 출구 공간으로 사용하도록 설계되었는지 여부"@ko-KR , "Indique si cet objet est conçu pour servir de sortie en cas d'incendie (VRAI) ou non (FAUX). Cas d'un espace comme un couloir conçu pour servir d'espace de sortie, par exemple pour l'évacuation en cas d'incendie."@fr-FR , "避難出口(TRUE)か、通常の出口(FALSE)かを示すフラグ。"@ja-JP , "Angabe, ob das Fenster ein Notausgang gemäß der nationalen oder regionalen Brandschutzverordnung ist (JA), oder nicht (NEIN)."@de-DE , "Indication whether this object is designed to serve as an exit in the case of fire (TRUE) or not (FALSE).\nHere it defines an exit ramp in accordance to the national building code."@en , "Indication whether this object is designed to serve as an exit in the case of fire (TRUE) or not (FALSE).\nHere it defines an exit stair in accordance to the national building code."@en , "Angabe, ob der Raum einen Notausgang für den Brandfall hat und als ein Notausgangs(sammel)raum im Sinne der Brandschutzverordnung gilt (WAHR), oder nicht (FALSCH)."@de-DE , "このオブジェクトが火災の場合に出口として使われるように設計されているかどうかを示すブーリアン値。(TRUE)はい、(FALSE)いいえ。\nここに、空間(例えば廊下)は、例えば火災避難目的のために出口空間として使われるよう設計されているかどうか。"@ja-JP , "Indique si cet objet est conçu pour servir de sortie en cas d'incendie (VRAI) ou non (FAUX)."@fr-FR , "このオブジェクトが火災時の非常口として設計されているかどうかを示すブーリアン値。ここでは関連する建築基準法における出口ドアとして定義している。"@ja-JP , "Indication si l'objet est conçu pour servir de sortie en cas d'incendie (VRAI) ou non (FAUX). Cas d'un élément de transport comme un ascenseur conçu pour l'évacuation en cas d'incendie."@fr-FR , "このオブジェクト（開口）が火災の場合に出口として使われるように設計されているかどうかを示すブーリアン値。(TRUE)はい、(FALSE)いいえ。\nここに、空間(例えば廊下)は、例えば火災避難目的のために出口空間として使われるよう設計されているかどうか。"@ja-JP , "表示该构件是否设计为火灾时的紧急出口。\n该属性的依据为国家建筑规范。"@zh-CN , "Indique si cet objet est conçu pour servir de sortie en cas d'incendie (VRAI) ou non (FAUX). Définition de la sortie de secours selon le Code National."@fr-FR , "Angabe, ob die Tür ein Notausgang gemäß der nationalen oder regionalen Brandschutzverordnung ist (JA), oder nicht (NEIN).."@de-DE , "German-description-10"@de-DE , "Indication whether this object is designed to serve as an exit in the case of fire (TRUE) or not (FALSE).\nHere it defines an exit door in accordance to the national building code."@en , "German-description-6"@de-DE , "Angabe ob dieses Transportelement als Rettungsweg im Brandfall zulässig ist (WAHR) oder nicht (FALSCH)."@de-DE , "Indication whether this object is designed to serve as an exit in the case of fire (TRUE) or not (FALSE). Here it defines an exit window in accordance to the national building code."@en , "Indication whether this object is designed to serve as an exit in the case of fire (TRUE) or not (FALSE).\nHere whether the transport element (in case of e.g., a lift) is designed to serve as a fire exit, e.g., for fire escape purposes."@en , "Indication whether this object is designed to serve as an exit in the case of fire (TRUE) or not (FALSE).\nHere whether the space (in case of e.g., a corridor) is designed to serve as an exit space, e.g., for fire escape purposes."@en , "여기에 공간 (예 복도), 예를 들면 화재 피난 목적을 위해 출구 공간으로 사용하도록 설계되었는지 여부"@ko-KR ;
        rdfs:label             "Notausgang"@de-DE , "Sortie de secours"@fr-FR , "是否为紧急出口"@zh-CN , "SortieSecours"@fr-FR , "Sortie Secours"@fr-FR , "fireExit"@en , "화재 출구 (피난 출구)"@ko-KR , "非常口区分"@ja-JP , "Rettungsweg"@de-DE , "Fluchtweg"@de-DE , "避難出口"@ja-JP ;
        rdfs:range             xsd:boolean ;
        schema:domainIncludes  <https://w3id.org/product/Stair> , <https://w3id.org/product/cZone> , <https://w3id.org/product/cSpatialZone> , <https://w3id.org/product/Space> , <https://w3id.org/product/OpeningElement> , <https://w3id.org/product/Window> , <https://w3id.org/product/Ramp> , <https://w3id.org/product/Door> , <https://w3id.org/product/TransportElement> .

props:earthFault1PolePowerFactorMaximumState
        a                      owl:DatatypeProperty ;
        rdfs:comment           "Power factor of the maximum 1 pole earth fault  current provided at the point of supply i.e. the fault between 1 phase and PE/PEN."@en , "電源供給時点の点1相とPE/PEN間の1極最大地絡電流力率。"@ja-JP , "전원 공급 시점 점 1 상 및 PE / PEN 사이의 1 극 최대 지락 전류 역률."@ko-KR ;
        rdfs:label             "earthFault1PolePowerFactorMaximumState"@en , "1極最大地絡電流力率"@ja-JP , "1 극 최대 지락 전류 역률"@ko-KR ;
        rdfs:range             xsd:decimal ;
        schema:domainIncludes  <https://w3id.org/product/ElectricFlowStorageDevice> .

props:waterPressureRange
        a                      owl:DatatypeProperty ;
        rdfs:comment           "Allowable water circuit working pressure range."@en ;
        rdfs:label             "waterPressureRange"@en ;
        schema:domainIncludes  <https://w3id.org/product/CooledBeam> .

props:isothermalMoistureCapacity
        a                      owl:DatatypeProperty ;
        rdfs:comment           "Based on water vapor density."@en ;
        rdfs:label             "isothermalMoistureCapacity"@en ;
        rdfs:range             <https://w3id.org/product/IsothermalMoistureCapacityMeasure> ;
        schema:domainIncludes  <https://w3id.org/product/Material> .

props:bladePositionAngle
        a                      owl:DatatypeProperty ;
        rdfs:comment           "Blade position angle; angle between the blade and flow direction ( 0 - 90)."@en ;
        rdfs:label             "bladePositionAngle"@en ;
        schema:domainIncludes  <https://w3id.org/product/Damper> .

props:upperVaporResistanceFactor
        a                      owl:DatatypeProperty ;
        rdfs:comment           "The vapor permeability relationship of air/material (typically value > 1), measured in high relative humidity (typically in 95/50 % RH)."@en ;
        rdfs:label             "upperVaporResistanceFactor"@en ;
        rdfs:range             <https://w3id.org/product/PositiveRatioMeasure> ;
        schema:domainIncludes  <https://w3id.org/product/Material> .

props:application  a           owl:DatatypeProperty ;
        rdfs:comment           "Indicates application of controller."@en , "The application of the unitary control element."@en , "Indicates application of actuator."@en , "加湿器の応用　(固定式：ダクト搬送系に設置する加湿器、可搬式：クト搬送系に設置しない加湿器)"@ja-JP , "Humidifier application.\n\nFixed: Humidifier installed in a ducted flow distribution system.\nPortable: Humidifier is not installed in a ducted flow distribution system."@en ;
        rdfs:label             "応用"@ja-JP , "application"@en ;
        schema:domainIncludes  <https://w3id.org/product/Humidifier> , <https://w3id.org/product/Controller%2FPROGRAMMABLE> , <https://w3id.org/product/UnitaryControlElement%2FINDICATORPANEL> , <https://w3id.org/product/Actuator> .

props:load  a                  owl:DatatypeProperty ;
        rdfs:comment           "Boiler real load."@en , "ボイラ実負荷"@ja-JP , "Charge effective de la chaudière."@fr-FR ;
        rdfs:label             "load"@en , "負荷"@ja-JP , "Charge"@fr-FR ;
        schema:domainIncludes  <https://w3id.org/product/Boiler> .

props:faucetTopDescription
        a                      owl:DatatypeProperty ;
        rdfs:comment           "Description of the operating mechanism/top of the faucet."@en , "操作機構/水栓の頂部の説明"@ja-JP ;
        rdfs:label             "faucetTopDescription"@en , "水栓の頂部"@ja-JP ;
        rdfs:range             xsd:string ;
        schema:domainIncludes  <https://w3id.org/product/Valve%2FFAUCET> .

props:flowrateLeakage
        a                      owl:DatatypeProperty ;
        rdfs:comment           "Leakage flowrate versus pressure difference."@en , "漏洩量と圧力差の関係"@ja-JP ;
        rdfs:label             "flowrateLeakage"@en , "漏洩流量"@ja-JP ;
        schema:domainIncludes  <https://w3id.org/product/PipeFitting> .

props:weatherDataStation
        a                      owl:DatatypeProperty ;
        rdfs:comment           "The site weather data station description or reference to the data source from which weather data was obtained for use in calculations."@en , "空調負荷計算時使用する気象データの気象台所在地。"@ja-JP , "공조 부하 계산시 사용하는 기상 데이터 기상대 위치."@ko-KR ;
        rdfs:label             "weatherDataStation"@en , "気象台所在地"@ja-JP , "기상대 위치"@ko-KR ;
        rdfs:range             xsd:string ;
        schema:domainIncludes  <https://w3id.org/product/Building> .

props:climateChangePerUnit
        a                      owl:DatatypeProperty ;
        rdfs:comment           "Quantity of greenhouse gases emitted calculated in equivalent CO2"@en , "CO2で計算された温室効果ガスの放出量。"@ja-JP , "CO2 등가 환산되는 온실 가스 발생량"@ko-KR , "Quantité d'émissions de gaz à effet de serre exprimée en Kg d'équivalent CO2 tels que définis dans la norme  ISO21930:2007 [NDT : ainsi que dans les normes PrEN15804:2008 et NF P01-010]."@fr-FR ;
        rdfs:label             "단위당 기후 변화"@ko-KR , "ChangementClimatiqueParUnite"@fr-FR , "climateChangePerUnit"@en , "単位あたり気候変動"@ja-JP ;
        rdfs:range             <https://w3id.org/product/MassMeasure> ;
        schema:domainIncludes  <https://w3id.org/product/Element> .

props:startCurrentFactor
        a                      owl:DatatypeProperty ;
        rdfs:comment           "IEC. Start current factor defines how large the peak starting current will become on the engine. StartCurrentFactor is multiplied to NominalCurrent and to give the start current."@en , "IEC. Start current factor defines how large the peek starting current will become on the engine. StartCurrentFactor is multiplied to NominalCurrent and we get the start current."@en , "시동 전류 계수는 엔진이 움직이기 시작했다 피크 기동 전류를 정의합니다. 시동 전류 계수는 정격 전류 시동시 전류를 곱한 것"@ko-KR , "始動電流係数はエンジンが動き始めた時のピーク始動電流を定義。始動電流係数は定格電流と始動時の電流を掛け合わせたもの。"@ja-JP ;
        rdfs:label             "始動電流係数"@ja-JP , "시동전류 계수"@ko-KR , "시동 전류 계수"@ko-KR , "startCurrentFactor"@en ;
        rdfs:range             xsd:decimal ;
        schema:domainIncludes  <https://w3id.org/product/ElectricMotor> , <https://w3id.org/product/ElectricGenerator> .

props:nominalLengthOrDiameter
        a                      owl:DatatypeProperty ;
        rdfs:comment           "The nominal length or, in the case of a vertical cylindrical tank, the nominal diameter of the tank."@en , "公称長さ又は垂直円筒形タンクの場合、タンクの公称直径"@ja-JP ;
        rdfs:label             "nominalLengthOrDiameter"@en , "公称長さ又は直径"@ja-JP ;
        rdfs:range             <https://w3id.org/product/PositiveLengthMeasure> ;
        schema:domainIncludes  <https://w3id.org/product/Tank> .

props:videoResolutionHeight
        a                      owl:DatatypeProperty ;
        rdfs:comment           "垂直方向のピクセル数を示す。"@ja-JP , "수직 픽셀 수를 나타낸다."@ko-KR , "세로 픽셀 수를 나타낸다."@ko-KR , "Indicates the number of vertical pixels, e.g. 1080."@en , "세로 픽셀 수."@ko-KR , "Indicates the number of vertical pixels (the largest native video resolution height)."@en , "垂直方向のピクセル数。"@ja-JP ;
        rdfs:label             "videoResolutionHeight"@en , "수직 해상도"@ko-KR , "垂直解像度"@ja-JP ;
        rdfs:range             xsd:int ;
        schema:domainIncludes  <https://w3id.org/product/AudioVisualAppliance%2FPROJECTOR> , <https://w3id.org/product/AudioVisualAppliance%2FCAMERA> , <https://w3id.org/product/AudioVisualAppliance%2FDISPLAY> .

props:indoorEnvironment
        a                      owl:DatatypeProperty ;
        rdfs:comment           "Adjustment of the service life resulting from the effect of the indoor environment (where appropriate)."@en ;
        rdfs:label             "indoorEnvironment"@en ;
        schema:domainIncludes  <https://w3id.org/product/System> .

props:isOutlookDesirable
        a                      owl:DatatypeProperty ;
        rdfs:comment           "Indique si la vue sur l'extérieur est souhaitable (VRAI) ou non (FAUX)."@fr-FR , "An indication of whether the outlook is desirable (set TRUE) or not (set FALSE)"@en , "Angabe, ob dieser Raum einen natürlichen Ausblick nach draussen gewähren soll (WAHR) oder dies nicht gefordert ist (FALSCH)."@de-DE , "外の眺望が望ましいかどうか。"@ja-JP ;
        rdfs:label             "isOutlookDesirable"@en , "Ausblick erwünscht"@de-DE , "眺望の善し悪し"@ja-JP , "VueExterieurSouhaitable"@fr-FR ;
        rdfs:range             xsd:boolean ;
        schema:domainIncludes  <https://w3id.org/product/cSpatialZone> , <https://w3id.org/product/Space> , <https://w3id.org/product/cZone> .

props:stemBaseChamfer
        a                      owl:DatatypeProperty ;
        rdfs:comment           "Stem base chamfer of the profile."@en ;
        rdfs:label             "stemBaseChamfer"@en ;
        rdfs:range             <https://w3id.org/product/NonNegativeLengthMeasure> ;
        schema:domainIncludes  <https://w3id.org/product/ArbitraryClosedProfileDef> .

props:shortening  a            owl:DatatypeProperty ;
        rdfs:comment           "The ratio of the distance by which a precast piece is shortened after release from its form (due to compression induced by prestressing) to its original (nominal) length."@en ;
        rdfs:label             "shortening"@en ;
        rdfs:range             <https://w3id.org/product/RatioMeasure> ;
        schema:domainIncludes  <https://w3id.org/product/BuildingElement> .

props:minimumSectionModulusY
        a                      owl:DatatypeProperty ;
        rdfs:comment           "Bending resistance about the ys axis at the point with minimum zs ordinate. For example measured in mm³."@en ;
        rdfs:label             "minimumSectionModulusY"@en ;
        rdfs:range             <https://w3id.org/product/SectionModulusMeasure> ;
        schema:domainIncludes  <https://w3id.org/product/ProfileDef> .

props:isNeutralSecondaryTerminalAvailable
        a                      owl:DatatypeProperty ;
        rdfs:comment           "An indication of whether the neutral point of the secondary winding is available as a terminal (=TRUE) or not (= FALSE)."@en , "二次巻線の中性点がターミナルの場合は（=TRUE）、違う場合は（= FALSE）として表示する"@ja-JP , "2 차 코일의 중성점 터미널의 경우 (= TRUE), 다른 경우는 (= FALSE)로 표시"@ko-KR ;
        rdfs:label             "isNeutralSecondaryTerminalAvailable"@en , "中性点第2ターミナルがあるかどうか"@ja-JP , "중성점 제 2 터미널 여부"@ko-KR ;
        rdfs:range             xsd:boolean ;
        schema:domainIncludes  <https://w3id.org/product/Transformer> .

props:xDirectionTieHoopCount
        a                      owl:DatatypeProperty ;
        rdfs:comment           "The number of bars with X direction tie hoop bars."@en , "Ｘ方向巾止筋の本数。"@ja-JP ;
        rdfs:label             "xDirectionTieHoopCount"@en , "Ｘ方向巾止め筋本数"@ja-JP ;
        rdfs:range             xsd:int ;
        schema:domainIncludes  <https://w3id.org/product/Column> .

props:releaseCurrent  a        owl:DatatypeProperty ;
        rdfs:comment           "The release current in [x In] for the initial tripping of the S-function."@en , "放出する電流は、S-functionの初期特性。"@ja-JP , "방출 전류는 S-function의 초기 특성."@ko-KR ;
        rdfs:label             "releaseCurrent"@en , "放出電流"@ja-JP , "방출전류"@ko-KR ;
        rdfs:range             <https://w3id.org/product/ElectricCurrentMeasure> ;
        schema:domainIncludes  <https://w3id.org/product/ProtectiveDeviceTrippingUnit> .

props:coolingDesignAirflow
        a                      owl:DatatypeProperty ;
        rdfs:comment           "The air flowrate required during the peak cooling conditions."@en , "ピーク時の冷房条件で要求される給気量。"@ja-JP ;
        rdfs:label             "coolingDesignAirflow"@en , "冷房設計吸気量"@ja-JP ;
        rdfs:range             <https://w3id.org/product/VolumetricFlowRateMeasure> ;
        schema:domainIncludes  <https://w3id.org/product/Space> .

props:sensibleEffectiveness
        a                      owl:DatatypeProperty ;
        rdfs:comment           "Sensible heat transfer effectiveness, where effectiveness is defined as the ratio of heat transfer to maximum possible heat transfer."@en , "顕熱効率\n効率は、最大可能熱交換に対する熱交換の比率で定義される"@ja-JP , "Efficacité d'échange de chaleur sensible, où l'efficacité est définie par le rapport entre l'échange de chaleur effectif et l'échange maximum possible."@fr-FR ;
        rdfs:label             "sensibleEffectiveness"@en , "顕熱効率"@ja-JP , "EfficacitéSensible"@fr-FR ;
        schema:domainIncludes  <https://w3id.org/product/AirToAirHeatRecovery> .

props:structuralClass
        a                      owl:DatatypeProperty ;
        rdfs:comment           "The structural class defined for the concrete structure (e.g. '1')."@en , "構造クラスはコンクリート構造を定義した。（例えば「１」）"@ja-JP , "구조 클래스는 콘크리트 구조를 정의했다 (예를 들어 \"1\")"@ko-KR ;
        rdfs:label             "structuralClass"@en , "構造クラス"@ja-JP , "구조 클래스"@ko-KR ;
        rdfs:range             xsd:string ;
        schema:domainIncludes  <https://w3id.org/product/BuildingElement> .

props:solarReflectanceBack
        a                      owl:DatatypeProperty ;
        rdfs:comment           "Reflectance at normal incidence (solar): back side. Defines the fraction of the solar ray that is reflected and not transmitted when the ray passes from one medium into another, at the \"back\" side of the other material, perpendicular to the surface. Dependent on material and surface characteristics."@en ;
        rdfs:label             "solarReflectanceBack"@en ;
        rdfs:range             <https://w3id.org/product/PositiveRatioMeasure> ;
        schema:domainIncludes  <https://w3id.org/product/Material> .

props:electroMagneticTrippingUnitType
        a                      owl:DatatypeProperty ;
        rdfs:comment           "A list of the available types of electric magnetic tripping unit  from which that required may be selected. These cover overload, none special, short circuit, motor protection and bi-metal tripping."@en , "電磁トリップ装置タイプを選択する。（過電流・配線用・モーター・バイメタル・その他）"@ja-JP , "전자 트립 장치 유형을 선택합니다. (과전류 · 배선 모터 바이메탈 기타)"@ko-KR ;
        rdfs:label             "electroMagneticTrippingUnitType"@en , "電磁トリップ装置タイプ"@ja-JP , "전자 트립장치 유형"@ko-KR ;
        schema:domainIncludes  <https://w3id.org/product/ProtectiveDeviceTrippingUnit%2FELECTROMAGNETIC> .

props:pressureDrop  a          owl:DatatypeProperty ;
        rdfs:comment           "Pressure drop."@en , "Drop in total pressure between inlet and outlet at nominal air-flow rate."@en , "設定風量での入口/出口間の全圧降下"@ja-JP , "Chute de pression totale entre l'entrée et la sortie en débit d'air nominal"@fr-FR ;
        rdfs:label             "圧力降下"@ja-JP , "Chute de pression"@fr-FR , "pressureDrop"@en ;
        schema:domainIncludes  <https://w3id.org/product/AirTerminal> , <https://w3id.org/product/Damper> .

props:fixingSocketHeight
        a                      owl:DatatypeProperty ;
        rdfs:comment           "The overall height of the fixing socket."@en , "固定ソケットの全体長さ。"@ja-JP , "고정 소켓의 전체 길이"@ko-KR ;
        rdfs:label             "fixingSocketHeight"@en , "全体長さ"@ja-JP , "전체 길이"@ko-KR ;
        rdfs:range             <https://w3id.org/product/PositiveLengthMeasure> ;
        schema:domainIncludes  <https://w3id.org/product/DiscreteAccessory%2FFixing%20socket> .

props:maximumShortCircuitTemperature
        a                      owl:DatatypeProperty ;
        rdfs:comment           "The maximum short circuit temperature at which a cable or bus is certified to operate."@en , "ケーブルや母線の最大短絡温度を示す。"@ja-JP , "케이블과 모선의 최대 단락 온도를 나타낸다."@ko-KR ;
        rdfs:label             "maximumShortCircuitTemperature"@en , "短絡許容最高温度"@ja-JP , "단락 허용 최고 온도"@ko-KR ;
        rdfs:range             <https://w3id.org/product/ThermodynamicTemperatureMeasure> ;
        schema:domainIncludes  <https://w3id.org/product/CableSegment%2FCABLESEGMENT> .

props:finishType  a            owl:DatatypeProperty ;
        rdfs:comment           "The type of finish for the air terminal."@en , "ターミナルの仕上げの形式（ANNODIZED,塗装他）"@ja-JP , "Le type de finition du terminal de ventilation."@fr-FR ;
        rdfs:label             "finishType"@en , "仕上げ形式"@ja-JP , "TypeFinition"@fr-FR ;
        schema:domainIncludes  <https://w3id.org/product/AirTerminal> .

props:solarReflectanceFront
        a                      owl:DatatypeProperty ;
        rdfs:comment           "Reflectance at normal incidence (solar): front side. Defines the fraction of the solar ray that is reflected and not transmitted when the ray passes from one medium into another, at the \"front\" side of the other material, perpendicular to the surface. Dependent on material and surface characteristics."@en ;
        rdfs:label             "solarReflectanceFront"@en ;
        rdfs:range             <https://w3id.org/product/PositiveRatioMeasure> ;
        schema:domainIncludes  <https://w3id.org/product/Material> .

props:cameraType  a            owl:DatatypeProperty ;
        rdfs:comment           "Indicates the type of camera."@en , "カメラの形式を示す。"@ja-JP , "카메라의 형식을 보여준다."@ko-KR ;
        rdfs:label             "cameraType"@en , "カメラ形式"@ja-JP , "카메라 형식"@ko-KR ;
        schema:domainIncludes  <https://w3id.org/product/AudioVisualAppliance%2FCAMERA> .

props:frameSize  a             owl:DatatypeProperty ;
        rdfs:comment           "Designation of the frame size according to the named range of frame sizes designated at the place of use or according to a given standard."@en , "フレームサイズの意味が実際の大きさを表示しているのか、規格表記なのかを指定。"@ja-JP , "프레임 크기의 의미가 실제 크기를 표시하고 있는지, 표준 표기인지 지정합니다."@ko-KR ;
        rdfs:label             "frameSize"@en , "フレームサイズ"@ja-JP , "프레임 크기"@ko-KR ;
        rdfs:range             xsd:string ;
        schema:domainIncludes  <https://w3id.org/product/ElectricMotor> .

props:applianceDiversity
        a                      owl:DatatypeProperty ;
        rdfs:comment           "기기의 부하율."@ko-KR , "기기의 부하율"@ko-KR , "Diversity of appliance load."@en , "機器の負荷率。"@ja-JP ;
        rdfs:label             "applianceDiversity"@en , "기기의 부하율"@ko-KR , "機器の負荷率"@ja-JP ;
        rdfs:range             <https://w3id.org/product/PositiveRatioMeasure> ;
        schema:domainIncludes  <https://w3id.org/product/Space> , <https://w3id.org/product/SpatialElement> , <https://w3id.org/product/SpatialZone> , <https://w3id.org/product/Zone> .

props:capacity  a              owl:DatatypeProperty ;
        rdfs:comment           "Cooling tower capacity in terms of heat transfer rate of the cooling tower between air stream and water stream."@en , "The product of the  ideal capacity and the overall volumetric efficiency of the compressor."@en , "Le produit de la puissance optimale par le rendement global du compresseur."@fr-FR ;
        rdfs:label             "capacity"@en , "Puissance"@fr-FR ;
        schema:domainIncludes  <https://w3id.org/product/CoolingTower> , <https://w3id.org/product/Chiller> .

props:sealMaterial  a          owl:DatatypeProperty ;
        rdfs:comment           "The material from which the damper seals are constructed."@en ;
        rdfs:label             "sealMaterial"@en ;
        schema:domainIncludes  <https://w3id.org/product/Damper> .

props:idealCapacity  a         owl:DatatypeProperty ;
        rdfs:comment           "Compressor capacity under ideal conditions."@en , "Puissance maximale sous des conditions idéales"@fr-FR ;
        rdfs:label             "idealCapacity"@en , "PuissanceMaximale"@fr-FR ;
        rdfs:range             <https://w3id.org/product/PowerMeasure> ;
        schema:domainIncludes  <https://w3id.org/product/Compressor> .

props:fragilityRating
        a                      owl:DatatypeProperty ;
        rdfs:comment           "脆弱性等級。当該国の建築法規による。"@ja-JP , "Indication de la fragilité du revêtement selon une classification nationale."@fr-FR , "Angabe zur Zerbrechlichkeit des Materials (zum Beispiel unter Brandlast oder Erschütterung) gemäß der nationalen oder regionalen Normen."@de-DE , "Indication on the fragility of the covering (e.g., under fire conditions).  It is given according to the national building code that might provide a classification for fragility."@en ;
        rdfs:label             "脆弱性等級"@ja-JP , "Fragilitätsklasse"@de-DE , "Fragilité"@fr-FR , "fragilityRating"@en ;
        rdfs:range             xsd:string ;
        schema:domainIncludes  <https://w3id.org/product/Covering> .

props:refrigerantFoulingResistance
        a                      owl:DatatypeProperty ;
        rdfs:comment           "Fouling resistance on the refrigerant side."@en ;
        rdfs:label             "refrigerantFoulingResistance"@en ;
        schema:domainIncludes  <https://w3id.org/product/Evaporator> , <https://w3id.org/product/Condenser> .

props:airHandlerConstruction
        a                      owl:DatatypeProperty ;
        rdfs:comment           "Enumeration defining how the air handler might be fabricated."@en , "空調機の組立方法の定義の列挙"@ja-JP ;
        rdfs:label             "airHandlerConstruction"@en , "空調機製造"@ja-JP ;
        schema:domainIncludes  <https://w3id.org/product/UnitaryEquipment%2FAIRHANDLER> .

props:spaceTemperature
        a                      owl:DatatypeProperty ;
        rdfs:comment           "Temperature of the space or zone, that is required from user/designer view point.  If no summer or winter space temperature requirements are given, it applies all year, otherwise for the intermediate period. Provide this value, if no temperatur range (Min-Max) is available."@en , "Geforderte Raumtemperatur, die nicht überschritten werden darf, gilt als ganzjährige Anforderung unabhängig vom Heizungs-, oder Kühlungsfall. Diese wird angegeben, wenn kein geforderter Temperaturbereich (Min - Max) vorhanden ist."@de-DE , "空間またはゾーンの温度。利用者/設計者の視点から要求される。もし夏季または冬季の室内温度要求が与えられないと、それは通年に、さもなければ中間季に適用される。"@ja-JP , "Temperature of the space."@en , "Température de l'espace ou de la zone spécifiée par l'usager ou le concepteur. Si les valeurs pour l'été et l'hiver ne sont pas connues, cette température s'applique toute l'année, sinon seulement en demi-saison. A fournir si les valeurs maximale et minimale ne sont pas connues."@fr-FR , "室内の温度"@ja-JP ;
        rdfs:label             "最高室内温度"@ja-JP , "spaceTemperature"@en , "室内温度"@ja-JP , "Raumtemperatur"@de-DE , "Température"@fr-FR ;
        rdfs:range             <https://w3id.org/product/ThermodynamicTemperatureMeasure> ;
        schema:domainIncludes  <https://w3id.org/product/cSpatialZone> , <https://w3id.org/product/cZone> , <https://w3id.org/product/Space> .

props:supportDuringTransportDocReference
        a                      owl:DatatypeProperty ;
        rdfs:comment           "Reference to an external document defining how the concrete element is supported during transportation."@en , "プレキャストコンクリート要素が輸送中における支持方法について書かれた外部ドキュメントの参照。"@ja-JP ;
        rdfs:label             "supportDuringTransportDocReference"@en , "輸送中の支持に関する参考文献"@ja-JP ;
        schema:domainIncludes  <https://w3id.org/product/BuildingElement> .

props:reinforcementSpacing
        a                      owl:DatatypeProperty ;
        rdfs:comment           "The spacing between reinforcing elements."@en , "補強要素間の距離"@ja-JP ;
        rdfs:label             "reinforcementSpacing"@en , "補強間隔"@ja-JP ;
        rdfs:range             <https://w3id.org/product/PositiveLengthMeasure> ;
        schema:domainIncludes  <https://w3id.org/product/DuctSegment> .

props:isSingleFlush  a         owl:DatatypeProperty ;
        rdfs:comment           "Indicates whether the cistern is single flush = TRUE (i.e. the same amount of water is used for each and every flush) or dual flush = FALSE (i.e. the amount of water used for a flush may be selected by the user to be high or low depending on the waste material to be removed)."@en , "単一フラッシュ= TRUE（各洗浄に同量の水が使用される）、デュアルフラッシュ= FALSE（洗浄する汚物に応じてハイまたはローをユーザが選択することができるフラッシュ使用）の指標を設定する。"@ja-JP ;
        rdfs:label             "isSingleFlush"@en , "単一のフラッシュ"@ja-JP ;
        rdfs:range             xsd:boolean ;
        schema:domainIncludes  <https://w3id.org/product/SanitaryTerminal%2FCISTERN> .

props:secondaryApparentPower
        a                      owl:DatatypeProperty ;
        rdfs:comment           "The power in VA (volt ampere) that has been transformed and is running out of the transformer on the secondary side."@en , "変圧器の2次側へ出力される電力（VA: アンペア）。"@ja-JP , "변압기 2 차측으로 출력되는 전력 (VA : 암페어)."@ko-KR ;
        rdfs:label             "secondaryApparentPower"@en , "第2電力"@ja-JP , "제 2 전원"@ko-KR ;
        rdfs:range             <https://w3id.org/product/PowerMeasure> ;
        schema:domainIncludes  <https://w3id.org/product/Transformer> .

props:shortCircuit1PolePowerFactorMaximumState
        a                      owl:DatatypeProperty ;
        rdfs:comment           "Power factor of the maximum 1 pole short circuit current provided at the point of supply i.e. the fault between 1 phase and N."@en , "電源供給時点の点1相とN間の1極最大短絡電流力率。"@ja-JP , "전원 공급 시점 점 1 단계와 N 사이의 1 극 최대 단락 전류 역률."@ko-KR ;
        rdfs:label             "shortCircuit1PolePowerFactorMaximumState"@en , "1極最大短絡電流力率"@ja-JP , "1 극 최대 단락 전류 역률"@ko-KR ;
        rdfs:range             xsd:decimal ;
        schema:domainIncludes  <https://w3id.org/product/ElectricFlowStorageDevice> .

props:torsionalConstantX
        a                      owl:DatatypeProperty ;
        rdfs:comment           "Torsional constant about xs. For example measured in mm4."@en ;
        rdfs:label             "torsionalConstantX"@en ;
        rdfs:range             <https://w3id.org/product/MomentOfInertiaMeasure> ;
        schema:domainIncludes  <https://w3id.org/product/ProfileDef> .

props:airflowType  a           owl:DatatypeProperty ;
        rdfs:comment           "Enumeration defining the functional type of air flow through the terminal."@en , "ターミナルを通過する気流の機能タイプ（給気、還気、排気他）"@ja-JP , "Enumération définissant le type fonctionnel de débit à travers le terminal"@fr-FR ;
        rdfs:label             "airflowType"@en , "エアフロータイプ"@ja-JP , "Type de débit d'air"@fr-FR ;
        schema:domainIncludes  <https://w3id.org/product/AirTerminal> .

props:boltSize  a              owl:DatatypeProperty ;
        rdfs:comment           "Size of the bolts securing the flange."@en , "フランジを締めるボルトの大きさ"@ja-JP ;
        rdfs:label             "boltSize"@en , "ボルトの大きさ"@ja-JP ;
        rdfs:range             <https://w3id.org/product/PositiveLengthMeasure> ;
        schema:domainIncludes  <https://w3id.org/product/PipeSegment> .

props:threadLength  a          owl:DatatypeProperty ;
        rdfs:comment           "Nominal length of the thread"@en ;
        rdfs:label             "threadLength"@en ;
        rdfs:range             <https://w3id.org/product/PositiveLengthMeasure> ;
        schema:domainIncludes  <https://w3id.org/product/MechanicalFastener%2FBOLT> .

props:torque  a                owl:DatatypeProperty ;
        rdfs:comment           "Indicates the maximum close-off torque for the actuator."@en , "アクチュエータの最大締め切りトルクを示す。"@ja-JP , "액츄에이터의 최대 마감 토크를 나타낸다."@ko-KR ;
        rdfs:label             "torque"@en , "最大トルク"@ja-JP , "최대 토크"@ko-KR ;
        rdfs:range             <https://w3id.org/product/TorqueMeasure> ;
        schema:domainIncludes  <https://w3id.org/product/Actuator> .

props:numberOfDrafts  a        owl:DatatypeProperty ;
        rdfs:comment           "单根烟囱内的烟道数目，烟道即烟囱内供空气流通的连续孔道。"@zh-CN , "Nombre de conduits, percements continus par lesquels passe l'air à l'intérieur d'une cheminée simple."@fr-FR , "Number of the chimney drafts, continuous holes in the chimney through which the air passes, within the single chimney."@en , "一つの煙突で、煙突の筒（chimney draft）、空気が流れる連続した穴の数。"@ja-JP , "Anzahl der Schornsteinzüge innerhalb eines Schornsteins. Gewöhnlich ein-, zwei, drei oder vierzügig."@de-DE ;
        rdfs:label             "烟道数"@zh-CN , "Nombre de conduits"@fr-FR , "穴の数"@ja-JP , "Zügigkeit"@de-DE , "numberOfDrafts"@en ;
        rdfs:range             <https://w3id.org/product/CountMeasure> ;
        schema:domainIncludes  <https://w3id.org/product/Chimney> .

props:scheduleCost  a          owl:DatatypeProperty ;
        rdfs:comment           "The budgeted cost on behalf of the resource allocation."@en , "資源配分のための予定されているコスト。"@ja-JP ;
        rdfs:label             "scheduleCost"@en , "予定コスト"@ja-JP ;
        schema:domainIncludes  <https://w3id.org/product/ConstructionResource> .

props:highestSeatingHeight
        a                      owl:DatatypeProperty ;
        rdfs:comment           "The value of seating height of high level if the chair height is adjustable."@en ;
        rdfs:label             "highestSeatingHeight"@en ;
        rdfs:range             <https://w3id.org/product/PositiveLengthMeasure> ;
        schema:domainIncludes  <https://w3id.org/product/Furniture%2FCHAIR> .

props:countedEfficiencyCurve
        a                      owl:DatatypeProperty ;
        rdfs:comment           "Counted efficiency curve as a function of dust holding weight, efficiency = f (dust holding weight)."@en ;
        rdfs:label             "countedEfficiencyCurve"@en ;
        schema:domainIncludes  <https://w3id.org/product/Filter%2FAIRPARTICLEFILTER> .

props:hasDrive  a              owl:DatatypeProperty ;
        rdfs:comment           "Indication whether this object has an automatic drive to operate it (TRUE) or no drive (FALSE)"@en , "Indique si cet objet est doté d'une motorisation (VRAI) ou non (FAUX)."@fr-FR , "Angabe, ob dieses Bauteil einen automatischen Antrieb zum Öffnen und Schließen besitzt (JA) oder nicht (NEIN)."@de-DE ;
        rdfs:label             "Antrieb"@de-DE , "Motorisé"@fr-FR , "hasDrive"@en ;
        rdfs:range             xsd:boolean ;
        schema:domainIncludes  <https://w3id.org/product/Window> , <https://w3id.org/product/Door> .

props:directionOfRotation
        a                      owl:DatatypeProperty ;
        rdfs:comment           "The direction of the centrifugal fan wheel rotation when viewed from the drive side of the fan.\n\nCLOCKWISE: Clockwise. \nCOUNTERCLOCKWISE: Counter-clockwise. \nOTHER: Other type of fan rotation."@en , "ファンの駆動側から見たホイール回転方向\nCLOCKWISE　　時計回り\n COUNTERCLOCKWISE　反時計回り\n OTHER　その他"@ja-JP ;
        rdfs:label             "directionOfRotation"@en , "角度方向"@ja-JP ;
        schema:domainIncludes  <https://w3id.org/product/Fan%2FCENTRIFUGAL> .

props:closureRatingEnum
        a                      owl:DatatypeProperty ;
        rdfs:comment           "Enumeration that identifies the closure rating for the damper."@en ;
        rdfs:label             "closureRatingEnum"@en ;
        schema:domainIncludes  <https://w3id.org/product/Damper%2FFIRESMOKEDAMPER> , <https://w3id.org/product/Damper%2FFIREDAMPER> .

props:secondaryCurrentType
        a                      owl:DatatypeProperty ;
        rdfs:comment           "A list of the secondary current types that can result from transformer output."@en , "変圧器より出力される第2電流の種類の一覧。"@ja-JP , "변압기에서 출력되는 제 2 전류의 종류 목록입니다."@ko-KR ;
        rdfs:label             "secondaryCurrentType"@en , "第2電流タイプ"@ja-JP , "제 2 전류 타입"@ko-KR ;
        schema:domainIncludes  <https://w3id.org/product/Transformer> .

props:fluid  a                 owl:DatatypeProperty ;
        rdfs:comment           "The properties of the hydronic fluid used for heat transfer within the coil tubes."@en , "Les propriétés du fluide utilisé pour l'échange thermique à l'intérieur des tubes de la batterie."@fr-FR ;
        rdfs:label             "fluid"@en , "Fluide"@fr-FR ;
        schema:domainIncludes  <https://w3id.org/product/Coil> .

props:wallCovering  a          owl:DatatypeProperty ;
        rdfs:comment           "Label to indicate the material or finish of the space flooring. The label is used for room book information and often displayed in room stamp.\n\nThe material information is provided in absence of an IfcCovering (type=CLADDING) object with own shape representation and material assignment. In case of inconsistency the material assigned to IfcCovering elements takes precedence."@en , "Angabe des Materials für die Wandbekleidung, oder den Wandbelag Diese Angabe wird im Raumbuch verwendet und oft im Raumstempel angezeigt.\n\nDie Materialangabe wird übernommen, wenn kein eigenes Bekleidungsobjekt (IfcCovering mit PredefinedType = CLADDING) für die Wandbekleidung dem Raum zugeordnet ist. Bei Inkonsistenzen (wenn beides gegeben ist), hat die Materialangabe des zugeordneten Bekleidungsobjekts Priorität."@de-DE , "Indication sur la nature du revêtement de mur […]. L'information sur le matériau est fournie en l'absence d'un objet de la classe IfcCovering (Type=CLADDING) avec sa propre représentation de forme et une assignation à un matériau. En cas d'incohérence, c'est le matériau assigné à l'instance de IfcCovering qui prime."@fr-FR , "部屋の壁材質または仕上げに関するラベル（識別情報）。このラベル名は部屋リスト情報や部屋情報表示の際に利用される。"@ja-JP ;
        rdfs:label             "壁仕上げ"@ja-JP , "RevetementMur"@fr-FR , "wallCovering"@en , "Wandbekleidung"@de-DE ;
        rdfs:range             xsd:string ;
        schema:domainIncludes  <https://w3id.org/product/Space> .

props:thermalTransmittance
        a                      owl:DatatypeProperty ;
        rdfs:comment           "熱貫流率U値。ここでは壁を通した熱移動の方向における全体の熱還流率を示す。"@ja-JP , "Thermal transmittance coefficient (U-Value) of the element. Here the total thermal transmittance coefficient through the beam within the direction of the thermal flow (including all materials).\n\nNote: new property in IFC4"@en , "材料の熱貫流率（U値）。ここでは、煙突全体の熱の流れる方向の熱貫流率（全ての材料を含む）。"@ja-JP , "Wärmedurchgangskoeffizient (U-Wert) der Materialschichten.\nHier der Gesamtwärmedurchgangskoeffizient des Fensters."@de-DE , "材料的导热系数（U值）。\n表示该烟囱在传热方向上的整体导热系数（包括所有材料）。\n注：IFC2x4新添属性"@zh-CN , "Thermal transmittance coefficient (U-Value) of the element. It is the total thermal transmittance coefficient through the building element proxy within the direction of the thermal flow (including all materials).\n\nNote: new property in IFC4"@en , "Coefficient de transmission thermique surfacique (U). C'est le coefficient global de transmission thermique à travers la membrure dans la direction du flux thermique (tous matériaux inclus). Nouvelle propriété de la version 2x4."@fr-FR , "熱貫流率U値。ここではスラブを通した熱移動の方向における全体の熱還流率を示す。"@ja-JP , "Wärmedurchgangskoeffizient (U-Wert) der Materialschichten.\nHier der Gesamtwärmedurchgangskoeffizient der Tür."@de-DE , "Coefficient de transmission thermique surfacique (U) d'un métériau d'une certaine épaisseur pour cet élément"@fr-FR , "Thermal transmittance coefficient (U-Value) of a material of a certain thickness for this element."@en , "材料的导热系数（U值）。\n适用于门的整体结构。"@zh-CN , "熱貫流率（U値）。\nここでは（すべての材料を含む）屋根面を通した全体の熱還流率を示す。"@ja-JP , "Wärmedurchgangskoeffizient (U-Wert) der Materialschichten.\nHier der Gesamtwärmedurchgangskoeffizient der Decke (für alle Schichten)."@de-DE , "Wärmedurchgangskoeffizient (U-Wert) der Materialschichten.\nHier der Gesamtwärmedurchgangskoeffizient der Dachkonstruktion (für alle Schichten)."@de-DE , "Thermal transmittance coefficient (U-Value) of the element. Here the total thermal transmittance coefficient through the column within the direction of the thermal flow (including all materials).\n\nNore: new property in IFC4"@en , "Coefficient de transmission thermique surfacique (U). C'est le coefficient global de transmission thermique à travers le mur dans la direction du flux thermique (tous matériaux inclus). Nouvelle propriété de la version 2x4."@fr-FR , "Wärmedurchgangskoeffizient (U-Wert) der Materialschichten.\nHier der Gesamtwärmedurchgangskoeffizient des Balkens (in Richtung des Wärmeflusses), angegeben ohne den inneren und äußeren Wärmeübergangswiderstand."@de-DE , "材料的导热系数（U值）。\n\n表示该梁在传热方向上的整体导热系数（包括所有材料）。\n\n注：IFC2x4新添属性"@zh-CN , "Wärmedurchgangskoeffizient (U-Wert) der Materialschichten.\nHier der Gesamtwärmedurchgangskoeffizient des Schornsteins (in Richtung des Wärmeflusses), angegeben ohne den inneren und äußeren Wärmeübergangswiderstand."@de-DE , "Coefficient de transmission thermique surfacique (U). C'est le coefficient global de transmission thermique à travers la dalle (tous matériaux inclus)."@fr-FR , "Coefficient de transmission thermique (U) qui s'applique à l'ensemble de la plaque."@fr-FR , "熱貫流率U値。ここでは窓を通した熱移動の方向における全体の熱還流率を示す。"@ja-JP , "Thermal transmittance coefficient (U-Value) of a material.\nHere the total thermal transmittance coefficient through the member within the direction of the thermal flow (including all materials).\nNote: new property in IFC4."@en , "Coefficient de transmission thermique surfacique (U). C'est le coefficient global de transmission thermique à travers la poutre dans la direction du flux thermique (tous matériaux inclus). Nouvelle propriété de la version 2x4."@fr-FR , "Coefficient de transmission thermique surfacique (U). C'est le coefficient global de transmission thermique à travers le revêtement dans la direction du flux thermique (tous matériaux inclus). Nouvelle propriété de la version 2x4."@fr-FR , "Thermal transmittance coefficient (U-Value) of a material.\nHere the total thermal transmittance coefficient through the wall (including all materials)."@en , "Wärmedurchgangskoeffizient (U-Wert) der Materialschichten.\nHier der Gesamtwärmedurchgangskoeffizient der Platte (für alle Schichten)."@de-DE , "熱貫流率U値。ここではメンバーオブジェクトを通した熱移動の方向における全体の熱還流率を示す。"@ja-JP , "Coefficient de transmission thermique surfacique (U). C'est le coefficient global de transmission thermique à travers le poteau dans la direction du flux thermique (tous matériaux inclus). Nouvelle propriété de la version 2x4."@fr-FR , "熱貫流率U値。"@ja-JP , "材料的导热系数（U值）。\n\n表示该柱在传热方向上的整体导热系数（包括所有材料）。\n\n注：IFC2x4新添属性"@zh-CN , "熱貫流率U値。ここでは柱を通した熱移動の方向における全体の熱還流率を示す。"@ja-JP , "材料的导热系数（U值）。\n表示穿过该屋顶表面的整体导热系数（包括所有材料）"@zh-CN , "材料的导热系数（U值）。\n适用于窗的整体结构。"@zh-CN , "Thermal transmittance coefficient (U-Value) of a material. Here the total thermal transmittance coefficient through the slab (including all materials)."@en , "材料的导热系数（U值）。\n表示该墙在传热方向上的整体导热系数（包括所有材料）。"@zh-CN , "Coefficient de transmission thermique surfacique (U). C'est le coefficient global de transmission thermique à travers la cheminée dans la direction du flux thermique (tous matériaux inclus). Nouvelle propriété de la version 2x4."@fr-FR , "熱貫流率U値。ここではオブジェクトを通した熱移動の方向における全体の熱還流率を示す。"@ja-JP , "Coefficient de transmission thermique surfacique (U). C'est le coefficient global de transmission thermique à travers l'élément dans la direction du flux thermique (tous matériaux inclus). Nouvelle propriété de la version 2x4."@fr-FR , "熱貫流率U値。ここではカーテンウォールを通した熱移動の方向における全体の熱還流率を示す。"@ja-JP , "材料的导热系数（U值）。\n表示该构件在传热方向上的整体导热系数（包括所有材料）。\n注：IFC2x4新添属性"@zh-CN , "熱貫流率U値。ここではカバリングを通した熱移動の方向における全体の熱還流率を示す。"@ja-JP , "熱貫流率U値。\nここでは（すべての材料を含む）梁を通した熱移動の方向における全体の熱還流率を示す。\n注：IFC2x4の新しいプロパティ"@ja-JP , "材料の熱貫流率（U値）。すべての扉部材に適応される。"@ja-JP , "Thermal transmittance coefficient (U-Value) of an element. \nHere the total thermal transmittance coefficient through the covering (including all materials)."@en , "材料的导热系数（U值）。\n表示穿过该板的整体导热系数（包括所有材料）。"@zh-CN , "Coefficient de transmission thermique surfacique (U). C'est le coefficient global de transmission thermique à travers la surface de la couverture (tous matériaux inclus)."@fr-FR , "Coefficient de transmission thermique (U) d'un matériau. Il s'applique à l'ensemble de la porte."@fr-FR , "Thermal transmittance coefficient (U-Value) of a material.\nHere the total thermal transmittance coefficient through the roof surface (including all materials)."@en , "Wärmedurchgangskoeffizient (U-Wert) der Materialschichten. Angegeben wird der  Gesamtwärmedurchgangskoeffizient des Proxy-Elements (in Richtung des Wärmeflusses), ohne den inneren und äußeren Wärmeübergangswiderstand."@de-DE , "Coefficient de transmission thermique surfacique (U). C'est le coefficient global de transmission thermique à travers le mur (tous matériaux inclus)."@fr-FR , "Thermal transmittance coefficient (U-Value) of an element. Here the total thermal transmittance coefficient through the chimney within the direction of the thermal flow (including all materials)."@en , "Wärmedurchgangskoeffizient (U-Wert) der Materialschichten.\nHier der Gesamtwärmedurchgangskoeffizient der Bekleidung (für alle Schichten)."@de-DE , "Wärmedurchgangskoeffizient (U-Wert) der Materialschichten.\nHier der Gesamtwärmedurchgangskoeffizient der Wand (für alle Schichten)."@de-DE , "Coefficient de transmission thermique (U) d'un matériau. Il s'applique à l'ensemble de la fenêtre."@fr-FR , "材料的导热系数（U值）。\n表示穿过该墙的整体导热系数（包括所有材料）。"@zh-CN , "Thermal transmittance coefficient (U-Value) of a material.\nIt applies to the total door construction."@en , "材料的导热系数（U值）。\n表示该烟囱在传热方向上的整体导热系数（包括所有材料）。"@zh-CN , "材料的导热系数（U值）。\n表示穿过该覆盖层的整体导热系数（包括所有材料）。"@zh-CN ;
        rdfs:label             "Transmission thermique surfacique"@fr-FR , "TransmissionThermique"@fr-FR , "导热系数"@zh-CN , "thermalTransmittance"@en , "U-Wert"@de-DE , "熱貫流率"@ja-JP ;
        rdfs:range             <https://w3id.org/product/ThermalTransmittanceMeasure> ;
        schema:domainIncludes  <https://w3id.org/product/Beam> , <https://w3id.org/product/Wall> , <https://w3id.org/product/Member> , <https://w3id.org/product/CurtainWall> , <https://w3id.org/product/Column> , <https://w3id.org/product/ShadingDevice> , <https://w3id.org/product/Slab> , <https://w3id.org/product/Roof> , <https://w3id.org/product/Covering> , <https://w3id.org/product/BuildingElementProxy> , <https://w3id.org/product/Plate> , <https://w3id.org/product/Door> , <https://w3id.org/product/Window> , <https://w3id.org/product/Chimney> .

props:riskOwner  a             owl:DatatypeProperty ;
        rdfs:comment           "A determination of who is the owner of the risk by reference to principal roles of organizations within a project. Determination of the specific organization should be by reference to instances of IfcActorRole assigned to instances of IfcOrganization (if assigned)."@en ;
        rdfs:label             "riskOwner"@en ;
        schema:domainIncludes  <https://w3id.org/product/Process> .

props:leakageClass  a          owl:DatatypeProperty ;
        rdfs:comment           "Nominal leakage rating for the system components."@en , "ダクトシステム各部位の漏れ率。"@ja-JP , "덕트 시스템 각 부위의 누출 비율."@ko-KR ;
        rdfs:label             "leakageClass"@en , "漏れ率"@ja-JP , "누설비율"@ko-KR ;
        rdfs:range             <https://w3id.org/product/PressureMeasure> ;
        schema:domainIncludes  <https://w3id.org/product/DistributionSystem%2FVENTILATION> .

props:earthFailureDeviceType
        a                      owl:DatatypeProperty ;
        rdfs:comment           "A list of the available types of circuit breaker from which that required may be selected where:\n\nStandard: Device that operates without a time delay.\nTimeDelayed: Device that operates after a time delay."@en , "以下の中から選択が必要となる場合の遮断機タイプのリスト：\n\nスタンダード：遅延無しで動作する機器\n遅延：一定時間を経た後で動作する機器"@ja-JP , "다음 중 선택이 필요한 경우 차단기 유형 목록 : 스탠다드 : 지연없이 동작하는 기기 지연 : 일정 시간이 지난 후에 동작하는 기기 \""@ko-KR ;
        rdfs:label             "earthFailureDeviceType"@en , "漏電回路遮断機のタイプ"@ja-JP , "누전 회로 차단기의 유형"@ko-KR ;
        schema:domainIncludes  <https://w3id.org/product/ProtectiveDevice%2FEARTHLEAKAGECIRCUITBREAKER> .

props:sizingMethod  a          owl:DatatypeProperty ;
        rdfs:comment           "Identifies whether the damper is sized nominally or with exact measurements:\n\nNOMINAL: Nominal sizing method. \nEXACT: Exact sizing method."@en ;
        rdfs:label             "sizingMethod"@en ;
        schema:domainIncludes  <https://w3id.org/product/Damper> .

props:ratedCurrent  a          owl:DatatypeProperty ;
        rdfs:comment           "The current that a device is designed to handle."@en ;
        rdfs:label             "ratedCurrent"@en ;
        schema:domainIncludes  <https://w3id.org/product/DistributionElement> .

props:requestSourceName
        a                      owl:DatatypeProperty ;
        rdfs:comment           "The person making the request, where known."@en , "要請源の識別を確認するための特定の名称またはラベル。電子メールの場合、電子メールアドレスに相当する。"@ja-JP ;
        rdfs:label             "requestSourceName"@en , "要請ソースラベル"@ja-JP ;
        schema:domainIncludes  <https://w3id.org/product/ActionRequest> .

props:assemblyPlace  a         owl:DatatypeProperty ;
        rdfs:comment           "Enumeration defining where the assembly is intended to take place, either in a factory or on the building site."@en , "Enumeration defining where the assembly is intended to take place, either in a factory, other offsite location or on the building site."@en ;
        rdfs:label             "assemblyPlace"@en ;
        schema:domainIncludes  <https://w3id.org/product/Element> .

props:shearModulus  a          owl:DatatypeProperty ;
        rdfs:comment           "A measure of the shear modulus of elasticity of the material."@en ;
        rdfs:label             "shearModulus"@en ;
        rdfs:range             <https://w3id.org/product/ModulusOfElasticityMeasure> ;
        schema:domainIncludes  <https://w3id.org/product/Material> .

props:coilLength  a            owl:DatatypeProperty ;
        rdfs:comment           "Length of coil."@en ;
        rdfs:label             "coilLength"@en ;
        rdfs:range             <https://w3id.org/product/PositiveLengthMeasure> ;
        schema:domainIncludes  <https://w3id.org/product/CooledBeam> .

props:faucetFunction  a        owl:DatatypeProperty ;
        rdfs:comment           "Defines the operating temperature of a faucet that may be specified."@en , "水栓の作動温度を明確に定義する。"@ja-JP ;
        rdfs:label             "faucetFunction"@en , "水栓機能"@ja-JP ;
        schema:domainIncludes  <https://w3id.org/product/Valve%2FFAUCET> .

props:glassThickness1
        a                      owl:DatatypeProperty ;
        rdfs:comment           "最初の（室内側）ガラスの厚み。"@ja-JP , "第一层（内侧）玻璃的厚度。"@zh-CN , "German-description-2"@de-DE , "Epaisseur de la première couche de verre (côté intérieur)"@fr-FR , "Thickness of the first (inner) glass layer."@en ;
        rdfs:label             "glassThickness1"@en , "German-name-2"@de-DE , "EpaisseurVitrage1"@fr-FR , "ガラス厚1"@ja-JP , "玻璃厚度1"@zh-CN ;
        rdfs:range             <https://w3id.org/product/PositiveLengthMeasure> ;
        schema:domainIncludes  <https://w3id.org/product/Door> , <https://w3id.org/product/cWindow> .

props:bladeMaterial  a         owl:DatatypeProperty ;
        rdfs:comment           "The material from which the damper blades are constructed."@en ;
        rdfs:label             "bladeMaterial"@en ;
        schema:domainIncludes  <https://w3id.org/product/Damper> .

props:numberOfPanels  a        owl:DatatypeProperty ;
        rdfs:comment           "Number of panels."@en , "パネルの数"@ja-JP ;
        rdfs:label             "numberOfPanels"@en , "パネルの数"@ja-JP ;
        rdfs:range             xsd:int ;
        schema:domainIncludes  <https://w3id.org/product/SpaceHeater> .

props:boilingPoint  a          owl:DatatypeProperty ;
        rdfs:comment           "The boiling point of the material (fluid)."@en ;
        rdfs:label             "boilingPoint"@en ;
        rdfs:range             <https://w3id.org/product/ThermodynamicTemperatureMeasure> ;
        schema:domainIncludes  <https://w3id.org/product/Material> .

props:thermalIrEmissivityBack
        a                      owl:DatatypeProperty ;
        rdfs:comment           "Thermal IR emissivity: back side. Defines the fraction of thermal energy emitted per unit area to \"blackbody\" at the same temperature, through the \"back\" side of the material."@en ;
        rdfs:label             "thermalIrEmissivityBack"@en ;
        rdfs:range             <https://w3id.org/product/PositiveRatioMeasure> ;
        schema:domainIncludes  <https://w3id.org/product/Material> .

props:options  a               owl:DatatypeProperty ;
        rdfs:comment           "A statement of the options available in the agreement."@en ;
        rdfs:label             "options"@en ;
        rdfs:range             xsd:string ;
        schema:domainIncludes  <https://w3id.org/product/SpatialStructureElement> .

props:shortOutsideTopBarPitch
        a                      owl:DatatypeProperty ;
        rdfs:comment           "The pitch length of the short outside top bar."@en , "短辺方向・柱列帯・上端の鉄筋間隔。"@ja-JP ;
        rdfs:label             "shortOutsideTopBarPitch"@en , "短辺・柱列帯・上端ピッチ"@ja-JP ;
        rdfs:range             <https://w3id.org/product/PositiveLengthMeasure> ;
        schema:domainIncludes  <https://w3id.org/product/Slab> .

props:i5  a                    owl:DatatypeProperty ;
        rdfs:comment           "The upper electromagnetic testing current limit in [x In], indicating that for currents larger than I5, the tripping time shall be shorter than or equal to the associated tripping time, T5, i.e. the device shall trip instantaneous."@en , "電磁の高試験電流限界値を [x In], 電流は I4 よりも低い値を示す。トリップ時間は関連する T5 と瞬時に遮断する定格使用電流の時間よりも長い。"@ja-JP , "전자의 높은 시험 전류 한계를 [x In] 전류는 I4보다 낮은 값을 나타낸다. 트립 시간은 관련 T5 즉석에서 차단하는 정격 사용 전류의 시간보다 길다."@ko-KR ;
        rdfs:label             "i5"@en , "I5"@ja-JP , "I5"@ko-KR ;
        rdfs:range             xsd:decimal ;
        schema:domainIncludes  <https://w3id.org/product/ProtectiveDeviceTrippingUnit%2FELECTROMAGNETIC> .

props:leakageFullyClosed
        a                      owl:DatatypeProperty ;
        rdfs:comment           "Leakage when fully closed."@en ;
        rdfs:label             "leakageFullyClosed"@en ;
        rdfs:range             <https://w3id.org/product/VolumetricFlowRateMeasure> ;
        schema:domainIncludes  <https://w3id.org/product/Damper> .

props:numberOfParallelCircuits
        a                      owl:DatatypeProperty ;
        rdfs:comment           "Number of parallel circuits."@en ;
        rdfs:label             "numberOfParallelCircuits"@en ;
        rdfs:range             xsd:int ;
        schema:domainIncludes  <https://w3id.org/product/CableSegment> .

props:atmosphericAcidification
        a                      owl:DatatypeProperty ;
        rdfs:comment           "算出されたSO2と等しい大気中の酸性化の責任を負うガスの量。"@ja-JP , "Quantity of gases responsible for the atmospheric acidification calculated in equivalent SO2."@en , "Quantité de gaz responsables de l'acidification atmosphérique exprimée en Kg d'équivalent SO2, selon les normes PrEN15804:2008 [NDT : ou NF P01-010]"@fr-FR , "SO2에 해당 환산된 대기 산성 화의 원인이되는 가스량"@ko-KR ;
        rdfs:label             "AcidificationAtmospherique"@fr-FR , "atmosphericAcidification"@en , "大気の酸性化"@ja-JP , "대기산성화"@ko-KR ;
        rdfs:range             <https://w3id.org/product/MassMeasure> ;
        schema:domainIncludes  <https://w3id.org/product/Element> .

props:nominalParticleGeometricMeanDiameter
        a                      owl:DatatypeProperty ;
        rdfs:comment           "Particle geometric mean diameter associated with nominal efficiency."@en ;
        rdfs:label             "nominalParticleGeometricMeanDiameter"@en ;
        rdfs:range             <https://w3id.org/product/PositiveLengthMeasure> ;
        schema:domainIncludes  <https://w3id.org/product/Filter> .

props:maximumPlateThickness
        a                      owl:DatatypeProperty ;
        rdfs:comment           "This value may be needed for stress analysis and to handle buckling problems. It can also be derived from the given profile geometry or classification and therefore it is only an optional feature allowing for an explicit description. For example measured in mm."@en ;
        rdfs:label             "maximumPlateThickness"@en ;
        rdfs:range             <https://w3id.org/product/PositiveLengthMeasure> ;
        schema:domainIncludes  <https://w3id.org/product/ProfileDef> .

props:bodyMaterial  a          owl:DatatypeProperty ;
        rdfs:comment           "Material from which the body of the valve is constructed."@en , "弁の本体が作られている材料"@ja-JP ;
        rdfs:label             "bodyMaterial"@en , "本体材料"@ja-JP ;
        schema:domainIncludes  <https://w3id.org/product/Valve> .

props:iCU60947  a              owl:DatatypeProperty ;
        rdfs:comment           "The ultimate breaking capacity in [A] for an MCB tested in accordance with the IEC 60947 series."@en , "IEC의 60947 시리즈를 기반으로 테스트 회로 차단기 및 모터 보호 장치의 단락 차단 용량 [A]."@ko-KR , "IECの60947シリーズに基づいてテスト配線用遮断機またはモータ保護装置のための遮断容量を[A]で設定。"@ja-JP , "IEC의 60947 시리즈를 기반으로 테스트 배선용 차단기 또는 모터 보호 장치를위한 차단 용량 [A]로 설정."@ko-KR , "IECの60947シリーズに基づいてテストされた回路遮断機及びモータ保護装置の短絡遮断容量[A]。"@ja-JP , "IEC의 60948 시리즈를 기반으로 시험한 MCB의 정격 한계 단락 차단 용량 [A]로 설정."@ko-KR , "The ultimate breaking capacity in [A] for a circuit breaker or motor protection device tested in accordance with the IEC 60947 series."@en , "IECの60947シリーズに基づいてテストされたMCBの定格限界短絡遮断容量を[A]で設定。"@ja-JP ;
        rdfs:label             "정격한계단락 차단 용량"@ko-KR , "iCU60947"@en , "定格限界短絡遮断容量"@ja-JP , "ICU60947"@ja-JP , "ICU60947"@ko-KR , "정격 한계 단락 차단 용량"@ko-KR ;
        rdfs:range             <https://w3id.org/product/ElectricCurrentMeasure> ;
        schema:domainIncludes  <https://w3id.org/product/ProtectiveDevice%2FCIRCUITBREAKER> , <https://w3id.org/product/ProtectiveDevice> .

props:airResistanceCurve
        a                      owl:DatatypeProperty ;
        rdfs:comment           "Air resistance curve (w/ fan only); Pressure = f ( flow rate)."@en , "空気抵抗曲線（送風機のみ）圧力＝ｆ（流速）"@ja-JP ;
        rdfs:label             "airResistanceCurve"@en , "空気抵抗曲線"@ja-JP ;
        schema:domainIncludes  <https://w3id.org/product/SpaceHeater> .

props:functionalUnitReference
        a                      owl:DatatypeProperty ;
        rdfs:comment           "데이터베이스 또는 분류에 대한 참조"@ko-KR , "データベースやクラスへの参照。"@ja-JP , "Référence à une base de données ou à une classification [NDT : référence, par exemple, à l'identification d'un produit dans la base INIES]"@fr-FR , "Reference to a database or a classification"@en ;
        rdfs:label             "ReferenceUniteFonctionnelle"@fr-FR , "機能単位参照"@ja-JP , "functionalUnitReference"@en , "기능단위참조"@ko-KR ;
        rdfs:range             xsd:string ;
        schema:domainIncludes  <https://w3id.org/product/Element> .

props:adjustmentValues
        a                      owl:DatatypeProperty ;
        rdfs:comment           "A list of time adjustment values that may be applied to a tripping unit for an AdjustmentValueType = LIST. A minimum of 1 and a maximum of 16 adjustment values may be specified. Note that this property should not have a value for an  AdjustmentValueType = RANGE."@en , "A list of current adjustment values that may be applied to a tripping unit for an AdjustmentValueType = LIST. A minimum of 1 and a maximum of 16 adjustment values may be specified. Note that this property should not have a value for an  AdjustmentValueType = RANGE."@en , "時間調整値を１から16で設定。範囲では、ない事を注意。"@ja-JP , "시간 조정 값을 1에서 16로 설정. 범위는없는 것을주의."@ko-KR ;
        rdfs:label             "adjustmentValues"@en , "調整値"@ja-JP , "조정 값"@ko-KR ;
        schema:domainIncludes  <https://w3id.org/product/ProtectiveDeviceTrippingUnit> .

props:atmosphericPressure
        a                      owl:DatatypeProperty ;
        rdfs:comment           "周囲の大気圧"@ja-JP , "周囲大気圧"@ja-JP , "標準大気圧(外気圧）"@ja-JP , "Ambient atmospheric pressure."@en , "Pression atmosphérique ambiante."@fr-FR , "Pression atmosphérique ambiante"@fr-FR ;
        rdfs:label             "標準大気圧（外気圧）"@ja-JP , "大気圧"@ja-JP , "atmosphericPressure"@en , "Pression atmosphérique"@fr-FR ;
        schema:domainIncludes  <https://w3id.org/product/AirTerminalBox> , <https://w3id.org/product/DuctSegment> , <https://w3id.org/product/Coil> , <https://w3id.org/product/Humidifier> , <https://w3id.org/product/DuctFitting> .

props:nonHazardousWastePerUnit
        a                      owl:DatatypeProperty ;
        rdfs:comment           "Quantity of non hazardous waste generated"@en , "Quantité de déchets non dangereux générés tels que définis dans la norme  ISO21930:2007 [NDT : et dans la norme NF P01-010]."@fr-FR , "비 유해 폐기물의 발생량"@ko-KR , "生成された無害な排気量。"@ja-JP ;
        rdfs:label             "DechetsNonDangereuxParUnite"@fr-FR , "単位あたり非有害廃棄物"@ja-JP , "단위당 비 유해 폐기물"@ko-KR , "nonHazardousWastePerUnit"@en ;
        rdfs:range             <https://w3id.org/product/MassMeasure> ;
        schema:domainIncludes  <https://w3id.org/product/Element> .

props:secondarySurfaceArea
        a                      owl:DatatypeProperty ;
        rdfs:comment           "Secondary heat transfer surface area created by fins."@en , "Surface d'échange thermique au secondaire crée par les ailettes."@fr-FR ;
        rdfs:label             "secondarySurfaceArea"@en , "SurfaceEchangeSecondaire"@fr-FR ;
        rdfs:range             <https://w3id.org/product/AreaMeasure> ;
        schema:domainIncludes  <https://w3id.org/product/Coil> .

props:fillGas  a               owl:DatatypeProperty ;
        rdfs:comment           "German-description-5"@de-DE , "两层玻璃之间填充气体的名称。仅供参考。"@zh-CN , "Name of the gas by which the gap between two glass layers is filled. It is given for information purposes only."@en , "Nom du gaz remplissant l'espace entre deux couches de verre. Donné à titre informatif seulement."@fr-FR , "2枚のガラス間の隙間に充填されたガスの名称。これは情報目的専用に提供される。"@ja-JP ;
        rdfs:label             "fillGas"@en , "German-name-5"@de-DE , "GazEntreVitrages"@fr-FR , "填充气体"@zh-CN , "充填ガス種"@ja-JP ;
        rdfs:range             xsd:string ;
        schema:domainIncludes  <https://w3id.org/product/Door> , <https://w3id.org/product/cWindow> .

props:dimensionalChangeCoefficient
        a                      owl:DatatypeProperty ;
        rdfs:comment           "Weighted dimensional change coefficient, relative to 1% change in moisture content."@en ;
        rdfs:label             "dimensionalChangeCoefficient"@en ;
        rdfs:range             <https://w3id.org/product/PositiveRatioMeasure> ;
        schema:domainIncludes  <https://w3id.org/product/Material%2FWood> .

props:workMonthDuration
        a                      owl:DatatypeProperty ;
        rdfs:comment           "The elapsed time within a worktime-based month. For presentation purposes, applications may choose to display IfcTask durations in work months where IfcTaskTime.DurationType=WORKTIME. This value must be less than or equal to 744 hours (an elapsed month of 31 days); if omitted then 160 hours is assumed."@en , "作業時間を基にした経過時間の週数の月数。"@ja-JP ;
        rdfs:label             "workMonthDuration"@en , "作業月数"@ja-JP ;
        rdfs:range             xsd:duration ;
        schema:domainIncludes  <https://w3id.org/product/WorkControl> .

props:minimumHeadroom
        a                      owl:DatatypeProperty ;
        rdfs:comment           "Minumal geforderte lichte Höhe für diesen Raum."@de-DE , "Headroom required for the activity assigned to this space."@en , "この空間に割り当てられた用途に必要な頭上あき高。"@ja-JP , "Hauteur de passage requise pour l'usage assigné à l'espace"@fr-FR ;
        rdfs:label             "最小頭上あき高"@ja-JP , "Lichte Höhe"@de-DE , "minimumHeadroom"@en , "HauteurPassageMinimale"@fr-FR ;
        rdfs:range             <https://w3id.org/product/LengthMeasure> ;
        schema:domainIncludes  <https://w3id.org/product/Space> , <https://w3id.org/product/cZone> , <https://w3id.org/product/cSpatialZone> .

props:coolingEfficiency
        a                      owl:DatatypeProperty ;
        rdfs:comment           "Coefficient of Performance: Ratio of cooling energy output to energy input under full load operating conditions."@en , "性能係数全負荷運転状態でのエネルギー入力に対する冷却エネルギー出力の割合"@ja-JP ;
        rdfs:label             "coolingEfficiency"@en , "冷却効率"@ja-JP ;
        rdfs:range             <https://w3id.org/product/PositiveRatioMeasure> ;
        schema:domainIncludes  <https://w3id.org/product/UnitaryEquipment%2FAIRCONDITIONINGUNIT> .

props:electricalSystemCategory
        a                      owl:DatatypeProperty ;
        rdfs:comment           "Designates the voltage range of the circuit, according to IEC.  HIGHVOLTAGE indicates >1000V AC or >1500V DV; LOWVOLTAGE indicates 50-1000V AC or 120-1500V DC; EXTRALOWVOLTAGE indicates <50V AC or <120V DC."@en , "IECに準拠した回路の電圧レンジを示す。次の列挙型の値を取る。(HIGHVOLTAGE indicates >1000V AC or >1500V DV; LOWVOLTAGE indicates 50-1000V AC or 120-1500V DC; EXTRALOWVOLTAGE indicates <50V AC or <120V DC.)"@ja-JP , "IEC에 따른 회로의 전압 범위를 나타낸다. 다음 열거 형의 값을 받는다. (HIGHVOLTAGE indicates> 1000V AC or> 1500V DV; LOWVOLTAGE indicates 50-1000V AC or 120-1500V DC; EXTRALOWVOLTAGE indicates <50V AC or <120V DC)"@ko-KR ;
        rdfs:label             "electricalSystemCategory"@en , "電気システムのカテゴリー"@ja-JP , "전기 시스템 카테고리"@ko-KR ;
        schema:domainIncludes  <https://w3id.org/product/DistributionSystem%2FELECTRICAL> .

props:coverageArea  a          owl:DatatypeProperty ;
        rdfs:comment           "The area that the sprinkler is designed to protect."@en , "センサでカバーされている床面積。(通常、センターがセンサの位置にある円として測定される)"@ja-JP , "スプリンクラーの設計保護区画面積。"@ja-JP , "The area that is covered by the sensor (typically measured as a circle whose center is at the location of the sensor)."@en , "센서 커버되는 바닥 면적. (일반적으로 센터 센서의 위치에있는 원형으로 측정되는)"@ko-KR , "センサでカバーされている範囲。(通常、センターがセンサの位置にある円として測定される)"@ja-JP , "센서 커버하는 범위. (일반적으로 센터 센서의 위치에있는 원형으로 측정되는)"@ko-KR , "The floor area that is covered by the sensor (typically measured as a circle whose center is at the location of the sensor)."@en ;
        rdfs:label             "カバー面積"@ja-JP , "측정 범위"@ko-KR , "測定範囲"@ja-JP , "coverageArea"@en ;
        rdfs:range             <https://w3id.org/product/AreaMeasure> ;
        schema:domainIncludes  <https://w3id.org/product/Sensor%2FGASSENSOR> , <https://w3id.org/product/Sensor%2FHEATSENSOR> , <https://w3id.org/product/Sensor%2FSMOKESENSOR> , <https://w3id.org/product/FireSuppressionTerminal%2FSPRINKLER> .

props:strengthClass  a         owl:DatatypeProperty ;
        rdfs:comment           "Classification of the concrete strength in accordance with the concrete design code which is applied in the project."@en , "Klassifikation der Betonfestigkeit gemäß der aktuellen, im Projekt angewandten, Norm."@de-DE ;
        rdfs:label             "strengthClass"@en , "Betonfestigkeitsklasse"@de-DE ;
        rdfs:range             xsd:string ;
        schema:domainIncludes  <https://w3id.org/product/BuildingElement> .

props:actualWork  a            owl:DatatypeProperty ;
        rdfs:comment           "The actual work on behalf of the resource allocation."@en , "資源配分のための実績の作業。"@ja-JP ;
        rdfs:label             "actualWork"@en , "実績作業時間"@ja-JP ;
        schema:domainIncludes  <https://w3id.org/product/ConstructionResource> .

props:compressorCondenserHeatGain
        a                      owl:DatatypeProperty ;
        rdfs:comment           "Heat gain between condenser inlet to compressor outlet."@en ;
        rdfs:label             "compressorCondenserHeatGain"@en ;
        schema:domainIncludes  <https://w3id.org/product/Condenser> .

props:selectorType  a          owl:DatatypeProperty ;
        rdfs:comment           "A list of the available types of selector switch from which that required may be selected."@en , "選択が必要となる、切替えスイッチの一覧リスト。"@ja-JP , "전환스위치 목록"@ko-KR ;
        rdfs:label             "selectorType"@en , "セレクター（スイッチ）タイプ"@ja-JP , "스위치 타입"@ko-KR ;
        schema:domainIncludes  <https://w3id.org/product/SwitchingDevice%2FSELECTORSWITCH> .

props:speakerMounting
        a                      owl:DatatypeProperty ;
        rdfs:comment           "Indicates how the speaker is designed to be mounted."@en , "取付可能な方法を示す。"@ja-JP , "붙일 수있는 방법을 보여준다."@ko-KR ;
        rdfs:label             "speakerMounting"@en , "取付可能方法"@ja-JP , "설치 가능 방법"@ko-KR ;
        schema:domainIncludes  <https://w3id.org/product/AudioVisualAppliance%2FSPEAKER> .

props:wetCoilFraction
        a                      owl:DatatypeProperty ;
        rdfs:comment           "Fraction of coil surface area that is wet (0-1)."@en , "Fraction de la surface de la batterie qui est humide (0 à 1)."@fr-FR ;
        rdfs:label             "wetCoilFraction"@en , "FractionBatterieHumide"@fr-FR ;
        rdfs:range             <https://w3id.org/product/NormalisedRatioMeasure> ;
        schema:domainIncludes  <https://w3id.org/product/Coil> .

props:selfExtinguishing60332_3
        a                      owl:DatatypeProperty ;
        rdfs:comment           "自己消化ケーブル/コアはIEC 60332.3.に準じる。"@ja-JP , "Self Extinguishing cable/core according to IEC 60332.3."@en , "IEC 60332.3.에 규정되어있는 자기 소화 케이블"@ko-KR , "자기 소화 케이블 / 코어는 IEC 60332.3.에 준한다."@ko-KR , "IEC 60332.3.に規定されている自己消火ケーブル。"@ja-JP ;
        rdfs:label             "자기 소화 케이블"@ko-KR , "자동 소화 60332_3"@ko-KR , "自動消火60332_3"@ja-JP , "selfExtinguishing60332_3"@en , "自己消火ケーブル"@ja-JP ;
        rdfs:range             xsd:boolean ;
        schema:domainIncludes  <https://w3id.org/product/CableSegment%2FCABLESEGMENT> , <https://w3id.org/product/CableSegment%2FCORESEGMENT> .

props:breakerUnitIPICurve
        a                      owl:DatatypeProperty ;
        rdfs:comment           "A curve that establishes the let through peak current of a breaker unit when a particular prospective current is applied.  Note that the breaker unit IPI curve is defined within a Cartesian coordinate system and this fact must be asserted within the property set:\n\n(1) Defining value: A list of minimum 2 and maximum 16 numbers providing the currents in [A] for points in the I/Î log/log coordinate space. The curve is drawn as a straight line between two consecutive points.\n(2) Defined value: A list of minimum 2 and maximum 16 numbers providing the let-through peak currents, Î, in [A] for points in the I/Î log/log coordinate space. The curve is drawn as a straight line between two consecutive points."@en , "適用された電流と通過する遮断機のエネルギーを示した曲線\n （1）定義値：ProspectiveCurrent（固有電流）：\n   電流/I2tで示される最小2から最大8のリストで電流[A]を定義します。\n   カーブが連続する2つの点を結ぶ直線として描かれています。\n\n\n （2）定義値：LetThroughEnergy：\n   電流/I2tで示される最小2から最大8のリストで通過エネルギー電流[[A2s]を定義します。\n   カーブが連続する2つの点を結ぶ直線として描かれています。"@ja-JP , "적용된 전류 통과 차단기의 에너지를 나타낸 곡선 (1) 정의 값 : ProspectiveCurrent (고유 전류) :    전류 / I2t에 표시된 최소 2에서 최대 8 개의 목록에서 전류 [A]를 정의합니다.    커브가 연속되는 두 개의 점을 연결하는 직선으로 그려져 있습니다.  (2) 정의 값 : LetThroughEnergy :    전류 / I2t에 표시된 최소 2에서 최대 8 개의 목록에서 통과 에너지 전류 [A2s을 정의합니다.    커브가 연속되는 두 개의 점을 연결하는 직선으로 그려져 있습니다."@ko-KR ;
        rdfs:label             "breakerUnitIPICurve"@en , "遮断機曲線"@ja-JP , "차단기 곡선"@ko-KR ;
        schema:domainIncludes  <https://w3id.org/product/ProtectiveDevice> .

props:threadDiameter  a        owl:DatatypeProperty ;
        rdfs:comment           "Nominal diameter of the thread, if different from the bolt's overall nominal diameter"@en ;
        rdfs:label             "threadDiameter"@en ;
        rdfs:range             <https://w3id.org/product/PositiveLengthMeasure> ;
        schema:domainIncludes  <https://w3id.org/product/MechanicalFastener%2FBOLT> .

props:riserHeight  a           owl:DatatypeProperty ;
        rdfs:comment           "Vertical distance from tread to tread. \nThe riser height is supposed to be equal for all steps of a stair or stair flight."@en , "Hauteur de la contremarche, supposée homogène pour toutes les marches de l'escalier ou de la volée de marches."@fr-FR , "踏面と踏面の垂直方向の距離。この蹴上げ高さ値は、一連の階段において同じ値と仮定する。"@ja-JP , "German-description-4"@de-DE , "踏板之间的垂直高度。\n楼梯或梯段所有梯级的踢板高度应当一致。"@zh-CN ;
        rdfs:label             "Steigung"@de-DE , "riserHeight"@en , "踢板高度"@zh-CN , "HauteurContreMarche"@fr-FR , "蹴上げ高さ"@ja-JP ;
        rdfs:range             <https://w3id.org/product/PositiveLengthMeasure> ;
        schema:domainIncludes  <https://w3id.org/product/Stair> , <https://w3id.org/product/StairFlight> .

props:fireFightingLift
        a                      owl:DatatypeProperty ;
        rdfs:comment           "Indication whether the elevator is designed to serve as a fire fighting lift the case of fire (TRUE) or not (FALSE). A fire fighting lift is used by fire fighters to access the location of fire and to evacuate people."@en , "火災時に消防エレベーターとしての利用を想定して設計されているかどうかを示す。消防エレベーターは火災現場へ消防士を運んだり人を避難させるために使われる。"@ja-JP , "Indique si l'ascenseur est conçu pour servir d'ascenseur pompier (VRAI) ou non (FAUX). Un ascenseur pompier est utilisé par les pompiers pour accéder à l'endroit du feu et évacuer les personnes."@fr-FR , "Angabe, ob der Aufzug als ein Feuerwerksaufzug vorgesehen ist (WAHR) oder nicht (FALSCH). Ein Feuerwehraufzug ist ein besonders abgesicherter Aufzug der der Feuerwehr im Branfall ein Erreichen der Branetage ermöglicht."@de-DE ;
        rdfs:label             "LargeurPassage"@fr-FR , "消防エレベーター"@ja-JP , "fireFightingLift"@en , "Feuerwehraufzug"@de-DE ;
        rdfs:range             xsd:boolean ;
        schema:domainIncludes  <https://w3id.org/product/TransportElement%2FELEVATOR> .

props:netPlannedArea  a        owl:DatatypeProperty ;
        rdfs:comment           "계획된 건물 층 인터넷 공간이 있습니다. 건물 계획시 사용됩니다."@ko-KR , "Geforderte Nettofläche des Geschosses laut Raumprogramm."@de-DE , "計画されたネット面積。建物計画に際に使用。（通常は、柱型等を抜いた面積となる）"@ja-JP , "Surface programmée nette totale de l'étage. Telle que définie lors de la programmation."@fr-FR , "Surface programmée nette totale du bâtiment. Telle que définie lors de la programmation."@fr-FR , "Surface programmée nette totale de la pièce. Telle que définie lors de la programmation."@fr-FR , "Total planned net area for the building storey. Used for programming the building storey."@en , "Total planned net area for the zone. Used for programming the zone."@en , "計画された建物階のネット面積。建物計画の際に使用。"@ja-JP , "Total planned net area for the space. Used for programming the space."@en , "Geforderte Nettofläche des Gebäudes laut Raumprogramm."@de-DE , "Total planned net area for the building  Used for programming the building."@en , "객실의 총 계획 인터넷 공간이 있습니다. 공간 계획시 사용된다."@ko-KR ;
        rdfs:label             "Surface programmée nette"@fr-FR , "Nettofläche nach Raumprogramm"@de-DE , "계획 인터넷 면적"@ko-KR , "netPlannedArea"@en , "計画ネット面積"@ja-JP ;
        rdfs:range             <https://w3id.org/product/AreaMeasure> ;
        schema:domainIncludes  <https://w3id.org/product/Building> , <https://w3id.org/product/Space> , <https://w3id.org/product/Zone> , <https://w3id.org/product/BuildingStorey> .

props:centreOfGravityInX
        a                      owl:DatatypeProperty ;
        rdfs:comment           "Location of the profile's centre of gravity (geometric centroid), measured along xp."@en ;
        rdfs:label             "centreOfGravityInX"@en ;
        rdfs:range             <https://w3id.org/product/LengthMeasure> ;
        schema:domainIncludes  <https://w3id.org/product/ProfileDef> .

props:totalHeatTransferRate
        a                      owl:DatatypeProperty ;
        rdfs:comment           "一次空気流の全熱交換量"@ja-JP , "Puissance thermique totale"@fr-FR , "Total heat transfer rate."@en , "全熱交換量"@ja-JP , "Total heat transfer rate to primary air flow."@en ;
        rdfs:label             "totalHeatTransferRate"@en , "PuissanceThermiqueTotale"@fr-FR , "全熱交換量"@ja-JP ;
        schema:domainIncludes  <https://w3id.org/product/AirToAirHeatRecovery> , <https://w3id.org/product/EvaporativeCooler> .

props:operationalEfficiency
        a                      owl:DatatypeProperty ;
        rdfs:comment           "Operational efficiency: boiler output divided by total energy input (electrical and fuel)."@en , "運転効率：\n全入力エネルギ（電力または燃料）でボイラ出力を割る"@ja-JP , "Efficacité opérationnelle: production de la chaudière divisée par l'apport total d'énergie (électrique et combustible)."@fr-FR ;
        rdfs:label             "operationalEfficiency"@en , "運転効率"@ja-JP , "EfficacitéOpérationnelle"@fr-FR ;
        schema:domainIncludes  <https://w3id.org/product/Boiler> .

props:isAutomaticFlush
        a                      owl:DatatypeProperty ;
        rdfs:comment           "Boolean value that determines if the cistern is flushed automatically either after each use or periodically (TRUE) or whether manual flushing is required (FALSE)."@en , "貯水タンクは、使用後に自動的または定期的に洗浄する場合（TRUE）、手動で洗浄する場合（FALSE）をブーリアン値で指定する。"@ja-JP ;
        rdfs:label             "isAutomaticFlush"@en , "自動フラッシュか"@ja-JP ;
        rdfs:range             xsd:boolean ;
        schema:domainIncludes  <https://w3id.org/product/SanitaryTerminal%2FCISTERN> .

props:vacancyRateInCategoryFuture
        a                      owl:DatatypeProperty ;
        rdfs:comment           "Percentage of vacancy found in the particular category expected in the future."@en , "Taux de vacance attendu dans le futur pour la catégorie."@fr-FR ;
        rdfs:label             "vacancyRateInCategoryFuture"@en , "TauxVacanceFuturParCategorie"@fr-FR ;
        rdfs:range             <https://w3id.org/product/PositiveRatioMeasure> ;
        schema:domainIncludes  <https://w3id.org/product/Building> .

props:maximumPowerOutput
        a                      owl:DatatypeProperty ;
        rdfs:comment           "엔진의 최대 출력 정격"@ko-KR , "엔진의 최대 출력 정격."@ko-KR , "エンジンの最大出力定格。"@ja-JP , "The maximum output power rating of the engine."@en ;
        rdfs:label             "maximumPowerOutput"@en , "최대 출력"@ko-KR , "最大出力"@ja-JP ;
        rdfs:range             <https://w3id.org/product/PowerMeasure> ;
        schema:domainIncludes  <https://w3id.org/product/ElectricGenerator> , <https://w3id.org/product/ElectricMotor> .

props:numberOfPoles  a         owl:DatatypeProperty ;
        rdfs:comment           "The number of live lines that is intemnded to be handled by the device."@en ;
        rdfs:label             "numberOfPoles"@en ;
        rdfs:range             xsd:int ;
        schema:domainIncludes  <https://w3id.org/product/DistributionElement> .

props:switchDisconnectorType
        a                      owl:DatatypeProperty ;
        rdfs:comment           "A list of the available types of switch disconnector from which that required may be selected where:\n\nCenterBreak: A disconnector in which both contacts of each pole are movable and engage at a point substantially midway between their supports. (IEC 441-14-08)\nDividedSupport: A disconnector in which the fixed and moving contacts of each pole are not supported by a common base or frame. (IEC 441-14-06)\nDoubleBreak: A disconnector that opens a circuit at two points. (IEC 441-14-09)\nEarthingSwitch: A disconnector in which the fixed and moving contacts of each pole are not supported by a common base or frame. (IEC 441-14-07)\nIsolator: A disconnector which in the open position satisfies isolating requirements. (IEC 441-14-12)"@en , "以下より選択が必要となる、スイッチ断路機の一覧リスト：\n\nセンターブレイク： 各極の両方の接点は可動式で、実質的に中間付近を保持する断路器。 (IEC 441-14-08)\nDividedSupport： 各極の固定側と移動側接点が、共通のベースまたはフレームではサポートされない断路器。(IEC 441-14-06)\n二点切り断路器： 2点で回路を開く断路器 (IEC 441-14-09)\n接地開閉器 ： 各極の固定側と移動側接点が、共通のベースまたはフレームではサポートされない断路器。(IEC 441-14-07)\n断路器： 解放位置の分離要件を満たす、断路器。(IEC 441-14-12)"@ja-JP , "아래에서 선택이 필요한 스위치 단로 기의 목록 목록 : 센터 브레이크 : 각 국의 두 접점은 가동 식에서 실질적으로 중간 부근을 유지 단로기. (IEC 441-14-08) DividedSupport : 각 국의 고정 측과 ​​이동 측의 접점이 공통 기반 또는 프레임이 지원되지 않는 단로기. (IEC 441-14-06) 두가지 끄고 단로기 : 2 점 회로를 열 단로기 (IEC 441-14-09) 접지 개폐기 : 각 국의 고정 측과 ​​이동 측의 접점이 공통 기반 또는 프레임이 지원되지 않는 단로기. (IEC 441-14-07) 단로기 : 해제 위치 격리 요구 사항을 충족 단로기. (IEC 441-14-12)"@ko-KR ;
        rdfs:label             "switchDisconnectorType"@en , "高圧遮断機タイプ"@ja-JP , "고압차단기 유형"@ko-KR ;
        schema:domainIncludes  <https://w3id.org/product/SwitchingDevice%2FSWITCHDISCONNECTOR> .

props:faultPriorityType
        a                      owl:DatatypeProperty ;
        rdfs:comment           "Identifies the predefined types of priority that can be assigned from which the type may be set where:\n\nHigh: action is required urgently.\nMedium: action can occur within a reasonable period of time.\nLow: action can occur when convenient."@en ;
        rdfs:label             "faultPriorityType"@en ;
        schema:domainIncludes  <https://w3id.org/product/ProjectOrder%2FMAINTENANCEWORKORDER> .

props:diversity  a             owl:DatatypeProperty ;
        rdfs:comment           "The ratio, expressed as a numerical\nvalue or as a percentage, of the\nsimultaneous maximum demand of\na group of electrical appliances or\nconsumers within a specified period,\nto the sum of their individual maximum\ndemands within the same\nperiod. The group of electrical appliances is in this case connected to this circuit. Defenition from IEC 60050, IEV 691-10-04 \nNOTE1: It is often not desirable to size each conductor in a distribution system to support the total connected load at that point in the network. Diversity is applied on the basis of the anticipated loadings that are likely to result from all loads not being connected at the same time.\nNOTE2: Diversity is applied to final circuits only, not to sub-main circuits supplying other DBs."@en , "ある期間中同じ回路にある複数電気設備の同時最大負荷と各設備の合計負荷の比率。"@ja-JP , "일정 기간 동안 동일 회로에 여러 전기 설비의 동시 최대 부하와 각 설비의 총 부하의 비율."@ko-KR ;
        rdfs:label             "diversity"@en , "負荷率"@ja-JP , "부하율"@ko-KR ;
        rdfs:range             <https://w3id.org/product/PositiveRatioMeasure> ;
        schema:domainIncludes  <https://w3id.org/product/DistributionSystem%2FELECTRICAL> .

props:stemTopWidth  a          owl:DatatypeProperty ;
        rdfs:comment           "Stem top width of the profile."@en ;
        rdfs:label             "stemTopWidth"@en ;
        rdfs:range             <https://w3id.org/product/PositiveLengthMeasure> ;
        schema:domainIncludes  <https://w3id.org/product/ArbitraryClosedProfileDef> .

props:isAisle  a               owl:DatatypeProperty ;
        rdfs:comment           "Indicates that this parking zone is for accessing the parking units, i.e. an aisle (TRUE) and not a parking unit itself (FALSE)"@en , "Indique si cette zone du parking, comme une allée, est réservée à l'accès (VRAI) ou non (FAUX)."@fr-FR , "駐車場の通路部分(TRUE)か駐車部部分(FALSE)かを示すフラグ。"@ja-JP ;
        rdfs:label             "isAisle"@en , "NombreUnites"@fr-FR , "通路か駐車スペースの判別"@ja-JP ;
        rdfs:range             xsd:boolean ;
        schema:domainIncludes  <https://w3id.org/product/Space%2FPARKING> .

props:concealedFlooring
        a                      owl:DatatypeProperty ;
        rdfs:comment           "この部屋（空間）が隠蔽された床空間を持つように設計されているかどうかを示すブーリアン値。隠蔽された床空間とは、上げ床の下の空間。"@ja-JP , "Indication whether this space is designed to have a concealed flooring space (TRUE) or not (FALSE). A concealed flooring space is normally meant to be the space beneath a raised floor."@en , "Indique si la pièce comprend un faux plancher (VRAI) ou non (FAUX)"@fr-FR , "Angabe, ob dieser Raum mit einem aufgeständerten Fußboden ausgestattet ist (JA), oder nicht (NEIN)."@de-DE ;
        rdfs:label             "FauxPlancher"@fr-FR , "隠蔽床"@ja-JP , "concealedFlooring"@en , "Installationsboden"@de-DE ;
        rdfs:range             xsd:boolean ;
        schema:domainIncludes  <https://w3id.org/product/Space> .

props:warrantyStartDate
        a                      owl:DatatypeProperty ;
        rdfs:comment           "The date on which the warranty commences."@en ;
        rdfs:label             "warrantyStartDate"@en ;
        rdfs:range             xsd:date ;
        schema:domainIncludes  <https://w3id.org/product/Element> .

props:hasExteriorInsulation
        a                      owl:DatatypeProperty ;
        rdfs:comment           "TRUE if the silencer has exterior insulation. FALSE if it does not."@en , "サイレンサに外部保温があるときTRUE"@ja-JP ;
        rdfs:label             "hasExteriorInsulation"@en , "外部保温"@ja-JP ;
        rdfs:range             xsd:boolean ;
        schema:domainIncludes  <https://w3id.org/product/DuctSilencer> .

props:waterIsPotable  a        owl:DatatypeProperty ;
        rdfs:comment           "Indication of whether the water flow from the hydrant is potable (set TRUE) or non potable (set FALSE)."@en , "消火栓の水が飲用かどうかの表示（飲用：TRUEを設定、飲用以外：FALSEを設定）。"@ja-JP ;
        rdfs:label             "waterIsPotable"@en , "飲用水かどうか"@ja-JP ;
        rdfs:range             xsd:boolean ;
        schema:domainIncludes  <https://w3id.org/product/FireSuppressionTerminal%2FFIREHYDRANT> .

props:lowestSeatingHeight
        a                      owl:DatatypeProperty ;
        rdfs:comment           "The value of seating height of low level if the chair height is adjustable."@en ;
        rdfs:label             "lowestSeatingHeight"@en ;
        rdfs:range             <https://w3id.org/product/PositiveLengthMeasure> ;
        schema:domainIncludes  <https://w3id.org/product/Furniture%2FCHAIR> .

props:lampMaintenanceFactor
        a                      owl:DatatypeProperty ;
        rdfs:comment           "Non recoverable losses of luminous flux of a lamp due to lamp depreciation; i.e. the decreasing of light output of a luminaire due to aging and dirt."@en , "回復不可能な光量減少が原因の光源自体の光束の低下、たとえば照明器具の老朽化や汚れによる光量の減少。"@ja-JP , "복구할 수없는 광량 감소가 원인 광원 자체의 광속 저하, 예를 들어 조명기구의 노후화 및 오염에 의한 광량 감소."@ko-KR ;
        rdfs:label             "lampMaintenanceFactor"@en , "保守率"@ja-JP , "보수  비율"@ko-KR ;
        rdfs:range             xsd:decimal ;
        schema:domainIncludes  <https://w3id.org/product/Lamp> .

props:internalShadingCoefficient
        a                      owl:DatatypeProperty ;
        rdfs:comment           "Coefficient de transmission du rayonnement de la protection solaire intérieure, symbole \"Valeur-b\". Valeur adimensionnelle."@fr-FR , "German-description-2"@de-DE , "Radiation transmission coefficient of the inside shading device, symbol \"b-value\". It is a value without unit."@en , "内部遮阳设备的辐射透射系数，符号为b值。无单位。"@zh-CN ;
        rdfs:label             "internalShadingCoefficient"@en , "内部遮阳系数"@zh-CN , "CoefficientMasqueInterieur"@fr-FR , "German-name-2"@de-DE ;
        rdfs:range             <https://w3id.org/product/PositiveRatioMeasure> ;
        schema:domainIncludes  <https://w3id.org/product/cWindow> , <https://w3id.org/product/Door> .

props:supplyWaterTemperatureCooling
        a                      owl:DatatypeProperty ;
        rdfs:comment           "Supply water temperature in cooling mode."@en ;
        rdfs:label             "supplyWaterTemperatureCooling"@en ;
        schema:domainIncludes  <https://w3id.org/product/CooledBeam> .

props:heatTransferSurfaceArea
        a                      owl:DatatypeProperty ;
        rdfs:comment           "Total heat transfer area of the vessel."@en , "容器の伝熱部面積の合計"@ja-JP , "Surface totale d'échange de chaleur du foyer"@fr-FR ;
        rdfs:label             "heatTransferSurfaceArea"@en , "伝熱面積"@ja-JP , "SurfaceEchangeChaleur"@fr-FR ;
        rdfs:range             <https://w3id.org/product/AreaMeasure> ;
        schema:domainIncludes  <https://w3id.org/product/Boiler> .

props:beamHeatingCapacity
        a                      owl:DatatypeProperty ;
        rdfs:comment           "Heating capacity of beam. This excludes heating capacity of supply air."@en ;
        rdfs:label             "beamHeatingCapacity"@en ;
        schema:domainIncludes  <https://w3id.org/product/CooledBeam> .

props:breakerUnitFuseMeltingCurve
        a                      owl:DatatypeProperty ;
        rdfs:comment           "A curve that establishes the energy required to melt the fuse of a breaker unit when a particular prospective melting current is applied.  Note that the breaker unit fuse melting curve is defined within a Cartesian coordinate system and this fact must be:\n\n(1) Defining value: ProspectiveCurrentMelting :A list of minimum 2 and maximum 8 numbers providing the currents in [A] for points in the\ncurrent/melting_energy log/log coordinate space. The curve is drawn as a straight line between two consecutive points.\n(2) Defined value: MeltingEnergy: A list of minimum 2 and maximum 8 numbers providing the energy whereby the fuse is starting to melt, I2t, in [A2s] for points in the current/melting_energy log/log coordinate space. The curve is drawn as a straight line between two consecutive points."@en , "想定外の電流が流れた時に遮断機のフューズを溶かすために必要なエネルギーを表す曲線。\n  想定外の電流が流れた時に遮断機のフューズを溶かすために必要なエネルギーを表す曲線。\n\n  （1）定義値：融解電流：電流/ 融解エネルギーで示される最小2から最大8のリストで電流[A]を定義します。\n   カーブが連続する2つの点を結ぶ直線として描かれています。\n  （2）定義値：融解エネルギー：/電流/融解エネルギーの位置[A2s]で示される2～16の想定されるフューズが溶解始める電流[A2s]を定義します。カーブが連続する2つの点を結ぶ直線として描かれています。"@ja-JP , "예상치 못한 전류가 흐를 때 차단기의 퓨즈를 녹이는 데 필요한 에너지를 나타내는 곡선.   예상외의 전류가 흘렀을 때에 차단기의 퓨즈를 녹이는 데 필요한 에너지를 나타내는 곡선.   (1) 정의 값 : 융해 전류 : 전류 / 융해 에너지에 표시된 최소 2에서 최대 8 개의 목록에서 전류 [A]를 정의합니다.    커브가 연속되는 두 개의 점을 연결하는 직선으로 그려져 있습니다.   (2) 정의 값 : 융해 에너지 :/ 전류 / 융해 에너지의 위치 [A2s에서 나타나는 2 ~ 16 예상되는 퓨즈가 용해 시작 전류 [A2s을 정의합니다. 커브가 연속되는 두 개의 점을 연결하는 직선으로 그려져 있습니다."@ko-KR ;
        rdfs:label             "breakerUnitFuseMeltingCurve"@en , "フューズ遮断機融解曲線"@ja-JP , "퓨즈 차단기 융해 곡선"@ko-KR ;
        schema:domainIncludes  <https://w3id.org/product/ProtectiveDevice> .

props:heatingDesignAirflow
        a                      owl:DatatypeProperty ;
        rdfs:comment           "The air flowrate required during the peak heating conditions, but could also be determined by minimum ventilation requirement or minimum air change requirements."@en ;
        rdfs:label             "heatingDesignAirflow"@en ;
        rdfs:range             <https://w3id.org/product/VolumetricFlowRateMeasure> ;
        schema:domainIncludes  <https://w3id.org/product/Space> .

props:shaftPower  a            owl:DatatypeProperty ;
        rdfs:comment           "The actual shaft power input to the compressor."@en , "La puissance mécanique appliquée au niveau de l'arbre du compresseur."@fr-FR ;
        rdfs:label             "shaftPower"@en , "PuissanceArbre"@fr-FR ;
        schema:domainIncludes  <https://w3id.org/product/Compressor> .

props:storageType  a           owl:DatatypeProperty ;
        rdfs:comment           "Defines the general material category intended to be stored."@en , "一般的な材料種別が格納される"@ja-JP ;
        rdfs:label             "storageType"@en , "貯蔵タイプ"@ja-JP ;
        schema:domainIncludes  <https://w3id.org/product/Tank> .

props:wetBulbTemperature
        a                      owl:DatatypeProperty ;
        rdfs:comment           "Wet bulb temperature of the air."@en , "Wet bulb temperature of the fluid; only applicable if the fluid is air."@en ;
        rdfs:label             "wetBulbTemperature"@en ;
        schema:domainIncludes  <https://w3id.org/product/DistributionPort%2FAIRCONDITIONING> .

props:momentOfInertiaYZ
        a                      owl:DatatypeProperty ;
        rdfs:comment           "Moment of inertia about ys and zs (product moment of area). For example measured in mm4."@en ;
        rdfs:label             "momentOfInertiaYZ"@en ;
        rdfs:range             <https://w3id.org/product/MomentOfInertiaMeasure> ;
        schema:domainIncludes  <https://w3id.org/product/ProfileDef> .

props:nominalCountedEfficiency
        a                      owl:DatatypeProperty ;
        rdfs:comment           "Nominal filter efficiency based the particle count concentration before and after the filter against particles with a certain size distribution."@en ;
        rdfs:label             "nominalCountedEfficiency"@en ;
        rdfs:range             xsd:decimal ;
        schema:domainIncludes  <https://w3id.org/product/Filter%2FAIRPARTICLEFILTER> .

props:cornerFixingPlateThickness
        a                      owl:DatatypeProperty ;
        rdfs:comment           "The thickness of the L-shaped corner plate."@en , "L型コーナープレートの板厚。"@ja-JP , "L 형 코너 플레이트의 두께"@ko-KR ;
        rdfs:label             "cornerFixingPlateThickness"@en , "板厚"@ja-JP , "두께"@ko-KR ;
        rdfs:range             <https://w3id.org/product/PositiveLengthMeasure> ;
        schema:domainIncludes  <https://w3id.org/product/DiscreteAccessory%2FCorner%20fixing%20plate> .

props:ventilationAirFlowrate
        a                      owl:DatatypeProperty ;
        rdfs:comment           "Ventilation outside air requirement for the space."@en , "必要外気量。"@ja-JP , "필요 외기 량."@ko-KR ;
        rdfs:label             "ventilationAirFlowrate"@en , "外気量"@ja-JP , "외기량"@ko-KR ;
        rdfs:range             <https://w3id.org/product/VolumetricFlowRateMeasure> ;
        schema:domainIncludes  <https://w3id.org/product/Space> .

props:actuationType  a         owl:DatatypeProperty ;
        rdfs:comment           "Enumeration that identifies the different types of dampers."@en ;
        rdfs:label             "actuationType"@en ;
        schema:domainIncludes  <https://w3id.org/product/Damper%2FFIRESMOKEDAMPER> , <https://w3id.org/product/Damper%2FFIREDAMPER> .

props:maintenanceFactor
        a                      owl:DatatypeProperty ;
        rdfs:comment           "The arithmetical allowance made for depreciation of lamps and reflective equipment from their initial values due to dirt, fumes, or age."@en , "汚れ、煙、年数による初期からのランプや反射装置の低減許容計算。"@ja-JP , "먼지, 연기, 연수의 초기부터 램프와 반사 장치의 저감 허용 계산."@ko-KR ;
        rdfs:label             "maintenanceFactor"@en , "保守率"@ja-JP , "보수 비율"@ko-KR ;
        rdfs:range             xsd:decimal ;
        schema:domainIncludes  <https://w3id.org/product/LightFixture> .

props:integratedLightingType
        a                      owl:DatatypeProperty ;
        rdfs:comment           "Integrated lighting in cooled beam."@en ;
        rdfs:label             "integratedLightingType"@en ;
        schema:domainIncludes  <https://w3id.org/product/CooledBeam> .

props:primaryVoltage  a        owl:DatatypeProperty ;
        rdfs:comment           "The voltage that is going to be transformed and that runs into the transformer on the primary side."@en , "変圧器の1次側に伝送される電圧。"@ja-JP , "변압기 1 차 측에 전송되는 전압."@ko-KR ;
        rdfs:label             "primaryVoltage"@en , "第1電圧"@ja-JP , "제 1 전압"@ko-KR ;
        rdfs:range             <https://w3id.org/product/ElectricVoltageMeasure> ;
        schema:domainIncludes  <https://w3id.org/product/Transformer> .

props:diagonalTrussCrossBarDiameter
        a                      owl:DatatypeProperty ;
        rdfs:comment           "The nominal diameter of the diagonal cross-bars."@en , "斜めクロスバーの公称直径。"@ja-JP , "대각선 크로스바 공칭 지름"@ko-KR ;
        rdfs:label             "diagonalTrussCrossBarDiameter"@en , "クロスバー径"@ja-JP , "크로스바 지름"@ko-KR ;
        rdfs:range             <https://w3id.org/product/PositiveLengthMeasure> ;
        schema:domainIncludes  <https://w3id.org/product/DiscreteAccessory%2FDiagonal%20truss%20connector> .

props:moistureDiffusivity
        a                      owl:DatatypeProperty ;
        rdfs:comment           "Moisture diffusivity is a transport property that is frequently used in the hygrothermal analysis of building envelope components."@en ;
        rdfs:label             "moistureDiffusivity"@en ;
        rdfs:range             <https://w3id.org/product/MoistureDiffusivityMeasure> ;
        schema:domainIncludes  <https://w3id.org/product/Material> .

props:range  a                 owl:DatatypeProperty ;
        rdfs:comment           "The physical range of values."@en , "The physical range of values supported by the device."@en ;
        rdfs:label             "range"@en ;
        schema:domainIncludes  <https://w3id.org/product/Controller%2FPROPORTIONAL> , <https://w3id.org/product/Controller%2FMULTIPOSITION> , <https://w3id.org/product/Controller%2FFLOATING> .

props:videoCaptionMode
        a                      owl:DatatypeProperty ;
        rdfs:comment           "クローズドキャプションモードを示す。(字幕機能）"@ja-JP , "자막 모드를 나타낸다.(자막 기능)"@ko-KR , "Indicates closed captioning modes."@en , "자막 모드를 나타낸다. (자막 기능)"@ko-KR , "Indicates video closed captioning modes."@en ;
        rdfs:label             "비디오 캡쳐모드"@ko-KR , "ビデオキャプションモード"@ja-JP , "videoCaptionMode"@en , "비디오 캡션 모드"@ko-KR ;
        schema:domainIncludes  <https://w3id.org/product/AudioVisualAppliance%2FPROJECTOR> , <https://w3id.org/product/AudioVisualAppliance%2FDISPLAY> .

props:upperTime1  a            owl:DatatypeProperty ;
        rdfs:comment           "The time in [s], indicating that tripping times of the upper time/current curve lower than UpperTime1 is determined by the I2t part of the L-function."@en , "[s]の時間,上時間より低い上部の時間/特性曲線のトリップ時間は、L-関数ののI2t部分によって決定される。"@ja-JP , "[s]의 시간에 시간 더 낮은 위 시간 / 특성 곡선의 트립 시간은 L-함수의 I2t 부분에 의해 결정된다"@ko-KR ;
        rdfs:label             "upperTime1"@en , "上時間1"@ja-JP , "상시간1"@ko-KR ;
        rdfs:range             <https://w3id.org/product/TimeMeasure> ;
        schema:domainIncludes  <https://w3id.org/product/ProtectiveDeviceTrippingUnit> .

props:reinforcementVolumeRatio
        a                      owl:DatatypeProperty ;
        rdfs:comment           "The required ratio of the effective mass of the reinforcement to the effective volume of the concrete of a reinforced concrete structural element."@en , "Das geforderte Verhältnis der effektiven Masse der Bewehrung im Verhältnis zur effektiven Masse des Betons für dieses Element."@de-DE ;
        rdfs:label             "reinforcementVolumeRatio"@en , "Bewehrungsgrad Volumen"@de-DE ;
        rdfs:range             <https://w3id.org/product/MassDensityMeasure> ;
        schema:domainIncludes  <https://w3id.org/product/BuildingElement> .

props:instantaneousTrippingTime
        a                      owl:DatatypeProperty ;
        rdfs:comment           "Instantaneous tripping time. The set value of the instantaneous tripping time if adjustable."@en ;
        rdfs:label             "instantaneousTrippingTime"@en ;
        rdfs:range             <https://w3id.org/product/TimeMeasure> ;
        schema:domainIncludes  <https://w3id.org/product/ProtectiveDevice> .

props:isPermanentID  a         owl:DatatypeProperty ;
        rdfs:comment           "Indique si l'identifiant est permanent (VRAI) ou non (FAUX)"@fr-FR , "Indicates whether the identity assigned to a building is permanent (= TRUE) or temporary (=FALSE)."@en , "부지 ID가 영구적인 것인지 여부를 나타내는  값입니다."@ko-KR , "建物IDが恒久的なIDかどうかのブーリアン値。"@ja-JP , "敷地IDが恒久的なものかどうかを示すブーリアン値。"@ja-JP , "Indique si l'identifiant attribuée au bâtiment est permanent (=VRAI) ou temporaire (=FAUX)."@fr-FR , "Angabe, on das angegebene Gebäudekennzeichen permanent ist (TRUE), oder eine temporäre Antragsnummer (FALSE)."@de-DE , "Indicates whether the identity assigned to a land parcel is permanent (= TRUE) or temporary (=FALSE)."@en , "건물 ID가 영구적인 ID 여부값"@ko-KR ;
        rdfs:label             "恒久ID区分"@ja-JP , "IdPermanent"@fr-FR , "Gebäudekennzeichen permanent"@de-DE , "영구 ID 구분"@ko-KR , "永久ID区分"@ja-JP , "isPermanentID"@en ;
        rdfs:range             xsd:boolean ;
        schema:domainIncludes  <https://w3id.org/product/Building> , <https://w3id.org/product/Site> .

props:massPerLength  a         owl:DatatypeProperty ;
        rdfs:comment           "Mass per length, i.e. mass of a beam with a unit length of extrusion. For example measured in kg/m."@en ;
        rdfs:label             "massPerLength"@en ;
        rdfs:range             <https://w3id.org/product/MassPerLengthMeasure> ;
        schema:domainIncludes  <https://w3id.org/product/ProfileDef> .

props:shortInsideEndLowerBarPitch
        a                      owl:DatatypeProperty ;
        rdfs:comment           "The pitch length of the short inside end lower bar."@en , "短辺方向・柱間帯・下端端部の鉄筋間隔。"@ja-JP ;
        rdfs:label             "shortInsideEndLowerBarPitch"@en , "短辺・柱列帯・下端端部ピッチ"@ja-JP ;
        rdfs:range             <https://w3id.org/product/PositiveLengthMeasure> ;
        schema:domainIncludes  <https://w3id.org/product/Slab> .

props:youngModulus  a          owl:DatatypeProperty ;
        rdfs:comment           "A measure of the Young's modulus of elasticity of the material."@en ;
        rdfs:label             "youngModulus"@en ;
        rdfs:range             <https://w3id.org/product/ModulusOfElasticityMeasure> ;
        schema:domainIncludes  <https://w3id.org/product/Material> .

props:coilPosition  a          owl:DatatypeProperty ;
        rdfs:comment           "Defines the relationship between a fan and a coil.\n\nDrawThrough: Fan located downstream of the coil.\nBlowThrough: Fan located upstream of the coil."@en , "Fanとコイル間の関係定義\nDwawThrough:ファンはコイルの下流に位置\nBlowThrough:ファンはコイルの上流に位置"@ja-JP ;
        rdfs:label             "coilPosition"@en , "コイル位置"@ja-JP ;
        schema:domainIncludes  <https://w3id.org/product/Fan> .

props:fixingSocketThreadDiameter
        a                      owl:DatatypeProperty ;
        rdfs:comment           "The nominal diameter of the thread."@en , "線の公称直径。"@ja-JP , "고정 소켓의 전체 길이"@ko-KR ;
        rdfs:label             "fixingSocketThreadDiameter"@en , "公称径"@ja-JP , "공칭 지름"@ko-KR ;
        rdfs:range             <https://w3id.org/product/PositiveLengthMeasure> ;
        schema:domainIncludes  <https://w3id.org/product/DiscreteAccessory%2FFixing%20socket> .

props:signalOffset  a          owl:DatatypeProperty ;
        rdfs:comment           "Offset constant added to modfied signal."@en , "오프셋 상수 변경 신호에 추가됨"@ko-KR ;
        rdfs:label             "signalOffset"@en , "옵셋"@ko-KR ;
        rdfs:range             xsd:decimal ;
        schema:domainIncludes  <https://w3id.org/product/Controller%2FFLOATING> .

props:nominalPartLoadRatio
        a                      owl:DatatypeProperty ;
        rdfs:comment           "Allowable part load ratio range."@en , "許容部分負荷比範囲"@ja-JP , "Plage de charge partielle admissible"@fr-FR ;
        rdfs:label             "nominalPartLoadRatio"@en , "設計部分負荷比率"@ja-JP , "PlageNominaleChargePartielle"@fr-FR ;
        schema:domainIncludes  <https://w3id.org/product/Boiler> .

props:totalEffectivenessTable
        a                      owl:DatatypeProperty ;
        rdfs:comment           "Total heat transfer effectiveness curve as a function of the primary and secondary air flow rate."@en , "一次と二次空気量の関数としての全熱交換効率曲線"@ja-JP , "Courbe d'efficacité d'échange thermique total en tant que fonction du débit d'air au primaire et débit d'air au secondaire"@fr-FR ;
        rdfs:label             "totalEffectivenessTable"@en , "全熱効率テーブル"@ja-JP , "DiagrammeEfficacitéTotale"@fr-FR ;
        schema:domainIncludes  <https://w3id.org/product/AirToAirHeatRecovery> .

props:shearCentreZ  a          owl:DatatypeProperty ;
        rdfs:comment           "Location of the profile's shear centre, measured along zs."@en ;
        rdfs:label             "shearCentreZ"@en ;
        rdfs:range             <https://w3id.org/product/LengthMeasure> ;
        schema:domainIncludes  <https://w3id.org/product/ProfileDef> .

props:innerDiameter  a         owl:DatatypeProperty ;
        rdfs:comment           "配管の実内径(リストの複数の数字の解釈については呼び径参照)"@ja-JP , "The actual inner diameter of the pipe."@en , "配管の実内径。"@ja-JP ;
        rdfs:label             "innerDiameter"@en , "内径"@ja-JP ;
        rdfs:range             <https://w3id.org/product/PositiveLengthMeasure> ;
        schema:domainIncludes  <https://w3id.org/product/PipeSegment> , <https://w3id.org/product/DistributionPort%2FCHEMICAL> .

props:frameDepth  a            owl:DatatypeProperty ;
        rdfs:comment           "The length (or depth) of the damper frame."@en ;
        rdfs:label             "frameDepth"@en ;
        rdfs:range             <https://w3id.org/product/PositiveLengthMeasure> ;
        schema:domainIncludes  <https://w3id.org/product/Damper> .

props:loadSafetyFactor
        a                      owl:DatatypeProperty ;
        rdfs:comment           "空調負荷計算用の安全率（割増係数）。"@ja-JP , "공조 부하 계산을위한 안전율 (할증 계수)"@ko-KR , "Load safety factor."@en , "공조 부하 계산을위한 안전율 (할증 계수)."@ko-KR ;
        rdfs:label             "부하의 안전율"@ko-KR , "負荷の安全率"@ja-JP , "loadSafetyFactor"@en ;
        rdfs:range             <https://w3id.org/product/PositiveRatioMeasure> ;
        schema:domainIncludes  <https://w3id.org/product/Space> , <https://w3id.org/product/SpatialElement> , <https://w3id.org/product/Zone> , <https://w3id.org/product/SpatialZone> .

props:coverWidth  a            owl:DatatypeProperty ;
        rdfs:comment           "The length measured along the x-axis in the local coordinate system of the cover of the oil interceptor."@en , "局所座標系のY軸で測定された溝防臭弁カバーの長さ。"@ja-JP , "The length measured along the y-axis in the local coordinate system of the cover of the gully trap."@en , "局所座標系のY軸で測定された防臭弁カバーの長さ。"@ja-JP , "The length measured along the y-axis in the local coordinate system of the cover of the  trap."@en , "The length measured along the y-axis in the local coordinate system of the cover of the  drain."@en , "The length measured along the y-axis in the local coordinate system of the cover of the  waste."@en , "局所座標系のY軸で測定された配管カバーの長さ。"@ja-JP ;
        rdfs:label             "カバーの幅"@ja-JP , "coverWidth"@en , "カバー幅"@ja-JP ;
        rdfs:range             <https://w3id.org/product/PositiveLengthMeasure> ;
        schema:domainIncludes  <https://w3id.org/product/WasteTerminal%2FFLOORWASTE> , <https://w3id.org/product/WasteTerminal%2FGULLYTRAP> , <https://w3id.org/product/WasteTerminal%2FROOFDRAIN> , <https://w3id.org/product/WasteTerminal%2FFLOORTRAP> , <https://w3id.org/product/Interceptor> , <https://w3id.org/product/WasteTerminal%2FGULLYSUMP> .

props:yDirectionTieHoopBarPitch
        a                      owl:DatatypeProperty ;
        rdfs:comment           "The Y direction pitch length of the tie hoop."@en , "Y方向巾止筋の間隔。"@ja-JP ;
        rdfs:label             "yDirectionTieHoopBarPitch"@en , "Y方向巾止め筋間隔"@ja-JP ;
        rdfs:range             <https://w3id.org/product/PositiveLengthMeasure> ;
        schema:domainIncludes  <https://w3id.org/product/Column> .

props:numberOfRiser  a         owl:DatatypeProperty ;
        rdfs:comment           "该楼梯所包含的踢板总数。"@zh-CN , "该梯段所包含的踢板总数。"@zh-CN , "Nombre total de contremarches de l'escalier"@fr-FR , "German-description-2"@de-DE , "Total number of the risers included in the stair."@en , "階段の蹴上げ数。"@ja-JP , "Total number of the risers included in the stair flight."@en ;
        rdfs:label             "蹴上げ数"@ja-JP , "numberOfRiser"@en , "Anzahl der Steigungen"@de-DE , "踢板数"@zh-CN , "NombreContreMarches"@fr-FR ;
        rdfs:range             <https://w3id.org/product/CountMeasure> ;
        schema:domainIncludes  <https://w3id.org/product/Stair> , <https://w3id.org/product/StairFlight> .

props:e  a                     owl:DatatypeProperty ;
        rdfs:comment           "Measure e according to ISO 2553"@en ;
        rdfs:label             "e"@en ;
        rdfs:range             <https://w3id.org/product/PositiveLengthMeasure> ;
        schema:domainIncludes  <https://w3id.org/product/Fastener%2FWELD> .

props:temperatureClassification
        a                      owl:DatatypeProperty ;
        rdfs:comment           "Enumeration defining the temperature classification of the space heater surface temperature.\nlow temperature - surface temperature is relatively low, usually heated by hot water or electricity.\nhigh temperature - surface temperature is relatively high, usually heated by gas or steam."@en , "暖房用ヒーター表面温度の温度分類を定義。低温タイプ-お湯またｈ電気によるものの表面温度は相対的に低い。高温タイプ-ガスまたは蒸気によって熱するタイプの表面温度は比較的高い。"@ja-JP ;
        rdfs:label             "temperatureClassification"@en , "温度分類"@ja-JP ;
        schema:domainIncludes  <https://w3id.org/product/SpaceHeater> .

props:spacing  a               owl:DatatypeProperty ;
        rdfs:comment           "Distance between fins on a tube in the tube bundle."@en , "チューブ束内のフィン間の距離"@ja-JP ;
        rdfs:label             "spacing"@en , "間隔"@ja-JP ;
        rdfs:range             <https://w3id.org/product/PositiveLengthMeasure> ;
        schema:domainIncludes  <https://w3id.org/product/TubeBundle%2FFINNED> .

props:netPositiveSuctionHead
        a                      owl:DatatypeProperty ;
        rdfs:comment           "Minimum liquid pressure at the pump inlet to prevent cavitation."@en , "キャビテーションを防ぐポンプ入口の最小限の流体圧力"@ja-JP ;
        rdfs:label             "netPositiveSuctionHead"@en , "正味吸入側水頭"@ja-JP ;
        rdfs:range             <https://w3id.org/product/PressureMeasure> ;
        schema:domainIncludes  <https://w3id.org/product/Pump> .

props:realPower  a             owl:DatatypeProperty ;
        rdfs:comment           "Real power."@en , "有効電力。"@ja-JP ;
        rdfs:label             "realPower"@en , "有効電力"@ja-JP ;
        schema:domainIncludes  <https://w3id.org/product/DistributionPort%2FELECTRICAL> .

props:colorRenderingIndex
        a                      owl:DatatypeProperty ;
        rdfs:comment           "The CRI indicates how well a light source renders eight standard colors compared to perfect reference lamp with the same color temperature. The CRI scale ranges from 1 to 100, with 100 representing perfect rendering properties."@en , "同じ色温度の基準光源で、規定された8色の試験色票での光源による色彩の再表現を比較する。CRIの評価スケールは1～100で、基準光源の場合を100とする。"@ja-JP , "같은 색온도의 기준 광원으로 규정된 8 가지 시험 색 표의 광원에 의한 색채를 다시 표현을 비교한다. CRI의 평가 척도는 1에서 100에서 기준 광원의 경우 100로한다."@ko-KR ;
        rdfs:label             "colorRenderingIndex"@en , "演色評価数"@ja-JP , "연색 평가수"@ko-KR ;
        rdfs:range             xsd:int ;
        schema:domainIncludes  <https://w3id.org/product/Lamp> .

props:yDirectionTieHoopCount
        a                      owl:DatatypeProperty ;
        rdfs:comment           "The number of bars with Y direction tie hoop bars."@en , "Y方向巾止筋の本数。"@ja-JP ;
        rdfs:label             "yDirectionTieHoopCount"@en , "Y方向巾止め筋本数"@ja-JP ;
        rdfs:range             xsd:int ;
        schema:domainIncludes  <https://w3id.org/product/Column> .

props:numberOfSources
        a                      owl:DatatypeProperty ;
        rdfs:comment           "Number of sources ."@en , "電球数。"@ja-JP , "전구수"@ko-KR ;
        rdfs:label             "numberOfSources"@en , "電球数"@ja-JP , "전구수"@ko-KR ;
        rdfs:range             xsd:int ;
        schema:domainIncludes  <https://w3id.org/product/LightFixture> .

props:condition  a             owl:DatatypeProperty ;
        rdfs:comment           "Table mapping alarm condition identifiers to descriptive labels, which may be used for interpreting Pset_AlarmPHistory.Condition."@en , "Pset_AlarmPHistory.Conditionで使用される、警報条件の識別子とラベル情報のマッピングを行う。"@ja-JP , "Indicates alarm condition over time.  The range of possible values and their meanings is defined by Pset_AlarmTypeCommon.Condition.  An empty value indicates no present alarm condition."@en ;
        rdfs:label             "条件"@ja-JP , "condition"@en ;
        schema:domainIncludes  <https://w3id.org/product/Alarm> .

props:testPressure  a          owl:DatatypeProperty ;
        rdfs:comment           "The maximum pressure to which the valve has been subjected under test."@en , "試験の時、掛けられる最高圧力"@ja-JP ;
        rdfs:label             "testPressure"@en , "試験圧力"@ja-JP ;
        rdfs:range             <https://w3id.org/product/PressureMeasure> ;
        schema:domainIncludes  <https://w3id.org/product/Valve> .

props:isolatorCompressibility
        a                      owl:DatatypeProperty ;
        rdfs:comment           "The compressibility of the vibration isolator."@en , "振動絶縁材の圧縮率の圧縮率"@ja-JP ;
        rdfs:label             "isolatorCompressibility"@en , "振動絶縁材の圧縮率"@ja-JP ;
        rdfs:range             <https://w3id.org/product/RatioMeasure> ;
        schema:domainIncludes  <https://w3id.org/product/VibrationIsolator> .

props:frameThickness  a        owl:DatatypeProperty ;
        rdfs:comment           "The thickness of the damper frame material."@en ;
        rdfs:label             "frameThickness"@en ;
        rdfs:range             <https://w3id.org/product/PositiveLengthMeasure> ;
        schema:domainIncludes  <https://w3id.org/product/Damper> .

props:voltageLevel  a          owl:DatatypeProperty ;
        rdfs:comment           "The voltage levels of the protective device for which the data of the instance is valid. More than one value may be selected in the enumeration."@en , "The voltage level of the protective device for which the data of the instance is valid. More than one value may be selected in the enumeration."@en , "전압레벨을 선택합니다."@ko-KR , "保護装置が作動する電圧レベルを選択。\n[U230,U400,U525,U690,U1000,その他,不明,無]"@ja-JP , "The voltage levels of the fuse for which the data of the instance is valid. More than one value may be selected in the enumeration."@en , "The voltage levels for which the data of the instance is valid. More than one value may be selected in the enumeration."@en , "전압 레벨을 선택합니다."@ko-KR , "보호 장치가 작동 전압 레벨을 선택합니다. [U230, U400, U525, U690, U1000, 기타 알 수 없음, 무"@ko-KR , "電圧レベルを選択。"@ja-JP ;
        rdfs:label             "전압 레벨"@ko-KR , "voltageLevel"@en , "전압레벨"@ko-KR , "電圧レベル"@ja-JP ;
        schema:domainIncludes  <https://w3id.org/product/ProtectiveDevice%2FFUSEDISCONNECTOR> , <https://w3id.org/product/ProtectiveDevice> , <https://w3id.org/product/ProtectiveDevice%2FCIRCUITBREAKER> .

props:labels  a                owl:DatatypeProperty ;
        rdfs:comment           "Table mapping values to labels, where such labels indicate the meanings of True and False, such as 'Open' and 'Closed'"@en , "Table mapping values to labels, where each entry corresponds to an integer within the ValueRange."@en , "Table mapping values to labels, where such labels indicate transition points such as 'Hi', 'Lo', 'HiHi', or 'LoLo'."@en ;
        rdfs:label             "labels"@en ;
        schema:domainIncludes  <https://w3id.org/product/Controller%2FTWOPOSITION> , <https://w3id.org/product/Controller%2FPROPORTIONAL> , <https://w3id.org/product/Controller%2FMULTIPOSITION> , <https://w3id.org/product/Controller%2FFLOATING> .

props:edgeFixingPlateThickness
        a                      owl:DatatypeProperty ;
        rdfs:comment           "The thickness of the L-shaped edge plate."@en , "L型端部プレートの板厚。"@ja-JP , "L 형 단부 플레이트의 두께"@ko-KR ;
        rdfs:label             "edgeFixingPlateThickness"@en , "板厚"@ja-JP , "두께"@ko-KR ;
        rdfs:range             <https://w3id.org/product/PositiveLengthMeasure> ;
        schema:domainIncludes  <https://w3id.org/product/DiscreteAccessory%2FEdge%20fixing%20plate> .

props:marketCategory  a        owl:DatatypeProperty ;
        rdfs:comment           "Category of use e.g. residential, commercial, recreation etc."@en , "Catégorie d'usage (résidentiel, commercial, loisir,…)"@fr-FR ;
        rdfs:label             "CategorieUsage"@fr-FR , "marketCategory"@en , "CategorieMarche"@fr-FR ;
        rdfs:range             xsd:string ;
        schema:domainIncludes  <https://w3id.org/product/Building> .

props:reinforcementAreaRatio
        a                      owl:DatatypeProperty ;
        rdfs:comment           "The required ratio of the effective area of the reinforcement to the effective area of the concrete At any section of a reinforced concrete structural element."@en , "Das geforderte Verhältnis der effektiven flächenbezogenen Masse der Bewehrung im Verhältnis zur effektiven Fläche des Betons für dieses Element."@de-DE ;
        rdfs:label             "reinforcementAreaRatio"@en , "Bewehrungsgrad Fläche"@de-DE ;
        rdfs:range             <https://w3id.org/product/AreaDensityMeasure> ;
        schema:domainIncludes  <https://w3id.org/product/BuildingElement> .

props:draftBaseOffset
        a                      owl:DatatypeProperty ;
        rdfs:comment           "Draft base offset of the profile."@en ;
        rdfs:label             "draftBaseOffset"@en ;
        rdfs:range             <https://w3id.org/product/NonNegativeLengthMeasure> ;
        schema:domainIncludes  <https://w3id.org/product/ArbitraryProfileDefWithVoids> .

props:totalHeatLoss  a         owl:DatatypeProperty ;
        rdfs:comment           "The total amount of heat or energy lost by the space at the time of the space's peak heating conditions."@en , "ピーク時の室内最大暖房負荷時に取得・損失した熱或いはエネルギー。"@ja-JP , "최대의 실내 최대 난방 부하에 취득 · 손실 열 또는 에너지."@ko-KR ;
        rdfs:label             "totalHeatLoss"@en , "熱ロスの合計"@ja-JP , "열 손실 합계"@ko-KR ;
        rdfs:range             <https://w3id.org/product/PowerMeasure> ;
        schema:domainIncludes  <https://w3id.org/product/Space> .

props:bottomCover  a           owl:DatatypeProperty ;
        rdfs:comment           "Bottom cover of the profile."@en ;
        rdfs:label             "bottomCover"@en ;
        rdfs:range             <https://w3id.org/product/PositiveLengthMeasure> ;
        schema:domainIncludes  <https://w3id.org/product/ArbitraryProfileDefWithVoids> .
